@prefix rdf:     <http://www.w3.org/1999/02/22-rdf-syntax-ns#> .
@prefix rdfs:    <http://www.w3.org/2000/01/rdf-schema#> .
@prefix owl:     <http://www.w3.org/2002/07/owl#> .
@prefix skos:    <http://www.w3.org/2004/02/skos/core#> .
@prefix foaf:    <http://xmlns.com/foaf/0.1/> .
@prefix scovo:   <http://purl.org/NET/scovo#> .
@prefix void:    <http://rdfs.org/ns/void#> .
@prefix vcard:   <http://www.w3.org/2006/vcard/ns#> .
@prefix sdmx:    <http://purl.org/linked-data/sdmx#> .
@prefix sdmx-concept:    <http://purl.org/linked-data/sdmx/2009/concept#> .
@prefix sdmx-dimension:  <http://purl.org/linked-data/sdmx/2009/dimension#> .
@prefix sdmx-attribute:  <http://purl.org/linked-data/sdmx/2009/attribute#> .
@prefix sdmx-measure:    <http://purl.org/linked-data/sdmx/2009/measure#> .
@prefix sdmx-metadata:   <http://purl.org/linked-data/sdmx/2009/metadata#> .
@prefix sdmx-code:       <http://purl.org/linked-data/sdmx/2009/code#> .
@prefix sdmx-subject:    <http://purl.org/linked-data/sdmx/2009/subject#> .
@prefix dcterms:         <http://purl.org/dc/terms/>.
@prefix qb:              <http://purl.org/linked-data/cube#> .

<http://purl.org/linked-data/sdmx/2009/metadata#>
    a owl:Ontology;
    rdfs:label "The vocabulary about SDMX metadata."@en;
	rdfs:label "有关SDMX元数据的词汇集"@zh-CN;
    rdfs:comment "These annotations is added by chuci.info."@en;
    rdfs:comment "这些本体声明标记由chuci.info添加。"@zh-CN .

# ACCESSIBILITY
sdmx-metadata:accessibility a sdmx:MetadataProperty, rdf:Property  ;
    qb:concept sdmx-concept:accessibility ;
    rdfs:label "Accessibility"@en ;
    rdfs:comment """The ease and the conditions under which statistical information can be obtained."""@en ;
	rdfs:label "可访问性"@zh-CN ;
	rdfs:comment """可以得到统计信息的便利性和条件。"""@zh-CN ;
    rdfs:isDefinedBy <http://sdmx.org/wp-content/uploads/2009/01/01_sdmx_cog_annex_1_cdc_2009.pdf> .

# ACCURACY
sdmx-metadata:accuracy a sdmx:MetadataProperty, rdf:Property  ;
    qb:concept sdmx-concept:accuracy ;
    rdfs:label "Accuracy"@en ;
    rdfs:comment """Closeness of computations or estimates to the exact or true values that the statistics were intended to measure."""@en ;
	rdfs:label "准确性"@zh-CN ;
	rdfs:comment """在将进行的测量中，计算值或估计值与确切的或真实的统计值的接近程度。"""@zh-CN ;
    rdfs:isDefinedBy <http://sdmx.org/wp-content/uploads/2009/01/01_sdmx_cog_annex_1_cdc_2009.pdf> .

# ACCURACY_OVERALL
sdmx-metadata:accuracyOverall a sdmx:MetadataProperty, rdf:Property  ;
    qb:concept sdmx-concept:accuracyOverall ;
    rdfs:label "Accuracy - overall"@en ;
    rdfs:comment """Assessment of accuracy, linked to a certain data set or domain, which is summarising the various components into one single measure."""@en ;
	rdfs:label "准确性--整体"@zh-CN ;
	rdfs:comment """评估的准确性，连接到一个特定的数据集或域，它汇总了在一个单一测量中的各种组件。"""@zh-CN ;
    rdfs:isDefinedBy <http://sdmx.org/wp-content/uploads/2009/01/01_sdmx_cog_annex_1_cdc_2009.pdf> .

# NONSAMPLING_ERR
sdmx-metadata:nonsamplingErr a sdmx:MetadataProperty, rdf:Property  ;
    qb:concept sdmx-concept:nonsamplingErr ;
    rdfs:label "Accuracy - nonsampling error"@en ;
    rdfs:comment """Error in sample estimates which cannot be attributed to sampling fluctuations."""@en ;
	rdfs:label "准确性--非抽样误差"@zh-CN ;
	rdfs:comment """样本估计中的错误，不能归咎于抽样波动。"""@zh-CN ;
    rdfs:isDefinedBy <http://sdmx.org/wp-content/uploads/2009/01/01_sdmx_cog_annex_1_cdc_2009.pdf> .

# SAMPLING_ERR
sdmx-metadata:samplingErr a sdmx:MetadataProperty, rdf:Property  ;
    qb:concept sdmx-concept:samplingErr ;
    rdfs:label "Accuracy - sampling error"@en ;
    rdfs:comment """That part of the difference between a population value and an estimate thereof, derived from a random sample, which is due to the fact that only a subset of the population is enumerated."""@en ;
    rdfs:label "准确性--抽样误差"@zh-CN ;
	rdfs:comment """总数值和其估值之间的差异部分，来自于一个随机样本，这是由于这样的事实，枚举的只是总数的一个子集。"""@zh-CN ;
	rdfs:isDefinedBy <http://sdmx.org/wp-content/uploads/2009/01/01_sdmx_cog_annex_1_cdc_2009.pdf> .

# ADJUSTMENT
sdmx-metadata:adjustment a sdmx:MetadataProperty, rdf:Property  ;
    qb:concept sdmx-concept:adjustment ;
    rdfs:label "Adjustment"@en ;
    rdfs:comment """The set of procedures employed to modify statistical data to enable it to conform to national or international standards or to address data quality differences when compiling specific data sets."""@en ;
    rdfs:label "校准"@zh-CN ;
	rdfs:comment """一套用于修改统计数据的程序，使其能够符合国家或国际标准或编译特定的数据集时解决数据质量的差异。"""@zh-CN ;
	rdfs:isDefinedBy <http://sdmx.org/wp-content/uploads/2009/01/01_sdmx_cog_annex_1_cdc_2009.pdf> .

# ADJUST_CODED
sdmx-metadata:adjustCoded a sdmx:MetadataProperty, rdf:Property  ;
    qb:concept sdmx-concept:adjustCoded ;
    rdfs:label "Adjustment - coded"@en ;
    rdfs:comment """Type of adjustment used, represented by a code."""@en ;
	rdfs:label "校准--编码"@zh-CN ;
	rdfs:comment """校准的类型，通过编码表示。"""@zh-CN ;
    rdfs:isDefinedBy <http://sdmx.org/wp-content/uploads/2009/01/01_sdmx_cog_annex_1_cdc_2009.pdf> .

# ADJUST_DETAIL
sdmx-metadata:adjustDetail a sdmx:MetadataProperty, rdf:Property  ;
    qb:concept sdmx-concept:adjustDetail ;
    rdfs:label "Adjustment - detail"@en ;
    rdfs:comment """Textual description of the type of adjustment used."""@en ;
	rdfs:label "校准--详述"@zh-CN ;
	rdfs:comment """有关校准类型的文本描述。"""@zh-CN ;
    rdfs:isDefinedBy <http://sdmx.org/wp-content/uploads/2009/01/01_sdmx_cog_annex_1_cdc_2009.pdf> .

# AGE
sdmx-metadata:age a sdmx:MetadataProperty, rdf:Property  ;
    qb:concept sdmx-concept:age ;
    rdfs:label "Age"@en ;
    rdfs:comment """The length of time that a person has lived or a thing has existed."""@en ;
	rdfs:label "年龄"@zh-CN ;
	rdfs:comment """一个人生存或一个事物存在的时间长度。"""@zh-CN ;
    rdfs:isDefinedBy <http://sdmx.org/wp-content/uploads/2009/01/01_sdmx_cog_annex_1_cdc_2009.pdf> .

# BASE_PER
sdmx-metadata:basePer a sdmx:MetadataProperty, rdf:Property  ;
    qb:concept sdmx-concept:basePer ;
    rdfs:label "Base Period"@en ;
    rdfs:comment """The period of time used as the base of an index number, or to which a constant price series refers."""@en ;
	rdfs:label "基本周期"@zh-CN ;
	rdfs:comment """时间周期，作为索引号的基数，或者一个恒定的价格所涉及的周期。"""@zh-CN ;
    rdfs:isDefinedBy <http://sdmx.org/wp-content/uploads/2009/01/01_sdmx_cog_annex_1_cdc_2009.pdf> .

# CIVIL_STATUS
sdmx-metadata:civilStatus a sdmx:MetadataProperty, rdf:Property  ;
    qb:concept sdmx-concept:civilStatus ;
    rdfs:label "Civil Status"@en ;
    rdfs:comment """Legal, conjugal status of each individual in relation to the marriage laws or customs of the country."""@en ;
	rdfs:label "婚姻状况"@zh-CN ;
	rdfs:comment """就国家的婚姻法律或习俗而言，每一个人的婚姻状态。"""@zh-CN ;
    rdfs:isDefinedBy <http://sdmx.org/wp-content/uploads/2009/01/01_sdmx_cog_annex_1_cdc_2009.pdf> .

# CLARITY
sdmx-metadata:clarity a sdmx:MetadataProperty, rdf:Property  ;
    qb:concept sdmx-concept:clarity ;
    rdfs:label "Clarity"@en ;
    rdfs:comment """The extent to which easily comprehensible metadata are available, where these metadata are necessary to give a full understanding of statistical data."""@en ;
    rdfs:label "清晰度"@zh-CN ;
	rdfs:comment """元数据容易理解的程度，必要时对统计数据给予充分的认识。"""@zh-CN ;
	rdfs:isDefinedBy <http://sdmx.org/wp-content/uploads/2009/01/01_sdmx_cog_annex_1_cdc_2009.pdf> .

# CLASS_SYSTEM
sdmx-metadata:classSystem a sdmx:MetadataProperty, rdf:Property  ;
    qb:concept sdmx-concept:classSystem ;
    rdfs:label "Classification systems"@en ;
    rdfs:comment """Arrangement or division of objects into groups based on characteristics which the objects have in common."""@en ;
	rdfs:label "分类系统"@zh-CN ;
	rdfs:comment """基于对象有共同的特点，将对象安排或划分成组。"""@zh-CN ;
    rdfs:isDefinedBy <http://sdmx.org/wp-content/uploads/2009/01/01_sdmx_cog_annex_1_cdc_2009.pdf> .

# COHERENCE
sdmx-metadata:coherence a sdmx:MetadataProperty, rdf:Property  ;
    qb:concept sdmx-concept:coherence ;
    rdfs:label "Coherence"@en ;
    rdfs:comment """Adequacy of statistics to be combined in different ways and for various uses."""@en ;
	rdfs:label "相干性"@zh-CN ;
	rdfs:comment """充足的统计数据要结合不同的方式和不同的用途。"""@zh-CN ;
    rdfs:isDefinedBy <http://sdmx.org/wp-content/uploads/2009/01/01_sdmx_cog_annex_1_cdc_2009.pdf> .

# COHER_X_DOM
sdmx-metadata:coherXDom a sdmx:MetadataProperty, rdf:Property  ;
    qb:concept sdmx-concept:coherXDom ;
    rdfs:label "Coherence - cross domain"@en ;
    rdfs:comment """Extent to which statistics are reconcilable with those obtained through other data sources or statistical domains."""@en ;
	rdfs:label "相干性--交叉域"@zh-CN ;
	rdfs:comment """统计数据与从其他数据源或统计领域获得的数据进行调和的程度。"""@zh-CN ;
    rdfs:isDefinedBy <http://sdmx.org/wp-content/uploads/2009/01/01_sdmx_cog_annex_1_cdc_2009.pdf> .

# COHER_INTERNAL
sdmx-metadata:coherInternal a sdmx:MetadataProperty, rdf:Property  ;
    qb:concept sdmx-concept:coherInternal ;
    rdfs:label "Coherence - Internal"@en ;
    rdfs:comment """Extent to which statistics are consistent within a given data set."""@en ;
	rdfs:label "相干性--内部"@zh-CN ;
	rdfs:comment """统计数据与一个给定的数据集相一致的程度。"""@zh-CN ;
    rdfs:isDefinedBy <http://sdmx.org/wp-content/uploads/2009/01/01_sdmx_cog_annex_1_cdc_2009.pdf> .

# COMMENT
sdmx-metadata:comment a sdmx:MetadataProperty, rdf:Property  ;
    qb:concept sdmx-concept:comment ;
    rdfs:label "Comment"@en ;
    rdfs:comment """Supplementary descriptive text which can be attached to data or metadata."""@en ;
	rdfs:label "注释"@zh-CN ;
	rdfs:comment """附加到数据或元数据的补充描述性文本。"""@zh-CN ;
    rdfs:isDefinedBy <http://sdmx.org/wp-content/uploads/2009/01/01_sdmx_cog_annex_1_cdc_2009.pdf> .

# COMPARABILITY
sdmx-metadata:comparability a sdmx:MetadataProperty, rdf:Property  ;
    qb:concept sdmx-concept:comparability ;
    rdfs:label "Comparability"@en ;
    rdfs:comment """The extent to which differences between statistics can be attributed to differences between the true values of the statistical characteristics."""@en ;
	rdfs:label "可比性"@zh-CN ;
	rdfs:comment """统计数据之间的差异可以在何种程度上归因于统计特征的真值之间的差异。"""@zh-CN ;
    rdfs:isDefinedBy <http://sdmx.org/wp-content/uploads/2009/01/01_sdmx_cog_annex_1_cdc_2009.pdf> .

# COMPAR_DOMAINS
sdmx-metadata:comparDomains a sdmx:MetadataProperty, rdf:Property  ;
    qb:concept sdmx-concept:comparDomains ;
    rdfs:label "Comparability - between domains"@en ;
    rdfs:comment """Extent to which statistics are comparable between different statistical domains."""@en ;
	rdfs:label "可比性--域间"@zh-CN ;
	rdfs:comment """统计数据可以在不同的统计领域之间进行比较的程度。"""@zh-CN ;
    rdfs:isDefinedBy <http://sdmx.org/wp-content/uploads/2009/01/01_sdmx_cog_annex_1_cdc_2009.pdf> .

# COMPAR_GEO
sdmx-metadata:comparGeo a sdmx:MetadataProperty, rdf:Property  ;
    qb:concept sdmx-concept:comparGeo ;
    rdfs:label "Comparability - geographical"@en ;
    rdfs:comment """Extent to which statistics are comparable between geographical areas."""@en ;
	rdfs:label "可比性--地域"@zh-CN ;
	rdfs:comment """统计数据可以在地理区域之间进行比较的程度。"""@zh-CN ;
    rdfs:isDefinedBy <http://sdmx.org/wp-content/uploads/2009/01/01_sdmx_cog_annex_1_cdc_2009.pdf> .

# COMPAR_TIME
sdmx-metadata:comparTime a sdmx:MetadataProperty, rdf:Property  ;
    qb:concept sdmx-concept:comparTime ;
    rdfs:label "Comparability - over time"@en ;
    rdfs:comment """Extent to which statistics are comparable or reconcilable over time."""@en ;
	rdfs:label "可比性--时效"@zh-CN ;
	rdfs:comment """随着时间推移，统计数据具有可比性或调和的。"""@zh-CN ;
    rdfs:isDefinedBy <http://sdmx.org/wp-content/uploads/2009/01/01_sdmx_cog_annex_1_cdc_2009.pdf> .

# COMPILING_ORG
sdmx-metadata:compilingOrg a sdmx:MetadataProperty, rdf:Property  ;
    qb:concept sdmx-concept:compilingOrg ;
    rdfs:label "Compiling agency"@en ;
    rdfs:comment """The organisation compiling the data being reported."""@en ;
	rdfs:label "编制机构"@zh-CN ;
	rdfs:comment """将数据编制成报表的组织机构。"""@zh-CN ;
    rdfs:isDefinedBy <http://sdmx.org/wp-content/uploads/2009/01/01_sdmx_cog_annex_1_cdc_2009.pdf> .

# CONF
sdmx-metadata:conf a sdmx:MetadataProperty, rdf:Property  ;
    qb:concept sdmx-concept:conf ;
    rdfs:label "Confidentiality"@en ;
    rdfs:comment """A property of data indicating the extent to which their unauthorised disclosure could be prejudicial or harmful to the interest of the source or other relevant parties."""@en ;
    rdfs:label "保密性"@zh-CN ;
	rdfs:comment """该数据属性说明数据未经授权而披露，可能会损害或有害数据来源或其他相关各方的利益。"""@zh-CN ;
	rdfs:isDefinedBy <http://sdmx.org/wp-content/uploads/2009/01/01_sdmx_cog_annex_1_cdc_2009.pdf> .

# CONF_DATA_TR
sdmx-metadata:confDataTr a sdmx:MetadataProperty, rdf:Property  ;
    qb:concept sdmx-concept:confDataTr ;
    rdfs:label "Confidentiality - data treatment"@en ;
    rdfs:comment """Rules applied for treating the data set to ensure statistical confidentiality and prevent unauthorised disclosure."""@en ;
	rdfs:label "保密性--数据处理"@zh-CN ;
	rdfs:comment """适用于处理数据集的规则，以确保统计的保密性，防止未经授权而披露。"""@zh-CN ;
    rdfs:isDefinedBy <http://sdmx.org/wp-content/uploads/2009/01/01_sdmx_cog_annex_1_cdc_2009.pdf> .

# CONF_POLICY
sdmx-metadata:confPolicy a sdmx:MetadataProperty, rdf:Property  ;
    qb:concept sdmx-concept:confPolicy ;
    rdfs:label "Confidentiality - policy"@en ;
    rdfs:comment """Legislative measures or other formal procedures which prevent unauthorised disclosure of data that identify a person or economic entity either directly or indirectly."""@en ;
    rdfs:label "保密性--政策"@zh-CN ;
	rdfs:comment """立法措施或其他正式程序，用于直接或间接辨识一个人或经济实体，以防止数据未获授权而披露。"""@zh-CN ;
	rdfs:isDefinedBy <http://sdmx.org/wp-content/uploads/2009/01/01_sdmx_cog_annex_1_cdc_2009.pdf> .

# CONF_STATUS
sdmx-metadata:confStatus a sdmx:MetadataProperty, rdf:Property  ;
    qb:concept sdmx-concept:confStatus ;
    rdfs:label "Confidentiality - status"@en ;
    rdfs:comment """Information about the confidentiality status of the object to which this attribute is attached."""@en ;
	rdfs:label "保密性--状态"@zh-CN ;
	rdfs:comment """这个属性附加到对象上，描述该对象的保密状态的信息。"""@zh-CN ;
    rdfs:isDefinedBy <http://sdmx.org/wp-content/uploads/2009/01/01_sdmx_cog_annex_1_cdc_2009.pdf> .

# CONTACT
sdmx-metadata:contact a sdmx:MetadataProperty, rdf:Property  ;
    qb:concept sdmx-concept:contact ;
    rdfs:label "Contact"@en ;
    rdfs:comment """Individual or organisational contact points for the data or metadata, including information on how to reach the contact points."""@en ;
	rdfs:label "联系"@zh-CN ;
	rdfs:comment """数据或元数据的个体或组织联系点，包括如何到达接触点的信息。"""@zh-CN ;
    rdfs:isDefinedBy <http://sdmx.org/wp-content/uploads/2009/01/01_sdmx_cog_annex_1_cdc_2009.pdf> .

# CONTACT_EMAIL
sdmx-metadata:contactEmail a sdmx:MetadataProperty, rdf:Property  ;
    qb:concept sdmx-concept:contactEmail ;
    rdfs:label "Contact email address"@en ;
    rdfs:comment """E-mail address of the contact points for the data or metadata."""@en ;
	rdfs:label "联系--Email"@zh-CN ;
	rdfs:comment """数据或元数据的接触点的Email地址。"""@zh-CN ;
    rdfs:isDefinedBy <http://sdmx.org/wp-content/uploads/2009/01/01_sdmx_cog_annex_1_cdc_2009.pdf> .

# CONTACT_FAX
sdmx-metadata:contactFax a sdmx:MetadataProperty, rdf:Property  ;
    qb:concept sdmx-concept:contactFax ;
    rdfs:label "Contact fax number"@en ;
    rdfs:comment """Fax number of the contact points for the data or metadata."""@en ;
	rdfs:label "联系--传真"@zh-CN ;
	rdfs:comment """数据或元数据的接触点的传真号码。"""@zh-CN ;
    rdfs:isDefinedBy <http://sdmx.org/wp-content/uploads/2009/01/01_sdmx_cog_annex_1_cdc_2009.pdf> .

# CONTACT_MAIL
sdmx-metadata:contactMail a sdmx:MetadataProperty, rdf:Property  ;
    qb:concept sdmx-concept:contactMail ;
    rdfs:label "Contact mail address"@en ;
    rdfs:comment """The postal address of the contact points for the data or metadata."""@en ;
	rdfs:label "联系--邮件地址"@zh-CN ;
	rdfs:comment """数据或元数据的接触点的邮件地址。"""@zh-CN ;
    rdfs:isDefinedBy <http://sdmx.org/wp-content/uploads/2009/01/01_sdmx_cog_annex_1_cdc_2009.pdf> .

# CONTACT_NAME
sdmx-metadata:contactName a sdmx:MetadataProperty, rdf:Property  ;
    qb:concept sdmx-concept:contactName ;
    rdfs:label "Contact name"@en ;
    rdfs:comment """The name of the contact points for the data or metadata."""@en ;
	rdfs:label "联系--名称"@zh-CN ;
	rdfs:comment """数据或元数据的接触点的名称。"""@zh-CN ;
    rdfs:isDefinedBy <http://sdmx.org/wp-content/uploads/2009/01/01_sdmx_cog_annex_1_cdc_2009.pdf> .

# CONTACT_ORGANISATION
sdmx-metadata:contactOrganisation a sdmx:MetadataProperty, rdf:Property  ;
    qb:concept sdmx-concept:contactOrganisation ;
    rdfs:label "Contact organisation"@en ;
    rdfs:comment """The name of the organisation of the contact points for the data or metadata."""@en ;
	rdfs:label "联系--组织"@zh-CN ;
	rdfs:comment """数据或元数据的接触点的组织名称。"""@zh-CN ;
    rdfs:isDefinedBy <http://sdmx.org/wp-content/uploads/2009/01/01_sdmx_cog_annex_1_cdc_2009.pdf> .

# ORGANISATION_UNIT
sdmx-metadata:organisationUnit a sdmx:MetadataProperty, rdf:Property  ;
    qb:concept sdmx-concept:organisationUnit ;
    rdfs:label "Contact organization unit"@en ;
    rdfs:comment """An addressable subdivision of an organization."""@en ;
	rdfs:label "联系--组织单元"@zh-CN ;
	rdfs:comment """组织的分部地址。"""@zh-CN ;
    rdfs:isDefinedBy <http://sdmx.org/wp-content/uploads/2009/01/01_sdmx_cog_annex_1_cdc_2009.pdf> .

# CONTACT_FUNCT
sdmx-metadata:contactFunct a sdmx:MetadataProperty, rdf:Property  ;
    qb:concept sdmx-concept:contactFunct ;
    rdfs:label "Contact person job title"@en ;
    rdfs:comment """The area of technical responsibility of the contact, such as "methodology", "database management" or "dissemination"."""@en ;
    rdfs:label "联系人职位"@zh-CN ;
	rdfs:comment """联系人的技术负责领域，比如“方法”，“数据库管理”或“传播”。"""@zh-CN ;
	rdfs:isDefinedBy <http://sdmx.org/wp-content/uploads/2009/01/01_sdmx_cog_annex_1_cdc_2009.pdf> .

# CONTACT_PHONE
sdmx-metadata:contactPhone a sdmx:MetadataProperty, rdf:Property  ;
    qb:concept sdmx-concept:contactPhone ;
    rdfs:label "Contact phone number"@en ;
    rdfs:comment """The telephone number of the contact points for the data or metadata."""@en ;
	rdfs:label "联系人电话"@zh-CN ;
	rdfs:comment """数据或元数据的联系点的电话号码。"""@zh-CN ;
    rdfs:isDefinedBy <http://sdmx.org/wp-content/uploads/2009/01/01_sdmx_cog_annex_1_cdc_2009.pdf> .

# COST_BURDEN
sdmx-metadata:costBurden a sdmx:MetadataProperty, rdf:Property  ;
    qb:concept sdmx-concept:costBurden ;
    rdfs:label "Cost and Burden"@en ;
    rdfs:comment """Costs associated with the collection and production of a statistical product and burden on respondents."""@en ;
	rdfs:label "成本和负担"@zh-CN ;
	rdfs:comment """与采集和生成统计产品有关的花费和受访者负担。"""@zh-CN ;
    rdfs:isDefinedBy <http://sdmx.org/wp-content/uploads/2009/01/01_sdmx_cog_annex_1_cdc_2009.pdf> .

# COST_BURDEN_EFF
sdmx-metadata:costBurdenEff a sdmx:MetadataProperty, rdf:Property  ;
    qb:concept sdmx-concept:costBurdenEff ;
    rdfs:label "Cost and Burden - efficiency management"@en ;
    rdfs:comment """Cost benefit analysis, effectiveness of execution of medium term statistical programs, and ensuring efficient use of resources."""@en ;
	rdfs:label "成本和负担--效率管理"@zh-CN ;
	rdfs:comment """成本效益分析，中期统计方案的执行成效，以及确保资源的有效利用。"""@zh-CN ;
    rdfs:isDefinedBy <http://sdmx.org/wp-content/uploads/2009/01/01_sdmx_cog_annex_1_cdc_2009.pdf> .

# COST_BURDEN_RES
sdmx-metadata:costBurdenRes a sdmx:MetadataProperty, rdf:Property  ;
    qb:concept sdmx-concept:costBurdenRes ;
    rdfs:label "Cost and Burden - resources"@en ;
    rdfs:comment """Staff, facilities, computing resources, and financing to undertake statistical production."""@en ;
	rdfs:label "成本和负担--资源"@zh-CN ;
	rdfs:comment """承担统计产品的工作人员，设施，计算资源和资金。"""@zh-CN ;
    rdfs:isDefinedBy <http://sdmx.org/wp-content/uploads/2009/01/01_sdmx_cog_annex_1_cdc_2009.pdf> .

# VIS_AREA
sdmx-metadata:visArea a sdmx:MetadataProperty, rdf:Property  ;
    qb:concept sdmx-concept:visArea ;
    rdfs:label "Counterpart Reference Area"@en ;
    rdfs:comment """The secondary area, as opposed to reference area, to which the measured data is in relation."""@en ;
	rdfs:label "对应的参照区域"@zh-CN ;
	rdfs:comment """相对于参照区域的次级区域，测量数据与该区域有关。"""@zh-CN ;
    rdfs:isDefinedBy <http://sdmx.org/wp-content/uploads/2009/01/01_sdmx_cog_annex_1_cdc_2009.pdf> .

# COVERAGE
sdmx-metadata:coverage a sdmx:MetadataProperty, rdf:Property  ;
    qb:concept sdmx-concept:coverage ;
    rdfs:label "Coverage"@en ;
    rdfs:comment """The definition of the population that statistics aim to cover."""@en ;
	rdfs:label "覆盖"@zh-CN ;
	rdfs:comment """统计总数定义的目标是覆盖。"""@zh-CN ;
    rdfs:isDefinedBy <http://sdmx.org/wp-content/uploads/2009/01/01_sdmx_cog_annex_1_cdc_2009.pdf> .

# COVERAGE_SECTOR
sdmx-metadata:coverageSector a sdmx:MetadataProperty, rdf:Property  ;
    qb:concept sdmx-concept:coverageSector ;
    rdfs:label "Coverage - sector"@en ;
    rdfs:comment """Main economic or other sectors covered by the statistics."""@en ;
	rdfs:label "覆盖--行业"@zh-CN ;
	rdfs:comment """统计涵盖的是主要经济或其他行业。"""@zh-CN ;
    rdfs:isDefinedBy <http://sdmx.org/wp-content/uploads/2009/01/01_sdmx_cog_annex_1_cdc_2009.pdf> .

# COVERAGE_TIME
sdmx-metadata:coverageTime a sdmx:MetadataProperty, rdf:Property  ;
    qb:concept sdmx-concept:coverageTime ;
    rdfs:label "Coverage- time"@en ;
    rdfs:comment """The length of time for which data are available."""@en ;
	rdfs:label "覆盖--时间"@zh-CN ;
	rdfs:comment """数据可用的时间长度。"""@zh-CN ;
    rdfs:isDefinedBy <http://sdmx.org/wp-content/uploads/2009/01/01_sdmx_cog_annex_1_cdc_2009.pdf> .

# CURRENCY
sdmx-metadata:currency a sdmx:MetadataProperty, rdf:Property  ;
    qb:concept sdmx-concept:currency ;
    rdfs:label "Currency"@en ;
    rdfs:comment """Monetary denomination of the object being measured."""@en ;
	rdfs:label "货币"@zh-CN ;
	rdfs:comment """测量对象的货币面额。"""@zh-CN ;
    rdfs:isDefinedBy <http://sdmx.org/wp-content/uploads/2009/01/01_sdmx_cog_annex_1_cdc_2009.pdf> .

# COLL_METHOD
sdmx-metadata:collMethod a sdmx:MetadataProperty, rdf:Property  ;
    qb:concept sdmx-concept:collMethod ;
    rdfs:label "Data Collection Method"@en ;
    rdfs:comment """Systematic process of gathering data for official statistics."""@en ;
	rdfs:label "数据采集方法"@zh-CN ;
	rdfs:comment """官方统计收集数据的系统化流程。"""@zh-CN ;
    rdfs:isDefinedBy <http://sdmx.org/wp-content/uploads/2009/01/01_sdmx_cog_annex_1_cdc_2009.pdf> .

# DATA_COMP
sdmx-metadata:dataComp a sdmx:MetadataProperty, rdf:Property  ;
    qb:concept sdmx-concept:dataComp ;
    rdfs:label "Data Compilation"@en ;
    rdfs:comment """Operations performed on data to derive new information according to a given set of rules."""@en ;
	rdfs:label "数据编制"@zh-CN ;
	rdfs:comment """按照给定的规则集，在数据上执行的操作，以生成新的信息。"""@zh-CN ;
    rdfs:isDefinedBy <http://sdmx.org/wp-content/uploads/2009/01/01_sdmx_cog_annex_1_cdc_2009.pdf> .

# DISS_ORG
sdmx-metadata:dissOrg a sdmx:MetadataProperty, rdf:Property  ;
    qb:concept sdmx-concept:dissOrg ;
    rdfs:label "Data Dissemination Agency"@en ;
    rdfs:comment """The organisation disseminating the data."""@en ;
	rdfs:label "数据发布机构"@zh-CN ;
	rdfs:comment """发布数据的组织机构。"""@zh-CN ;
    rdfs:isDefinedBy <http://sdmx.org/wp-content/uploads/2009/01/01_sdmx_cog_annex_1_cdc_2009.pdf> .

# DATA_EDITING
sdmx-metadata:dataEditing a sdmx:MetadataProperty, rdf:Property  ;
    qb:concept sdmx-concept:dataEditing ;
    rdfs:label "Data Editing"@en ;
    rdfs:comment """Activity aimed at detecting and correcting errors, logical inconsistencies and suspicious data."""@en ;
	rdfs:label "数据编辑"@zh-CN ;
	rdfs:comment """旨在检测和校正错误、逻辑不一致和可疑数据的活动。"""@zh-CN ;
    rdfs:isDefinedBy <http://sdmx.org/wp-content/uploads/2009/01/01_sdmx_cog_annex_1_cdc_2009.pdf> .

# DATA_PRES
sdmx-metadata:dataPres a sdmx:MetadataProperty, rdf:Property  ;
    qb:concept sdmx-concept:dataPres ;
    rdfs:label "Data Presentation"@en ;
    rdfs:comment """Description of the disseminated data."""@en ;
	rdfs:label "数据简报"@zh-CN ;
	rdfs:comment """发布数据的描述。"""@zh-CN ;
    rdfs:isDefinedBy <http://sdmx.org/wp-content/uploads/2009/01/01_sdmx_cog_annex_1_cdc_2009.pdf> .

# DATA_DESCR
sdmx-metadata:dataDescr a sdmx:MetadataProperty, rdf:Property  ;
    qb:concept sdmx-concept:dataDescr ;
    rdfs:label "Data Presentation - data description"@en ;
    rdfs:comment """Main characteristics of the data set described in an easily understandable manner, referring to the data and indicators disseminated."""@en ;
	rdfs:label "数据简报--数据描述"@zh-CN ;
	rdfs:comment """以简单易懂的方式描述数据集的主要特征，涉及发布的数据和指标。"""@zh-CN ;
    rdfs:isDefinedBy <http://sdmx.org/wp-content/uploads/2009/01/01_sdmx_cog_annex_1_cdc_2009.pdf> .

# DISS_DET
sdmx-metadata:dissDet a sdmx:MetadataProperty, rdf:Property  ;
    qb:concept sdmx-concept:dissDet ;
    rdfs:label "Data Presentation - disseminated detail"@en ;
    rdfs:comment """Disseminated domain, measure, and time period breakdowns of statistics in the dataset."""@en ;
	rdfs:label "数据简报--发布细节"@zh-CN ;
	rdfs:comment """发布的数据集中统计信息划分的领域、测量和时间段。"""@zh-CN ;
    rdfs:isDefinedBy <http://sdmx.org/wp-content/uploads/2009/01/01_sdmx_cog_annex_1_cdc_2009.pdf> .

# DATA_PROVIDER
sdmx-metadata:dataProvider a sdmx:MetadataProperty, rdf:Property  ;
    qb:concept sdmx-concept:dataProvider ;
    rdfs:label "Data Provider"@en ;
    rdfs:comment """Organisation which produces data or metadata"""@en ;
	rdfs:label "数据提供者"@zh-CN ;
	rdfs:comment """生成数据或元数据的组织机构。"""@zh-CN ;
    rdfs:isDefinedBy <http://sdmx.org/wp-content/uploads/2009/01/01_sdmx_cog_annex_1_cdc_2009.pdf> .

# DATA_REV
sdmx-metadata:dataRev a sdmx:MetadataProperty, rdf:Property  ;
    qb:concept sdmx-concept:dataRev ;
    rdfs:label "Data Revision"@en ;
    rdfs:comment """Any change in a value of a statistic released to the public."""@en ;
	rdfs:label "数据修订"@zh-CN ;
	rdfs:comment """向公众发布的统计值的任何变更。"""@zh-CN ;
    rdfs:isDefinedBy <http://sdmx.org/wp-content/uploads/2009/01/01_sdmx_cog_annex_1_cdc_2009.pdf> .

# REV_POLICY
sdmx-metadata:revPolicy a sdmx:MetadataProperty, rdf:Property  ;
    qb:concept sdmx-concept:revPolicy ;
    rdfs:label "Data Revision - policy"@en ;
    rdfs:comment """Policy aimed at ensuring the transparency of disseminated data, whereby preliminary data are compiled that are later revised."""@en ;
	rdfs:label "数据修订--策略"@zh-CN ;
	rdfs:comment """这些策略旨在确保发布数据的透明度，据此在日后对已编制的初步数据进行修订。"""@zh-CN ;
    rdfs:isDefinedBy <http://sdmx.org/wp-content/uploads/2009/01/01_sdmx_cog_annex_1_cdc_2009.pdf> .

# REV_PRACTICE
sdmx-metadata:revPractice a sdmx:MetadataProperty, rdf:Property  ;
    qb:concept sdmx-concept:revPractice ;
    rdfs:label "Data Revision - practice"@en ;
    rdfs:comment """Information on the data revision practice."""@en ;
	rdfs:label "数据修订--实践"@zh-CN ;
	rdfs:comment """有关数据修订实践的信息。"""@zh-CN ;
    rdfs:isDefinedBy <http://sdmx.org/wp-content/uploads/2009/01/01_sdmx_cog_annex_1_cdc_2009.pdf> .

# REV_STUDY
sdmx-metadata:revStudy a sdmx:MetadataProperty, rdf:Property  ;
    qb:concept sdmx-concept:revStudy ;
    rdfs:label "Data Revision - studies"@en ;
    rdfs:comment """Information about data revision studies and analyses."""@en ;
	rdfs:label "数据修订--研究"@zh-CN ;
	rdfs:comment """有关数据修订研究和分析的信息。"""@zh-CN ;
    rdfs:isDefinedBy <http://sdmx.org/wp-content/uploads/2009/01/01_sdmx_cog_annex_1_cdc_2009.pdf> .

# DSI
sdmx-metadata:dsi a sdmx:MetadataProperty, rdf:Property  ;
    qb:concept sdmx-concept:dsi ;
    rdfs:label "Data Set Identifier"@en ;
    rdfs:comment """Sequence of characters identifying the data set with which it is associated."""@en ;
	rdfs:label "数据集标识符"@zh-CN ;
	rdfs:comment """识别数据集并与它相关联的字符序列。"""@zh-CN ;
    rdfs:isDefinedBy <http://sdmx.org/wp-content/uploads/2009/01/01_sdmx_cog_annex_1_cdc_2009.pdf> .

# DATA_UPDATE
sdmx-metadata:dataUpdate a sdmx:MetadataProperty, rdf:Property  ;
    qb:concept sdmx-concept:dataUpdate ;
    rdfs:label "Data Update"@en ;
    rdfs:comment """The date on which the data element was inserted or modified in the database."""@en ;
	rdfs:label "数据更新"@zh-CN ;
	rdfs:comment """在数据库中插入或修改数据元素的日期。"""@zh-CN ;
    rdfs:isDefinedBy <http://sdmx.org/wp-content/uploads/2009/01/01_sdmx_cog_annex_1_cdc_2009.pdf> .

# DATA_VALIDATION
sdmx-metadata:dataValidation a sdmx:MetadataProperty, rdf:Property  ;
    qb:concept sdmx-concept:dataValidation ;
    rdfs:label "Data Validation"@en ;
    rdfs:comment """Process of monitoring the results of data compilation and ensuring the quality of the statistical results."""@en ;
	rdfs:label "数据验证"@zh-CN ;
	rdfs:comment """一个流程，用以监测数据编制的结果，并确保统计结果的质量。"""@zh-CN ;
    rdfs:isDefinedBy <http://sdmx.org/wp-content/uploads/2009/01/01_sdmx_cog_annex_1_cdc_2009.pdf> .

# DATA_VAL_INTER
sdmx-metadata:dataValInter a sdmx:MetadataProperty, rdf:Property  ;
    qb:concept sdmx-concept:dataValInter ;
    rdfs:label "Data Validation - intermediate"@en ;
    rdfs:comment """Validation that intermediate calculations leading to statistical outputs have been correctly done."""@en ;
	rdfs:label "数据验证--中间"@zh-CN ;
	rdfs:comment """导致统计输出正确产生的中间计算的验证。"""@zh-CN ;
    rdfs:isDefinedBy <http://sdmx.org/wp-content/uploads/2009/01/01_sdmx_cog_annex_1_cdc_2009.pdf> .

# DATA_VAL_OUTPUT
sdmx-metadata:dataValOutput a sdmx:MetadataProperty, rdf:Property  ;
    qb:concept sdmx-concept:dataValOutput ;
    rdfs:label "Data Validation - output"@en ;
    rdfs:comment """Assessment of discrepancies and other problems in statistical outputs."""@en ;
	rdfs:label "数据验证--输出"@zh-CN ;
	rdfs:comment """有关统计输出的出入和其他问题的评定。"""@zh-CN ;
    rdfs:isDefinedBy <http://sdmx.org/wp-content/uploads/2009/01/01_sdmx_cog_annex_1_cdc_2009.pdf> .

# DATA_VAL_SOURCE
sdmx-metadata:dataValSource a sdmx:MetadataProperty, rdf:Property  ;
    qb:concept sdmx-concept:dataValSource ;
    rdfs:label "Data Validation - source"@en ;
    rdfs:comment """Assessment of discrepancies and other problems related to source data."""@en ;
	rdfs:label "数据验证--源"@zh-CN ;
	rdfs:comment """有关统计输出的出入和其他问题的评定。"""@zh-CN ;
    rdfs:isDefinedBy <http://sdmx.org/wp-content/uploads/2009/01/01_sdmx_cog_annex_1_cdc_2009.pdf> .

# DECIMALS
sdmx-metadata:decimals a sdmx:MetadataProperty, rdf:Property  ;
    qb:concept sdmx-concept:decimals ;
    rdfs:label "Decimals"@en ;
    rdfs:comment """The number of digits of an observation to the right of a decimal point."""@en ;
	rdfs:label "小数"@zh-CN ;
	rdfs:comment """观察一个小数点右边的数字的数量。"""@zh-CN ;
    rdfs:isDefinedBy <http://sdmx.org/wp-content/uploads/2009/01/01_sdmx_cog_annex_1_cdc_2009.pdf> .

# DISS_FORMAT
sdmx-metadata:dissFormat a sdmx:MetadataProperty, rdf:Property  ;
    qb:concept sdmx-concept:dissFormat ;
    rdfs:label "Dissemination Format"@en ;
    rdfs:comment """Media by which statistical data and metadata are disseminated."""@en ;
	rdfs:label "发布格式"@zh-CN ;
	rdfs:comment """统计数据和元数据发布的媒体格式。"""@zh-CN ;
    rdfs:isDefinedBy <http://sdmx.org/wp-content/uploads/2009/01/01_sdmx_cog_annex_1_cdc_2009.pdf> .

# MICRO_DAT_ACC
sdmx-metadata:microDatAcc a sdmx:MetadataProperty, rdf:Property  ;
    qb:concept sdmx-concept:microDatAcc ;
    rdfs:label "Dissemination Format - mirco-data access"@en ;
    rdfs:comment """Information on whether micro-data are also disseminated."""@en ;
	rdfs:label "发布格式--微数据访问"@zh-CN ;
	rdfs:comment """有关微数据是否已经发布的信息。"""@zh-CN ;
    rdfs:isDefinedBy <http://sdmx.org/wp-content/uploads/2009/01/01_sdmx_cog_annex_1_cdc_2009.pdf> .

# NEWS_REL
sdmx-metadata:newsRel a sdmx:MetadataProperty, rdf:Property  ;
    qb:concept sdmx-concept:newsRel ;
    rdfs:label "Dissemination Format - news release"@en ;
    rdfs:comment """Regular or ad-hoc press releases linked to the data."""@en ;
	rdfs:label "发布格式--新闻稿"@zh-CN ;
	rdfs:comment """链接到数据的新闻稿的正规或临时链接。"""@zh-CN ;
    rdfs:isDefinedBy <http://sdmx.org/wp-content/uploads/2009/01/01_sdmx_cog_annex_1_cdc_2009.pdf> .

# ONLINE_DB
sdmx-metadata:onlineDb a sdmx:MetadataProperty, rdf:Property  ;
    qb:concept sdmx-concept:onlineDb ;
    rdfs:label "Dissemination Format - online database"@en ;
    rdfs:comment """Information about on-line databases in which the disseminated data can be accessed."""@en ;
	rdfs:label "发布格式--在线数据库"@zh-CN ;
	rdfs:comment """可以访问已发布数据的在线数据库的信息。"""@zh-CN ;
    rdfs:isDefinedBy <http://sdmx.org/wp-content/uploads/2009/01/01_sdmx_cog_annex_1_cdc_2009.pdf> .

# DISS_OTHER
sdmx-metadata:dissOther a sdmx:MetadataProperty, rdf:Property  ;
    qb:concept sdmx-concept:dissOther ;
    rdfs:label "Dissemination Format - other"@en ;
    rdfs:comment """References to the most important other data dissemination done."""@en ;
	rdfs:label "发布格式--其它"@zh-CN ;
	rdfs:comment """对其他最重要的数据传播工作的引用。"""@zh-CN ;
    rdfs:isDefinedBy <http://sdmx.org/wp-content/uploads/2009/01/01_sdmx_cog_annex_1_cdc_2009.pdf> .

# PUBLICATIONS
sdmx-metadata:publications a sdmx:MetadataProperty, rdf:Property  ;
    qb:concept sdmx-concept:publications ;
    rdfs:label "Dissemination Format - publications"@en ;
    rdfs:comment """Regular or ad-hoc publications in which the data are made available to the public."""@en ;
	rdfs:label "发布格式--出版物"@zh-CN ;
	rdfs:comment """用于将数据提供给公众的正规或临时出版物。"""@zh-CN ;
    rdfs:isDefinedBy <http://sdmx.org/wp-content/uploads/2009/01/01_sdmx_cog_annex_1_cdc_2009.pdf> .

# DOC_METHOD
sdmx-metadata:docMethod a sdmx:MetadataProperty, rdf:Property  ;
    qb:concept sdmx-concept:docMethod ;
    rdfs:label "Documentation on methodology"@en ;
    rdfs:comment """Descriptive text and references to methodological documents available."""@en ;
	rdfs:label "方法论文档"@zh-CN ;
	rdfs:comment """有关可用的方法论文档的描述性文字和引用。"""@zh-CN ;
    rdfs:isDefinedBy <http://sdmx.org/wp-content/uploads/2009/01/01_sdmx_cog_annex_1_cdc_2009.pdf> .

# ADV_NOTICE
sdmx-metadata:advNotice a sdmx:MetadataProperty, rdf:Property  ;
    qb:concept sdmx-concept:advNotice ;
    rdfs:label "Documentation on methodology - advance notice"@en ;
    rdfs:comment """Policy on notifying the public of changes in methodology, indicating whether the public is notified before a methodological change affects disseminated data and, if so, how long before."""@en ;
    rdfs:label "方法论文档--预先通知"@zh-CN ;
	rdfs:comment """通知公众有关方法上变化的策略，说明在方法论的变化影响发布的数据之前是否通知了公众，如果已经影响了数据，影响了多久。"""@zh-CN ;
	rdfs:isDefinedBy <http://sdmx.org/wp-content/uploads/2009/01/01_sdmx_cog_annex_1_cdc_2009.pdf> .

# EDUCATION_LEV
sdmx-metadata:educationLev a sdmx:MetadataProperty, rdf:Property  ;
    qb:concept sdmx-concept:educationLev ;
    rdfs:label "Education Level"@en ;
    rdfs:comment """The highest level of an educational programme the person has successfully completed."""@en ;
	rdfs:label "教育程度"@zh-CN ;
	rdfs:comment """某个人已经成功完成的教育计划的最高水平。"""@zh-CN ;
    rdfs:isDefinedBy <http://sdmx.org/wp-content/uploads/2009/01/01_sdmx_cog_annex_1_cdc_2009.pdf> .

# EMBARGO_TIME
sdmx-metadata:embargoTime a sdmx:MetadataProperty, rdf:Property  ;
    qb:concept sdmx-concept:embargoTime ;
    rdfs:label "Embargo Time"@en ;
    rdfs:comment """The exact time at which the data could be made available to the public."""@en ;
	rdfs:label "限制时间"@zh-CN ;
	rdfs:comment """数据向公众公开的确切时间。"""@zh-CN ;
    rdfs:isDefinedBy <http://sdmx.org/wp-content/uploads/2009/01/01_sdmx_cog_annex_1_cdc_2009.pdf> .

# FREQ
sdmx-metadata:freq a sdmx:MetadataProperty, rdf:Property  ;
    qb:concept sdmx-concept:freq ;
    rdfs:label "Frequency"@en ;
    rdfs:comment """The time interval at which observations occur over a given time period."""@en ;
	rdfs:label "频率"@zh-CN ;
	rdfs:comment """在给定的时间段内，观察发生的时间间隔。"""@zh-CN ;
    rdfs:isDefinedBy <http://sdmx.org/wp-content/uploads/2009/01/01_sdmx_cog_annex_1_cdc_2009.pdf> .

# FREQ_DETAIL
sdmx-metadata:freqDetail a sdmx:MetadataProperty, rdf:Property  ;
    qb:concept sdmx-concept:freqDetail ;
    rdfs:label "Frequency Detail"@en ;
    rdfs:comment """A further specification of the frequency to include more detailed information about the type of frequency and frequencies not commonly used."""@en ;
	rdfs:label "频率细节"@zh-CN ;
	rdfs:comment """进一步的规范，包括有关频率类型和不常用频率的更多细节信息。"""@zh-CN ;
    rdfs:isDefinedBy <http://sdmx.org/wp-content/uploads/2009/01/01_sdmx_cog_annex_1_cdc_2009.pdf> .

# FREQ_COLL
sdmx-metadata:freqColl a sdmx:MetadataProperty, rdf:Property  ;
    qb:concept sdmx-concept:freqColl ;
    rdfs:label "Frequency of data collection"@en ;
    rdfs:comment """Frequency with which the source data are collected."""@en ;
	rdfs:label "数据采集频率"@zh-CN ;
	rdfs:comment """采集源数据的频率。"""@zh-CN ;
    rdfs:isDefinedBy <http://sdmx.org/wp-content/uploads/2009/01/01_sdmx_cog_annex_1_cdc_2009.pdf> .

# FREQ_DISS
sdmx-metadata:freqDiss a sdmx:MetadataProperty, rdf:Property  ;
    qb:concept sdmx-concept:freqDiss ;
    rdfs:label "Frequency of dissemination"@en ;
    rdfs:comment """The time interval at which the statistics are disseminated over a given time period."""@en ;
	rdfs:label "发布频率"@zh-CN ;
	rdfs:comment """在一个给定的时间段内发布统计数据的时间间隔。"""@zh-CN ;
    rdfs:isDefinedBy <http://sdmx.org/wp-content/uploads/2009/01/01_sdmx_cog_annex_1_cdc_2009.pdf> .

# GROSS_NET
sdmx-metadata:grossNet a sdmx:MetadataProperty, rdf:Property  ;
    qb:concept sdmx-concept:grossNet ;
    rdfs:label "Grossing/Netting"@en ;
    rdfs:comment """Form of consolidation used in presenting the data."""@en ;
	rdfs:label "总收入/净额结算"@zh-CN ;
	rdfs:comment """用于呈现数据的综合账目表格。"""@zh-CN ;
    rdfs:isDefinedBy <http://sdmx.org/wp-content/uploads/2009/01/01_sdmx_cog_annex_1_cdc_2009.pdf> .

# IND_TYPE
sdmx-metadata:indType a sdmx:MetadataProperty, rdf:Property  ;
    qb:concept sdmx-concept:indType ;
    rdfs:label "Index Type"@en ;
    rdfs:comment """The type of index number used in the statistical production process."""@en ;
	rdfs:label "索引类型"@zh-CN ;
	rdfs:comment """在统计数据生成的过程中使用的索引号的类型。"""@zh-CN ;
    rdfs:isDefinedBy <http://sdmx.org/wp-content/uploads/2009/01/01_sdmx_cog_annex_1_cdc_2009.pdf> .

# INST_MANDATE
sdmx-metadata:instMandate a sdmx:MetadataProperty, rdf:Property  ;
    qb:concept sdmx-concept:instMandate ;
    rdfs:label "Institutional Mandate"@en ;
    rdfs:comment """Set of rules or other formal set of instructions assigning responsibility as well as the authority to an organisation for the collection, processing, and dissemination of statistics."""@en ;
    rdfs:label "机构授权"@zh-CN ;
	rdfs:comment """规则设置或其他正式分配的责任，与组织收集、处理、传播统计数据一样的授权。"""@zh-CN ;
	rdfs:isDefinedBy <http://sdmx.org/wp-content/uploads/2009/01/01_sdmx_cog_annex_1_cdc_2009.pdf> .

# INST_MAN_SHAR
sdmx-metadata:instManShar a sdmx:MetadataProperty, rdf:Property  ;
    qb:concept sdmx-concept:instManShar ;
    rdfs:label "Institutional Mandate - data sharing"@en ;
    rdfs:comment """Arrangements or procedures for data sharing and coordination between data producing agencies."""@en ;
	rdfs:label "机构授权--数据分享"@zh-CN ;
	rdfs:comment """进行数据共享的部署或流程，以及与生产数据的机构之间的协作。"""@zh-CN ;
    rdfs:isDefinedBy <http://sdmx.org/wp-content/uploads/2009/01/01_sdmx_cog_annex_1_cdc_2009.pdf> .

# INST_MAN_LA_OA
sdmx-metadata:instManLaOa a sdmx:MetadataProperty, rdf:Property  ;
    qb:concept sdmx-concept:instManLaOa ;
    rdfs:label "Institutional Mandate - legal acts and other agreements."@en ;
    rdfs:comment """Legal acts or other formal or informal agreements that assign responsibility as well as the authority to an agency for the collection, processing, and dissemination of statistics."""@en ;
    rdfs:label "机构授权--法律行为和其他协议"@zh-CN ;
	rdfs:comment """法律行为或其他正式或非正式的协议，向机构分配责任和权力，以收集、处理、传播统计数据 。"""@zh-CN ;
	rdfs:isDefinedBy <http://sdmx.org/wp-content/uploads/2009/01/01_sdmx_cog_annex_1_cdc_2009.pdf> .

# I_M_RES_REL
sdmx-metadata:iMResRel a sdmx:MetadataProperty, rdf:Property  ;
    qb:concept sdmx-concept:iMResRel ;
    rdfs:label "Institutional Mandate - respondent relations."@en ;
    rdfs:comment """Measures to encourage statistical reporting and/or to sanction non-reporting."""@en ;
	rdfs:label "机构授权--回应者关系"@zh-CN ;
	rdfs:comment """鼓励统计报告和/或批准非报告的措施。"""@zh-CN ;
    rdfs:isDefinedBy <http://sdmx.org/wp-content/uploads/2009/01/01_sdmx_cog_annex_1_cdc_2009.pdf> .

# M_AGENCY
sdmx-metadata:mAgency a sdmx:MetadataProperty, rdf:Property  ;
    qb:concept sdmx-concept:mAgency ;
    rdfs:label "Maintenance Agency"@en ;
    rdfs:comment """The organisation or other expert body that maintains a domain-specific data or metadata structure definition."""@en ;
	rdfs:label "维护机构"@zh-CN ;
	rdfs:comment """负责维护特定领域的数据或元数据的结构定义的组织或其他专家机构。"""@zh-CN ;
    rdfs:isDefinedBy <http://sdmx.org/wp-content/uploads/2009/01/01_sdmx_cog_annex_1_cdc_2009.pdf> .

# META_UPDATE
sdmx-metadata:metaUpdate a sdmx:MetadataProperty, rdf:Property  ;
    qb:concept sdmx-concept:metaUpdate ;
    rdfs:label "Metadata Update"@en ;
    rdfs:comment """The date on which the metadata element was inserted or modified in the database."""@en ;
	rdfs:label "元数据更新"@zh-CN ;
	rdfs:comment """在数据库中插入或修改元数据元素的日期。"""@zh-CN ;
    rdfs:isDefinedBy <http://sdmx.org/wp-content/uploads/2009/01/01_sdmx_cog_annex_1_cdc_2009.pdf> .

# META_CERTIFIED
sdmx-metadata:metaCertified a sdmx:MetadataProperty, rdf:Property  ;
    qb:concept sdmx-concept:metaCertified ;
    rdfs:label "Metadata Update - last certified"@en ;
    rdfs:comment """Date of the latest certification provided by the domain manager to confirm that the metadata posted are still up-to-date, even if the content has not been amended."""@en ;
    rdfs:label "元数据更新--最后认证"@zh-CN ;
	rdfs:comment """由域管理员提供的最后认证日期，用以确认发布的元数据是最新的，即使内容没有作出修订。"""@zh-CN ;
	rdfs:isDefinedBy <http://sdmx.org/wp-content/uploads/2009/01/01_sdmx_cog_annex_1_cdc_2009.pdf> .

# META_POSTED
sdmx-metadata:metaPosted a sdmx:MetadataProperty, rdf:Property  ;
    qb:concept sdmx-concept:metaPosted ;
    rdfs:label "Metadata Update - last posted"@en ;
    rdfs:comment """Date of the latest dissemination of the metadata."""@en ;
	rdfs:label "元数据更新--最后发布"@zh-CN ;
	rdfs:comment """元数据最后发布的日期。"""@zh-CN ;
    rdfs:isDefinedBy <http://sdmx.org/wp-content/uploads/2009/01/01_sdmx_cog_annex_1_cdc_2009.pdf> .

# META_LAST_UPDATE
sdmx-metadata:metaLastUpdate a sdmx:MetadataProperty, rdf:Property  ;
    qb:concept sdmx-concept:metaLastUpdate ;
    rdfs:label "Metadata Update - last update"@en ;
    rdfs:comment """Date of last update of the content of the metadata."""@en ;
	rdfs:label "元数据更新--最后更新"@zh-CN ;
	rdfs:comment """元数据内容的最后更新日期。"""@zh-CN ;
    rdfs:isDefinedBy <http://sdmx.org/wp-content/uploads/2009/01/01_sdmx_cog_annex_1_cdc_2009.pdf> .

# OBS_VALUE
sdmx-metadata:obsValue a sdmx:MetadataProperty, rdf:Property  ;
    qb:concept sdmx-concept:obsValue ;
    rdfs:label "Observation"@en ;
    rdfs:comment """The value of a particular variable at a particular period."""@en ;
	rdfs:label "观测"@zh-CN ;
	rdfs:comment """在一个特定的时期特定变量的值。"""@zh-CN ;
    rdfs:isDefinedBy <http://sdmx.org/wp-content/uploads/2009/01/01_sdmx_cog_annex_1_cdc_2009.pdf> .

# OBS_PRE_BREAK
sdmx-metadata:obsPreBreak a sdmx:MetadataProperty, rdf:Property  ;
    qb:concept sdmx-concept:obsPreBreak ;
    rdfs:label "Observation Pre-break Value"@en ;
    rdfs:comment """The observation, at a time series break period, that was calculated using the old methodology."""@en ;
	rdfs:label "观测预判值"@zh-CN ;
	rdfs:comment """在一个时间序列的中断时间，使用旧方法计算出的值。"""@zh-CN ;
    rdfs:isDefinedBy <http://sdmx.org/wp-content/uploads/2009/01/01_sdmx_cog_annex_1_cdc_2009.pdf> .

# OBS_STATUS
sdmx-metadata:obsStatus a sdmx:MetadataProperty, rdf:Property  ;
    qb:concept sdmx-concept:obsStatus ;
    rdfs:label "Observation Status"@en ;
    rdfs:comment """Information on the quality of a value or an unusual or missing value."""@en ;
	rdfs:label "观测状态"@zh-CN ;
	rdfs:comment """有关一个值或不寻常值或缺失值的质量信息。"""@zh-CN ;
    rdfs:isDefinedBy <http://sdmx.org/wp-content/uploads/2009/01/01_sdmx_cog_annex_1_cdc_2009.pdf> .

# OCCUPATION
sdmx-metadata:occupation a sdmx:MetadataProperty, rdf:Property  ;
    qb:concept sdmx-concept:occupation ;
    rdfs:label "Occupation"@en ;
    rdfs:comment """Job or position held by an individual who performs a set of tasks and duties."""@en ;
	rdfs:label "职业"@zh-CN ;
	rdfs:comment """由某个人所持有的工作或职位，这个人需要执行一系列的任务和职责。"""@zh-CN ;
    rdfs:isDefinedBy <http://sdmx.org/wp-content/uploads/2009/01/01_sdmx_cog_annex_1_cdc_2009.pdf> .

# ORIG_DATA_ID
sdmx-metadata:origDataId a sdmx:MetadataProperty, rdf:Property  ;
    qb:concept sdmx-concept:origDataId ;
    rdfs:label "Original Data Identifier"@en ;
    rdfs:comment """The data identifier as found in the originating database."""@en ;
	rdfs:label "原始数据标识符"@zh-CN ;
	rdfs:comment """在原始数据库中的数据标识符。"""@zh-CN ;
    rdfs:isDefinedBy <http://sdmx.org/wp-content/uploads/2009/01/01_sdmx_cog_annex_1_cdc_2009.pdf> .

# PROF
sdmx-metadata:prof a sdmx:MetadataProperty, rdf:Property  ;
    qb:concept sdmx-concept:prof ;
    rdfs:label "Professionalism"@en ;
    rdfs:comment """The standard, skill and ability suitable for producing statistics of good quality."""@en ;
	rdfs:label "专业性"@zh-CN ;
	rdfs:comment """适合生成好质量的统计数据的标准、技能和能力。"""@zh-CN ;
    rdfs:isDefinedBy <http://sdmx.org/wp-content/uploads/2009/01/01_sdmx_cog_annex_1_cdc_2009.pdf> .

# PROF_COND
sdmx-metadata:profCond a sdmx:MetadataProperty, rdf:Property  ;
    qb:concept sdmx-concept:profCond ;
    rdfs:label "Professionalism - code of conduct"@en ;
    rdfs:comment """Provision for assuring the qualifications of staff and allowing staff to perform their functions without intervention motivated by non-statistical objectives."""@en ;
    rdfs:label "专业性--操守准则"@zh-CN ;
	rdfs:comment """提供保证工作人员的资格，使工作人员能够履行其职责，没有出于非统计目的的进行干预。"""@zh-CN ;
	rdfs:isDefinedBy <http://sdmx.org/wp-content/uploads/2009/01/01_sdmx_cog_annex_1_cdc_2009.pdf> .

# PROF_IMP
sdmx-metadata:profImp a sdmx:MetadataProperty, rdf:Property  ;
    qb:concept sdmx-concept:profImp ;
    rdfs:label "Professionalism - impartiality"@en ;
    rdfs:comment """Description of the elements providing assurances that statistics are produced on an impartial basis."""@en ;
	rdfs:label "专业性--公正"@zh-CN ;
	rdfs:comment """该元素描述提供了保证，统计数据是在公正的基础上产生的。"""@zh-CN ;
    rdfs:isDefinedBy <http://sdmx.org/wp-content/uploads/2009/01/01_sdmx_cog_annex_1_cdc_2009.pdf> .

# PROF_METH
sdmx-metadata:profMeth a sdmx:MetadataProperty, rdf:Property  ;
    qb:concept sdmx-concept:profMeth ;
    rdfs:label "Professionalism - methodology"@en ;
    rdfs:comment """Describes the elements providing assurances that the choices of sources and statistical techniques as well as decisions about dissemination are informed solely by statistical considerations."""@en ;
    rdfs:label "专业性--方法"@zh-CN ;
	rdfs:comment """该元素描述提供了保证，来源和统计技术的选择以及传播决策，基于统计考量将被单独通知。"""@zh-CN ;
	rdfs:isDefinedBy <http://sdmx.org/wp-content/uploads/2009/01/01_sdmx_cog_annex_1_cdc_2009.pdf> .

# PROF_STAT_COM
sdmx-metadata:profStatCom a sdmx:MetadataProperty, rdf:Property  ;
    qb:concept sdmx-concept:profStatCom ;
    rdfs:label "Professionalism - statistical commentary"@en ;
    rdfs:comment """Describes the elements providing assurances that the statistical entity is entitled to comment on erroneous interpretation and misuse of statistics."""@en ;
    rdfs:label "专业性--统计注释"@zh-CN ;
	rdfs:comment """该元素描述提供了保证，统计实体有权对统计数据的错误诠释和滥用发表评论。"""@zh-CN ;
	rdfs:isDefinedBy <http://sdmx.org/wp-content/uploads/2009/01/01_sdmx_cog_annex_1_cdc_2009.pdf> .

# PUNCTUALITY
sdmx-metadata:punctuality a sdmx:MetadataProperty, rdf:Property  ;
    qb:concept sdmx-concept:punctuality ;
    rdfs:label "Punctuality"@en ;
    rdfs:comment """Time lag between the actual delivery of the data and the target date when it should have been delivered."""@en ;
	rdfs:label "正点率"@zh-CN ;
	rdfs:comment """当数据应该已经交付时，实际交付时间和应该交付时间的时滞。"""@zh-CN ;
    rdfs:isDefinedBy <http://sdmx.org/wp-content/uploads/2009/01/01_sdmx_cog_annex_1_cdc_2009.pdf> .

# QUALITY_MGMNT
sdmx-metadata:qualityMgmnt a sdmx:MetadataProperty, rdf:Property  ;
    qb:concept sdmx-concept:qualityMgmnt ;
    rdfs:label "Quality Management"@en ;
    rdfs:comment """Systems and frameworks in place within an organisation to manage the quality of statistical products and processes."""@en ;
	rdfs:label "质量管理"@zh-CN ;
	rdfs:comment """在组织内管理统计产品和流程的质量的系统和框架。"""@zh-CN ;
    rdfs:isDefinedBy <http://sdmx.org/wp-content/uploads/2009/01/01_sdmx_cog_annex_1_cdc_2009.pdf> .

# QUALITY_ASSMNT
sdmx-metadata:qualityAssmnt a sdmx:MetadataProperty, rdf:Property  ;
    qb:concept sdmx-concept:qualityAssmnt ;
    rdfs:label "Quality Management - assessment"@en ;
    rdfs:comment """Overall assessment of data quality, based on standard quality criteria."""@en ;
	rdfs:label "质量管理--评估"@zh-CN ;
	rdfs:comment """基于标准的质量标准，数据质量的整体评估。"""@zh-CN ;
    rdfs:isDefinedBy <http://sdmx.org/wp-content/uploads/2009/01/01_sdmx_cog_annex_1_cdc_2009.pdf> .

# QUALITY_ASSURE
sdmx-metadata:qualityAssure a sdmx:MetadataProperty, rdf:Property  ;
    qb:concept sdmx-concept:qualityAssure ;
    rdfs:label "Quality Management - assurance"@en ;
    rdfs:comment """Guidelines focusing on quality in general and dealing with quality of statistical programmes, including measures for ensuring the efficient use of resources."""@en ;
    rdfs:label "质量管理--保证"@zh-CN ;
	rdfs:comment """专注于一般质量的指引和处理统计方案的质量，包括采取措施以确保有效地利用资源。"""@zh-CN ;
	rdfs:isDefinedBy <http://sdmx.org/wp-content/uploads/2009/01/01_sdmx_cog_annex_1_cdc_2009.pdf> .

# QUALITY_DOC
sdmx-metadata:qualityDoc a sdmx:MetadataProperty, rdf:Property  ;
    qb:concept sdmx-concept:qualityDoc ;
    rdfs:label "Quality Management - documentation"@en ;
    rdfs:comment """Documentation on procedures applied for quality management and quality assessment."""@en ;
	rdfs:label "质量管理--文档"@zh-CN ;
	rdfs:comment """应用了质量管理和质量评估的流程文档。"""@zh-CN ;
    rdfs:isDefinedBy <http://sdmx.org/wp-content/uploads/2009/01/01_sdmx_cog_annex_1_cdc_2009.pdf> .

# RECORDING
sdmx-metadata:recording a sdmx:MetadataProperty, rdf:Property  ;
    qb:concept sdmx-concept:recording ;
    rdfs:label "Recording Basis"@en ;
    rdfs:comment """Processes and standards employed in calculating statistical aggregates."""@en ;
	rdfs:label "记录依据"@zh-CN ;
	rdfs:comment """在计算统计总量时用到的流程或标准。"""@zh-CN ;
    rdfs:isDefinedBy <http://sdmx.org/wp-content/uploads/2009/01/01_sdmx_cog_annex_1_cdc_2009.pdf> .

# REF_AREA
sdmx-metadata:refArea a sdmx:MetadataProperty, rdf:Property  ;
    qb:concept sdmx-concept:refArea ;
    rdfs:label "Reference Area"@en ;
    rdfs:comment """The country or geographic area to which the measured statistical phenomenon relates."""@en ;
	rdfs:label "引用区域"@zh-CN ;
	rdfs:comment """测量的统计现象所关联的国家或地理区域。"""@zh-CN ;
    rdfs:isDefinedBy <http://sdmx.org/wp-content/uploads/2009/01/01_sdmx_cog_annex_1_cdc_2009.pdf> .

# REF_PERIOD
sdmx-metadata:refPeriod a sdmx:MetadataProperty, rdf:Property  ;
    qb:concept sdmx-concept:refPeriod ;
    rdfs:label "Reference Period"@en ;
    rdfs:comment """The period of time or point in time to which the measured observation is intended to refer."""@en ;
	rdfs:label "引用时段"@zh-CN ;
	rdfs:comment """测量的观察值意在指向的时段或时间点。"""@zh-CN ;
    rdfs:isDefinedBy <http://sdmx.org/wp-content/uploads/2009/01/01_sdmx_cog_annex_1_cdc_2009.pdf> .

# REF_PER_WGTS
sdmx-metadata:refPerWgts a sdmx:MetadataProperty, rdf:Property  ;
    qb:concept sdmx-concept:refPerWgts ;
    rdfs:label "Reference Period - weights"@en ;
    rdfs:comment """Dates or periods to which the observations used to compile the weights refer."""@en ;
	rdfs:label "引用时段--权重"@zh-CN ;
	rdfs:comment """观测用于编制的权重所涉及的日期或时段。"""@zh-CN ;
    rdfs:isDefinedBy <http://sdmx.org/wp-content/uploads/2009/01/01_sdmx_cog_annex_1_cdc_2009.pdf> .

# REL_POLICY
sdmx-metadata:relPolicy a sdmx:MetadataProperty, rdf:Property  ;
    qb:concept sdmx-concept:relPolicy ;
    rdfs:label "Release Policy"@en ;
    rdfs:comment """Rules for disseminating statistical data to interested parties."""@en ;
	rdfs:label "发行策略"@zh-CN ;
	rdfs:comment """向有关方面传播统计数据的规则。"""@zh-CN ;
    rdfs:isDefinedBy <http://sdmx.org/wp-content/uploads/2009/01/01_sdmx_cog_annex_1_cdc_2009.pdf> .

# REL_POL_LEG_ACTS
sdmx-metadata:relPolLegActs a sdmx:MetadataProperty, rdf:Property  ;
    qb:concept sdmx-concept:relPolLegActs ;
    rdfs:label "Release Policy - legal acts and other agreements"@en ;
    rdfs:comment """Legal acts and other agreements pertaining to data access."""@en ;
	rdfs:label "发行策略--法律行为和其他协议"@zh-CN ;
	rdfs:comment """有关数据访问的法律行为和其他协议。"""@zh-CN ;
    rdfs:isDefinedBy <http://sdmx.org/wp-content/uploads/2009/01/01_sdmx_cog_annex_1_cdc_2009.pdf> .

# REL_COMMENT
sdmx-metadata:relComment a sdmx:MetadataProperty, rdf:Property  ;
    qb:concept sdmx-concept:relComment ;
    rdfs:label "Release Policy - policy commentary"@en ;
    rdfs:comment """Legal acts and other agreements pertaining to data access."""@en ;
	rdfs:label "发行策略--策略注释"@zh-CN ;
	rdfs:comment """有关数据访问的法律行为和其他协议。"""@zh-CN ;
    rdfs:isDefinedBy <http://sdmx.org/wp-content/uploads/2009/01/01_sdmx_cog_annex_1_cdc_2009.pdf> .

# REL_CAL_POLICY
sdmx-metadata:relCalPolicy a sdmx:MetadataProperty, rdf:Property  ;
    qb:concept sdmx-concept:relCalPolicy ;
    rdfs:label "Release Policy - release calendar"@en ;
    rdfs:comment """The schedule of statistical release dates."""@en ;
	rdfs:label "发行策略--发行日历"@zh-CN ;
	rdfs:comment """统计数据发布日期的时间表。"""@zh-CN ;
    rdfs:isDefinedBy <http://sdmx.org/wp-content/uploads/2009/01/01_sdmx_cog_annex_1_cdc_2009.pdf> .

# REL_CAL_ACCESS
sdmx-metadata:relCalAccess a sdmx:MetadataProperty, rdf:Property  ;
    qb:concept sdmx-concept:relCalAccess ;
    rdfs:label "Release Policy - release calendar access"@en ;
    rdfs:comment """Access to the release calendar information."""@en ;
	rdfs:label "发行策略--发行日历获取"@zh-CN ;
	rdfs:comment """获取发行日历信息。"""@zh-CN ;
    rdfs:isDefinedBy <http://sdmx.org/wp-content/uploads/2009/01/01_sdmx_cog_annex_1_cdc_2009.pdf> .

# REL_POL_TRA
sdmx-metadata:relPolTra a sdmx:MetadataProperty, rdf:Property  ;
    qb:concept sdmx-concept:relPolTra ;
    rdfs:label "Release Policy - transparency"@en ;
    rdfs:comment """Dissemination of the release policy to the public."""@en ;
	rdfs:label "发行策略--透明度"@zh-CN ;
	rdfs:comment """面向公众的发行策略的传播。"""@zh-CN ;
    rdfs:isDefinedBy <http://sdmx.org/wp-content/uploads/2009/01/01_sdmx_cog_annex_1_cdc_2009.pdf> .

# REL_POL_US_AC
sdmx-metadata:relPolUsAc a sdmx:MetadataProperty, rdf:Property  ;
    qb:concept sdmx-concept:relPolUsAc ;
    rdfs:label "Release Policy - user access"@en ;
    rdfs:comment """The policy for release of the data to users, the scope of dissemination (eg, to the public, to selected users), how users are informed that the data are being released, and whether the policy provides determines the dissemination of statistical data to all users."""@en ;
    rdfs:label "发行策略--用户访问"@zh-CN ;
	rdfs:comment """向用户发布数据的策略，传播的范围（例如，向社会公开，向选定的用户），是如何通知用户数据已经发行的，以及策略是否提供了将数据传播到所有用户的判定。"""@zh-CN ;
	rdfs:isDefinedBy <http://sdmx.org/wp-content/uploads/2009/01/01_sdmx_cog_annex_1_cdc_2009.pdf> .

# RELEVANCE
sdmx-metadata:relevance a sdmx:MetadataProperty, rdf:Property  ;
    qb:concept sdmx-concept:relevance ;
    rdfs:label "Relevance"@en ;
    rdfs:comment """The degree to which statistical information meets the real or perceived needs of clients."""@en ;
	rdfs:label "相关性"@zh-CN ;
	rdfs:comment """统计信息满足客户的实际或想象的需求的程度。"""@zh-CN ;
    rdfs:isDefinedBy <http://sdmx.org/wp-content/uploads/2009/01/01_sdmx_cog_annex_1_cdc_2009.pdf> .

# COMPLETENESS
sdmx-metadata:completeness a sdmx:MetadataProperty, rdf:Property  ;
    qb:concept sdmx-concept:completeness ;
    rdfs:label "Relevance - Completeness"@en ;
    rdfs:comment """The extent to which all statistics that are needed are available."""@en ;
	rdfs:label "相关性--完备性"@zh-CN ;
	rdfs:comment """在何种程度上所需要的所有统计数据都可用。"""@zh-CN ;
    rdfs:isDefinedBy <http://sdmx.org/wp-content/uploads/2009/01/01_sdmx_cog_annex_1_cdc_2009.pdf> .

# USER_NEEDS
sdmx-metadata:userNeeds a sdmx:MetadataProperty, rdf:Property  ;
    qb:concept sdmx-concept:userNeeds ;
    rdfs:label "Relevance - user needs"@en ;
    rdfs:comment """Description of users and their respective needs with respect to the statistical data."""@en ;
	rdfs:label "相关性--用户需求"@zh-CN ;
	rdfs:comment """描述用户和他们各自的需求方面的统计数据。"""@zh-CN ;
    rdfs:isDefinedBy <http://sdmx.org/wp-content/uploads/2009/01/01_sdmx_cog_annex_1_cdc_2009.pdf> .

# USER_SAT
sdmx-metadata:userSat a sdmx:MetadataProperty, rdf:Property  ;
    qb:concept sdmx-concept:userSat ;
    rdfs:label "Relevance - user satisifaction"@en ;
    rdfs:comment """Measure to determine user satisfaction."""@en ;
	rdfs:label "相关性--用户满意度"@zh-CN ;
	rdfs:comment """判断用户满意度的测量。"""@zh-CN ;
    rdfs:isDefinedBy <http://sdmx.org/wp-content/uploads/2009/01/01_sdmx_cog_annex_1_cdc_2009.pdf> .

# REP_AGENCY
sdmx-metadata:repAgency a sdmx:MetadataProperty, rdf:Property  ;
    qb:concept sdmx-concept:repAgency ;
    rdfs:label "Reporting Agency"@en ;
    rdfs:comment """The organisation that supplies the data for a given  instance of the statistics."""@en ;
	rdfs:label "报告机构"@zh-CN ;
	rdfs:comment """该组织对一个给定的统计实例提供数据。"""@zh-CN ;
    rdfs:isDefinedBy <http://sdmx.org/wp-content/uploads/2009/01/01_sdmx_cog_annex_1_cdc_2009.pdf> .

# SAMPLING
sdmx-metadata:sampling a sdmx:MetadataProperty, rdf:Property  ;
    qb:concept sdmx-concept:sampling ;
    rdfs:label "Sampling"@en ;
    rdfs:comment """The process of selecting a number of cases from all the cases in a particular group or universe."""@en ;
	rdfs:label "采样"@zh-CN ;
	rdfs:comment """在一个特定的组或领域，从所有实例中选择一些实例的流程。"""@zh-CN ;
    rdfs:isDefinedBy <http://sdmx.org/wp-content/uploads/2009/01/01_sdmx_cog_annex_1_cdc_2009.pdf> .

# SEX
sdmx-metadata:sex a sdmx:MetadataProperty, rdf:Property  ;
    qb:concept sdmx-concept:sex ;
    rdfs:label "Sex"@en ;
    rdfs:comment """The state of being male or female."""@en ;
	rdfs:label "性别"@zh-CN ;
	rdfs:comment """男、女。"""@zh-CN ;
    rdfs:isDefinedBy <http://sdmx.org/wp-content/uploads/2009/01/01_sdmx_cog_annex_1_cdc_2009.pdf> .

# SOURCE_TYPE
sdmx-metadata:sourceType a sdmx:MetadataProperty, rdf:Property  ;
    qb:concept sdmx-concept:sourceType ;
    rdfs:label "Source Data"@en ;
    rdfs:comment """Characteristics and components of the raw statistical data used for compiling statistical aggregates."""@en ;
	rdfs:label "源数据"@zh-CN ;
	rdfs:comment """用于编制统计聚集的原始数据的特征和组件。"""@zh-CN ;
    rdfs:isDefinedBy <http://sdmx.org/wp-content/uploads/2009/01/01_sdmx_cog_annex_1_cdc_2009.pdf> .

# STAT_CONC_DEF
sdmx-metadata:statConcDef a sdmx:MetadataProperty, rdf:Property  ;
    qb:concept sdmx-concept:statConcDef ;
    rdfs:label "Statistical Concepts and Definitions"@en ;
    rdfs:comment """Statistical characteristics of statistical observations."""@en ;
	rdfs:label "统计概念与定义"@zh-CN ;
	rdfs:comment """统计观测值的统计特征。"""@zh-CN ;
    rdfs:isDefinedBy <http://sdmx.org/wp-content/uploads/2009/01/01_sdmx_cog_annex_1_cdc_2009.pdf> .

# STAT_POP
sdmx-metadata:statPop a sdmx:MetadataProperty, rdf:Property  ;
    qb:concept sdmx-concept:statPop ;
    rdfs:label "Statistical Population"@en ;
    rdfs:comment """The total membership or population or "universe" of a defined class of people, objects or events."""@en ;
	rdfs:label "统计总数"@zh-CN ;
	rdfs:comment """成员总数或人口或定义的一类人、物或事件的“全体”。"""@zh-CN ;
    rdfs:isDefinedBy <http://sdmx.org/wp-content/uploads/2009/01/01_sdmx_cog_annex_1_cdc_2009.pdf> .

# STAT_UNIT
sdmx-metadata:statUnit a sdmx:MetadataProperty, rdf:Property  ;
    qb:concept sdmx-concept:statUnit ;
    rdfs:label "Statistical Unit"@en ;
    rdfs:comment """Entity for which information is sought and for which statistics are ultimately compiled."""@en ;
	rdfs:label "统计部门"@zh-CN ;
	rdfs:comment """寻求信息和最终编制统计数据的实体。"""@zh-CN ;
    rdfs:isDefinedBy <http://sdmx.org/wp-content/uploads/2009/01/01_sdmx_cog_annex_1_cdc_2009.pdf> .

# TIME_FORMAT
sdmx-metadata:timeFormat a sdmx:MetadataProperty, rdf:Property  ;
    qb:concept sdmx-concept:timeFormat ;
    rdfs:label "Time Format"@en ;
    rdfs:comment """Technical format in which time is represented for the measured phenomenon."""@en ;
	rdfs:label "时间格式"@zh-CN ;
	rdfs:comment """表示测量现象的时间的技术格式。"""@zh-CN ;
    rdfs:isDefinedBy <http://sdmx.org/wp-content/uploads/2009/01/01_sdmx_cog_annex_1_cdc_2009.pdf> .

# TIME_PERIOD
sdmx-metadata:timePeriod a sdmx:MetadataProperty, rdf:Property  ;
    qb:concept sdmx-concept:timePeriod ;
    rdfs:label "Time Period"@en ;
    rdfs:comment """The period of time or point in time to which the measured observation refers."""@en ;
	rdfs:label "时段"@zh-CN ;
	rdfs:comment """实测所指的一段时间或时间点。"""@zh-CN ;
    rdfs:isDefinedBy <http://sdmx.org/wp-content/uploads/2009/01/01_sdmx_cog_annex_1_cdc_2009.pdf> .

# TIME_PER_COLLECT
sdmx-metadata:timePerCollect a sdmx:MetadataProperty, rdf:Property  ;
    qb:concept sdmx-concept:timePerCollect ;
    rdfs:label "Time Period - collection"@en ;
    rdfs:comment """Dates or periods during which the observations have been collected (such as middle, average or end of period) to compile the indicator for the target reference period."""@en ;
    rdfs:label "时段--采集"@zh-CN ;
	rdfs:comment """在目标参考时段编制采集的观测数据的日期或时段。"""@zh-CN ;
	rdfs:isDefinedBy <http://sdmx.org/wp-content/uploads/2009/01/01_sdmx_cog_annex_1_cdc_2009.pdf> .

# TIMELINESS
sdmx-metadata:timeliness a sdmx:MetadataProperty, rdf:Property  ;
    qb:concept sdmx-concept:timeliness ;
    rdfs:label "Timeliness"@en ;
    rdfs:comment """Length of time between data availability and the event or phenomenon they describe."""@en ;
	rdfs:label "时效性"@zh-CN ;
	rdfs:comment """数据的可用性和它们所描述的事件或现象之间的时间长度。"""@zh-CN ;
    rdfs:isDefinedBy <http://sdmx.org/wp-content/uploads/2009/01/01_sdmx_cog_annex_1_cdc_2009.pdf> .

# TIME_OUTPUT
sdmx-metadata:timeOutput a sdmx:MetadataProperty, rdf:Property  ;
    qb:concept sdmx-concept:timeOutput ;
    rdfs:label "Timeliness - output"@en ;
    rdfs:comment """The lapse of time between the end of a reference period and dissemination of the data."""@en ;
	rdfs:label "时效性--输出"@zh-CN ;
	rdfs:comment """数据的引用期结束和传播之间的时间间隔。"""@zh-CN ;
    rdfs:isDefinedBy <http://sdmx.org/wp-content/uploads/2009/01/01_sdmx_cog_annex_1_cdc_2009.pdf> .

# TIME_SOURCE
sdmx-metadata:timeSource a sdmx:MetadataProperty, rdf:Property  ;
    qb:concept sdmx-concept:timeSource ;
    rdfs:label "Timeliness - source data"@en ;
    rdfs:comment """The time between the end of a reference period and actual receipt of the data by the compiling agency."""@en ;
	rdfs:label "时效性--源数据"@zh-CN ;
	rdfs:comment """编制机构对数据的引用期结束和实际收到数据之间的时间。"""@zh-CN ;
    rdfs:isDefinedBy <http://sdmx.org/wp-content/uploads/2009/01/01_sdmx_cog_annex_1_cdc_2009.pdf> .

# TITLE
sdmx-metadata:title a sdmx:MetadataProperty, rdf:Property  ;
    qb:concept sdmx-concept:title ;
    rdfs:label "Title"@en ;
    rdfs:comment """Textual label used as identification of a statistical object."""@en ;
	rdfs:label "标题"@zh-CN ;
	rdfs:comment """用于标识一个统计对象的文字标签。"""@zh-CN ;
    rdfs:isDefinedBy <http://sdmx.org/wp-content/uploads/2009/01/01_sdmx_cog_annex_1_cdc_2009.pdf> .

# UNIT_MULT
sdmx-metadata:unitMult a sdmx:MetadataProperty, rdf:Property  ;
    qb:concept sdmx-concept:unitMult ;
    rdfs:label "Unit Multiplier"@en ;
    rdfs:comment """Exponent in base 10 specified so that multiplying the observation numeric values by 10^UNIT_MULT gives a value expressed in the UNIT."""@en ;
	rdfs:label "单位乘数"@zh-CN ;
	rdfs:comment """指定以10为基数的指数，观察数值乘以10^ UNIT_MULT给出了用UNIT表示的值。"""@zh-CN ;
    rdfs:isDefinedBy <http://sdmx.org/wp-content/uploads/2009/01/01_sdmx_cog_annex_1_cdc_2009.pdf> .

# UNIT_MEASURE
sdmx-metadata:unitMeasure a sdmx:MetadataProperty, rdf:Property  ;
    qb:concept sdmx-concept:unitMeasure ;
    rdfs:label "Unit of Measure"@en ;
    rdfs:comment """The unit in which the data values are measured."""@en ;
	rdfs:label "测量单位"@zh-CN ;
	rdfs:comment """测量数据值的单位。"""@zh-CN ;
    rdfs:isDefinedBy <http://sdmx.org/wp-content/uploads/2009/01/01_sdmx_cog_annex_1_cdc_2009.pdf> .

# UNIT_MEAS_DETAIL
sdmx-metadata:unitMeasDetail a sdmx:MetadataProperty, rdf:Property  ;
    qb:concept sdmx-concept:unitMeasDetail ;
    rdfs:label "Unit of Measure Detail"@en ;
    rdfs:comment """Additional textual information on the unit of measure."""@en ;
	rdfs:label "测量单位细节"@zh-CN ;
	rdfs:comment """测量单位的附加文本信息。"""@zh-CN ;
    rdfs:isDefinedBy <http://sdmx.org/wp-content/uploads/2009/01/01_sdmx_cog_annex_1_cdc_2009.pdf> .

# VALUATION
sdmx-metadata:valuation a sdmx:MetadataProperty, rdf:Property  ;
    qb:concept sdmx-concept:valuation ;
    rdfs:label "Valuation"@en ;
    rdfs:comment """The definition of the price per unit, for goods and services flows and asset stocks."""@en ;
	rdfs:label "计价"@zh-CN ;
	rdfs:comment """对商品和服务的流动和资产股每单位的价格的定义。"""@zh-CN ;
    rdfs:isDefinedBy <http://sdmx.org/wp-content/uploads/2009/01/01_sdmx_cog_annex_1_cdc_2009.pdf> .

### Linking COG metadata concepts to standard vocabularies - to be reviewed ###

sdmx-metadata:comment rdfs:subPropertyOf rdfs:comment .
sdmx-metadata:contactEmail rdfs:subPropertyOf  vcard:email .
sdmx-metadata:contactFax rdfs:subPropertyOf vcard:fax .
sdmx-metadata:contactMail rdfs:subPropertyOf vcard:adr .
sdmx-metadata:contactName rdfs:subPropertyOf vcard:fn .
sdmx-metadata:contactOrganisation rdfs:subPropertyOf vcard:organization-name .
sdmx-metadata:organisationUnit rdfs:subPropertyOf vcard:organization-unit .
sdmx-metadata:contactFunct rdfs:subPropertyOf vcard:role .
sdmx-metadata:contactPhone rdfs:subPropertyOf vcard:tel .

### Binding to the corresponding COG Code lists ###

sdmx-metadata:currency a qb:CodedProperty ;
    qb:codeList sdmx-code:currency ;
    rdfs:range sdmx-code:Currency .

sdmx-metadata:area a qb:CodedProperty ;
    qb:codeList sdmx-code:area ;
    rdfs:range sdmx-code:Area .

sdmx-metadata:decimals a qb:CodedProperty ;
    qb:codeList sdmx-code:decimals ;
    rdfs:range sdmx-code:Decimals .

sdmx-metadata:freq a qb:CodedProperty ;
    qb:codeList sdmx-code:freq ;
    rdfs:range sdmx-code:Freq .

sdmx-metadata:confStatus a qb:CodedProperty ;
    qb:codeList sdmx-code:confStatus ;
    rdfs:range sdmx-code:ConfStatus .

sdmx-metadata:obsStatus a qb:CodedProperty ;
    qb:codeList sdmx-code:obsStatus ;
    rdfs:range sdmx-code:ObsStatus .

sdmx-metadata:sex a qb:CodedProperty ;
    qb:codeList sdmx-code:sex ;
    rdfs:range sdmx-code:Sex .

sdmx-metadata:timeFormat a qb:CodedProperty ;
    qb:codeList sdmx-code:timeFormat ;
    rdfs:range sdmx-code:TimeFormat .

sdmx-metadata:unitMult a qb:CodedProperty ;
    qb:codeList sdmx-code:unitMult ;
    rdfs:range sdmx-code:UnitMult .

