@prefix rdf:     <http://www.w3.org/1999/02/22-rdf-syntax-ns#> .
@prefix rdfs:    <http://www.w3.org/2000/01/rdf-schema#> .
@prefix owl:     <http://www.w3.org/2002/07/owl#> .
@prefix skos:    <http://www.w3.org/2004/02/skos/core#> .
@prefix foaf:    <http://xmlns.com/foaf/0.1/> .
@prefix scovo:   <http://purl.org/NET/scovo#> .
@prefix void:    <http://rdfs.org/ns/void#> .
@prefix vcard:   <http://www.w3.org/2006/vcard/ns#> .
@prefix sdmx:    <http://purl.org/linked-data/sdmx#> .
@prefix sdmx-concept:    <http://purl.org/linked-data/sdmx/2009/concept#> .
@prefix sdmx-dimension:  <http://purl.org/linked-data/sdmx/2009/dimension#> .
@prefix sdmx-attribute:  <http://purl.org/linked-data/sdmx/2009/attribute#> .
@prefix sdmx-measure:    <http://purl.org/linked-data/sdmx/2009/measure#> .
@prefix sdmx-metadata:   <http://purl.org/linked-data/sdmx/2009/metadata#> .
@prefix sdmx-code:       <http://purl.org/linked-data/sdmx/2009/code#> .
@prefix sdmx-subject:    <http://purl.org/linked-data/sdmx/2009/subject#> .
@prefix dcterms:         <http://purl.org/dc/terms/>.
@prefix qb:              <http://purl.org/linked-data/cube#> .

<http://purl.org/linked-data/sdmx/2009/subject#>
    a owl:Ontology;
    rdfs:label "The vocabulary about SDMX subject."@en;
	rdfs:label "有关SDMX主题的词汇集"@zh-CN;
    rdfs:comment "These annotations is added by chuci.info."@en;
    rdfs:comment "这些本体声明标记由chuci.info添加。"@zh-CN .

sdmx-subject:subjectMatterDomain a skos:ConceptScheme;
    skos:prefLabel "SDMX Statistical Subject-Matter Domains - concept scheme"@en;
	skos:prefLabel "SDMX统计主题领域 - 概念体系"@zh-CN;
    rdfs:label "SDMX Statistical Subject-Matter Domains"@en;
	rdfs:label "SDMX统计主题领域 - 概念体系"@zh-CN;
    skos:note """The SDMX Content Guidelines for Statistical Subject-Matter Domains."""@en;
	skos:note ""统计主题领域的SDMX内容指导"""@zh-CN;
    skos:definition <http://sdmx.org/wp-content/uploads/2009/01/03_sdmx_cog_annex_3_smd_2009.pdf> ;
    rdfs:seeAlso sdmx-subject:SubjectMatterDomain .

sdmx-subject:SubjectMatterDomain a rdfs:Class, owl:Class;
    rdfs:subClassOf skos:Concept ;
    rdfs:label "SDMX Statistical Subject-Matter Domains - concept class"@en;
	rdfs:label "SDMX统计主题领域 - 概念类"@zh-CN;
    rdfs:comment """The SDMX Content Guidelines for Statistical Subject-Matter Domains."""@en;
	rdfs:comment """统计主题领域的SDMX内容指导"""@zh-CN;
    rdfs:seeAlso sdmx-subject:subjectMatterDomain .

sdmx-subject:1 a skos:Concept, sdmx:Concept, sdmx-subject:SubjectMatterDomain;
    skos:topConceptOf sdmx-subject:subjectMatterDomain;
    skos:prefLabel "Demographic and social statistics"@en ;
	skos:prefLabel "人口与社会统计"@zh-CN;
    skos:notation "1" ;
    skos:definition """Time-use - statistics on the use of time by individuals, often related to work-life balance (reconciling family responsibilities and paid work); unpaid work. 
Excludes 
- working time (1.2)"""@en;
	skos:definition """时间使用 - 个人使用时间上的统计数据，往往涉及到工作与生活的平衡（兼顾家庭责任和有偿工作）;无偿工作。
不包括
- 工作时间（1.2）"""@zh-CN;
	. 
sdmx-subject:subjectMatterDomain skos:hasTopConcept sdmx-subject:1 .

sdmx-subject:1.1 a skos:Concept, sdmx:Concept, sdmx-subject:SubjectMatterDomain;
    skos:broader sdmx-subject:1;
    skos:prefLabel "Population and migration"@en ;
	skos:prefLabel "人口与移民"@zh-CN;
    skos:notation "1.1" ;
    skos:definition """Population and migration - covers work in population and demographic statistics, topics like demography, vital statistics, population structures and growth, demographic projections, families and households (marriages, divorces, household size), migration, refugees and asylum seekers. 
Excludes
- causes of death (1.4)"""@en;
	skos:definition """人口和迁移 - 涵盖人口和人口统计工作，比如人口统计、生命统计、人口结构和增长、人口预测、家人和家庭（结婚，离婚，家庭规模）、移民、难民和寻求庇护者之类的主题。
不包括
 - 死亡原因（1.4）"""@zh-CN;
	. 

sdmx-subject:1.2 a skos:Concept, sdmx:Concept, sdmx-subject:SubjectMatterDomain;
    skos:broader sdmx-subject:1;
    skos:prefLabel "Labour"@en ;
	skos:prefLabel ""@zh-CN;
    skos:notation "1.2" ;
    skos:definition """Labour -  covers statistics on labour force, labour market, employment and unemployment; the more detailed topics include economically active population, labour conditions, health and safety at work (accidents at work, occupational injuries and diseases, work-related health problems), working time and other working conditions, strikes and lockouts, job vacancies, job creation. 
Excludes 
- migrant workers (1.1)
- unemployment insurance and unemployment benefits (1.6)
- trade union membership (1.10)
- unpaid work (1.11)
- statistics on earnings, wages and salaries (2.8)
- labour cost (2.8)"""@en;
	skos:definition """劳工 - 包括劳动力、劳动力市场、就业和失业的统计数据；更详细的主题包括经济活动人口、劳工条件、健康和工作安全（工伤事故，工伤及职业病，与工作有关的健康问题）、工作时间和其他工作条件、罢工和停工、职位空缺、创造就业机会。
不包括
 - 外来务工人员（1.1）
 - 失业保险和失业救济金人数（1.6）
 - 工会会员（1.10）
 - 无偿工作（1.11）
 - 收入、工资和薪金的统计数字（2.8）
 - 劳动力成本（2.8）"""@zh-CN;
	. 

sdmx-subject:1.3 a skos:Concept, sdmx:Concept, sdmx-subject:SubjectMatterDomain;
    skos:broader sdmx-subject:1;
    skos:prefLabel "Education"@en ;
	skos:prefLabel "教育"@zh-CN;
    skos:notation "1.3" ;
    skos:definition """Education - includes educational participation, illiteracy, educational institutions and systems, human and financial resources invested in education, lifelong learning, vocational training and adult learning, impact of education, assessments of student performance, etc."""@en;
	skos:definition """教育 - 包括入学机会、文盲、教育机构和系统、在教育中投入的人力和财力资源、终身学习、职业培训和成人教育、教育的影响、评估学生的表现等等。"""@zh-CN;
	. 

sdmx-subject:1.4 a skos:Concept, sdmx:Concept, sdmx-subject:SubjectMatterDomain;
    skos:broader sdmx-subject:1;
    skos:prefLabel "Health"@en ;
	skos:prefLabel "健康"@zh-CN;
    skos:notation "1.4" ;
    skos:definition """Health - covers the health and mortality related statistical activities, including topics like life expectancy, health status, health and safety, health determinants (including lifestyle, nutrition, smoking, alcohol abuse), health resources and expenditure, health care systems, morbidity and mortality (including infant and child mortality), hospital admission, causes of illness and death, specific diseases (e.g. AIDS), disabilities, pharmaceutical consumption and sales, health personnel, remuneration of health professions, environmental health status, health inequality, health accounts.
Excludes 
- work related health and safety (1.2) 
- victimisation from criminal behaviour (1.8)
- traffic accidents and injuries (2.4.4)"""@en;
	skos:definition """健康 - 涵盖了与健康和死亡率有关的统计活动，包括预期寿命、健康状况、健康和安全、健康的决定因素（包括生活方式、营养、吸烟、酗酒）、卫生资源和支出、医疗保健系统、发病率和死亡率（包括婴儿和儿童死亡率）、入院、疾病和死亡原因、特定疾病（如艾滋病）、残疾人、消费和销售医药、保健人员、保健专业的薪酬、环境的健康状况、医疗不平等、健康账户等主题。
不包括
 - 与工作有关健康和安全（1.2）
 - 从犯罪行为受害（1.8）
 - 交通事故和受伤（2.4.4）"""@zh-CN;
	. 

sdmx-subject:1.5 a skos:Concept, sdmx:Concept, sdmx-subject:SubjectMatterDomain;
    skos:broader sdmx-subject:1;
    skos:prefLabel "Income and consumption"@en ;
	skos:prefLabel "收入与消费"@zh-CN;
    skos:notation "1.5" ;
    skos:definition """Income and consumption - covers statistics on household income and expenditures from household viewpoint (all types of income and expenditure), including topics like distribution of incomes, in-kind income, income transfers received and paid, income- or expenditure-based measures of poverty, consumer protection, consumption patterns, consumer goods and durables, household wealth and debts.
Excludes 
- social protection schemes against various risks (1.6)
- tax schemes (2.5)
- poverty in a multidimensional sense (3.3.1) 
- living conditions (3.3.1)
- social inclusion/exclusion (3.3.1)"""@en;
	skos:definition """收入与消费 - 涵盖了从家庭的角度的家庭收入和支出（各类收入和支出）的统计数据，包括收入分配、实物收入、转移收入和支付、基于收入或支出的扶贫措施、消费者权益保护、消费模式、消费品和耐用消费品、家庭财富和债务等等主题。
不包括
- 对各种风险的社会保障计划（1.6）
- 税收计划（2.5）
- 在多维贫困感（3.3.1）
- 居住条件（3.3.1）
- 社会纳入/排除（3.3.1）"""@zh-CN;
	. 

sdmx-subject:1.6 a skos:Concept, sdmx:Concept, sdmx-subject:SubjectMatterDomain;
    skos:broader sdmx-subject:1;
    skos:prefLabel "Social protection"@en ;
	skos:prefLabel "社会保护"@zh-CN;
    skos:notation "1.6" ;
    skos:definition """Social protection - deals with statistics on measures to protect people against the risks of inadequate incomes associated with unemployment, ill health, invalidity, old age, parental responsibilities, or inadequate income following the loss of a spouse or parent, etc., includes statistics on pension beneficiaries, social security schemes, social protection expenditure, etc.
Excludes 
- insurance companies as economic actors (2.4.6)
- pension funds as actors in financial markets(2.4.6)"""@en;
	skos:definition """社会保护 - 处理措施，保障人民群众应对有关失业、生病、残疾、年老、父母的责任等收入不足的风险，或者失去配偶或父母后带来的收入不足等，包括养老金受益者、社会保障计划、社会保障开支等统计数据。
不包括
 - 作为经济参与者的保险公司（2.4.6）
 - 养老基金作为金融市场的参与者（2.4.6）"""@zh-CN;
	. 

sdmx-subject:1.7 a skos:Concept, sdmx:Concept, sdmx-subject:SubjectMatterDomain;
    skos:broader sdmx-subject:1;
    skos:prefLabel "Human settlements and housing"@en ;
	skos:prefLabel "人类定居和住房"@zh-CN;
    skos:notation "1.7" ;
    skos:definition """Human settlements and housing - covers statistical activities on housing, dwellings and human settlements
Excludes 
- rents (2.7)"""@en;
	skos:definition """人类定居和住房 - 覆盖了有关住房、住宅和定居的统计活动。
不包括
 - 租金（2.7）"""@zh-CN;
	. 

sdmx-subject:1.8 a skos:Concept, sdmx:Concept, sdmx-subject:SubjectMatterDomain;
    skos:broader sdmx-subject:1;
    skos:prefLabel "Justice and crime"@en ;
	skos:prefLabel "司法和犯罪"@zh-CN;
    skos:notation "1.8" ;
    skos:definition """Justice and crime - activities including crime, convictions, operation of criminal justice systems, justice, safety, victims, clear-up rates, prison population, illicit drug production, trafficking and use, etc."""@en;
	skos:definition """司法和犯罪 - 包括犯罪、定罪、刑事司法体系的运转、司法、安全、受害者、破案率、监狱人口、非法药物的生产、贩运和使用等活动。"""@zh-CN;
	. 

sdmx-subject:1.9 a skos:Concept, sdmx:Concept, sdmx-subject:SubjectMatterDomain;
    skos:broader sdmx-subject:1;
    skos:prefLabel "Culture"@en ;
	skos:prefLabel "文化"@zh-CN;
    skos:notation "1.9" ;
    skos:definition """Culture - statistics dealing with cultural activities in society, like theatre, cinemas, museums, libraries, mass media, book production, sports, etc., including expenditure and financing of culture."""@en;
	skos:definition """文化 - 处理社会文化活动的统计，如剧院、电影院、博物馆、图书馆、大众传媒、图书制作、体育等，包括文化的支出和融资。"""@zh-CN;
	. 

sdmx-subject:1.10 a skos:Concept, sdmx:Concept, sdmx-subject:SubjectMatterDomain;
    skos:broader sdmx-subject:1;
    skos:prefLabel "Political and other community activities"@en ;
	skos:prefLabel "政治和其他社会活动"@zh-CN;
    skos:notation "1.10" ;
    skos:definition """Political and other community activities - statistics on voting turnout, participation in political and other community activities, trade union membership, social dialogue, civil society, social capital, etc."""@en;
	skos:definition """政治和其他社会活动 - 有关政治和其他社会活动的投票率、参与、工会会员、社会对话、公民社会、社会资本等。"""@zh-CN;
	. 

sdmx-subject:1.11 a skos:Concept, sdmx:Concept, sdmx-subject:SubjectMatterDomain;
    skos:broader sdmx-subject:1;
    skos:prefLabel "Time use"@en ;
	skos:prefLabel "使用时间"@zh-CN;
    skos:notation "1.11" ;
    skos:definition """"""@en;
	skos:definition """。"""@zh-CN;
	. 

sdmx-subject:2 a skos:Concept, sdmx:Concept, sdmx-subject:SubjectMatterDomain;
    skos:topConceptOf sdmx-subject:subjectMatterDomain;
    skos:prefLabel "Economic statistics"@en ;
	skos:prefLabel "经济统计"@zh-CN;
    skos:notation "2" ;
    skos:definition """"""@en;
	skos:definition """。"""@zh-CN;
	. 
sdmx-subject:subjectMatterDomain skos:hasTopConcept sdmx-subject:2 .

sdmx-subject:2.1 a skos:Concept, sdmx:Concept, sdmx-subject:SubjectMatterDomain;
    skos:broader sdmx-subject:2;
    skos:prefLabel "Macroeconomic statistics"@en ;
	skos:prefLabel "宏观经济统计"@zh-CN;
    skos:notation "2.1" ;
    skos:definition """Macroeconomic statistics - all activities that are dealing with economy wide statistics at macro level that go beyond, or are different from National Accounts, whether annual, quarterly or monthly. Examples are macroeconomic databases that combine national accounts and other macroeconomic indicators like Main Economic Indicators (OECD), Principal European Economic Indicators (Eurostat), etc. ; business tendency and consumer opinion surveys, economic growth, stability and structural adjustment, cyclical indicators, statistics for business cycle analysis.
Excludes: 
- methodology and frameworks of national accounts (2.2.)
- collection and dissemination of national accounts and productivity data not linked to other macroeconomic statistics (2.2)"""@en;
	skos:definition """宏观经济统计 - 在宏观层面上处理广泛的经济统计的所有活动，超越或不同于年度、季度或月度国民经济核算。例如结合了国民经济核算和其他宏观经济指标的宏观经济数据库，如主要经济指标（OECD），欧洲主要经济指标（欧盟统计局）等；业务趋势和消费者意见调查，经济增长，稳定和结构调整，周期性指标，商业周期分析的统计信息。
不包括：
 - 国民经济核算的方法和框架（2.2）
 - 不与其他宏观经济统计数据关联的国民经济核算和生产率数据的采集与编制"""@zh-CN;
	. 

sdmx-subject:2.2 a skos:Concept, sdmx:Concept, sdmx-subject:SubjectMatterDomain;
    skos:broader sdmx-subject:2;
    skos:prefLabel "Economic accounts"@en ;
	skos:prefLabel "经济核算"@zh-CN;
    skos:notation "2.2" ;
    skos:definition """Economic accounts - covers work on National Accounts in both current and constant prices, dealing with topics like implementation of the 1993 System National Accounts (1993 SNA), update of the 1993 SNA, European System of Accounts (ESA95), Gross Domestic Product (GDP), Gross National Income (GNI), non-observed and informal economy, measurement of capital, input-output tables, balance sheets, etc.
Excludes 
- agricultural economic accounts (in 2.4.1)
- tourism satellite accounts (in 2.4.5)
- detailed general government accounts (2.5)
- financial accounts(2.5)
- price statistics(2.7)
- environmental accounts (3.1)"""@en;
	skos:definition """经济核算 - 涵盖了当前价格和恒定价格的国民经济核算工作，处理了诸如实施1993年国民经济核算系统（1993年SNA）、1993年SNA更新、欧洲账户体系（ESA 95）、国内生产总值（GDP）、国民总收入（GNI）、观测和非正规的经济、资本计量、投入产出表、资产负债表等主题。
不包括
 - 农业经济核算（2.4.1）
 - 旅游附属核算（2.4.5）
 - 详细的一般政府核算（2.5）
 - 财务核算（2.5）
 - 物价统计（2.7）
 - 环境核算（3.1）"""@zh-CN;
	. 

sdmx-subject:2.3 a skos:Concept, sdmx:Concept, sdmx-subject:SubjectMatterDomain;
    skos:broader sdmx-subject:2;
    skos:prefLabel "Business statistics"@en ;
	skos:prefLabel "商业统计"@zh-CN;
    skos:notation "2.3" ;
    skos:definition """Business statistics - economy wide statistics on the activities of enterprises, covers work on economic statistics across different sectors (as opposed to 2.4 that deals with specific individual sectors), deals with topics like statistics on economic activities of enterprises, business demography, business investment, business services, demand for services, industrial performance, enterprises by size class, industrial production, commodities, structure of sales and services, outputs of the service industries, non-profit institutions.
Excludes:
- business tendency surveys (2.1)
- international trade (2.6)
- prices (2.7)
- labour cost (2.8)
- science and technology (2.9)
- ICT (3.3.3)
- activities of foreign affiliates and multinational companies (3.3.4)"""@en;
	skos:definition """商业统计 - 有关企业活动的经济范围的统计信息，涵盖了跨越不同部门的经济统计工作（相对于2.4涉及的具体的个别部门），涉及了诸如企业的经济活动的统计数据、商务人口、商业投资、商业服务、服务需求、产业表现、企业按规模分类、工业生产、商品、销售和服务结构、服务业输出、非营利性机构等主题。
不包括：
 - 商业趋势调查（2.1）
 - 国际贸易（2.6）
 - 价格（2.7）
 - 劳动力成本（2.8）
 - 科学和技术（2.9）
 - ICT（3.3.3）
 - 外国子公司和跨国公司的业务（3.3.4）"""@zh-CN;
	. 

sdmx-subject:2.4 a skos:Concept, sdmx:Concept, sdmx-subject:SubjectMatterDomain;
    skos:broader sdmx-subject:2;
    skos:prefLabel "Sectoral statistics"@en ;
	skos:prefLabel "行业统计"@zh-CN;
    skos:notation "2.4" ;
    skos:definition """Sectoral statistics - statistical activities dealing with one of the specific branches of industry or services mentioned at the three digit level of the classification.
Excludes: 
- education (1.3) 
- health (1.4)
- social security (1.6)
- culture (1.9)
- statistics covering the whole industrial sector (2.3)
- statistics covering the whole service or market service sector (2.3)
- distributive trade (2.3)
- government and public sector statistics (2.5)
- research and development (2.9) 
- telecommunication statistics (3.3.3)"""@en;
	skos:definition """行业统计 - 处理在第三级分类中提到的提到的行业或服务的特定分支之一的统计活动。
不包括：
 - 教育（1.3）
 - 健康（1.4）
 - 社会保障（1.6）
 - 文化（1.9）
 - 涵盖了整个工业行业的统计（2.3）
 - 涵盖了整个服务或市场服务行业的统计（2.3）
 - 批发零售业（2.3）
 - 政府和公共部门的统计（2.5）
 - 研究及开发（2.9）
 - 电信统计（3.3.3）"""@zh-CN;
	. 

sdmx-subject:2.4.1 a skos:Concept, sdmx:Concept, sdmx-subject:SubjectMatterDomain;
    skos:broader sdmx-subject:2.4;
    skos:prefLabel "Agriculture, forestry, fisheries"@en ;
	skos:prefLabel "农业、林业、渔业"@zh-CN;
    skos:notation "2.4.1" ;
    skos:definition """Agriculture, forestry, fisheries - includes all agriculture, forestry and fishery related statistics, e.g. agricultural monetary statistics (agricultural economic accounts), agricultural structures (farm structure), trade in agricultural products, agricultural labour input, crop and animal production, agricultural commodities, agro-industry statistics (including food production and safety), organic farming and organic food, government expenditure for agriculture, fishing and forestry, products source and use tables, forest and forest product statistics, forest resource assessment and forest fire, trade in forest products, fisheries.
Excludes 
- agricultural and similar prices (2.7)
- rural development (3.2)"""@en;
	skos:definition """农业、林业、渔业 - 包括所有与农业、林业和渔业相关的统计数据，比如农业金融统计数据（农业经济账）、农业结构（农场结构）、农产品贸易、农业的劳动投入、农作物和畜牧生产、农业商品、农产品加工业统计数据（包括食品生产和安全）、有机农业和有机食品、农业的政府开支、渔业和林业产品的来源和使用表、森林和森林产品的统计、森林资源评估、森林火灾、林产品和渔业贸易。
不包括
 - 农业和相似的价格（2.7）
 - 农村发展（3.2）"""@zh-CN;
	. 

sdmx-subject:2.4.2 a skos:Concept, sdmx:Concept, sdmx-subject:SubjectMatterDomain;
    skos:broader sdmx-subject:2.4;
    skos:prefLabel "Energy"@en ;
	skos:prefLabel "能源"@zh-CN;
    skos:notation "2.4.2" ;
    skos:definition """Energy - energy supply, energy use, energy balances, security of supply, energy markets, trade in energy, energy efficiency, renewable energy sources, government expenditure on energy.
Excludes
- energy prices (2.7)"""@en;
	skos:definition """能源 - 能源供应、能源利用、能源平衡、供应安全、能源市场、能源交易、能源效率、可再生能源、在能源上的政府支出。
不包括
 - 能源价格（2.7）"""@zh-CN;
	. 

sdmx-subject:2.4.3 a skos:Concept, sdmx:Concept, sdmx-subject:SubjectMatterDomain;
    skos:broader sdmx-subject:2.4;
    skos:prefLabel "Mining, manufacturing, construction"@en ;
	skos:prefLabel "矿业、制造业、建筑业"@zh-CN;
    skos:notation "2.4.3" ;
    skos:definition """Mining, manufacturing, construction - statistics on specific industrial activities, e.g. steel, shipbuilding, and on construction, trade in specific products related to mining, manufacturing and construction.
Excludes
- prices of manufactured products (2.7)
- construction prices (2.7)"""@en;
	skos:definition """矿业、制造业、建筑业 - 特定工业活动统计，例如钢铁、造船、建筑，与采矿业、制造业和建筑相关的特定产品的贸易。
不包括
 - 制造业产品价格（2.7）
 - 建造价格（2.7）"""@zh-CN;
	. 

sdmx-subject:2.4.4 a skos:Concept, sdmx:Concept, sdmx-subject:SubjectMatterDomain;
    skos:broader sdmx-subject:2.4;
    skos:prefLabel "Transport"@en ;
	skos:prefLabel "运输"@zh-CN;
    skos:notation "2.4.4" ;
    skos:definition """Transport - covers statistics on all modes of transport (air, rail, road, inland waterways, sea), includes topics like transport infrastructure, equipment, traffic flows, personal mobility, safety, energy consumption, transport enterprises, passengers and freight transport, transport sector trends, road traffic accidents.
Excludes
- transport prices (2.7)"""@en;
	skos:definition """运输 - 涵盖了所有运输模式（空运，铁路，公路，内河航道，海）的统计，包括诸如交通基础设施、设备、交通流量、个人移动性、安全性、能耗、运输企业、乘客和货物运输、运输行业的发展趋势、道路交通事故等等方面的主题。
不包括
 - 运输价格（2.7）"""@zh-CN;
	. 

sdmx-subject:2.4.5 a skos:Concept, sdmx:Concept, sdmx-subject:SubjectMatterDomain;
    skos:broader sdmx-subject:2.4;
    skos:prefLabel "Tourism"@en ;
	skos:prefLabel "旅游"@zh-CN;
    skos:notation "2.4.5" ;
    skos:definition """Tourism - covers statistics regarding visitor activity (such as arrivals/departures, overnight stays, expenditures, purpose of the visit, etc.) associated to different forms of tourism (inbound, domestic and outbound), tourism industries activity and infrastructure, employment and tourism satellite accounts. 
Excludes
- prices for tourist services (2.7)
- environmental impacts (3.1)"""@en;
	skos:definition """旅游 - 涵盖了有关的游客活动（如抵港/离港航班，过夜，支出，访问目的等）的统计，这些活动都和不同形式的旅游（入境，国内和出境）、旅游行业活动和基础设施、就业和旅游有关联。
不包括
 - 旅游服务的价格（2.7）
 - 对环境的影响（3.1）"""@zh-CN;
	. 

sdmx-subject:2.4.6 a skos:Concept, sdmx:Concept, sdmx-subject:SubjectMatterDomain;
    skos:broader sdmx-subject:2.4;
    skos:prefLabel "Banking, insurance, financial statistics"@en ;
	skos:prefLabel "银行、保险、金融统计数据"@zh-CN;
    skos:notation "2.4.6" ;
    skos:definition """Banking, insurance, financial statistics - money, banking and financial market statistics, including financial accounts, money supply, interest rates, exchange rates, stock market indicators, securities, bank profitability, private sector insurance and pension fund statistics, Financial Soundness Indicators. 
Excludes 
- beneficiaries of private pension funds (1.6) 
- financing of state pension and of other state social security schemes (2.5)"""@en;
	skos:definition """银行、保险、金融统计数据 - 货币，银行和金融市场的统计数据，包括财务账目，货币供应量，利率，汇率，股市的指标，证券，银行盈利能力，私营行业的保险和养老保险基金的统计，金融稳健指标。
不包括
 - 私人养老基金的受益者（1.6）
 - 国家养老金和其他国家社会保障计划的融资（2.5）"""@zh-CN;
	. 

sdmx-subject:2.5 a skos:Concept, sdmx:Concept, sdmx-subject:SubjectMatterDomain;
    skos:broader sdmx-subject:2;
    skos:prefLabel "Government finance, fiscal and public sector statistics"@en ;
	skos:prefLabel "政府财政、财政和公共部门统计数据"@zh-CN;
    skos:notation "2.5" ;
    skos:definition """Government finance, fiscal and public sector statistics - all statistics related to the government sector, including debt and deficit, revenue and expenditure, accounts of the government sector, central government, tax rates and revenues, tax and benefit systems, financing of state pension and other state social security schemes, public sector employment.
Excludes 
- government expenditure in specific areas, like health (1.4), education (1.3), research and development (2.9), etc."""@en;
	skos:definition """政府财政、财政和公共部门统计数据 - 所有与政府部门相关的统计数据，包括债务和赤字、收入和支出、政府部门的帐目、中央政府、税率和收入、税收和福利制度、国家养老金和其他国家的社会保障计划的筹资、公共部门就业。
不包括
 - 在特定领域的政府开支，如医疗（1.4），教育（1.3），研究和开发（2.9）等"""@zh-CN;
	. 

sdmx-subject:2.6 a skos:Concept, sdmx:Concept, sdmx-subject:SubjectMatterDomain;
    skos:broader sdmx-subject:2;
    skos:prefLabel "International trade and balance of payments"@en ;
	skos:prefLabel "国际贸易和国际收支"@zh-CN;
    skos:notation "2.6" ;
    skos:definition """International trade and balance of payments - deals with statistics on all cross-border transactions recorded in the balance of payments, includes topics like trade in goods and services, external positions and debt, foreign direct investment, foreign affiliated trade, tariffs, market access, foreign aid, development assistance, resource flows to developing countries.
Excludes: 
- trade in specific commodities/services mentioned in 2.4.1 to 2.4.5
- multinational companies and activities of foreign affiliates (3.3.4)"""@en;
	skos:definition """国际贸易和国际收支 - 处理所有在国际收支平衡表中有关跨境交易记录的统计数据，包括商品和服务贸易、外商直接投资、外国附属贸易、关税、市场准入、对外援助、发展援助、流向发展中国家的资源等方面的主题。
不包括：
 - 在2.4.1 到 2.4.5 中提到的特定商品/服务的贸易
 - 跨国公司和外国附属公司的活动（3.3.4）"""@zh-CN;
	. 

sdmx-subject:2.7 a skos:Concept, sdmx:Concept, sdmx-subject:SubjectMatterDomain;
    skos:broader sdmx-subject:2;
    skos:prefLabel "Prices"@en ;
	skos:prefLabel "价格"@zh-CN;
    skos:notation "2.7" ;
    skos:definition """Prices - covers any statistical activity dealing with prices, including Purchasing Power Parities (PPPs) and international comparisons of GDP, covers topics like Consumer Price Indices (CPI), inflation, Producer Price Indices (PPI), price indexes for specific products and services (e.g. Information and Communication Technology products). 
Excludes 
- interest rates (2.4.6)
- wages (2.8)"""@en;
	skos:definition """价格 - 涵盖任何处理价格的统计活动，包括购买力平价（PPPs）和国内生产总值（GDP）的国际比较，涵盖了消费物价指数（CPI）、通货膨胀、生产者价格指数（PPI）、特定产品和服务的价格指数（例如，信息和通信技术产品）等主题。
不包括
 - 利率（2.4.6）
 - 薪酬（2.8）"""@zh-CN;
	. 

sdmx-subject:2.8 a skos:Concept, sdmx:Concept, sdmx-subject:SubjectMatterDomain;
    skos:broader sdmx-subject:2;
    skos:prefLabel "Labor cost"@en ;
	skos:prefLabel "劳动力成本"@zh-CN;
    skos:notation "2.8" ;
    skos:definition """Labour cost - statistics activities on labour cost, earning and wages, both for structural and short-term statistics. 
Excludes
- wages as part of total income of private households (1.5)"""@en;
	skos:definition """劳动力成本 - 有关劳动力成本的统计活动，收入和薪酬，无论结构性的还是短期的统计数据。
不包括
 - 作为私人家庭总收入的一部分的薪酬（1.5）"""@zh-CN;
	. 

sdmx-subject:2.9 a skos:Concept, sdmx:Concept, sdmx-subject:SubjectMatterDomain;
    skos:broader sdmx-subject:2;
    skos:prefLabel "Science, technology and innovation"@en ;
	skos:prefLabel "科学、技术与创新"@zh-CN;
    skos:notation "2.9" ;
    skos:definition """Science, technology and innovation - includes Research and Development (R&D), innovation, patents, human resources (in science, technology and innovation), high tech industries and knowledge based services, biotechnology, financing of R&D and innovation. 
Excludes: 
- information and communication technologies (ICTs) (3.3.3)"""@en;
	skos:definition """科学、技术与创新 - 包括研究开发（R&D），创新，专利，人力资源（在科学、技术和创新方面的），高科技产业和以知识为基础的服务，生物技术，研发和创新的融资。
不包括：
 - 信息和通信技术（ICT）（3.3.3）"""@zh-CN;
	. 

sdmx-subject:3 a skos:Concept, sdmx:Concept, sdmx-subject:SubjectMatterDomain;
    skos:topConceptOf sdmx-subject:subjectMatterDomain;
    skos:prefLabel "Environment and multi-domain statistics"@en ;
	skos:prefLabel "环境和多领域统计数据"@zh-CN;
    skos:notation "3" ;
    skos:definition """"""@en;
	skos:definition """。"""@zh-CN;
	. 
sdmx-subject:subjectMatterDomain skos:hasTopConcept sdmx-subject:3 .

sdmx-subject:3.1 a skos:Concept, sdmx:Concept, sdmx-subject:SubjectMatterDomain;
    skos:broader sdmx-subject:3;
    skos:prefLabel "Environment"@en ;
	skos:prefLabel "环境"@zh-CN;
    skos:notation "3.1" ;
    skos:definition """Environment - includes topics like climate, climate change, biodiversity, environment and health, natural resources, soil, water, air, landscape, waste, environmental expenditure, expenditure for the protection of the environment, environmental accounts, agri-environmental indicators, environmental pressure, environmental impact of industry, transport, energy etc., environmental monitoring, material flow analysis, environmental decoupling indicators, pollution, ecosystems, land use and cover, environmental protection, nationally protected areas.
Excludes
- environment as part of sustainable development (3.3.6)"""@en;
	skos:definition """环境 - 包括气候，气候变化，生物多样性，环境与健康，自然资源，土壤，水，空气，景观，浪费，环境支出，环境保护支出，环境核算，农业环境指标，环境压力，工业对环境的影响，交通运输，能源等，环境监测，物质流分析，环境脱钩指标，污染，生态系统，土地利用和覆盖，环保，国家重点保护的区域等主题。
不包括
 - 作为可持续发展的一部分的环境（3.3.6）"""@zh-CN;
	. 

sdmx-subject:3.2 a skos:Concept, sdmx:Concept, sdmx-subject:SubjectMatterDomain;
    skos:broader sdmx-subject:3;
    skos:prefLabel "Regional and small area statistics"@en ;
	skos:prefLabel "区域和小地区统计"@zh-CN;
    skos:notation "3.2" ;
    skos:definition """Regional and small area statistics - activities dealing with regional statistics and statistics referring to sub-national areas or areas based on administrative units, urban and rural statistics, rural development, regional accounts, regional typologies, and regional disparities."""@en;
	skos:definition """区域和小地区统计 - 处理区域统计数据和涉及国家以下一级地区或行政单位的区域的统计数据的活动，如城市和农村统计，农村发展，区域帐户，区域类型学和地区差距等。"""@zh-CN;
	. 

sdmx-subject:3.3 a skos:Concept, sdmx:Concept, sdmx-subject:SubjectMatterDomain;
    skos:broader sdmx-subject:3;
    skos:prefLabel "Multi-domain statistics and indicators"@en ;
	skos:prefLabel "多领域的统计数据和指标"@zh-CN;
    skos:notation "3.3" ;
    skos:definition """Multi-domain statistics and indicators - deals with conceptual or data work based on a specific thematic approach to outputs that cut across several economic, social or environmental subject areas; the two-digit-level of the classification covers activities dealing with such type of issues that are not explicitly mentioned at the three-digit level.
Excludes: 
- multi-domain statistics based on a regional approach (3.2)
- yearbook type of compendia or similar products by international organisations not following a specific thematic approach (3.4)"""@en;
	skos:definition """多领域的统计数据和指标 - 处理基于特定主题性方法的概念或数据，输出跨越了几个经济、社会和环境的学科领域，两位数水平的分类涵盖了处理这种类型问题的活动，这里没有明确提及三位数的水平。
不包括：
 - 基于区域办法的多领域统计（3.2）
 - 经由国际组织的、没有一个特定的主题性方法的年报类型纲要或类似产品（3.4）"""@zh-CN;
	. 

sdmx-subject:3.3.1 a skos:Concept, sdmx:Concept, sdmx-subject:SubjectMatterDomain;
    skos:broader sdmx-subject:3.3;
    skos:prefLabel "Living conditions, poverty, and cross-cutting social issues"@en ;
	skos:prefLabel "生活条件、贫困和跨领域的社会问题"@zh-CN;
    skos:notation "3.3.1" ;
    skos:definition """Living conditions, poverty and cross-cutting social issues - includes work on multidimensional methods to measure poverty, living conditions in the broad sense, social inclusion/exclusion, social indicators, and social situation.
Excludes:
- purely monetary approach to poverty (1.5)
Excludes: 
- multi-domain statistics based on a regional approach (3.2)
- yearbook type of compendia or similar products by international organisations not following a specific thematic approach (3.4)"""@en;
	skos:definition """生活条件、贫困和跨领域的社会问题 - 包括衡量贫困的多层面方法，广泛意义上的生活条件，社会包容/排斥，社会指标和社会状况。
不包括：
 - 贫困的纯金融方法（1.5）
不包括：
 - 基于区域办法的多领域统计（3.2）
 - 经由国际组织的、没有一个特定的主题性方法的年报类型纲要或类似产品（3.4）"""@zh-CN;
	. 

sdmx-subject:3.3.2 a skos:Concept, sdmx:Concept, sdmx-subject:SubjectMatterDomain;
    skos:broader sdmx-subject:3.3;
    skos:prefLabel "Gender and special population groups"@en ;
	skos:prefLabel "性别和特殊群体"@zh-CN;
    skos:notation "3.3.2" ;
    skos:definition """Gender and special population groups - their living conditions and role in the society: comparisons men/women and situation of special population groups like children, youth, women, elderly, disabled, minority groups, etc."""@en;
	skos:definition """性别和特殊群体 - 他们的生活条件和在社会中的角色；男/女比较和特殊群体的情况，如儿童，青少年，妇女，老年人，残疾人，少数群体等。"""@zh-CN;
	. 

sdmx-subject:3.3.3 a skos:Concept, sdmx:Concept, sdmx-subject:SubjectMatterDomain;
    skos:broader sdmx-subject:3.3;
    skos:prefLabel "Information society"@en ;
	skos:prefLabel "信息社会"@zh-CN;
    skos:notation "3.3.3" ;
    skos:definition """Information society - statistics allowing to assess the use and impact of information and communication technologies on society, includes access and use of ICTs (including Internet), ICT expenditure and investment, ICT infrastructure, telecommunication networks, electronic communications, e-government, electronic commerce, e-learning, broadband penetration, ICT services, communication tariffs, network infrastructure, revenues, expenses and investment of operators, Internet indicators, trade in telecommunications equipment."""@en;
	skos:definition """信息社会 - 统计数据允许评估信息和通信技术的使用和对社会的影响，包括信息和通信技术（包括互联网）的获取和使用，信息和通信技术的支出和投资，信息和通信技术基础设施，电信网络，电子通信，电子政务，电子商务，电子学习，宽带普及率，信息和通信技术服务，通信运价，网络基础设施，运营商的收入、开支和投资，互联网指标，电信设备贸易等。"""@zh-CN;
	. 

sdmx-subject:3.3.4 a skos:Concept, sdmx:Concept, sdmx-subject:SubjectMatterDomain;
    skos:broader sdmx-subject:3.3;
    skos:prefLabel "Globalisation"@en ;
	skos:prefLabel "全球化"@zh-CN;
    skos:notation "3.3.4" ;
    skos:definition """Globalisation - deals with measuring the economic activities of multinational companies, as well as with attempts to measure globalisation through a variety of components from other subject areas."""@en;
	skos:definition """全球化 - 衡量跨国公司的经济活动，以及通过来自其他学科领域的各种组件来尝试衡量全球化。"""@zh-CN;
	. 

sdmx-subject:3.3.5 a skos:Concept, sdmx:Concept, sdmx-subject:SubjectMatterDomain;
    skos:broader sdmx-subject:3.3;
    skos:prefLabel "Indicators related to the Millennium Development Goals"@en ;
	skos:prefLabel "有关千年发展目标的指标"@zh-CN;
    skos:notation "3.3.5" ;
    skos:definition """Indicators related to the Millennium Development Goals - work on sets of indicators to monitor the achievement of the Millennium Development Goals agreed upon at the UN Millennium Summit."""@en;
	skos:definition """有关千年发展目标的指标 - 有关一组指标的工作，以监测在联合国千年首脑会议上商定的千年发展目标的实现。"""@zh-CN;
	. 

sdmx-subject:3.3.6 a skos:Concept, sdmx:Concept, sdmx-subject:SubjectMatterDomain;
    skos:broader sdmx-subject:3.3;
    skos:prefLabel "Sustainable development"@en ;
	skos:prefLabel "可持续发展"@zh-CN;
    skos:notation "3.3.6" ;
    skos:definition """Sustainable development - work on indicators and frameworks to monitor the economic, social and environmental dimensions of sustainable development."""@en;
	skos:definition """可持续发展 - 有关指标和框架的工作，以监测可持续发展的经济、社会和环境等方面。"""@zh-CN;
	. 

sdmx-subject:3.3.7 a skos:Concept, sdmx:Concept, sdmx-subject:SubjectMatterDomain;
    skos:broader sdmx-subject:3.3;
    skos:prefLabel "Entrepreneurship"@en ;
	skos:prefLabel "创业"@zh-CN;
    skos:notation "3.3.7" ;
    skos:definition """Entrepreneurship - the measurement of the determinants, performance and impact of entrepreneurial activities of people and organisations."""@en;
	skos:definition """创业 - 有关个人和组织的创业活动的决定因素、性能和影响的测量。"""@zh-CN;
	. 

sdmx-subject:3.4 a skos:Concept, sdmx:Concept, sdmx-subject:SubjectMatterDomain;
    skos:broader sdmx-subject:3;
    skos:prefLabel "Yearbooks and similar compendia"@en ;
	skos:prefLabel "年报和同类简编"@zh-CN;
    skos:notation "3.4" ;
    skos:definition """Yearbooks and similar compendia - multi-domain statistical publications, databases and other data products without specific thematic or issue-oriented focus.
Excludes:
- Multi-domain statistical products based on specific thematic approaches, like sustainable development, MDGs etc. (under 3.3.1 to 3.3.5)"""@en;
	skos:definition """年报和同类简编 - 多领域统计数据出版物，数据库和其他数据产品，无需特定的主题或议题为导向的焦点。
不包括：
 - 基于特定主题性的方法的多领域的统计产品，如可持续发展，千年发展目标等（根据3.3.1至3.3.5）"""@zh-CN;
	. 

