@prefix rdf:            <http://www.w3.org/1999/02/22-rdf-syntax-ns#> .
@prefix rdfs:           <http://www.w3.org/2000/01/rdf-schema#> .
@prefix owl:            <http://www.w3.org/2002/07/owl#> .
@prefix xsd:            <http://www.w3.org/2001/XMLSchema#> .
@prefix skos:           <http://www.w3.org/2004/02/skos/core#> .
@prefix foaf:           <http://xmlns.com/foaf/0.1/> .
@prefix sdmx:           <http://purl.org/linked-data/sdmx#> .
@prefix dcterms:        <http://dublincore.org/documents/dcmi-terms/>.
@prefix qb:             <http://purl.org/linked-data/cube#> .
@prefix sdmx-concept:    <http://purl.org/linked-data/sdmx/2009/concept#> .

<http://purl.org/linked-data/sdmx>
    a owl:Ontology;
    owl:versionInfo "0.3";
    rdfs:label "SDMX-RDF vocabulary";
	rdfs:label "SDMX-RDF词汇集"@zh-CN;
    rdfs:comment "This vocabulary extends the data cube vocabulary to support publication of statistical data in RDF, using an information model based on SDMX";
	rdfs:comment "这个词汇集试用了基于SDMX的信息模型，扩展了数据立方体（data cube）词汇集，支持以RDF格式发布统计数据。"@zh-CN;
    dcterms:created "2010-02-05"^^xsd:date;
    dcterms:modified "2010-07-22"^^xsd:date;
    dcterms:title "Vocabulary for publishing SDMX statistical data in RDF"@en;
	dcterms:title "使用RDF发布SDMX统计数据的词汇集"@zh-CN;;
    dcterms:source <http://sdmx.org>;
    dcterms:references <http://sdmx.org/?page_id=16#package>;
    dcterms:contributor [foaf:mbox "richard@cyganiak.de"],
                        [foaf:mbox "jeni@jenitennison.com"],
                        [foaf:mbox "arofan.gregory@earthlink.net"],
                        [foaf:mbox "ian@epimorphics.com"],
                        [foaf:mbox "dave@epimorphics.com"];
    .
  
# --- Note ---------------------------

# In the revised structure, as developed at ODaF2010, the core representation
# of multidimensional data is covered by a general purpose "data cube" vocabulary.

# This SDMX-RDF vocabulary is now an extension to the Data Cube core to cover
# notions specific to aggregate statistical information as modelled in SDMX.

# The current version just covers the representation of Concept Roles.
# Future work will develop the SDMX vocabulary in more detail, based upon 
# the earlier SDMX-RDF draft.

# --- DataStructureDefinitions ---------------------------

sdmx:DataStructureDefinition a rdfs:Class, owl:Class;
    rdfs:label "Data Structure Definition"@en;
	rdfs:label "数据结构定义"@zh-CN;
    rdfs:comment "A specialization of qb:DataStructureDefinition which additional constraints: if there are multiple measures then a MeasureDimensionProperty must be included in the DSD"@en;
	rdfs:comment "表示qb:DataStructureDefinition的一个特化，并附加了一些额外的限制：如果存在多个测量，那么DSD中必须包含一个MeasureDimensionProperty。"@zh-CN;
    rdfs:subClassOf qb:DataStructureDefinition ;
    .
    
# --- Concepts ---------------------------
            
sdmx:CodeList a rdfs:Class, owl:Class;
    rdfs:label "Concept scheme"@en;
	rdfs:label "概念体系"@zh-CN;
    rdfs:subClassOf skos:ConceptScheme;
    .
    
sdmx:Concept a rdfs:Class, owl:Class;
    rdfs:label "concept"@en;
	rdfs:label "概念"@zh-CN;
    rdfs:subClassOf skos:Concept;
    rdfs:comment "Denotes an SDMX concept, used in the particular SDMX terminological sense, which is in principle narrower than skos:Concept";
	rdfs:comment "代表了一个SDMX概念，用于特定的SDMX术语意义上，原则上它比skos:Concept狭窄。"@zh-CN;
    .

# --- Concept Roles ---------------------------
            
sdmx:ConceptRole a rdfs:Class, owl:Class;
    rdfs:label "Concept role (abstract)"@en;
	rdfs:label "概念角色（抽象）"@zh-CN;
    rdfs:subClassOf sdmx:Concept;
    rdfs:comment "Abstract superclass of classes denoting statistical roles which be played by concepts"@en;
	rdfs:comment "表示由概念扮演统计角色的类的抽象超类。"@zh-CN;
    .

sdmx:FrequencyRole a rdfs:Class, owl:Class;
    rdfs:label "Frequency property"@en;
	rdfs:label "频率属性"@zh-CN;
    rdfs:comment "concept for a dimension or attribute that plays the role of frequency"@en;
	rdfs:comment "一个维度或特征的概念，扮演了频率角色"@zh-CN;
    rdfs:subClassOf sdmx:ConceptRole;
    .
sdmx:CountRole a rdfs:Class, owl:Class;
    rdfs:label "Count property"@en;
	rdfs:label "计数属性"@zh-CN;
    rdfs:comment "concept for a dimension or attribute that plays the role of an identifier where the identifier is taken from a known system of counts (e.g. the Nth current dataset update for a given day)"@en;
	rdfs:comment "扮演标识角色的纬度或属性的概念，这个标识来自一个已知的计数系统（如在某天更新的第 n 个当前数据集）"@zh-CN;
    rdfs:subClassOf sdmx:ConceptRole;
    .
sdmx:EntityRole a rdfs:Class, owl:Class;
    rdfs:label "Entity property"@en;
	rdfs:label "实体属性"@zh-CN;
    rdfs:comment "concept for a dimension or attribute that plays the role of the DataAttribute subject to whom the data refers (e.g. the reporting agent for primary reporting, the country for secondary reporting)"@en;
	rdfs:comment "一个纬度或特征的概念，扮演DataAttribute主语的角色，数据涉及到了这个DataAttribute主语（如主要报表的报表代理，次要报表的国家）"@zh-CN;
    rdfs:subClassOf sdmx:ConceptRole;
    .
sdmx:TimeRole a rdfs:Class, owl:Class;
    rdfs:label "Time property"@en;
	rdfs:label "时间属性"@zh-CN;
    rdfs:comment "concept for a dimension that specifies the time of the observation of the primaryMeasure"@en;
	rdfs:comment "一个纬度概念，指定了primaryMeasure的观察时间"@zh-CN;
    rdfs:subClassOf sdmx:ConceptRole;
    .
sdmx:MeasureTypeRole a rdfs:Class, owl:Class;
    rdfs:label "Measure type property"@en;
	rdfs:label "测量类型属性"@zh-CN;
    rdfs:comment "concept for a dimension that plays the role of identifying a type of measure"@en;
	rdfs:comment "一个纬度概念，扮演了标识测量类型的角色"@zh-CN;
    rdfs:subClassOf sdmx:ConceptRole;
    .
sdmx:NonObsTimeRole a rdfs:Class, owl:Class;
    rdfs:label "Non-observation time property"@en;
	rdfs:label "非观察时间属性"@zh-CN;
    rdfs:comment "concept for a dimension or attribute that plays the role of a date/time identifier in the KeyFamily which is not related to the time of the observation"@en;
	rdfs:comment "一个纬度或特征的概念，扮演了在KeyFamily总的日期/时间标识符的角色，它与观察时间无关"@zh-CN;
    rdfs:subClassOf sdmx:ConceptRole;
    .
sdmx:IdentityRole a rdfs:Class, owl:Class;
    rdfs:label "Identity property"@en;
	rdfs:label "标识属性"@zh-CN;
    rdfs:comment "concept for a dimension or attribute that plays the role of an identifier which is taken from a known scheme of identifiers."@en;
	rdfs:comment "一个纬度或特征的概念，扮演了标识符的角色，这个标识符来自已知的标识符体系"@zh-CN;
    rdfs:subClassOf sdmx:ConceptRole;
    .
sdmx:PrimaryMeasureRole a rdfs:Class, owl:Class;
    rdfs:label "Primary measure property"@en;
	rdfs:label "主要测量属性"@zh-CN;
    rdfs:comment "concept for a measure that plays the role of the observation in a time series"@en;
	rdfs:comment "一个测量概念，扮演了在时间序列中的观察角色"@zh-CN;
    rdfs:subClassOf sdmx:ConceptRole;
    .
            
# --- Linking to the reusable generic concepts from qb ---------------------------

qb:measureType qb:concept sdmx:measureTypeConcept .

sdmx:measureTypeConcept a sdmx:MeasureTypeRole, sdmx:ConceptRole, skos:Concept;
    rdfs:label "measureType"@en;
	rdfs:label "测量类型"@zh-CN;
    rdfs:comment "The concept corresponding to the generic measure type dimension which indicates which measure is being denoted by the primary measure on an observation"@en;
	rdfs:comment "对应通用测量类型纬度的概念，表明在一次观察中由主要测量表示的测量"@zh-CN;
    .

# --- Support for round-tripping the primary measure ---------------------------
            
sdmx:primaryMeasure a rdf:Property, owl:ObjectProperty;
    rdfs:label "primary measure"@en;
	rdfs:label "主要测量"@zh-CN;
    rdfs:comment "Indicates an additional component used as the primary measure within the SDMX data. In the case of multi-measure data sets the RDF representation uses the specific measure rather than a subsuming overall measure. This property records the subsuming primary measure (typically sdmx-measure:obsValue) to enable round tripping of this information."@en; 
	rdfs:comment "表示作为一个在SDMX数据中用作主要测量的附加组件。在有多个测量数据的情况下。RDF表示使用具体测量，而不是一个归并整体测量。此属性记录了归并的主要测量（通常是sdmx-measure:obsValue）以支持信息回返。"@zh-CN;
    rdfs:domain sdmx:DataStructureDefinition;
    rdfs:range  qb:MeasureProperty ;
    .            