@prefix rdf:     <http://www.w3.org/1999/02/22-rdf-syntax-ns#> .
@prefix rdfs:    <http://www.w3.org/2000/01/rdf-schema#> .
@prefix owl:     <http://www.w3.org/2002/07/owl#> .
@prefix skos:    <http://www.w3.org/2004/02/skos/core#> .
@prefix foaf:    <http://xmlns.com/foaf/0.1/> .
@prefix scovo:   <http://purl.org/NET/scovo#> .
@prefix void:    <http://rdfs.org/ns/void#> .
@prefix vcard:   <http://www.w3.org/2006/vcard/ns#> .
@prefix sdmx:    <http://purl.org/linked-data/sdmx#> .
@prefix sdmx-concept:    <http://purl.org/linked-data/sdmx/2009/concept#> .
@prefix sdmx-dimension:  <http://purl.org/linked-data/sdmx/2009/dimension#> .
@prefix sdmx-attribute:  <http://purl.org/linked-data/sdmx/2009/attribute#> .
@prefix sdmx-measure:    <http://purl.org/linked-data/sdmx/2009/measure#> .
@prefix sdmx-metadata:   <http://purl.org/linked-data/sdmx/2009/metadata#> .
@prefix sdmx-code:       <http://purl.org/linked-data/sdmx/2009/code#> .
@prefix sdmx-subject:    <http://purl.org/linked-data/sdmx/2009/subject#> .
@prefix dcterms:         <http://purl.org/dc/terms/>.
@prefix qb:              <http://purl.org/linked-data/cube#> .

<http://purl.org/linked-data/sdmx/2009/code>
    a owl:Ontology;
    rdfs:label "The vocabulary about SDMX code."@en;
	rdfs:label "有关SDMX代码的词汇集"@zh-CN;
    rdfs:comment "These annotations is added by chuci.info."@en;
    rdfs:comment "这些本体声明标记由chuci.info添加。"@zh-CN .

# CL_CURRENCY
sdmx-code:currency a skos:ConceptScheme, sdmx:CodeList;
    skos:prefLabel "code list for Currency (CURRENCY) - codelist scheme"@en;
	skos:prefLabel "货币（CURRENCY）代码列表--代码列表体系"@zh-CN;
    rdfs:label "code list for Currency (CURRENCY) - codelist scheme"@en;
	rdfs:label ""@zh-CN;
    skos:notation "CL_CURRENCY";
    skos:note """This code list provides code values for currencies."""@en;
	skos:note """这个代码列表提供了有关货币的代码值。"""@zh-CN;
    skos:definition <http://sdmx.org/wp-content/uploads/2009/01/02_sdmx_cog_annex_2_cl_2009.pdf> ;
    rdfs:seeAlso sdmx-code:Currency .

sdmx-code:Currency a rdfs:Class, owl:Class;
    rdfs:subClassOf skos:Concept ;
    rdfs:label "code list for Currency (CURRENCY) - codelist class"@en;
	rdfs:label "货币（CURRENCY）代码列表--代码列表类"@zh-CN;
    rdfs:comment """This code list provides code values for currencies."""@en;
	rdfs:comment """这个代码列表提供了有关货币的代码值。"""@zh-CN;
    rdfs:seeAlso sdmx-code:currency .

# CL_AREA
sdmx-code:area a skos:ConceptScheme, sdmx:CodeList;
    skos:prefLabel "Code list for providing values to concepts such as 'Reference area' and/or 'Counterpart area' - codelist scheme"@en;
	skos:prefLabel "为如“参考区域”和/或“对应区域”的概念提供值的代码列表 -- 代码列表体系"@zh-CN;
    rdfs:label "Code list for providing values to concepts such as 'Reference area' and/or 'Counterpart area' - codelist scheme"@en;
	rdfs:label "为如“参考区域”和/或“对应区域”的概念提供值的代码列表 -- 代码列表体系"@zh-CN;
    skos:notation "CL_AREA";
    skos:note """: This code list provides code values for geographical areas, defined as areas included within the borders of a country, region, group of countries, etc."""@en;
    skos:note """这个代码列表为地理区域提供了代码值，这些区域被定义包含在一国境内，区域内，国家集团内。"""@zh-CN;
	skos:definition <http://sdmx.org/wp-content/uploads/2009/01/02_sdmx_cog_annex_2_cl_2009.pdf> ;
    rdfs:seeAlso sdmx-code:Area .

sdmx-code:Area a rdfs:Class, owl:Class;
    rdfs:subClassOf skos:Concept ;
    rdfs:label "Code list for providing values to concepts such as 'Reference area' and/or 'Counterpart area' - codelist class"@en;
	rdfs:label "为如“参考区域”和/或“对应区域”的概念提供值的代码列表 -- 代码列表类"@zh-CN;
    rdfs:comment """: This code list provides code values for geographical areas, defined as areas included within the borders of a country, region, group of countries, etc."""@en;
    rdfs:comment """这个代码列表为地理区域提供了代码值，这些区域被定义包含在一国境内，区域内，国家集团内。"""@zh-CN;
	rdfs:seeAlso sdmx-code:area .

# CL_DECIMALS
sdmx-code:decimals a skos:ConceptScheme, sdmx:CodeList;
    skos:prefLabel "Code list for Decimals (DECIMALS) - codelist scheme"@en;
	skos:prefLabel "小数（DECIMALS）的代码列表 - 代码列表体系"@zh-CN;
    rdfs:label "Code list for Decimals (DECIMALS) - codelist scheme"@en;
	rdfs:label "小数（DECIMALS）的代码列表 - 代码列表体系"@zh-CN;
    skos:notation "CL_DECIMALS";
    skos:note """It provides a list of values showing the number of decimal digits used in the data."""@en;
	skos:note """它提供了一个显示用于数据中的小数位数的数字的值列表。"""@zh-CN;
    skos:definition <http://sdmx.org/wp-content/uploads/2009/01/02_sdmx_cog_annex_2_cl_2009.pdf> ;
    rdfs:seeAlso sdmx-code:Decimals .

sdmx-code:Decimals a rdfs:Class, owl:Class;
    rdfs:subClassOf skos:Concept ;
    rdfs:label "Code list for Decimals (DECIMALS) - codelist class"@en;
	rdfs:label "小数（DECIMALS）的代码列表 - 代码列表类"@zh-CN;
    rdfs:comment """It provides a list of values showing the number of decimal digits used in the data."""@en;
	rdfs:comment """它提供了一个显示用于数据中的小数位数的数字的值列表。"""@zh-CN;
    rdfs:seeAlso sdmx-code:decimals .

<http://purl.org/linked-data/sdmx/2009/code#decimals-0> a skos:Concept, sdmx:Concept, sdmx-code:Decimals;
    skos:topConceptOf sdmx-code:decimals;
    skos:inScheme     sdmx-code:decimals;
    skos:prefLabel "Zero"@en ;
	skos:prefLabel "0"@zh-CN;
    skos:notation "0" ;
    . 
sdmx-code:decimals skos:hasTopConcept <http://purl.org/linked-data/sdmx/2009/code#decimals-0> .

<http://purl.org/linked-data/sdmx/2009/code#decimals-1> a skos:Concept, sdmx:Concept, sdmx-code:Decimals;
    skos:topConceptOf sdmx-code:decimals;
    skos:inScheme     sdmx-code:decimals;
    skos:prefLabel "One"@en ;
	skos:prefLabel "1"@zh-CN;
    skos:notation "1" ;
    . 
sdmx-code:decimals skos:hasTopConcept <http://purl.org/linked-data/sdmx/2009/code#decimals-1> .

<http://purl.org/linked-data/sdmx/2009/code#decimals-2> a skos:Concept, sdmx:Concept, sdmx-code:Decimals;
    skos:topConceptOf sdmx-code:decimals;
    skos:inScheme     sdmx-code:decimals;
    skos:prefLabel "Two"@en ;
	skos:prefLabel "2"@zh-CN;
    skos:notation "2" ;
    . 
sdmx-code:decimals skos:hasTopConcept <http://purl.org/linked-data/sdmx/2009/code#decimals-2> .

<http://purl.org/linked-data/sdmx/2009/code#decimals-3> a skos:Concept, sdmx:Concept, sdmx-code:Decimals;
    skos:topConceptOf sdmx-code:decimals;
    skos:inScheme     sdmx-code:decimals;
    skos:prefLabel "Three"@en ;
	skos:prefLabel "3"@zh-CN;
    skos:notation "3" ;
    . 
sdmx-code:decimals skos:hasTopConcept <http://purl.org/linked-data/sdmx/2009/code#decimals-3> .

<http://purl.org/linked-data/sdmx/2009/code#decimals-4> a skos:Concept, sdmx:Concept, sdmx-code:Decimals;
    skos:topConceptOf sdmx-code:decimals;
    skos:inScheme     sdmx-code:decimals;
    skos:prefLabel "Four"@en ;
	skos:prefLabel "4"@zh-CN;
    skos:notation "4" ;
    . 
sdmx-code:decimals skos:hasTopConcept <http://purl.org/linked-data/sdmx/2009/code#decimals-4> .

<http://purl.org/linked-data/sdmx/2009/code#decimals-5> a skos:Concept, sdmx:Concept, sdmx-code:Decimals;
    skos:topConceptOf sdmx-code:decimals;
    skos:inScheme     sdmx-code:decimals;
    skos:prefLabel "Five"@en ;
	skos:prefLabel "5"@zh-CN;
    skos:notation "5" ;
    . 
sdmx-code:decimals skos:hasTopConcept <http://purl.org/linked-data/sdmx/2009/code#decimals-5> .

<http://purl.org/linked-data/sdmx/2009/code#decimals-6> a skos:Concept, sdmx:Concept, sdmx-code:Decimals;
    skos:topConceptOf sdmx-code:decimals;
    skos:inScheme     sdmx-code:decimals;
    skos:prefLabel "Six"@en ;
	skos:prefLabel "6"@zh-CN;
    skos:notation "6" ;
    . 
sdmx-code:decimals skos:hasTopConcept <http://purl.org/linked-data/sdmx/2009/code#decimals-6> .

<http://purl.org/linked-data/sdmx/2009/code#decimals-7> a skos:Concept, sdmx:Concept, sdmx-code:Decimals;
    skos:topConceptOf sdmx-code:decimals;
    skos:inScheme     sdmx-code:decimals;
    skos:prefLabel "Seven"@en ;
	skos:prefLabel "7"@zh-CN;
    skos:notation "7" ;
    . 
sdmx-code:decimals skos:hasTopConcept <http://purl.org/linked-data/sdmx/2009/code#decimals-7> .

<http://purl.org/linked-data/sdmx/2009/code#decimals-8> a skos:Concept, sdmx:Concept, sdmx-code:Decimals;
    skos:topConceptOf sdmx-code:decimals;
    skos:inScheme     sdmx-code:decimals;
    skos:prefLabel "Eight"@en ;
	skos:prefLabel "8"@zh-CN;
    skos:notation "8" ;
    . 
sdmx-code:decimals skos:hasTopConcept <http://purl.org/linked-data/sdmx/2009/code#decimals-8> .

<http://purl.org/linked-data/sdmx/2009/code#decimals-9> a skos:Concept, sdmx:Concept, sdmx-code:Decimals;
    skos:topConceptOf sdmx-code:decimals;
    skos:inScheme     sdmx-code:decimals;
    skos:prefLabel "Nine"@en ;
	skos:prefLabel "9"@zh-CN;
    skos:notation "9" ;
    . 
sdmx-code:decimals skos:hasTopConcept <http://purl.org/linked-data/sdmx/2009/code#decimals-9> .

# CL_FREQ
sdmx-code:freq a skos:ConceptScheme, sdmx:CodeList;
    skos:prefLabel "Code list for Frequency (FREQ) - codelist scheme"@en;
	skos:prefLabel "频率（FREQ）的代码列表 -- 代码列表体系"@zh-CN;
    rdfs:label "Code list for Frequency (FREQ) - codelist scheme"@en;
	rdfs:label "频率（FREQ）的代码列表 -- 代码列表体系"@zh-CN;
    skos:notation "CL_FREQ";
    skos:note """It provides a list of values indicating the "frequency" of the data (e.g. monthly) and, thus, indirectly, also implying the type of "time reference" that could be used for identifying the data with respect time."""@en;
    skos:note """它提供了一组表示数据的频率的值（如，每月），因此，间接地，也意味着“时间基准”的类型，可用于识别带有时间的数据。"""@zh-CN;
	skos:definition <http://sdmx.org/wp-content/uploads/2009/01/02_sdmx_cog_annex_2_cl_2009.pdf> ;
    rdfs:seeAlso sdmx-code:Freq .

sdmx-code:Freq a rdfs:Class, owl:Class;
    rdfs:subClassOf skos:Concept ;
    rdfs:label "Code list for Frequency (FREQ) - codelist class"@en;
	rdfs:label "频率（FREQ）的代码列表 -- 代码列表类"@zh-CN;
    rdfs:comment """It provides a list of values indicating the "frequency" of the data (e.g. monthly) and, thus, indirectly, also implying the type of "time reference" that could be used for identifying the data with respect time."""@en;
    rdfs:comment """它提供了一组表示数据的频率的值（如，每月），因此，间接地，也意味着“时间基准”的类型，可用于识别带有时间的数据。"""@zh-CN;
	rdfs:seeAlso sdmx-code:freq .

<http://purl.org/linked-data/sdmx/2009/code#freq-A> a skos:Concept, sdmx:Concept, sdmx-code:Freq;
    skos:topConceptOf sdmx-code:freq;
    skos:inScheme     sdmx-code:freq;
    skos:prefLabel "Annual"@en ;
	skos:prefLabel "全年"@zh-CN;
    skos:notation "A" ;
    skos:definition """It is typically used for annual data. This can also serve cases of multi-annual data (data that appear once every two, three or, possibly, five years).  Descriptive information on the multiannual characteristics (e.g. frequency of the series in practice and other methodological information can be provided at the dataflow level, as long as these characteristics are applicable for the entire dataflow)."""@en ; 
    skos:definition """它通常用于年度数据。这也可以服务于多年度数据的情况（每两年、三年、或可能五年出现一次的数据）。多年期特性的描述信息（例如，实践中的系列和其他方法学信息的频率，可以在数据流的水平上提供，只要这些特征是适用于在整个数据流）。"""@zh-CN;
	. 
sdmx-code:freq skos:hasTopConcept <http://purl.org/linked-data/sdmx/2009/code#freq-A> .

<http://purl.org/linked-data/sdmx/2009/code#freq-B> a skos:Concept, sdmx:Concept, sdmx-code:Freq;
    skos:topConceptOf sdmx-code:freq;
    skos:inScheme     sdmx-code:freq;
    skos:prefLabel "Daily - business week"@en ;
	skos:prefLabel "每日 - 工作周"@zh-CN;
    skos:notation "B" ;
    skos:definition """Similar to "daily", however there are no observations for Saturday and Sunday (so, neither "missing values" nor "numeric values" should be provided for Saturday and Sunday). This treatment ("business") is one way to deal with such cases, but it is not the only option. Such a time series could alternatively be considered daily ("D"), thus, with missing values in the weekend."""@en ; 
    skos:definition """类似于“每日”然而没有关于周六和周日的观测（所以，不应为周六和周日提供“缺失值”或“数值”）。这种处理（“业务”）是处理这类问题的一种方式，但它不是唯一的选择。这样一个时间序列或者可以被认为是缺失了周末的值的每天（“D”）。"""@zh-CN;
	. 
sdmx-code:freq skos:hasTopConcept <http://purl.org/linked-data/sdmx/2009/code#freq-B> .

<http://purl.org/linked-data/sdmx/2009/code#freq-D> a skos:Concept, sdmx:Concept, sdmx-code:Freq;
    skos:topConceptOf sdmx-code:freq;
    skos:inScheme     sdmx-code:freq;
    skos:prefLabel "Daily"@en ;
	skos:prefLabel "每日"@zh-CN;
    skos:notation "D" ;
    . 
sdmx-code:freq skos:hasTopConcept <http://purl.org/linked-data/sdmx/2009/code#freq-D> .

<http://purl.org/linked-data/sdmx/2009/code#freq-M> a skos:Concept, sdmx:Concept, sdmx-code:Freq;
    skos:topConceptOf sdmx-code:freq;
    skos:inScheme     sdmx-code:freq;
    skos:prefLabel "Monthly"@en ;
	skos:prefLabel "每月"@zh-CN;
    skos:notation "M" ;
    . 
sdmx-code:freq skos:hasTopConcept <http://purl.org/linked-data/sdmx/2009/code#freq-M> .

<http://purl.org/linked-data/sdmx/2009/code#freq-N> a skos:Concept, sdmx:Concept, sdmx-code:Freq;
    skos:topConceptOf sdmx-code:freq;
    skos:inScheme     sdmx-code:freq;
    skos:prefLabel "Minutely"@en ;
	skos:prefLabel "每分钟"@zh-CN;
    skos:notation "N" ;
    skos:definition """While N denotes "minutely", usually, there may be no observations every minute (for several series the frequency is usually "irregular" within a day/days). And though observations may be sparse (not collected every minute), missing values do not need to be given for the minutes when no observations exist: in any case the time stamp determines when an observation is observed."""@en ; 
    skos:definition """虽然N表示“每分钟”，通常情况下，每分钟有可能没有观测（某几个系列的频率在一天之/几天内通常是“非正规”的）。此外，尽管观察可能是稀疏的（并不是每分钟都有收集数据），当没有观测存在时，不需要为分钟指定缺失值；在任何情况下，时间戳决定了一个观测值是否是观测的。"""@zh-CN;
	. 
sdmx-code:freq skos:hasTopConcept <http://purl.org/linked-data/sdmx/2009/code#freq-N> .

<http://purl.org/linked-data/sdmx/2009/code#freq-Q> a skos:Concept, sdmx:Concept, sdmx-code:Freq;
    skos:topConceptOf sdmx-code:freq;
    skos:inScheme     sdmx-code:freq;
    skos:prefLabel "Quarterly"@en ;
	skos:prefLabel "每季度"@zh-CN;
    skos:notation "Q" ;
    . 
sdmx-code:freq skos:hasTopConcept <http://purl.org/linked-data/sdmx/2009/code#freq-Q> .

<http://purl.org/linked-data/sdmx/2009/code#freq-S> a skos:Concept, sdmx:Concept, sdmx-code:Freq;
    skos:topConceptOf sdmx-code:freq;
    skos:inScheme     sdmx-code:freq;
    skos:prefLabel "Half Yearly, semester"@en ;
	skos:prefLabel "半年"@zh-CN;
    skos:notation "S" ;
    . 
sdmx-code:freq skos:hasTopConcept <http://purl.org/linked-data/sdmx/2009/code#freq-S> .

<http://purl.org/linked-data/sdmx/2009/code#freq-W> a skos:Concept, sdmx:Concept, sdmx-code:Freq;
    skos:topConceptOf sdmx-code:freq;
    skos:inScheme     sdmx-code:freq;
    skos:prefLabel "Weekly"@en ;
	skos:prefLabel "每周"@zh-CN;
    skos:notation "W" ;
    . 
sdmx-code:freq skos:hasTopConcept <http://purl.org/linked-data/sdmx/2009/code#freq-W> .

# CL_CONF_STATUS
sdmx-code:confStatus a skos:ConceptScheme, sdmx:CodeList;
    skos:prefLabel "code list for Confidentiality Status (CONF_STATUS) - codelist scheme"@en;
	skos:prefLabel "机密状态（CONF_STATUS）的代码列表 - 代码列表体系"@zh-CN;
    rdfs:label "code list for Confidentiality Status (CONF_STATUS) - codelist scheme"@en;
	rdfs:label "机密状态（CONF_STATUS）的代码列表 - 代码列表体系"@zh-CN;
    skos:notation "CL_CONF_STATUS";
    skos:note """this code list provides coded information about the sensitivity and confidentiality status of the data."""@en;
	skos:note """这个代码列表提供了有关数据的敏感性和机密状态的代码信息。"""@zh-CN;
    skos:definition <http://sdmx.org/wp-content/uploads/2009/01/02_sdmx_cog_annex_2_cl_2009.pdf> ;
    rdfs:seeAlso sdmx-code:ConfStatus .

sdmx-code:ConfStatus a rdfs:Class, owl:Class;
    rdfs:subClassOf skos:Concept ;
    rdfs:label "code list for Confidentiality Status (CONF_STATUS) - codelist class"@en;
	rdfs:label "机密状态（CONF_STATUS）的代码列表 - 代码列表类"@zh-CN;
    rdfs:comment """this code list provides coded information about the sensitivity and confidentiality status of the data."""@en;
	rdfs:comment """这个代码列表提供了有关数据的敏感性和机密状态的代码信息。"""@zh-CN;
    rdfs:seeAlso sdmx-code:confStatus .

<http://purl.org/linked-data/sdmx/2009/code#confStatus-C> a skos:Concept, sdmx:Concept, sdmx-code:ConfStatus;
    skos:topConceptOf sdmx-code:confStatus;
    skos:inScheme     sdmx-code:confStatus;
    skos:prefLabel "Confidential statistical information"@en ;
	skos:prefLabel "机密的统计信息"@zh-CN;
    skos:notation "C" ;
    skos:definition """Confidential statistical information (primary confidentiality) due to identifiable respondents.  Measures also should be taken to prevent not only direct access, but also indirect deduction or calculation by other users and parties, probably by considering and treating additional observations as "confidential" (secondary confidentiality management)."""@en ; 
    skos:definition """机密的统计信息（首要机密）是依赖于可识别的受访者。应采取措施，不仅防止直接访问，也防止其他用户和当事方的间接推论或计算，可能是通过考虑和处理作为“机密”（二级保密管理）的更多的观测。"""@zh-CN;
	. 
sdmx-code:confStatus skos:hasTopConcept <http://purl.org/linked-data/sdmx/2009/code#confStatus-C> .

<http://purl.org/linked-data/sdmx/2009/code#confStatus-D> a skos:Concept, sdmx:Concept, sdmx-code:ConfStatus;
    skos:topConceptOf sdmx-code:confStatus;
    skos:inScheme     sdmx-code:confStatus;
    skos:prefLabel "Secondary confidentiality set by the sender, not for publication"@en ;
	skos:prefLabel "发送方的二级机密设置，不用于出版"@zh-CN;
    skos:notation "D" ;
    skos:definition """Used by the sender of the data to flag (beyond the confidential statistical information) one or more additional observations of the dataset so that the receiver knows that he/she should suppress these observations in subsequent stages of processing (especially, dissemination) in order to prevent third parties to indirectly deduct (e.g. through accounting identities or other formulas) the observations that are genuinely flagged with "C"."""@en ; 
    skos:definition """由数据的发送者使用，对一个或多个附加的观测数据集进行标志（超出了机密的的统计信息），以使接收者知道，在后续处理阶段（尤其是，传播），他/她应该压制这些观察，以防止第三方间接扣除（例如通过会计恒等式或公式）真正以“C”标记的观测。"""@zh-CN;
	. 
sdmx-code:confStatus skos:hasTopConcept <http://purl.org/linked-data/sdmx/2009/code#confStatus-D> .

<http://purl.org/linked-data/sdmx/2009/code#confStatus-F> a skos:Concept, sdmx:Concept, sdmx-code:ConfStatus;
    skos:topConceptOf sdmx-code:confStatus;
    skos:inScheme     sdmx-code:confStatus;
    skos:prefLabel "Free"@en ;
	skos:prefLabel ""@zh-CN;
    skos:notation "F" ;
    skos:definition """It is used for observations for observations for which there are no special sensitivity considerations and which can be freely shared. Please note:
In some institutional environments the term "unclassified" is used in a sense that still denotes implied restrictions in the circulation of information. If this is the case, this organisation may probably consider that "free" (value F) is not the appropriate corresponding tag for this kind of "unclassified" category and it may be that "non-publishable / restricted" (value N) may be more appropriate.
The focus of this code is not to describe and anticipate all potential permissible uses (e.g. permission to re-disseminate). Thus, the use of "F" does not allow safe assumptions with respect to the permission to "re-disseminate" (freely or at a price) the received or accessed information (e.g. on web or paper), especially on a massive and regular basis (legal and copyright constraints may apply). Usually, source organisations provide information and guidance on re-dissemination issues, either on their websites or on their paper publications."""@en ; 
    skos:definition """它是用来观察没有特殊的敏感性考虑并且可以自由共享的观测。请注意：
在一些体制环境中，术语“未分类”是在一定意义上仍然用来表示信息流通的隐含限制。如果是这样的话，该组织可以考虑“自由”（F值）可能不是这种“机密”类别对应的标签，“未发布/受限制”（N值）可能更合适。
该代码的焦点不是描述和预测所有潜在的用途（例如允许重新传播）。因此，对于“再传播”（免费或收取一定费用）收到的或访问的信息（如网页或纸）方面的权限，使用“F”不会允许安全假设，尤其是在大规模和不变的成分上面（法律和版权方面的限制可能更适用）。通常情况下，源组织对于再传播的问题提供信息和指导，无论是在自己的网站或它们的纸质出版物上面。"""@zh-CN;
	. 
sdmx-code:confStatus skos:hasTopConcept <http://purl.org/linked-data/sdmx/2009/code#confStatus-F> .

<http://purl.org/linked-data/sdmx/2009/code#confStatus-N> a skos:Concept, sdmx:Concept, sdmx-code:ConfStatus;
    skos:topConceptOf sdmx-code:confStatus;
    skos:inScheme     sdmx-code:confStatus;
    skos:prefLabel "Not for publication, restricted for internal use only"@en ;
	skos:prefLabel "不供刊发，仅限内部使用"@zh-CN;
    skos:notation "N" ;
    skos:definition """Used to denote observations that are restricted for internal use only within organisations."""@en ; 
	skos:definition """用来表示仅限于在组织内部使用的观察。"""@zh-CN;
    . 
sdmx-code:confStatus skos:hasTopConcept <http://purl.org/linked-data/sdmx/2009/code#confStatus-N> .

<http://purl.org/linked-data/sdmx/2009/code#confStatus-S> a skos:Concept, sdmx:Concept, sdmx-code:ConfStatus;
    skos:topConceptOf sdmx-code:confStatus;
    skos:inScheme     sdmx-code:confStatus;
    skos:prefLabel "Secondary confidentiality set and managed by the receiver, not for publication"@en ;
	skos:prefLabel "二次机密设置和由接收方管理，不供刊发"@zh-CN;
    skos:notation "S" ;
    skos:definition """If senders do not manage the secondary confidentiality in their data and/or there are also other countries' data involved (with the intention to eventually compile a regional-wide aggregate that is going to be published), the value "S" is used by the receiver to flag additional suppressed observations (within sender's data and/or within the datasets of other senders) in subsequent stages of processing (especially, dissemination) in order to prevent third parties to indirectly deduct the observations that were genuinely flagged with "C" by the sender."""@en ; 
    skos:definition """如果发送者不在他们的数据中管理二级机密，且/或也有涉及其他国家的数据（有意向最终编制一份即将出版的区域范围内的聚合数据），“S”值用于在处理的后续阶段（尤其，传播），由接收者标记额外抑制的观察（在发送者的数据中和/或其他发送者的数据集内），以防止第三方间接扣除真正以“C”标记的观测。"""@zh-CN;
	. 
sdmx-code:confStatus skos:hasTopConcept <http://purl.org/linked-data/sdmx/2009/code#confStatus-S> .

# CL_OBS_STATUS
sdmx-code:obsStatus a skos:ConceptScheme, sdmx:CodeList;
    skos:prefLabel "Observation status - codelist scheme"@en;
	skos:prefLabel ""@zh-CN;
    rdfs:label "Observation status - codelist scheme"@en;
	rdfs:label "观察状态 - 代码列表体系"@zh-CN;
    skos:notation "CL_OBS_STATUS";
    skos:note """This code list provides coded information about the "status" of an observation (with respect events such as the ones reflected in the codes composing the code list)."""@en;
    skos:note """这个代码列表提供了有关“状态”的编码信息（如体现在由代码组成的代码列表那些对应的事件）。"""@zh-CN;
	skos:definition <http://sdmx.org/wp-content/uploads/2009/01/02_sdmx_cog_annex_2_cl_2009.pdf> ;
    rdfs:seeAlso sdmx-code:ObsStatus .

sdmx-code:ObsStatus a rdfs:Class, owl:Class;
    rdfs:subClassOf skos:Concept ;
    rdfs:label "Observation status - codelist class"@en;
	rdfs:label "观察状态 - 代码列表类"@zh-CN;
    rdfs:comment """This code list provides coded information about the "status" of an observation (with respect events such as the ones reflected in the codes composing the code list)."""@en;
    rdfs:comment """这个代码列表提供了有关“状态”的编码信息（如体现在由代码组成的代码列表那些对应的事件）。"""@zh-CN;
	rdfs:seeAlso sdmx-code:obsStatus .

<http://purl.org/linked-data/sdmx/2009/code#obsStatus-A> a skos:Concept, sdmx:Concept, sdmx-code:ObsStatus;
    skos:topConceptOf sdmx-code:obsStatus;
    skos:inScheme     sdmx-code:obsStatus;
    skos:prefLabel "Normal"@en ;
	skos:prefLabel "正常"@zh-CN;
    skos:notation "A" ;
    skos:definition """Normal is the default value (if no value is provided) and is used when no special coded qualification is assumed. Usually, in this case, it can be assumed that the source agency assigns sufficient confidence to the provided observation and/or the value is not expected to be dramatically revised."""@en ; 
    skos:definition """正常，是默认值（如果没有提供任何值），在没有特殊的编码资格时作为假设使用。一般，在这种情况下，可以假设源机构对所提供的观察和/或预期将不会大幅修改值，给予了足够的信心，。"""@zh-CN;
	. 
sdmx-code:obsStatus skos:hasTopConcept <http://purl.org/linked-data/sdmx/2009/code#obsStatus-A> .

<http://purl.org/linked-data/sdmx/2009/code#obsStatus-B> a skos:Concept, sdmx:Concept, sdmx-code:ObsStatus;
    skos:topConceptOf sdmx-code:obsStatus;
    skos:inScheme     sdmx-code:obsStatus;
    skos:prefLabel "Break"@en ;
	skos:prefLabel "改变"@zh-CN;
    skos:notation "B" ;
    skos:definition """Break observations are characterised as such when different content exist or a different methodology has been applied to this observation as compared with the preceding one (the one given for the previous period)."""@en ; 
    skos:definition """改变观察的特点是，当存在不同的内容时或者与前一个（前一段时间给出的）相比将不同的方法应用到这个观察时。"""@zh-CN;
	. 
sdmx-code:obsStatus skos:hasTopConcept <http://purl.org/linked-data/sdmx/2009/code#obsStatus-B> .

<http://purl.org/linked-data/sdmx/2009/code#obsStatus-E> a skos:Concept, sdmx:Concept, sdmx-code:ObsStatus;
    skos:topConceptOf sdmx-code:obsStatus;
    skos:inScheme     sdmx-code:obsStatus;
    skos:prefLabel "Estimated value"@en ;
	skos:prefLabel "估算值"@zh-CN;
    skos:notation "E" ;
    skos:definition """Observation obtained through an estimation methodology (e.g. to produce back-casts) or based on the use of a limited amount of data or ad hoc sampling and through additional calculations (e.g. to produce a value at an early stage of the production stage while not all data are available). It may also be used in case of experimental data (e.g. in the context of a pilot ahead of a full scale production process) or in case of data of (anticipated/assessed) low quality. If needed, additional (uncoded) information can be provided through (free text) "comments" at the observation level or at a higher level."""@en ; 
    skos:definition """通过估算方法（如produce back-casts）或使用一个有限数据量或临时采样，通过额外的计算（例如，在生产阶段的早期阶段当全部数据不可用时产生的一个值）得到的观察。这也可以用于实验数据的情况（例如，在全面投产流程之前的背景下的一项试验）或者（预期/评估）低质量的数据的情况。如果需要，可以在观察级别或在更高级别，通过（自由文本）“注释”提供额外的（未编码）信息。"""@zh-CN;
	. 
sdmx-code:obsStatus skos:hasTopConcept <http://purl.org/linked-data/sdmx/2009/code#obsStatus-E> .

<http://purl.org/linked-data/sdmx/2009/code#obsStatus-F> a skos:Concept, sdmx:Concept, sdmx-code:ObsStatus;
    skos:topConceptOf sdmx-code:obsStatus;
    skos:inScheme     sdmx-code:obsStatus;
    skos:prefLabel "Forecast value"@en ;
	skos:prefLabel "预测值"@zh-CN;
    skos:notation "F" ;
    . 
sdmx-code:obsStatus skos:hasTopConcept <http://purl.org/linked-data/sdmx/2009/code#obsStatus-F> .

<http://purl.org/linked-data/sdmx/2009/code#obsStatus-I> a skos:Concept, sdmx:Concept, sdmx-code:ObsStatus;
    skos:topConceptOf sdmx-code:obsStatus;
    skos:inScheme     sdmx-code:obsStatus;
    skos:prefLabel "Imputed value (CCSA definition)"@en ;
	skos:prefLabel "需移除的值（CCSA定义）"@zh-CN;
    skos:notation "I" ;
    skos:definition """Observation imputed by international organisations to replace or fill gaps in national data series, in line with the recommendations of the Committee for the Coordination of Statistical Activities (CCSA)."""@en ; 
    skos:definition """由国际组织在国家数据系列中，根据统计活动协调委员会（CCSA）的建议来替换或填补空白的观察。"""@zh-CN;
	. 
sdmx-code:obsStatus skos:hasTopConcept <http://purl.org/linked-data/sdmx/2009/code#obsStatus-I> .

<http://purl.org/linked-data/sdmx/2009/code#obsStatus-M> a skos:Concept, sdmx:Concept, sdmx-code:ObsStatus;
    skos:topConceptOf sdmx-code:obsStatus;
    skos:inScheme     sdmx-code:obsStatus;
    skos:prefLabel "Missing value"@en ;
	skos:prefLabel "缺失值"@zh-CN;
    skos:notation "M" ;
    skos:definition """Data can be missing due to various reasons:  data do not exist, are insignificant (or not collected because they are below a certain threshold), are unreliable, are not relevant for the period, or other reason not elsewhere specified."""@en ; 
    skos:definition """由于各方面的原因，数据时可以缺失的：数据不存在，是微不足道的（或因为他们低于某一阈值而未被收集），是不可靠的，在当期是不相关的，或者由于其他原因未列明。"""@zh-CN;
	. 
sdmx-code:obsStatus skos:hasTopConcept <http://purl.org/linked-data/sdmx/2009/code#obsStatus-M> .

<http://purl.org/linked-data/sdmx/2009/code#obsStatus-P> a skos:Concept, sdmx:Concept, sdmx-code:ObsStatus;
    skos:topConceptOf sdmx-code:obsStatus;
    skos:inScheme     sdmx-code:obsStatus;
    skos:prefLabel "Provisional value"@en ;
	skos:prefLabel "临时值"@zh-CN;
    skos:notation "P" ;
    skos:definition """An observation is characterised as "provisional" when the source agency - while it bases its calculations on its standard production methodology - considers that the data, almost certainly, are expected to be revised."""@en ; 
	skos:definition """这类观察的特点是“临时”的数据，当源机构--虽然它根据它的标准生成方法进行计算--认为数据几乎肯定是预计将要进行修订的时候。"""@zh-CN;
    . 
sdmx-code:obsStatus skos:hasTopConcept <http://purl.org/linked-data/sdmx/2009/code#obsStatus-P> .

<http://purl.org/linked-data/sdmx/2009/code#obsStatus-S> a skos:Concept, sdmx:Concept, sdmx-code:ObsStatus;
    skos:topConceptOf sdmx-code:obsStatus;
    skos:inScheme     sdmx-code:obsStatus;
    skos:prefLabel "Strike"@en ;
	skos:prefLabel "罢工"@zh-CN;
    skos:notation "S" ;
    skos:definition """A known strike that occurred in the corresponding period that may have affected the observation or caused a missing value."""@en ; 
	skos:definition """发生在相应期间的已知罢工，可能会影响观察或导致丢失值。"""@zh-CN;
    . 
sdmx-code:obsStatus skos:hasTopConcept <http://purl.org/linked-data/sdmx/2009/code#obsStatus-S> .

# CL_SEX
sdmx-code:sex a skos:ConceptScheme, sdmx:CodeList;
    skos:prefLabel "Code list for Sex (SEX) - codelist scheme"@en;
	skos:prefLabel ""@zh-CN;
    rdfs:label "Code list for Sex (SEX) - codelist scheme"@en;
	rdfs:label "性别（SEX）代码列表 - 代码列表体系"@zh-CN;
    skos:notation "CL_SEX";
    skos:note """This  code list provides the gender."""@en;
	skos:note """该代码列表提供了性别。"""@zh-CN;
    skos:definition <http://sdmx.org/wp-content/uploads/2009/01/02_sdmx_cog_annex_2_cl_2009.pdf> ;
    rdfs:seeAlso sdmx-code:Sex .

sdmx-code:Sex a rdfs:Class, owl:Class;
    rdfs:subClassOf skos:Concept ;
    rdfs:label "Code list for Sex (SEX) - codelist class"@en;
	rdfs:label "性别（SEX）代码列表 - 代码列表类"@zh-CN;
    rdfs:comment """This  code list provides the gender."""@en;
	rdfs:comment """该代码列表提供了性别。"""@zh-CN;
    rdfs:seeAlso sdmx-code:sex .

<http://purl.org/linked-data/sdmx/2009/code#sex-F> a skos:Concept, sdmx:Concept, sdmx-code:Sex;
    skos:topConceptOf sdmx-code:sex;
    skos:inScheme     sdmx-code:sex;
    skos:prefLabel "Female"@en ;
	skos:prefLabel "女"@zh-CN;
    skos:notation "F" ;
    . 
sdmx-code:sex skos:hasTopConcept <http://purl.org/linked-data/sdmx/2009/code#sex-F> .

<http://purl.org/linked-data/sdmx/2009/code#sex-M> a skos:Concept, sdmx:Concept, sdmx-code:Sex;
    skos:topConceptOf sdmx-code:sex;
    skos:inScheme     sdmx-code:sex;
    skos:prefLabel "Male"@en ;
	skos:prefLabel "男"@zh-CN;
    skos:notation "M" ;
    . 
sdmx-code:sex skos:hasTopConcept <http://purl.org/linked-data/sdmx/2009/code#sex-M> .

<http://purl.org/linked-data/sdmx/2009/code#sex-U> a skos:Concept, sdmx:Concept, sdmx-code:Sex;
    skos:topConceptOf sdmx-code:sex;
    skos:inScheme     sdmx-code:sex;
    skos:prefLabel "Not specified or unknown"@en ;
	skos:prefLabel "未设置/未知"@zh-CN;
    skos:notation "U" ;
    . 
sdmx-code:sex skos:hasTopConcept <http://purl.org/linked-data/sdmx/2009/code#sex-U> .

<http://purl.org/linked-data/sdmx/2009/code#sex-N> a skos:Concept, sdmx:Concept, sdmx-code:Sex;
    skos:topConceptOf sdmx-code:sex;
    skos:inScheme     sdmx-code:sex;
    skos:prefLabel "Not applicable"@en ;
	skos:prefLabel "不适用"@zh-CN;
    skos:notation "N" ;
    . 
sdmx-code:sex skos:hasTopConcept <http://purl.org/linked-data/sdmx/2009/code#sex-N> .

<http://purl.org/linked-data/sdmx/2009/code#sex-T> a skos:Concept, sdmx:Concept, sdmx-code:Sex;
    skos:topConceptOf sdmx-code:sex;
    skos:inScheme     sdmx-code:sex;
    skos:prefLabel "Total"@en ;
	skos:prefLabel "合计"@zh-CN;
    skos:notation "T" ;
    . 
sdmx-code:sex skos:hasTopConcept <http://purl.org/linked-data/sdmx/2009/code#sex-T> .

# CL_TIME_FORMAT
sdmx-code:timeFormat a skos:ConceptScheme, sdmx:CodeList;
    skos:prefLabel "Code list for the Time Format as written in the SDMX-EDI and SDMX-ML messages - codelist scheme"@en;
	skos:prefLabel "采用SDMX-EDI和SDMX-ML信息书写的时间格式代码列表 - 代码列表体系"@zh-CN;
    rdfs:label "Code list for the Time Format as written in the SDMX-EDI and SDMX-ML messages - codelist scheme"@en;
	rdfs:label ""@zh-CN;
    skos:notation "CL_TIME_FORMAT";
    skos:note """These codes (based on the ISO 8601 standard) indicate the type of time references used in the data. The numeric codes below (203, 102,...,702) are used only in the SDMX-EDI messages; and the alphanumeric codes (P1D...PT1M) only in the SDMX-ML messages."""@en;
    skos:note """这些代码（基于ISO 8601标准）指出了在数据中引用时间的类型。下面的数字代码（203,102，……，702）只用于SDMX-EDI信息，而字母代码（P1D……PT1M）只用于SDMX-ML信息。"""@zh-CN;
	skos:definition <http://sdmx.org/wp-content/uploads/2009/01/02_sdmx_cog_annex_2_cl_2009.pdf> ;
    rdfs:seeAlso sdmx-code:TimeFormat .

sdmx-code:TimeFormat a rdfs:Class, owl:Class;
    rdfs:subClassOf skos:Concept ;
    rdfs:label "Code list for the Time Format as written in the SDMX-EDI and SDMX-ML messages - codelist class"@en;
	rdfs:label "采用SDMX-EDI和SDMX-ML信息书写的时间格式代码列表 - 代码列表类"@zh-CN;
    rdfs:comment """These codes (based on the ISO 8601 standard) indicate the type of time references used in the data. The numeric codes below (203, 102,...,702) are used only in the SDMX-EDI messages; and the alphanumeric codes (P1D...PT1M) only in the SDMX-ML messages."""@en;
    rdfs:comment """。"""@zh-CN;
	rdfs:seeAlso sdmx-code:timeFormat .

<http://purl.org/linked-data/sdmx/2009/code#timeFormat-102> a skos:Concept, sdmx:Concept, sdmx-code:TimeFormat;
    skos:topConceptOf sdmx-code:timeFormat;
    skos:inScheme     sdmx-code:timeFormat;
    skos:prefLabel "CCYYMMDD"@en ;
	skos:prefLabel "CCYYMMDD"@zh-CN;
    skos:notation "102" ;
    skos:definition """(for daily and business series) year/month/day"""@en ; 
	skos:definition """（每日或工作日的系列）年/月/日。"""@zh-CN;
    . 
sdmx-code:timeFormat skos:hasTopConcept <http://purl.org/linked-data/sdmx/2009/code#timeFormat-102> .

<http://purl.org/linked-data/sdmx/2009/code#timeFormat-203> a skos:Concept, sdmx:Concept, sdmx-code:TimeFormat;
    skos:topConceptOf sdmx-code:timeFormat;
    skos:inScheme     sdmx-code:timeFormat;
    skos:prefLabel "CCYYMMDDhhmm"@en ;
	skos:prefLabel "CCYYMMDDhhmm"@zh-CN;
    skos:notation "203" ;
    skos:definition """(for series with freq. higher than daily) year/month/day/hours/minutes"""@en ; 
	skos:definition """（频率高于日的系列）年/月/日/时/分。"""@zh-CN;
    . 
sdmx-code:timeFormat skos:hasTopConcept <http://purl.org/linked-data/sdmx/2009/code#timeFormat-203> .

<http://purl.org/linked-data/sdmx/2009/code#timeFormat-602> a skos:Concept, sdmx:Concept, sdmx-code:TimeFormat;
    skos:topConceptOf sdmx-code:timeFormat;
    skos:inScheme     sdmx-code:timeFormat;
    skos:prefLabel "CCYY"@en ;
	skos:prefLabel "CCYY"@zh-CN;
    skos:notation "602" ;
    skos:definition """(for annual series) year"""@en ; 
	skos:definition """（年的系列）年。"""@zh-CN;
    . 
sdmx-code:timeFormat skos:hasTopConcept <http://purl.org/linked-data/sdmx/2009/code#timeFormat-602> .

<http://purl.org/linked-data/sdmx/2009/code#timeFormat-604> a skos:Concept, sdmx:Concept, sdmx-code:TimeFormat;
    skos:topConceptOf sdmx-code:timeFormat;
    skos:inScheme     sdmx-code:timeFormat;
    skos:prefLabel "CCYYS"@en ;
	skos:prefLabel "CCYYS"@zh-CN;
    skos:notation "604" ;
    skos:definition """(for half yearly series) year/semester"""@en ; 
	skos:definition """（半年的系列）年/半年。"""@zh-CN;
    . 
sdmx-code:timeFormat skos:hasTopConcept <http://purl.org/linked-data/sdmx/2009/code#timeFormat-604> .

<http://purl.org/linked-data/sdmx/2009/code#timeFormat-608> a skos:Concept, sdmx:Concept, sdmx-code:TimeFormat;
    skos:topConceptOf sdmx-code:timeFormat;
    skos:inScheme     sdmx-code:timeFormat;
    skos:prefLabel "CCYYQ"@en ;
	skos:prefLabel "CCYYQ"@zh-CN;
    skos:notation "608" ;
    skos:definition """(for quarterly series) year/quarter"""@en ; 
	skos:definition """（季度的系列）年/季。"""@zh-CN;
    . 
sdmx-code:timeFormat skos:hasTopConcept <http://purl.org/linked-data/sdmx/2009/code#timeFormat-608> .

<http://purl.org/linked-data/sdmx/2009/code#timeFormat-610> a skos:Concept, sdmx:Concept, sdmx-code:TimeFormat;
    skos:topConceptOf sdmx-code:timeFormat;
    skos:inScheme     sdmx-code:timeFormat;
    skos:prefLabel "CCYYMM"@en ;
	skos:prefLabel "CCYYMM"@zh-CN;
    skos:notation "610" ;
    skos:definition """(for monthly series) year/month"""@en ; 
	skos:definition """（月的系列）年/月。"""@zh-CN;
    . 
sdmx-code:timeFormat skos:hasTopConcept <http://purl.org/linked-data/sdmx/2009/code#timeFormat-610> .

<http://purl.org/linked-data/sdmx/2009/code#timeFormat-616> a skos:Concept, sdmx:Concept, sdmx-code:TimeFormat;
    skos:topConceptOf sdmx-code:timeFormat;
    skos:inScheme     sdmx-code:timeFormat;
    skos:prefLabel "CCYYWW"@en ;
	skos:prefLabel "CCYYWW"@zh-CN;
    skos:notation "616" ;
    skos:definition """(for weekly series) year/ week"""@en ; 
	skos:definition """（周的系列）年/周。"""@zh-CN;
    . 
sdmx-code:timeFormat skos:hasTopConcept <http://purl.org/linked-data/sdmx/2009/code#timeFormat-616> .

<http://purl.org/linked-data/sdmx/2009/code#timeFormat-702> a skos:Concept, sdmx:Concept, sdmx-code:TimeFormat;
    skos:topConceptOf sdmx-code:timeFormat;
    skos:inScheme     sdmx-code:timeFormat;
    skos:prefLabel "CCYYCCYY"@en ;
	skos:prefLabel "CCYYCCYY"@zh-CN;
    skos:notation "702" ;
    skos:definition """(for annual series) from year to year"""@en ; 
	skos:definition """（年的系列）从 年 到 年。"""@zh-CN;
    . 
sdmx-code:timeFormat skos:hasTopConcept <http://purl.org/linked-data/sdmx/2009/code#timeFormat-702> .

<http://purl.org/linked-data/sdmx/2009/code#timeFormat-704> a skos:Concept, sdmx:Concept, sdmx-code:TimeFormat;
    skos:topConceptOf sdmx-code:timeFormat;
    skos:inScheme     sdmx-code:timeFormat;
    skos:prefLabel "CCYYSCCYYS"@en ;
	skos:prefLabel "CCYYSCCYYS"@zh-CN;
    skos:notation "704" ;
    skos:definition """(for half yearly series) from half-year to half-year"""@en ; 
	skos:definition """（半年的系列）从 半年 到 半年。"""@zh-CN;
    . 
sdmx-code:timeFormat skos:hasTopConcept <http://purl.org/linked-data/sdmx/2009/code#timeFormat-704> .

<http://purl.org/linked-data/sdmx/2009/code#timeFormat-708> a skos:Concept, sdmx:Concept, sdmx-code:TimeFormat;
    skos:topConceptOf sdmx-code:timeFormat;
    skos:inScheme     sdmx-code:timeFormat;
    skos:prefLabel "CCYYQCCYYQ"@en ;
	skos:prefLabel "CCYYQCCYYQ"@zh-CN;
    skos:notation "708" ;
    skos:definition """(for quarterly series) from year/quarter to year/quarter"""@en ; 
    skos:definition """（季度的系列）从 年/季 到 年/季。"""@zh-CN;
	. 
sdmx-code:timeFormat skos:hasTopConcept <http://purl.org/linked-data/sdmx/2009/code#timeFormat-708> .

<http://purl.org/linked-data/sdmx/2009/code#timeFormat-710> a skos:Concept, sdmx:Concept, sdmx-code:TimeFormat;
    skos:topConceptOf sdmx-code:timeFormat;
    skos:inScheme     sdmx-code:timeFormat;
    skos:prefLabel "CCYYMMCCYYMM"@en ;
	skos:prefLabel "CCYYMMCCYYMM"@zh-CN;
    skos:notation "710" ;
    skos:definition """(for monthly series) from year/month to year/month"""@en ; 
	skos:definition """（每月的系列）从 年/月 到 年/月。"""@zh-CN;
    . 
sdmx-code:timeFormat skos:hasTopConcept <http://purl.org/linked-data/sdmx/2009/code#timeFormat-710> .

<http://purl.org/linked-data/sdmx/2009/code#timeFormat-711> a skos:Concept, sdmx:Concept, sdmx-code:TimeFormat;
    skos:topConceptOf sdmx-code:timeFormat;
    skos:inScheme     sdmx-code:timeFormat;
    skos:prefLabel "CCYYMMDDCCYYMMDD"@en ;
	skos:prefLabel "CCYYMMDDCCYYMMDD"@zh-CN;
    skos:notation "711" ;
    skos:definition """(for daily and business series) from year/month/day to year/month/day"""@en ;
	skos:definition """（每日或工作日的系列）从 年/月/日 到 年/月/日。"""@zh-CN; 
    . 
sdmx-code:timeFormat skos:hasTopConcept <http://purl.org/linked-data/sdmx/2009/code#timeFormat-711> .

<http://purl.org/linked-data/sdmx/2009/code#timeFormat-716> a skos:Concept, sdmx:Concept, sdmx-code:TimeFormat;
    skos:topConceptOf sdmx-code:timeFormat;
    skos:inScheme     sdmx-code:timeFormat;
    skos:prefLabel "CCYYWWCCYYWW"@en ;
	skos:prefLabel "CCYYWWCCYYWW"@zh-CN;
    skos:notation "716" ;
    skos:definition """(for weekly series) from year/week to year/week"""@en ;
	skos:definition """（每周的系列）从 年/周 到 年/周。"""@zh-CN;
    . 
sdmx-code:timeFormat skos:hasTopConcept <http://purl.org/linked-data/sdmx/2009/code#timeFormat-716> .

<http://purl.org/linked-data/sdmx/2009/code#timeFormat-719> a skos:Concept, sdmx:Concept, sdmx-code:TimeFormat;
    skos:topConceptOf sdmx-code:timeFormat;
    skos:inScheme     sdmx-code:timeFormat;
    skos:prefLabel "CCYYMMDDhhmmmCCYYMMDDhhmmm"@en ;
	skos:prefLabel "CCYYMMDDhhmmmCCYYMMDDhhmmm"@zh-CN;
    skos:notation "719" ;
    skos:definition """(for series with freq. higher than daily) year/month/day/hours/minutes to year/month/day/hours/minutes."""@en ;
	skos:definition """（频率高于日的系列）从 年/月/日/时/分 到 年/月/日/时/分。"""@zh-CN;
    . 
sdmx-code:timeFormat skos:hasTopConcept <http://purl.org/linked-data/sdmx/2009/code#timeFormat-719> .

<http://purl.org/linked-data/sdmx/2009/code#timeFormat-P1D> a skos:Concept, sdmx:Concept, sdmx-code:TimeFormat;
    skos:topConceptOf sdmx-code:timeFormat;
    skos:inScheme     sdmx-code:timeFormat;
    skos:prefLabel "Daily (or Business)"@en ;
	skos:prefLabel "每天（或者营业时间）"@zh-CN;
    skos:notation "P1D" ;
    . 
sdmx-code:timeFormat skos:hasTopConcept <http://purl.org/linked-data/sdmx/2009/code#timeFormat-P1D> .

<http://purl.org/linked-data/sdmx/2009/code#timeFormat-P1M> a skos:Concept, sdmx:Concept, sdmx-code:TimeFormat;
    skos:topConceptOf sdmx-code:timeFormat;
    skos:inScheme     sdmx-code:timeFormat;
    skos:prefLabel "Monthly"@en ;
	skos:prefLabel "每月"@zh-CN;
    skos:notation "P1M" ;
    . 
sdmx-code:timeFormat skos:hasTopConcept <http://purl.org/linked-data/sdmx/2009/code#timeFormat-P1M> .

<http://purl.org/linked-data/sdmx/2009/code#timeFormat-P1Y> a skos:Concept, sdmx:Concept, sdmx-code:TimeFormat;
    skos:topConceptOf sdmx-code:timeFormat;
    skos:inScheme     sdmx-code:timeFormat;
    skos:prefLabel "Annual"@en ;
	skos:prefLabel "全年"@zh-CN;
    skos:notation "P1Y" ;
    . 
sdmx-code:timeFormat skos:hasTopConcept <http://purl.org/linked-data/sdmx/2009/code#timeFormat-P1Y> .

<http://purl.org/linked-data/sdmx/2009/code#timeFormat-P3M> a skos:Concept, sdmx:Concept, sdmx-code:TimeFormat;
    skos:topConceptOf sdmx-code:timeFormat;
    skos:inScheme     sdmx-code:timeFormat;
    skos:prefLabel "Quarterly"@en ;
	skos:prefLabel "每季"@zh-CN;
    skos:notation "P3M" ;
    . 
sdmx-code:timeFormat skos:hasTopConcept <http://purl.org/linked-data/sdmx/2009/code#timeFormat-P3M> .

<http://purl.org/linked-data/sdmx/2009/code#timeFormat-P6M> a skos:Concept, sdmx:Concept, sdmx-code:TimeFormat;
    skos:topConceptOf sdmx-code:timeFormat;
    skos:inScheme     sdmx-code:timeFormat;
    skos:prefLabel "Half-yearly"@en ;
	skos:prefLabel "每半年"@zh-CN;
    skos:notation "P6M" ;
    . 
sdmx-code:timeFormat skos:hasTopConcept <http://purl.org/linked-data/sdmx/2009/code#timeFormat-P6M> .

<http://purl.org/linked-data/sdmx/2009/code#timeFormat-P7D> a skos:Concept, sdmx:Concept, sdmx-code:TimeFormat;
    skos:topConceptOf sdmx-code:timeFormat;
    skos:inScheme     sdmx-code:timeFormat;
    skos:prefLabel "Weekly"@en ;
	skos:prefLabel "每周"@zh-CN;
    skos:notation "P7D" ;
    . 
sdmx-code:timeFormat skos:hasTopConcept <http://purl.org/linked-data/sdmx/2009/code#timeFormat-P7D> .

<http://purl.org/linked-data/sdmx/2009/code#timeFormat-PT1M> a skos:Concept, sdmx:Concept, sdmx-code:TimeFormat;
    skos:topConceptOf sdmx-code:timeFormat;
    skos:inScheme     sdmx-code:timeFormat;
    skos:prefLabel "Minutely"@en ;
	skos:prefLabel "每分钟"@zh-CN;
    skos:notation "PT1M" ;
    . 
sdmx-code:timeFormat skos:hasTopConcept <http://purl.org/linked-data/sdmx/2009/code#timeFormat-PT1M> .

# CL_UNIT_MULT
sdmx-code:unitMult a skos:ConceptScheme, sdmx:CodeList;
    skos:prefLabel "code list for the Unit Multiplier (UNIT_MULT) - codelist scheme"@en;
	skos:prefLabel "单位乘数（UNIT_MULT）的代码列表 - 代码列表体系"@zh-CN;
    rdfs:label "code list for the Unit Multiplier (UNIT_MULT) - codelist scheme"@en;
	rdfs:label "单位乘数（UNIT_MULT）的代码列表 - 代码列表体系"@zh-CN;
    skos:notation "CL_UNIT_MULT";
    skos:note """it provides code values for indicating the magnitude in the units of measurements."""@en;
	skos:note """它提供了代码值，用于指示在测量单位的大小。"""@zh-CN;
    skos:definition <http://sdmx.org/wp-content/uploads/2009/01/02_sdmx_cog_annex_2_cl_2009.pdf> ;
    rdfs:seeAlso sdmx-code:UnitMult .

sdmx-code:UnitMult a rdfs:Class, owl:Class;
    rdfs:subClassOf skos:Concept ;
    rdfs:label "code list for the Unit Multiplier (UNIT_MULT) - codelist class"@en;
	rdfs:label "单位乘数（UNIT_MULT）的代码列表 - 代码列表类"@zh-CN;
    rdfs:comment """it provides code values for indicating the magnitude in the units of measurements."""@en;
	rdfs:comment """它提供了代码值，用于指示在测量单位的大小。"""@zh-CN;
    rdfs:seeAlso sdmx-code:unitMult .

<http://purl.org/linked-data/sdmx/2009/code#unitMult-0> a skos:Concept, sdmx:Concept, sdmx-code:UnitMult;
    skos:topConceptOf sdmx-code:unitMult;
    skos:inScheme     sdmx-code:unitMult;
    skos:prefLabel "Units"@en ;
	skos:prefLabel "单位"@zh-CN;
    skos:notation "0" ;
    . 
sdmx-code:unitMult skos:hasTopConcept <http://purl.org/linked-data/sdmx/2009/code#unitMult-0> .

<http://purl.org/linked-data/sdmx/2009/code#unitMult-1> a skos:Concept, sdmx:Concept, sdmx-code:UnitMult;
    skos:topConceptOf sdmx-code:unitMult;
    skos:inScheme     sdmx-code:unitMult;
    skos:prefLabel "Tens"@en ;
	skos:prefLabel "十"@zh-CN;
    skos:notation "1" ;
    . 
sdmx-code:unitMult skos:hasTopConcept <http://purl.org/linked-data/sdmx/2009/code#unitMult-1> .

<http://purl.org/linked-data/sdmx/2009/code#unitMult-2> a skos:Concept, sdmx:Concept, sdmx-code:UnitMult;
    skos:topConceptOf sdmx-code:unitMult;
    skos:inScheme     sdmx-code:unitMult;
    skos:prefLabel "Hundreds"@en ;
	skos:prefLabel "百"@zh-CN;
    skos:notation "2" ;
    . 
sdmx-code:unitMult skos:hasTopConcept <http://purl.org/linked-data/sdmx/2009/code#unitMult-2> .

<http://purl.org/linked-data/sdmx/2009/code#unitMult-3> a skos:Concept, sdmx:Concept, sdmx-code:UnitMult;
    skos:topConceptOf sdmx-code:unitMult;
    skos:inScheme     sdmx-code:unitMult;
    skos:prefLabel "Thousands"@en ;
	skos:prefLabel "千"@zh-CN;
    skos:notation "3" ;
    . 
sdmx-code:unitMult skos:hasTopConcept <http://purl.org/linked-data/sdmx/2009/code#unitMult-3> .

<http://purl.org/linked-data/sdmx/2009/code#unitMult-4> a skos:Concept, sdmx:Concept, sdmx-code:UnitMult;
    skos:topConceptOf sdmx-code:unitMult;
    skos:inScheme     sdmx-code:unitMult;
    skos:prefLabel "Tens of thousands"@en ;
	skos:prefLabel "万"@zh-CN;
    skos:notation "4" ;
    . 
sdmx-code:unitMult skos:hasTopConcept <http://purl.org/linked-data/sdmx/2009/code#unitMult-4> .

<http://purl.org/linked-data/sdmx/2009/code#unitMult-6> a skos:Concept, sdmx:Concept, sdmx-code:UnitMult;
    skos:topConceptOf sdmx-code:unitMult;
    skos:inScheme     sdmx-code:unitMult;
    skos:prefLabel "Millions"@en ;
	skos:prefLabel "百万"@zh-CN;
    skos:notation "6" ;
    . 
sdmx-code:unitMult skos:hasTopConcept <http://purl.org/linked-data/sdmx/2009/code#unitMult-6> .

<http://purl.org/linked-data/sdmx/2009/code#unitMult-9> a skos:Concept, sdmx:Concept, sdmx-code:UnitMult;
    skos:topConceptOf sdmx-code:unitMult;
    skos:inScheme     sdmx-code:unitMult;
    skos:prefLabel "Billions"@en ;
	skos:prefLabel "十亿"@zh-CN;
    skos:notation "9" ;
    . 
sdmx-code:unitMult skos:hasTopConcept <http://purl.org/linked-data/sdmx/2009/code#unitMult-9> .

<http://purl.org/linked-data/sdmx/2009/code#unitMult-12> a skos:Concept, sdmx:Concept, sdmx-code:UnitMult;
    skos:topConceptOf sdmx-code:unitMult;
    skos:inScheme     sdmx-code:unitMult;
    skos:prefLabel "Trillions"@en ;
	skos:prefLabel "万亿"@zh-CN;
    skos:notation "12" ;
    . 
sdmx-code:unitMult skos:hasTopConcept <http://purl.org/linked-data/sdmx/2009/code#unitMult-12> .

<http://purl.org/linked-data/sdmx/2009/code#unitMult-15> a skos:Concept, sdmx:Concept, sdmx-code:UnitMult;
    skos:topConceptOf sdmx-code:unitMult;
    skos:inScheme     sdmx-code:unitMult;
    skos:prefLabel "Quadrillions"@en ;
	skos:prefLabel "千万亿"@zh-CN;
    skos:notation "15" ;
    . 
sdmx-code:unitMult skos:hasTopConcept <http://purl.org/linked-data/sdmx/2009/code#unitMult-15> .

