<?xml version="1.0" encoding="UTF-8"?><!-- 
This is a draft RDF Schema for AgMES Namespace (ags) This has been based on the draft version of AgMES for Document-like information objects provided at:   ftp://ext-ftp.fao.org/agris/papers/AGMESNS-DLIO_en.doc
URL of this schema is:  http://www.fao.org/agris/agmes/schemas/1.1/ags
For Comments: Please write to FAO-Agris-Caris@fao.org with the subject line ATTN: GAURI 
--><!--
Schema change history (2005-07-04): 
	- Add DOI as scheme for identifier
    - Change 'edition' to 'descriptionEdition'
    - Change 'statement' and 'termsofuse' to  'rightsStatement' and  'rightsTermsOfUse'
    - Add CODEN as a scheme for citationIdentifier
--><!DOCTYPE rdf:RDF[
	<!ENTITY rdfns 'http://www.w3.org/1999/02/22-rdf-syntax-ns#'>
	<!ENTITY rdfsns 'http://www.w3.org/2000/01/rdf-schema#'>
	<!ENTITY dcns 'http://purl.org/dc/elements/1.1/'>
	<!ENTITY dctermsns 'http://purl.org/dc/terms/'>
	<!ENTITY dctypens 'http://purl.org/dc/dcmitype/'>
	<!ENTITY agsns 'http://purl.org/agmes/1.1/'>
	<!ENTITY aglsns 'http://www.agls.gov.au/rdf/1.2/agls.rdfs'>
]><rdf:RDF xmlns:rdf="http://www.w3.org/1999/02/22-rdf-syntax-ns#" xmlns:rdfs="http://www.w3.org/2000/01/rdf-schema#" xmlns:dc="http://purl.org/dc/elements/1.1/" xmlns:dcterms="http://purl.org/dc/terms/" xmlns:dctype="http://purl.org/dc/dcmitype/" xmlns:ags="http://purl.org/agmes/1.1/" xmlns:agls="http://www.agls.gov.au/rdf/1.2/agls.rdfs"><!-- Description of Schema / Description de schéma / Descripción de esquema --><rdf:Description rdf:about="http://purl.org/agmes/1.1/"><dc:title xml:lang="en">The Agricultural Metadata Element Set v.1.1 -- RDF schema Declaration</dc:title><dc:date>2005-07-04</dc:date><dc:description xml:lang="en">The objectives of the AgMES Project include development and proposal of agricultural information standards and ontologies for the combined purpose of resource discovery, interoperability and effective data exchange between and among uniquely and richly described agricultural resources. The AgMES as a namespace complements DC in that it provides newly coined elements deemed necessary for complete description of information resources. </dc:description><dc:identifier rdf:resource="http://www.fao.org/agris/agmes/schemas/1.1/ags" /><dc:identifier rdf:resource="http://purl.org/agmes/1.1/" /><dc:publisher>FAO</dc:publisher><dc:format>RDF/XML</dc:format><dc:language>English, French, Spanish</dc:language><dc:relation rdf:resource="http://www.fao.org/agris/agmes/" /></rdf:Description><!-- Begin:Title --><!-- Title refinement : Title Supplement --><rdf:Property rdf:about="http://purl.org/agmes/1.1/titleSupplement"><rdfs:label xml:lang="en">Title Supplement </rdfs:label><rdfs:comment xml:lang="en">Secondary information related to the title.</rdfs:comment><rdfs:subPropertyOf rdf:resource="http://purl.org/dc/elements/1.1/title" /><rdfs:isDefinedBy rdf:resource="http://purl.org/agmes/1.1/" /></rdf:Property><!-- End/ Fin / Fin: Title --><!-- Begin: Creator  --><!-- Creator refinement : Corporate Creator --><rdf:Property rdf:about="http://purl.org/agmes/1.1/creatorCorporate"><rdfs:label xml:lang="en">Corporate Creator</rdfs:label><rdfs:comment xml:lang="en">Organization or a group of people identified by a name responsible for creating or making contributions to the intellectual content of the resource.</rdfs:comment><rdfs:subPropertyOf rdf:resource="http://purl.org/dc/elements/1.1/creator" /><rdfs:isDefinedBy rdf:resource="http://purl.org/agmes/1.1/" /></rdf:Property><!-- Creator refinement : Personal Creator --><rdf:Property rdf:about="http://purl.org/agmes/1.1/creatorPersonal"><rdfs:label xml:lang="en">Personal Creator </rdfs:label><rdfs:comment xml:lang="en">Person responsible for creating or making contributions to the intellectual content of the resource.</rdfs:comment><rdfs:subPropertyOf rdf:resource="http://purl.org/dc/elements/1.1/creator" /><rdfs:isDefinedBy rdf:resource="http://purl.org/agmes/1.1/" /></rdf:Property><!-- Creator refinement : Conference as a Creator --><rdf:Property rdf:about="http://purl.org/agmes/1.1/creatorConference"><rdfs:label xml:lang="en"> Conference as a Creator </rdfs:label><rdfs:comment xml:lang="en">Conferences are named meetings of individuals or representatives of various bodies for the purpose of discussing and acting on topics of common interest, or meetings of representatives of a corporate body that constitute its legislative or governing body.</rdfs:comment><rdfs:subPropertyOf rdf:resource="http://purl.org/dc/elements/1.1/creator" /><rdfs:isDefinedBy rdf:resource="http://purl.org/agmes/1.1/" /></rdf:Property><!-- End/ Fin / Fin: Creator --><!-- Begin:Publisher --><!-- Publisher refinement : Name of Publisher --><rdf:Property rdf:about="http://purl.org/agmes/1.1/pubisherName"><rdfs:label xml:lang="en"> Name of the Publisher </rdfs:label><rdfs:comment xml:lang="en"> A publisher is the individual, group, or organization named in the document as being responsible for that document's publication, distribution, issuing, or release.</rdfs:comment><rdfs:subPropertyOf rdf:resource="http://purl.org/dc/elements/1.1/Publisher" /><rdfs:isDefinedBy rdf:resource="http://purl.org/agmes/1.1/" /></rdf:Property><!-- Publisher refinement : Place of Publication --><rdf:Property rdf:about="http://purl.org/agmes/1.1/publisherPlace"><rdfs:label xml:lang="en"> Place of Publication </rdfs:label><rdfs:comment xml:lang="en"> The place of publication of an item is the city, town, or other locality associated with the name of the publisher entered in the Publisher Name field.</rdfs:comment><rdfs:subPropertyOf rdf:resource="http://purl.org/dc/elements/1.1/Publisher" /><rdfs:isDefinedBy rdf:resource="http://purl.org/agmes/1.1/" /></rdf:Property><!-- End/ Fin / Fin: Publisher --><!-- Begin: Subject --><!-- Subject refinement : Classification --><rdf:Property rdf:about="http://purl.org/agmes/1.1/subjectClassification"><rdfs:label xml:lang="en">Subject Classification</rdfs:label><rdfs:comment xml:lang="en">The systematic arranging into classes (classifying), according to common characteristics or affinities,  things, topics, themes or notions which are the subject of any branch of science or of a methodical inquiry.</rdfs:comment><rdfs:subPropertyOf rdf:resource="http://purl.org/dc/elements/1.1/subject" /><rdfs:range rdf:resource="http://purl.org/agmes/1.1/ClassificationScheme" /><rdfs:isDefinedBy rdf:resource="http://purl.org/agmes/1.1/" /></rdf:Property><!-- Subject refinement : Thesaurus --><rdf:Property rdf:about="http://purl.org/agmes/1.1/subjectThesaurus"><rdfs:label xml:lang="en"> Subject Thesaurus</rdfs:label><rdfs:comment xml:lang="en">A classified list of terms or keywords, in a particular field, for use in indexing and information retrieval.</rdfs:comment><rdfs:subPropertyOf rdf:resource="http://purl.org/dc/elements/1.1/subject" /><rdfs:range rdf:resource="http://purl.org/agmes/1.1/ThesaurusScheme" /><rdfs:isDefinedBy rdf:resource="http://purl.org/agmes/1.1/" /></rdf:Property><!-- Classification range declarations --><!-- Encoding Scheme declarations --><rdfs:Class rdf:about="http://purl.org/agmes/1.1/ClassificationScheme"><rdfs:label xml:lang="en">Subject Encoding Schemes</rdfs:label><rdfs:comment xml:lang="en">A set of subject encoding schemes and/or formats.</rdfs:comment><rdfs:isDefinedBy rdf:resource="http://purl.org/dc/terms/" /></rdfs:Class><!-- Schemes for Subject Classification : ASC --><rdfs:Class rdf:about="http://purl.org/agmes/1.1/ASC"><rdfs:label xml:lang="en">AGRIS Subject Categories</rdfs:label><rdfs:comment xml:lang="en">AGRIS Subject Categories are subject categories for indexing of agricultural resources developed and maintained by FAO.</rdfs:comment><rdfs:subClassOf rdf:resource="http://purl.org/agmes/1.1/ClassificationScheme" /><rdfs:isDefinedBy rdf:resource="http://purl.org/agmes/1.1/" /><rdfs:seeAlso rdf:resource="http://www.fao.org/agris/ " /></rdfs:Class><!-- Schemes for Subject Classification : CABC --><rdfs:Class rdf:about="http://purl.org/agmes/1.1/CABC"><rdfs:label xml:lang="en">CABI Codes</rdfs:label><rdfs:comment xml:lang="en">CABI Codes are themain subject headings derived from the classification schemes used in the AGRICOLA and AGRIS databases, to group resources in to a specific subject maintained by CAB  
International.</rdfs:comment><rdfs:subClassOf rdf:resource="http://purl.org/agmes/1.1/ClassificationScheme" /><rdfs:isDefinedBy rdf:resource="http://purl.org/agmes/1.1/" /><rdfs:seeAlso rdf:resource="http://www.cabi-publishing.org/ " /></rdfs:Class><!-- Thesaurus range declarations --><!-- Encoding Schemes declarations --><rdfs:Class rdf:about="http://purl.org/agmes/1.1/ThesaurusScheme"><rdfs:label xml:lang="en">Thesuaurs Schemes</rdfs:label><rdfs:comment xml:lang="en">A set of subject encoding schemes and/or formats.</rdfs:comment><rdfs:isDefinedBy rdf:resource="http://purl.org/agmes/1.1/" /></rdfs:Class><!-- Schemes for Subject Thesaurus :  AGROVOC--><rdfs:Class rdf:about="http://purl.org/agmes/1.1/AGROVOC"><rdfs:label xml:lang="en">AGROVOC</rdfs:label><rdfs:comment xml:lang="en">Multilingual agricultural thesaurus produced by FAO, and used for indexing and cataloguing.</rdfs:comment><rdfs:subClassOf rdf:resource="http://purl.org/agmes/1.1/ThesaurusScheme" /><rdfs:isDefinedBy rdf:resource="http://purl.org/agmes/1.1/" /><rdfs:seeAlso rdf:resource="http://www.fao.org/agrovoc/" /></rdfs:Class><!-- Schemes for Subject Thesaurus : CABT --><rdfs:Class rdf:about="http://purl.org/agmes/1.1/CABT"><rdfs:label xml:lang="en">CABI Thesaurus</rdfs:label><rdfs:comment xml:lang="en">A controlled vocabulary of terms, especially key words, in agricultural sciences for use in indexing and information retrieval created and produced by CAB International. </rdfs:comment><rdfs:subClassOf rdf:resource="http://purl.org/agmes/1.1/ThesaurusScheme" /><rdfs:isDefinedBy rdf:resource="http://purl.org/agmes/1.1/" /><rdfs:seeAlso rdf:resource="http://www.cabi-publishing.org/ " /></rdfs:Class><!-- Schemes for Subject Thesaurus :  ASFAT--><rdfs:Class rdf:about="http://purl.org/agmes/1.1/ASFAT"><rdfs:label xml:lang="en">Aquatic Science and Fisheries Abstracts Thesaurus</rdfs:label><rdfs:comment xml:lang="en">A controlled vocabulary of terms, especially key words, in fisheries for use in indexing and information retrieval created by ASFA (Aquatic Sciences and Fisheries Abstracts).</rdfs:comment><rdfs:subClassOf rdf:resource="http://purl.org/agmes/1.1/ThesaurusScheme" /><rdfs:isDefinedBy rdf:resource="http://purl.org/agmes/1.1/" /><rdfs:seeAlso rdf:resource="http://www.csa.com/helpV3/ab.html" /></rdfs:Class><!-- Schemes for Subject Thesaurus :  NALT--><rdfs:Class rdf:about="http://purl.org/agmes/1.1/NALT"><rdfs:label xml:lang="en">National Agricultural Library Thesaurus</rdfs:label><rdfs:comment xml:lang="en">A controlled vocabulary of terms, especially key words, in agricultural sciences for use in indexing and information retrieval created by National Agricultural Library (NAL) of United States.</rdfs:comment><rdfs:subClassOf rdf:resource="http://purl.org/agmes/1.1/ThesaurusScheme" /><rdfs:isDefinedBy rdf:resource="http://purl.org/agmes/1.1/" /><rdfs:seeAlso rdf:resource="http://agclass.nal.usda.gov/agt/agt.htm" /></rdfs:Class><!-- End/ Fin / Fin: Subject --><!-- Begin: Description --><!-- Description refinement declarations : Notes--><rdf:Property rdf:about="http://purl.org/agmes/1.1/descriptionNotes"><rdfs:label xml:lang="en">Notes</rdfs:label><rdfs:comment xml:lang="en">Brief statement, annotation, comment, or/and elucidation concerning any aspect of the resource.</rdfs:comment><rdfs:subPropertyOf rdf:resource="http://purl.org/dc/elements/1.1/description" /><rdfs:isDefinedBy rdf:resource="http://purl.org/agmes/1.1/" /></rdf:Property><!-- Description refinement declarations : Edition--><rdf:Property rdf:about="http://purl.org/agmes/1.1/descriptionedition"><rdfs:label xml:lang="en">edition statement</rdfs:label><rdfs:comment xml:lang="en">The formally designated version of the resource.</rdfs:comment><rdfs:subPropertyOf rdf:resource="http://purl.org/dc/elements/1.1/description" /><rdfs:isDefinedBy rdf:resource="http://purl.org/agmes/1.1/" /></rdf:Property><!-- End/ Fin / Fin: Description --><!-- Begin: Identifier --><!-- Identifier refinement declarations --><!-- Identifier range declarations --><rdf:Description rdf:about="http://purl.org/dc/elements/1.1/identifier"><rdfs:range rdf:resource="http://purl.org/agmes/1.1/AgsIdentifierScheme" /></rdf:Description><!-- Encoding Scheme declarations --><rdfs:Class rdf:about="http://purl.org/agmes/1.1/AgsIdentifierScheme"><rdfs:label xml:lang="en">Identifier Encoding Schemes from AgMES</rdfs:label><rdfs:comment xml:lang="en">A set of Identified encoding schemes and/or formats. </rdfs:comment><rdfs:isDefinedBy rdf:resource="http://purl.org/agmes/1.1/" /></rdfs:Class><rdfs:Class rdf:about="http://purl.org/agmes/1.1/JN"><rdfs:label xml:lang="en">Job Number</rdfs:label><rdfs:comment xml:lang="en">Number allotted to a resource for purposes of identification and 
retrieval</rdfs:comment><rdfs:subClassOf rdf:resource="http://purl.org/agmes/1.1/AgsIdentifierScheme" /><rdfs:isDefinedBy rdf:resource="http://purl.org/agmes/1.1/" /></rdfs:Class><rdfs:Class rdf:about="http://purl.org/agmes/1.1/RN"><rdfs:label xml:lang="en">Report Number</rdfs:label><rdfs:comment xml:lang="en"> A number uniquely identifying a report.  A report is a formal statement of the results of an investigation, proceedings at a meeting, or of any occurrence, event or matter on which definite information is required.</rdfs:comment><rdfs:subClassOf rdf:resource="http://purl.org/agmes/1.1/AgsIdentifierScheme" /><rdfs:isDefinedBy rdf:resource="http://purl.org/agmes/1.1/" /></rdfs:Class><rdfs:Class rdf:about="http://purl.org/agmes/1.1/ISSN"><rdfs:label xml:lang="en">ISSN </rdfs:label><rdfs:comment xml:lang="en"> International Standards Serial Number.  It is an eight-digit number which identifies periodical publications as such, including electronic serials. </rdfs:comment><rdfs:subClassOf rdf:resource="http://purl.org/agmes/1.1/AgsIdentifierScheme" /><rdfs:isDefinedBy rdf:resource="http://purl.org/agmes/1.1/" /><rdfs:seeAlso rdf:resource="http://www.issn.org/" /></rdfs:Class><rdfs:Class rdf:about="http://purl.org/agmes/1.1/ISBN"><rdfs:label xml:lang="en">ISBN </rdfs:label><rdfs:comment xml:lang="en"> International Standard Book Number. The ISBN is a unique machine-readable identification number used to uniquely mark a book. 159 countries and territories are officially ISBN members. </rdfs:comment><rdfs:subClassOf rdf:resource="http://purl.org/agmes/1.1/AgsIdentifierScheme" /><rdfs:isDefinedBy rdf:resource="http://purl.org/agmes/1.1/" /><rdfs:seeAlso rdf:resource="http://www.isbn.org/standards/home/index.asp" /></rdfs:Class><rdfs:Class rdf:about="http://purl.org/agmes/1.1/DOI"><rdfs:label xml:lang="en">DOI </rdfs:label><rdfs:comment xml:lang="en"> The Digital Object Identifier (DOI) is a system for identifying content objects in the digital environment. DOIs are names assigned to any entity for use on digital networks. They are used to provide current information, including where they (or information about them) can be found on the Internet. Information about a digital object may change over time, including where to find it, but its DOI will not change. </rdfs:comment><rdfs:subClassOf rdf:resource="http://purl.org/agmes/1.1/AgsIdentifierScheme" /><rdfs:isDefinedBy rdf:resource="http://purl.org/agmes/1.1/" /><rdfs:seeAlso rdf:resource="http://www.doi.org/" /></rdfs:Class><!-- End/ Fin / Fin: Identifier --><!-- Begin: Relation --><!-- Relation refinement declarations --><rdf:Property rdf:about="http://purl.org/agmes/1.1/relationIsTranslationOf"><rdfs:label xml:lang="en">Is Translation Of</rdfs:label><rdfs:comment xml:lang="en">The described resource is a translation of the referenced resource. </rdfs:comment><rdfs:subPropertyOf rdf:resource="http://purl.org/dc/elements/1.1/relation" /><rdfs:isDefinedBy rdf:resource="http://purl.org/agmes/1.1/" /></rdf:Property><rdf:Property rdf:about="http://purl.org/agmes/1.1/relationHasTranslation"><rdfs:label xml:lang="en">Has Translation</rdfs:label><rdfs:comment xml:lang="en">The described resource has a translation, namely, the referenced resource. </rdfs:comment><rdfs:subPropertyOf rdf:resource="http://purl.org/dc/elements/1.1/relation" /><rdfs:isDefinedBy rdf:resource="http://purl.org/agmes/1.1/" /></rdf:Property><!-- End/ Fin / Fin: Relation --><!-- Begin: Rights --><!-- Rights refinement declarations --><rdf:Property rdf:about="http://purl.org/agmes/1.1/rightsStatement"><rdfs:label xml:lang="en"> Statement </rdfs:label><rdfs:comment xml:lang="en">Written assertion of ownership rights relating to resource.  Contains management statement for the resource or references a service providing such information. Also encompasses Intellectual Property Rights (IPR). If the Rights element is absent, no assumptions can be made about the status of these and other rights with respect to the resource.</rdfs:comment><rdfs:subPropertyOf rdf:resource="http://purl.org/dc/elements/1.1/rights" /><rdfs:isDefinedBy rdf:resource="http://purl.org/agmes/1.1/" /></rdf:Property><rdf:Property rdf:about="http://purl.org/agmes/1.1/rightsTermsOfUse"><rdfs:label xml:lang="en"> Terms of Use </rdfs:label><rdfs:comment xml:lang="en">Extent and manner of use permitted to, and restrictions covering use of resource by the public. If the Rights element is absent, no assumptions can be made about the status of these and other rights with respect to the resource.</rdfs:comment><rdfs:subPropertyOf rdf:resource="http://purl.org/dc/elements/1.1/rights" /><rdfs:isDefinedBy rdf:resource="http://purl.org/agmes/1.1/" /></rdf:Property><!-- End/ Fin / Fin: Relation --><!-- Begin : Availability --><!-- Availability refinement declarations --><rdf:Property rdf:about="http://purl.org/agmes/1.1/availabilityNumber"><rdfs:label xml:lang="en"> Availability Number </rdfs:label><rdfs:comment xml:lang="en">An unambiguous reference to the resource within a given context.</rdfs:comment><rdfs:subPropertyOf rdf:resource="http://www.agls.gov.au/rdf/1.2/availability" /><rdfs:range rdf:resource="http://purl.org/agmes/1.1/AgsAvailabilityNumberScheme" /><rdfs:isDefinedBy rdf:resource="http://purl.org/agmes/1.1/" /></rdf:Property><rdf:Property rdf:about="http://purl.org/agmes/1.1/availabilityLocation"><rdfs:label xml:lang="en"> Availability Location </rdfs:label><rdfs:comment xml:lang="en">An unambiguous reference to the location of the resource.</rdfs:comment><rdfs:subPropertyOf rdf:resource="http://www.agls.gov.au/rdf/1.2/availability" /><rdfs:isDefinedBy rdf:resource="http://purl.org/agmes/1.1/" /></rdf:Property><!-- Encoding Scheme declarations --><rdfs:Class rdf:about="http://purl.org/agmes/1.1/AgsAvailabilityNumberScheme"><rdfs:label xml:lang="en">Identifier Encoding Schemes from AgMES Availability Number</rdfs:label><rdfs:comment xml:lang="en">A set of Identified encoding schemes and/or formats.</rdfs:comment><rdfs:isDefinedBy rdf:resource="http://purl.org/agmes/1.1/" /></rdfs:Class><rdfs:Class rdf:about="http://purl.org/agmes/1.1/MN"><rdfs:label xml:lang="en">Microfiche Number</rdfs:label><rdfs:comment xml:lang="en"> Microfiche Number is a unique number identifying a microfiche, i.e. document photographed in reduced size for viewing on projector. </rdfs:comment><rdfs:subClassOf rdf:resource="http://purl.org/agmes/1.1/AgsAvailabilityNumberScheme" /><rdfs:isDefinedBy rdf:resource="http://purl.org/agmes/1.1/" /></rdfs:Class><rdfs:Class rdf:about="http://purl.org/agmes/1.1/CN"><rdfs:label xml:lang="en">Call Number</rdfs:label><rdfs:comment xml:lang="en"> Call Number </rdfs:comment><rdfs:subClassOf rdf:resource="http://purl.org/agmes/1.1/AgsAvailabilityNumberScheme" /><rdfs:isDefinedBy rdf:resource="http://purl.org/agmes/1.1/" /></rdfs:Class><rdfs:Class rdf:about="http://purl.org/agmes/1.1/AN"><rdfs:label xml:lang="en">Accession Number</rdfs:label><rdfs:comment xml:lang="en"> Accession Number is a unique number assigned to each record in a database or at an organization. Accession number should always be accompanied by the holding place information. </rdfs:comment><rdfs:subClassOf rdf:resource="http://purl.org/agmes/1.1/AgsAvailabilityNumberScheme" /><rdfs:isDefinedBy rdf:resource="http://purl.org/agmes/1.1/" /></rdfs:Class><!-- Begin: Citation --><!-- Citation  Declaration --><rdf:Property rdf:about="http://purl.org/agmes/1.1/citation"><rdfs:label xml:lang="en">Citation</rdfs:label><rdfs:comment xml:lang="en"> Citation information of a journal.</rdfs:comment><rdfs:domain rdf:resource="http://www.w3.org/2000/01/rdf-schema#Resource" /><rdfs:isDefinedBy rdf:resource="http://purl.org/agmes/1.1/" /></rdf:Property><!-- Citation refinement : Title --><rdf:Property rdf:about="http://purl.org/agmes/1.1/citationTitle"><rdfs:label xml:lang="en"> Title of the Serial</rdfs:label><rdfs:comment xml:lang="en">The serial title, also known as the key-title, is a name ascribed to a serial publication and is inseparably associated with its ISSN.</rdfs:comment><rdfs:subPropertyOf rdf:resource="http://purl.org/agmes/1.1/citation" /><rdfs:isDefinedBy rdf:resource="http://purl.org/agmes/1.1/" /></rdf:Property><!-- Citation refinement : Identifier --><rdf:Property rdf:about="http://purl.org/agmes/1.1/citationIdentifier"><rdfs:label xml:lang="en"> Identifier of the serial</rdfs:label><rdfs:comment xml:lang="en">A global standard identifier of a journal. This would usually be an ISSN, but may follow some other standards such as CODEN.</rdfs:comment><rdfs:subPropertyOf rdf:resource="http://purl.org/agmes/1.1/citation" /><rdfs:range rdf:resource="http://purl.org/agmes/1.1/AgsIdentifierScheme" /><rdfs:isDefinedBy rdf:resource="http://purl.org/agmes/1.1/" /></rdf:Property><!-- Citation range declarations --><rdf:Description rdf:about="http://purl.org/agmes/1.1/citationIdentifier"><rdfs:range rdf:resource="http://purl.org/agmes/1.1/AgscitationIdentifierScheme" /></rdf:Description><!-- Encoding Scheme declarations --><rdfs:Class rdf:about="http://purl.org/agmes/1.1/AgsIdentifierScheme"><rdfs:label xml:lang="en">Citation Identifier Encoding Schemes from AgMES</rdfs:label><rdfs:comment xml:lang="en">A set of Identified encoding schemes and/or formats. </rdfs:comment><rdfs:isDefinedBy rdf:resource="http://purl.org/agmes/1.1/" /></rdfs:Class><rdfs:Class rdf:about="http://purl.org/agmes/1.1/ISSN"><rdfs:label xml:lang="en">ISSN </rdfs:label><rdfs:comment xml:lang="en"> International Standards Serial Number.  It is an eight-digit number which identifies periodical publications as such, including electronic serials. </rdfs:comment><rdfs:subClassOf rdf:resource="http://purl.org/agmes/1.1/AgscitationIdentifierScheme" /><rdfs:isDefinedBy rdf:resource="http://purl.org/agmes/1.1/" /><rdfs:seeAlso rdf:resource="http://www.issn.org/" /></rdfs:Class><rdfs:Class rdf:about="http://purl.org/agmes/1.1/CODEN"><rdfs:label xml:lang="en">CODEN </rdfs:label><rdfs:comment xml:lang="en"> A system of alphanumeric codes developed by the American Society for Testing and Materials (ASTM ) to uniquely and permanently identify sci-tech serial and monographic publications. Responsibility for administering the system was transferred to Chemical Abstracts Service (CAS ) in 1975. The CODEN is used in electronic information systems to process bibliographic data because it is more concise than the full title and less ambiguous than an abbreviated title."  </rdfs:comment><rdfs:subClassOf rdf:resource="http://purl.org/agmes/1.1/AgscitationIdentifierScheme" /><rdfs:isDefinedBy rdf:resource="http://purl.org/agmes/1.1/" /></rdfs:Class><!-- Citation refinement : Number --><rdf:Property rdf:about="http://purl.org/agmes/1.1/citationNumber"><rdfs:label xml:lang="en">Number of the issue </rdfs:label><rdfs:comment xml:lang="en">The issue, part or number which denotes a particular issue of a journal, as it appears on the cover. In many cases this indicates a part of a journal volume.</rdfs:comment><rdfs:subPropertyOf rdf:resource="http://purl.org/agmes/1.1/citation" /><rdfs:isDefinedBy rdf:resource="http://purl.org/agmes/1.1/" /></rdf:Property><!-- Citation refinement : Chronology--><rdf:Property rdf:about="http://purl.org/agmes/1.1/citationChronology"><rdfs:label xml:lang="en">Chronological Designation of the issue</rdfs:label><rdfs:comment xml:lang="en">Chronology is the formal date of a particular issue of a journal, as it appears on the cover in conjunction with the serial title.</rdfs:comment><rdfs:subPropertyOf rdf:resource="http://purl.org/agmes/1.1/citation" /><rdfs:isDefinedBy rdf:resource="http://purl.org/agmes/1.1/" /></rdf:Property></rdf:RDF>