<?xml version="1.0" encoding="utf-8"?>
<!DOCTYPE rdf:RDF[
  <!ENTITY label "http://www.w3.org/2004/12/q/contentlabel#">
]>
<!--
  -  Base RDF schema for content labelling vocabularies.
  -  Last Updated: 2005/07/04
 -->
<rdf:RDF xmlns:rdf="http://www.w3.org/1999/02/22-rdf-syntax-ns#"
  xmlns:rdfs="http://www.w3.org/2000/01/rdf-schema#"
  xmlns="http://www.w3.org/2004/12/q/contentlabel#"
  xmlns:label="http://www.w3.org/2004/12/q/contentlabel#"
  xml:base="http://www.w3.org/2004/12/q/contentlabel#">
  <rdfs:Class rdf:ID="ContentLabel">
    <rdfs:label xml:lang="en">Content Label</rdfs:label>
    <rdfs:comment xml:lang="en">
      The type of resource which provides a description of the
      content of one or more resources. A label:ContentLabel consists of one or
      more label:descriptor instances and zero or more label:hasModifier instances.
    </rdfs:comment>
  </rdfs:Class>
  <rdfs:Class rdf:ID="Category">
    <rdfs:label xml:lang="en">Category</rdfs:label>
    <rdfs:comment xml:lang="en">
      A labelling category groups together several descriptions about the same
      kind of content. A label:category instance consists of one or more
      label:descriptor instances.
    </rdfs:comment>
  </rdfs:Class>
  <rdf:Property rdf:ID="descriptor">
    <rdfs:label xml:lang="en">descriptor</rdfs:label>
    <rdfs:domain rdf:resource="#ContentLabel" />
  </rdf:Property>
  <rdf:Property rdf:ID="hasDescriptor">
    <rdfs:label xml:lang="en">has  Descriptor</rdfs:label>
    <rdfs:domain rdf:resource="#Category" />
    <rdfs:range rdf:resource="#descriptor" />
  </rdf:Property>
  <rdf:Property rdf:ID="isMoreSevereThan">
    <rdfs:label xml:lang="en">is More Severe Than</rdfs:label>
    <rdfs:domain rdf:resource="#Category" />
    <rdfs:range rdf:resource="#descriptor" />
  </rdf:Property>
  <!--
    A contentLabel may have an associated modifier. The modifier specifies
    the context(s) that apply to the labelled resource(s).
  -->
  <rdf:Property rdf:ID="hasModifier">
    <rdfs:label xml:lang="en">has Modifier</rdfs:label>
    <rdfs:comment xml:lang="en">
      A contentLabel has an associated modifier. The modifier specifies
      the context(s) that apply to the labelled resource(s).
    </rdfs:comment>
    <rdfs:domain rdf:resource="#ContentLabel" />
    <rdfs:range rdf:resource="#Modifier" />
  </rdf:Property>
  <rdfs:Class rdf:ID="Modifier">
    <rdfs:comment>A contextual modifier for a content label.</rdfs:comment>
  </rdfs:Class>
  <!--
    A resource, or group of resources, may have several Content Labels associated with them via the different predicate arcs:
    - hasDefaultLabel
    - hasLabel
    - hasFrequentScenes
    - hasSeveralScenes
    - hasOccasionalScenes
    - hasSingleScene
  -->
  <rdf:Property rdf:ID="hasDefaultLabel">
    <rdfs:label xml:lang="en">has Default Label</rdfs:label>
    <rdfs:comment xml:lang="en">
      A group of resources may have a default Content Label. Clients SHOULD override a default Content Label
      if a specific label is identified for the same resource group.
    </rdfs:comment>
    <rdfs:range rdf:resource="#ContentLabel" />
  </rdf:Property>
  <rdf:Property rdf:ID="hasLabel">
    <rdfs:label xml:lang="en">has Label</rdfs:label>
    <rdfs:comment xml:lang="en">
      A resource, or group of resources, has an associated Content Label. If the resource has a duration (such as a movie
      or a game) then the description linked by hasLabel will apply throughout. The description may be augmented by
      subsequent frequency modifers.
    </rdfs:comment>
    <rdfs:range rdf:resource="#ContentLabel" />
  </rdf:Property>
  <!-- Analogous properties are provided for management information -->
  <rdf:Property rdf:ID="hasDefaultManagementInfo">
    <rdfs:label xml:lang="en">has Default Management Information</rdfs:label>
    <rdfs:comment xml:lang="en">
      A group of resources may have a default Management Information set. Clients SHOULD override default
      management information if specific information is identified for the same resource group.
    </rdfs:comment>
    <rdfs:range rdf:resource="#ContentLabel" />
  </rdf:Property>
  <rdf:Property rdf:ID="hasManagementInfo">
    <rdfs:label xml:lang="en">has Management Information</rdfs:label>
    <rdfs:comment xml:lang="en">
      A resource, or group of resources, has associated Management Information.
    </rdfs:comment>
    <rdfs:range rdf:resource="#ContentLabel" />
  </rdf:Property>
  <!-- Classification info can be supplied in the same way but note that these do NOT have a range of Content Label -->
  <rdf:Property rdf:ID="hasDefaultClassification">
    <rdfs:label xml:lang="en">has Default Classification</rdfs:label>
    <rdfs:comment xml:lang="en">
      A group of resources may have a default classification. Clients SHOULD override the default
      classification if specific information is identified for the same resource group. This does NOT have a range of Content Label
    </rdfs:comment>
  </rdf:Property>
  <rdf:Property rdf:ID="hasClassification">
    <rdfs:label xml:lang="en">has Classification</rdfs:label>
    <rdfs:comment xml:lang="en">
      A resource, or group of resources, has associated classification.
    </rdfs:comment>
  </rdf:Property>
  <!--
  Frequency modifiers. The following perform the same function as hasLabel in that they associate a content label with
  a resource. However, these give information about the frequency with which the resource is applicable where this is less than
  100% of the time. 
  -->
  <rdf:Property rdf:ID="hasFrequentScenes">
    <rdfs:label xml:lang="en">has Frequent Scenes</rdfs:label>
    <rdfs:comment xml:lang="en">
      A resource such as a movie or game has frequent scenes described by the label linked by this property
    </rdfs:comment>
    <rdfs:range rdf:resource="#ContentLabel" />
  </rdf:Property>
  <rdf:Property rdf:ID="hasSeveralScenes">
    <rdfs:label xml:lang="en">has Several Scenes</rdfs:label>
    <rdfs:comment xml:lang="en">
      A resource such as a movie or game has several scenes described by the label linked by this property
    </rdfs:comment>
    <rdfs:range rdf:resource="#ContentLabel" />
  </rdf:Property>
  <rdf:Property rdf:ID="hasOccasionalScenes">
    <rdfs:label xml:lang="en">has Occasional Scenes</rdfs:label>
    <rdfs:comment xml:lang="en">
      A resource such as a movie or game has occasional scenes described by the label linked by this property
    </rdfs:comment>
    <rdfs:range rdf:resource="#ContentLabel" />
  </rdf:Property>
  <rdf:Property rdf:ID="hasSingleScene">
    <rdfs:label xml:lang="en">has Single Scene</rdfs:label>
    <rdfs:comment xml:lang="en">
      A resource such as a movie or game has a single scene described by the label linked by this property
    </rdfs:comment>
    <rdfs:range rdf:resource="#ContentLabel" />
  </rdf:Property>
  <!-- Rule section -->
  <rdfs:Class rdf:ID="Ruleset">
    <rdfs:label xml:lang="en">Ruleset</rdfs:label>
    <rdfs:comment xml:lang="en">
      The Ruleset Class contains the "global values" for the group. These include the host restrictions, the default descriptions
      and the rules for identifying which URI has which label.
    </rdfs:comment>
  </rdfs:Class>
  <rdf:Property rdf:ID="hasHostRetsrictions">
    <rdfs:label xml:lang="en">hasHostRestrictions</rdfs:label>
    <rdfs:comment xml:lang="en">A property to link a Ruleset to a list of Hosts</rdfs:comment>
    <rdfs:domain rdf:type="#Ruleset" />
    <rdfs:range rdf:type="#Hosts" />
  </rdf:Property>
  <rdfs:Class rdf:ID="Hosts">
    <rdfs:label xml:lang="en">Hosts</rdfs:label>
    <rdfs:comment>A placeholder for a list of hosts for which labelling data is available</rdfs:comment>
    <rdfs:subClassOf rdf:type="#Ruleset" />
  </rdfs:Class>
  <rdf:Property rdf:ID="hostRetsriction">
    <rdfs:label xml:lang="en">A host for which descriptions may be applied</rdfs:label>
    <rdfs:domain rdf:type="#Hosts" />
    <rdfs:range rdf:type="xsd:string" />
  </rdf:Property>
  <rdfs:Class rdf:ID="UnionOf">
    <rdfs:label xml:lang="en">Union Of (logical OR)</rdfs:label>
  </rdfs:Class>
  <rdfs:Class rdf:ID="IntersectionOf">
    <rdfs:label xml:lang="en">Intersection Of (logical AND)</rdfs:label>
  </rdfs:Class>
  <rdf:Property rdf:ID="hasURI">
    <rdfs:label xml:lang="en">has URI</rdfs:label>
    <rdfs:comment xml:lang="en">
      The hasURI property takes a string as its value. This string should be processed as a Perl5 Regular Expression
    </rdfs:comment>
    <rdfs:range rdf:type="xsd:string" />
  </rdf:Property>
  <!-- Label Authority -->
  <rdf:Property rdf:ID="authorityFor">
    <rdfs:label xml:lang="en">authority For</rdfs:label>
    <rdfs:comment xml:lang="en">
      This is used in a description of the RDF instance itself, not the labelled resource. Its value is the namespace of
      the labels about which information concerning the labelling organisation may be obtained. It should be paired with a
      dc:creator property for this purpose.
    </rdfs:comment>
    <rdfs:range rdf:type="xsd:string" />
  </rdf:Property>
</rdf:RDF>