<rdf:RDF xmlns:rdf="http://www.w3.org/1999/02/22-rdf-syntax-ns#" xmlns:rdfs="http://www.w3.org/2000/01/rdf-schema#" xmlns:owl="http://www.w3.org/2002/07/owl#" xmlns:sumo="http://reliant.teknowledge.com/DAML/SUMO.owl#" xmlns="http://reliant.teknowledge.com/DAML/Mid-level-ontology.owl#"><rdfs:Class rdf:ID="Aborting"><rdfs:subClassOf rdf:resource="http://reliant.teknowledge.com/DAML/SUMO.owl#Removing" /><rdfs:comment>Removing a human fetus from a Pregnant woman 

in such a way that the fetus cannot survive.</rdfs:comment></rdfs:Class><rdfs:Class rdf:ID="AcademicDegree"><rdfs:subClassOf rdf:resource="http://reliant.teknowledge.com/DAML/SUMO.owl#Certificate" /><rdfs:comment>A Certificate that demonstrates that the holder 

of the Certificate has successfully completed an EducationalProgram.</rdfs:comment></rdfs:Class><rdfs:Class rdf:ID="Accelerating"><rdfs:subClassOf rdf:resource="http://reliant.teknowledge.com/DAML/SUMO.owl#Translocation" /><rdfs:subClassOf rdf:resource="http://reliant.teknowledge.com/DAML/SUMO.owl#Increasing" /><rdfs:comment>Increasing the speed with which someone 

or something is moving.</rdfs:comment></rdfs:Class><rdfs:Class rdf:ID="Accountant"><rdfs:subClassOf rdf:resource="#Profession" /><rdfs:comment>The Profession of being an Accountant.</rdfs:comment></rdfs:Class><rdfs:Class rdf:ID="Accrediting"><rdfs:subClassOf rdf:resource="http://reliant.teknowledge.com/DAML/SUMO.owl#Declaring" /><rdfs:comment>Any process of certifying an EducationalOrganization.</rdfs:comment></rdfs:Class><rdfs:Class rdf:ID="Acre"><rdfs:subClassOf rdf:resource="http://reliant.teknowledge.com/DAML/SUMO.owl#AreaMeasure" /><rdf:type rdf:resource="http://reliant.teknowledge.com/DAML/SUMO.owl#UnitOfMeasure" /><rdfs:comment>A UnitOfMeasure equal to 4840 square yards.</rdfs:comment></rdfs:Class><rdfs:Class rdf:ID="AcuteAngle"><rdfs:subClassOf rdf:resource="http://reliant.teknowledge.com/DAML/SUMO.owl#TwoDimensionalAngle" /><rdfs:comment>Any TwoDimensionalAngle that has an 

angularMeasure that is less than 90 AngularDegrees.</rdfs:comment></rdfs:Class><rdfs:Class rdf:ID="Address"><rdfs:subClassOf rdf:resource="http://reliant.teknowledge.com/DAML/SUMO.owl#RelationalAttribute" /><rdfs:comment>A RelationalAttribute that indicates an address 

where an Agent can regularly be contacted.</rdfs:comment></rdfs:Class><rdfs:Class rdf:ID="Advertising"><rdfs:subClassOf rdf:resource="http://reliant.teknowledge.com/DAML/SUMO.owl#Disseminating" /><rdfs:comment>A Disseminating whose purpose is to 

promote the sale of an Object represented in a Text or Icon 

(the advertisement).</rdfs:comment></rdfs:Class><rdfs:Class rdf:ID="Aerating"><rdfs:subClassOf rdf:resource="http://reliant.teknowledge.com/DAML/SUMO.owl#Combining" /><rdfs:comment>Combining a substance with Air.</rdfs:comment></rdfs:Class><rdfs:Class rdf:ID="Aerator"><rdfs:subClassOf rdf:resource="http://reliant.teknowledge.com/DAML/SUMO.owl#Device" /><rdfs:comment>A Device whose purpose is to mix Substances with 

Air.</rdfs:comment></rdfs:Class><rdfs:Class rdf:ID="AerobicExerciseDevice"><rdfs:subClassOf rdf:resource="#RecreationOrExerciseDevice" /><rdfs:comment>An RecreationOrExerciseDevice whose purpose is 

to develop the cardiovascular system.</rdfs:comment></rdfs:Class><rdfs:Class rdf:ID="Afternoon"><rdfs:subClassOf rdf:resource="#DayTime" /><rdfs:comment>The class of TimeIntervals that begin at noon and 

end at Sunset.</rdfs:comment></rdfs:Class><rdfs:Class rdf:ID="Agency"><rdfs:subClassOf rdf:resource="http://reliant.teknowledge.com/DAML/SUMO.owl#CommercialAgent" /><rdfs:comment>A CommercialAgent whose customers are all other 

CommercialAgents, e.g. staffing agencies, food-service providers, etc.</rdfs:comment></rdfs:Class><rdfs:Class rdf:about="http://reliant.teknowledge.com/DAML/SUMO.owl#Agent"></rdfs:Class><rdfs:Class rdf:ID="Agriculture"><rdfs:subClassOf rdf:resource="http://reliant.teknowledge.com/DAML/SUMO.owl#Maintaining" /><rdfs:comment>Agriculture is a class of Processes 

in which land, plants, or animals are cultivated in order to produce 

food or other organic products.</rdfs:comment></rdfs:Class><rdfs:Class rdf:ID="AirForce"><rdfs:subClassOf rdf:resource="#MilitaryService" /><rdfs:comment>AirForce is the subclass of MilitaryService 

that comprises military air forces.</rdfs:comment></rdfs:Class><rdfs:Class rdf:ID="AirStream"><rdfs:subClassOf rdf:resource="#FlowRegion" /><rdfs:subClassOf rdf:resource="http://reliant.teknowledge.com/DAML/SUMO.owl#Air" /><rdfs:comment>AirStream is the class of FlowRegions that 

consist of air.</rdfs:comment></rdfs:Class><rdfs:Class rdf:ID="AirTransportation"><rdfs:subClassOf rdf:resource="http://reliant.teknowledge.com/DAML/SUMO.owl#Transportation" /><rdfs:comment>Any instance of Transportation where the 

instrument is an Aircraft and which is through an AtmosphericRegion.</rdfs:comment></rdfs:Class><rdfs:Class rdf:ID="Aircraft"><rdfs:subClassOf rdf:resource="http://reliant.teknowledge.com/DAML/SUMO.owl#Vehicle" /><rdfs:comment>Any Vehicle which is capable of 

AirTransportation.  Note that this class covers both fixed-wing aircraft

and helicopters.</rdfs:comment></rdfs:Class><rdfs:Class rdf:ID="AircraftCarrier"><rdfs:subClassOf rdf:resource="#MilitaryShip" /><rdfs:comment>A MilitaryShip on which MilitaryAircraft can land 

and take off.</rdfs:comment></rdfs:Class><rdfs:Class rdf:ID="Airplane"><rdfs:subClassOf rdf:resource="#Aircraft" /><rdfs:comment>Airplane is the subclass of Aircraft that 

are fixed-wing aircraft which carry their own power sources.  Airplane 

includes jet airplanes and propeller planes, but not gliders.</rdfs:comment></rdfs:Class><rdfs:Class rdf:ID="Airport"><rdfs:subClassOf rdf:resource="#TransitTerminal" /><rdfs:subClassOf rdf:resource="http://reliant.teknowledge.com/DAML/SUMO.owl#LandTransitway" /><rdfs:comment>Airport is the subclass of TransitTerminals 

for Airplanes (fixed-wing Aircraft).</rdfs:comment></rdfs:Class><rdfs:Class rdf:ID="Airway"><rdfs:subClassOf rdf:resource="http://reliant.teknowledge.com/DAML/SUMO.owl#Transitway" /><rdfs:comment>The class of Transitways used to transport Air 

to a location where it is absent or insufficient.</rdfs:comment></rdfs:Class><rdfs:Class rdf:ID="Alcohol"><rdfs:subClassOf rdf:resource="#OrganicCompound" /><rdfs:comment>OrganicCompounds that are produced from hydrocarbons 

by distillation.</rdfs:comment></rdfs:Class><rdfs:Class rdf:ID="AlcoholicBeverage"><rdfs:subClassOf rdf:resource="http://reliant.teknowledge.com/DAML/SUMO.owl#Beverage" /><rdfs:subClassOf rdf:resource="#Depressant" /><rdfs:comment>Any Beverage that contains Alcohol.</rdfs:comment></rdfs:Class><rdfs:Class rdf:ID="Alkaloid"><rdfs:subClassOf rdf:resource="#ChemicalBase" /><rdfs:subClassOf rdf:resource="http://reliant.teknowledge.com/DAML/SUMO.owl#PlantSubstance" /><rdfs:subClassOf rdf:resource="http://reliant.teknowledge.com/DAML/SUMO.owl#BiologicallyActiveSubstance" /><rdfs:comment>A ChemicalBase found in Plants that has 

physiological and psychological effects.</rdfs:comment></rdfs:Class><rdfs:Class rdf:ID="AlphabeticCharacter"><rdfs:subClassOf rdf:resource="http://reliant.teknowledge.com/DAML/SUMO.owl#Character" /><rdfs:comment>Any Character that is comprised of a single 

alphabetical character, e.g. A, B, C, D, ...</rdfs:comment></rdfs:Class><rdfs:Class rdf:ID="Aluminum"><rdfs:subClassOf rdf:resource="http://reliant.teknowledge.com/DAML/SUMO.owl#ElementalSubstance" /><atomicNumber>13</atomicNumber><rdfs:comment>Silvery-white lustrous metallic element of group 

3 of the periodic table.  Highly reactive but protected by a thin 

transparent layer of the oxide which quickly forms in air.  There are many 

alloys of aluminum, as well as a good number of industrial uses.  Makes up 

8.1 percent of the Earth's crust, by weight.  Isolated in 1825 by H.C.  

Oersted.</rdfs:comment></rdfs:Class><rdfs:Class rdf:ID="Alveolus"><rdfs:subClassOf rdf:resource="http://reliant.teknowledge.com/DAML/SUMO.owl#BodyVessel" /><rdfs:subClassOf rdf:resource="http://reliant.teknowledge.com/DAML/SUMO.owl#AnimalAnatomicalStructure" /><rdfs:comment>Tiny sacs in the Lung which absorb Oxygen 

which is delivered to them by the BronchialDucts.</rdfs:comment></rdfs:Class><rdfs:Class rdf:ID="Ambassador"><rdfs:subClassOf rdf:resource="#DiplomaticAgent" /><rdfs:comment>Ambassador is the class of DiplomaticAgents 

that are the most highly-ranked foreign service representatives from the 

government of one country to another.</rdfs:comment></rdfs:Class><rdfs:Class rdf:ID="Ambulance"><rdfs:subClassOf rdf:resource="#EmergencyRoadVehicle" /><rdfs:comment>Ambulance is the subclass of 

EmergencyRoadVehicles that represents ambulances.</rdfs:comment></rdfs:Class><rdfs:Class rdf:ID="Ambush"><rdfs:subClassOf rdf:resource="http://reliant.teknowledge.com/DAML/SUMO.owl#Maneuver" /><rdfs:comment>Any Maneuver in a ViolentContest where one contestParticipant 

attempts to conceal himself from another contestParticipant so that he can Attack the 

other contestParticipant.</rdfs:comment></rdfs:Class><rdfs:Class rdf:ID="AmericanCity"><rdfs:subClassOf rdf:resource="http://reliant.teknowledge.com/DAML/SUMO.owl#City" /><rdfs:comment>The class of cities that are in the 

UnitedStates.</rdfs:comment></rdfs:Class><rdfs:Class rdf:ID="AmericanState"><rdfs:subClassOf rdf:resource="http://reliant.teknowledge.com/DAML/SUMO.owl#StateOrProvince" /><rdfs:comment>The class of states that make up the 

UnitedStates.</rdfs:comment></rdfs:Class><rdfs:Class rdf:ID="AminoAcid"><rdfs:subClassOf rdf:resource="#ChemicalAcid" /><rdfs:subClassOf rdf:resource="#OrganicCompound" /><rdfs:comment>Organic acids that are the building blocks of 

Proteins.</rdfs:comment></rdfs:Class><rdfs:Class rdf:ID="Ampere"><rdfs:subClassOf rdf:resource="http://reliant.teknowledge.com/DAML/SUMO.owl#FunctionQuantity" /><rdf:type rdf:resource="http://reliant.teknowledge.com/DAML/SUMO.owl#SystemeInternationalUnit" /><rdfs:comment>SI electric current measure.  Symbol: A. It is 

one of the base units in SI. It is defined as follows: the Ampere is 

that constant current which, if maintained in two straight parallel 

conductors of infinite length, of negligible circular cross-section, and 

placed 1 Meter apart in a vacuum, would produce between these conductors 

a force equal to 2*10^(-7) Newton per Meter of length.</rdfs:comment></rdfs:Class><rdfs:Class rdf:ID="Amu"><rdfs:subClassOf rdf:resource="http://reliant.teknowledge.com/DAML/SUMO.owl#MassMeasure" /><rdf:type rdf:resource="http://reliant.teknowledge.com/DAML/SUMO.owl#UnitOfMeasure" /><rdfs:comment>Atomic mass unit.  Symbol: u. It is the mass of 

the twelfth part of an atom of the Carbon 12 isotope.</rdfs:comment></rdfs:Class><rdfs:Class rdf:ID="AnaerobicExerciseDevice"><rdfs:subClassOf rdf:resource="#RecreationOrExerciseDevice" /><sumo:disjoint rdf:resource="#AerobicExerciseDevice" /><rdfs:comment>An RecreationOrExerciseDevice whose purpose 

is to develop Muscles without also developing the cardiovascular system.</rdfs:comment></rdfs:Class><rdfs:Class rdf:ID="Anchor"><rdfs:subClassOf rdf:resource="http://reliant.teknowledge.com/DAML/SUMO.owl#AttachingDevice" /><rdfs:comment>An AttachingDevice which is large hook or set of hooks 

that are used to secure a Ship on the open water.</rdfs:comment></rdfs:Class><rdfs:Class rdf:ID="Angstrom"><rdfs:subClassOf rdf:resource="http://reliant.teknowledge.com/DAML/SUMO.owl#LengthMeasure" /><rdf:type rdf:resource="http://reliant.teknowledge.com/DAML/SUMO.owl#UnitOfMeasure" /><rdfs:comment>The Angstrom is a LengthMeasure. 

1 Angstrom = 10^(-10) m</rdfs:comment></rdfs:Class><rdfs:Class rdf:ID="AnimalController"><rdfs:subClassOf rdf:resource="http://reliant.teknowledge.com/DAML/SUMO.owl#Device" /><rdfs:comment>Any Device which is used to control the 

movements of an Animal or Human, e.g. leashes, reins, harnesses, muzzles, 

bridles, shackles, handcuffs, etc.</rdfs:comment></rdfs:Class><rdfs:Class rdf:ID="AnimalPoweredDevice"><rdfs:subClassOf rdf:resource="http://reliant.teknowledge.com/DAML/SUMO.owl#Device" /><rdfs:comment>AnimalPoweredDevice is the subclass 

of Devices that function with power supplied by animals.  Examples: 

oxcarts, horse-drawn plows, mule-driven mills.</rdfs:comment></rdfs:Class><rdfs:Class rdf:ID="AnimalResidence"><rdfs:subClassOf rdf:resource="http://reliant.teknowledge.com/DAML/SUMO.owl#Artifact" /><rdfs:comment>An Artifact which is intended to house 

Animals and not Humans.  Note that an AnimalResidence may or may not 

be a StationaryArtifact, e.g. a horse stall is stationary while a doghouse 

generally is not.</rdfs:comment></rdfs:Class><rdfs:Class rdf:ID="AnimalShell"><rdfs:subClassOf rdf:resource="http://reliant.teknowledge.com/DAML/SUMO.owl#AnimalAnatomicalStructure" /><rdfs:subClassOf rdf:resource="http://reliant.teknowledge.com/DAML/SUMO.owl#BodyPart" /><rdfs:comment>A hard shell of calcium that serves as a 

supporting structure for some Invertebrates.</rdfs:comment></rdfs:Class><rdfs:Class rdf:ID="AnimalTeam"><rdfs:subClassOf rdf:resource="#GroupOfAnimals" /><rdfs:comment>A GroupOfAnimals which are Pulling something.</rdfs:comment></rdfs:Class><rdfs:Class rdf:ID="Ankle"><rdfs:subClassOf rdf:resource="#BodyJoint" /><rdfs:comment>The joint in the Leg that connects the tibia and the 

fibula to the talus.</rdfs:comment></rdfs:Class><rdfs:Class rdf:ID="Announcement"><rdfs:subClassOf rdf:resource="http://reliant.teknowledge.com/DAML/SUMO.owl#FactualText" /><rdfs:comment>Any Text which contains information about 

an event in the future.</rdfs:comment></rdfs:Class><rdfs:Class rdf:ID="Answering"><rdfs:subClassOf rdf:resource="http://reliant.teknowledge.com/DAML/SUMO.owl#Stating" /><rdfs:comment>Responding to a Questioning, i.e. trying to answer 

someone's question.</rdfs:comment></rdfs:Class><rdfs:Class rdf:ID="AntInsect"><rdfs:subClassOf rdf:resource="http://reliant.teknowledge.com/DAML/SUMO.owl#Insect" /><rdfs:comment>A colony Insect of three types:  males, 

QueenInsect, and worker ants.</rdfs:comment></rdfs:Class><rdfs:Class rdf:ID="AnteMeridiem"><rdfs:subClassOf rdf:resource="http://reliant.teknowledge.com/DAML/SUMO.owl#TimeInterval" /><rdfs:comment>The class of TimeIntervals that begin at midnight 

and end at noon.</rdfs:comment></rdfs:Class><rdfs:Class rdf:ID="Antelope"><rdfs:subClassOf rdf:resource="http://reliant.teknowledge.com/DAML/SUMO.owl#HoofedMammal" /><rdfs:comment>A HoofedMammal with long legs and backward-facing horns.  

This class includes gazelles, addax, blackbucks, etc.</rdfs:comment></rdfs:Class><rdfs:Class rdf:ID="Antenna"><rdfs:subClassOf rdf:resource="#CommunicationDevice" /><rdfs:comment>A CommunicationDevice which enables or improves 

the reception of RadioEmissions by another CommunicationDevice (the 

radio or television receiver).</rdfs:comment></rdfs:Class><rdfs:Class rdf:ID="Antibiotic"><rdfs:subClassOf rdf:resource="http://reliant.teknowledge.com/DAML/SUMO.owl#BiologicallyActiveSubstance" /><rdfs:comment>A BiologicallyActiveSubstance than can kill 

instances of Bacterium.</rdfs:comment></rdfs:Class><rdfs:Class rdf:ID="Antibody"><rdfs:subClassOf rdf:resource="http://reliant.teknowledge.com/DAML/SUMO.owl#Protein" /><rdfs:comment>An immunoglobulin which is produced by the body 

and which has the ability to neutralize Antigens.</rdfs:comment></rdfs:Class><rdfs:Class rdf:ID="Antigen"><rdfs:subClassOf rdf:resource="http://reliant.teknowledge.com/DAML/SUMO.owl#BiologicallyActiveSubstance" /><rdfs:comment>Any BiologicallyActiveSubstance that has the 

capacity to stimulate the production of Antibodies.</rdfs:comment></rdfs:Class><rdfs:Class rdf:ID="AntigenA"><rdfs:subClassOf rdf:resource="#Antigen" /><rdfs:comment>An Antigen that is carried in the red blood 

cells of those with BloodTypeA.</rdfs:comment></rdfs:Class><rdfs:Class rdf:ID="AntigenB"><rdfs:subClassOf rdf:resource="#Antigen" /><rdfs:comment>An Antigen that is carried in the red blood 

cells of those with BloodTypeB.</rdfs:comment></rdfs:Class><rdfs:Class rdf:ID="ApartmentBuilding"><rdfs:subClassOf rdf:resource="http://reliant.teknowledge.com/DAML/SUMO.owl#ResidentialBuilding" /><sumo:disjoint rdf:resource="http://reliant.teknowledge.com/DAML/SUMO.owl#SingleFamilyResidence" /><rdfs:comment>A ResidentialBuilding containing 

ApartmentUnits.</rdfs:comment></rdfs:Class><rdfs:Class rdf:ID="ApartmentUnit"><rdfs:subClassOf rdf:resource="http://reliant.teknowledge.com/DAML/SUMO.owl#SingleFamilyResidence" /><rdfs:comment>A SingleFamilyResidence that is not owned 

by any member of the SocialUnit that lives there.</rdfs:comment></rdfs:Class><rdfs:Class rdf:ID="Apple"><rdfs:subClassOf rdf:resource="http://reliant.teknowledge.com/DAML/SUMO.owl#FruitOrVegetable" /><rdfs:subClassOf rdf:resource="http://reliant.teknowledge.com/DAML/SUMO.owl#Food" /><rdfs:comment>A FruitOrVegetable that has a tart to sweet taste and 

a spherical shape.</rdfs:comment></rdfs:Class><rdfs:Class rdf:ID="Application"><rdfs:subClassOf rdf:resource="#FormText" /><rdfs:comment>A FormText whose purpose is to obtain admission 

to an Organization or to receive assistance from an Organization.</rdfs:comment></rdfs:Class><rdfs:Class rdf:ID="Appointing"><rdfs:subClassOf rdf:resource="http://reliant.teknowledge.com/DAML/SUMO.owl#Declaring" /><rdfs:comment>Any instance of Declaring by which the 

patient is assigned to a Position within an Organization where 

the patient previously had no position.  For example, the appointments 

of people to non-elective offices in a government.</rdfs:comment></rdfs:Class><rdfs:Class rdf:ID="Apron"><rdfs:subClassOf rdf:resource="http://reliant.teknowledge.com/DAML/SUMO.owl#Clothing" /><rdfs:comment>An item of Clothing that protects the front and 

middle part of the body while one is Cooking or doing other work.</rdfs:comment></rdfs:Class><rdfs:Class rdf:ID="Argon"><rdfs:subClassOf rdf:resource="http://reliant.teknowledge.com/DAML/SUMO.owl#ElementalSubstance" /><atomicNumber>18</atomicNumber><rdfs:comment>Monatomic noble gas.  Makes up 0.93 percent of the 

air.  Colourless, odorless.  Is inert and has no true compounds.  Lord 

Rayleigh and Sir william Ramsey identified argon in 1894.</rdfs:comment></rdfs:Class><rdfs:Class rdf:ID="Arguing"><rdfs:subClassOf rdf:resource="http://reliant.teknowledge.com/DAML/SUMO.owl#Stating" /><rdfs:comment>Any Stating which has the form of an Argument.</rdfs:comment></rdfs:Class><rdfs:Class rdf:ID="AridClimateZone"><rdfs:subClassOf rdf:resource="#ClimateZone" /><rdfs:comment>AridClimateZone is the 

class of regions in which the climate is characterized by 

a distinct dry season.  Annual rate of moisture evaporation 

exceeds annual rate of precipitation. This is Class B in the 

Koeppen climate system.</rdfs:comment></rdfs:Class><rdfs:Class rdf:ID="Arm"><rdfs:subClassOf rdf:resource="#Limb" /><rdfs:comment>The upper Limbs of a Primate.</rdfs:comment></rdfs:Class><rdfs:Class rdf:ID="Army"><rdfs:subClassOf rdf:resource="#MilitaryService" /><rdfs:comment>MilitaryServices that are land forces.</rdfs:comment></rdfs:Class><rdfs:Class rdf:ID="Arriving"><rdfs:subClassOf rdf:resource="http://reliant.teknowledge.com/DAML/SUMO.owl#Translocation" /><rdfs:comment>The final part of any instance of Translocation.</rdfs:comment></rdfs:Class><rdfs:Class rdf:ID="ArrowFigure"><rdfs:subClassOf rdf:resource="http://reliant.teknowledge.com/DAML/SUMO.owl#Icon" /><rdfs:comment>An Icon which has the shape of an arrow and 

which is used to indicate direction or a relationship betwee two things.</rdfs:comment></rdfs:Class><rdfs:Class rdf:ID="ArrowProjectile"><rdfs:subClassOf rdf:resource="#Projectile" /><rdfs:comment>A long, thin Projectile with a pointed tip is 

fired from a bow.</rdfs:comment></rdfs:Class><rdfs:Class rdf:ID="ArtCritic"><rdfs:subClassOf rdf:resource="#Journalist" /><rdfs:comment>The Profession of reporting and critiquing current 

ArtWorks.</rdfs:comment></rdfs:Class><rdfs:Class rdf:ID="ArtPainting"><rdfs:subClassOf rdf:resource="http://reliant.teknowledge.com/DAML/SUMO.owl#ContentDevelopment" /><rdfs:subClassOf rdf:resource="#Painting" /><rdfs:comment>Any ContentDevelopment that results in a 

PaintedPicture.</rdfs:comment></rdfs:Class><rdfs:Class rdf:ID="ArtSchool"><rdfs:subClassOf rdf:resource="#School" /><rdfs:comment>Any School whose aim is to teach students 

how to create ArtWorks.</rdfs:comment></rdfs:Class><rdfs:Class rdf:ID="ArtStudio"><rdfs:subClassOf rdf:resource="#Workshop" /><rdfs:comment>A Workshop devoted to the creation of ArtWorks.</rdfs:comment></rdfs:Class><rdfs:Class rdf:ID="Artery"><rdfs:subClassOf rdf:resource="#BloodVessel" /><rdfs:comment>Any BloodVessel which transfers Blood from 

the Heart to the extremities of the body.</rdfs:comment></rdfs:Class><rdfs:Class rdf:ID="ArtificialSatellite"><rdfs:subClassOf rdf:resource="#Satellite" /><rdfs:subClassOf rdf:resource="http://reliant.teknowledge.com/DAML/SUMO.owl#Device" /><rdfs:comment>An ArtificialSatellite is a Device

that orbits the earth in space and performs various functions such as

aiding in communication, photographing the earth's surface, and others.</rdfs:comment></rdfs:Class><rdfs:Class rdf:ID="ArtilleryGun"><rdfs:subClassOf rdf:resource="#Gun" /><rdfs:comment>A Gun that is too large to be carried and fired 

by a single Human.  Typically, ArtilleryGuns are on wheels.</rdfs:comment></rdfs:Class><rdfs:Class rdf:ID="Asphalt"><rdfs:subClassOf rdf:resource="#RefinedPetroleumProduct" /><sumo:disjoint rdf:resource="#FossilFuel" /><rdfs:comment>Asphalt is the subclass of 

RefinedPetroleumProducts that are asphalts.</rdfs:comment></rdfs:Class><rdfs:Class rdf:ID="Atmosphere"><rdfs:subClassOf rdf:resource="http://reliant.teknowledge.com/DAML/SUMO.owl#Region" /><rdfs:comment>Atmosphere is a mixture of gases 

surrounding any celestial object that has a gravitational field 

strong enough to prevent the gases from escaping.</rdfs:comment></rdfs:Class><rdfs:Class rdf:ID="AtmosphericPressureMeasure"><rdfs:subClassOf rdf:resource="http://reliant.teknowledge.com/DAML/SUMO.owl#ConstantQuantity" /><rdfs:comment>AtmosphericPressureMeasure is the class 

of UnitsOfMeasure used to measure pressure (barometricPressure), 

e.g., InchMercury.</rdfs:comment></rdfs:Class><rdfs:Class rdf:ID="AtmosphericRegion"><rdfs:subClassOf rdf:resource="#SpaceRegion" /><rdfs:comment>AtmosphericRegion is the class of 

all subregions of EarthsAtmosphere.</rdfs:comment></rdfs:Class><rdfs:Class rdf:ID="AtomGram"><rdfs:subClassOf rdf:resource="http://reliant.teknowledge.com/DAML/SUMO.owl#MassMeasure" /><rdf:type rdf:resource="http://reliant.teknowledge.com/DAML/SUMO.owl#UnitOfMeasure" /><rdfs:comment>MassMeasure that is also known as the gram-atom.  

Defined as the mass in grams of 1 Mole of pure substance.  For example, 

1 AtomGram of Carbon 12 will be 12 Grams of pure Carbon 12.  2 AtomGrams 

of the same substance will be 24 Grams of it.  This is an unusual unit in 

that it is essentially 1 Mole of 'stuff' measured in grams, so that the 

actual value (i.e. mass) depends on the type of substance.</rdfs:comment></rdfs:Class><rdfs:Class rdf:ID="AtomicGroup"><rdfs:subClassOf rdf:resource="http://reliant.teknowledge.com/DAML/SUMO.owl#CompoundSubstance" /><rdfs:comment>Two or more Atoms that are bound together and 

comprise part of a Molecule.</rdfs:comment></rdfs:Class><rdfs:Class rdf:ID="Atrophy"><rdfs:subClassOf rdf:resource="http://reliant.teknowledge.com/DAML/SUMO.owl#PathologicProcess" /><rdfs:subClassOf rdf:resource="http://reliant.teknowledge.com/DAML/SUMO.owl#Decreasing" /><rdfs:comment>Any decrease in the size of an Organ which is due to 

disease or lack of use.</rdfs:comment></rdfs:Class><rdfs:Class rdf:ID="Attorney"><rdfs:subClassOf rdf:resource="#Profession" /><rdfs:comment>The Profession of practicing law, whether as a 

judge or as a legal advocate.</rdfs:comment></rdfs:Class><rdfs:Class rdf:ID="AttorneyGeneral"><rdfs:subClassOf rdf:resource="#Attorney" /><rdfs:subClassOf rdf:resource="#GovernmentOfficer" /><rdfs:comment>The head law officer of a GeopoliticalArea, 

usually a Nation or StateOrProvince.</rdfs:comment></rdfs:Class><rdfs:Class rdf:ID="AudioRecording"><rdfs:subClassOf rdf:resource="http://reliant.teknowledge.com/DAML/SUMO.owl#Text" /><rdfs:comment>Any Text which is a recording of 

RadiatingSound.</rdfs:comment></rdfs:Class><rdfs:Class rdf:ID="Auditorium"><rdfs:subClassOf rdf:resource="http://reliant.teknowledge.com/DAML/SUMO.owl#Building" /><rdfs:comment>Any Building whose purpose is to hold concerts, 

sports events, plays, etc. before an audience.  This class includes theaters, 

sports stadiums, university auditoriums, etc.</rdfs:comment></rdfs:Class><rdfs:Class rdf:ID="AuditoriumSeat"><rdfs:subClassOf rdf:resource="#Seat" /><rdfs:comment>A Seat within an Auditorium from which one 

can observe the PerformanceStage.</rdfs:comment></rdfs:Class><rdfs:Class rdf:ID="AuthorizationOfTransaction"><rdfs:subClassOf rdf:resource="#FinancialService" /><rdfs:subClassOf rdf:resource="http://reliant.teknowledge.com/DAML/SUMO.owl#RegulatoryProcess" /><rdfs:comment>An activity which approves or 

disapproves a transaction.</rdfs:comment></rdfs:Class><rdfs:Class rdf:ID="AutomaticGun"><rdfs:subClassOf rdf:resource="#Gun" /><rdfs:comment>A Gun that fires a burst of Projectiles 

with each pull of the trigger.  Also known as a machine gun.</rdfs:comment></rdfs:Class><rdfs:Class rdf:ID="Automobile"><rdfs:subClassOf rdf:resource="#SelfPoweredRoadVehicle" /><rdfs:comment>Automobile is a subclass of 

SelfPoweredRoadVehicles including passenger cars, family vans, light 

trucks, and sport utility vehicles.  In general, this class covers 

four-wheeled passenger road vehicles.</rdfs:comment></rdfs:Class><rdfs:Class rdf:ID="Avocado"><rdfs:subClassOf rdf:resource="http://reliant.teknowledge.com/DAML/SUMO.owl#FruitOrVegetable" /><rdfs:subClassOf rdf:resource="http://reliant.teknowledge.com/DAML/SUMO.owl#Food" /><rdfs:comment>A FruitOrVegetable that is shaped like a pear and 

has a dark green skin and a rich meat.</rdfs:comment></rdfs:Class><rdfs:Class rdf:ID="Axle"><rdfs:subClassOf rdf:resource="http://reliant.teknowledge.com/DAML/SUMO.owl#Device" /><rdfs:comment>Axle is a class of Devices each of which can 

be paired with two VehicleWheels to rotate and move a RoadVehicle.</rdfs:comment></rdfs:Class><rdfs:Class rdf:ID="BacterialDisease"><rdfs:subClassOf rdf:resource="#InfectiousDisease" /><rdfs:comment>A disease that is caused by instances of 

Bacterium.</rdfs:comment></rdfs:Class><rdfs:Class rdf:ID="Bag"><rdfs:subClassOf rdf:resource="#Container" /><rdfs:comment>Any Container which is made of Fabric.</rdfs:comment></rdfs:Class><rdfs:Class rdf:ID="Baking"><rdfs:subClassOf rdf:resource="http://reliant.teknowledge.com/DAML/SUMO.owl#Cooking" /><rdfs:subClassOf rdf:resource="http://reliant.teknowledge.com/DAML/SUMO.owl#Heating" /><rdfs:comment>Any instance of Cooking where the instrument 

is an Oven.</rdfs:comment></rdfs:Class><rdfs:Class rdf:ID="Ball"><rdfs:subClassOf rdf:resource="#GamePiece" /><rdfs:comment>Any GamePiece which has the shape of a sphere.</rdfs:comment></rdfs:Class><rdfs:Class rdf:ID="BallisticMissile"><rdfs:subClassOf rdf:resource="#Missile" /><rdfs:comment>A Missile which is guided for the first stage 

of its flight but then falls to its target for the second stage.</rdfs:comment></rdfs:Class><rdfs:Class rdf:ID="Ballot"><rdfs:subClassOf rdf:resource="#FormText" /><rdfs:comment>A FormText which is used in Voting.  A list of 

candidates is printed on the form, and the voter selects the candidate he/she 

wants to vote for.</rdfs:comment></rdfs:Class><rdfs:Class rdf:ID="Bandage"><rdfs:subClassOf rdf:resource="#FabricArtifact" /><rdfs:comment>A piece of Fabric that is used to cover an 

open wound.</rdfs:comment></rdfs:Class><rdfs:Class rdf:ID="Banker"><rdfs:subClassOf rdf:resource="#SkilledOccupation" /><rdfs:comment>Any SkilledOccupation which involves working in a 

FinancialBank.</rdfs:comment></rdfs:Class><rdfs:Class rdf:ID="Baptizing"><rdfs:subClassOf rdf:resource="http://reliant.teknowledge.com/DAML/SUMO.owl#ReligiousProcess" /><rdfs:subClassOf rdf:resource="http://reliant.teknowledge.com/DAML/SUMO.owl#JoiningAnOrganization" /><rdfs:comment>A ReligiousProcess which marks the acceptance of 

the person being baptized into the ReligiousOrganization.</rdfs:comment></rdfs:Class><rdfs:Class rdf:ID="BargainSale"><rdfs:subClassOf rdf:resource="#OfferingForSale" /><rdfs:comment>Offering to sell something to someone at a 

reduced price.</rdfs:comment></rdfs:Class><rdfs:Class rdf:ID="Barking"><rdfs:subClassOf rdf:resource="http://reliant.teknowledge.com/DAML/SUMO.owl#RadiatingSound" /><rdfs:comment>Any instance of RadiatingSound which is produced 

by a Canine.</rdfs:comment></rdfs:Class><rdfs:Class rdf:ID="Baseball"><rdfs:subClassOf rdf:resource="#TeamSport" /><rdfs:comment>A TeamSport which involves two teams of 9 players 

each that take turns at bat and attempt to score runs.  Note that each instance 

of Baseball is a baseball game.</rdfs:comment></rdfs:Class><rdfs:Class rdf:ID="BaseballBase"><rdfs:subClassOf rdf:resource="#GameArtifact" /><rdfs:comment>Any of four regions which must each be 

successively touched after a BaseballHit in order to complete a 

BaseballRun.</rdfs:comment></rdfs:Class><rdfs:Class rdf:ID="BaseballBat"><rdfs:subClassOf rdf:resource="#GameArtifact" /><rdfs:comment>A bat which is used to hit the ball in 

Baseball.</rdfs:comment></rdfs:Class><rdfs:Class rdf:ID="BaseballDugout"><rdfs:subClassOf rdf:resource="http://reliant.teknowledge.com/DAML/SUMO.owl#Building" /><rdfs:comment>A Building which is used to house the members 

of both Baseball teams while a game is being played.</rdfs:comment></rdfs:Class><rdfs:Class rdf:ID="BaseballField"><rdfs:subClassOf rdf:resource="#SportsFacility" /><rdfs:comment>A SportsFacility which is dedicated to 

Baseball.</rdfs:comment></rdfs:Class><rdfs:Class rdf:ID="BaseballHit"><rdfs:subClassOf rdf:resource="#GameShot" /><rdfs:subClassOf rdf:resource="#BaseballManeuver" /><rdfs:comment>Any base hit in Baseball.</rdfs:comment></rdfs:Class><rdfs:Class rdf:ID="BaseballInning"><rdfs:subClassOf rdf:resource="#BaseballManeuver" /><rdfs:comment>A division of a Baseball game.  A normal game 

consists of 9 innings, and each inning involves a turn a bat for both teams.</rdfs:comment></rdfs:Class><rdfs:Class rdf:ID="BaseballManeuver"><rdfs:subClassOf rdf:resource="http://reliant.teknowledge.com/DAML/SUMO.owl#Maneuver" /><rdfs:comment>Any Maneuver in Baseball.</rdfs:comment></rdfs:Class><rdfs:Class rdf:ID="BaseballRun"><rdfs:subClassOf rdf:resource="#BaseballHit" /><rdfs:subClassOf rdf:resource="#Score" /><rdfs:comment>A Score in Baseball.  It consists of hitting 

the ball with the bat and then touching all four bases of the diamond before 

being tagged with the ball by a member of the opposite team.</rdfs:comment></rdfs:Class><rdfs:Class rdf:ID="BaseballSingle"><rdfs:subClassOf rdf:resource="#BaseballHit" /><rdfs:comment>Any BaseballHit where the batter makes it 

safely to first base by hitting the ball.</rdfs:comment></rdfs:Class><rdfs:Class rdf:ID="BaseballSteal"><rdfs:subClassOf rdf:resource="#BaseballManeuver" /><sumo:disjoint rdf:resource="#BaseballWalk" /><sumo:disjoint rdf:resource="#BaseballHit" /><rdfs:comment>Any move from one base to another which is neither 

a BaseballWalk nor a BaseballHit.</rdfs:comment></rdfs:Class><rdfs:Class rdf:ID="BaseballTeam"><rdfs:subClassOf rdf:resource="#SportsTeam" /><rdfs:comment>The class of SportsTeams that play Baseball.</rdfs:comment></rdfs:Class><rdfs:Class rdf:ID="BaseballWalk"><rdfs:subClassOf rdf:resource="#BaseballManeuver" /><sumo:disjoint rdf:resource="#BaseballHit" /><rdfs:comment>Taking first base after four balls have been 

called by the umpire.</rdfs:comment></rdfs:Class><rdfs:Class rdf:ID="Basement"><rdfs:subClassOf rdf:resource="#BuildingLevel" /><rdfs:comment>A BuildingLevel which satisfies two conditions, viz. it is 

lower than all of the other BuildingLevels in the same Building and it is below 

ground level.</rdfs:comment></rdfs:Class><rdfs:Class rdf:ID="Basketball"><rdfs:subClassOf rdf:resource="#TeamSport" /><rdfs:comment>A TeamSport which involves two teams of 5 players 

each.  The object of the game is to put the ball through a hoop.</rdfs:comment></rdfs:Class><rdfs:Class rdf:ID="Bathing"><rdfs:subClassOf rdf:resource="#Washing" /><rdfs:comment>Washing the entire body of a Human or Animal.</rdfs:comment></rdfs:Class><rdfs:Class rdf:ID="BathingDevice"><rdfs:subClassOf rdf:resource="#WashingDevice" /><rdfs:comment>A WashingDevice which is intended to be used by 

Humans for washing their bodies.  Note that this class covers bathtubs, showers, 

etc.</rdfs:comment></rdfs:Class><rdfs:Class rdf:ID="Bathroom"><rdfs:subClassOf rdf:resource="http://reliant.teknowledge.com/DAML/SUMO.owl#Room" /><rdfs:comment>A Room that contains a WashBasin and 

possibly a Toilet.</rdfs:comment></rdfs:Class><rdfs:Class rdf:ID="Baton"><rdfs:subClassOf rdf:resource="http://reliant.teknowledge.com/DAML/SUMO.owl#Device" /><rdfs:comment>A thin stick which is used for OrchestralConducting.</rdfs:comment></rdfs:Class><rdfs:Class rdf:ID="Battery"><rdfs:subClassOf rdf:resource="http://reliant.teknowledge.com/DAML/SUMO.owl#Device" /><rdfs:comment>Battery is a subclass of Device.  Batteries are 

devices that use chemical means to store or produce electrical power.</rdfs:comment></rdfs:Class><rdfs:Class rdf:ID="BecomingDrunk"><rdfs:subClassOf rdf:resource="http://reliant.teknowledge.com/DAML/SUMO.owl#PsychologicalProcess" /><sumo:disjoint rdf:resource="#SoberingUp" /><rdfs:comment>The process of transitioning from a state of 

being Sober to a state of being Drunk.</rdfs:comment></rdfs:Class><rdfs:Class rdf:ID="Becquerel"><rdfs:subClassOf rdf:resource="http://reliant.teknowledge.com/DAML/SUMO.owl#TimeDependentQuantity" /><rdf:type rdf:resource="http://reliant.teknowledge.com/DAML/SUMO.owl#SystemeInternationalUnit" /><rdfs:comment>SI activity measure.  Symbol: Bq.  It measures 

the amount of radioactivity contained in a given sample of matter. It is 

that quantity of a radioactive element in which there is one atomic 

disintegration per SecondDuration.  Becquerel = s^(-1).</rdfs:comment></rdfs:Class><rdfs:Class rdf:ID="Bed"><rdfs:subClassOf rdf:resource="#Furniture" /><rdfs:comment>A piece of Furniture which is primarily for sleeping.</rdfs:comment></rdfs:Class><rdfs:Class rdf:ID="Bedroom"><rdfs:subClassOf rdf:resource="http://reliant.teknowledge.com/DAML/SUMO.owl#Room" /><rdfs:comment>A Room intended primarily for sleeping.</rdfs:comment></rdfs:Class><rdfs:Class rdf:ID="Bee"><rdfs:subClassOf rdf:resource="http://reliant.teknowledge.com/DAML/SUMO.owl#Insect" /><rdfs:comment>A hairy Insect, some species of which produce honey 

and/or sting.</rdfs:comment></rdfs:Class><rdfs:Class rdf:ID="Beef"><rdfs:subClassOf rdf:resource="http://reliant.teknowledge.com/DAML/SUMO.owl#Meat" /><rdfs:comment>Meat that was originally part of a Cow.</rdfs:comment></rdfs:Class><rdfs:Class rdf:ID="Beer"><rdfs:subClassOf rdf:resource="#AlcoholicBeverage" /><rdfs:comment>An AlcoholicBeverage that is prepared by fermenting 

malt and hops.</rdfs:comment></rdfs:Class><rdfs:Class rdf:ID="BeginningOperations"><rdfs:subClassOf rdf:resource="http://reliant.teknowledge.com/DAML/SUMO.owl#OrganizationalProcess" /><sumo:disjoint rdf:resource="#CeasingOperations" /><rdfs:comment>The process of an Organization 

commencing operations.  In the case of a Corporation, this would be 

the process of going into business.</rdfs:comment></rdfs:Class><rdfs:Class rdf:ID="Bell"><rdfs:subClassOf rdf:resource="#PercussionInstrument" /><rdfs:comment>A PercussionInstrument which is made of Metal and 

which produces a single tone when it is struck.</rdfs:comment></rdfs:Class><rdfs:Class rdf:ID="Belt"><rdfs:subClassOf rdf:resource="http://reliant.teknowledge.com/DAML/SUMO.owl#Clothing" /><rdfs:comment>A piece of Clothing that is worn around the waist 

of a pair of Trousers.</rdfs:comment></rdfs:Class><rdfs:Class rdf:ID="Bequeathing"><rdfs:subClassOf rdf:resource="http://reliant.teknowledge.com/DAML/SUMO.owl#UnilateralGiving" /><rdfs:comment>Any UnilateralGiving where the agent 

wills some part of his/her property to someone else upon his/her death.</rdfs:comment></rdfs:Class><rdfs:Class rdf:ID="Bicycle"><rdfs:subClassOf rdf:resource="#Cycle-TransportationDevice" /><rdfs:comment>Bicycle is a class of two-wheeled, 

UserPoweredVehicles.</rdfs:comment></rdfs:Class><rdfs:Class rdf:ID="BiochemicalAgent"><rdfs:subClassOf rdf:resource="http://reliant.teknowledge.com/DAML/SUMO.owl#SelfConnectedObject" /><rdfs:comment>A BiologicalAgent or a ChemicalAgent.</rdfs:comment></rdfs:Class><rdfs:Class rdf:ID="BiochemicalAttack"><rdfs:subClassOf rdf:resource="http://reliant.teknowledge.com/DAML/SUMO.owl#Attack" /><rdfs:comment>Attacks in which a BiochemicalWeapon 

is used against an Organism.</rdfs:comment></rdfs:Class><rdfs:Class rdf:ID="BiochemicalWeapon"><rdfs:subClassOf rdf:resource="#WeaponOfMassDestruction" /><rdfs:comment>A WeaponOfMassDestruction that is 

either a BiologicalWeapon or a ChemicalWeapon, i.e. not a 

RadioactiveWeapon.</rdfs:comment></rdfs:Class><rdfs:Class rdf:ID="Biography"><rdfs:subClassOf rdf:resource="#HistoricalAccount" /><rdfs:comment>A HistoricalAccount which is concerned 

with the life of a single Human.</rdfs:comment></rdfs:Class><rdfs:Class rdf:ID="BiologicalAgent"><rdfs:subClassOf rdf:resource="#BiochemicalAgent" /><rdfs:comment>A naturally occurring Substance, a 

synthetic analogue of such a substance or an Organism that is capable 

of inflicting severe harm on other Organisms.  All BiologicalWeapons 

contain a BiologicalAgent.</rdfs:comment></rdfs:Class><rdfs:Class rdf:ID="BiologicalConception"><rdfs:subClassOf rdf:resource="http://reliant.teknowledge.com/DAML/SUMO.owl#OrganOrTissueProcess" /><rdfs:comment>The production of a zygote from the fusion 

of a male and female gamete.</rdfs:comment></rdfs:Class><rdfs:Class rdf:ID="BiologicalSpecies"><rdfs:subClassOf rdf:resource="http://reliant.teknowledge.com/DAML/SUMO.owl#Class" /><rdfs:comment>The Class of all biological species, i.e. 

the class of all classes of Organism whose instances can interbreed.</rdfs:comment></rdfs:Class><rdfs:Class rdf:ID="BiologicalWeapon"><rdfs:subClassOf rdf:resource="#BiochemicalWeapon" /><rdfs:comment>Weapons which contain a sample of 

ToxicOrganism or a BiologicallyActiveSubstance that is produced by a 

ToxicOrganism (or a synthetic analogue of the latter).</rdfs:comment></rdfs:Class><rdfs:Class rdf:ID="Biopsy"><rdfs:subClassOf rdf:resource="http://reliant.teknowledge.com/DAML/SUMO.owl#DiagnosticProcess" /><rdfs:comment>Any DiagnosticProcess which involves the examination of 

BodySubstances taken from a living Organism.</rdfs:comment></rdfs:Class><rdfs:Class rdf:ID="BirdEgg"><rdfs:subClassOf rdf:resource="http://reliant.teknowledge.com/DAML/SUMO.owl#Egg" /><rdfs:comment>Any Egg that is produced by a Bird.</rdfs:comment></rdfs:Class><rdfs:Class rdf:ID="Biting"><rdfs:subClassOf rdf:resource="http://reliant.teknowledge.com/DAML/SUMO.owl#Grabbing" /><rdfs:comment>Any instance of Grabbing where the instrument is 

the Mouth of the agent.</rdfs:comment></rdfs:Class><rdfs:Class rdf:ID="Blanket"><rdfs:subClassOf rdf:resource="#FabricArtifact" /><rdfs:comment>An Artifact made of Fabric whose function is 

to cover a sleeping person while he/she sleeps.</rdfs:comment></rdfs:Class><rdfs:Class rdf:ID="Bleeding"><rdfs:subClassOf rdf:resource="http://reliant.teknowledge.com/DAML/SUMO.owl#AutonomicProcess" /><rdfs:comment>The release of Blood from an Animal in response 

to an Injuring of some sort.</rdfs:comment></rdfs:Class><rdfs:Class rdf:ID="Bloating"><rdfs:subClassOf rdf:resource="http://reliant.teknowledge.com/DAML/SUMO.owl#Increasing" /><rdfs:subClassOf rdf:resource="http://reliant.teknowledge.com/DAML/SUMO.owl#PathologicProcess" /><rdfs:comment>Any Process where the stomach or instestines of a 

Human or Animal become distended from excessive gas.</rdfs:comment></rdfs:Class><rdfs:Class rdf:ID="Blockade"><rdfs:subClassOf rdf:resource="http://reliant.teknowledge.com/DAML/SUMO.owl#Maneuver" /><rdfs:comment>Any Maneuver in a Contest where one contestParticipant 

attempts to deny access to something that is wanted by another contestParticipant.</rdfs:comment></rdfs:Class><rdfs:Class rdf:ID="BloodCell"><rdfs:subClassOf rdf:resource="http://reliant.teknowledge.com/DAML/SUMO.owl#Cell" /><rdfs:subClassOf rdf:resource="http://reliant.teknowledge.com/DAML/SUMO.owl#AnimalAnatomicalStructure" /><rdfs:comment>A Cell that is normally present in Blood.</rdfs:comment></rdfs:Class><rdfs:Class rdf:ID="BloodTypeA"><rdfs:subClassOf rdf:resource="http://reliant.teknowledge.com/DAML/SUMO.owl#Blood" /><rdfs:comment>The subclass of Blood that contains AntigenA 

and does not contain AntigenB.</rdfs:comment></rdfs:Class><rdfs:Class rdf:ID="BloodTypeAB"><rdfs:subClassOf rdf:resource="http://reliant.teknowledge.com/DAML/SUMO.owl#Blood" /><rdfs:comment>The subclass of Blood that contains both 

AntigenA and AntigenB.</rdfs:comment></rdfs:Class><rdfs:Class rdf:ID="BloodTypeB"><rdfs:subClassOf rdf:resource="http://reliant.teknowledge.com/DAML/SUMO.owl#Blood" /><rdfs:comment>The subclass of Blood that contains AntigenB 

and does not contain AntigenA.</rdfs:comment></rdfs:Class><rdfs:Class rdf:ID="BloodTypeO"><rdfs:subClassOf rdf:resource="http://reliant.teknowledge.com/DAML/SUMO.owl#Blood" /><rdfs:comment>The subclass of Blood that contains neither 

AntigenA nor AntigenB.</rdfs:comment></rdfs:Class><rdfs:Class rdf:ID="BloodVessel"><rdfs:subClassOf rdf:resource="http://reliant.teknowledge.com/DAML/SUMO.owl#BodyVessel" /><rdfs:subClassOf rdf:resource="http://reliant.teknowledge.com/DAML/SUMO.owl#AnimalAnatomicalStructure" /><rdfs:comment>Any BodyVessel which is used to circulate 

Blood from one part of the body to another.</rdfs:comment></rdfs:Class><rdfs:Class rdf:ID="Blueprint"><rdfs:subClassOf rdf:resource="http://reliant.teknowledge.com/DAML/SUMO.owl#Icon" /><rdfs:comment>An Icon which is a scale model of an Artifact, 

whether the Artifact actually exists or not.</rdfs:comment></rdfs:Class><rdfs:Class rdf:ID="Blushing"><rdfs:subClassOf rdf:resource="http://reliant.teknowledge.com/DAML/SUMO.owl#AutonomicProcess" /><rdfs:comment>The process of turning red in response to a 

stimulus which has a deep emotional effect.</rdfs:comment></rdfs:Class><rdfs:Class rdf:ID="BoardOrBlock"><rdfs:subClassOf rdf:resource="http://reliant.teknowledge.com/DAML/SUMO.owl#Artifact" /><rdfs:comment>A piece of material with flat, rectangular sides.  

Note that boards and blocks are lumped into a single concept, because the 

difference between these notions cannot be precisely defined.</rdfs:comment></rdfs:Class><rdfs:Class rdf:ID="Boarding"><rdfs:subClassOf rdf:resource="http://reliant.teknowledge.com/DAML/SUMO.owl#Translocation" /><rdfs:comment>Getting on a Vehicle, e.g. getting into an 

Automobile, boarding an Aircraft, etc.</rdfs:comment></rdfs:Class><rdfs:Class rdf:ID="BoatDeck"><rdfs:subClassOf rdf:resource="http://reliant.teknowledge.com/DAML/SUMO.owl#Artifact" /><rdfs:comment>One of the levels of a Watercraft, e.g. the 

upper deck and lower deck of small boats with a cabin.</rdfs:comment></rdfs:Class><rdfs:Class rdf:ID="BodyJoint"><rdfs:subClassOf rdf:resource="http://reliant.teknowledge.com/DAML/SUMO.owl#AnimalAnatomicalStructure" /><rdfs:comment>BodyJunctions where different parts of the same 

Skeleton come together.</rdfs:comment></rdfs:Class><rdfs:Class rdf:ID="BodyOfWater"><rdfs:subClassOf rdf:resource="http://reliant.teknowledge.com/DAML/SUMO.owl#WaterArea" /><rdfs:subClassOf rdf:resource="http://reliant.teknowledge.com/DAML/SUMO.owl#SelfConnectedObject" /><rdfs:comment>A BodyOfWater is a connected body of 

water with established boundaries marked by either geographical features 

or conventional borders.</rdfs:comment></rdfs:Class><rdfs:Class rdf:ID="Bodybuilding"><rdfs:subClassOf rdf:resource="http://reliant.teknowledge.com/DAML/SUMO.owl#Sport" /><rdfs:comment>A sport which involves the development of one's 

Muscles and competition against other bodybuilders.</rdfs:comment></rdfs:Class><rdfs:Class rdf:ID="Bomber"><rdfs:subClassOf rdf:resource="#MilitaryAircraft" /><rdfs:comment>Any MilitaryAircraft whose purpose is to deliver 

ExplosiveDevices.</rdfs:comment></rdfs:Class><rdfs:Class rdf:ID="Bond"><rdfs:subClassOf rdf:resource="http://reliant.teknowledge.com/DAML/SUMO.owl#FinancialInstrument" /><rdfs:comment>A debt instrument issued for a period of more than one year with 

the purpose of raising capital by borrowing. The Federal government, states, cities, 

corporations, and many other types of institutions sell bonds. A bond is generally a 

promise to repay the principal along with interest on a specified maturityDate.</rdfs:comment></rdfs:Class><rdfs:Class rdf:ID="BotanicalTree"><rdfs:subClassOf rdf:resource="http://reliant.teknowledge.com/DAML/SUMO.owl#FloweringPlant" /><rdfs:comment>BotanicalTree is an imprecise term 

for a perennial woody plant that is larger than a bush or shrub, 

generally understood to describe a large growth having one main trunk 

with few or no branches projecting from its base, a well-developed crown 

of foliage, and a height at maturity of at least 12 feet.</rdfs:comment></rdfs:Class><rdfs:Class rdf:ID="Bottle"><rdfs:subClassOf rdf:resource="#FluidContainer" /><rdfs:comment>A Container whose top is narrower than its bottom, 

which has no handle, and which is intended to store Liquids.</rdfs:comment></rdfs:Class><rdfs:Class rdf:ID="Bowing"><rdfs:subClassOf rdf:resource="#Inclining" /><rdfs:subClassOf rdf:resource="http://reliant.teknowledge.com/DAML/SUMO.owl#Gesture" /><rdfs:comment>Any downward motion of the body that indicates respect 

for or submission to another Agent.</rdfs:comment></rdfs:Class><rdfs:Class rdf:ID="Box"><rdfs:subClassOf rdf:resource="#Container" /><rdfs:comment>Any six-sided Container whose sides are 

rectangular in shape.</rdfs:comment></rdfs:Class><rdfs:Class rdf:ID="Boxcar"><rdfs:subClassOf rdf:resource="#FreightCar" /><rdfs:comment>Boxcar is the subclass of Railcars that are 

general-purpose closed cars for hauling freight.</rdfs:comment></rdfs:Class><rdfs:Class rdf:ID="Boxing"><rdfs:subClassOf rdf:resource="http://reliant.teknowledge.com/DAML/SUMO.owl#ViolentContest" /><rdfs:subClassOf rdf:resource="http://reliant.teknowledge.com/DAML/SUMO.owl#Sport" /><rdfs:comment>A sport which involves two participants who try to 

knock each other out in a limited number of rounds.  Note that each instance 

of Boxing is a boxing match.</rdfs:comment></rdfs:Class><rdfs:Class rdf:ID="Boy"><rdfs:subClassOf rdf:resource="#HumanChild" /><rdfs:subClassOf rdf:resource="http://reliant.teknowledge.com/DAML/SUMO.owl#Man" /><rdfs:comment>A HumanChild who is Male.</rdfs:comment></rdfs:Class><rdfs:Class rdf:ID="Brain"><rdfs:subClassOf rdf:resource="http://reliant.teknowledge.com/DAML/SUMO.owl#Organ" /><rdfs:subClassOf rdf:resource="http://reliant.teknowledge.com/DAML/SUMO.owl#AnimalAnatomicalStructure" /><rdfs:comment>The seat of the central nervous system.</rdfs:comment></rdfs:Class><rdfs:Class rdf:ID="Brandy"><rdfs:subClassOf rdf:resource="#DistilledAlcoholicBeverage" /><rdfs:comment>A DistilledAlcoholicBeverage that is prepared by 

distilling Wine.</rdfs:comment></rdfs:Class><rdfs:Class rdf:ID="Brass"><rdfs:subClassOf rdf:resource="#MetallicAlloy" /><rdfs:comment>A MetallicAlloy made from Copper and Zinc.</rdfs:comment></rdfs:Class><rdfs:Class rdf:ID="BreadOrBiscuit"><rdfs:subClassOf rdf:resource="#PreparedFood" /><rdfs:comment>Food that consists largely of grain flour 

and water.  Note that this class covers crackers, cookies, as well as any 

self-connected instance of bread, whether it is a loaf, a slice, a chunk 

of bread, etc.</rdfs:comment></rdfs:Class><rdfs:Class rdf:ID="BreakabilityAttribute"><rdfs:subClassOf rdf:resource="http://reliant.teknowledge.com/DAML/SUMO.owl#InternalAttribute" /><rdfs:comment>A subclass of Attributes for 

characterizing the breakability of CorpuscularObjects.</rdfs:comment></rdfs:Class><rdfs:Class rdf:ID="Breast"><rdfs:subClassOf rdf:resource="http://reliant.teknowledge.com/DAML/SUMO.owl#AnimalAnatomicalStructure" /><rdfs:subClassOf rdf:resource="http://reliant.teknowledge.com/DAML/SUMO.owl#Organ" /><rdfs:comment>The paired Organs which are part of the chests 

of Primates.</rdfs:comment></rdfs:Class><rdfs:Class rdf:ID="Brick"><rdfs:subClassOf rdf:resource="#BoardOrBlock" /><rdfs:comment>A block of fired Clay that is used in Constructing.</rdfs:comment></rdfs:Class><rdfs:Class rdf:ID="Bridge"><rdfs:subClassOf rdf:resource="http://reliant.teknowledge.com/DAML/SUMO.owl#LandTransitway" /><rdfs:subClassOf rdf:resource="http://reliant.teknowledge.com/DAML/SUMO.owl#StationaryArtifact" /><rdfs:comment>Bridge is the subclass of LandTransitways 

that are artifacts used for crossing water or air-filled gaps that 

could not be transited over a natural surface.</rdfs:comment></rdfs:Class><rdfs:Class rdf:ID="BrigadierGeneral"><rdfs:subClassOf rdf:resource="#MilitaryGeneral" /><rdfs:comment>A MilitaryGeneral that ranks below 

a MajorGeneral.</rdfs:comment></rdfs:Class><rdfs:Class rdf:ID="BroadcastNetwork"><rdfs:subClassOf rdf:resource="#CommunicationSystem" /><rdfs:comment>BroadcastNetwork is the subclass of 

CommunicationSystems consisting of BroadcastingStations that are linked 

electronically and managed or owned by one organization.</rdfs:comment></rdfs:Class><rdfs:Class rdf:ID="BroadcastProgram"><rdfs:subClassOf rdf:resource="http://reliant.teknowledge.com/DAML/SUMO.owl#Series" /><rdfs:comment>A Series of episodes that are broadcast 

on television or radio.</rdfs:comment></rdfs:Class><rdfs:Class rdf:ID="Broadcasting"><rdfs:subClassOf rdf:resource="http://reliant.teknowledge.com/DAML/SUMO.owl#Disseminating" /><rdfs:subClassOf rdf:resource="#RadioEmission" /><rdfs:comment>Disseminating information by using a 

CommunicationDevice that radiates RadioEmissions.</rdfs:comment></rdfs:Class><rdfs:Class rdf:ID="BroadcastingStation"><rdfs:subClassOf rdf:resource="http://reliant.teknowledge.com/DAML/SUMO.owl#StationaryArtifact" /><rdfs:subClassOf rdf:resource="#CommunicationDevice" /><rdfs:comment>A BroadcastingStation is

a TelevisionStation or a RadioStation.</rdfs:comment></rdfs:Class><rdfs:Class rdf:ID="BronchialDuct"><rdfs:subClassOf rdf:resource="http://reliant.teknowledge.com/DAML/SUMO.owl#BodyVessel" /><rdfs:subClassOf rdf:resource="http://reliant.teknowledge.com/DAML/SUMO.owl#AnimalAnatomicalStructure" /><rdfs:comment>Any BodyVessel which is located in a 

Lung and which carries oxygen from the trachea to the alveoli.</rdfs:comment></rdfs:Class><rdfs:Class rdf:ID="Brood"><rdfs:subClassOf rdf:resource="#GroupOfAnimals" /><rdfs:comment>A GroupOfAnimals that are all born at the same time 

and to the same parents.</rdfs:comment></rdfs:Class><rdfs:Class rdf:ID="Broom"><rdfs:subClassOf rdf:resource="#BrushOrComb" /><rdfs:comment>A BrushOrComb whose purpose is to remove dirt and other 

small particles from floors.</rdfs:comment></rdfs:Class><rdfs:Class rdf:ID="BrushOrComb"><rdfs:subClassOf rdf:resource="http://reliant.teknowledge.com/DAML/SUMO.owl#Device" /><rdfs:comment>A Device which consists of a handle and bristles and 

whose purpose is to remove particles from something or to smooth something out.</rdfs:comment></rdfs:Class><rdfs:Class rdf:ID="Bubble"><rdfs:subClassOf rdf:resource="http://reliant.teknowledge.com/DAML/SUMO.owl#CorpuscularObject" /><rdfs:comment>A globe which has a Liquid surface and which contains 

a Gas.</rdfs:comment></rdfs:Class><rdfs:Class rdf:ID="Buffalo"><rdfs:subClassOf rdf:resource="http://reliant.teknowledge.com/DAML/SUMO.owl#HoofedMammal" /><sumo:disjoint rdf:resource="#DomesticAnimal" /><rdfs:comment>A HoofedMammal with long hair whose habitat is the 

plains of NorthAmerica.</rdfs:comment></rdfs:Class><rdfs:Class rdf:ID="Bugle"><rdfs:subClassOf rdf:resource="#HornInstrument" /><rdfs:comment>A HornInstrument that has no valves.</rdfs:comment></rdfs:Class><rdfs:Class rdf:ID="BuildingLevel"><rdfs:subClassOf rdf:resource="http://reliant.teknowledge.com/DAML/SUMO.owl#StationaryArtifact" /><rdfs:comment>The story or level of a building, e.g. the Basement, 

the Attic, the ground level, the fourteenth floor, etc.</rdfs:comment></rdfs:Class><rdfs:Class rdf:ID="Bull"><rdfs:subClassOf rdf:resource="#Cow" /><rdfs:comment>A Cow that is Male.</rdfs:comment></rdfs:Class><rdfs:Class rdf:ID="Bullet"><rdfs:subClassOf rdf:resource="#Projectile" /><rdfs:comment>A Projectile that is designed to be fired by a Gun.</rdfs:comment></rdfs:Class><rdfs:Class rdf:ID="BumbleBee"><rdfs:subClassOf rdf:resource="#Bee" /><rdfs:comment>A large Bee which lacks a stinger.</rdfs:comment></rdfs:Class><rdfs:Class rdf:ID="Burrow"><rdfs:subClassOf rdf:resource="#Cave" /><rdfs:comment>A small Cave created by an Animal for the purpose 

of inhabiting it.</rdfs:comment></rdfs:Class><rdfs:Class rdf:ID="Burying"><rdfs:subClassOf rdf:resource="http://reliant.teknowledge.com/DAML/SUMO.owl#Putting" /><rdfs:comment>Putting something in the ground and then covering 

it with Soil.</rdfs:comment></rdfs:Class><rdfs:Class rdf:ID="Bus"><rdfs:subClassOf rdf:resource="#SelfPoweredRoadVehicle" /><rdfs:comment>Bus is the subclass of SelfPoweredRoadVehicles 

that can transport large numbers of passengers (i.e., dozens) at one 

time.</rdfs:comment></rdfs:Class><rdfs:Class rdf:ID="BusinessCompetition"><rdfs:subClassOf rdf:resource="http://reliant.teknowledge.com/DAML/SUMO.owl#Contest" /><rdfs:comment>Any Contest where the contestParticipants 

are CommercialAgents and the aim is to win as many customers as possible.</rdfs:comment></rdfs:Class><rdfs:Class rdf:ID="Butter"><rdfs:subClassOf rdf:resource="#PreparedFood" /><rdfs:comment>An emulsion of fat which is produced by churning Milk.</rdfs:comment></rdfs:Class><rdfs:Class rdf:ID="Button"><rdfs:subClassOf rdf:resource="http://reliant.teknowledge.com/DAML/SUMO.owl#AttachingDevice" /><rdfs:comment>An AttachingDevice that is used on Clothing.</rdfs:comment></rdfs:Class><rdfs:Class rdf:ID="CPU"><rdfs:subClassOf rdf:resource="#ComputerHardware" /><rdfs:comment>CPU (Central Processing Unit) is the computing part 

of the computer.</rdfs:comment></rdfs:Class><rdfs:Class rdf:ID="Cafeteria"><rdfs:subClassOf rdf:resource="#Restaurant" /><rdfs:comment>Any Restaurant which does not offer table service.  

Food is selected and purchased at a central counter.</rdfs:comment></rdfs:Class><rdfs:Class rdf:ID="Calcium"><rdfs:subClassOf rdf:resource="http://reliant.teknowledge.com/DAML/SUMO.owl#ElementalSubstance" /><atomicNumber>20</atomicNumber><rdfs:comment>Soft grey metallic element belonging to group 2 of 

the periodic table.  Used a reducing agent in the extraction of thorium, 

zirconium and uranium.  Essential element for living organisms.</rdfs:comment></rdfs:Class><rdfs:Class rdf:ID="Calf"><rdfs:subClassOf rdf:resource="#Cow" /><rdfs:comment>A young Cow, i.e. a Cow that is NonFullyFormed.</rdfs:comment></rdfs:Class><rdfs:Class rdf:ID="Camera"><rdfs:subClassOf rdf:resource="http://reliant.teknowledge.com/DAML/SUMO.owl#Device" /><rdfs:comment>A Device which is capable of Photographing.</rdfs:comment></rdfs:Class><rdfs:Class rdf:ID="Campground"><rdfs:subClassOf rdf:resource="http://reliant.teknowledge.com/DAML/SUMO.owl#LandArea" /><rdfs:comment>A LandArea whose purpose is to have MobileResidences 

(e.g. recreational vehicles, mobile homes, Tents, etc.) located there.</rdfs:comment></rdfs:Class><rdfs:Class rdf:ID="Canal"><rdfs:subClassOf rdf:resource="#Waterway" /><rdfs:subClassOf rdf:resource="http://reliant.teknowledge.com/DAML/SUMO.owl#StationaryArtifact" /><rdfs:comment>Canal is the subclass of Waterways that are 

Artifacts constructed for the passage of Ships.</rdfs:comment></rdfs:Class><rdfs:Class rdf:ID="Candela"><rdfs:subClassOf rdf:resource="http://reliant.teknowledge.com/DAML/SUMO.owl#FunctionQuantity" /><rdf:type rdf:resource="http://reliant.teknowledge.com/DAML/SUMO.owl#SystemeInternationalUnit" /><rdfs:comment>SI luminosity intensity measure.  Symbol: cd. 

It is one of the base units in SI, and it is currently defined as 

follows:  the Candela is the luminous intensity, in a given direction, 

of a source that emits monochromatic radiation of frequency 540*10^12 

Hertz and that has a radiant intensity in that direction of 1/683 

Watt per Steradian.</rdfs:comment></rdfs:Class><rdfs:Class rdf:ID="Candle"><rdfs:subClassOf rdf:resource="#IlluminationDevice" /><rdfs:comment>An IlluminationDevice that consists of Wax and a wick, 

which is lit with a flame.</rdfs:comment></rdfs:Class><rdfs:Class rdf:ID="Canyon"><rdfs:subClassOf rdf:resource="#LandForm" /><rdfs:comment>Canyon is the subclass of LandForms that are 

narrow valleys with steep sides, usually created by water erosion.</rdfs:comment></rdfs:Class><rdfs:Class rdf:ID="Capillary"><rdfs:subClassOf rdf:resource="#BloodVessel" /><rdfs:comment>A very small BloodVessel that connects arterioles 

(very small Arteries) with venules (very small Veins).</rdfs:comment></rdfs:Class><rdfs:Class rdf:ID="CaptainOfficer"><rdfs:subClassOf rdf:resource="#MilitaryOfficer" /><rdfs:comment>A commissioned MilitaryOfficer who ranks 

above a Lieutenant but below a MajorOfficer.</rdfs:comment></rdfs:Class><rdfs:Class rdf:ID="Carbon"><rdfs:subClassOf rdf:resource="http://reliant.teknowledge.com/DAML/SUMO.owl#ElementalSubstance" /><atomicNumber>6</atomicNumber><rdfs:comment>Carbon is a member of group 14 of the periodic 

table.  It has three allotropic forms of it, diamonds, graphite and 

fullerite.  Carbon-14 is commonly used in radioactive dating.  Carbon 

occurs in all organic life and is the basis of organic chemistry.  Carbon 

has the interesting chemical property of being able to bond with itself, 

and a wide variety of other elements.</rdfs:comment></rdfs:Class><rdfs:Class rdf:ID="CareOrganization"><rdfs:subClassOf rdf:resource="http://reliant.teknowledge.com/DAML/SUMO.owl#Organization" /><rdfs:comment>Any Organization whose purpose is to 

provide medical care for for Humans who reside there, either permanently 

or temporarily.</rdfs:comment></rdfs:Class><rdfs:Class rdf:ID="CargoShip"><rdfs:subClassOf rdf:resource="#Ship" /><rdfs:comment>CargoShip is the subclass of Ships that 

transport goods in exchange for payment.  CargoShip includes ships 

that carry all kinds of cargo, including oil and bulk products as well 

as packaged, palletized, or containerized goods.</rdfs:comment></rdfs:Class><rdfs:Class rdf:ID="Carpenter"><rdfs:subClassOf rdf:resource="#OccupationalTrade" /><rdfs:comment>Any occupation that involves creating and repairing 

Artifacts that are made chiefly of Wood.</rdfs:comment></rdfs:Class><rdfs:Class rdf:ID="Catching"><rdfs:subClassOf rdf:resource="http://reliant.teknowledge.com/DAML/SUMO.owl#Touching" /><rdfs:subClassOf rdf:resource="http://reliant.teknowledge.com/DAML/SUMO.owl#Maneuver" /><rdfs:comment>Any Maneuver in a Game which results in a 

situation where the agent grasps the Ball.</rdfs:comment></rdfs:Class><rdfs:Class rdf:ID="CausingHappiness"><rdfs:subClassOf rdf:resource="http://reliant.teknowledge.com/DAML/SUMO.owl#BiologicalProcess" /><rdfs:comment>Any Process whose result is that the 

patient of the process is happy.</rdfs:comment></rdfs:Class><rdfs:Class rdf:ID="CausingPain"><rdfs:subClassOf rdf:resource="#CausingUnhappiness" /><rdfs:comment>Any Process whose result is that the 

patient of the process is in Pain.</rdfs:comment></rdfs:Class><rdfs:Class rdf:ID="CausingUnhappiness"><rdfs:subClassOf rdf:resource="http://reliant.teknowledge.com/DAML/SUMO.owl#BiologicalProcess" /><rdfs:comment>Any Process whose result is that the 

patient of the process is unhappy.</rdfs:comment></rdfs:Class><rdfs:Class rdf:ID="CavalryUnit"><rdfs:subClassOf rdf:resource="#MilitaryUnit" /><rdfs:comment>MilitaryUnits composed primarily of Soldiers 

who are mounted, i.e. who perform their combat missions from a Horse or 

Vehicle.</rdfs:comment></rdfs:Class><rdfs:Class rdf:ID="Cave"><rdfs:subClassOf rdf:resource="http://reliant.teknowledge.com/DAML/SUMO.owl#Hole" /><rdfs:comment>A large Hole in the earth which can be entered either 

from a WaterArea or from the surface of the earth.</rdfs:comment></rdfs:Class><rdfs:Class rdf:ID="CeasingOperations"><rdfs:subClassOf rdf:resource="http://reliant.teknowledge.com/DAML/SUMO.owl#OrganizationalProcess" /><rdfs:comment>The process of an Organization 

ceasing operations, i.e. its folding or going out of business in 

some other fashion.</rdfs:comment></rdfs:Class><rdfs:Class rdf:ID="Ceiling"><rdfs:subClassOf rdf:resource="http://reliant.teknowledge.com/DAML/SUMO.owl#StationaryArtifact" /><rdfs:comment>A StationaryArtifact that is the top surface 

of a Room.</rdfs:comment></rdfs:Class><rdfs:Class rdf:ID="CellNucleus"><rdfs:subClassOf rdf:resource="http://reliant.teknowledge.com/DAML/SUMO.owl#BodyPart" /><rdfs:comment>The part of the Cell that contains DNA and 

RNA.</rdfs:comment></rdfs:Class><rdfs:Class rdf:ID="Cellulose"><rdfs:subClassOf rdf:resource="http://reliant.teknowledge.com/DAML/SUMO.owl#PlantSubstance" /><rdfs:subClassOf rdf:resource="http://reliant.teknowledge.com/DAML/SUMO.owl#Carbohydrate" /><rdfs:comment>The main component of Plant Tissue.</rdfs:comment></rdfs:Class><rdfs:Class rdf:ID="Cement"><rdfs:subClassOf rdf:resource="http://reliant.teknowledge.com/DAML/SUMO.owl#Mixture" /><rdfs:comment>Cement is a subclass of Mixture 

whose instances may contain various minerals or ores, prepared by 

heating and pulverizing, and used in binding Concrete or in laying 

brick or stone.</rdfs:comment></rdfs:Class><rdfs:Class rdf:ID="Cemetery"><rdfs:subClassOf rdf:resource="http://reliant.teknowledge.com/DAML/SUMO.owl#LandArea" /><rdfs:comment>A LandArea which is used for burying the dead.</rdfs:comment></rdfs:Class><rdfs:Class rdf:ID="CentrifugalMotion"><rdfs:subClassOf rdf:resource="#Rotating" /><sumo:disjoint rdf:resource="#CentripetalMotion" /><rdfs:comment>Any instance of Rotating where there is 

Motion away from the center of the Rotating.</rdfs:comment></rdfs:Class><rdfs:Class rdf:ID="CentripetalMotion"><rdfs:subClassOf rdf:resource="#Rotating" /><rdfs:comment>Any instance of Rotating where there is 

Motion towards the center of the Rotating.</rdfs:comment></rdfs:Class><rdfs:Class rdf:ID="Century"><rdfs:subClassOf rdf:resource="http://reliant.teknowledge.com/DAML/SUMO.owl#TimeDuration" /><rdf:type rdf:resource="http://reliant.teknowledge.com/DAML/SUMO.owl#UnitOfMeasure" /><rdfs:comment>The TimeDuration of 100 years.</rdfs:comment></rdfs:Class><rdfs:Class rdf:ID="CerealGrain"><rdfs:subClassOf rdf:resource="http://reliant.teknowledge.com/DAML/SUMO.owl#Seed" /><rdfs:subClassOf rdf:resource="http://reliant.teknowledge.com/DAML/SUMO.owl#Food" /><rdfs:comment>Any Seed which is produced by the cereal grasses, 

e.g. rice, corn, wheat, etc.</rdfs:comment></rdfs:Class><rdfs:Class rdf:ID="Chair"><rdfs:subClassOf rdf:resource="#Seat" /><rdfs:comment>A Seat that is designed to accommodate a single 

Human.  Note that this class includes stools, as well as Seats with 

arms and/or backs.</rdfs:comment></rdfs:Class><rdfs:Class rdf:ID="ChangingClothing"><rdfs:subClassOf rdf:resource="http://reliant.teknowledge.com/DAML/SUMO.owl#Transfer" /><rdfs:comment>Any instance of a process of 

RemovingClothing or PuttingOnClothing.</rdfs:comment></rdfs:Class><rdfs:Class rdf:ID="Chapter"><rdfs:subClassOf rdf:resource="http://reliant.teknowledge.com/DAML/SUMO.owl#Article" /><rdfs:comment>A numbered and/or titled section of a Book, which is 

typically indicated in a table of contents for the Book.</rdfs:comment></rdfs:Class><rdfs:Class rdf:ID="ChargingAFee"><rdfs:subClassOf rdf:resource="http://reliant.teknowledge.com/DAML/SUMO.owl#FinancialTransaction" /><rdfs:comment>An activity of a fee being charged</rdfs:comment></rdfs:Class><rdfs:Class rdf:ID="Check"><rdfs:subClassOf rdf:resource="http://reliant.teknowledge.com/DAML/SUMO.owl#FinancialInstrument" /><rdfs:comment>A FinancialInstrument drawn against deposited funds, 

to pay a specified amount of money to a specific person upon demand.</rdfs:comment></rdfs:Class><rdfs:Class rdf:ID="CheckingAccount"><rdfs:subClassOf rdf:resource="#DepositAccount" /><rdfs:comment>A bank account against which the depositor 

can draw checks</rdfs:comment></rdfs:Class><rdfs:Class rdf:ID="ChemicalAcid"><rdfs:subClassOf rdf:resource="http://reliant.teknowledge.com/DAML/SUMO.owl#CompoundSubstance" /><sumo:disjoint rdf:resource="#ChemicalBase" /><rdfs:comment>A bitter CompoundSubstance that is capable of 

reacting with a ChemicalBase and forming a ChemicalSalt.</rdfs:comment></rdfs:Class><rdfs:Class rdf:ID="ChemicalAgent"><rdfs:subClassOf rdf:resource="#BiochemicalAgent" /><rdfs:subClassOf rdf:resource="http://reliant.teknowledge.com/DAML/SUMO.owl#CompoundSubstance" /><rdfs:subClassOf rdf:resource="http://reliant.teknowledge.com/DAML/SUMO.owl#BiologicallyActiveSubstance" /><sumo:disjoint rdf:resource="http://reliant.teknowledge.com/DAML/SUMO.owl#OrganicObject" /><rdfs:comment>Synthetic compounds that are not an analogue 

of anything occurring naturally and that can result in serious burns, 

paralysis, and death to Organisms.</rdfs:comment></rdfs:Class><rdfs:Class rdf:ID="ChemicalBase"><rdfs:subClassOf rdf:resource="http://reliant.teknowledge.com/DAML/SUMO.owl#CompoundSubstance" /><rdfs:comment>A CompoundSubstance that is capable of 

reacting with a ChemicalAcid and forming a ChemicalSalt.</rdfs:comment></rdfs:Class><rdfs:Class rdf:ID="ChemicalReduction"><rdfs:subClassOf rdf:resource="http://reliant.teknowledge.com/DAML/SUMO.owl#ChemicalSynthesis" /><sumo:disjoint rdf:resource="#Oxidation" /><rdfs:comment>Any ChemicalProcess where Electrons 

are added to the substance undergoing the ChemicalProcess.</rdfs:comment></rdfs:Class><rdfs:Class rdf:ID="ChemicalSalt"><rdfs:subClassOf rdf:resource="http://reliant.teknowledge.com/DAML/SUMO.owl#CompoundSubstance" /><rdfs:comment>A bitter CompoundSubstance that is formed in a 

chemical reaction of a ChemicalBase with a ChemicalAcid.</rdfs:comment></rdfs:Class><rdfs:Class rdf:ID="ChemicalWeapon"><rdfs:subClassOf rdf:resource="#BiochemicalWeapon" /><rdfs:comment>Weapons that damage or destroy Organisms by means 

of a ChemicalAgent.</rdfs:comment></rdfs:Class><rdfs:Class rdf:ID="ChestOrCabinet"><rdfs:subClassOf rdf:resource="#Furniture" /><rdfs:subClassOf rdf:resource="#Container" /><rdfs:comment>Any piece of Furniture which is also a 

Container, e.g. a chest of drawers, a memory chest, an armoire, etc.</rdfs:comment></rdfs:Class><rdfs:Class rdf:ID="Chewing"><rdfs:subClassOf rdf:resource="http://reliant.teknowledge.com/DAML/SUMO.owl#BodyMotion" /><rdfs:comment>Breaking up or mashing Food with one's teeth.</rdfs:comment></rdfs:Class><rdfs:Class rdf:ID="Chicken"><rdfs:subClassOf rdf:resource="http://reliant.teknowledge.com/DAML/SUMO.owl#Bird" /><rdfs:subClassOf rdf:resource="#DomesticAnimal" /><rdfs:comment>A subclass of Bird that is raised for its meat 

and for its eggs.</rdfs:comment></rdfs:Class><rdfs:Class rdf:ID="ChickenMeat"><rdfs:subClassOf rdf:resource="http://reliant.teknowledge.com/DAML/SUMO.owl#Meat" /><rdfs:comment>Meat that was originally part of a Chicken.</rdfs:comment></rdfs:Class><rdfs:Class rdf:ID="Chimney"><rdfs:subClassOf rdf:resource="http://reliant.teknowledge.com/DAML/SUMO.owl#StationaryArtifact" /><rdfs:subClassOf rdf:resource="http://reliant.teknowledge.com/DAML/SUMO.owl#Device" /><rdfs:comment>A thin passageway through which Smoke from a controlled 

fire is conducted outside of a Building or Room.</rdfs:comment></rdfs:Class><rdfs:Class rdf:ID="Chin"><rdfs:subClassOf rdf:resource="http://reliant.teknowledge.com/DAML/SUMO.owl#AnimalAnatomicalStructure" /><rdfs:subClassOf rdf:resource="http://reliant.teknowledge.com/DAML/SUMO.owl#BodyPart" /><rdfs:comment>A part of the Face which protrudes slightly and which 

is lower than all other parts of the Face.</rdfs:comment></rdfs:Class><rdfs:Class rdf:ID="Chlorine"><rdfs:subClassOf rdf:resource="http://reliant.teknowledge.com/DAML/SUMO.owl#ElementalSubstance" /><atomicNumber>17</atomicNumber><rdfs:comment>Halogen element.  Poisonous greenish-yellow gas.  

Occurs widely in nature as sodium chloride in seawater.  Reacts directly 

with many elements and compounds, strong oxidizing agent.  Discovered by 

Karl Scheele in 1774.  Humphrey David confirmed it as an element in 

1810.</rdfs:comment></rdfs:Class><rdfs:Class rdf:ID="Cholesterol"><rdfs:subClassOf rdf:resource="#Steroid" /><rdfs:subClassOf rdf:resource="http://reliant.teknowledge.com/DAML/SUMO.owl#AnimalSubstance" /><rdfs:comment>A Steroid that is produced by the Liver and that 

is believed to be closely associated with various cardiological disorders.</rdfs:comment></rdfs:Class><rdfs:Class rdf:ID="Choreographing"><rdfs:subClassOf rdf:resource="http://reliant.teknowledge.com/DAML/SUMO.owl#Planning" /><rdfs:comment>Planning that results in a sequence of dance 

steps that are executed as part of a Performance.</rdfs:comment></rdfs:Class><rdfs:Class rdf:ID="ChristianBible"><rdfs:subClassOf rdf:resource="http://reliant.teknowledge.com/DAML/SUMO.owl#Book" /><sumo:subsumesContentClass rdf:resource="#NewTestament" /><sumo:subsumesContentClass rdf:resource="#OldTestament" /><rdfs:comment>Any instance of the collection of writings which 

is regarded as scripture by those who embrace Christianity.</rdfs:comment></rdfs:Class><rdfs:Class rdf:ID="ChristianGospel"><rdfs:subClassOf rdf:resource="http://reliant.teknowledge.com/DAML/SUMO.owl#Text" /><rdfs:comment>Four books in the New Testament of the 

ChristianBible that describe the life and teachings of Jesus Christ 

and that are referred to, respectively, as Matthew, Mark, Luke, and John.</rdfs:comment></rdfs:Class><rdfs:Class rdf:ID="ChristianService"><rdfs:subClassOf rdf:resource="#ReligiousService" /><rdfs:comment>Any ReligiousService that is conducted by 

members of Christianity.</rdfs:comment></rdfs:Class><rdfs:Class rdf:ID="Chromatography"><rdfs:subClassOf rdf:resource="http://reliant.teknowledge.com/DAML/SUMO.owl#Separating" /><rdfs:comment>Processes of Separating a LiquidMixture or 

a GasMixture into some or all of the PureSubstances that comprise it.</rdfs:comment></rdfs:Class><rdfs:Class rdf:ID="Chromium"><rdfs:subClassOf rdf:resource="http://reliant.teknowledge.com/DAML/SUMO.owl#ElementalSubstance" /><atomicNumber>24</atomicNumber><rdfs:comment>Hard silvery transition element.  Used in 

decorative electroplating.  Discovered in 1797 by Vauquelin.</rdfs:comment></rdfs:Class><rdfs:Class rdf:ID="CigarOrCigarette"><rdfs:subClassOf rdf:resource="#SmokingDevice" /><rdfs:comment>A tube of thin paper containing finely ground 

tobacco that is smoked.</rdfs:comment></rdfs:Class><rdfs:Class rdf:ID="Circle"><rdfs:subClassOf rdf:resource="#Oval" /><rdfs:comment>The class of Ovals such that all GeometricPoints 

that make up the Circle are equidistant from a single GeometricPoint, 

known as the center of the Circle.</rdfs:comment></rdfs:Class><rdfs:Class rdf:ID="CircleSector"><rdfs:subClassOf rdf:resource="http://reliant.teknowledge.com/DAML/SUMO.owl#ClosedTwoDimensionalFigure" /><rdfs:comment>A slice of a Circle, i.e. any 

ClosedTwoDimensionalFigure which consists of two Radii and the arc of 

the Circle that they bound.</rdfs:comment></rdfs:Class><rdfs:Class rdf:ID="CityBlock"><rdfs:subClassOf rdf:resource="http://reliant.teknowledge.com/DAML/SUMO.owl#LandArea" /><rdfs:comment>A square-shaped area surrounded by Roadways 

which is part of a City and typically contains Buildings.</rdfs:comment></rdfs:Class><rdfs:Class rdf:ID="CityDistrict"><rdfs:subClassOf rdf:resource="http://reliant.teknowledge.com/DAML/SUMO.owl#GeopoliticalArea" /><rdfs:comment>Any geopoliticalSubdivision of a City.</rdfs:comment></rdfs:Class><rdfs:Class rdf:ID="CityGovernment"><rdfs:subClassOf rdf:resource="http://reliant.teknowledge.com/DAML/SUMO.owl#Government" /><rdfs:comment>CityGovernment is the class of 

governments of Cities.</rdfs:comment></rdfs:Class><rdfs:Class rdf:ID="CivilWar"><rdfs:subClassOf rdf:resource="http://reliant.teknowledge.com/DAML/SUMO.owl#War" /><rdfs:comment>A War in which the fighting GeopoliticalAreas 

are both part of the same Nation.</rdfs:comment></rdfs:Class><rdfs:Class rdf:ID="Clamp"><rdfs:subClassOf rdf:resource="http://reliant.teknowledge.com/DAML/SUMO.owl#AttachingDevice" /><rdfs:comment>An AttachingDevice which is designed to attach 

two things together by means of a movable part which can be tightened 

or loosened.</rdfs:comment></rdfs:Class><rdfs:Class rdf:ID="Clapping"><rdfs:subClassOf rdf:resource="#HandGesture" /><rdfs:subClassOf rdf:resource="http://reliant.teknowledge.com/DAML/SUMO.owl#RadiatingSound" /><rdfs:comment>Bringing the Hands together repeatedly to make 

a loud noise.</rdfs:comment></rdfs:Class><rdfs:Class rdf:ID="Classroom"><rdfs:subClassOf rdf:resource="http://reliant.teknowledge.com/DAML/SUMO.owl#Room" /><rdfs:comment>Any Room in a School where education 

takes place.</rdfs:comment></rdfs:Class><rdfs:Class rdf:ID="Clay"><rdfs:subClassOf rdf:resource="#Soil" /><rdfs:comment>Fine-grained soil consisting of mineral particles, not 

necessarily clay minerals, that are less than 0.002 mm in their maximum dimension.</rdfs:comment></rdfs:Class><rdfs:Class rdf:ID="Cleric"><rdfs:subClassOf rdf:resource="#ReligiousPosition" /><rdfs:comment>Any Position which involves being in charge of or ministering 

to a ReligousOrganization.</rdfs:comment></rdfs:Class><rdfs:Class rdf:ID="ClericalSecretary"><rdfs:subClassOf rdf:resource="#SkilledOccupation" /><rdfs:comment>The class of Positions where the position 

holder is responsible for clerical duties, e.g. typing documents, answering 

phones, keeping schedules, etc.</rdfs:comment></rdfs:Class><rdfs:Class rdf:ID="ClimateZone"><rdfs:subClassOf rdf:resource="http://reliant.teknowledge.com/DAML/SUMO.owl#GeographicArea" /><rdfs:comment>ClimateZone is a subclass of GeographicArea in which regions 

are classified according to their long-term weather conditions. 

The subclasses of ClimateZone are based on the Koeppen Climate 

Classification system.  In the Koeppen system, climate zones are 

distinguished based on temperatures and rainfall.</rdfs:comment></rdfs:Class><rdfs:Class rdf:ID="Cloak"><rdfs:subClassOf rdf:resource="http://reliant.teknowledge.com/DAML/SUMO.owl#Clothing" /><rdfs:comment>A piece of Clothing that covers the whole body 

except the face (and possibly entire head), hands, and feet.</rdfs:comment></rdfs:Class><rdfs:Class rdf:ID="Clock"><rdfs:subClassOf rdf:resource="http://reliant.teknowledge.com/DAML/SUMO.owl#MeasuringDevice" /><rdfs:comment>Any Device that measures and represents TimeDuration 

or TimePosition.</rdfs:comment></rdfs:Class><rdfs:Class rdf:ID="Closet"><rdfs:subClassOf rdf:resource="http://reliant.teknowledge.com/DAML/SUMO.owl#Room" /><rdfs:comment>A relatively small Room used for storage.</rdfs:comment></rdfs:Class><rdfs:Class rdf:ID="Closing"><rdfs:subClassOf rdf:resource="http://reliant.teknowledge.com/DAML/SUMO.owl#Motion" /><rdfs:comment>The Class of Processes where an aperture is 

closed in an Object.</rdfs:comment></rdfs:Class><rdfs:Class rdf:ID="ClosingContract"><rdfs:subClassOf rdf:resource="http://reliant.teknowledge.com/DAML/SUMO.owl#Committing" /><rdfs:comment>Completing a Contract of some sort, 

e.g. the purchase of a house, closing a business deal, etc.</rdfs:comment></rdfs:Class><rdfs:Class rdf:ID="ClosingEyes"><rdfs:subClassOf rdf:resource="#EyeMotion" /><rdfs:comment>The EyeMotion of tensing the eye lids so that 

the corneas are not exposed to light.</rdfs:comment></rdfs:Class><rdfs:Class rdf:ID="ClothingSuit"><rdfs:subClassOf rdf:resource="http://reliant.teknowledge.com/DAML/SUMO.owl#Collection" /><rdfs:comment>A Collection of instances of Clothing that 

are designed to be worn together.</rdfs:comment></rdfs:Class><rdfs:Class rdf:ID="Coach"><rdfs:subClassOf rdf:resource="#SkilledOccupation" /><rdfs:comment>Any occupation that involves training an athlete or a 

sports team.</rdfs:comment></rdfs:Class><rdfs:Class rdf:ID="Coal"><rdfs:subClassOf rdf:resource="#FossilFuel" /><rdfs:subClassOf rdf:resource="#OrganicCompound" /><rdfs:subClassOf rdf:resource="http://reliant.teknowledge.com/DAML/SUMO.owl#Mineral" /><rdfs:comment>Coal is the class representing brownish-black or 

black solid combustible organic substances formed by the decomposition 

of vegetable matter, under the influence of moisture, pressure, and 

temperature.</rdfs:comment></rdfs:Class><rdfs:Class rdf:ID="CoastGuard"><rdfs:subClassOf rdf:resource="http://reliant.teknowledge.com/DAML/SUMO.owl#PoliceOrganization" /><rdfs:comment>CoastGuard is the subclass of GovernmentOrganizations 

that enforce the maritime laws of a Nation and guard its Seacoast.  This may be 

a military or quasi-military organization.</rdfs:comment></rdfs:Class><rdfs:Class rdf:ID="Coat"><rdfs:subClassOf rdf:resource="#OutdoorClothing" /><rdfs:comment>Clothing that has sleeves and covers from the neck 

down.  Coats are intended to be worn outdoors.</rdfs:comment></rdfs:Class><rdfs:Class rdf:ID="Coconut"><rdfs:subClassOf rdf:resource="http://reliant.teknowledge.com/DAML/SUMO.owl#FruitOrVegetable" /><rdfs:subClassOf rdf:resource="http://reliant.teknowledge.com/DAML/SUMO.owl#Food" /><rdfs:comment>A FruitOrVegetable that is produced by a type of palm 

and has an edible white meat.</rdfs:comment></rdfs:Class><rdfs:Class rdf:ID="Coffee"><rdfs:subClassOf rdf:resource="http://reliant.teknowledge.com/DAML/SUMO.owl#Beverage" /><rdfs:subClassOf rdf:resource="#PreparedFood" /><rdfs:comment>A Beverage which is prepared by infusing ground, 

roasted coffee beans into hot water.</rdfs:comment></rdfs:Class><rdfs:Class rdf:ID="Coffin"><rdfs:subClassOf rdf:resource="#Container" /><rdfs:comment>A Container for a HumanCorpse.</rdfs:comment></rdfs:Class><rdfs:Class rdf:ID="ColdClimateZone"><rdfs:subClassOf rdf:resource="#ClimateZone" /><rdfs:comment>ColdClimateZone is the subclass 

of ClimateZone that is characterized by a warmest month with average 

temperature less than 10 degrees Celsius and a coldest month with 

average temperature less than -3 degrees Celsius.  This is Koeppen climate 

system Type D.</rdfs:comment></rdfs:Class><rdfs:Class rdf:ID="ColdDampClimateZone"><rdfs:subClassOf rdf:resource="#ColdClimateZone" /><rdfs:comment>ColdDampClimateZone is the 

subclass of ColdClimateZone that is characterized by having more 

than 30 mm of precipitation in the driest month.  This is subtype 

'Df' in the Koeppen climate system.</rdfs:comment></rdfs:Class><rdfs:Class rdf:ID="Collage"><rdfs:subClassOf rdf:resource="http://reliant.teknowledge.com/DAML/SUMO.owl#ArtWork" /><sumo:disjoint rdf:resource="http://reliant.teknowledge.com/DAML/SUMO.owl#RepresentationalArtWork" /><rdfs:comment>Any abstract ArtWork that is produced by arranging 

bits of paper or photographs.</rdfs:comment></rdfs:Class><rdfs:Class rdf:ID="Collar"><rdfs:subClassOf rdf:resource="http://reliant.teknowledge.com/DAML/SUMO.owl#Clothing" /><rdfs:comment>A piece of Clothing that fits around the Neck.  

A Collar is always part of a Coat or a Shirt.</rdfs:comment></rdfs:Class><rdfs:Class rdf:ID="College"><rdfs:subClassOf rdf:resource="#PostSecondarySchool" /><rdfs:comment>A School which admits students who have 

graduated from high school and which confers a bachelor's degree, 

normally requiring four years of study.  Note that a College does 

not confer any graduate degrees.  For institutions that confer both 

bachelor's and graduate degrees, the concept University should be 

used.</rdfs:comment></rdfs:Class><rdfs:Class rdf:ID="CollegeFreshman"><rdfs:subClassOf rdf:resource="#CollegeStudentPosition" /><rdfs:comment>The Positions of a student at a PostSecondarySchool 

who has completed less than one year at the school.</rdfs:comment></rdfs:Class><rdfs:Class rdf:ID="CollegeJunior"><rdfs:subClassOf rdf:resource="#CollegeStudentPosition" /><rdfs:comment>The Positions of a student at a PostSecondarySchool 

who has completed at least two years and less than three years at the school.</rdfs:comment></rdfs:Class><rdfs:Class rdf:ID="CollegeSenior"><rdfs:subClassOf rdf:resource="#CollegeStudentPosition" /><rdfs:comment>The Positions of a student at a PostSecondarySchool 

who has completed at least three years and less than four years at the school.</rdfs:comment></rdfs:Class><rdfs:Class rdf:ID="CollegeSophomore"><rdfs:subClassOf rdf:resource="#CollegeStudentPosition" /><rdfs:comment>The Positions of a student at a PostSecondarySchool 

who has completed at least one year and less than two years at the school.</rdfs:comment></rdfs:Class><rdfs:Class rdf:ID="CollegeStudentPosition"><rdfs:subClassOf rdf:resource="http://reliant.teknowledge.com/DAML/SUMO.owl#Position" /><rdfs:comment>Any Position at a PostSecondarySchool 

which is occupied exclusively by students.</rdfs:comment></rdfs:Class><rdfs:Class rdf:ID="Colonel"><rdfs:subClassOf rdf:resource="#MilitaryOfficer" /><rdfs:comment>A commissioned MilitaryOfficer who ranks above 

a lieutenant colonel and below a brigadier general.</rdfs:comment></rdfs:Class><rdfs:Class rdf:ID="Comedian"><rdfs:subClassOf rdf:resource="#EntertainmentProfession" /><rdfs:comment>Positions which involve performing stand-up comedy, which 

is recorded and/or performed in front of live audiences.</rdfs:comment></rdfs:Class><rdfs:Class rdf:ID="CommercialBuilding"><rdfs:subClassOf rdf:resource="http://reliant.teknowledge.com/DAML/SUMO.owl#Building" /><rdfs:subClassOf rdf:resource="#PlaceOfCommerce" /><rdfs:comment>A Building which is intended for 

organizational activities, e.g. retail or wholesale selling, manufacturing, 

office work, etc.</rdfs:comment></rdfs:Class><rdfs:Class rdf:ID="CommercialShipping"><rdfs:subClassOf rdf:resource="#Shipping" /><rdfs:subClassOf rdf:resource="http://reliant.teknowledge.com/DAML/SUMO.owl#CommercialService" /><rdfs:comment>CommercialShipping is the subclass of 

Transportation events in which a commercial agent provides transportation 

of goods for remuneration.</rdfs:comment></rdfs:Class><rdfs:Class rdf:ID="CommercialUnit"><rdfs:subClassOf rdf:resource="#PlaceOfCommerce" /><rdfs:comment>A Room or suite of Rooms intended for 

clerical and/or professional work of a single Organization.</rdfs:comment></rdfs:Class><rdfs:Class rdf:ID="Commission"><rdfs:subClassOf rdf:resource="http://reliant.teknowledge.com/DAML/SUMO.owl#Organization" /><rdfs:comment>A small, temporary Organization whose purpose 

is to investigate some issue.</rdfs:comment></rdfs:Class><rdfs:Class rdf:ID="CommonCarrier"><rdfs:subClassOf rdf:resource="#TransportationCompany" /><sumo:disjoint rdf:resource="#ContractCarrier" /><rdfs:comment>CommonCarrier is the subclass of 

TransportationCompany whose instances must offer services to all 

customers.  Contrast with ContractCarrier.</rdfs:comment></rdfs:Class><rdfs:Class rdf:about="http://reliant.teknowledge.com/DAML/SUMO.owl#Communication"><sumo:relatedInternalConcept rdf:resource="#CommunicationDevice" /></rdfs:Class><rdfs:Class rdf:ID="CommunicationDevice"><rdfs:subClassOf rdf:resource="http://reliant.teknowledge.com/DAML/SUMO.owl#EngineeringComponent" /><rdfs:comment>A CommunicationDevice is a Device

which serves at the instrument in a Communication Process by allowing

the communicated message to be conveyed between the participants.</rdfs:comment></rdfs:Class><rdfs:Class rdf:ID="CommunicationOrganization"><rdfs:subClassOf rdf:resource="http://reliant.teknowledge.com/DAML/SUMO.owl#Organization" /><rdfs:comment>CommunicationOrganization is 

the subclass of Organizations that manage Communications over physical 

infrastructure owned or leased by the organization.  Such organizations 

may also produce and disseminate information, entertainment, or other 

content.  Also see MediaOrganization.</rdfs:comment></rdfs:Class><rdfs:Class rdf:ID="CommunicationSystem"><rdfs:subClassOf rdf:resource="http://reliant.teknowledge.com/DAML/SUMO.owl#Collection" /><rdfs:comment>CommunicationSystem is a complex 

system with various components, enabling communication (in some 

medium) between points in a specific area, whether local or worldwide.</rdfs:comment></rdfs:Class><rdfs:Class rdf:ID="CommunistParty"><rdfs:subClassOf rdf:resource="#PoliticalParty" /><rdfs:comment>Any PoliticalParty that advocates for a 

CommunistState.</rdfs:comment></rdfs:Class><rdfs:Class rdf:ID="Compartment"><rdfs:subClassOf rdf:resource="#Container" /><rdfs:comment>A Container which is part of another Container, 

e.g. a drawer, a zippered pouch in a piece of luggage, a compartment in a TV 

dinner, etc.</rdfs:comment></rdfs:Class><rdfs:Class rdf:ID="Compass"><rdfs:subClassOf rdf:resource="http://reliant.teknowledge.com/DAML/SUMO.owl#Device" /><rdfs:comment>A Device that indicates the direction of North.</rdfs:comment></rdfs:Class><rdfs:Class rdf:ID="ComposingMusic"><rdfs:subClassOf rdf:resource="http://reliant.teknowledge.com/DAML/SUMO.owl#ContentDevelopment" /><rdfs:comment>ContentDevelopment which results in a 

MusicalComposition.</rdfs:comment></rdfs:Class><rdfs:Class rdf:ID="Computer"><rdfs:subClassOf rdf:resource="#ElectricDevice" /><rdfs:comment>A programmable ElectricDevice that is capable of 

processing data.  Note that this class comprises the physical parts of a 

computer system, i.e. the machinery and equipment.</rdfs:comment></rdfs:Class><rdfs:Class rdf:ID="ComputerHardware"><rdfs:subClassOf rdf:resource="http://reliant.teknowledge.com/DAML/SUMO.owl#EngineeringComponent" /><rdfs:comment>This class covers any component of 

a Computer.</rdfs:comment></rdfs:Class><rdfs:Class rdf:ID="ComputerMemory"><rdfs:subClassOf rdf:resource="#ComputerHardware" /><rdfs:comment>The computer's workspace (physically, 

a collection of RAM chips). It is an important resource, since it 

determines the size and number of programs that can be run at the 

same time, as well as the amount of data that can be processed 

instantly.</rdfs:comment></rdfs:Class><rdfs:Class rdf:ID="ComputerProcess"><rdfs:subClassOf rdf:resource="http://reliant.teknowledge.com/DAML/SUMO.owl#InternalChange" /><rdfs:comment>The class of Processes which involve 

manipulating data by a Computer.  This covers individual operations 

of a Computer as well as complete realizations of ComputerPrograms.</rdfs:comment></rdfs:Class><rdfs:Class rdf:ID="Concealing"><rdfs:subClassOf rdf:resource="http://reliant.teknowledge.com/DAML/SUMO.owl#Putting" /><rdfs:comment>Locating something in such a way that it cannot 

be seen.</rdfs:comment></rdfs:Class><rdfs:Class rdf:ID="Concentrating"><rdfs:subClassOf rdf:resource="http://reliant.teknowledge.com/DAML/SUMO.owl#Removing" /><rdfs:comment>Removing a Liquid from a Solution to 

increase the concentration of the Solution.</rdfs:comment></rdfs:Class><rdfs:Class rdf:ID="Concrete"><rdfs:subClassOf rdf:resource="http://reliant.teknowledge.com/DAML/SUMO.owl#Mixture" /><rdfs:comment>Concrete is a subclass of Mixture 

used as building materials.  Concrete is made up of Mineral pieces 

(sand or gravel) and a Cement material used to bind them together.</rdfs:comment></rdfs:Class><rdfs:Class rdf:ID="CondominiumBuilding"><rdfs:subClassOf rdf:resource="http://reliant.teknowledge.com/DAML/SUMO.owl#ResidentialBuilding" /><sumo:disjoint rdf:resource="http://reliant.teknowledge.com/DAML/SUMO.owl#SingleFamilyResidence" /><rdfs:comment>A ResidentialBuilding containing 

CondominiumUnits.</rdfs:comment></rdfs:Class><rdfs:Class rdf:ID="CondominiumUnit"><rdfs:subClassOf rdf:resource="http://reliant.teknowledge.com/DAML/SUMO.owl#SingleFamilyResidence" /><rdfs:comment>A SingleFamilyResidence that may be owned 

by a member of the SocialUnit that lives there.</rdfs:comment></rdfs:Class><rdfs:Class rdf:ID="Cone"><rdfs:subClassOf rdf:resource="http://reliant.teknowledge.com/DAML/SUMO.owl#ThreeDimensionalFigure" /><rdfs:comment>The class of ThreeDimensionalFigures which are 

produced by rotating a RightTriangle around its RightAngle.</rdfs:comment></rdfs:Class><rdfs:Class rdf:ID="ConfederateSoldier"><rdfs:subClassOf rdf:resource="#Soldier" /><rdfs:comment>Any Soldier that served on the confederate side 

during the American Civil War.</rdfs:comment></rdfs:Class><rdfs:Class rdf:ID="Congratulating"><rdfs:subClassOf rdf:resource="#ExpressingApproval" /><rdfs:comment>Any ExpressingApproval to a person for 

something that the person did in the past and that is regarded as being 

to the benefit of the person congratulated.</rdfs:comment></rdfs:Class><rdfs:Class rdf:ID="ConjugatedSubstance"><rdfs:subClassOf rdf:resource="http://reliant.teknowledge.com/DAML/SUMO.owl#CompoundSubstance" /><rdfs:comment>A CompoundSubstance that results from 

the ChemicalSynthesis of two or more CompoundSubstances.</rdfs:comment></rdfs:Class><rdfs:Class rdf:ID="Consonant"><rdfs:subClassOf rdf:resource="#AlphabeticCharacter" /><rdfs:comment>An AlphabeticCharacter that denotes a speech sound 

that results in audible friction when it is pronounced.</rdfs:comment></rdfs:Class><rdfs:Class rdf:ID="ConstrictorSnake"><rdfs:subClassOf rdf:resource="#Snake" /><rdfs:comment>A Snake that lacks venom and kills its 

prey by crushing it to death.</rdfs:comment></rdfs:Class><rdfs:Class rdf:ID="Container"><rdfs:subClassOf rdf:resource="#Holder" /><rdfs:comment>Any Holder whose purpose is to contain 

something else.  Note that Container is more specific in meaning 

than Holder, because a Container must have a Hole that is at 

least partially filled by the thing contained.</rdfs:comment></rdfs:Class><rdfs:Class rdf:ID="ContinentalClimateZone"><rdfs:subClassOf rdf:resource="#TemperateClimateZone" /><rdfs:comment>ContinentalClimateZone is a subclass of TemperateClimateZone that is 

characterized by cold winters and hot summers.</rdfs:comment></rdfs:Class><rdfs:Class rdf:ID="ContraceptiveDevice"><rdfs:subClassOf rdf:resource="http://reliant.teknowledge.com/DAML/SUMO.owl#Device" /><rdfs:comment>Devices which permit sexual intercourse but 

which reduce the likelihood of conception.</rdfs:comment></rdfs:Class><rdfs:Class rdf:ID="ContractCarrier"><rdfs:subClassOf rdf:resource="#TransportationCompany" /><rdfs:comment>ContractCarrier is the subclass of 

TransportationCompany whose instances offer services to only one  

customer, under contract.  Contrast with CommonCarrier.</rdfs:comment></rdfs:Class><rdfs:Class rdf:ID="ControlledSubstance"><rdfs:subClassOf rdf:resource="http://reliant.teknowledge.com/DAML/SUMO.owl#BiologicallyActiveSubstance" /><rdfs:comment>ControlledSubstance is 

the subclass of BiologicallyActiveSubstances whose distribution 

and use is controlled by government regulation.</rdfs:comment></rdfs:Class><rdfs:Class rdf:ID="CoolingDevice"><rdfs:subClassOf rdf:resource="http://reliant.teknowledge.com/DAML/SUMO.owl#Device" /><rdfs:comment>A Device whose purpose is Cooling something, 

e.g. air conditioners, refrigerators, freezers, etc.</rdfs:comment></rdfs:Class><rdfs:Class rdf:ID="Copper"><rdfs:subClassOf rdf:resource="http://reliant.teknowledge.com/DAML/SUMO.owl#ElementalSubstance" /><atomicNumber>29</atomicNumber><rdfs:comment>Red-brown transition element.  Known by the Romans 

as 'cuprum.' Extracted and used for thousands of years.  Malleable, 

ductile and an excellent conductor of heat and electricity.  When in moist 

conditions, a greenish layer forms on the outside.</rdfs:comment></rdfs:Class><rdfs:Class rdf:ID="Copying"><rdfs:subClassOf rdf:resource="http://reliant.teknowledge.com/DAML/SUMO.owl#Making" /><rdfs:comment>Making a copy of something.</rdfs:comment></rdfs:Class><rdfs:Class rdf:ID="Corn"><rdfs:subClassOf rdf:resource="#CerealGrain" /><rdfs:comment>A CerealGrain which is found on long ears of a Plant 

native to the Americas.</rdfs:comment></rdfs:Class><rdfs:Class rdf:ID="Coroner"><rdfs:subClassOf rdf:resource="#GovernmentOfficer" /><rdfs:comment>A GovernmentOfficer who investigates deaths that are 

suspected of being due to something other than natural causes.</rdfs:comment></rdfs:Class><rdfs:Class rdf:ID="Corporal"><rdfs:subClassOf rdf:resource="#MilitaryOfficer" /><rdfs:comment>A noncomissioned MilitaryOfficer.</rdfs:comment></rdfs:Class><rdfs:Class rdf:ID="Corresponding"><rdfs:subClassOf rdf:resource="http://reliant.teknowledge.com/DAML/SUMO.owl#LinguisticCommunication" /><rdfs:comment>Instances of LinguisticCommunication which 

are achieved by means of Texts that are mailed between the persons 

communicating with one another.</rdfs:comment></rdfs:Class><rdfs:Class rdf:ID="Cotton"><rdfs:subClassOf rdf:resource="http://reliant.teknowledge.com/DAML/SUMO.owl#PlantAnatomicalStructure" /><rdfs:comment>Fibers from the cotton plant that are used in 

Making CottonFabric.</rdfs:comment></rdfs:Class><rdfs:Class rdf:ID="CottonFabric"><rdfs:subClassOf rdf:resource="http://reliant.teknowledge.com/DAML/SUMO.owl#Fabric" /><rdfs:comment>Any Fabric that is made entirely out of Cotton.</rdfs:comment></rdfs:Class><rdfs:Class rdf:ID="Coulomb"><rdfs:subClassOf rdf:resource="http://reliant.teknowledge.com/DAML/SUMO.owl#TimeDependentQuantity" /><rdf:type rdf:resource="http://reliant.teknowledge.com/DAML/SUMO.owl#SystemeInternationalUnit" /><rdfs:comment>SI electric charge measure.  Symbol: C. It is 

the quantity of electric charge transported through a cross section of 

a conductor in an electric circuit during each SecondDuration by a 

current of 1 Ampere.  Coulomb = s*A.</rdfs:comment></rdfs:Class><rdfs:Class rdf:ID="County"><rdfs:subClassOf rdf:resource="http://reliant.teknowledge.com/DAML/SUMO.owl#GeopoliticalArea" /><rdfs:subClassOf rdf:resource="http://reliant.teknowledge.com/DAML/SUMO.owl#LandArea" /><rdfs:comment>A GeopoliticalArea that is a subdivision of a 

StateOrProvince.  Aside from City, this is the smallest geopolitical 

subdivision, and it is known by various names in various counties, e.g. 

parrish, commune, etc.</rdfs:comment></rdfs:Class><rdfs:Class rdf:ID="CourtRoom"><rdfs:subClassOf rdf:resource="http://reliant.teknowledge.com/DAML/SUMO.owl#Room" /><rdfs:comment>Any Room whose purpose is to realize 

JudicialProcesses.</rdfs:comment></rdfs:Class><rdfs:Class rdf:ID="Cow"><rdfs:subClassOf rdf:resource="http://reliant.teknowledge.com/DAML/SUMO.owl#HoofedMammal" /><rdfs:subClassOf rdf:resource="#DomesticAnimal" /><rdfs:comment>A domesticated HoofedMammal that is raised for milk 

and beef, and is also used for work.</rdfs:comment></rdfs:Class><rdfs:Class rdf:ID="Crane"><rdfs:subClassOf rdf:resource="#MaterialHandlingEquipment" /><rdfs:comment>Crane is a subclass of mechanical Devices 

that consist of a HoistingDevice on a moveable boom, designed to 

assist in moving heavy loads.</rdfs:comment></rdfs:Class><rdfs:Class rdf:ID="CreditAccount"><rdfs:subClassOf rdf:resource="#LiabilityAccount" /><rdfs:comment>Credit extended by a business to a customer.</rdfs:comment></rdfs:Class><rdfs:Class rdf:ID="CreditCardAccount"><rdfs:subClassOf rdf:resource="#CreditAccount" /><rdfs:comment>A type of CreditAccount which uses a CreditCard for 

FinancialTransactions.</rdfs:comment></rdfs:Class><rdfs:Class rdf:ID="CreditUnion"><rdfs:subClassOf rdf:resource="#FinancialCompany" /><rdfs:comment>Credit unions are non-profit, member-owned, 

financial cooperatives. They are operated entirely by and for their 

members. When money is deposited in a credit union, the depositor 

becomes a member of the union because the deposit is considered partial 

ownership in the credit union. Many large organizations have established 

credit unions for their employees.</rdfs:comment></rdfs:Class><rdfs:Class rdf:ID="Creek"><rdfs:subClassOf rdf:resource="#BodyOfWater" /><rdfs:subClassOf rdf:resource="http://reliant.teknowledge.com/DAML/SUMO.owl#StreamWaterArea" /><rdfs:subClassOf rdf:resource="http://reliant.teknowledge.com/DAML/SUMO.owl#FreshWaterArea" /><sumo:disjoint rdf:resource="#River" /><rdfs:comment>Creek is the class of small streams of fresh 

water flowing through land, usually into a River.</rdfs:comment></rdfs:Class><rdfs:Class rdf:ID="CreoleLanguage"><rdfs:subClassOf rdf:resource="http://reliant.teknowledge.com/DAML/SUMO.owl#SpokenHumanLanguage" /><rdfs:comment>A CreoleLanguage is a PidginLanguage that 

has developed and become the mother tongue for a community of people. This 

process is called 'creolization' and results in an expanded vocabulary and 

grammar structure that allow for communication as rich and complex as that of 

non-creole languages. While pidgins are regarded as reduced languages, creoles

are considered expanded languages. That is, while pidgins develop to enable 

communication in relatively isolated domains, creoles allow for a full range 

of expressive possibilities on a par with more 'recognized' languages.</rdfs:comment></rdfs:Class><rdfs:Class rdf:ID="CriminalAction"><rdfs:subClassOf rdf:resource="http://reliant.teknowledge.com/DAML/SUMO.owl#IntentionalProcess" /><rdfs:comment>Any IntentionalProcess that violates a Law.</rdfs:comment></rdfs:Class><rdfs:Class rdf:ID="CriminalGang"><rdfs:subClassOf rdf:resource="http://reliant.teknowledge.com/DAML/SUMO.owl#GroupOfPeople" /><rdfs:comment>A GroupOfPeople which exists (partially or 

wholly) for the purpose of CriminalAction.</rdfs:comment></rdfs:Class><rdfs:Class rdf:ID="CubicFoot"><rdf:type rdf:resource="http://reliant.teknowledge.com/DAML/SUMO.owl#UnitOfMeasure" /><rdfs:subClassOf rdf:resource="http://reliant.teknowledge.com/DAML/SUMO.owl#VolumeMeasure" /><rdfs:comment>CubicFoot is a unit for measuring volume, 

equal to a volume of one foot length in each dimension of length, width, 

and height.</rdfs:comment></rdfs:Class><rdfs:Class rdf:ID="CultivatedLandArea"><rdfs:subClassOf rdf:resource="http://reliant.teknowledge.com/DAML/SUMO.owl#LandArea" /><rdfs:comment>A LandArea which is dedicated to 

Agriculture, e.g. Lawns, gardens, and fields for growing crops.</rdfs:comment></rdfs:Class><rdfs:Class rdf:about="http://reliant.teknowledge.com/DAML/SUMO.owl#Cup"><rdfs:subClassOf rdf:resource="#FluidContainer" /><rdfs:comment>An open FluidContainer that is intended to serve a 

Beverage to a single person.  Note that this class includes both cups 

with handles and drinking glasses.</rdfs:comment></rdfs:Class><rdfs:Class rdf:ID="Curb"><rdfs:subClassOf rdf:resource="http://reliant.teknowledge.com/DAML/SUMO.owl#StationaryArtifact" /><rdfs:comment>A raised concrete or asphalt structure that connects a 

Sidewalk with a Roadway.</rdfs:comment></rdfs:Class><rdfs:Class rdf:ID="Curtain"><rdfs:subClassOf rdf:resource="#WindowCovering" /><rdfs:subClassOf rdf:resource="#FabricArtifact" /><rdfs:comment>A piece of Fabric whose purpose is Covering a 

Window so as to keep out the light or prevent people from seeing inside.</rdfs:comment></rdfs:Class><rdfs:Class rdf:ID="CuttingDevice"><rdfs:subClassOf rdf:resource="http://reliant.teknowledge.com/DAML/SUMO.owl#Device" /><rdfs:comment>Any Device whose purpose is Cutting something 

else.  This class covers knives of all times, axes, saws, razors, chisels etc.</rdfs:comment></rdfs:Class><rdfs:Class rdf:ID="Cycle-TransportationDevice"><rdfs:subClassOf rdf:resource="#LandVehicle" /><rdfs:subClassOf rdf:resource="#UserPoweredDevice" /><rdfs:comment>Cycle-TransportationDevice 

is a class of wheeled, pedal-driven UserPoweredVehicles that are 

designed to be ridden on roads or trails.</rdfs:comment></rdfs:Class><rdfs:Class rdf:ID="Cylinder"><rdfs:subClassOf rdf:resource="http://reliant.teknowledge.com/DAML/SUMO.owl#ThreeDimensionalFigure" /><rdfs:comment>The class of ThreeDimensionalFigures such that 

all GeometricPoints that make up the Cylinder are equidistant from a 

OneDimensionalFigure, known as the axis of the Cylinder.</rdfs:comment></rdfs:Class><rdfs:Class rdf:ID="Dam"><rdfs:subClassOf rdf:resource="http://reliant.teknowledge.com/DAML/SUMO.owl#StationaryArtifact" /><rdfs:comment>Dam is the subclass of StationaryArtifacts that 

are walls built across a stream or river to hold back water.</rdfs:comment></rdfs:Class><rdfs:Class rdf:ID="Dancing"><rdfs:subClassOf rdf:resource="http://reliant.teknowledge.com/DAML/SUMO.owl#BodyMotion" /><rdfs:comment>Any BodyMotion of Humans which is 

deliberately coordinated with music.</rdfs:comment></rdfs:Class><rdfs:Class rdf:ID="DateFruit"><rdfs:subClassOf rdf:resource="http://reliant.teknowledge.com/DAML/SUMO.owl#FruitOrVegetable" /><rdfs:subClassOf rdf:resource="http://reliant.teknowledge.com/DAML/SUMO.owl#Food" /><rdfs:comment>A FruitOrVegetable that is produced by the date 

palm.</rdfs:comment></rdfs:Class><rdfs:Class rdf:ID="DaySchool"><rdfs:subClassOf rdf:resource="#School" /><rdfs:comment>A School that does not board its students, i.e. 

students attend classes during the day and then return to a private residence 

for the night.</rdfs:comment></rdfs:Class><rdfs:Class rdf:ID="DayTime"><rdfs:subClassOf rdf:resource="http://reliant.teknowledge.com/DAML/SUMO.owl#TimeInterval" /><rdfs:comment>The class of TimeIntervals that begin at Sunrise 

and end at Sunset.</rdfs:comment></rdfs:Class><rdfs:Class rdf:ID="Deacon"><rdfs:subClassOf rdf:resource="#ReligiousPosition" /><rdfs:subClassOf rdf:resource="#PartTimePosition" /><rdfs:comment>Any Position within a ReligiousOrganization that is held 

by a layman, which is part-time, and which involves assisting a Cleric.</rdfs:comment></rdfs:Class><rdfs:Class rdf:ID="DeafSignLanguage"><rdfs:subClassOf rdf:resource="http://reliant.teknowledge.com/DAML/SUMO.owl#ManualHumanLanguage" /><rdfs:comment>A DeafSignLanguage is a

ManualHumanLanguage primarily intended for communication between a

deaf individual and a hearing individual or between deaf individuals.</rdfs:comment></rdfs:Class><rdfs:Class rdf:ID="Debating"><rdfs:subClassOf rdf:resource="http://reliant.teknowledge.com/DAML/SUMO.owl#Contest" /><rdfs:subClassOf rdf:resource="http://reliant.teknowledge.com/DAML/SUMO.owl#LinguisticCommunication" /><rdfs:comment>A Contest where each participant holds a different 

view regarding some issue, and each participant attempts to prove, by 

rhetoric or evidence, that his/her own views about a particular matter are 

correct and/or that the views of the other participants are incorrect.</rdfs:comment></rdfs:Class><rdfs:Class rdf:ID="Deboarding"><rdfs:subClassOf rdf:resource="http://reliant.teknowledge.com/DAML/SUMO.owl#Translocation" /><rdfs:comment>Getting off a Vehicle, e.g. getting out of an 

Automobile, deplaning, getting off a Watercraft, etc.</rdfs:comment></rdfs:Class><rdfs:Class rdf:ID="Decade"><rdfs:subClassOf rdf:resource="http://reliant.teknowledge.com/DAML/SUMO.owl#TimeDuration" /><rdf:type rdf:resource="http://reliant.teknowledge.com/DAML/SUMO.owl#UnitOfMeasure" /><rdfs:comment>The TimeDuration of 10 years.</rdfs:comment></rdfs:Class><rdfs:Class rdf:ID="Decelerating"><rdfs:subClassOf rdf:resource="http://reliant.teknowledge.com/DAML/SUMO.owl#Translocation" /><rdfs:subClassOf rdf:resource="http://reliant.teknowledge.com/DAML/SUMO.owl#Decreasing" /><rdfs:comment>Decreasing the speed with which someone 

or something is moving.</rdfs:comment></rdfs:Class><rdfs:Class rdf:ID="DefinedContributionPlan"><rdfs:subClassOf rdf:resource="#PensionPlan" /><rdfs:comment>A company retirement plan, such as 

a 401(k) or 403(b), in which the employee elects to defer some amount of 

his/her salary into the plan and bears the investment risk.</rdfs:comment></rdfs:Class><rdfs:Class rdf:ID="Dentist"><rdfs:subClassOf rdf:resource="#Profession" /><rdfs:comment>The Profession of being a dentist, i.e. diagnosing 

and treating problems related to the teeth.</rdfs:comment></rdfs:Class><rdfs:Class rdf:ID="DependencyOrSpecialSovereigntyArea"><rdfs:subClassOf rdf:resource="http://reliant.teknowledge.com/DAML/SUMO.owl#GeopoliticalArea" /><rdfs:comment>DependencyOrSpecialSovereigntyArea 

is a subclass of GeopoliticalArea, representing the classification 'Dependency or 

Special Sovereignty Area' used by the CIA World Fact Book.</rdfs:comment></rdfs:Class><rdfs:Class rdf:ID="Deposit"><rdfs:subClassOf rdf:resource="http://reliant.teknowledge.com/DAML/SUMO.owl#FinancialTransaction" /><sumo:disjoint rdf:resource="#Withdrawal" /><rdfs:comment>An Activity of money being transferred into a customer's 

account at a financial institution.</rdfs:comment></rdfs:Class><rdfs:Class rdf:ID="DepositAccount"><rdfs:subClassOf rdf:resource="#FinancialAccount" /><rdfs:comment>An account where money is deposited for checking, 

savings or brokerage use.</rdfs:comment></rdfs:Class><rdfs:Class rdf:ID="DepositingACheck"><rdfs:subClassOf rdf:resource="#UsingAnAccount" /><rdfs:comment>An activity of depositing a check into a 

FinancialCompany.</rdfs:comment></rdfs:Class><rdfs:Class rdf:ID="Depressant"><rdfs:subClassOf rdf:resource="http://reliant.teknowledge.com/DAML/SUMO.owl#BiologicallyActiveSubstance" /><rdfs:comment>Any BiologicallyActiveSubstance which has 

the effect of depressing the central nervous system, i.e. decreasing 

function or activity in the Brain or SpinalCord.</rdfs:comment></rdfs:Class><rdfs:Class rdf:ID="Deputy"><rdfs:subClassOf rdf:resource="#PoliceOfficer" /><rdfs:comment>A Position which authorizes the holder of the position 

to act as the sheriff when the sheriff is not available.</rdfs:comment></rdfs:Class><rdfs:Class rdf:ID="DesertClimateZone"><rdfs:subClassOf rdf:resource="#AridClimateZone" /><rdfs:comment>DesertClimateZone 

is the class of AridClimateZones characterized by 

sparse, desert vegetation.  Koeppen system 'BW'.</rdfs:comment></rdfs:Class><rdfs:Class rdf:ID="Desk"><rdfs:subClassOf rdf:resource="#Table" /><rdfs:comment>A Table for a single person which is intended to be 

used for paperwork.</rdfs:comment></rdfs:Class><rdfs:Class rdf:ID="Detergent"><rdfs:subClassOf rdf:resource="http://reliant.teknowledge.com/DAML/SUMO.owl#Mixture" /><rdfs:comment>Any Mixture whose purpose is to remove Soil 

and/or other undesirable substances from the surfaces of objects.</rdfs:comment></rdfs:Class><rdfs:Class rdf:ID="DeviceAttribute"><rdfs:subClassOf rdf:resource="http://reliant.teknowledge.com/DAML/SUMO.owl#ObjectiveNorm" /><rdfs:comment>This class contains Attributes that 

are specific to the functioning of Devices.</rdfs:comment></rdfs:Class><rdfs:Class rdf:ID="DeviceStateAttribute"><rdfs:subClassOf rdf:resource="#DeviceAttribute" /><rdfs:comment>DeviceStateAttribute is the class 

of attributes that represent different states that a Device may be in.  

Examples: DeviceOff, DeviceOn, DeviceOpen, and DeviceClosed.</rdfs:comment></rdfs:Class><rdfs:Class rdf:ID="Dialysis"><rdfs:subClassOf rdf:resource="http://reliant.teknowledge.com/DAML/SUMO.owl#Separating" /><rdfs:comment>Any process of Separating a Solution into two or more 

constituent PureSubstances by means of their unequal diffusion through membranes 

that are partially permeable.</rdfs:comment></rdfs:Class><rdfs:Class rdf:ID="Diamond"><rdfs:subClassOf rdf:resource="http://reliant.teknowledge.com/DAML/SUMO.owl#Mineral" /><rdfs:subClassOf rdf:resource="#Carbon" /><rdfs:comment>Crystalline Carbon that is valued as a gem and 

used in industrial applications.</rdfs:comment></rdfs:Class><rdfs:Class rdf:ID="Dictionary"><rdfs:subClassOf rdf:resource="#ReferenceText" /><rdfs:comment>A ReferenceText which specifies the meanings 

of the Words of a Language or of a technical jargon.</rdfs:comment></rdfs:Class><rdfs:Class rdf:ID="DieselEngine"><rdfs:subClassOf rdf:resource="#InternalCombustionEngine" /><rdfs:comment>DieselEngine is the subclass of 

InternalCombustionEngines that use DieselFuel as their resource.</rdfs:comment></rdfs:Class><rdfs:Class rdf:ID="DieselFuel"><rdfs:subClassOf rdf:resource="#RefinedPetroleumProduct" /><rdfs:subClassOf rdf:resource="#FossilFuel" /><rdfs:comment>DieselFuel is the subclass of 

RefinedPetroleumProducts that are fuels for diesel engines.</rdfs:comment></rdfs:Class><rdfs:Class rdf:ID="Diet"><rdfs:subClassOf rdf:resource="http://reliant.teknowledge.com/DAML/SUMO.owl#Plan" /><rdfs:comment>A Plan regarding what one is allowed to eat.</rdfs:comment></rdfs:Class><rdfs:Class rdf:ID="Digging"><rdfs:subClassOf rdf:resource="http://reliant.teknowledge.com/DAML/SUMO.owl#IntentionalProcess" /><rdfs:subClassOf rdf:resource="http://reliant.teknowledge.com/DAML/SUMO.owl#SurfaceChange" /><rdfs:comment>Any Process of removing or turning over the Soil.</rdfs:comment></rdfs:Class><rdfs:Class rdf:ID="DigitAppendage"><rdfs:subClassOf rdf:resource="http://reliant.teknowledge.com/DAML/SUMO.owl#AnimalAnatomicalStructure" /><rdfs:subClassOf rdf:resource="http://reliant.teknowledge.com/DAML/SUMO.owl#BodyPart" /><rdfs:comment>Any of the extremities of Limbs that are 

found in the higer Vertebrates and the Amphibians.</rdfs:comment></rdfs:Class><rdfs:Class rdf:ID="DigitCharacter"><rdfs:subClassOf rdf:resource="http://reliant.teknowledge.com/DAML/SUMO.owl#Character" /><sumo:disjoint rdf:resource="#AlphabeticCharacter" /><rdfs:comment>Any Character that is comprised of a single digit, 

i.e. one of the numerals 0, 1, 2, 3, 4, 5, 6, 7, 8, 9.</rdfs:comment></rdfs:Class><rdfs:Class rdf:ID="Diluting"><rdfs:subClassOf rdf:resource="http://reliant.teknowledge.com/DAML/SUMO.owl#Putting" /><rdfs:comment>Adding a Liquid to a Solution to decrease 

the concentration of the Solution.</rdfs:comment></rdfs:Class><rdfs:Class rdf:ID="DiningRoom"><rdfs:subClassOf rdf:resource="http://reliant.teknowledge.com/DAML/SUMO.owl#Room" /><rdfs:comment>A Room intended primarily for Eating.</rdfs:comment></rdfs:Class><rdfs:Class rdf:ID="DiplomaticAgent"><rdfs:subClassOf rdf:resource="#ForeignServicePosition" /><rdfs:comment>DiplomaticAgent is the class of Positions 

where one is charged to represent one national government to another nation 

or international organization.  This includes any Ambassador or head of 

a diplomatic mission.  Individuals with this attribute may also hold a 

career diplomatic position (see ForeignServicePosition).</rdfs:comment></rdfs:Class><rdfs:Class rdf:ID="DirectedGraph"><rdfs:subClassOf rdf:resource="#Graph" /><rdfs:comment>The Class of directed graphs.  A 

directed graph is a Graph in which all GraphArcs

have direction, i.e. every GraphArc has an initial node (see 

InitialNodeFn) and a terminal node (see TerminalNodeFn).</rdfs:comment></rdfs:Class><rdfs:Class rdf:ID="Dish"><rdfs:subClassOf rdf:resource="#Holder" /><rdfs:comment>A Holder for Food while the Food is being eaten.</rdfs:comment></rdfs:Class><rdfs:Class rdf:ID="Dismounting"><rdfs:subClassOf rdf:resource="http://reliant.teknowledge.com/DAML/SUMO.owl#BodyMotion" /><rdfs:comment>Any BodyMotion which results in not being On 

something else.</rdfs:comment></rdfs:Class><rdfs:Class rdf:ID="DisplacementHullWatercraft"><rdfs:subClassOf rdf:resource="#Watercraft" /><sumo:disjoint rdf:resource="#PlaningHullWatercraft" /><rdfs:comment>DisplacementHullWatercraft is 

a subclass of Watercraft with hulls designed to move water aside as they 

move through the water.  Contrast with PlaningHullWatercraft.</rdfs:comment></rdfs:Class><rdfs:Class rdf:ID="DisplayArtifact"><rdfs:subClassOf rdf:resource="http://reliant.teknowledge.com/DAML/SUMO.owl#Artifact" /><rdfs:comment>Something for posting content so 

that it can be disseminated to the public.</rdfs:comment></rdfs:Class><rdfs:Class rdf:ID="DistilledAlcoholicBeverage"><rdfs:subClassOf rdf:resource="#AlcoholicBeverage" /><rdfs:comment>An AlcoholicBeverage that has 

had some part of its Water content removed by distillation.  This class 

covers drinks of unmixed, hard liquor.</rdfs:comment></rdfs:Class><rdfs:Class rdf:ID="Divorcing"><rdfs:subClassOf rdf:resource="http://reliant.teknowledge.com/DAML/SUMO.owl#Declaring" /><rdfs:comment>A legal act whereby a marriage is dissolved.</rdfs:comment></rdfs:Class><rdfs:Class rdf:ID="Documentary"><rdfs:subClassOf rdf:resource="#MotionPicture" /><rdfs:subClassOf rdf:resource="http://reliant.teknowledge.com/DAML/SUMO.owl#FactualText" /><rdfs:comment>A MotionPicture which purports to represent the 

facts about a person, event, etc.</rdfs:comment></rdfs:Class><rdfs:Class rdf:ID="Dodging"><rdfs:subClassOf rdf:resource="http://reliant.teknowledge.com/DAML/SUMO.owl#BodyMotion" /><rdfs:subClassOf rdf:resource="http://reliant.teknowledge.com/DAML/SUMO.owl#IntentionalProcess" /><rdfs:comment>Purposely moving one's body in such a way as 

to avoid being hit by something.</rdfs:comment></rdfs:Class><rdfs:Class rdf:ID="DomesticAnimal"><rdfs:subClassOf rdf:resource="http://reliant.teknowledge.com/DAML/SUMO.owl#Animal" /><sumo:disjoint rdf:resource="http://reliant.teknowledge.com/DAML/SUMO.owl#Human" /><rdfs:comment>Any Animal that is kept by a Human, as 

a pet, as livestock, for exhibition, etc.</rdfs:comment></rdfs:Class><rdfs:Class rdf:ID="DomesticCat"><rdfs:subClassOf rdf:resource="#DomesticAnimal" /><rdfs:subClassOf rdf:resource="http://reliant.teknowledge.com/DAML/SUMO.owl#Feline" /><rdfs:comment>A variety of Feline which has been domesticated 

by selective breeding.</rdfs:comment></rdfs:Class><rdfs:Class rdf:ID="DomesticDog"><rdfs:subClassOf rdf:resource="#DomesticAnimal" /><rdfs:subClassOf rdf:resource="http://reliant.teknowledge.com/DAML/SUMO.owl#Canine" /><rdfs:comment>Canines which have evolved from the common 

wolf by selective breeding.</rdfs:comment></rdfs:Class><rdfs:Class rdf:ID="Donkey"><rdfs:subClassOf rdf:resource="http://reliant.teknowledge.com/DAML/SUMO.owl#HoofedMammal" /><rdfs:subClassOf rdf:resource="#DomesticAnimal" /><rdfs:comment>A domesticated HoofedMammal that is used for 

work.</rdfs:comment></rdfs:Class><rdfs:Class rdf:ID="Door"><rdfs:subClassOf rdf:resource="http://reliant.teknowledge.com/DAML/SUMO.owl#Artifact" /><rdfs:comment>An Artifact that restricts and permits access to a 

StationaryArtifact (e.g. Building or Room) depending on whether the 

Door is open or locked.  Note that the class Door also covers gates, 

because it is not possible to define objective criteria that reliably 

distinguish doors from gates.</rdfs:comment></rdfs:Class><rdfs:Class rdf:ID="Doorway"><rdfs:subClassOf rdf:resource="http://reliant.teknowledge.com/DAML/SUMO.owl#StationaryArtifact" /><rdfs:comment>A StationaryArtifact consisting of a frame that 

holds a Door.</rdfs:comment></rdfs:Class><rdfs:Class rdf:ID="Dormitory"><rdfs:subClassOf rdf:resource="http://reliant.teknowledge.com/DAML/SUMO.owl#ResidentialBuilding" /><rdfs:subClassOf rdf:resource="http://reliant.teknowledge.com/DAML/SUMO.owl#TemporaryResidence" /><sumo:disjoint rdf:resource="http://reliant.teknowledge.com/DAML/SUMO.owl#SingleFamilyResidence" /><rdfs:comment>A TemporaryResidence which is owned by a School 

and which is used to house students while they take classes at the School.</rdfs:comment></rdfs:Class><rdfs:Class rdf:ID="Dough"><rdfs:subClassOf rdf:resource="#PreparedFood" /><rdfs:subClassOf rdf:resource="http://reliant.teknowledge.com/DAML/SUMO.owl#Mixture" /><rdfs:comment>A Mixture of Flour, Water, etc. which is used in 

making BreadOrBiscuits.</rdfs:comment></rdfs:Class><rdfs:Class rdf:ID="Downtown"><rdfs:subClassOf rdf:resource="#CityDistrict" /><rdfs:comment>The commercial center of a City.  The part of the 

City that contains more shops and offices than any other part.</rdfs:comment></rdfs:Class><rdfs:Class rdf:ID="DramaticActing"><rdfs:subClassOf rdf:resource="http://reliant.teknowledge.com/DAML/SUMO.owl#Pretending" /><rdfs:comment>Playing a character in a Performance, 

MotionPicture, etc.</rdfs:comment></rdfs:Class><rdfs:Class rdf:ID="DramaticCast"><rdfs:subClassOf rdf:resource="http://reliant.teknowledge.com/DAML/SUMO.owl#GroupOfPeople" /><rdfs:comment>The GroupOfPeople who engage in DramaticActing 

as part of the realization of a single FictionalText.</rdfs:comment></rdfs:Class><rdfs:Class rdf:ID="DramaticDirecting"><rdfs:subClassOf rdf:resource="http://reliant.teknowledge.com/DAML/SUMO.owl#Guiding" /><rdfs:comment>The process of directing a DramaticActing 

in a MotionPicture or the Performance of a DramaticPlay.</rdfs:comment></rdfs:Class><rdfs:Class rdf:ID="DramaticPerformance"><rdfs:subClassOf rdf:resource="#Performance" /><rdfs:comment>A Performance that consists exclusively of 

DramaticActing, e.g. a live performance of Death_of_a_Salesman in front 

of an audience.</rdfs:comment></rdfs:Class><rdfs:Class rdf:ID="DramaticPlay"><rdfs:subClassOf rdf:resource="http://reliant.teknowledge.com/DAML/SUMO.owl#FictionalText" /><rdfs:comment>A FictionalText that is intended to be realized 

as DramaticActing.</rdfs:comment></rdfs:Class><rdfs:Class rdf:ID="Drawing"><rdfs:subClassOf rdf:resource="http://reliant.teknowledge.com/DAML/SUMO.owl#ContentDevelopment" /><rdfs:subClassOf rdf:resource="http://reliant.teknowledge.com/DAML/SUMO.owl#SurfaceChange" /><rdfs:comment>Any ContentDevelopment that results in a Sketch.</rdfs:comment></rdfs:Class><rdfs:Class rdf:ID="DrawingACheck"><rdfs:subClassOf rdf:resource="#UsingAnAccount" /><rdfs:comment>An activity of paying by a check.</rdfs:comment></rdfs:Class><rdfs:Class rdf:ID="Dreaming"><rdfs:subClassOf rdf:resource="#Imagining" /><sumo:disjoint rdf:resource="http://reliant.teknowledge.com/DAML/SUMO.owl#IntentionalProcess" /><rdfs:comment>A Process of producing metal images which occurs 

while one is Asleep.</rdfs:comment></rdfs:Class><rdfs:Class rdf:ID="Dress"><rdfs:subClassOf rdf:resource="http://reliant.teknowledge.com/DAML/SUMO.owl#Clothing" /><rdfs:comment>An item of Clothing which covers the lower body 

(and possibly torso) of a Woman.</rdfs:comment></rdfs:Class><rdfs:Class rdf:ID="DressingRoom"><rdfs:subClassOf rdf:resource="http://reliant.teknowledge.com/DAML/SUMO.owl#Room" /><rdfs:comment>Any Room which is intended for 

ChangingClothing.</rdfs:comment></rdfs:Class><rdfs:Class rdf:ID="Drilling"><rdfs:subClassOf rdf:resource="http://reliant.teknowledge.com/DAML/SUMO.owl#IntentionalProcess" /><rdfs:subClassOf rdf:resource="http://reliant.teknowledge.com/DAML/SUMO.owl#SurfaceChange" /><rdfs:comment>Any Process of producing a hole in a 

SelfConnectedObject which involves rotating a long, thin bit.</rdfs:comment></rdfs:Class><rdfs:Class rdf:ID="Dripping"><rdfs:subClassOf rdf:resource="http://reliant.teknowledge.com/DAML/SUMO.owl#LiquidMotion" /><rdfs:comment>Any LiquidMotion where the Liquid is moved 

drop by drop.</rdfs:comment></rdfs:Class><rdfs:Class rdf:ID="DriveComponent"><rdfs:subClassOf rdf:resource="http://reliant.teknowledge.com/DAML/SUMO.owl#EngineeringComponent" /><rdfs:comment>An EngineeringComponent whose purpose is to 

transfer force from one part of a Device to another part.</rdfs:comment></rdfs:Class><rdfs:Class rdf:ID="DriversLicense"><rdfs:subClassOf rdf:resource="#License" /><rdfs:comment>A License which identifies the holder and 

indicates that he has the right to drive a certain class of RoadVehicle.</rdfs:comment></rdfs:Class><rdfs:Class rdf:ID="Driveway"><rdfs:subClassOf rdf:resource="http://reliant.teknowledge.com/DAML/SUMO.owl#Roadway" /><rdfs:comment>A small, private Roadway that is used for parking 

Automobiles or for connecting a Garage to a public Roadway.</rdfs:comment></rdfs:Class><rdfs:Class rdf:ID="Drought"><rdfs:subClassOf rdf:resource="http://reliant.teknowledge.com/DAML/SUMO.owl#WeatherProcess" /><rdfs:comment>Drought is the subclass of WeatherProcess 

that represents long periods without precipitation, which is damaging 

to crops, livestock, and human life.</rdfs:comment></rdfs:Class><rdfs:Class rdf:ID="DrugStore"><rdfs:subClassOf rdf:resource="#RetailStore" /><rdfs:comment>A RetailStore that sells Medicine, and 

perhaps other items as well.</rdfs:comment></rdfs:Class><rdfs:Class rdf:ID="Drum"><rdfs:subClassOf rdf:resource="#PercussionInstrument" /><rdfs:comment>An atonal PercussionInstrument which consists of a 

hollow cylinder and a fabric stretched across at least one end of the 

cylinder.</rdfs:comment></rdfs:Class><rdfs:Class rdf:ID="DryWinterColdClimateZone"><rdfs:subClassOf rdf:resource="#ColdClimateZone" /><rdfs:comment>DryWinterColdClimateZone 

is a subclass of ColdClimateZone that is characterized by having 

at least ten times as much precipitation in the wettest summer month 

as in the driest winter month.  This is Koeppen climate system subtype 

'Dw'.</rdfs:comment></rdfs:Class><rdfs:Class rdf:ID="Duck"><rdfs:subClassOf rdf:resource="http://reliant.teknowledge.com/DAML/SUMO.owl#Bird" /><rdfs:comment>A subclass of Bird with webbed feet and a large bill.  

Some ducks live in the wild, and some are raised for meat and/or eggs.</rdfs:comment></rdfs:Class><rdfs:Class rdf:ID="DutyTax"><rdfs:subClassOf rdf:resource="#Tax" /><rdfs:comment>A Tax that is levied on imports and/or exports.</rdfs:comment></rdfs:Class><rdfs:Class rdf:ID="Ear"><rdfs:subClassOf rdf:resource="http://reliant.teknowledge.com/DAML/SUMO.owl#Organ" /><rdfs:subClassOf rdf:resource="http://reliant.teknowledge.com/DAML/SUMO.owl#AnimalAnatomicalStructure" /><rdfs:comment>The Organ of hearing.</rdfs:comment></rdfs:Class><rdfs:Class rdf:ID="EarthTremor"><rdfs:subClassOf rdf:resource="#Tremor" /><rdfs:subClassOf rdf:resource="http://reliant.teknowledge.com/DAML/SUMO.owl#GeologicalProcess" /><rdfs:comment>An EarthTremor is an individual seismic 

event in which the earth shakes due to release of seismic pressures.</rdfs:comment></rdfs:Class><rdfs:Class rdf:ID="Earthquake"><rdfs:subClassOf rdf:resource="http://reliant.teknowledge.com/DAML/SUMO.owl#GeologicalProcess" /><rdfs:comment>Earthquake is the class of events in 

which the earth shakes while its layers readjust due to tensional 

stresses in the surface of the earth.  A single earthquake may consist 

of one or more EarthTremors.</rdfs:comment></rdfs:Class><rdfs:Class rdf:ID="Echoing"><rdfs:subClassOf rdf:resource="http://reliant.teknowledge.com/DAML/SUMO.owl#RadiatingSound" /><rdfs:comment>Instances of RadiatingSound where the instrument 

is a surface which bounces sound waves back to their origin, where they can 

be heard again.</rdfs:comment></rdfs:Class><rdfs:Class rdf:ID="EconomicAttribute"><rdfs:subClassOf rdf:resource="#PoliticoEconomicAttribute" /><rdfs:comment>EconomicAttribute is the class 

of terms including all Attributes used to characterize the 

economic systems or development levels of Nations or dependent 

GeopoliticalAreas.</rdfs:comment></rdfs:Class><rdfs:Class rdf:ID="EconomicRelation"><rdfs:subClassOf rdf:resource="http://reliant.teknowledge.com/DAML/SUMO.owl#BinaryRelation" /><rdfs:comment>A class of Relations which are used 

to specify various economic measures, e.g. the GDP, the consumer price 

index, and the trade deficit.</rdfs:comment></rdfs:Class><rdfs:Class rdf:ID="EconomicSystemAttribute"><rdfs:subClassOf rdf:resource="#EconomicAttribute" /><rdfs:comment>EconomicSystemAttribute 

is the class of Attributes that describe the type of economic 

system that a country or area has.  For example, CapitalistEconomy 

or SocialistEconomy.</rdfs:comment></rdfs:Class><rdfs:Class rdf:ID="EducationalCourse"><rdfs:subClassOf rdf:resource="#EducationalProgram" /><rdfs:comment>A schedule of class meetings offered by an 

EducationalOrganization.</rdfs:comment></rdfs:Class><rdfs:Class rdf:ID="EducationalProgram"><rdfs:subClassOf rdf:resource="http://reliant.teknowledge.com/DAML/SUMO.owl#Plan" /><rdfs:comment>A series of EducationalCourses that must 

be completed to receive an AcademicDegree or other Certificate.  Note that 

an EducationalProgram, unlike an EducationalCourse, may be realized at more 

than one EducationalOrganization.</rdfs:comment></rdfs:Class><rdfs:Class rdf:ID="Elbow"><rdfs:subClassOf rdf:resource="#BodyJoint" /><rdfs:comment>The joint in the Arm connecting the forearm and the 

upper arm.</rdfs:comment></rdfs:Class><rdfs:Class rdf:ID="ElectoralCollegeElection"><rdfs:subClassOf rdf:resource="#GeneralElection" /><rdfs:comment>ElectoralCollegeElection is 

the class of Elections in which the outcome is decided by the votes of 

electors who have been chosen by popular vote, rather than directly by 

results of the popular vote.  ElectoralCollegeElection is an indirect 

method of election, in contrast to PopularElection.</rdfs:comment></rdfs:Class><rdfs:Class rdf:ID="ElectricDevice"><rdfs:subClassOf rdf:resource="http://reliant.teknowledge.com/DAML/SUMO.owl#Device" /><rdfs:comment>Any Device that is powered by electricity.</rdfs:comment></rdfs:Class><rdfs:Class rdf:ID="ElectricMotor"><rdfs:subClassOf rdf:resource="#Engine" /><rdfs:subClassOf rdf:resource="#ElectricDevice" /><rdfs:comment>ElectricMotor is the subclass of Engines 

that produce mechanical power from electricity.</rdfs:comment></rdfs:Class><rdfs:Class rdf:ID="ElectricalSignalling"><rdfs:subClassOf rdf:resource="#Signalling" /><rdfs:comment>ElectricalSignalling is the 

subclass of Signalling processes that involve control of an electrical 

current.  Cf. ElectronicSignalling.</rdfs:comment></rdfs:Class><rdfs:Class rdf:ID="ElectrifiedRailwayCar"><rdfs:subClassOf rdf:resource="#RollingStock" /><rdfs:subClassOf rdf:resource="#SelfPoweredVehicle" /><rdfs:subClassOf rdf:resource="#ElectricDevice" /><rdfs:comment>ElectrifiedRailwayCar is the 

subclass of railway cars that are powered by electricity, which is 

provided to the car through an overhead link or electrified third rail.</rdfs:comment></rdfs:Class><rdfs:Class rdf:ID="ElectronVolt"><rdfs:subClassOf rdf:resource="http://reliant.teknowledge.com/DAML/SUMO.owl#FunctionQuantity" /><rdf:type rdf:resource="http://reliant.teknowledge.com/DAML/SUMO.owl#UnitOfMeasure" /><rdfs:comment>The ElectronVolt is an energy measure.  

Symbol: eV.  It is the kinetic energy acquired by an electron in passing 

through a potential difference of 1 Volt in a vacuum.</rdfs:comment></rdfs:Class><rdfs:Class rdf:ID="ElectronicSignalling"><rdfs:subClassOf rdf:resource="#Signalling" /><rdfs:comment>ElectronicSignalling is the 

subclass of Signalling processes that involve a signal generated by 

a computer.</rdfs:comment></rdfs:Class><rdfs:Class rdf:ID="Elephant"><rdfs:subClassOf rdf:resource="#Herbivore" /><rdfs:comment>A very large, almost hairless Herbivore with a long 

trunk.</rdfs:comment></rdfs:Class><rdfs:Class rdf:ID="Elevator"><rdfs:subClassOf rdf:resource="http://reliant.teknowledge.com/DAML/SUMO.owl#TransportationDevice" /><rdfs:comment>A TransportationDevice consisting of a car that moves 

up and down in a vertical shaft so that people can move from one floor to another 

in a building.</rdfs:comment></rdfs:Class><rdfs:Class rdf:ID="Embracing"><rdfs:subClassOf rdf:resource="http://reliant.teknowledge.com/DAML/SUMO.owl#Touching" /><rdfs:comment>The class of Touching processes where one Human 

hugs another one.</rdfs:comment></rdfs:Class><rdfs:Class rdf:ID="EmergencyRoadVehicle"><rdfs:subClassOf rdf:resource="#EmergencyVehicle" /><rdfs:subClassOf rdf:resource="#SelfPoweredRoadVehicle" /><rdfs:comment>EmergencyRoadVehicle is the 

subclass of EmergencyVehicle that includes RoadVehicles designed 

for special use in emergencies, e.g., Ambulances, FireEngines.</rdfs:comment></rdfs:Class><rdfs:Class rdf:ID="EmergencyVehicle"><rdfs:subClassOf rdf:resource="#SelfPoweredVehicle" /><rdfs:comment>EmergencyVehicle is the subclass of 

Vehicles that are used for special-purpose emergency response.</rdfs:comment></rdfs:Class><rdfs:Class rdf:ID="EmploymentFiring"><rdfs:subClassOf rdf:resource="http://reliant.teknowledge.com/DAML/SUMO.owl#TerminatingEmployment" /><rdfs:comment>Involuntarily ending one's employment.  

Note that this covers termination due to inadequate performance, as 

well as layoffs.</rdfs:comment></rdfs:Class><rdfs:Class rdf:ID="Engine"><rdfs:subClassOf rdf:resource="#Transducer" /><rdfs:comment>Engine is a subclass of Transducer.  Engines 

are devices for converting some form of energy resource into mechanical 

power.</rdfs:comment></rdfs:Class><rdfs:Class rdf:ID="EntertainmentCompany"><rdfs:subClassOf rdf:resource="http://reliant.teknowledge.com/DAML/SUMO.owl#CommercialAgent" /><rdfs:comment>Any business whose services include 

Performances.  This class covers nightclubs, commercial live theaters, 

and comedy clubs.</rdfs:comment></rdfs:Class><rdfs:Class rdf:ID="EntertainmentProfession"><rdfs:subClassOf rdf:resource="#SkilledOccupation" /><rdfs:comment>Positions which involve creating 

content or performances that are intended to entertain.  This class covers 

the TheaterProfession, FilmMakingProfession, being a comedian, etc.</rdfs:comment></rdfs:Class><rdfs:Class rdf:ID="Entombing"><rdfs:subClassOf rdf:resource="http://reliant.teknowledge.com/DAML/SUMO.owl#Putting" /><rdfs:comment>More commonly known as burying, this is the class 

of processes of putting a HumanCorpse into a Tomb.  Note that this class 

is not a subclass of Burying, since some Tombs are not covered with Soil, 

e.g. those in a mausoleum.</rdfs:comment></rdfs:Class><rdfs:Class rdf:ID="Envelope"><rdfs:subClassOf rdf:resource="#Container" /><rdfs:comment>A sealable Container for one or more pieces of 

paper which is designed to protect the papers while they are transferred to 

someone.</rdfs:comment></rdfs:Class><rdfs:Class rdf:ID="Enzyme"><rdfs:subClassOf rdf:resource="http://reliant.teknowledge.com/DAML/SUMO.owl#Protein" /><rdfs:comment>A complex Protein that is produced by living 

cells and which catalyzes specific biochemical reactions. There are six 

main types of enzymes:  oxidoreductases, transferases, hydrolases, 

lyases, isomerases, and ligases.</rdfs:comment></rdfs:Class><rdfs:Class rdf:ID="Erosion"><rdfs:subClassOf rdf:resource="http://reliant.teknowledge.com/DAML/SUMO.owl#GeologicalProcess" /><rdfs:subClassOf rdf:resource="http://reliant.teknowledge.com/DAML/SUMO.owl#Removing" /><rdfs:comment>Erosion is the subclass of Removing processes 

in which rock and soil material are removed from LandForms in one area 

and deposited elsewhere by wind, running water, ice, heat, and other 

GeologicalProcesses.</rdfs:comment></rdfs:Class><rdfs:Class rdf:ID="Escaping"><rdfs:subClassOf rdf:resource="http://reliant.teknowledge.com/DAML/SUMO.owl#Translocation" /><rdfs:comment>Any instance of Translocation where the agent brings 

it about that he/she is no longer confined without having the right to do 

so.</rdfs:comment></rdfs:Class><rdfs:Class rdf:ID="Espionage"><rdfs:subClassOf rdf:resource="http://reliant.teknowledge.com/DAML/SUMO.owl#PoliticalProcess" /><rdfs:subClassOf rdf:resource="http://reliant.teknowledge.com/DAML/SUMO.owl#Investigating" /><rdfs:comment>Any Investigating by one Government of another 

Government where the second Government does not know that it is being 

spied upon.</rdfs:comment></rdfs:Class><rdfs:Class rdf:ID="EuropeanCity"><rdfs:subClassOf rdf:resource="http://reliant.teknowledge.com/DAML/SUMO.owl#City" /><rdfs:comment>The class of cities that are in Europe.</rdfs:comment></rdfs:Class><rdfs:Class rdf:ID="EuropeanNation"><rdfs:subClassOf rdf:resource="http://reliant.teknowledge.com/DAML/SUMO.owl#Nation" /><rdfs:comment>The class of nations that are in Europe.</rdfs:comment></rdfs:Class><rdfs:Class rdf:ID="Execution"><rdfs:subClassOf rdf:resource="http://reliant.teknowledge.com/DAML/SUMO.owl#Killing" /><rdfs:comment>Killing of a Human by a Government for 

the commission of a CriminalAction.</rdfs:comment></rdfs:Class><rdfs:Class rdf:ID="ExecutiveResidence"><rdfs:subClassOf rdf:resource="http://reliant.teknowledge.com/DAML/SUMO.owl#PermanentResidence" /><rdfs:comment>A Residence of a chiefOfState, e.g. 

the White House, a state governor's mansion, Buckingham Palace, etc.</rdfs:comment></rdfs:Class><rdfs:Class rdf:ID="Exhaling"><rdfs:subClassOf rdf:resource="http://reliant.teknowledge.com/DAML/SUMO.owl#Breathing" /><rdfs:comment>Any instance of Breathing where the breath is 

expelled from the Lungs.</rdfs:comment></rdfs:Class><rdfs:Class rdf:ID="Explosion"><rdfs:subClassOf rdf:resource="http://reliant.teknowledge.com/DAML/SUMO.owl#Radiating" /><rdfs:comment>Any sudden and massive release of energy that is 

the product of a chemical reaction.</rdfs:comment></rdfs:Class><rdfs:Class rdf:ID="ExplosiveDevice"><rdfs:subClassOf rdf:resource="http://reliant.teknowledge.com/DAML/SUMO.owl#Device" /><rdfs:comment>A Device whose purpose is to explode.  Note 

that ExplosiveDevice is not a subclass of Weapon, since explosives can be 

used in demolition work and in fireworks displays, for example.</rdfs:comment></rdfs:Class><rdfs:Class rdf:ID="ExplosiveMine"><rdfs:subClassOf rdf:resource="#ExplosiveDevice" /><rdfs:subClassOf rdf:resource="http://reliant.teknowledge.com/DAML/SUMO.owl#Weapon" /><rdfs:comment>An ExplosiveDevice which is designed to 

explode when there is movement over it, e.g. by a person on foot, by a 

RoadVehicle, etc.</rdfs:comment></rdfs:Class><rdfs:Class rdf:ID="ExplosiveSubstance"><rdfs:subClassOf rdf:resource="http://reliant.teknowledge.com/DAML/SUMO.owl#Substance" /><rdfs:comment>Any Substance which is capable of exploding.</rdfs:comment></rdfs:Class><rdfs:Class rdf:ID="Exporting"><rdfs:subClassOf rdf:resource="http://reliant.teknowledge.com/DAML/SUMO.owl#FinancialTransaction" /><rdfs:comment>Exporting is the class of actions in 

which there is a ChangeOfPossession of goods shipped from a 

provider in one Nation to a destination in another Nation. 

Typically, there are Selling and Buying events associated 

with an Exporting.  Either the seller or the exporting country 

may be considered the origin of Exporting.</rdfs:comment></rdfs:Class><rdfs:Class rdf:ID="ExpressingApproval"><rdfs:subClassOf rdf:resource="http://reliant.teknowledge.com/DAML/SUMO.owl#Expressing" /><rdfs:comment>Expressing favor about a physical thing 

or a state of affairs.</rdfs:comment></rdfs:Class><rdfs:Class rdf:ID="ExpressingDisapproval"><rdfs:subClassOf rdf:resource="http://reliant.teknowledge.com/DAML/SUMO.owl#Expressing" /><rdfs:comment>Expressing disfavor about a physical 

thing or a state of affairs.</rdfs:comment></rdfs:Class><rdfs:Class rdf:ID="ExpressingFarewell"><rdfs:subClassOf rdf:resource="http://reliant.teknowledge.com/DAML/SUMO.owl#Expressing" /><rdfs:comment>Any instance of Expressing an acknowledgment 

of a person's departure.  Note that this class is not a subclass of 

LinguisticCommunication, because it covers gestures of departure, e.g. Waving 

and Nodding in certain circumstances.</rdfs:comment></rdfs:Class><rdfs:Class rdf:ID="Expressway"><rdfs:subClassOf rdf:resource="#SurfacedRoadway" /><rdfs:comment>Expressway is the subclass of 

SurfacedRoadways that are multiple-lane, limited-access highways 

designed for rapid travel by MotorVehicles.</rdfs:comment></rdfs:Class><rdfs:Class rdf:ID="Eye"><rdfs:subClassOf rdf:resource="http://reliant.teknowledge.com/DAML/SUMO.owl#Organ" /><rdfs:subClassOf rdf:resource="http://reliant.teknowledge.com/DAML/SUMO.owl#AnimalAnatomicalStructure" /><rdfs:comment>The Organ of sight.</rdfs:comment></rdfs:Class><rdfs:Class rdf:ID="EyeGlass"><rdfs:subClassOf rdf:resource="#OpticalDevice" /><rdfs:comment>A lens or pair of lenses with or without frames whose 

purpose is to to correct a defect in vision.  This class covers ordinary eye 

glasses, reading glasses, contact lenses, monocles, etc.</rdfs:comment></rdfs:Class><rdfs:Class rdf:ID="EyeMotion"><rdfs:subClassOf rdf:resource="http://reliant.teknowledge.com/DAML/SUMO.owl#BodyMotion" /><rdfs:comment>Any Motion where a patient is the agent's 

own Eyelid or Eyelids.</rdfs:comment></rdfs:Class><rdfs:Class rdf:ID="Eyelid"><rdfs:subClassOf rdf:resource="#Skin" /><rdfs:comment>Folds of Skin that can be manipulated to 

cover or uncover Eyes.</rdfs:comment></rdfs:Class><rdfs:Class rdf:ID="FabricArtifact"><rdfs:subClassOf rdf:resource="http://reliant.teknowledge.com/DAML/SUMO.owl#Artifact" /><rdfs:comment>Any Artifact that is made out of Fabric.</rdfs:comment></rdfs:Class><rdfs:Class rdf:ID="Face"><rdfs:subClassOf rdf:resource="http://reliant.teknowledge.com/DAML/SUMO.owl#AnimalAnatomicalStructure" /><rdfs:subClassOf rdf:resource="http://reliant.teknowledge.com/DAML/SUMO.owl#BodyPart" /><rdfs:comment>The part of the Head from forehead to chin and 

from ear to ear.</rdfs:comment></rdfs:Class><rdfs:Class rdf:ID="FacialExpression"><rdfs:subClassOf rdf:resource="http://reliant.teknowledge.com/DAML/SUMO.owl#Gesture" /><rdfs:comment>Any Gesture whose instrument is the Face.</rdfs:comment></rdfs:Class><rdfs:Class rdf:ID="FacialHair"><rdfs:subClassOf rdf:resource="#Hair" /><rdfs:comment>Hair that grows on the Face.  This 

class covers bears, mustaches, sideburns, midnight shadow, etc.</rdfs:comment></rdfs:Class><rdfs:Class rdf:ID="Fact"><rdfs:subClassOf rdf:resource="#Statement" /><rdfs:comment>The class of Statements that are True.</rdfs:comment></rdfs:Class><rdfs:Class rdf:ID="Factory"><rdfs:subClassOf rdf:resource="http://reliant.teknowledge.com/DAML/SUMO.owl#Building" /><rdfs:comment>A building intended to house a process that 

produces goods of some value.</rdfs:comment></rdfs:Class><rdfs:Class rdf:ID="FallSeason"><rdfs:subClassOf rdf:resource="#SeasonOfYear" /><rdfs:comment>The SeasonOfYear that begins at the autumnal 

equinox and ends at the winter solstice.</rdfs:comment></rdfs:Class><rdfs:Class rdf:ID="Falling"><rdfs:subClassOf rdf:resource="http://reliant.teknowledge.com/DAML/SUMO.owl#Translocation" /><rdfs:subClassOf rdf:resource="#MotionDownward" /><sumo:disjoint rdf:resource="http://reliant.teknowledge.com/DAML/SUMO.owl#IntentionalProcess" /><rdfs:comment>The class of Translocations where 

something moves from a higher location to a lower location 

under the force of gravity and without intending to do so.</rdfs:comment></rdfs:Class><rdfs:Class rdf:ID="FallingAsleep"><rdfs:subClassOf rdf:resource="http://reliant.teknowledge.com/DAML/SUMO.owl#PsychologicalProcess" /><sumo:disjoint rdf:resource="#WakingUp" /><rdfs:comment>The process of transitioning from a state of 

being Awake to a state of being Asleep.</rdfs:comment></rdfs:Class><rdfs:Class rdf:ID="Fallout"><rdfs:subClassOf rdf:resource="#Powder" /><rdfs:comment>Radioactive powder that is typically dispersed by 

the explosion of a nuclear weapon.</rdfs:comment></rdfs:Class><rdfs:Class rdf:ID="FamilyBusiness"><rdfs:subClassOf rdf:resource="#Partnership" /><rdfs:comment>A Partnership that is owned by a single 

family.</rdfs:comment></rdfs:Class><rdfs:Class rdf:ID="FanDevice"><rdfs:subClassOf rdf:resource="#CoolingDevice" /><rdfs:comment>A CoolingDevice which consists simply of one or more 

blades that circulate the air.  Note that this class covers both electrical fans 

and fans that are manually operated.</rdfs:comment></rdfs:Class><rdfs:Class rdf:ID="Farad"><rdfs:subClassOf rdf:resource="http://reliant.teknowledge.com/DAML/SUMO.owl#FunctionQuantity" /><rdf:type rdf:resource="http://reliant.teknowledge.com/DAML/SUMO.owl#SystemeInternationalUnit" /><rdfs:comment>SI capacitance measure.  Symbol: F.  It is the 

capacitance of a capacitator between the plates of which there appears 

a difference of potential of 1 Volt when it is charged by a quantity 

of electricity equal to 1 Coulomb.  Farad = C/V = 

m^(-2)*kg(-1)*s^4*A^2.</rdfs:comment></rdfs:Class><rdfs:Class rdf:ID="Farm"><rdfs:subClassOf rdf:resource="http://reliant.teknowledge.com/DAML/SUMO.owl#StationaryArtifact" /><rdfs:comment>A StationaryArtifact consisting of a cultivated 

LandArea and Buildings for maintaining the land and/or the Animals 

on the land.</rdfs:comment></rdfs:Class><rdfs:Class rdf:ID="FarmBuilding"><rdfs:subClassOf rdf:resource="http://reliant.teknowledge.com/DAML/SUMO.owl#Building" /><sumo:disjoint rdf:resource="http://reliant.teknowledge.com/DAML/SUMO.owl#ResidentialBuilding" /><rdfs:comment>A Building on a Farm that is used for keeping 

DomesticAnimals, Fodder or harvested crops.</rdfs:comment></rdfs:Class><rdfs:Class rdf:ID="FarmHand"><rdfs:subClassOf rdf:resource="#OccupationalTrade" /><rdfs:comment>OccupationalTrades which involve Agriculture.</rdfs:comment></rdfs:Class><rdfs:Class rdf:ID="Feather"><rdfs:subClassOf rdf:resource="http://reliant.teknowledge.com/DAML/SUMO.owl#AnimalAnatomicalStructure" /><rdfs:subClassOf rdf:resource="http://reliant.teknowledge.com/DAML/SUMO.owl#BodyPart" /><rdfs:comment>Each instance of this class is one of the structures 

that make up the external covering of Birds.</rdfs:comment></rdfs:Class><rdfs:Class rdf:ID="Feeding"><rdfs:subClassOf rdf:resource="http://reliant.teknowledge.com/DAML/SUMO.owl#Giving" /><rdfs:comment>Giving Food to a Human or Animal.</rdfs:comment></rdfs:Class><rdfs:Class rdf:ID="FemaleCow"><rdfs:subClassOf rdf:resource="#Cow" /><rdfs:comment>A Cow that is Female.</rdfs:comment></rdfs:Class><rdfs:Class rdf:ID="Fence"><rdfs:subClassOf rdf:resource="http://reliant.teknowledge.com/DAML/SUMO.owl#StationaryArtifact" /><rdfs:comment>A StationaryArtifact that serves to demarcate or

to prevent access to or from the area that the Fence surrounds.</rdfs:comment></rdfs:Class><rdfs:Class rdf:ID="Fertilizer"><rdfs:subClassOf rdf:resource="http://reliant.teknowledge.com/DAML/SUMO.owl#Mixture" /><rdfs:comment>Any Mixture which is used to provide nutrients to 

living Plants.  Fertilizers can be made up of plant or animal material, e.g. 

compost, or they can be entirely synthetic, e.g. ammonium nitrate.</rdfs:comment></rdfs:Class><rdfs:Class rdf:ID="Field"><rdfs:subClassOf rdf:resource="http://reliant.teknowledge.com/DAML/SUMO.owl#LandArea" /><rdfs:comment>A LandArea that has been cleared of BotanicalTrees.  

Note that a Field is not necessarily used for the cultivation of crops and 

that a Field may be small.</rdfs:comment></rdfs:Class><rdfs:Class rdf:ID="Fighter"><rdfs:subClassOf rdf:resource="#MilitaryAircraft" /><rdfs:comment>Any high-speed MilitaryAircraft whose purpose is 

to destroy enemy MilitaryAircraft.</rdfs:comment></rdfs:Class><rdfs:Class rdf:ID="FileDevice"><rdfs:subClassOf rdf:resource="http://reliant.teknowledge.com/DAML/SUMO.owl#Device" /><rdfs:comment>A Device whose purpose is to make something 

smoother by removing small particles from an Object.  For example, a nail 

file is used to even out the tips of one's finger nails.</rdfs:comment></rdfs:Class><rdfs:Class rdf:ID="FillingAnOrder"><rdfs:subClassOf rdf:resource="http://reliant.teknowledge.com/DAML/SUMO.owl#FinancialTransaction" /><rdfs:comment>Execute an order or buy or sell a Security.</rdfs:comment></rdfs:Class><rdfs:Class rdf:ID="FilmDirector"><rdfs:subClassOf rdf:resource="#FilmMakingProfession" /><rdfs:comment>Positions which involve directing MotionPictures.</rdfs:comment></rdfs:Class><rdfs:Class rdf:ID="FilmMaking"><rdfs:subClassOf rdf:resource="http://reliant.teknowledge.com/DAML/SUMO.owl#ContentDevelopment" /><rdfs:comment>ContentDevelopment where the result is a 

MotionPicture.</rdfs:comment></rdfs:Class><rdfs:Class rdf:ID="FilmMakingProfession"><rdfs:subClassOf rdf:resource="#EntertainmentProfession" /><rdfs:comment>Positions which involve FilmMaking, 

i.e. acting in films, directing films, producing films, etc.</rdfs:comment></rdfs:Class><rdfs:Class rdf:ID="FilmProducer"><rdfs:subClassOf rdf:resource="#FilmMakingProfession" /><rdfs:comment>Positions which involve producing MotionPictures, 

i.e arranging the financing for the MotionPicture and supervising its production.</rdfs:comment></rdfs:Class><rdfs:Class rdf:ID="Filter"><rdfs:subClassOf rdf:resource="http://reliant.teknowledge.com/DAML/SUMO.owl#Device" /><rdfs:comment>A Device whose purpose is to remove part of a 

Solution that is passed through the Filter.</rdfs:comment></rdfs:Class><rdfs:Class rdf:ID="FinancialAccount"><sumo:subAttribute rdf:resource="http://reliant.teknowledge.com/DAML/SUMO.owl#Contract" /><rdfs:comment>A formal banking, brokerage, or business 

relationship established to provide for regular services, dealings, and 

other financial transactions.</rdfs:comment></rdfs:Class><rdfs:Class rdf:ID="FinancialBank"><rdfs:subClassOf rdf:resource="#FinancialCompany" /><rdfs:comment>An organization, chartered by a state 

or federal government, which does most or all of the following: receives 

Deposits, honors FinancialInstruments drawn on them, and pays 

interest on them; discounts Notes, makes Loans, and invests in 

SecuredLoans; collects Checks, Drafts and Notes, certifies 

depositor's checks; and issues drafts and Cashier's checks.</rdfs:comment></rdfs:Class><rdfs:Class rdf:ID="FinancialBill"><rdfs:subClassOf rdf:resource="#FinancialText" /><rdfs:comment>A brief statement that the stated amount 

of money is owed by the person to whom the bill is delivered.</rdfs:comment></rdfs:Class><rdfs:Class rdf:ID="FinancialCompany"><rdfs:subClassOf rdf:resource="http://reliant.teknowledge.com/DAML/SUMO.owl#CommercialAgent" /><rdfs:comment>The class FinancialCompany 

includes, as subclasses, FinancialBank, CreditUnion and SavingsAndLoan.</rdfs:comment></rdfs:Class><rdfs:Class rdf:ID="FinancialService"><rdfs:subClassOf rdf:resource="http://reliant.teknowledge.com/DAML/SUMO.owl#CommercialService" /><rdfs:comment>Services performed by 

FinancialOrganizations.</rdfs:comment></rdfs:Class><rdfs:Class rdf:ID="FinancialText"><rdfs:subClassOf rdf:resource="#Report" /><rdfs:comment>A Report about monetary figures.  This 

class covers FinancialBills, balance sheets, account statements, etc.</rdfs:comment></rdfs:Class><rdfs:Class rdf:ID="Financing"><rdfs:subClassOf rdf:resource="http://reliant.teknowledge.com/DAML/SUMO.owl#Funding" /><rdfs:subClassOf rdf:resource="#FinancialService" /><rdfs:comment>Any Funding which is provided by a FinancialCompany 

with the aim of making a profit on the money invested.</rdfs:comment></rdfs:Class><rdfs:Class rdf:ID="Finger"><rdfs:subClassOf rdf:resource="#DigitAppendage" /><rdfs:comment>The five extremities of Hands.</rdfs:comment></rdfs:Class><rdfs:Class rdf:ID="Fingerprint"><rdfs:subClassOf rdf:resource="http://reliant.teknowledge.com/DAML/SUMO.owl#ShapeAttribute" /><rdfs:subClassOf rdf:resource="http://reliant.teknowledge.com/DAML/SUMO.owl#BiologicalAttribute" /><rdfs:comment>That pattern of arches, loops, and whorls that mark 

the imprint of a Finger.</rdfs:comment></rdfs:Class><rdfs:Class rdf:ID="FireEngine"><rdfs:subClassOf rdf:resource="#EmergencyRoadVehicle" /><rdfs:comment>FireEngine is the subclass of 

EmergencyRoadVehicles that represents fire engines.</rdfs:comment></rdfs:Class><rdfs:Class rdf:ID="Firearm"><rdfs:subClassOf rdf:resource="#Gun" /><rdfs:comment>A Gun that is small enough to be carried and fired by 

a single Human.</rdfs:comment></rdfs:Class><rdfs:Class rdf:ID="Fireplace"><rdfs:subClassOf rdf:resource="http://reliant.teknowledge.com/DAML/SUMO.owl#StationaryArtifact" /><rdfs:subClassOf rdf:resource="http://reliant.teknowledge.com/DAML/SUMO.owl#Device" /><rdfs:comment>A Device in a Building which is used for burning wood, 

coal, etc for heat.</rdfs:comment></rdfs:Class><rdfs:Class rdf:ID="FishMeat"><rdfs:subClassOf rdf:resource="http://reliant.teknowledge.com/DAML/SUMO.owl#Meat" /><rdfs:comment>Meat that was originally part of a Fish.</rdfs:comment></rdfs:Class><rdfs:Class rdf:ID="Fishing"><rdfs:subClassOf rdf:resource="#Hunting" /><rdfs:comment>Fishing is the class of Processes in which 

Fish are hunted.</rdfs:comment></rdfs:Class><rdfs:Class rdf:ID="FixedHoliday"><rdfs:subClassOf rdf:resource="#Holiday" /><rdfs:comment>FixedHoliday is the class of Holidays 

whose observance is fixed to recurrences of the calendar day that the 

holiday commemorates.</rdfs:comment></rdfs:Class><rdfs:Class rdf:ID="Flag"><rdfs:subClassOf rdf:resource="http://reliant.teknowledge.com/DAML/SUMO.owl#Icon" /><rdfs:comment>An Icon made of Fabric that refers to a particular 

GeopoliticalArea.</rdfs:comment></rdfs:Class><rdfs:Class rdf:ID="Flooding"><rdfs:subClassOf rdf:resource="http://reliant.teknowledge.com/DAML/SUMO.owl#LiquidMotion" /><rdfs:comment>Flooding is the subclass of LiquidMotion 

processes in which the water level of a Waterway rises or water spreads 

over a flood plain along a Waterway.</rdfs:comment></rdfs:Class><rdfs:Class rdf:ID="Floor"><rdfs:subClassOf rdf:resource="http://reliant.teknowledge.com/DAML/SUMO.owl#StationaryArtifact" /><rdfs:comment>A StationaryArtifact that is the bottom surface 

of a Room.</rdfs:comment></rdfs:Class><rdfs:Class rdf:ID="Flour"><rdfs:subClassOf rdf:resource="#PreparedFood" /><rdfs:subClassOf rdf:resource="#Powder" /><rdfs:comment>A Powder that is prepared from CerealGrain, e.g. 

wheat flour, rice flour, etc.  Flour is most often used in the making 

of BreadOrBiscuits.</rdfs:comment></rdfs:Class><rdfs:Class rdf:ID="FlowRegion"><rdfs:subClassOf rdf:resource="http://reliant.teknowledge.com/DAML/SUMO.owl#SelfConnectedObject" /><rdfs:comment>FlowRegion is a class of things whose 

boundaries are relatively stable but whose constitutive material is 

continuously moving through the region itself and being replaced by 

other, similar material.  Each FlowRegion is constituted by a stream 

of matter moving as a whole.  A FlowRegion may be liquid or gaseous.  

A wind may be considered as a Process or as a FlowRegion, similarly 

an ocean current or a WaterWave.  Note that certain 

properties belong to the FlowRegion itself (e.g., mass, length, volume, 

temperature, and speed or velocity of the region moving as a whole), 

while other properties of interest belong to the Motion of its 

constitutive stuff (e.g., velocity, direction).  The motion of 

a FlowRegion as a whole (e.g. the jet stream moves within the atmosphere) 

is distinguished from the motion of the pieces of stuff constituting the 

FlowRegion.</rdfs:comment></rdfs:Class><rdfs:Class rdf:ID="Flower"><rdfs:subClassOf rdf:resource="http://reliant.teknowledge.com/DAML/SUMO.owl#PlantAnatomicalStructure" /><rdfs:subClassOf rdf:resource="http://reliant.teknowledge.com/DAML/SUMO.owl#Organ" /><rdfs:comment>The reproductive organ of FloweringPlants.</rdfs:comment></rdfs:Class><rdfs:Class rdf:ID="FluidContainer"><rdfs:subClassOf rdf:resource="#Container" /><rdfs:comment>A Container which is used to store Fluids,  

i.e. Liquids and Gases.</rdfs:comment></rdfs:Class><rdfs:Class rdf:ID="FlyInsect"><rdfs:subClassOf rdf:resource="http://reliant.teknowledge.com/DAML/SUMO.owl#Insect" /><rdfs:comment>Insects with Wings and two Limbs.</rdfs:comment></rdfs:Class><rdfs:Class rdf:ID="Flying"><rdfs:subClassOf rdf:resource="http://reliant.teknowledge.com/DAML/SUMO.owl#Translocation" /><rdfs:comment>Any instance of Translocation which is through an 

AtmosphericRegion and which is powered by the Wings of an Animal.</rdfs:comment></rdfs:Class><rdfs:Class rdf:ID="Focusing"><rdfs:subClassOf rdf:resource="http://reliant.teknowledge.com/DAML/SUMO.owl#QuantityChange" /><rdfs:comment>Altering the relative distance of a Lens 

so that a visual image is sharper.</rdfs:comment></rdfs:Class><rdfs:Class rdf:ID="Fodder"><rdfs:subClassOf rdf:resource="http://reliant.teknowledge.com/DAML/SUMO.owl#Food" /><rdfs:comment>Fodder is the subclass of Food that is intended 

for instances of DomesticAnimal.</rdfs:comment></rdfs:Class><rdfs:Class rdf:ID="Fog"><rdfs:subClassOf rdf:resource="http://reliant.teknowledge.com/DAML/SUMO.owl#WaterCloud" /><rdfs:comment>Any WaterCloud that is in contact with the ground.</rdfs:comment></rdfs:Class><rdfs:Class rdf:ID="Folding"><rdfs:subClassOf rdf:resource="http://reliant.teknowledge.com/DAML/SUMO.owl#ShapeChange" /><rdfs:comment>Bending something in such a way that one part of 

it covers another part.</rdfs:comment></rdfs:Class><rdfs:Class rdf:ID="Foot"><rdfs:subClassOf rdf:resource="http://reliant.teknowledge.com/DAML/SUMO.owl#AnimalAnatomicalStructure" /><rdfs:subClassOf rdf:resource="http://reliant.teknowledge.com/DAML/SUMO.owl#BodyPart" /><rdfs:comment>The lower part of a Limb, the part which makes contact 

with the ground in locomotion of the Animal.</rdfs:comment></rdfs:Class><rdfs:Class rdf:ID="Football"><rdfs:subClassOf rdf:resource="#TeamSport" /><rdfs:comment>A TeamSport where each team tries to place the ball 

in the other's goal.  Note that each instance of Football is a football game.</rdfs:comment></rdfs:Class><rdfs:Class rdf:ID="FootballManeuver"><rdfs:subClassOf rdf:resource="http://reliant.teknowledge.com/DAML/SUMO.owl#Maneuver" /><rdfs:comment>Any Maneuver in Football.</rdfs:comment></rdfs:Class><rdfs:Class rdf:ID="FootballPass"><rdfs:subClassOf rdf:resource="#FootballManeuver" /><rdfs:comment>Any FootballManeuver where the member of one 

team throws the ball to another member of the same team.</rdfs:comment></rdfs:Class><rdfs:Class rdf:ID="FootballTeam"><rdfs:subClassOf rdf:resource="#SportsTeam" /><rdfs:comment>The class of SportsTeams that play Football.</rdfs:comment></rdfs:Class><rdfs:Class rdf:ID="FootballTouchdown"><rdfs:subClassOf rdf:resource="#FootballManeuver" /><rdfs:subClassOf rdf:resource="#Score" /><rdfs:comment>Any FootballManeuver which is also a 

Score, i.e. any play in a Football game which results in one team 

being in possession of the ball on the inside of the opponent's goal line.</rdfs:comment></rdfs:Class><rdfs:Class rdf:ID="ForeignServicePosition"><rdfs:subClassOf rdf:resource="http://reliant.teknowledge.com/DAML/SUMO.owl#Position" /><rdfs:comment>ForeignServicePosition is the 

subclass of Positions that belong to foreign service personnel working 

for a national government or international organization.</rdfs:comment></rdfs:Class><rdfs:Class rdf:ID="Forest"><rdfs:subClassOf rdf:resource="http://reliant.teknowledge.com/DAML/SUMO.owl#LandArea" /><sumo:disjoint rdf:resource="#Field" /><rdfs:comment>Forest is the class of large LandAreas that 

are covered by trees and associated undergrowth, either growing wild or 

managed for the purpose of timber production.</rdfs:comment></rdfs:Class><rdfs:Class rdf:ID="FormOfGovernment"><rdfs:subClassOf rdf:resource="#PoliticoEconomicAttribute" /><rdfs:comment>FormOfGovernment is a class of 

Attributes used to describe the characteristics of a government, 

especially a NationalGovernment.  The concept FormOfGovernment is 

interpreted broadly enough to include Anarchy and Factionalism.</rdfs:comment></rdfs:Class><rdfs:Class rdf:ID="FormText"><rdfs:subClassOf rdf:resource="http://reliant.teknowledge.com/DAML/SUMO.owl#Text" /><rdfs:comment>A page or set of pages containing spaces where 

information is to be entered by an Agent.</rdfs:comment></rdfs:Class><rdfs:Class rdf:ID="FormalMeeting"><rdfs:subClassOf rdf:resource="http://reliant.teknowledge.com/DAML/SUMO.owl#Meeting" /><sumo:disjoint rdf:resource="#SocialParty" /><rdfs:comment>Any Meeting which is the result of Planning 

and whose purpose is not socializing.  This covers organizatinal meetings, as 

well as events like funerals.</rdfs:comment></rdfs:Class><rdfs:Class rdf:ID="FossilFuel"><rdfs:subClassOf rdf:resource="#Fuel" /><rdfs:subClassOf rdf:resource="#PetroleumProduct" /><rdfs:comment>FossilFuel is the subclass of Fuel whose 

instances are derived from fossilized organic deposits, such as Coal 

and LiquefiedPetroleumGas.</rdfs:comment></rdfs:Class><rdfs:Class rdf:ID="Founding"><rdfs:subClassOf rdf:resource="http://reliant.teknowledge.com/DAML/SUMO.owl#Declaring" /><rdfs:subClassOf rdf:resource="http://reliant.teknowledge.com/DAML/SUMO.owl#OrganizationalProcess" /><rdfs:comment>Setting up an Organization.</rdfs:comment></rdfs:Class><rdfs:Class rdf:ID="Fox"><rdfs:subClassOf rdf:resource="http://reliant.teknowledge.com/DAML/SUMO.owl#Canine" /><rdfs:comment>Canines with a bushy tail and pointed ears and nose.  

Foxes tend to be much smaller than most DomesticDogs.</rdfs:comment></rdfs:Class><rdfs:Class rdf:ID="FreeAtom"><rdfs:subClassOf rdf:resource="http://reliant.teknowledge.com/DAML/SUMO.owl#Atom" /><rdfs:comment>Any Atom which is not part of a Molecule.</rdfs:comment></rdfs:Class><rdfs:Class rdf:ID="FreightCar"><rdfs:subClassOf rdf:resource="#Railcar" /><rdfs:comment>FreightCar is the subclass of Railcars that 

are used for hauling freight: bulk materials, manufactured goods, and other 

commodities.</rdfs:comment></rdfs:Class><rdfs:Class rdf:ID="Frightening"><rdfs:subClassOf rdf:resource="http://reliant.teknowledge.com/DAML/SUMO.owl#PsychologicalProcess" /><rdfs:comment>Any PsychologicalProcess where the patient 

comes to feel Anxiety.</rdfs:comment></rdfs:Class><rdfs:Class rdf:ID="Frowning"><rdfs:subClassOf rdf:resource="#FacialExpression" /><rdfs:comment>Furrowing the forehead in such a way as to convey 

unhappiness.</rdfs:comment></rdfs:Class><rdfs:Class rdf:ID="Fuel"><rdfs:subClassOf rdf:resource="http://reliant.teknowledge.com/DAML/SUMO.owl#Substance" /><rdfs:comment>Fuel is the class of Substances that can be 

used as resources in Combustion processes in order to produce heat.  

Mechanical energy can be produced by burning fuel in an Engine.</rdfs:comment></rdfs:Class><rdfs:Class rdf:ID="FullTimePosition"><rdfs:subClassOf rdf:resource="http://reliant.teknowledge.com/DAML/SUMO.owl#Position" /><rdfs:comment>Any Position where the employee is either 

salaried or paid for at least 40 hour of work per week.</rdfs:comment></rdfs:Class><rdfs:Class rdf:ID="Funeral"><rdfs:subClassOf rdf:resource="#FormalMeeting" /><rdfs:comment>A FormalMeeting whose purpose is to commemorate 

the death of someone.</rdfs:comment></rdfs:Class><rdfs:Class rdf:ID="Furniture"><rdfs:subClassOf rdf:resource="http://reliant.teknowledge.com/DAML/SUMO.owl#Artifact" /><sumo:disjoint rdf:resource="http://reliant.teknowledge.com/DAML/SUMO.owl#Device" /><rdfs:comment>Any free-standing Artifacts which are not 

Devices and which are used in day-to-day living.</rdfs:comment></rdfs:Class><rdfs:Class rdf:ID="GainingConsciousness"><rdfs:subClassOf rdf:resource="http://reliant.teknowledge.com/DAML/SUMO.owl#PsychologicalProcess" /><rdfs:comment>The process of transitioning from a state 

of being Unconscious to a state of being Awake.</rdfs:comment></rdfs:Class><rdfs:Class rdf:ID="GameArtifact"><rdfs:subClassOf rdf:resource="http://reliant.teknowledge.com/DAML/SUMO.owl#Artifact" /><rdfs:comment>An Artifact that is designed to be used 

in a Game.</rdfs:comment></rdfs:Class><rdfs:Class rdf:ID="GameAttribute"><rdfs:subClassOf rdf:resource="http://reliant.teknowledge.com/DAML/SUMO.owl#ContestAttribute" /><rdfs:comment>Any ContestAttribute that is specific 

to a Game.</rdfs:comment></rdfs:Class><rdfs:Class rdf:ID="GameBoard"><rdfs:subClassOf rdf:resource="#GameArtifact" /><rdfs:comment>A GameArtifact which is intended to be used as the 

game area for playing a particular game.</rdfs:comment></rdfs:Class><rdfs:Class rdf:ID="GameCall"><rdfs:subClassOf rdf:resource="http://reliant.teknowledge.com/DAML/SUMO.owl#Deciding" /><rdfs:subClassOf rdf:resource="http://reliant.teknowledge.com/DAML/SUMO.owl#Declaring" /><rdfs:comment>A decision issued by an official referee in a 

Game.  Note that GameCall is a subclass of Declaring, because these 

decisions have binding, normative force.</rdfs:comment></rdfs:Class><rdfs:Class rdf:ID="GameDie"><rdfs:subClassOf rdf:resource="#GamePiece" /><rdfs:comment>A small cube with 1 to 6 dots on each face that is 

used to generate numbers at random in a Game.</rdfs:comment></rdfs:Class><rdfs:Class rdf:ID="GameGoal"><rdfs:subClassOf rdf:resource="#GameArtifact" /><rdfs:comment>The location where a GameShot must end up if it 

is to constitute a Score.</rdfs:comment></rdfs:Class><rdfs:Class rdf:ID="GamePiece"><rdfs:subClassOf rdf:resource="#GameArtifact" /><rdfs:comment>A GameArtifact that is moved in a game area.</rdfs:comment></rdfs:Class><rdfs:Class rdf:ID="GameReferee"><rdfs:subClassOf rdf:resource="#SkilledOccupation" /><rdfs:comment>A position which involves adjudicating contested 

Maneuvers in a Game, i.e. deciding whether or not the Maneuvers are 

permitted by the rules of the Game.</rdfs:comment></rdfs:Class><rdfs:Class rdf:ID="GameShot"><rdfs:subClassOf rdf:resource="http://reliant.teknowledge.com/DAML/SUMO.owl#Impelling" /><rdfs:subClassOf rdf:resource="http://reliant.teknowledge.com/DAML/SUMO.owl#Maneuver" /><rdfs:comment>Impelling a GamePiece for the purpose of 

scoring a point or preventing the opposing player or team from scoring 

a point.  Note that this class does not cover shots which are disallowed 

by the rules of the game.</rdfs:comment></rdfs:Class><rdfs:Class rdf:ID="Garage"><rdfs:subClassOf rdf:resource="http://reliant.teknowledge.com/DAML/SUMO.owl#StationaryArtifact" /><rdfs:comment>A Building or part of a Building which is intended 

to house one or more Automobiles.</rdfs:comment></rdfs:Class><rdfs:Class rdf:ID="Gasoline"><rdfs:subClassOf rdf:resource="#RefinedPetroleumProduct" /><rdfs:subClassOf rdf:resource="#FossilFuel" /><rdfs:comment>Gasoline is the subclass of 

RefinedPetroleumProducts that are fuels for internal combustion engines.</rdfs:comment></rdfs:Class><rdfs:Class rdf:ID="GasolineEngine"><rdfs:subClassOf rdf:resource="#InternalCombustionEngine" /><rdfs:comment>GasolineEngine is the subclass of 

InternalCombustionEngines that use Gasoline as their resource.</rdfs:comment></rdfs:Class><rdfs:Class rdf:ID="Gastropod"><rdfs:subClassOf rdf:resource="http://reliant.teknowledge.com/DAML/SUMO.owl#Mollusk" /><rdfs:comment>A Mollusk with a distinct head that has no 

shell (e.g. slugs) or a univalve shell (e.g. snails).</rdfs:comment></rdfs:Class><rdfs:Class rdf:ID="GeneralElection"><rdfs:subClassOf rdf:resource="http://reliant.teknowledge.com/DAML/SUMO.owl#Election" /><rdfs:comment>GeneralElection is the subclass of 

Elections that are held at regular intervals and in which all or most 

constituencies of a GeopoliticalArea participate.</rdfs:comment></rdfs:Class><rdfs:Class rdf:ID="Germanium"><rdfs:subClassOf rdf:resource="http://reliant.teknowledge.com/DAML/SUMO.owl#ElementalSubstance" /><atomicNumber>32</atomicNumber><rdfs:comment>Lustrous hard metalloid element, belongs to 

group 14 of the periodic table.  Forms a large number of organometallic 

compounds.  Predicted by Mendeleev in 1871, it was actually found in 1886 

by Winkler.</rdfs:comment></rdfs:Class><rdfs:Class rdf:ID="Girl"><rdfs:subClassOf rdf:resource="#HumanChild" /><rdfs:subClassOf rdf:resource="http://reliant.teknowledge.com/DAML/SUMO.owl#Woman" /><rdfs:comment>A HumanChild who is Female.</rdfs:comment></rdfs:Class><rdfs:Class rdf:ID="Gland"><rdfs:subClassOf rdf:resource="http://reliant.teknowledge.com/DAML/SUMO.owl#Organ" /><rdfs:subClassOf rdf:resource="http://reliant.teknowledge.com/DAML/SUMO.owl#AnimalAnatomicalStructure" /><rdfs:comment>An Organ that removes Substances from the Blood, 

alters them in some way, and then releases them.</rdfs:comment></rdfs:Class><rdfs:Class rdf:ID="Glass"><rdfs:subClassOf rdf:resource="http://reliant.teknowledge.com/DAML/SUMO.owl#Mixture" /><rdfs:comment>A transparent or translucent Mixture of silicates.</rdfs:comment></rdfs:Class><rdfs:Class rdf:ID="Glove"><rdfs:subClassOf rdf:resource="http://reliant.teknowledge.com/DAML/SUMO.owl#Clothing" /><rdfs:comment>Clothing that is intended to be worn on the Hand.  

Note that this class covers both gloves which have individual compartments 

for each of the Fingers and mittens.</rdfs:comment></rdfs:Class><rdfs:Class rdf:ID="Glue"><rdfs:subClassOf rdf:resource="http://reliant.teknowledge.com/DAML/SUMO.owl#Solution" /><rdfs:comment>Any Solution whose purpose is to be used as the instrument 

of Attaching one thing to another or one part of something to another part.</rdfs:comment></rdfs:Class><rdfs:Class rdf:ID="Goat"><rdfs:subClassOf rdf:resource="http://reliant.teknowledge.com/DAML/SUMO.owl#HoofedMammal" /><rdfs:subClassOf rdf:resource="#DomesticAnimal" /><rdfs:comment>A domesticated HoofedMammal that is raised primarily 

for milk.</rdfs:comment></rdfs:Class><rdfs:Class rdf:ID="Gold"><rdfs:subClassOf rdf:resource="http://reliant.teknowledge.com/DAML/SUMO.owl#ElementalSubstance" /><atomicNumber>79</atomicNumber><rdfs:comment>Gold is gold colored.  It is the most malleable and 

ductile metal known.  There is only one stable isotope of gold, and five 

radioisotopes of gold, Au-195 being the most stable with a half-life of 

186 days.  Gold is used as a monetary standard, in jewelry, dentistry, 

electronics.  Au-198 is used in treating cancer and some other medical 

conditions.  Gold has been known to exist as far back as 2600 BC.  Gold 

comes from the Anglo-Saxon word gold.  Its symbol, Au, comes from the 

Latin word aurum, which means gold.  Gold is not particularly toxic, 

however it is known to cause damage to the liver and kidneys in some.</rdfs:comment></rdfs:Class><rdfs:Class rdf:ID="Golf"><rdfs:subClassOf rdf:resource="http://reliant.teknowledge.com/DAML/SUMO.owl#Sport" /><rdfs:comment>A sport which has a course of 9 or 18 holes and where 

the object is to hit a ball with a club into each hole in turn with the fewest 

number of strokes.</rdfs:comment></rdfs:Class><rdfs:Class rdf:ID="GolfHole"><rdfs:subClassOf rdf:resource="#GolfManeuver" /><rdfs:comment>A division of a Golf game.  A normal game 

consists of 9 to 18 holes, and each hole involves a turn for each of 

the players in the Golf game.</rdfs:comment></rdfs:Class><rdfs:Class rdf:ID="GolfManeuver"><rdfs:subClassOf rdf:resource="http://reliant.teknowledge.com/DAML/SUMO.owl#Maneuver" /><rdfs:comment>Any Maneuver in Golf.</rdfs:comment></rdfs:Class><rdfs:Class rdf:ID="Goose"><rdfs:subClassOf rdf:resource="http://reliant.teknowledge.com/DAML/SUMO.owl#Bird" /><rdfs:comment>A subclass of Bird with webbed feet and a long neck 

and a large body.  These Birds are often raised for their meat.</rdfs:comment></rdfs:Class><rdfs:Class rdf:ID="GovernmentOfficer"><rdfs:subClassOf rdf:resource="#Profession" /><rdfs:comment>Any Profession where the position occupied 

is within a GovernmentOrganization.</rdfs:comment></rdfs:Class><rdfs:Class rdf:ID="GovernmentSecretary"><rdfs:subClassOf rdf:resource="#SkilledOccupation" /><rdfs:comment>The class of Positions where the position holder 

is head of an adminstrative department of Government.</rdfs:comment></rdfs:Class><rdfs:Class rdf:ID="GraduateSchool"><rdfs:subClassOf rdf:resource="#PostSecondarySchool" /><rdfs:comment>A School which is devoted to a specific 

subject area, which admits students that have a bachelor's degree, which 

grants masters and/or doctorate degrees, and which is part of a University.</rdfs:comment></rdfs:Class><rdfs:Class rdf:ID="Graph"><rdfs:subClassOf rdf:resource="http://reliant.teknowledge.com/DAML/SUMO.owl#Abstract" /><rdfs:comment>The Class of graphs, where a graph is understood 

to be a set of GraphNodes connected by GraphArcs.  Note that this 

Class includes only connected graphs, i.e. graphs in which there is a 

GraphPath between any two GraphNodes.  Note too that every Graph 

is assumed to contain at least two GraphArcs and three GraphNodes.</rdfs:comment></rdfs:Class><rdfs:Class rdf:ID="GraphArc"><rdfs:subClassOf rdf:resource="#GraphElement" /><rdfs:comment>Graphs are comprised of GraphNodes 

and GraphArcs.  Every GraphArc links two GraphNodes.</rdfs:comment></rdfs:Class><rdfs:Class rdf:ID="GraphCircuit"><rdfs:subClassOf rdf:resource="#GraphPath" /><rdfs:comment>A GraphPath that begins (see 

BeginNodeFn) and ends (see EndNodeFn) at the same 

GraphNode.</rdfs:comment></rdfs:Class><rdfs:Class rdf:ID="GraphDiagram"><rdfs:subClassOf rdf:resource="http://reliant.teknowledge.com/DAML/SUMO.owl#Icon" /><rdfs:comment>An Icon which depicts one or more quantities.</rdfs:comment></rdfs:Class><rdfs:Class rdf:ID="GraphElement"><rdfs:subClassOf rdf:resource="http://reliant.teknowledge.com/DAML/SUMO.owl#Abstract" /><rdfs:comment>Noncompositional parts of Graphs.  

These parts are restricted to GraphNodes and GraphArcs.</rdfs:comment></rdfs:Class><rdfs:Class rdf:ID="GraphLoop"><rdfs:subClassOf rdf:resource="#GraphArc" /><rdfs:comment>A GraphArc in which a GraphNode is 

linked to itself.</rdfs:comment></rdfs:Class><rdfs:Class rdf:ID="GraphNode"><rdfs:subClassOf rdf:resource="#GraphElement" /><rdfs:comment>Graphs are comprised of GraphNodes 

and GraphArcs.  Every GraphNode is linked by a GraphArc.</rdfs:comment></rdfs:Class><rdfs:Class rdf:ID="GraphPath"><rdfs:subClassOf rdf:resource="#DirectedGraph" /><rdfs:comment>Informally, a single, directed route between 

two GraphNodes in a Graph.  Formally, a DirectedGraph that is a 

subGraph of the original Graph and such that no two GraphArcs in 

the DirectedGraph have the same intial node (see InitialNodeFn) or 

the same terminal node (see TerminalNodeFn).</rdfs:comment></rdfs:Class><rdfs:Class rdf:ID="Grass"><rdfs:subClassOf rdf:resource="http://reliant.teknowledge.com/DAML/SUMO.owl#FloweringPlant" /><rdfs:comment>FloweringPlants with green, narrow leaves that are 

used for lawns and Fields.</rdfs:comment></rdfs:Class><rdfs:Class rdf:ID="Grasshopper"><rdfs:subClassOf rdf:resource="http://reliant.teknowledge.com/DAML/SUMO.owl#Insect" /><rdfs:comment>Insects with enormous legs that are used for 

jumping.</rdfs:comment></rdfs:Class><rdfs:Class rdf:ID="Gray"><rdf:type rdf:resource="#SecondaryColor" /><rdfs:comment>A SecondaryColor that results from mixing Black and 

White.</rdfs:comment><rdfs:subClassOf rdf:resource="http://reliant.teknowledge.com/DAML/SUMO.owl#FunctionQuantity" /><rdf:type rdf:resource="http://reliant.teknowledge.com/DAML/SUMO.owl#SystemeInternationalUnit" /><rdfs:comment>SI absorbed dose measure.  Symbol: Gy.  It measures 

the dose of radiation absorbed in living tissue. It is equal approximately 

to the absorbed dose delivered when the energy per unit mass imparted to

matter by ionizing radiation is 1 Joule per kilogram.  Gray = J/kg 

= m^2*s^(-2).</rdfs:comment></rdfs:Class><rdfs:Class rdf:ID="Greeting"><rdfs:subClassOf rdf:resource="http://reliant.teknowledge.com/DAML/SUMO.owl#Expressing" /><rdfs:comment>Any instance of Expressing an acknowledgment of a 

person's arrival.  Note that this class is not a subclass of LinguisticCommunication, 

because it covers gestures of greeting, e.g. Waving and Nodding in certain 

circumstances.</rdfs:comment></rdfs:Class><rdfs:Class rdf:ID="GroceryStore"><rdfs:subClassOf rdf:resource="#RetailStore" /><rdfs:comment>A RetailStore that sells Food, and perhaps 

other items as well.</rdfs:comment></rdfs:Class><rdfs:Class rdf:ID="GroupOfAnimals"><rdfs:subClassOf rdf:resource="http://reliant.teknowledge.com/DAML/SUMO.owl#Group" /><rdfs:comment>Any Group which contains exclusively 

non-human members.</rdfs:comment></rdfs:Class><rdfs:Class rdf:ID="Guitar"><rdfs:subClassOf rdf:resource="#StringInstrument" /><rdfs:comment>A StringInstrument that has six to twelve strings and 

is played by strumming with one hand while grasping frets with the other hand.</rdfs:comment></rdfs:Class><rdfs:Class rdf:ID="Gulf"><rdfs:subClassOf rdf:resource="#BodyOfWater" /><rdfs:subClassOf rdf:resource="http://reliant.teknowledge.com/DAML/SUMO.owl#SaltWaterArea" /><rdfs:comment>Gulf is the class of extensions of a Sea or 

Ocean that reach into a land mass or are partially enclosed by a 

LandArea.</rdfs:comment></rdfs:Class><rdfs:Class rdf:ID="Gun"><rdfs:subClassOf rdf:resource="#ProjectileLauncher" /><rdfs:comment>A ProjectileLauncher that shoots Bullets.</rdfs:comment></rdfs:Class><rdfs:Class rdf:ID="GunBarrel"><rdfs:subClassOf rdf:resource="http://reliant.teknowledge.com/DAML/SUMO.owl#EngineeringComponent" /><rdfs:comment>The part of a Gun through which a Projectile travels 

when it is fired.</rdfs:comment></rdfs:Class><rdfs:Class rdf:ID="GunPowder"><rdfs:subClassOf rdf:resource="http://reliant.teknowledge.com/DAML/SUMO.owl#Mixture" /><rdfs:comment>A Mixture of potassium nitrate, sulfur, and 

charcoal that is used in ExplosiveDevices and to propell Projectiles 

in ProjectileWeapons.</rdfs:comment></rdfs:Class><rdfs:Class rdf:ID="GunStock"><rdfs:subClassOf rdf:resource="http://reliant.teknowledge.com/DAML/SUMO.owl#EngineeringComponent" /><rdfs:comment>The part of a Gun that is placed against the 

shoulder to absorb some of the recoil action when it is fired.</rdfs:comment></rdfs:Class><rdfs:Class rdf:ID="GunTrigger"><rdfs:subClassOf rdf:resource="http://reliant.teknowledge.com/DAML/SUMO.owl#EngineeringComponent" /><rdfs:comment>The part of the Gun which is pulled in Shooting 

the Gun.</rdfs:comment></rdfs:Class><rdfs:Class rdf:ID="Gymnastics"><rdfs:subClassOf rdf:resource="http://reliant.teknowledge.com/DAML/SUMO.owl#Sport" /><rdfs:comment>A sport which involves exercises of agility on a 

range of gymnastic equipment.</rdfs:comment></rdfs:Class><rdfs:Class rdf:ID="Hailing"><rdfs:subClassOf rdf:resource="http://reliant.teknowledge.com/DAML/SUMO.owl#Precipitation" /><rdfs:comment>Hailing is a precipitation process 

in which water falls in a Solid state with round, hard pellets.</rdfs:comment></rdfs:Class><rdfs:Class rdf:ID="Hair"><rdfs:subClassOf rdf:resource="http://reliant.teknowledge.com/DAML/SUMO.owl#AnimalAnatomicalStructure" /><rdfs:comment>A filament that covers part of the body of many 

Mammals.</rdfs:comment></rdfs:Class><rdfs:Class rdf:ID="HairRemoval"><rdfs:subClassOf rdf:resource="http://reliant.teknowledge.com/DAML/SUMO.owl#Removing" /><rdfs:comment>Removing (some or all) the Hair from the 

body of an Animal.  Note that this covers shaving hair, cutting hair, 

pulling hair out by the roots, etc.</rdfs:comment></rdfs:Class><rdfs:Class rdf:ID="Hammer"><rdfs:subClassOf rdf:resource="http://reliant.teknowledge.com/DAML/SUMO.owl#Device" /><rdfs:comment>A Device that is used to pound Nails into a 

surface, where they become firmly attached.</rdfs:comment></rdfs:Class><rdfs:Class rdf:ID="Hand"><rdfs:subClassOf rdf:resource="http://reliant.teknowledge.com/DAML/SUMO.owl#AnimalAnatomicalStructure" /><rdfs:subClassOf rdf:resource="http://reliant.teknowledge.com/DAML/SUMO.owl#BodyPart" /><rdfs:comment>The grasping, fingered part of an upper limb of a 

Primate.</rdfs:comment></rdfs:Class><rdfs:Class rdf:ID="HandGesture"><rdfs:subClassOf rdf:resource="http://reliant.teknowledge.com/DAML/SUMO.owl#Gesture" /><rdfs:comment>Any Gesture which involves the Hands.</rdfs:comment></rdfs:Class><rdfs:Class rdf:ID="Handle"><rdfs:subClassOf rdf:resource="http://reliant.teknowledge.com/DAML/SUMO.owl#EngineeringComponent" /><rdfs:comment>The part or parts of an Artifact that are designed to be 

held with the Hands when the Artifact is used or carried.</rdfs:comment></rdfs:Class><rdfs:Class rdf:ID="Hanging"><rdfs:subClassOf rdf:resource="#Suffocating" /><rdfs:comment>Suffocating someone by suspending him/her from 

a rope wound around the neck until asphyxiation occurs.</rdfs:comment></rdfs:Class><rdfs:Class rdf:ID="HardDiskDrive"><rdfs:subClassOf rdf:resource="#ComputerHardware" /><rdfs:comment>The primary computer storage medium, which 

is made of one or more aluminum or glass platters, coated with a 

ferromagnetic material. Most hard disks are fixed disks, which are 

permanently sealed in the drive.</rdfs:comment></rdfs:Class><rdfs:Class rdf:ID="Harvesting"><rdfs:subClassOf rdf:resource="http://reliant.teknowledge.com/DAML/SUMO.owl#Removing" /><rdfs:comment>Gathering the plant results of Agriculture.</rdfs:comment></rdfs:Class><rdfs:Class rdf:ID="Hat"><rdfs:subClassOf rdf:resource="#OutdoorClothing" /><rdfs:comment>A type of Clothing that is worn on the Head.  Note 

that this class covers caps, bonnets, berets, etc.</rdfs:comment></rdfs:Class><rdfs:Class rdf:ID="Hay"><rdfs:subClassOf rdf:resource="#Fodder" /><rdfs:comment>Grass that has been cut and cured for use as Fodder.</rdfs:comment></rdfs:Class><rdfs:Class rdf:ID="Head"><rdfs:subClassOf rdf:resource="http://reliant.teknowledge.com/DAML/SUMO.owl#AnimalAnatomicalStructure" /><rdfs:subClassOf rdf:resource="http://reliant.teknowledge.com/DAML/SUMO.owl#BodyPart" /><rdfs:comment>The part of the body containing the sense organs and 

the brain.</rdfs:comment></rdfs:Class><rdfs:Class rdf:ID="Headlight"><rdfs:subClassOf rdf:resource="#VehicleLight" /><rdfs:comment>Any VehicleLight which is attached to the front 

of a Vehicle.</rdfs:comment></rdfs:Class><rdfs:Class rdf:ID="Heart"><rdfs:subClassOf rdf:resource="http://reliant.teknowledge.com/DAML/SUMO.owl#Organ" /><rdfs:subClassOf rdf:resource="http://reliant.teknowledge.com/DAML/SUMO.owl#AnimalAnatomicalStructure" /><rdfs:comment>The Organ that pumps Blood throughout the body.</rdfs:comment></rdfs:Class><rdfs:Class rdf:ID="HeatingDevice"><rdfs:subClassOf rdf:resource="http://reliant.teknowledge.com/DAML/SUMO.owl#Device" /><rdfs:comment>A Device whose purpose is Heating something, 

e.g. electric heaters, heat lamps, ovens, stoves, etc.</rdfs:comment></rdfs:Class><rdfs:Class rdf:ID="Helicopter"><rdfs:subClassOf rdf:resource="#Aircraft" /><rdfs:comment>Any Aircraft with rapidly rotating wings.</rdfs:comment></rdfs:Class><rdfs:Class rdf:ID="Helium"><rdfs:subClassOf rdf:resource="http://reliant.teknowledge.com/DAML/SUMO.owl#ElementalSubstance" /><atomicNumber>2</atomicNumber><rdfs:comment>Colourless, odourless gaseous nonmetallic element.  

Belongs to group 18 of the periodic table.  Lowest boiling point of all 

elements and can only be solidified under pressure.  Chemically inert, no 

known compounds.  Discovered in the solar spectrum in 1868 by Lockyer.</rdfs:comment></rdfs:Class><rdfs:Class rdf:ID="Hemisphere"><rdfs:subClassOf rdf:resource="http://reliant.teknowledge.com/DAML/SUMO.owl#GeographicArea" /><rdfs:comment>Any half of the PlanetEarth, e.g. the northern 

hemisphere, the southern hemisphere, the eastern hemisphere or the western 

hemisphere.</rdfs:comment></rdfs:Class><rdfs:Class rdf:ID="Hen"><rdfs:subClassOf rdf:resource="#Chicken" /><rdfs:comment>A Female Chicken.</rdfs:comment></rdfs:Class><rdfs:Class rdf:ID="Henry"><rdfs:subClassOf rdf:resource="http://reliant.teknowledge.com/DAML/SUMO.owl#FunctionQuantity" /><rdf:type rdf:resource="http://reliant.teknowledge.com/DAML/SUMO.owl#SystemeInternationalUnit" /><rdfs:comment>SI inductance measure.  Symbol: H.  One Henry 

is equivalent to one Volt divided by one Ampere per SecondDuration. 

If a current changing at the rate of one Ampere per SecondDuration 

induces an electromotive force of one Volt, the circuit has an 

inductance of one Henry.  Henry = Wb/A = m^2*kg*s^(-2)*A^(-2).</rdfs:comment></rdfs:Class><rdfs:Class rdf:ID="Herbivore"><rdfs:subClassOf rdf:resource="http://reliant.teknowledge.com/DAML/SUMO.owl#Mammal" /><sumo:disjoint rdf:resource="http://reliant.teknowledge.com/DAML/SUMO.owl#Carnivore" /><rdfs:comment>A plant-eating Mammal.</rdfs:comment></rdfs:Class><rdfs:Class rdf:ID="HighTide"><rdfs:subClassOf rdf:resource="#TidalProcess" /><rdfs:comment>HighTide is the class of TidalProcesses that 

occur twice a day in marine waters, in which the water level rises above 

the mean sea level.</rdfs:comment></rdfs:Class><rdfs:Class rdf:ID="Hijacking"><rdfs:subClassOf rdf:resource="#Robbing" /><rdfs:comment>Robbing a Vehicle and then driving it away.</rdfs:comment></rdfs:Class><rdfs:Class rdf:ID="Hinge"><rdfs:subClassOf rdf:resource="http://reliant.teknowledge.com/DAML/SUMO.owl#EngineeringComponent" /><rdfs:comment>An EngineeringComponent that connects one thing to 

another in such a way that they can move relative to one another.</rdfs:comment></rdfs:Class><rdfs:Class rdf:ID="HistoricalAccount"><rdfs:subClassOf rdf:resource="http://reliant.teknowledge.com/DAML/SUMO.owl#FactualText" /><rdfs:subClassOf rdf:resource="#NarrativeText" /><rdfs:comment>A FactualAccount that describes 

events that are believed by the author of the account to have 

occurred in the past.</rdfs:comment></rdfs:Class><rdfs:Class rdf:ID="HoistingDevice"><rdfs:subClassOf rdf:resource="#MaterialHandlingEquipment" /><rdfs:comment>HoistingDevice is a subclass of 

mechanical Devices that provide a mechanical advantage in lifting 

and lowering, e.g., by use of a block and tackle.</rdfs:comment></rdfs:Class><rdfs:Class rdf:ID="Holder"><rdfs:subClassOf rdf:resource="http://reliant.teknowledge.com/DAML/SUMO.owl#Device" /><rdfs:comment>A large class of Devices whose purpose is to hold 

something else, i.e. be the instrument of a Keeping.</rdfs:comment></rdfs:Class><rdfs:Class rdf:ID="Holiday"><rdfs:subClassOf rdf:resource="http://reliant.teknowledge.com/DAML/SUMO.owl#TimeInterval" /><rdfs:comment>Holiday is the class of time periods that are 

observed as holidays in a country, culture, or religion.  Holidays may 

recur annually on the same date, or they may be moveable, for example, 

Thanksgiving Day falls on the last Thursday of each November.</rdfs:comment></rdfs:Class><rdfs:Class rdf:ID="HolidayCard"><rdfs:subClassOf rdf:resource="http://reliant.teknowledge.com/DAML/SUMO.owl#ContentBearingObject" /><rdfs:comment>A stiff piece of Paper, usually folded over, which 

is sent to others in celebration of a Holiday.</rdfs:comment></rdfs:Class><rdfs:Class rdf:ID="Holster"><rdfs:subClassOf rdf:resource="#Container" /><rdfs:comment>A Container for a Pistol.  It is generally made of 

Leather and worn on either the shoulder or the waist.</rdfs:comment></rdfs:Class><rdfs:Class rdf:ID="HomeBase"><rdfs:subClassOf rdf:resource="#BaseballBase" /><rdfs:comment>The final BaseballBase which must be touched 

by the batter in order to achieve a BaseballRun.</rdfs:comment></rdfs:Class><rdfs:Class rdf:ID="HomeRun"><rdfs:subClassOf rdf:resource="#BaseballRun" /><rdfs:comment>A BaseballRun where the batter touches home base 

during his turn at bat.</rdfs:comment></rdfs:Class><rdfs:Class rdf:ID="Honey"><rdfs:subClassOf rdf:resource="http://reliant.teknowledge.com/DAML/SUMO.owl#AnimalSubstance" /><rdfs:subClassOf rdf:resource="http://reliant.teknowledge.com/DAML/SUMO.owl#Food" /><rdfs:comment>An edible, sweet Substance produced by some species of 

Bees.</rdfs:comment></rdfs:Class><rdfs:Class rdf:ID="Hoof"><rdfs:subClassOf rdf:resource="http://reliant.teknowledge.com/DAML/SUMO.owl#AnimalAnatomicalStructure" /><rdfs:subClassOf rdf:resource="http://reliant.teknowledge.com/DAML/SUMO.owl#BodyPart" /><rdfs:comment>The hard end of the Foot of a HoofedMammal.</rdfs:comment></rdfs:Class><rdfs:Class rdf:ID="Hormone"><rdfs:subClassOf rdf:resource="http://reliant.teknowledge.com/DAML/SUMO.owl#BodySubstance" /><rdfs:subClassOf rdf:resource="http://reliant.teknowledge.com/DAML/SUMO.owl#BiologicallyActiveSubstance" /><rdfs:comment>In Animals, a chemical secreted by an 

endocrine gland whose products are released into the circulating fluid.  

Plant hormones or synthetic hormones which are used only to alter or 

control various physiologic processes, e.g., reproductive control agents, 

are assigned to the Class BiologicallyActiveSubstance. Hormones act as 

chemical messengers and regulate various physiologic processes such as 

growth, reproduction, metabolism, etc.  They usually fall into two broad 

categories, viz. steroid hormones and peptide hormones.</rdfs:comment></rdfs:Class><rdfs:Class rdf:ID="Horn"><rdfs:subClassOf rdf:resource="http://reliant.teknowledge.com/DAML/SUMO.owl#Bone" /><rdfs:comment>An outgrowth of Bone that is found on some 

HoofedMammals.</rdfs:comment></rdfs:Class><rdfs:Class rdf:ID="HornInstrument"><rdfs:subClassOf rdf:resource="http://reliant.teknowledge.com/DAML/SUMO.owl#MusicalInstrument" /><rdfs:comment>A MusicalInstrument which is played by 

blowing it and which does not use a reed.</rdfs:comment></rdfs:Class><rdfs:Class rdf:ID="Horse"><rdfs:subClassOf rdf:resource="#DomesticAnimal" /><rdfs:subClassOf rdf:resource="http://reliant.teknowledge.com/DAML/SUMO.owl#HoofedMammal" /><rdfs:comment>A domesticated HoofedMammal that is used for 

transportation and work.</rdfs:comment></rdfs:Class><rdfs:Class rdf:ID="HorseRiding"><rdfs:subClassOf rdf:resource="http://reliant.teknowledge.com/DAML/SUMO.owl#Carrying" /><rdfs:comment>Any instance of Carrying where the Animal is 

a Horse.</rdfs:comment></rdfs:Class><rdfs:Class rdf:ID="Horsepower"><rdfs:subClassOf rdf:resource="http://reliant.teknowledge.com/DAML/SUMO.owl#FunctionQuantity" /><rdf:type rdf:resource="http://reliant.teknowledge.com/DAML/SUMO.owl#UnitOfMeasure" /><rdfs:comment>A power measure that is equal to 746 Watts.</rdfs:comment></rdfs:Class><rdfs:Class rdf:ID="Hospital"><rdfs:subClassOf rdf:resource="#CareOrganization" /><rdfs:subClassOf rdf:resource="http://reliant.teknowledge.com/DAML/SUMO.owl#TemporaryResidence" /><rdfs:comment>A CareOrganization where patients reside for a 

short period of time while they undergo treatment for a disease or disorder.</rdfs:comment></rdfs:Class><rdfs:Class rdf:ID="House"><rdfs:subClassOf rdf:resource="http://reliant.teknowledge.com/DAML/SUMO.owl#ResidentialBuilding" /><rdfs:subClassOf rdf:resource="http://reliant.teknowledge.com/DAML/SUMO.owl#SingleFamilyResidence" /><rdfs:comment>A ResidentialBuilding which is intended to be 

inhabited by members of the same SocialUnit.  Houses are distinguished 

from temporary housing like hotels and multi-family dwellings like condominium 

and apartment buildings.</rdfs:comment></rdfs:Class><rdfs:Class rdf:ID="HumanAdult"><rdfs:subClassOf rdf:resource="http://reliant.teknowledge.com/DAML/SUMO.owl#Human" /><rdfs:comment>The class of Humans that are 18 years of 

age or older.</rdfs:comment></rdfs:Class><rdfs:Class rdf:ID="HumanChild"><rdfs:subClassOf rdf:resource="#HumanYouth" /><rdfs:comment>A HumanYouth between birth and puberty, i.e a 

Human who is NonFullyFormed.</rdfs:comment></rdfs:Class><rdfs:Class rdf:ID="HumanCorpse"><rdfs:subClassOf rdf:resource="http://reliant.teknowledge.com/DAML/SUMO.owl#Human" /><rdfs:comment>A Human which is Dead.</rdfs:comment></rdfs:Class><rdfs:Class rdf:ID="HumanInfant"><rdfs:subClassOf rdf:resource="#HumanChild" /><rdfs:comment>A Human between birth and the first year of age.</rdfs:comment></rdfs:Class><rdfs:Class rdf:ID="HumanSlave"><rdfs:subClassOf rdf:resource="http://reliant.teknowledge.com/DAML/SUMO.owl#Human" /><rdfs:comment>A Human who is owned by someone else.</rdfs:comment></rdfs:Class><rdfs:Class rdf:ID="HumanYouth"><rdfs:subClassOf rdf:resource="http://reliant.teknowledge.com/DAML/SUMO.owl#Human" /><rdfs:comment>The class of Humans that are younger than 

18 years of age.</rdfs:comment></rdfs:Class><rdfs:Class rdf:ID="Humus"><rdfs:subClassOf rdf:resource="http://reliant.teknowledge.com/DAML/SUMO.owl#Mixture" /><rdfs:comment>Humus is decaying organic matter found in Soil and derived 

from dead animal and plant material.</rdfs:comment></rdfs:Class><rdfs:Class rdf:ID="Hunting"><rdfs:subClassOf rdf:resource="http://reliant.teknowledge.com/DAML/SUMO.owl#Pursuing" /><rdfs:comment>Hunting is the class of Processes in which 

an animal or animals are pursued and sometimes captured and/or killed.</rdfs:comment></rdfs:Class><rdfs:Class rdf:ID="Hydrocarbon"><rdfs:subClassOf rdf:resource="#OrganicCompound" /><rdfs:comment>Any OrganicCompound that contains only Carbon 

and Hydrogen.</rdfs:comment></rdfs:Class><rdfs:Class rdf:ID="Hydrogen"><rdfs:subClassOf rdf:resource="http://reliant.teknowledge.com/DAML/SUMO.owl#ElementalSubstance" /><atomicNumber>1</atomicNumber><rdfs:comment>Colourless, odourless gaseous chemical element.  

Lightest and most abundant element in the universe.  Present in water and 

in all organic compounds.  Chemically reacts with most elements.  

Discovered by Henry Cavendish in 1776.</rdfs:comment></rdfs:Class><rdfs:Class rdf:ID="Hypothalamus"><rdfs:subClassOf rdf:resource="http://reliant.teknowledge.com/DAML/SUMO.owl#BodyPart" /><rdfs:subClassOf rdf:resource="http://reliant.teknowledge.com/DAML/SUMO.owl#AnimalAnatomicalStructure" /><rdfs:comment>The part of the Brain lying below the 

thalamus that serves to regulate AutonomicProcesses.</rdfs:comment></rdfs:Class><rdfs:Class rdf:ID="Ice"><rdfs:subClassOf rdf:resource="http://reliant.teknowledge.com/DAML/SUMO.owl#Water" /><rdfs:comment>Water that has the PhysicalState of Solid.</rdfs:comment></rdfs:Class><rdfs:Class rdf:ID="IlluminationDevice"><rdfs:subClassOf rdf:resource="http://reliant.teknowledge.com/DAML/SUMO.owl#Device" /><rdfs:comment>Any Device whose purpose is to be a source of 

visible light.</rdfs:comment></rdfs:Class><rdfs:Class rdf:ID="Imagining"><rdfs:subClassOf rdf:resource="http://reliant.teknowledge.com/DAML/SUMO.owl#PsychologicalProcess" /><rdfs:comment>Forming a mental picture of something which 

is not present.</rdfs:comment></rdfs:Class><rdfs:Class rdf:ID="Immigrating"><rdfs:subClassOf rdf:resource="http://reliant.teknowledge.com/DAML/SUMO.owl#Translocation" /><rdfs:comment>Any Translocation by a Human from one Nation 

to another Nation where the person is not a citizen for the purpose of taking 

up residence.</rdfs:comment></rdfs:Class><rdfs:Class rdf:ID="Imprisoning"><rdfs:subClassOf rdf:resource="http://reliant.teknowledge.com/DAML/SUMO.owl#Confining" /><rdfs:comment>The class of Confining processes where the detainee 

is put in Prison.</rdfs:comment></rdfs:Class><rdfs:Class rdf:ID="InchMercury"><rdfs:subClassOf rdf:resource="#AtmosphericPressureMeasure" /><rdf:type rdf:resource="http://reliant.teknowledge.com/DAML/SUMO.owl#UnitOfMeasure" /><rdfs:comment>InchMercury is a UnitOfMeasure 

for barometricPressure.  It is used to express the number of 

inches of mercury supported in a mercurial barometer by the 

surrounding air pressure.</rdfs:comment></rdfs:Class><rdfs:Class rdf:ID="Inclining"><rdfs:subClassOf rdf:resource="http://reliant.teknowledge.com/DAML/SUMO.owl#BodyMotion" /><rdfs:subClassOf rdf:resource="#MotionDownward" /><rdfs:comment>Moving one's body downward from a vertical position.  

Note that this class covers cases of leaning forward, as well as those of 

reclining backwards.</rdfs:comment></rdfs:Class><rdfs:Class rdf:ID="IncomeTax"><rdfs:subClassOf rdf:resource="#Tax" /><rdfs:comment>A Tax on annual income.</rdfs:comment></rdfs:Class><rdfs:Class rdf:ID="IndependentState"><rdfs:subClassOf rdf:resource="http://reliant.teknowledge.com/DAML/SUMO.owl#GeopoliticalArea" /><rdfs:subClassOf rdf:resource="http://reliant.teknowledge.com/DAML/SUMO.owl#Nation" /><sumo:disjoint rdf:resource="#DependencyOrSpecialSovereigntyArea" /><rdfs:comment>IndependentState is a subclass of 

GeopoliticalArea, representing the classification 'Independent State' 

used by the CIA World Fact Book.</rdfs:comment></rdfs:Class><rdfs:Class rdf:ID="Indicating"><rdfs:subClassOf rdf:resource="http://reliant.teknowledge.com/DAML/SUMO.owl#Communication" /><rdfs:subClassOf rdf:resource="http://reliant.teknowledge.com/DAML/SUMO.owl#BodyMotion" /><rdfs:comment>Pointing out a person, place or thing with 

a BodyPart or with an Artifact.</rdfs:comment></rdfs:Class><rdfs:Class rdf:ID="IndividualRetirementAccount"><rdfs:subClassOf rdf:resource="#PensionPlan" /><rdfs:comment>A tax-deferred retirement 

account for an individual that permits individuals to set aside a certain 

amount per year, with earnings tax-deferred until withdrawals at retirement 

age(or earlier, with a penalty).  Only those who do not participate in a 

pension plan at work or who do participate and meet certain income guidelines 

can make deductible contributions to an IRA.  All others can make contributions 

to an IRA on a non-deductible basis.  Such contributions qualify as a deduction 

against income earned in that year and interest accumulates tax-deferred until 

the funds are withdrawn.</rdfs:comment></rdfs:Class><rdfs:Class rdf:ID="IndustrialPlant"><rdfs:subClassOf rdf:resource="http://reliant.teknowledge.com/DAML/SUMO.owl#StationaryArtifact" /><rdfs:comment>A Building or part of a Building or group 

of Buildings whose purpose is to Manufacture something.</rdfs:comment></rdfs:Class><rdfs:Class rdf:ID="Industry"><rdfs:subClassOf rdf:resource="http://reliant.teknowledge.com/DAML/SUMO.owl#Collection" /><rdfs:comment>The class of Collections of Corporations 

which are in the same line of business.</rdfs:comment></rdfs:Class><rdfs:Class rdf:ID="InfantryUnit"><rdfs:subClassOf rdf:resource="#MilitaryUnit" /><rdfs:comment>MilitaryUnits composed primarily of Soldiers 

who fight on foot, i.e. without the use of ArtilleryGuns.</rdfs:comment></rdfs:Class><rdfs:Class rdf:ID="InfectiousDisease"><rdfs:subClassOf rdf:resource="http://reliant.teknowledge.com/DAML/SUMO.owl#DiseaseOrSyndrome" /><rdfs:comment>Any DiseaseOrSyndrome that is caused by a 

Microorganism.</rdfs:comment></rdfs:Class><rdfs:Class rdf:ID="Inhaling"><rdfs:subClassOf rdf:resource="http://reliant.teknowledge.com/DAML/SUMO.owl#Breathing" /><rdfs:comment>Any instance of Breathing where the breath is 

taken into the Lungs.</rdfs:comment></rdfs:Class><rdfs:Class rdf:ID="Inheriting"><rdfs:subClassOf rdf:resource="http://reliant.teknowledge.com/DAML/SUMO.owl#UnilateralGetting" /><rdfs:comment>Any UnilateralGetting where the agent 

receives some part of the property of a person upon the death of the 

person.</rdfs:comment></rdfs:Class><rdfs:Class rdf:ID="Inlet"><rdfs:subClassOf rdf:resource="#BodyOfWater" /><rdfs:comment>Inlet is the class of bays or other recesses 

into the shore of a lake, sea, or river; includes narrow inlets, which 

are passages leading from open water through some barrier to a bay or 

lagoon.</rdfs:comment></rdfs:Class><rdfs:Class rdf:ID="Installing"><rdfs:subClassOf rdf:resource="http://reliant.teknowledge.com/DAML/SUMO.owl#Putting" /><rdfs:comment>Putting a Device in a location and configuring 

the Device so that it can be used as intended after the installation.</rdfs:comment></rdfs:Class><rdfs:Class rdf:ID="InstrumentalMusic"><rdfs:subClassOf rdf:resource="http://reliant.teknowledge.com/DAML/SUMO.owl#Music" /><rdfs:comment>Music which is produced exclusively 

by MusicalInstruments.</rdfs:comment></rdfs:Class><rdfs:Class rdf:ID="Insulin"><rdfs:subClassOf rdf:resource="#Hormone" /><rdfs:comment>A Hormone secreted by the Pancreas that is used 

to regulate the metabolism of Carbohydrates.</rdfs:comment></rdfs:Class><rdfs:Class rdf:ID="InsuranceCompany"><rdfs:subClassOf rdf:resource="http://reliant.teknowledge.com/DAML/SUMO.owl#CommercialAgent" /><rdfs:comment>A CommercialAgent that insures Agents 

for the payment of a premium or premiums.</rdfs:comment></rdfs:Class><rdfs:Class rdf:ID="InsurancePolicy"><rdfs:subClassOf rdf:resource="http://reliant.teknowledge.com/DAML/SUMO.owl#Certificate" /><rdfs:comment>A Certificate that states the terms of an 

insurance contract.</rdfs:comment></rdfs:Class><rdfs:Class rdf:ID="InterestBearingAccount"><rdfs:subClassOf rdf:resource="#FinancialAccount" /><rdfs:comment>FinancialAccounts that have a fixed 

or adjustable interest rate.</rdfs:comment></rdfs:Class><rdfs:Class rdf:ID="InternalCombustionEngine"><rdfs:subClassOf rdf:resource="#Engine" /><rdfs:comment>InternalCombustionEngine is 

the subclass of Engines in which a heat reaction that occurs inside 

the engine is transformed into mechanical energy.</rdfs:comment></rdfs:Class><rdfs:Class rdf:ID="InternationalOrganization"><rdfs:subClassOf rdf:resource="http://reliant.teknowledge.com/DAML/SUMO.owl#Organization" /><rdfs:comment>InternationalOrganization is 

the class of Organizations whose activities have international scope and 

which typically have members who are, or are from, different Nations.</rdfs:comment></rdfs:Class><rdfs:Class rdf:ID="Interviewing"><rdfs:subClassOf rdf:resource="#FormalMeeting" /><rdfs:comment>A FormalMeeting whose purpose is to acquire 

information from the interviewee that can be used in a media report.</rdfs:comment></rdfs:Class><rdfs:Class rdf:ID="Intestine"><rdfs:subClassOf rdf:resource="http://reliant.teknowledge.com/DAML/SUMO.owl#BodyVessel" /><rdfs:subClassOf rdf:resource="http://reliant.teknowledge.com/DAML/SUMO.owl#AnimalAnatomicalStructure" /><rdfs:comment>A BodyVessel which connects the Stomach to 

the anus and which is used in digesting Food.</rdfs:comment></rdfs:Class><rdfs:Class rdf:ID="Investing"><rdfs:subClassOf rdf:resource="http://reliant.teknowledge.com/DAML/SUMO.owl#FinancialTransaction" /><rdfs:comment>An activity of commiting money or capital in order to 

gain a financial return.</rdfs:comment></rdfs:Class><rdfs:Class rdf:ID="Iodine"><rdfs:subClassOf rdf:resource="http://reliant.teknowledge.com/DAML/SUMO.owl#ElementalSubstance" /><atomicNumber>53</atomicNumber><rdfs:comment>Dark violet nonmetallic element, belongs to group 

17 of the periodic table.  Insoluble in water.  Required as a trace 

element for living organisms.  One stable isotope, I-127 exists, in 

addition to fourteen radioactive isotopes.  Chemically the least reactive 

of the halogens, and the most electropositive metallic halogen.  

Discovered in 1812 by Courtois.</rdfs:comment></rdfs:Class><rdfs:Class rdf:ID="Ion"><rdfs:subClassOf rdf:resource="http://reliant.teknowledge.com/DAML/SUMO.owl#PureSubstance" /><rdfs:comment>An electronically charged Atom or Molecule.  In 

other words, a PureSubstance that has lost one of its Electrons.</rdfs:comment></rdfs:Class><rdfs:Class rdf:ID="Iron"><rdfs:subClassOf rdf:resource="http://reliant.teknowledge.com/DAML/SUMO.owl#ElementalSubstance" /><atomicNumber>26</atomicNumber><rdfs:comment>Silvery malleable and ductile metallic transition 

element.  Has nine isotopes and is the fourth most abundant element in the 

earth's crust.  Required by living organisms as a trace element (used in 

hemoglobin in humans.) Quite reactive, oxidizes in moist air, displaces 

hydrogen from dilute acids and combines with nonmetallic elements.</rdfs:comment></rdfs:Class><rdfs:Class rdf:ID="Ivory"><rdfs:subClassOf rdf:resource="http://reliant.teknowledge.com/DAML/SUMO.owl#Bone" /><rdfs:comment>A very hard substance that makes up the tusks of 

elephants and walruses.</rdfs:comment></rdfs:Class><rdfs:Class rdf:ID="Janitor"><rdfs:subClassOf rdf:resource="#UnskilledOccupation" /><rdfs:comment>Any Position which involves cleaning a Building 

or some of the Rooms within a Building.</rdfs:comment></rdfs:Class><rdfs:Class rdf:ID="Joule"><rdfs:subClassOf rdf:resource="http://reliant.teknowledge.com/DAML/SUMO.owl#FunctionQuantity" /><rdf:type rdf:resource="http://reliant.teknowledge.com/DAML/SUMO.owl#SystemeInternationalUnit" /><rdfs:comment>SI energy measure.  Symbol: J.  It is the work 

done when the point of application of 1 Newton is displaced a distance 

of 1 Meter in the direction of the force.  Joule = N*m = 

m^2*kg*s^(-2).</rdfs:comment></rdfs:Class><rdfs:Class rdf:ID="Journalist"><rdfs:subClassOf rdf:resource="#Profession" /><rdfs:comment>The Profession of being a news reporter, i.e. 

investigating and reporting, in a publication or broadcast program, current 

events.</rdfs:comment></rdfs:Class><rdfs:Class rdf:ID="Judge"><rdfs:subClassOf rdf:resource="#Attorney" /><rdfs:subClassOf rdf:resource="#GovernmentOfficer" /><rdfs:comment>An Attorney who has the power of deciding legal cases.</rdfs:comment></rdfs:Class><rdfs:Class rdf:ID="Jumping"><rdfs:subClassOf rdf:resource="http://reliant.teknowledge.com/DAML/SUMO.owl#BodyMotion" /><rdfs:subClassOf rdf:resource="#MotionUpward" /><rdfs:comment>Any MotionUpward which is done by one's body 

and which results in a situation where one's feet are unsupported.</rdfs:comment></rdfs:Class><rdfs:Class rdf:ID="JuniorCollege"><rdfs:subClassOf rdf:resource="#PostSecondarySchool" /><rdfs:comment>The class of PostSecondarySchools that 

offer an associate's degree and do not offer a bachelor's degree.</rdfs:comment></rdfs:Class><rdfs:Class rdf:ID="Jury"><rdfs:subClassOf rdf:resource="http://reliant.teknowledge.com/DAML/SUMO.owl#GroupOfPeople" /><rdfs:comment>A GroupOfPeople who are given the duty of rendering a 

verdict with respect to a LegalAction.</rdfs:comment></rdfs:Class><rdfs:Class rdf:ID="Key"><rdfs:subClassOf rdf:resource="#SecurityDevice" /><rdfs:comment>A Device which opens and closes a Lock.</rdfs:comment></rdfs:Class><rdfs:Class rdf:ID="Kicking"><rdfs:subClassOf rdf:resource="http://reliant.teknowledge.com/DAML/SUMO.owl#Impelling" /><rdfs:comment>Any instance of Impelling where the instrument 

is a Foot of the agent.</rdfs:comment></rdfs:Class><rdfs:Class rdf:ID="Kidnapping"><rdfs:subClassOf rdf:resource="#Robbing" /><rdfs:comment>Robbing a Human, i.e. taking him/her away 

with the threat of force.</rdfs:comment></rdfs:Class><rdfs:Class rdf:ID="Kidney"><rdfs:subClassOf rdf:resource="http://reliant.teknowledge.com/DAML/SUMO.owl#Organ" /><rdfs:subClassOf rdf:resource="http://reliant.teknowledge.com/DAML/SUMO.owl#AnimalAnatomicalStructure" /><rdfs:comment>An Organ that separates urine from other 

BodySubstances and passes it to the bladder.</rdfs:comment></rdfs:Class><rdfs:Class rdf:ID="KilowattHour"><rdf:type rdf:resource="http://reliant.teknowledge.com/DAML/SUMO.owl#UnitOfMeasure" /><rdfs:subClassOf rdf:resource="http://reliant.teknowledge.com/DAML/SUMO.owl#FunctionQuantity" /><rdfs:comment>KilowattHour is a UnitOfMeasure for 

energy that represents 1000 Watts (1 kW) of power expended over one 

hour (1 h) of time.  This is the unit commonly used in commercial 

power contexts.  It is equivalent to 3,600,000 Joules.</rdfs:comment></rdfs:Class><rdfs:Class rdf:ID="Kissing"><rdfs:subClassOf rdf:resource="http://reliant.teknowledge.com/DAML/SUMO.owl#Touching" /><rdfs:comment>The class of Touching processes where the lips 

are brought into contact with something else.</rdfs:comment></rdfs:Class><rdfs:Class rdf:ID="Kitchen"><rdfs:subClassOf rdf:resource="http://reliant.teknowledge.com/DAML/SUMO.owl#Room" /><rdfs:comment>A Room intended for Cooking.</rdfs:comment></rdfs:Class><rdfs:Class rdf:ID="Knee"><rdfs:subClassOf rdf:resource="#BodyJoint" /><rdfs:comment>The joint in the Leg connecting the tibia and fibula 

with the femur.</rdfs:comment></rdfs:Class><rdfs:Class rdf:ID="Knuckle"><rdfs:subClassOf rdf:resource="#BodyJoint" /><rdfs:comment>Any joint in a Finger.</rdfs:comment></rdfs:Class><rdfs:Class rdf:ID="Label"><rdfs:subClassOf rdf:resource="http://reliant.teknowledge.com/DAML/SUMO.owl#Text" /><rdfs:comment>A very brief Text that is attached to an Object 

and that indicates very specific information about the Object, e.g. its 

name, its monetaryValue, etc.</rdfs:comment></rdfs:Class><rdfs:Class rdf:ID="LaborStriking"><rdfs:subClassOf rdf:resource="http://reliant.teknowledge.com/DAML/SUMO.owl#OrganizationalProcess" /><rdfs:comment>A Process in which some or all of the 

employees of a UnionOrganization refuse to work until their pay is 

increased or their working conditions are improved in some respect.</rdfs:comment></rdfs:Class><rdfs:Class rdf:ID="Laboratory"><rdfs:subClassOf rdf:resource="http://reliant.teknowledge.com/DAML/SUMO.owl#StationaryArtifact" /><rdfs:comment>A Building, Room or suite of Rooms where 

scientific research, i.e. Experimenting, is conducted.</rdfs:comment></rdfs:Class><rdfs:Class rdf:ID="Ladder"><rdfs:subClassOf rdf:resource="http://reliant.teknowledge.com/DAML/SUMO.owl#Artifact" /><rdfs:comment>An Artifact which consists of two parallel supports 

connected by a series of rungs which can be used to ascend or descend.</rdfs:comment></rdfs:Class><rdfs:Class rdf:ID="Lamb"><rdfs:subClassOf rdf:resource="#Sheep" /><rdfs:comment>A young Sheep, i.e. a Sheep that is NonFullyFormed.</rdfs:comment></rdfs:Class><rdfs:Class rdf:ID="LandForm"><rdfs:subClassOf rdf:resource="http://reliant.teknowledge.com/DAML/SUMO.owl#LandArea" /><rdfs:comment>A LandForm is the class of geographically and/or 

geologically distinct areas that occur on Earth's surface, including mountains, 

hills, plains, valleys, deltas, and features of submerged land areas such as 

the ocean floor.</rdfs:comment></rdfs:Class><rdfs:Class rdf:about="http://reliant.teknowledge.com/DAML/SUMO.owl#LandTransitway"><rdfs:subClassOf rdf:resource="http://reliant.teknowledge.com/DAML/SUMO.owl#Transitway" /><rdfs:subClassOf rdf:resource="http://reliant.teknowledge.com/DAML/SUMO.owl#LandArea" /><rdfs:comment>LandTransitway is the subclass of 

Transitway that represents areas intended for motion over the ground.</rdfs:comment></rdfs:Class><rdfs:Class rdf:ID="LandTransportation"><rdfs:subClassOf rdf:resource="http://reliant.teknowledge.com/DAML/SUMO.owl#Transportation" /><rdfs:comment>Any instance of Transportation where the 

instrument is a LandVehicle.</rdfs:comment></rdfs:Class><rdfs:Class rdf:ID="LandVehicle"><rdfs:subClassOf rdf:resource="http://reliant.teknowledge.com/DAML/SUMO.owl#Vehicle" /><rdfs:comment>LandVehicle is the class of Vehicles that 

travel on land.  The two main types of LandVehicle are RoadVehicle and 

RollingStock.</rdfs:comment></rdfs:Class><rdfs:Class rdf:ID="Landing"><rdfs:subClassOf rdf:resource="http://reliant.teknowledge.com/DAML/SUMO.owl#Translocation" /><rdfs:comment>Any instance of Translocation which ends up on 

something other than an AtmosphericRegion and which has an instance of 

Flying as a subProcess.</rdfs:comment></rdfs:Class><rdfs:Class rdf:ID="LandlockedWater"><rdfs:subClassOf rdf:resource="#BodyOfWater" /><rdfs:comment>LandlockedWater includes water 

areas that are surrounded by land, including salt lakes, fresh 

water lakes, ponds, reservoirs, and (more or less) wetlands.</rdfs:comment></rdfs:Class><rdfs:Class rdf:ID="Laughing"><rdfs:subClassOf rdf:resource="http://reliant.teknowledge.com/DAML/SUMO.owl#Vocalizing" /><rdfs:subClassOf rdf:resource="#FacialExpression" /><rdfs:comment>Expressing happiness by Vocalizing in a 

certain way.</rdfs:comment></rdfs:Class><rdfs:Class rdf:ID="LawEnforcement"><rdfs:subClassOf rdf:resource="http://reliant.teknowledge.com/DAML/SUMO.owl#PoliticalProcess" /><rdfs:subClassOf rdf:resource="http://reliant.teknowledge.com/DAML/SUMO.owl#RegulatoryProcess" /><rdfs:comment>Any RegulatoryProcess where the agent is either 

a PoliceOrganization or a member of a PoliceOrganization.  This covers 

everything from issuing a traffic ticket to arresting someone on suspicion of having 

committed a Murder.</rdfs:comment></rdfs:Class><rdfs:Class rdf:ID="Lawn"><rdfs:subClassOf rdf:resource="#CultivatedLandArea" /><rdfs:comment>A CultivatedLandArea containing mowed Grass.</rdfs:comment></rdfs:Class><rdfs:Class rdf:ID="LayingEggs"><rdfs:subClassOf rdf:resource="http://reliant.teknowledge.com/DAML/SUMO.owl#OrganismProcess" /><rdfs:comment>Any OrganismProcess where an Egg is expelled 

from the body of a Animal, e.g. a Bird or Reptile laying eggs.</rdfs:comment></rdfs:Class><rdfs:Class rdf:ID="Lead"><rdfs:subClassOf rdf:resource="http://reliant.teknowledge.com/DAML/SUMO.owl#ElementalSubstance" /><atomicNumber>82</atomicNumber><rdfs:comment>Heavy dull grey ductile metallic element, belongs to 

group 14.  Used in building construction, lead-place accumulators, bullets 

and shot, and is part of solder, pewter, bearing metals, type metals and 

fusible alloys.</rdfs:comment></rdfs:Class><rdfs:Class rdf:ID="Leather"><rdfs:subClassOf rdf:resource="http://reliant.teknowledge.com/DAML/SUMO.owl#Fabric" /><rdfs:comment>A Fabric that is the result of tanning an Animal 

Skin.</rdfs:comment></rdfs:Class><rdfs:Class rdf:ID="Leaving"><rdfs:subClassOf rdf:resource="http://reliant.teknowledge.com/DAML/SUMO.owl#Translocation" /><rdfs:comment>The initial part of any instance of Translocation.</rdfs:comment></rdfs:Class><rdfs:Class rdf:ID="Lecture"><rdfs:subClassOf rdf:resource="http://reliant.teknowledge.com/DAML/SUMO.owl#Demonstrating" /><rdfs:subClassOf rdf:resource="http://reliant.teknowledge.com/DAML/SUMO.owl#Speaking" /><rdfs:comment>Any instance of Speaking which is done before an 

assembled audience.</rdfs:comment></rdfs:Class><rdfs:Class rdf:ID="Leg"><rdfs:subClassOf rdf:resource="#Limb" /><rdfs:comment>The lower Limbs of Primates.</rdfs:comment></rdfs:Class><rdfs:Class rdf:ID="LegalAppeal"><rdfs:subClassOf rdf:resource="http://reliant.teknowledge.com/DAML/SUMO.owl#Requesting" /><rdfs:subClassOf rdf:resource="http://reliant.teknowledge.com/DAML/SUMO.owl#JudicialProcess" /><rdfs:comment>Asking that a higher court reconsider a LegalDecision 

of a lower court.</rdfs:comment></rdfs:Class><rdfs:Class rdf:ID="LegalAquittal"><rdfs:subClassOf rdf:resource="http://reliant.teknowledge.com/DAML/SUMO.owl#LegalDecision" /><rdfs:comment>Any LegalDecision where the defendant is found 

not to be guilty of the crime for which the corresponding trial was held.</rdfs:comment></rdfs:Class><rdfs:Class rdf:ID="LegalAward"><rdfs:subClassOf rdf:resource="http://reliant.teknowledge.com/DAML/SUMO.owl#LegalDecision" /><rdfs:comment>Any LegalDecision which gives to the plaintiff of 

the corresponding LegalAction some amount of monetary compensation.</rdfs:comment></rdfs:Class><rdfs:Class rdf:ID="LegalCharge"><rdfs:subClassOf rdf:resource="http://reliant.teknowledge.com/DAML/SUMO.owl#LegalAction" /><rdfs:comment>Any LegalAction of which a Government is 

the agent.</rdfs:comment></rdfs:Class><rdfs:Class rdf:ID="LegalConviction"><rdfs:subClassOf rdf:resource="http://reliant.teknowledge.com/DAML/SUMO.owl#LegalDecision" /><rdfs:comment>Any LegalDecision where the defendant is found 

guilty of the crime for which the corresponding trial was held.</rdfs:comment></rdfs:Class><rdfs:Class rdf:ID="LegalDismissal"><rdfs:subClassOf rdf:resource="http://reliant.teknowledge.com/DAML/SUMO.owl#LegalDecision" /><rdfs:comment>Any LegalDecision where the LegalAction of 

the plaintiff is dismissed by the court, e.g. for lack of merit.</rdfs:comment></rdfs:Class><rdfs:Class rdf:ID="LegalOpinion"><rdfs:subClassOf rdf:resource="http://reliant.teknowledge.com/DAML/SUMO.owl#Argument" /><rdfs:comment>An Argument that explains the reasoning behind a 

LegalDecision.</rdfs:comment></rdfs:Class><rdfs:Class rdf:ID="LegalSummons"><rdfs:subClassOf rdf:resource="http://reliant.teknowledge.com/DAML/SUMO.owl#Ordering" /><rdfs:subClassOf rdf:resource="http://reliant.teknowledge.com/DAML/SUMO.owl#JudicialProcess" /><rdfs:comment>An official order that a person appear at a 

CourtRoom at a specified time.</rdfs:comment></rdfs:Class><rdfs:Class rdf:ID="LegalSystemAttribute"><rdfs:subClassOf rdf:resource="http://reliant.teknowledge.com/DAML/SUMO.owl#RelationalAttribute" /><rdfs:comment>LegalSystemAttribute is the class 

of Attributes that are used to characterize legal systems, as, e.g., 

according to their sources, areas of concern, or principles of 

organization.</rdfs:comment></rdfs:Class><rdfs:Class rdf:ID="LegislativeOrganization"><rdfs:subClassOf rdf:resource="http://reliant.teknowledge.com/DAML/SUMO.owl#Organization" /><rdfs:comment>LegislativeOrganization is the 

class of Organizations that have as their main purpose the passing of 

laws or regulations.</rdfs:comment></rdfs:Class><rdfs:Class rdf:ID="LemonFruit"><rdfs:subClassOf rdf:resource="http://reliant.teknowledge.com/DAML/SUMO.owl#FruitOrVegetable" /><rdfs:subClassOf rdf:resource="http://reliant.teknowledge.com/DAML/SUMO.owl#Food" /><rdfs:comment>A citrus FruitOrVegetable that has a yellow skin 

and a tart, acidic flavor.</rdfs:comment></rdfs:Class><rdfs:Class rdf:ID="Lengthening"><rdfs:subClassOf rdf:resource="http://reliant.teknowledge.com/DAML/SUMO.owl#Increasing" /><rdfs:comment>Increasing the length of something.</rdfs:comment></rdfs:Class><rdfs:Class rdf:ID="Lens"><rdfs:subClassOf rdf:resource="#OpticalDevice" /><rdfs:comment>An OpticalDevice which consists of a polished, 

transparent piece of glass or plastic.  Lenses are often part of 

other OpticalDevices.</rdfs:comment></rdfs:Class><rdfs:Class rdf:ID="Lesion"><rdfs:subClassOf rdf:resource="http://reliant.teknowledge.com/DAML/SUMO.owl#AbnormalAnatomicalStructure" /><rdfs:comment>Any AbnormalAnatomicalStructure which is the result of 

an Injuring and which is found on the surface of an Organ.</rdfs:comment></rdfs:Class><rdfs:Class rdf:ID="LiabilityAccount"><rdfs:subClassOf rdf:resource="#FinancialAccount" /><rdfs:comment>An account for which a person is liable.</rdfs:comment></rdfs:Class><rdfs:Class rdf:ID="Library"><rdfs:subClassOf rdf:resource="http://reliant.teknowledge.com/DAML/SUMO.owl#EducationalOrganization" /><rdfs:comment>An EducationalOrganization which is a repository 

of Texts which have been classified for efficient retrieval.</rdfs:comment></rdfs:Class><rdfs:Class rdf:ID="License"><rdfs:subClassOf rdf:resource="http://reliant.teknowledge.com/DAML/SUMO.owl#Certificate" /><rdfs:comment>License is the subclass of Certificates that 

are granted by a GovernmentOrganization and that authorize the performance 

of a kind of action, e.g., driving, exporting, travelling to another 

country, etc.</rdfs:comment></rdfs:Class><rdfs:Class rdf:ID="Licking"><rdfs:subClassOf rdf:resource="http://reliant.teknowledge.com/DAML/SUMO.owl#Touching" /><rdfs:comment>The class of Touching processes where the Tongue 

is brought into contact with something else.</rdfs:comment></rdfs:Class><rdfs:Class rdf:ID="Lieutenant"><rdfs:subClassOf rdf:resource="#MilitaryOfficer" /><rdfs:comment>A commissioned MilitaryOfficer.</rdfs:comment></rdfs:Class><rdfs:Class rdf:ID="Lightning"><rdfs:subClassOf rdf:resource="http://reliant.teknowledge.com/DAML/SUMO.owl#WeatherProcess" /><rdfs:subClassOf rdf:resource="http://reliant.teknowledge.com/DAML/SUMO.owl#Radiating" /><rdfs:comment>A WeatherProcess which involves a significant 

release of electricity from a Cloud.</rdfs:comment></rdfs:Class><rdfs:Class rdf:ID="LilacFlower"><rdfs:subClassOf rdf:resource="http://reliant.teknowledge.com/DAML/SUMO.owl#FloweringPlant" /><rdfs:comment>A FloweringPlant that has large clusters of 

aromatic flowers.</rdfs:comment></rdfs:Class><rdfs:Class rdf:ID="Limb"><rdfs:subClassOf rdf:resource="http://reliant.teknowledge.com/DAML/SUMO.owl#AnimalAnatomicalStructure" /><rdfs:subClassOf rdf:resource="http://reliant.teknowledge.com/DAML/SUMO.owl#BodyPart" /><rdfs:comment>Animal Appendages with joints that are used for movement 

and grasping.</rdfs:comment></rdfs:Class><rdfs:Class rdf:ID="LinguisticAttribute"><rdfs:subClassOf rdf:resource="http://reliant.teknowledge.com/DAML/SUMO.owl#InternalAttribute" /><rdfs:comment>Any Attribute that is 

expressed by a Language or class of Languages.</rdfs:comment></rdfs:Class><rdfs:Class rdf:ID="Lip"><rdfs:subClassOf rdf:resource="http://reliant.teknowledge.com/DAML/SUMO.owl#AnimalAnatomicalStructure" /><rdfs:subClassOf rdf:resource="http://reliant.teknowledge.com/DAML/SUMO.owl#BodyPart" /><rdfs:comment>Folds of Tissue surrounding the mouths of some 

Vertebrates.</rdfs:comment></rdfs:Class><rdfs:Class rdf:ID="LiquefiedPetroleumGas"><rdfs:subClassOf rdf:resource="#FossilFuel" /><rdfs:subClassOf rdf:resource="#RefinedPetroleumProduct" /><rdfs:comment>LiquefiedPetroleumGas is a 

compressed hydrocarbon gas.</rdfs:comment></rdfs:Class><rdfs:Class rdf:ID="LiquidBodySubstance"><rdfs:subClassOf rdf:resource="http://reliant.teknowledge.com/DAML/SUMO.owl#BodySubstance" /><rdfs:comment>Any BodySubstance which is Liquid 

under normal circumstances.</rdfs:comment></rdfs:Class><rdfs:Class rdf:ID="LiquorShot"><rdfs:subClassOf rdf:resource="#DistilledAlcoholicBeverage" /><rdfs:comment>A small serving of a DistilledAlcoholicBeverage.</rdfs:comment></rdfs:Class><rdfs:Class rdf:ID="Liver"><rdfs:subClassOf rdf:resource="http://reliant.teknowledge.com/DAML/SUMO.owl#Organ" /><rdfs:subClassOf rdf:resource="http://reliant.teknowledge.com/DAML/SUMO.owl#AnimalAnatomicalStructure" /><rdfs:comment>An Organ that secretes bile and serves metabolic 

functions.</rdfs:comment></rdfs:Class><rdfs:Class rdf:ID="LoadingWeapon"><rdfs:subClassOf rdf:resource="http://reliant.teknowledge.com/DAML/SUMO.owl#Inserting" /><rdfs:comment>Inserting ammunition into a ProjectileWeapon 

in such a way that the ammunition can be fired by the weapon.</rdfs:comment></rdfs:Class><rdfs:Class rdf:ID="Loan"><rdfs:subClassOf rdf:resource="#LiabilityAccount" /><rdfs:comment>An arrangement in which a lender gives money or property to a borrower, 

and the borrower agrees to return the property or repay the money, usually along with interest, 

at some future point(s) in time.</rdfs:comment></rdfs:Class><rdfs:Class rdf:ID="Lock"><rdfs:subClassOf rdf:resource="#SecurityDevice" /><rdfs:comment>A Device, which, through a Key or a combination prevents 

access to a Container or StationaryArtifact.</rdfs:comment></rdfs:Class><rdfs:Class rdf:ID="Locomotive"><rdfs:subClassOf rdf:resource="#RollingStock" /><rdfs:subClassOf rdf:resource="#SelfPoweredVehicle" /><rdfs:comment>Locomotive is the subclass of RollingStock

that represents train locomotives, including those with DieselEngines 

and with SteamEngines.</rdfs:comment></rdfs:Class><rdfs:Class rdf:ID="LosingConsciousness"><rdfs:subClassOf rdf:resource="http://reliant.teknowledge.com/DAML/SUMO.owl#PsychologicalProcess" /><sumo:disjoint rdf:resource="#GainingConsciousness" /><rdfs:comment>The process of transitioning from a state 

of being Awake to a state of being Unconscious.</rdfs:comment></rdfs:Class><rdfs:Class rdf:ID="LowTide"><rdfs:subClassOf rdf:resource="#TidalProcess" /><rdfs:comment>LowTide is the class of TidalProcesses that 

occur twice a day in marine waters, in which the water level falls below 

the mean sea level.</rdfs:comment></rdfs:Class><rdfs:Class rdf:ID="LowlandArea"><rdfs:subClassOf rdf:resource="#LandForm" /><rdfs:comment>A LowlandArea is a land area lower than the surrounding region, and usually level land.</rdfs:comment></rdfs:Class><rdfs:Class rdf:ID="Lumen"><rdfs:subClassOf rdf:resource="http://reliant.teknowledge.com/DAML/SUMO.owl#FunctionQuantity" /><rdf:type rdf:resource="http://reliant.teknowledge.com/DAML/SUMO.owl#SystemeInternationalUnit" /><rdfs:comment>SI luminous flux measure.  Symbol: lm.  It is the 

amount streaming outward through one solid angle of 1 Steradian from a 

uniform point source having an intensity of one Candela.  Lumen = 

cd*sr = cd * 1.</rdfs:comment></rdfs:Class><rdfs:Class rdf:ID="Lung"><rdfs:subClassOf rdf:resource="http://reliant.teknowledge.com/DAML/SUMO.owl#Organ" /><rdfs:subClassOf rdf:resource="http://reliant.teknowledge.com/DAML/SUMO.owl#AnimalAnatomicalStructure" /><rdfs:comment>A respiratory organ of Vertebrates.  Its function is 

to furnish the blood with oxygen and to remove carbon dioxide.</rdfs:comment></rdfs:Class><rdfs:Class rdf:ID="Lux"><rdfs:subClassOf rdf:resource="http://reliant.teknowledge.com/DAML/SUMO.owl#FunctionQuantity" /><rdf:type rdf:resource="http://reliant.teknowledge.com/DAML/SUMO.owl#SystemeInternationalUnit" /><rdfs:comment>SI illuminance measure.  Symbol: lx.  It is the 

amount of illumination provided when one Lumen is evenly distributed 

over an area of 1 square Meter. This is also equivalent to the 

illumination that would exist on a surface all points of which are one 

Meter from a point source of one Candela.  Lux = lm/m^2 = 

m^(-2)*cd.</rdfs:comment></rdfs:Class><rdfs:Class rdf:ID="LyingDown"><rdfs:subClassOf rdf:resource="http://reliant.teknowledge.com/DAML/SUMO.owl#BodyMotion" /><rdfs:comment>The BodyMotion of moving from a Sitting 

to a Prostrate position.</rdfs:comment></rdfs:Class><rdfs:Class rdf:ID="Lyrics"><rdfs:subClassOf rdf:resource="http://reliant.teknowledge.com/DAML/SUMO.owl#Text" /><rdfs:comment>Any Text which contains just the words of 

a MusicalComposition.</rdfs:comment></rdfs:Class><rdfs:Class rdf:ID="Magazine"><rdfs:subClassOf rdf:resource="http://reliant.teknowledge.com/DAML/SUMO.owl#Periodical" /><rdfs:comment>A Periodical that is softbound and printed on 

glossy paper.</rdfs:comment></rdfs:Class><rdfs:Class rdf:ID="Magnetism"><rdfs:subClassOf rdf:resource="http://reliant.teknowledge.com/DAML/SUMO.owl#Radiating" /><rdfs:comment>Any instance of Radiating which 

involves the attraction of Iron.</rdfs:comment></rdfs:Class><rdfs:Class rdf:ID="Maid"><rdfs:subClassOf rdf:resource="#ServicePosition" /><rdfs:comment>Any ServicePosition where various needs of a person 

or family are served over a long period of time.  Note that these Positions 

are, by definition, filled only by Women.</rdfs:comment></rdfs:Class><rdfs:Class rdf:ID="Mailbox"><rdfs:subClassOf rdf:resource="#Container" /><rdfs:comment>A Container whose purpose is to receive items 

that are mailed to the address associated with the Mailbox.</rdfs:comment></rdfs:Class><rdfs:Class rdf:ID="Mailing"><rdfs:subClassOf rdf:resource="http://reliant.teknowledge.com/DAML/SUMO.owl#Transfer" /><rdfs:comment>Any instance of Transfer where a postal system is 

used to move the patient, either a Message or a package.</rdfs:comment></rdfs:Class><rdfs:Class rdf:ID="MajorGeneral"><rdfs:subClassOf rdf:resource="#MilitaryGeneral" /><rdfs:comment>A MilitaryGeneral that ranks above a 

BrigadierGeneral.</rdfs:comment></rdfs:Class><rdfs:Class rdf:ID="Manifold"><rdfs:subClassOf rdf:resource="http://reliant.teknowledge.com/DAML/SUMO.owl#EngineeringComponent" /><rdfs:comment>A pipe which has several outlets for other pipes that 

flow into or out of it.</rdfs:comment></rdfs:Class><rdfs:Class rdf:ID="ManualLabor"><rdfs:subClassOf rdf:resource="http://reliant.teknowledge.com/DAML/SUMO.owl#Position" /><rdfs:comment>Any Position which involves manual 

work.</rdfs:comment></rdfs:Class><rdfs:Class rdf:ID="Map"><rdfs:subClassOf rdf:resource="http://reliant.teknowledge.com/DAML/SUMO.owl#Icon" /><rdfs:comment>An Icon which represents one or more GeographicAreas 

(or even the entire Earth).</rdfs:comment></rdfs:Class><rdfs:Class rdf:ID="Marble"><rdfs:subClassOf rdf:resource="#Rock" /><rdfs:comment>A metamorphic Rock that is used in Constructing 

and in creating Sculptures.</rdfs:comment></rdfs:Class><rdfs:Class rdf:ID="MarineCorps"><rdfs:subClassOf rdf:resource="http://reliant.teknowledge.com/DAML/SUMO.owl#MilitaryOrganization" /><sumo:relatedInternalConcept rdf:resource="#Navy" /><rdfs:comment>MarineCorps is the subclass of 

MilitaryOrganization consisting of infantry forces that are ship-based 

or otherwise affiliated with naval forces, and assigned to tasks such as 

protecting ships or taking beachhead positions.</rdfs:comment></rdfs:Class><rdfs:Class rdf:ID="Marshal"><rdfs:subClassOf rdf:resource="#PoliceOfficer" /><rdfs:comment>A PoliceOfficer whose responsibility is to enforce 

the decisions of a law court.</rdfs:comment></rdfs:Class><rdfs:Class rdf:ID="Massaging"><rdfs:subClassOf rdf:resource="http://reliant.teknowledge.com/DAML/SUMO.owl#TherapeuticProcess" /><rdfs:subClassOf rdf:resource="http://reliant.teknowledge.com/DAML/SUMO.owl#Touching" /><rdfs:comment>A subclass of TherapeuticProcess which involves 

kneading Muscles in such a way that tension is relieved, blood circulation 

is increased, etc.</rdfs:comment></rdfs:Class><rdfs:Class rdf:ID="Mast"><rdfs:subClassOf rdf:resource="http://reliant.teknowledge.com/DAML/SUMO.owl#Artifact" /><rdfs:comment>A large pole in the center of a Watercraft which is 

used to support a sail.</rdfs:comment></rdfs:Class><rdfs:Class rdf:ID="MatchDevice"><rdfs:subClassOf rdf:resource="http://reliant.teknowledge.com/DAML/SUMO.owl#Device" /><rdfs:comment>A small stick of carboard or wood that is treated 

with chemicals that can be easily ignited with friction.  MatchDevices are 

used for starting fires.</rdfs:comment></rdfs:Class><rdfs:Class rdf:ID="MaterialHandlingEquipment"><rdfs:subClassOf rdf:resource="http://reliant.teknowledge.com/DAML/SUMO.owl#Device" /><rdfs:comment>MaterialHandlingEquipment 

is a class of Devices that are equipment used for handling goods and 

supplies more efficiently or safely.  Examples are cranes, hoists, 

forklifts, conveyors, racks, etc.</rdfs:comment></rdfs:Class><rdfs:Class rdf:ID="Mating"><rdfs:subClassOf rdf:resource="http://reliant.teknowledge.com/DAML/SUMO.owl#OrganismProcess" /><rdfs:comment>Any process of sexual intercourse between two Humans 

or Animals.</rdfs:comment></rdfs:Class><rdfs:Class rdf:ID="MediaOrganization"><rdfs:subClassOf rdf:resource="http://reliant.teknowledge.com/DAML/SUMO.owl#Organization" /><rdfs:comment>MediaOrganization is the subclass 

of Organization for groups whose primary purpose is the production or 

dissemination of media content.  For organizations that physically enable 

Communication, see CommunicationOrganization.</rdfs:comment></rdfs:Class><rdfs:Class rdf:ID="MedicalClinic"><rdfs:subClassOf rdf:resource="#CareOrganization" /><sumo:disjoint rdf:resource="http://reliant.teknowledge.com/DAML/SUMO.owl#Residence" /><rdfs:comment>A CareOrganization which provides medical care 

on an out-patient basis only, i.e. there are no rooms where patients may take 

up residence for a period of time while they receive care.</rdfs:comment></rdfs:Class><rdfs:Class rdf:ID="MedicalDoctor"><rdfs:subClassOf rdf:resource="#Profession" /><rdfs:comment>The Profession of being a medical doctor, 

i.e. having attended medical school and being licensed to practice medicine.</rdfs:comment></rdfs:Class><rdfs:Class rdf:ID="MedicalSchool"><rdfs:subClassOf rdf:resource="#GraduateSchool" /><rdfs:comment>A GraduateSchool that is devoted to 

MedicalScience and that grants the degree of doctor of medicine.</rdfs:comment></rdfs:Class><rdfs:Class rdf:ID="Medicine"><rdfs:subClassOf rdf:resource="http://reliant.teknowledge.com/DAML/SUMO.owl#BiologicallyActiveSubstance" /><rdfs:comment>Any BiologicallyActiveSubstance which has a 

therapeutic effect under certain conditions.</rdfs:comment></rdfs:Class><rdfs:Class rdf:ID="MediterraneanClimateZone"><rdfs:subClassOf rdf:resource="#TemperateClimateZone" /><rdfs:comment>MediterraneanClimateZone 

is a subclass of TemperateClimateZone that is characterized by 

mild, cool, wet winters and warm dry summers.  Mediterranean shores 

are the archetype, but the Mediterranean climate is also found elsewhere.</rdfs:comment></rdfs:Class><rdfs:Class rdf:ID="Memorizing"><rdfs:subClassOf rdf:resource="http://reliant.teknowledge.com/DAML/SUMO.owl#Learning" /><rdfs:comment>The process of committing a Text to memory.</rdfs:comment></rdfs:Class><rdfs:Class rdf:ID="Menstruation"><rdfs:subClassOf rdf:resource="http://reliant.teknowledge.com/DAML/SUMO.owl#OrganOrTissueProcess" /><rdfs:comment>A periodic discharge of Blood and other 

BiologicalSubstances by Females that is part of a readjustment of 

the uterus.</rdfs:comment></rdfs:Class><rdfs:Class rdf:ID="Mercury"><rdfs:subClassOf rdf:resource="http://reliant.teknowledge.com/DAML/SUMO.owl#ElementalSubstance" /><atomicNumber>80</atomicNumber><rdfs:comment>Heavy silvery liquid metallic element, belongs to 

the zinc group.  Used in thermometers, barometers and other scientific 

apparatus.  Less reactive than zinc and cadmium, does not displace 

hydrogen from acids.  Forms a number of complexes and organomercury 

compounds.</rdfs:comment></rdfs:Class><rdfs:Class rdf:ID="Message"><rdfs:subClassOf rdf:resource="http://reliant.teknowledge.com/DAML/SUMO.owl#FactualText" /><rdfs:comment>A FactualText which is intended to be delivered to 

and read by a Human, GroupOfPeople or Organization.</rdfs:comment></rdfs:Class><rdfs:Class rdf:ID="Messaging"><rdfs:subClassOf rdf:resource="http://reliant.teknowledge.com/DAML/SUMO.owl#Transfer" /><rdfs:comment>Any instance of Transfer where a Message is the 

patient.</rdfs:comment></rdfs:Class><rdfs:Class rdf:ID="MetallicAlloy"><rdfs:subClassOf rdf:resource="http://reliant.teknowledge.com/DAML/SUMO.owl#Mixture" /><rdfs:comment>A Mixture of two or more Metals, and 

possibly nonmetallic elements as well.  For example, steel is an alloy 

containing iron and manganese.</rdfs:comment></rdfs:Class><rdfs:Class rdf:ID="Meteorite"><rdfs:subClassOf rdf:resource="#Meteoroid" /><rdfs:comment>Any Meteoroid that leaves traces on the surface 

of Earth.</rdfs:comment></rdfs:Class><rdfs:Class rdf:ID="Meteoroid"><rdfs:subClassOf rdf:resource="http://reliant.teknowledge.com/DAML/SUMO.owl#AstronomicalBody" /><rdfs:comment>Any AstronomicalBody that breaks through the 

atmosphere of Earth.</rdfs:comment></rdfs:Class><rdfs:Class rdf:ID="MetricTon"><rdf:type rdf:resource="http://reliant.teknowledge.com/DAML/SUMO.owl#UnitOfMeasure" /><rdfs:subClassOf rdf:resource="http://reliant.teknowledge.com/DAML/SUMO.owl#MassMeasure" /><rdfs:comment>MetricTon is a UnitOfMeasure that represents 

a weight of 2,205 PoundMass.</rdfs:comment></rdfs:Class><rdfs:Class rdf:ID="Microphone"><rdfs:subClassOf rdf:resource="#ElectricDevice" /><rdfs:subClassOf rdf:resource="#CommunicationDevice" /><rdfs:comment>A CommunicationDevice that converts sound 

into electrical energy.</rdfs:comment></rdfs:Class><rdfs:Class rdf:ID="Microscope"><rdfs:subClassOf rdf:resource="#OpticalDevice" /><rdfs:comment>An OpticalDevice with a stand and a focus, which is 

used for magnifying the images of things that are placed in the stand.</rdfs:comment></rdfs:Class><rdfs:Class rdf:ID="MiddleLatitudeDesertClimateZone"><rdfs:subClassOf rdf:resource="#DesertClimateZone" /><rdfs:comment>MiddleLatitudeDesertClimateZone is the subclass of 

DesertClimateZone characterized by a cool dry climate 

typical of middle latitude deserts.  This is subtype 'BWk' 

in the Keoppen climate system.</rdfs:comment></rdfs:Class><rdfs:Class rdf:ID="MidlatitudeContinentalClimateZone"><rdfs:subClassOf rdf:resource="#ClimateZone" /><rdfs:comment>MidlatitudeContinentalClimateZone is a subclass of 

TemperateClimateZone that is characterized by cool winters 

and hot summers.</rdfs:comment></rdfs:Class><rdfs:Class rdf:ID="MilitaryAircraft"><rdfs:subClassOf rdf:resource="#Aircraft" /><rdfs:subClassOf rdf:resource="#MilitaryVehicle" /><rdfs:comment>Any Aircraft which is made for a 

MilitaryOrganization.  This includes fighters, Bombers, attack 

helicopters, etc.</rdfs:comment></rdfs:Class><rdfs:Class rdf:ID="MilitaryArtifact"><rdfs:subClassOf rdf:resource="http://reliant.teknowledge.com/DAML/SUMO.owl#Artifact" /><rdfs:comment>Any Artifact which is made for a 

MilitaryOrganization.</rdfs:comment></rdfs:Class><rdfs:Class rdf:ID="MilitaryBrigade"><rdfs:subClassOf rdf:resource="#MilitaryUnit" /><rdfs:comment>Any MilitaryUnit with the rank of 

brigade.</rdfs:comment></rdfs:Class><rdfs:Class rdf:ID="MilitaryCompany"><rdfs:subClassOf rdf:resource="#MilitaryUnit" /><rdfs:comment>Any MilitaryUnit with the rank of 

company.</rdfs:comment></rdfs:Class><rdfs:Class rdf:ID="MilitaryCorps"><rdfs:subClassOf rdf:resource="#MilitaryUnit" /><rdfs:comment>Any MilitaryUnit with the rank of 

corps.</rdfs:comment></rdfs:Class><rdfs:Class rdf:ID="MilitaryDivision"><rdfs:subClassOf rdf:resource="#MilitaryUnit" /><rdfs:comment>Any MilitaryUnit with the rank of 

division.</rdfs:comment></rdfs:Class><rdfs:Class rdf:ID="MilitaryFront"><rdfs:subClassOf rdf:resource="http://reliant.teknowledge.com/DAML/SUMO.owl#GeographicArea" /><rdfs:comment>A GeographicArea along which opposing military 

forces confront one another in a Battle.</rdfs:comment></rdfs:Class><rdfs:Class rdf:ID="MilitaryGeneral"><rdfs:subClassOf rdf:resource="#MilitaryOfficer" /><rdfs:comment>MilitaryGeneral is a generic Position 

that indicates holding (or having held) the rank of General in some 

military force.  An indicator that someone uses the title, without 

committing to his or her exact rank or military affiliation.</rdfs:comment></rdfs:Class><rdfs:Class rdf:ID="MilitaryInfiltration"><rdfs:subClassOf rdf:resource="http://reliant.teknowledge.com/DAML/SUMO.owl#MilitaryProcess" /><rdfs:subClassOf rdf:resource="http://reliant.teknowledge.com/DAML/SUMO.owl#Translocation" /><rdfs:comment>Any Process by a MilitaryOrganization 

which involves moving through enemy positions without detection by the enemy.</rdfs:comment></rdfs:Class><rdfs:Class rdf:ID="MilitaryInstallation"><rdfs:subClassOf rdf:resource="http://reliant.teknowledge.com/DAML/SUMO.owl#StationaryArtifact" /><rdfs:subClassOf rdf:resource="#MilitaryArtifact" /><rdfs:comment>A StationaryArtifact consisting of grounds 

and Buildings that is intended to be used by a MilitaryOrganization.</rdfs:comment></rdfs:Class><rdfs:Class rdf:ID="MilitaryManeuver"><rdfs:subClassOf rdf:resource="http://reliant.teknowledge.com/DAML/SUMO.owl#Maneuver" /><rdfs:comment>Any Maneuver which takes place in a Battle 

and which is intended to secure a tactical advantage for one of the agents of 

the Battle.</rdfs:comment></rdfs:Class><rdfs:Class rdf:ID="MilitaryOfficer"><rdfs:subClassOf rdf:resource="#Soldier" /><rdfs:comment>The class of Soldiers who have authority or command.</rdfs:comment></rdfs:Class><rdfs:Class rdf:ID="MilitaryPlatoon"><rdfs:subClassOf rdf:resource="#MilitaryUnit" /><rdfs:comment>Any MilitaryUnit with the rank of 

platoon.</rdfs:comment></rdfs:Class><rdfs:Class rdf:ID="MilitaryPrivate"><rdfs:subClassOf rdf:resource="#Soldier" /><rdfs:comment>An enlisted Soldier of the lowest rank.</rdfs:comment></rdfs:Class><rdfs:Class rdf:ID="MilitaryRegiment"><rdfs:subClassOf rdf:resource="#MilitaryUnit" /><rdfs:comment>Any MilitaryUnit with the rank of 

regiment.</rdfs:comment></rdfs:Class><rdfs:Class rdf:ID="MilitaryReserveForce"><rdfs:subClassOf rdf:resource="http://reliant.teknowledge.com/DAML/SUMO.owl#MilitaryOrganization" /><rdfs:comment>MilitaryReserveForce is the subclass 

of MilitaryOrganizations that consist of forces trained in military 

procedures and activities, which are subject to being called to active duty 

if needed.</rdfs:comment></rdfs:Class><rdfs:Class rdf:ID="MilitaryService"><rdfs:subClassOf rdf:resource="http://reliant.teknowledge.com/DAML/SUMO.owl#MilitaryOrganization" /><rdfs:comment>A branch of the armed forces of a Nation.  

For example, there are five military services in the United States, the army, 

the navy, the air force, the marines, and the coast guard.</rdfs:comment></rdfs:Class><rdfs:Class rdf:ID="MilitaryShip"><rdfs:subClassOf rdf:resource="#Ship" /><rdfs:subClassOf rdf:resource="#MilitaryVehicle" /><rdfs:comment>Any Ship which is made for a MilitaryOrganization.  

This includes aircraft carriers, destroyers, etc.</rdfs:comment></rdfs:Class><rdfs:Class rdf:ID="MilitarySquad"><rdfs:subClassOf rdf:resource="#MilitaryUnit" /><rdfs:comment>Any MilitaryUnit with the rank of squad.</rdfs:comment></rdfs:Class><rdfs:Class rdf:ID="MilitarySurplus"><rdfs:subClassOf rdf:resource="#MilitaryArtifact" /><rdfs:comment>Any MilitaryArtifact which is sold to a 

non-military customer.</rdfs:comment></rdfs:Class><rdfs:Class rdf:ID="MilitaryTank"><rdfs:subClassOf rdf:resource="#MilitaryVehicle" /><rdfs:subClassOf rdf:resource="#RoadVehicle" /><rdfs:subClassOf rdf:resource="#ArtilleryGun" /><rdfs:comment>A MilitaryVehicle that moves along the ground 

on treaded wheels and that contains a large cannon.</rdfs:comment></rdfs:Class><rdfs:Class rdf:ID="MilitaryUnit"><rdfs:subClassOf rdf:resource="http://reliant.teknowledge.com/DAML/SUMO.owl#MilitaryOrganization" /><rdfs:comment>Any MilitaryOrganization that can be dispatched 

to an area of operations.</rdfs:comment></rdfs:Class><rdfs:Class rdf:ID="MilitaryVehicle"><rdfs:subClassOf rdf:resource="http://reliant.teknowledge.com/DAML/SUMO.owl#Vehicle" /><rdfs:comment>Any Vehicle which is intended to be 

used by a MilitaryOrganization.</rdfs:comment></rdfs:Class><rdfs:Class rdf:ID="MilitaryWatercraft"><rdfs:subClassOf rdf:resource="#Watercraft" /><rdfs:comment>MilitaryWatercraft is the class of 

all Watercraft owned or leased for use by some MilitaryOrganization.</rdfs:comment></rdfs:Class><rdfs:Class rdf:ID="Milk"><rdfs:subClassOf rdf:resource="#LiquidBodySubstance" /><rdfs:subClassOf rdf:resource="http://reliant.teknowledge.com/DAML/SUMO.owl#Beverage" /><rdfs:comment>A nutritious BodySubstance produced by Mammals.</rdfs:comment></rdfs:Class><rdfs:Class rdf:ID="Millennium"><rdfs:subClassOf rdf:resource="http://reliant.teknowledge.com/DAML/SUMO.owl#TimeDuration" /><rdfs:subClassOf rdf:resource="http://reliant.teknowledge.com/DAML/SUMO.owl#UnitOfMeasure" /><rdfs:comment>The TimeDuration of 1000 years.</rdfs:comment></rdfs:Class><rdfs:Class rdf:ID="MineOrWell"><rdfs:subClassOf rdf:resource="http://reliant.teknowledge.com/DAML/SUMO.owl#StationaryArtifact" /><rdfs:comment>An construction in the earth from which 

Minerals or Water is removed, either in pure form or as part of 

some other Substance.</rdfs:comment></rdfs:Class><rdfs:Class rdf:ID="Mirror"><rdfs:subClassOf rdf:resource="http://reliant.teknowledge.com/DAML/SUMO.owl#Artifact" /><rdfs:comment>An Artifact with a surface that is capable of 

displaying an image by reflecting light.</rdfs:comment></rdfs:Class><rdfs:Class rdf:ID="Missile"><rdfs:subClassOf rdf:resource="#Projectile" /><rdfs:subClassOf rdf:resource="#SelfPoweredDevice" /><rdfs:comment>A Projectile that is self-propelled and contains 

an ExplosiveDevice.</rdfs:comment></rdfs:Class><rdfs:Class rdf:ID="MissionOrganization"><rdfs:subClassOf rdf:resource="http://reliant.teknowledge.com/DAML/SUMO.owl#ReligiousOrganization" /><rdfs:comment>The class of ReligiousOrganizations 

that send members to foreign countries with the aim of converting citizens 

of those countries to the beliefs of the ReligiousOrganization.</rdfs:comment></rdfs:Class><rdfs:Class rdf:ID="MixedLanguage"><rdfs:subClassOf rdf:resource="http://reliant.teknowledge.com/DAML/SUMO.owl#SpokenHumanLanguage" /><rdfs:comment>A MixedLanguage is a SpokenHumanLanguage 

that combines grammar and lexical items from two or more languages to create 

a new language that is essentially a linguistic mixture.</rdfs:comment></rdfs:Class><rdfs:Class rdf:ID="MmMercury"><rdfs:subClassOf rdf:resource="#AtmosphericPressureMeasure" /><rdf:type rdf:resource="http://reliant.teknowledge.com/DAML/SUMO.owl#UnitOfMeasure" /><rdfs:comment>MmMercury is a UnitOfMeasure 

for barometricPressure.  It is used to express the number 

of millimeters of mercury supported in a mercurial barometer

 by the surrounding air pressure.</rdfs:comment></rdfs:Class><rdfs:Class rdf:ID="MobileResidence"><rdfs:subClassOf rdf:resource="http://reliant.teknowledge.com/DAML/SUMO.owl#Artifact" /><sumo:disjoint rdf:resource="http://reliant.teknowledge.com/DAML/SUMO.owl#Residence" /><rdfs:comment>Anything which serves to house people but 

which changes its location from time to time, e.g. a motorhome, a mobile 

home, a Tend, etc.  Note that MobileResidence is disjoint from Residence, 

because the latter is a subclass of StationaryArtifact.</rdfs:comment></rdfs:Class><rdfs:Class rdf:ID="ModellingPosition"><rdfs:subClassOf rdf:resource="http://reliant.teknowledge.com/DAML/SUMO.owl#Position" /><rdfs:comment>Any Position which involves posing for an 

artist or photographer.</rdfs:comment></rdfs:Class><rdfs:Class rdf:ID="Mole"><rdfs:subClassOf rdf:resource="http://reliant.teknowledge.com/DAML/SUMO.owl#MassMeasure" /><rdf:type rdf:resource="http://reliant.teknowledge.com/DAML/SUMO.owl#SystemeInternationalUnit" /><rdfs:comment>SI amount of substance unit. symbol: mol. It is one 

of the base units in SI. It is defined as follows:  the Mole is the 

amount of substance of a system which contains as many elementary entities 

as there are atoms in 0.012 Kilograms of carbon 12.  Note that, when this 

UnitOfMeasure is used, the elementary entities must be specified - they 

may be atoms, molecules, ions, electrons, etc. or groups of such 

particles.</rdfs:comment></rdfs:Class><rdfs:Class rdf:ID="MonophonicMusic"><rdfs:subClassOf rdf:resource="http://reliant.teknowledge.com/DAML/SUMO.owl#Music" /><rdfs:comment>Music which has a single part, i.e. Music 

which cannot be divided into two or more contemporaneous subProcesses which 

are also instances of Music.</rdfs:comment></rdfs:Class><rdfs:Class rdf:ID="MonsoonClimateZone"><rdfs:subClassOf rdf:resource="#TropicalClimateZone" /><rdfs:comment>MonsoonClimateZone is the class 

of TropicalClimateZones in which there is a short dry season between 

rains heavy enough to keep the ground wet all through the year.  This 

is Koeppen climate system subtype 'Aw'.</rdfs:comment></rdfs:Class><rdfs:Class rdf:ID="Monument"><rdfs:subClassOf rdf:resource="http://reliant.teknowledge.com/DAML/SUMO.owl#StationaryArtifact" /><rdfs:comment>A StationaryArtifact whose purpose is to commemorate 

a person, animal or event.</rdfs:comment></rdfs:Class><rdfs:Class rdf:ID="Moon"><rdfs:subClassOf rdf:resource="#NaturalSatellite" /><rdfs:comment>Moon is the class of NaturalSatellites that 

orbit planets or large asteroids.</rdfs:comment></rdfs:Class><rdfs:Class rdf:ID="Morning"><rdfs:subClassOf rdf:resource="#DayTime" /><rdfs:comment>The class of TimeIntervals that begin at Sunrise 

and end at noon.</rdfs:comment></rdfs:Class><rdfs:Class rdf:ID="MortarGun"><rdfs:subClassOf rdf:resource="#ArtilleryGun" /><rdfs:comment>A short-range Gun that is positioned on the ground 

at a high angle and fires explosive shells.</rdfs:comment></rdfs:Class><rdfs:Class rdf:ID="Mortgage"><rdfs:subClassOf rdf:resource="#Loan" /><rdfs:comment>A loan to finance the purchase of real estate, usually with specified payment 

periods and interest rates.</rdfs:comment></rdfs:Class><rdfs:Class rdf:ID="Moth"><rdfs:subClassOf rdf:resource="http://reliant.teknowledge.com/DAML/SUMO.owl#Insect" /><rdfs:comment>Nocturnal Insect with a large body and antennae.</rdfs:comment></rdfs:Class><rdfs:Class rdf:ID="MotionDownward"><rdfs:subClassOf rdf:resource="http://reliant.teknowledge.com/DAML/SUMO.owl#Motion" /><rdfs:comment>Motion where an Object is moving toward the 

ground.</rdfs:comment></rdfs:Class><rdfs:Class rdf:ID="MotionPicture"><rdfs:subClassOf rdf:resource="http://reliant.teknowledge.com/DAML/SUMO.owl#ContentBearingObject" /><rdfs:comment>A ContentBearingObject which depicts motion 

(and which may have an audio or text component as well).  This Class covers 

films, videos, etc.</rdfs:comment></rdfs:Class><rdfs:Class rdf:ID="MotionPictureScene"><rdfs:subClassOf rdf:resource="#MotionPicture" /><rdfs:comment>A discrete part of a MotionPicture which is set in 

the same time period and the same location.</rdfs:comment></rdfs:Class><rdfs:Class rdf:ID="MotionPictureShot"><rdfs:subClassOf rdf:resource="#MotionPicture" /><rdfs:comment>A unit of action in a MotionPicture, a 

MotionPictureShot is a sequence of images which are captured by a single 

camera without interruption.</rdfs:comment></rdfs:Class><rdfs:Class rdf:ID="MotionUpward"><rdfs:subClassOf rdf:resource="http://reliant.teknowledge.com/DAML/SUMO.owl#Motion" /><sumo:disjoint rdf:resource="#MotionDownward" /><rdfs:comment>Motion where an Object is moving away 

from the ground.</rdfs:comment></rdfs:Class><rdfs:Class rdf:ID="MotorOil"><rdfs:subClassOf rdf:resource="#PetroleumLubricant" /><rdfs:comment>MotorOil is the subclass of PetroleumLubricants 

that are used to lubricate motors.</rdfs:comment></rdfs:Class><rdfs:Class rdf:ID="Motorcycle"><rdfs:subClassOf rdf:resource="#SelfPoweredRoadVehicle" /><rdfs:comment>Motorcycle is the subclass of RoadVehicles 

that have two wheels one behind the other in the frame, upon which the rider 

sits on a seat above the engine.</rdfs:comment></rdfs:Class><rdfs:Class rdf:ID="MotorizedRailwayCar"><rdfs:subClassOf rdf:resource="#RollingStock" /><rdfs:subClassOf rdf:resource="#SelfPoweredVehicle" /><rdfs:comment>MotorizedRailwayCar is the subclass 

of railway cars that carry their own power source.</rdfs:comment></rdfs:Class><rdfs:Class rdf:ID="Mounting"><rdfs:subClassOf rdf:resource="http://reliant.teknowledge.com/DAML/SUMO.owl#BodyMotion" /><rdfs:comment>Any BodyMotion which results in being On 

something else.</rdfs:comment></rdfs:Class><rdfs:Class rdf:ID="Mouse"><rdfs:subClassOf rdf:resource="http://reliant.teknowledge.com/DAML/SUMO.owl#Rodent" /><rdfs:comment>A Rodent that has a hairless tail like a Rat 

but that is smaller than a Rat.</rdfs:comment></rdfs:Class><rdfs:Class rdf:ID="Mouth"><rdfs:subClassOf rdf:resource="http://reliant.teknowledge.com/DAML/SUMO.owl#AnimalAnatomicalStructure" /><rdfs:subClassOf rdf:resource="http://reliant.teknowledge.com/DAML/SUMO.owl#BodyPart" /><rdfs:comment>Part of the Face, used for Ingesting Food 

and Vocalizing.</rdfs:comment></rdfs:Class><rdfs:Class rdf:ID="MoveableHoliday"><rdfs:subClassOf rdf:resource="#Holiday" /><rdfs:comment>MoveableHoliday is the class of 

Holidays whose observance is not fixed to recurrences of any particular 

calendar day.  For example, Memorial Day is observed on the last Monday 

of May.</rdfs:comment></rdfs:Class><rdfs:Class rdf:ID="MovingResidence"><rdfs:subClassOf rdf:resource="http://reliant.teknowledge.com/DAML/SUMO.owl#Transfer" /><rdfs:comment>Any instance of the process of changing one's 

residence, i.e. moving one's belongings to a new home.</rdfs:comment></rdfs:Class><rdfs:Class rdf:ID="Mule"><rdfs:subClassOf rdf:resource="http://reliant.teknowledge.com/DAML/SUMO.owl#HoofedMammal" /><rdfs:subClassOf rdf:resource="#DomesticAnimal" /><rdfs:comment>The product of a Male Donkey and a Female 

Horse.  Mules are always sterile.</rdfs:comment></rdfs:Class><rdfs:Class rdf:ID="MultiGraph"><rdfs:subClassOf rdf:resource="#Graph" /><rdfs:comment>The Class of multigraphs.  A multigraph 

is a Graph containing at least one pair of GraphNodes that are 

connected by more than one GraphArc.</rdfs:comment></rdfs:Class><rdfs:Class rdf:ID="Murder"><rdfs:subClassOf rdf:resource="http://reliant.teknowledge.com/DAML/SUMO.owl#Killing" /><rdfs:subClassOf rdf:resource="#CriminalAction" /><rdfs:comment>Impermissible Killing of a Human.</rdfs:comment></rdfs:Class><rdfs:Class rdf:ID="Museum"><rdfs:subClassOf rdf:resource="http://reliant.teknowledge.com/DAML/SUMO.owl#EducationalOrganization" /><rdfs:comment>An EducationalOrganization where Artifacts of historic, 

scientific or aesthetic value are collected and exhibited.</rdfs:comment></rdfs:Class><rdfs:Class rdf:ID="MusicalComposition"><rdfs:subClassOf rdf:resource="http://reliant.teknowledge.com/DAML/SUMO.owl#Text" /><rdfs:comment>A Text that expresses the notes, 

words, etc. of a song or other sort of Music.</rdfs:comment></rdfs:Class><rdfs:Class rdf:ID="MusicalPerformance"><rdfs:subClassOf rdf:resource="#Performance" /><rdfs:comment>A Performance that consists exclusively of 

Music, e.g. an orchestra playing a symphony to an assembled audience.</rdfs:comment></rdfs:Class><rdfs:Class rdf:ID="MysteryStory"><rdfs:subClassOf rdf:resource="http://reliant.teknowledge.com/DAML/SUMO.owl#FictionalText" /><rdfs:comment>A FictionalText whose central plot element is a 

crime of some sort, usually a murder.</rdfs:comment></rdfs:Class><rdfs:Class rdf:ID="Nail"><rdfs:subClassOf rdf:resource="http://reliant.teknowledge.com/DAML/SUMO.owl#AttachingDevice" /><rdfs:comment>An AttachingDevice which is a thin piece of metal, with 

or without a head, that is fastened with a hammer.</rdfs:comment></rdfs:Class><rdfs:Class rdf:ID="NailDigit"><rdfs:subClassOf rdf:resource="http://reliant.teknowledge.com/DAML/SUMO.owl#AnimalAnatomicalStructure" /><rdfs:comment>Any of the horny structures which are found 

on the DigitAppendages of Primates and other Animals.</rdfs:comment></rdfs:Class><rdfs:Class rdf:ID="Narcotic"><rdfs:subClassOf rdf:resource="#ControlledSubstance" /><rdfs:comment>Narcotic is a subclass of addictive 

BiologicallyActiveSubstances that have damping effects on the 

nervous system and may be fatal in large doses.</rdfs:comment></rdfs:Class><rdfs:Class rdf:ID="NarrativeText"><rdfs:subClassOf rdf:resource="http://reliant.teknowledge.com/DAML/SUMO.owl#Text" /><rdfs:comment>Any Text that tells a story, whether true 

or false.</rdfs:comment></rdfs:Class><rdfs:Class rdf:ID="NationalFlag"><rdfs:subClassOf rdf:resource="#Flag" /><rdfs:comment>A Flag that is the official flag of a Nation, 

e.g. the stars and stripes is the NationalFlag of the UnitedStates.</rdfs:comment></rdfs:Class><rdfs:Class rdf:ID="NationalGovernment"><rdfs:subClassOf rdf:resource="http://reliant.teknowledge.com/DAML/SUMO.owl#Government" /><rdfs:comment>NationalGovernment is the class of 

governments of Nations.</rdfs:comment></rdfs:Class><rdfs:Class rdf:ID="NaturalSatellite"><rdfs:subClassOf rdf:resource="#Satellite" /><rdfs:subClassOf rdf:resource="http://reliant.teknowledge.com/DAML/SUMO.owl#AstronomicalBody" /><sumo:disjoint rdf:resource="http://reliant.teknowledge.com/DAML/SUMO.owl#Artifact" /><rdfs:comment>NaturalSatellite is the class of 

large, naturally occurring astronomical bodies orbiting some other 

AstronomicalBody.</rdfs:comment></rdfs:Class><rdfs:Class rdf:ID="Navy"><rdfs:subClassOf rdf:resource="#MilitaryService" /><rdfs:comment>MilitaryServices that are sea forces.</rdfs:comment></rdfs:Class><rdfs:Class rdf:ID="Neck"><rdfs:subClassOf rdf:resource="http://reliant.teknowledge.com/DAML/SUMO.owl#AnimalAnatomicalStructure" /><rdfs:subClassOf rdf:resource="http://reliant.teknowledge.com/DAML/SUMO.owl#BodyPart" /><rdfs:comment>The part of the body that connects the Head to the 

rest of the body.</rdfs:comment></rdfs:Class><rdfs:Class rdf:ID="Nectar"><rdfs:subClassOf rdf:resource="http://reliant.teknowledge.com/DAML/SUMO.owl#PlantSubstance" /><rdfs:comment>A sweet, sticky liquid that is produced by Plants 

and that attracts Insects.</rdfs:comment></rdfs:Class><rdfs:Class rdf:ID="Negotiating"><rdfs:subClassOf rdf:resource="http://reliant.teknowledge.com/DAML/SUMO.owl#Contest" /><rdfs:subClassOf rdf:resource="http://reliant.teknowledge.com/DAML/SUMO.owl#LinguisticCommunication" /><rdfs:comment>A Contest where each participant attempts to 

maximize his self-interest in a Promise that marks the end of the Contest.</rdfs:comment></rdfs:Class><rdfs:Class rdf:ID="NerveCell"><rdfs:subClassOf rdf:resource="http://reliant.teknowledge.com/DAML/SUMO.owl#Cell" /><rdfs:subClassOf rdf:resource="http://reliant.teknowledge.com/DAML/SUMO.owl#AnimalAnatomicalStructure" /><rdfs:comment>The Cells that make up a NervousSystem.</rdfs:comment></rdfs:Class><rdfs:Class rdf:ID="NervousSystem"><rdfs:subClassOf rdf:resource="http://reliant.teknowledge.com/DAML/SUMO.owl#Organ" /><rdfs:subClassOf rdf:resource="http://reliant.teknowledge.com/DAML/SUMO.owl#AnimalAnatomicalStructure" /><rdfs:comment>A system in Vertebrates that is made up of 

the Brain, the spinal cord, nerves, etc.</rdfs:comment></rdfs:Class><rdfs:Class rdf:ID="Nest"><rdfs:subClassOf rdf:resource="http://reliant.teknowledge.com/DAML/SUMO.owl#CorpuscularObject" /><rdfs:comment>Any structure which is created by nonhuman Animals for 

the purpose of giving birth to their offspring.</rdfs:comment></rdfs:Class><rdfs:Class rdf:ID="Neurosis"><rdfs:subClassOf rdf:resource="http://reliant.teknowledge.com/DAML/SUMO.owl#PsychologicalDysfunction" /><rdfs:comment>Any PsychologicalDysfunction which is not due 

to an organic impairment of the NervousSystem.</rdfs:comment></rdfs:Class><rdfs:Class rdf:ID="NewTestament"><rdfs:subClassOf rdf:resource="http://reliant.teknowledge.com/DAML/SUMO.owl#Book" /><sumo:subsumesContentClass rdf:resource="#ChristianGospel" /><rdfs:comment>The second and final part of the ChristianBible,

describing the life and teachings of Jesus Christ and the activities of his 

apostles.</rdfs:comment></rdfs:Class><rdfs:Class rdf:ID="NewsProgram"><rdfs:subClassOf rdf:resource="#BroadcastProgram" /><rdfs:comment>A BroadcastProgram that is devoted to 

reporting the latest events in a city, region, nation or the world at 

large.</rdfs:comment></rdfs:Class><rdfs:Class rdf:ID="Newspaper"><rdfs:subClassOf rdf:resource="http://reliant.teknowledge.com/DAML/SUMO.owl#Periodical" /><rdfs:comment>A Periodical that is published on a daily or 

weekly basis, that contains Reports, and whose issues are printed on 

newsprint paper.</rdfs:comment></rdfs:Class><rdfs:Class rdf:ID="Newton"><rdfs:subClassOf rdf:resource="http://reliant.teknowledge.com/DAML/SUMO.owl#FunctionQuantity" /><rdf:type rdf:resource="http://reliant.teknowledge.com/DAML/SUMO.owl#SystemeInternationalUnit" /><rdfs:comment>SI force measure.  Symbol: N. It is that force 

which gives to a mass of 1 kilogram an acceleration of 1 Meter per 

SecondDuration.  Newton = m*kg*s^(-2).</rdfs:comment></rdfs:Class><rdfs:Class rdf:ID="Nickel"><rdfs:subClassOf rdf:resource="http://reliant.teknowledge.com/DAML/SUMO.owl#ElementalSubstance" /><atomicNumber>28</atomicNumber><rdfs:comment>Malleable ductile silvery metallic transition 

element.  Discovered by A.F. Cronstedt in 1751.</rdfs:comment></rdfs:Class><rdfs:Class rdf:ID="NightTime"><rdfs:subClassOf rdf:resource="http://reliant.teknowledge.com/DAML/SUMO.owl#TimeInterval" /><rdfs:comment>The class of TimeIntervals that begin at Sunset

and end at Sunrise.</rdfs:comment></rdfs:Class><rdfs:Class rdf:ID="Nitrogen"><rdfs:subClassOf rdf:resource="http://reliant.teknowledge.com/DAML/SUMO.owl#ElementalSubstance" /><atomicNumber>7</atomicNumber><rdfs:comment>Colourless, gaseous element which belongs to 

group 15 of the periodic table.  Constitutes ~78 percent of the atmosphere 

and is an essential part of the ecosystem.  Nitrogen for industrial 

purposes is acquired by the fractional distillation of liquid air.  

Chemically inactive, reactive generally only at high temperatures or in 

electrical discharges.  It was discovered in 1772 by D.  Rutherford.</rdfs:comment></rdfs:Class><rdfs:Class rdf:ID="Nodding"><rdfs:subClassOf rdf:resource="http://reliant.teknowledge.com/DAML/SUMO.owl#Gesture" /><rdfs:comment>Moving the Head up and down or side to side 

to indicate approval or disapproval.</rdfs:comment></rdfs:Class><rdfs:Class rdf:ID="NonprofitOrganization"><rdfs:subClassOf rdf:resource="http://reliant.teknowledge.com/DAML/SUMO.owl#Organization" /><sumo:disjoint rdf:resource="http://reliant.teknowledge.com/DAML/SUMO.owl#CommercialAgent" /><rdfs:comment>Any Organization whose purpose is something 

other than making a profit.</rdfs:comment></rdfs:Class><rdfs:Class rdf:ID="NonspecificDisease"><rdfs:subClassOf rdf:resource="#InfectiousDisease" /><rdfs:comment>The class of InfectiousDiseases that 

are not caused by a single type of Microorganism.</rdfs:comment></rdfs:Class><rdfs:Class rdf:ID="Nose"><rdfs:subClassOf rdf:resource="http://reliant.teknowledge.com/DAML/SUMO.owl#Organ" /><rdfs:subClassOf rdf:resource="http://reliant.teknowledge.com/DAML/SUMO.owl#AnimalAnatomicalStructure" /><rdfs:comment>The Organ of Smelling.</rdfs:comment></rdfs:Class><rdfs:Class rdf:ID="Nostril"><rdfs:subClassOf rdf:resource="http://reliant.teknowledge.com/DAML/SUMO.owl#BodyVessel" /><rdfs:subClassOf rdf:resource="http://reliant.teknowledge.com/DAML/SUMO.owl#AnimalAnatomicalStructure" /><rdfs:comment>Either of two BodyVessels that run through the Nose 

and connect it to the Throat.</rdfs:comment></rdfs:Class><rdfs:Class rdf:ID="Novel"><rdfs:subClassOf rdf:resource="http://reliant.teknowledge.com/DAML/SUMO.owl#FictionalText" /><rdfs:subClassOf rdf:resource="http://reliant.teknowledge.com/DAML/SUMO.owl#Book" /><rdfs:comment>A FictionalText that is larger than a ShortStory 

and that is bound independently (i.e. it is a Book).</rdfs:comment></rdfs:Class><rdfs:Class rdf:ID="NuclearWeapon"><rdfs:subClassOf rdf:resource="#ExplosiveDevice" /><rdfs:subClassOf rdf:resource="http://reliant.teknowledge.com/DAML/SUMO.owl#Weapon" /><rdfs:comment>An ExplosiveDevice which achieves its effect 

by means of a critical mass of a radioactive substance.</rdfs:comment><rdfs:subClassOf rdf:resource="#RadioactiveWeapon" /><rdfs:comment>RadioactiveWeapons whose destructive power is 

achieved through nuclear energy.</rdfs:comment></rdfs:Class><rdfs:Class rdf:ID="OakWood"><rdfs:subClassOf rdf:resource="#WoodArtifact" /><rdfs:comment>Any WoodArtifact that is made from the Wood of an 

oak tree.</rdfs:comment></rdfs:Class><rdfs:Class rdf:ID="Oar"><rdfs:subClassOf rdf:resource="http://reliant.teknowledge.com/DAML/SUMO.owl#TransportationDevice" /><rdfs:comment>A Device consisting of a flat, broad surface attached to a 

handle that is used as an instrument in Rowing.</rdfs:comment></rdfs:Class><rdfs:Class rdf:ID="ObliqueAngle"><rdfs:subClassOf rdf:resource="http://reliant.teknowledge.com/DAML/SUMO.owl#TwoDimensionalAngle" /><rdfs:comment>Any TwoDimensionalAngle that has an 

angularMeasure that is greater than 90 AngularDegrees.</rdfs:comment></rdfs:Class><rdfs:Class rdf:ID="OccupationalTrade"><rdfs:subClassOf rdf:resource="#SkilledOccupation" /><rdfs:subClassOf rdf:resource="#ManualLabor" /><rdfs:comment>Any Position that involves skilled 

manual work.</rdfs:comment></rdfs:Class><rdfs:Class rdf:ID="Ocean"><rdfs:subClassOf rdf:resource="http://reliant.teknowledge.com/DAML/SUMO.owl#SaltWaterArea" /><rdfs:subClassOf rdf:resource="#BodyOfWater" /><rdfs:comment>Ocean is the class containing the oceans 

that are the major subdivisions of the WorldOcean.  According to 

the International Hydrographic Association, there are five oceans: 

the AtlanticOcean, PacificOcean, IndianOcean, SouthernOcean, 

and ArcticOcean.  Note: The largest oceans, the Atlantic and Pacific, 

are subdivided into Northern and Southern regions, but those regions 

are not separate Oceans.</rdfs:comment></rdfs:Class><rdfs:Class rdf:ID="OfferingForPurchase"><rdfs:subClassOf rdf:resource="http://reliant.teknowledge.com/DAML/SUMO.owl#Offering" /><rdfs:comment>Offering to buy something from someone.</rdfs:comment></rdfs:Class><rdfs:Class rdf:ID="OfferingForSale"><rdfs:subClassOf rdf:resource="http://reliant.teknowledge.com/DAML/SUMO.owl#Offering" /><rdfs:comment>Offering to sell something to someone.</rdfs:comment></rdfs:Class><rdfs:Class rdf:ID="Ohm"><rdfs:subClassOf rdf:resource="http://reliant.teknowledge.com/DAML/SUMO.owl#FunctionQuantity" /><rdf:type rdf:resource="http://reliant.teknowledge.com/DAML/SUMO.owl#SystemeInternationalUnit" /><rdfs:comment>SI electric resistance measure. It is the electric

resistance between two points of a conductor when a constant difference 

of potential of 1 Volt, applied between these two points,

produces in this conductor a current of 1 Ampere, this conductor not

being the force of any electromotive force.  Ohm = V/A = 

m^2*kg*s^(-3)*A^(-2).</rdfs:comment></rdfs:Class><rdfs:Class rdf:ID="Oil"><rdfs:subClassOf rdf:resource="http://reliant.teknowledge.com/DAML/SUMO.owl#Solution" /><rdfs:comment>A greasy, viscous Solution that cannot be mixed 

with Water.  Note that this general class covers petroleum oil, 

vegetable oil, animal fat, etc.</rdfs:comment></rdfs:Class><rdfs:Class rdf:ID="OilPaint"><rdfs:subClassOf rdf:resource="#Paint" /><sumo:disjoint rdf:resource="#WatercolorPaint" /><rdfs:comment>Any Paint which is an oil-based Solution.</rdfs:comment></rdfs:Class><rdfs:Class rdf:ID="OilPicture"><rdfs:subClassOf rdf:resource="#PaintedPicture" /><sumo:disjoint rdf:resource="#WatercolorPicture" /><rdfs:comment>Any OilPicture which is created 

with oil-based paints.</rdfs:comment></rdfs:Class><rdfs:Class rdf:ID="OldTestament"><rdfs:subClassOf rdf:resource="http://reliant.teknowledge.com/DAML/SUMO.owl#Book" /><rdfs:comment>The first part of the ChristianBible, describing 

the history of the Hebrew people.</rdfs:comment></rdfs:Class><rdfs:Class rdf:ID="OlympicGames"><rdfs:subClassOf rdf:resource="http://reliant.teknowledge.com/DAML/SUMO.owl#Sport" /><rdfs:comment>A sports event where athletes from various countries 

compete against one another.  The Olympics are now held every two years, either in 

the winter or the summer.</rdfs:comment></rdfs:Class><rdfs:Class rdf:ID="Opening"><rdfs:subClassOf rdf:resource="http://reliant.teknowledge.com/DAML/SUMO.owl#Motion" /><sumo:relatedInternalConcept rdf:resource="#Closing" /><rdfs:comment>The Class of Processes where an aperture is 

created in an Object.  Note that the aperture may be created intentionally, 

as when one opens a door, or unintentionally, as when the ground ruptures 

in a seismic event.</rdfs:comment></rdfs:Class><rdfs:Class rdf:ID="OpeningEyes"><rdfs:subClassOf rdf:resource="#EyeMotion" /><sumo:disjoint rdf:resource="#ClosingEyes" /><rdfs:comment>The EyeMotion of relaxing the eye lids so that 

the corneas are exposed to light.</rdfs:comment></rdfs:Class><rdfs:Class rdf:ID="Opera"><rdfs:subClassOf rdf:resource="#DramaticPlay" /><rdfs:comment>A DramaticPlay that is set to Music.</rdfs:comment></rdfs:Class><rdfs:Class rdf:ID="Opium"><rdfs:subClassOf rdf:resource="#Depressant" /><rdfs:subClassOf rdf:resource="http://reliant.teknowledge.com/DAML/SUMO.owl#PlantSubstance" /><rdfs:comment>A substance harvested from the seed capsules of the 

opium poppy that contains various powerful alkaloids.</rdfs:comment></rdfs:Class><rdfs:Class rdf:ID="OpticalDevice"><rdfs:subClassOf rdf:resource="http://reliant.teknowledge.com/DAML/SUMO.owl#Device" /><rdfs:comment>A Device which enables someone to see something 

more clearly or with greater magnification.</rdfs:comment></rdfs:Class><rdfs:Class rdf:ID="OrangeFruit"><rdfs:subClassOf rdf:resource="http://reliant.teknowledge.com/DAML/SUMO.owl#FruitOrVegetable" /><rdfs:subClassOf rdf:resource="http://reliant.teknowledge.com/DAML/SUMO.owl#Food" /><rdfs:comment>A citrus FruitOrVegetable that has an orange 

skin and a sweet, acidic flavor.</rdfs:comment></rdfs:Class><rdfs:Class rdf:ID="Orchestra"><rdfs:subClassOf rdf:resource="http://reliant.teknowledge.com/DAML/SUMO.owl#GroupOfPeople" /><rdfs:comment>A GroupOfPeople that create InstrumentalMusic 

together.  Note that this class covers marching bands, rock and jazz bands, 

as well as groups of people that play classical music together.</rdfs:comment></rdfs:Class><rdfs:Class rdf:ID="OrchestralConducting"><rdfs:subClassOf rdf:resource="http://reliant.teknowledge.com/DAML/SUMO.owl#Guiding" /><rdfs:comment>The Process of directing an orchestra.</rdfs:comment></rdfs:Class><rdfs:Class rdf:ID="Order"><rdfs:subClassOf rdf:resource="http://reliant.teknowledge.com/DAML/SUMO.owl#Sentence" /><rdfs:comment>A Sentence that expresses an order for something or 

that something be done.</rdfs:comment></rdfs:Class><rdfs:Class rdf:ID="OrganicCompound"><rdfs:subClassOf rdf:resource="http://reliant.teknowledge.com/DAML/SUMO.owl#CompoundSubstance" /><rdfs:comment>Any CompoundSubstance that has a Carbon 

base.</rdfs:comment></rdfs:Class><rdfs:Class rdf:ID="Organification"><rdfs:subClassOf rdf:resource="http://reliant.teknowledge.com/DAML/SUMO.owl#OrganOrTissueProcess" /><rdfs:comment>Any BiologicalProcess that results in 

the formation of an Organ.</rdfs:comment></rdfs:Class><rdfs:Class rdf:ID="OrganizationOfNations"><rdfs:subClassOf rdf:resource="#InternationalOrganization" /><rdfs:comment>InternationalOrganization is the 

class of Organizations whose members are Nations.</rdfs:comment></rdfs:Class><rdfs:Class rdf:ID="OrganizationalBoard"><rdfs:subClassOf rdf:resource="http://reliant.teknowledge.com/DAML/SUMO.owl#Organization" /><rdfs:comment>Part of an Organization that 

is responsible for managing the Organization.</rdfs:comment></rdfs:Class><rdfs:Class rdf:ID="OrganizationalMerging"><rdfs:subClassOf rdf:resource="http://reliant.teknowledge.com/DAML/SUMO.owl#OrganizationalProcess" /><rdfs:comment>The process of two or more 

Organizations merging into a single Organization.</rdfs:comment></rdfs:Class><rdfs:Class rdf:ID="Orthography"><rdfs:subClassOf rdf:resource="http://reliant.teknowledge.com/DAML/SUMO.owl#Procedure" /><rdfs:comment>A method for representing the sounds of a Language 

with written Characters.</rdfs:comment></rdfs:Class><rdfs:Class rdf:ID="Ossification"><rdfs:subClassOf rdf:resource="http://reliant.teknowledge.com/DAML/SUMO.owl#OrganOrTissueProcess" /><rdfs:comment>Any BiologicalProcess that results in the 

formation of Bones.</rdfs:comment></rdfs:Class><rdfs:Class rdf:ID="OutdoorClothing"><rdfs:subClassOf rdf:resource="http://reliant.teknowledge.com/DAML/SUMO.owl#Clothing" /><rdfs:comment>Clothing that is intended to be worn 

outdoors.</rdfs:comment></rdfs:Class><rdfs:Class rdf:ID="OuterSpaceRegion"><rdfs:subClassOf rdf:resource="#SpaceRegion" /><rdfs:comment>The class of all Regions which are 

neither GeographicAreas nor AtmosphericRegions.</rdfs:comment></rdfs:Class><rdfs:Class rdf:ID="Outside"><rdfs:subClassOf rdf:resource="http://reliant.teknowledge.com/DAML/SUMO.owl#Region" /><rdfs:comment>Any Region which is not enclosed by a Building 

or part of a Building.</rdfs:comment></rdfs:Class><rdfs:Class rdf:ID="Oval"><rdfs:subClassOf rdf:resource="http://reliant.teknowledge.com/DAML/SUMO.owl#ClosedTwoDimensionalFigure" /><rdfs:comment>The class of ClosedTwoDimensionalFigures that are 

produced by the intersection of a Cone with a ClosedTwoDimensionalFigure.</rdfs:comment></rdfs:Class><rdfs:Class rdf:ID="Oven"><rdfs:subClassOf rdf:resource="#HeatingDevice" /><rdfs:subClassOf rdf:resource="#Container" /><rdfs:comment>A HeatingDevice with a door for inserting and removing 

Food that is to be baked.</rdfs:comment></rdfs:Class><rdfs:Class rdf:ID="OverseasArea"><rdfs:subClassOf rdf:resource="#DependencyOrSpecialSovereigntyArea" /><rdfs:comment>OverseasArea is the class of 

GeopoliticalAreas that are related to a Nation as overseas 

territories, possessions, protectorates, or departments.</rdfs:comment></rdfs:Class><rdfs:Class rdf:ID="Owl"><rdfs:subClassOf rdf:resource="http://reliant.teknowledge.com/DAML/SUMO.owl#Bird" /><rdfs:comment>A nocturnal bird of prey with a large head and 

forward-facing eyes.</rdfs:comment></rdfs:Class><rdfs:Class rdf:ID="Oxidation"><rdfs:subClassOf rdf:resource="http://reliant.teknowledge.com/DAML/SUMO.owl#ChemicalDecomposition" /><rdfs:comment>Any ChemicalProcess where Electrons 

are removed from the substance undergoing the ChemicalProcess.</rdfs:comment></rdfs:Class><rdfs:Class rdf:ID="Oxygen"><rdfs:subClassOf rdf:resource="http://reliant.teknowledge.com/DAML/SUMO.owl#ElementalSubstance" /><atomicNumber>8</atomicNumber><rdfs:comment>A colourless, odourless gaseous element belonging to 

group 16 of the periodic table. It is the most abundant element present in 

the earth's crust. It also makes up 20.8 percent of the Earth's atmosphere.  

For industrial purposes, it is separated from liquid air by fractional 

distillation. It is used in high temperature welding, and in breathing. It 

commonly comes in the form of Oxygen, but is found as Ozone in the upper 

atmosphere. It was discovered by Priestley in 1774.</rdfs:comment></rdfs:Class><rdfs:Class rdf:ID="Page"><rdfs:subClassOf rdf:resource="http://reliant.teknowledge.com/DAML/SUMO.owl#Artifact" /><rdfs:comment>A single piece of Paper.</rdfs:comment></rdfs:Class><rdfs:Class rdf:ID="Paint"><rdfs:subClassOf rdf:resource="http://reliant.teknowledge.com/DAML/SUMO.owl#Solution" /><rdfs:comment>Any Solution which is capable of Coloring something.</rdfs:comment></rdfs:Class><rdfs:Class rdf:ID="PaintedPicture"><rdfs:subClassOf rdf:resource="http://reliant.teknowledge.com/DAML/SUMO.owl#ArtWork" /><rdfs:comment>Any ArtWork which is produced by Painting.</rdfs:comment></rdfs:Class><rdfs:Class rdf:ID="Painting"><rdfs:subClassOf rdf:resource="http://reliant.teknowledge.com/DAML/SUMO.owl#Covering" /><rdfs:subClassOf rdf:resource="http://reliant.teknowledge.com/DAML/SUMO.owl#Coloring" /><rdfs:comment>The application of Paint to a surface.  Note that 

this class covers both ArtPainting (the creation of PaintedPictures), as 

well as painting one's kitchen, for example.</rdfs:comment></rdfs:Class><rdfs:Class rdf:ID="Pancreas"><rdfs:subClassOf rdf:resource="#Gland" /><rdfs:comment>A large Gland that secretes Insulin and other 

substances.</rdfs:comment></rdfs:Class><rdfs:Class rdf:ID="Paper"><rdfs:subClassOf rdf:resource="http://reliant.teknowledge.com/DAML/SUMO.owl#Artifact" /><rdfs:comment>An Artifact made of cellulose pulp that is intended 

to contain a Text.</rdfs:comment></rdfs:Class><rdfs:Class rdf:ID="Paragraph"><rdfs:subClassOf rdf:resource="http://reliant.teknowledge.com/DAML/SUMO.owl#Text" /><rdfs:comment>A Text which consists of one or more sentences, 

begins with an indented line, and expresses a single topic.</rdfs:comment></rdfs:Class><rdfs:Class rdf:ID="Park"><rdfs:subClassOf rdf:resource="http://reliant.teknowledge.com/DAML/SUMO.owl#LandArea" /><rdfs:comment>A LandArea which is intended to be used for 

recreation and/or exercise.  Note that a Park can be either publicly 

or privately owned.</rdfs:comment></rdfs:Class><rdfs:Class rdf:ID="ParkingLot"><rdfs:subClassOf rdf:resource="http://reliant.teknowledge.com/DAML/SUMO.owl#StationaryArtifact" /><rdfs:comment>A LandArea which has been levelled, paved, and 

marked off for parking Automobiles.</rdfs:comment></rdfs:Class><rdfs:Class rdf:ID="Parliament"><rdfs:subClassOf rdf:resource="#LegislativeOrganization" /><rdfs:comment>Parliament is the subclass of 

LegislativeOrganizations similar to that of the United Kingdom.</rdfs:comment></rdfs:Class><rdfs:Class rdf:ID="PartTimePosition"><rdfs:subClassOf rdf:resource="http://reliant.teknowledge.com/DAML/SUMO.owl#Position" /><rdfs:comment>Any Position where the employee is not 

salaried and is paid for less than 40 hours of work per week.</rdfs:comment></rdfs:Class><rdfs:Class rdf:ID="Partnership"><rdfs:subClassOf rdf:resource="http://reliant.teknowledge.com/DAML/SUMO.owl#CommercialAgent" /><rdfs:comment>A CommercialAgent that is owned by more 

than one person.</rdfs:comment></rdfs:Class><rdfs:Class rdf:ID="PartyPlatform"><rdfs:subClassOf rdf:resource="http://reliant.teknowledge.com/DAML/SUMO.owl#FactualText" /><rdfs:comment>A Text which is authored by a PoliticalParty 

and which contains the core goals and principles of the PoliticalParty for a 

particular year or election cycle.</rdfs:comment></rdfs:Class><rdfs:Class rdf:ID="Pascal"><rdfs:subClassOf rdf:resource="http://reliant.teknowledge.com/DAML/SUMO.owl#FunctionQuantity" /><rdf:type rdf:resource="http://reliant.teknowledge.com/DAML/SUMO.owl#SystemeInternationalUnit" /><rdfs:comment>SI pressure measure.  Symbol:Pa. It is the 

pressure of one Newton per square Meter.  Pascal = N/m^2 

= m^(-1)*kg*s^(-2).</rdfs:comment></rdfs:Class><rdfs:Class rdf:ID="PassCertificate"><rdfs:subClassOf rdf:resource="http://reliant.teknowledge.com/DAML/SUMO.owl#Certificate" /><rdfs:comment>A Certificate that allows the holder to 

be at or away from a specified location, e.g. a pass for a leave of 

absence, a hall pass, a pass to enter a cleared facility, etc.</rdfs:comment></rdfs:Class><rdfs:Class rdf:ID="PassingABill"><rdfs:subClassOf rdf:resource="http://reliant.teknowledge.com/DAML/SUMO.owl#PoliticalProcess" /><rdfs:subClassOf rdf:resource="http://reliant.teknowledge.com/DAML/SUMO.owl#Declaring" /><rdfs:comment>The Process of converting a LegislativeBill 

into Law by a duly authorized legislative body of Government.</rdfs:comment></rdfs:Class><rdfs:Class rdf:ID="Passport"><rdfs:subClassOf rdf:resource="#License" /><rdfs:comment>A License which identifies the holder and permits 

travel between different countries.</rdfs:comment></rdfs:Class><rdfs:Class rdf:ID="PayCheck"><rdfs:subClassOf rdf:resource="#Check" /><rdfs:comment>A check issued to an employee in payment of salary or wages.</rdfs:comment></rdfs:Class><rdfs:Class rdf:ID="Payment"><rdfs:subClassOf rdf:resource="http://reliant.teknowledge.com/DAML/SUMO.owl#FinancialTransaction" /><rdfs:comment>The partial or complete discharge of an obligation by 

its settlement in the form of the transfer of funds, assets, or services equal 

to the monetary value of part or all of the debtor's obligation.</rdfs:comment></rdfs:Class><rdfs:Class rdf:ID="Pea"><rdfs:subClassOf rdf:resource="http://reliant.teknowledge.com/DAML/SUMO.owl#Seed" /><rdfs:subClassOf rdf:resource="http://reliant.teknowledge.com/DAML/SUMO.owl#Food" /><rdfs:comment>The edible Seed of a pea plant.</rdfs:comment></rdfs:Class><rdfs:Class rdf:ID="PearFruit"><rdfs:subClassOf rdf:resource="http://reliant.teknowledge.com/DAML/SUMO.owl#FruitOrVegetable" /><rdfs:subClassOf rdf:resource="http://reliant.teknowledge.com/DAML/SUMO.owl#Food" /><rdfs:comment>A FruitOrVegetable that has a thick skin and the 

shape of a tear drop.</rdfs:comment></rdfs:Class><rdfs:Class rdf:ID="Peeling"><rdfs:subClassOf rdf:resource="http://reliant.teknowledge.com/DAML/SUMO.owl#Removing" /><rdfs:comment>Removing the Skin (or part of the Skin) from 

an Organism.  Note that this class covers a large range of cases, including 

peeling an orange, pelting an Animal, etc.</rdfs:comment></rdfs:Class><rdfs:Class rdf:ID="Pencil"><rdfs:subClassOf rdf:resource="#WritingDevice" /><rdfs:comment>A WritingDevice that consists of an encased piece of 

graphite.</rdfs:comment></rdfs:Class><rdfs:Class rdf:ID="Peninsula"><rdfs:subClassOf rdf:resource="#LandForm" /><rdfs:comment>Peninsula is a subclass of LandForm consisting 

of pieces of land that extend into a BodyOfWater and are surrounded on 

three sides by water.  Typically Peninsulas are connected to the mainland 

by an Isthmus or neck of land that is narrower than the main portion of 

the peninsula (in contrast to Capes).</rdfs:comment></rdfs:Class><rdfs:Class rdf:ID="PensionPlan"><rdfs:subClassOf rdf:resource="#FinancialAccount" /><rdfs:comment>A qualified retirement plan set up by a 

corporation, labor union, government, or other organization for its 

employees.  Examples include profit-sharing plans, stock bonus and 

employee stock ownership plans, thrift plans, target benefit plans, 

money purchase plans, and defined benefit plans.</rdfs:comment></rdfs:Class><rdfs:Class rdf:ID="PercussionInstrument"><rdfs:subClassOf rdf:resource="http://reliant.teknowledge.com/DAML/SUMO.owl#MusicalInstrument" /><rdfs:comment>A MusicalInstrument which does not 

have strings and which is played by striking it.</rdfs:comment></rdfs:Class><rdfs:Class rdf:ID="Performance"><rdfs:subClassOf rdf:resource="http://reliant.teknowledge.com/DAML/SUMO.owl#Demonstrating" /><rdfs:comment>A Demonstrating which which is intended to entertain 

the audience, e.g. DramaticActing and/or Music.</rdfs:comment></rdfs:Class><rdfs:Class rdf:ID="PerformanceAct"><rdfs:subClassOf rdf:resource="#Performance" /><rdfs:comment>A discrete subProcess of a Performance, 

e.g. an act of a play, a movement of a performance of a symphony, etc.</rdfs:comment></rdfs:Class><rdfs:Class rdf:ID="PerformanceProgram"><rdfs:subClassOf rdf:resource="http://reliant.teknowledge.com/DAML/SUMO.owl#FactualText" /><rdfs:comment>A Text that describes the events 

and/or participants in a Performance.</rdfs:comment></rdfs:Class><rdfs:Class rdf:ID="PerformanceStage"><rdfs:subClassOf rdf:resource="http://reliant.teknowledge.com/DAML/SUMO.owl#StationaryArtifact" /><rdfs:comment>A large platform for theatrical plays, 

lectures, dances, music recitals, etc, which can be observed by an audience.</rdfs:comment></rdfs:Class><rdfs:Class rdf:ID="PerformanceStageWing"><rdfs:subClassOf rdf:resource="http://reliant.teknowledge.com/DAML/SUMO.owl#StationaryArtifact" /><rdfs:comment>A part of the PerformanceStage that is not 

visible to members of the audience.</rdfs:comment></rdfs:Class><rdfs:Class rdf:ID="PeriodicalPublisher"><rdfs:subClassOf rdf:resource="#Publisher" /><rdfs:comment>Any Publisher that publishes 

Periodicals, e.g. newspaper and magazine publishing houses.</rdfs:comment></rdfs:Class><rdfs:Class rdf:ID="Petroleum"><rdfs:subClassOf rdf:resource="#PetroleumProduct" /><rdfs:comment>Also known as crude oil.  It can be converted into 

RefinedPetroleumProducts.</rdfs:comment></rdfs:Class><rdfs:Class rdf:ID="PetroleumLubricant"><rdfs:subClassOf rdf:resource="#RefinedPetroleumProduct" /><rdfs:comment>PetroleumLubricant is the subclass of 

RefinedPetroleumProducts that are lubricants.</rdfs:comment></rdfs:Class><rdfs:Class rdf:ID="PetroleumProduct"><rdfs:subClassOf rdf:resource="#OrganicCompound" /><rdfs:comment>PetroleumProduct is a broad class that 

includes both crude oil (Petroleum) and RefinedPetroleumProducts.</rdfs:comment></rdfs:Class><rdfs:Class rdf:ID="Pharmacist"><rdfs:subClassOf rdf:resource="#Profession" /><rdfs:comment>The Profession of being a pharmacist, i.e. 

preparing and dispensing BiologicallyActiveSubstances.</rdfs:comment></rdfs:Class><rdfs:Class rdf:ID="Photograph"><rdfs:subClassOf rdf:resource="http://reliant.teknowledge.com/DAML/SUMO.owl#Icon" /><rdfs:comment>An Icon that is the result of a process of 

Photographing.</rdfs:comment></rdfs:Class><rdfs:Class rdf:ID="PhotographicFilm"><rdfs:subClassOf rdf:resource="http://reliant.teknowledge.com/DAML/SUMO.owl#Artifact" /><rdfs:comment>Celluloid covered with an emulsion which can 

be converted into photographic negatives by a Camera.</rdfs:comment></rdfs:Class><rdfs:Class rdf:ID="Photographing"><rdfs:subClassOf rdf:resource="http://reliant.teknowledge.com/DAML/SUMO.owl#ContentDevelopment" /><rdfs:comment>ContentDevelopment where the instrument 

is a camera and the result is a Photograph.</rdfs:comment></rdfs:Class><rdfs:Class rdf:ID="Piano"><rdfs:subClassOf rdf:resource="#StringInstrument" /><rdfs:comment>A StringInstrument which is played with keys that 

activate hammers that strike strings.</rdfs:comment></rdfs:Class><rdfs:Class rdf:ID="PictureFrame"><rdfs:subClassOf rdf:resource="http://reliant.teknowledge.com/DAML/SUMO.owl#Artifact" /><rdfs:comment>A frame which surrounds a PaintedPicture or 

Photograph and has the function of protecting and accenting the picture.</rdfs:comment></rdfs:Class><rdfs:Class rdf:ID="PidginLanguage"><rdfs:subClassOf rdf:resource="http://reliant.teknowledge.com/DAML/SUMO.owl#SpokenHumanLanguage" /><rdfs:comment>A PidginLanguage is not the native language 

of anyone but is used as an auxiliary or supplemental language between two 

mutually unintelligible speech communities. Pidgins are reduced languages, 

characterized by having a limited vocabulary and a simple grammar which serve 

to satisfy basic communication needs. Historically these languages have 

primarily arisen in trade centers and plantations (with slaves from different 

language backgrounds), areas where large groups of people lacking a common 

language need to communicate. By definition, a pidgin has no native speakers; 

it is always a person's second (or more) language.</rdfs:comment></rdfs:Class><rdfs:Class rdf:ID="Pig"><rdfs:subClassOf rdf:resource="http://reliant.teknowledge.com/DAML/SUMO.owl#HoofedMammal" /><rdfs:subClassOf rdf:resource="#DomesticAnimal" /><rdfs:comment>A domesticated HoofedMammal that is raised for pork.</rdfs:comment></rdfs:Class><rdfs:Class rdf:ID="Pigeon"><rdfs:subClassOf rdf:resource="http://reliant.teknowledge.com/DAML/SUMO.owl#Bird" /><rdfs:comment>A subclass of Bird with a stout body and short legs.</rdfs:comment></rdfs:Class><rdfs:Class rdf:ID="Pillow"><rdfs:subClassOf rdf:resource="http://reliant.teknowledge.com/DAML/SUMO.owl#Artifact" /><rdfs:comment>A soft, stuffed Artifact to support the Head or 

the body as a whole while one is sleeping or relaxing.</rdfs:comment></rdfs:Class><rdfs:Class rdf:ID="Pipeline"><rdfs:subClassOf rdf:resource="http://reliant.teknowledge.com/DAML/SUMO.owl#Transitway" /><rdfs:comment>Pipeline is the class of pipelines used 

to transport various kinds of fluids.</rdfs:comment></rdfs:Class><rdfs:Class rdf:ID="Pistol"><rdfs:subClassOf rdf:resource="#Firearm" /><rdfs:comment>A Firearm that is intended to be aimed and fired with a 

single hand.</rdfs:comment></rdfs:Class><rdfs:Class rdf:ID="PitchersMound"><rdfs:subClassOf rdf:resource="#GameArtifact" /><rdfs:comment>The place where the pitcher in Baseball 

stands when he is throwing balls to the batter.</rdfs:comment></rdfs:Class><rdfs:Class rdf:ID="Pitching"><rdfs:subClassOf rdf:resource="#Throwing" /><rdfs:comment>Throwing a Ball.</rdfs:comment></rdfs:Class><rdfs:Class rdf:ID="PituitaryGland"><rdfs:subClassOf rdf:resource="#Gland" /><rdfs:comment>The main Gland of the endocrine system.</rdfs:comment></rdfs:Class><rdfs:Class rdf:ID="PlaceOfCommerce"><rdfs:subClassOf rdf:resource="http://reliant.teknowledge.com/DAML/SUMO.owl#StationaryArtifact" /><rdfs:comment>A Building or part of a Building which is 

intended for organizational activities, e.g. retail or wholesale selling, 

manufacturing, office work, etc.</rdfs:comment></rdfs:Class><rdfs:Class rdf:ID="Planet"><rdfs:subClassOf rdf:resource="#NaturalSatellite" /><rdfs:comment>Planet is the class of large NaturalSatellites 

that revolve around a star.</rdfs:comment></rdfs:Class><rdfs:Class rdf:ID="PlaningHullWatercraft"><rdfs:subClassOf rdf:resource="#Watercraft" /><rdfs:comment>PlaningHullWatercraft is a subclass 

of Watercraft with hulls designed for a position partially on or above 

the water surface when they are in motion, in order to reduce drag.  See 

also DisplacementHullWatercraft.</rdfs:comment></rdfs:Class><rdfs:Class rdf:ID="PlantBranch"><rdfs:subClassOf rdf:resource="http://reliant.teknowledge.com/DAML/SUMO.owl#PlantAnatomicalStructure" /><rdfs:subClassOf rdf:resource="http://reliant.teknowledge.com/DAML/SUMO.owl#BodyPart" /><rdfs:comment>The stem of a Plant or any shoot arising from 

the stem of a Plant.</rdfs:comment></rdfs:Class><rdfs:Class rdf:ID="PlantLeaf"><rdfs:subClassOf rdf:resource="http://reliant.teknowledge.com/DAML/SUMO.owl#PlantAnatomicalStructure" /><rdfs:subClassOf rdf:resource="http://reliant.teknowledge.com/DAML/SUMO.owl#Organ" /><rdfs:comment>An Organ of Plants whose main purpose is 

photosynthesis.</rdfs:comment></rdfs:Class><rdfs:Class rdf:ID="PlantRoot"><rdfs:subClassOf rdf:resource="http://reliant.teknowledge.com/DAML/SUMO.owl#PlantAnatomicalStructure" /><rdfs:subClassOf rdf:resource="http://reliant.teknowledge.com/DAML/SUMO.owl#Organ" /><rdfs:comment>An Organ of Plants whose main purpose is 

twofold, viz. to absorb nutrients from the ground and to anchor the Plant 

in place.</rdfs:comment></rdfs:Class><rdfs:Class rdf:ID="Planting"><rdfs:subClassOf rdf:resource="http://reliant.teknowledge.com/DAML/SUMO.owl#Putting" /><rdfs:comment>Planting is the class of processes in 

which Plants are planted or transplanted, whether as seeds, seedlings, 

or mature plants.</rdfs:comment></rdfs:Class><rdfs:Class rdf:ID="Platinum"><rdfs:subClassOf rdf:resource="http://reliant.teknowledge.com/DAML/SUMO.owl#ElementalSubstance" /><atomicNumber>78</atomicNumber><rdfs:comment>Attractive greyish-white metal.  When pure, it is 

malleable and ductile.  Does not oxidize in air, insoluble in hydrochloric 

and nitric acid.  Corroded by halogens, cyandies, sulphur and alkalis.  

{Hydrogen} and {oxygen} react explosively in the presence of platinum.  

There are six stable isotopes and three radioisotopes, the most stable 

being Pt-193 with a half-life of 60 years.  Platinum is used in jewelry, 

laboratory equipment, electrical contacts, dentistry, and anti-pollution 

devices in cars.  PtCl2(NH3)2 is used to treat some forms of cancer.  

Platinum-{cobalt} alloys have magnetic properties.  It is also used in the 

definition of the Standard Hydrogen Electrode.  Discovered by Antonio de 

Ulloa in South America in 1735.  The name comes from the Spanish word 

platina which means silver.  Platinum metal is generally not a health 

concern due to its unreactivity, however platinum compounds should be 

considered highly toxic.</rdfs:comment></rdfs:Class><rdfs:Class rdf:ID="PlayingCard"><rdfs:subClassOf rdf:resource="#GameArtifact" /><rdfs:subClassOf rdf:resource="http://reliant.teknowledge.com/DAML/SUMO.owl#ContentBearingObject" /><rdfs:comment>A small piece of stiff paper with markings 

which is intended to be used for playing card games.</rdfs:comment></rdfs:Class><rdfs:Class rdf:ID="Pleading"><rdfs:subClassOf rdf:resource="http://reliant.teknowledge.com/DAML/SUMO.owl#Stating" /><rdfs:comment>Stating in a court of law a claim about whether or 

not one is guilty of the crime of which one has been accused.</rdfs:comment></rdfs:Class><rdfs:Class rdf:ID="Plug"><rdfs:subClassOf rdf:resource="http://reliant.teknowledge.com/DAML/SUMO.owl#Artifact" /><rdfs:comment>An Artifact which is designed to fit snugly within 

a Hole.</rdfs:comment></rdfs:Class><rdfs:Class rdf:ID="Plumber"><rdfs:subClassOf rdf:resource="#OccupationalTrade" /><rdfs:comment>Any occupation that involves installing, repairing, and 

replacing pipes and pipe fixtures.</rdfs:comment></rdfs:Class><rdfs:Class rdf:ID="Pocket"><rdfs:subClassOf rdf:resource="#FabricArtifact" /><rdfs:comment>A pouch of Fabric in an instance of Clothing where 

something can be kept.</rdfs:comment></rdfs:Class><rdfs:Class rdf:ID="Poisoning"><rdfs:subClassOf rdf:resource="http://reliant.teknowledge.com/DAML/SUMO.owl#Injuring" /><rdfs:comment>A Poisoning is caused by an external 

substance.  Since Poisoning is not possible without some biologic 

function which affects the Organism being injured, it is a subclass 

of BiologicalProcess.</rdfs:comment></rdfs:Class><rdfs:Class rdf:ID="PolarClimateZone"><rdfs:subClassOf rdf:resource="#ClimateZone" /><rdfs:comment>PolarClimateZone is a subclass of 

ClimateZone characterized by having an average temperature less than 

10 degrees Celsius in the warmest month.  This is Koeppen climate system 

Type E.  No agriculture is supported in polar climates.</rdfs:comment></rdfs:Class><rdfs:Class rdf:ID="PolarTypeFClimateZone"><rdfs:subClassOf rdf:resource="#PolarClimateZone" /><rdfs:comment>PolarTypeFClimateZone is a 

subclass of PolarClimateZone characterized by having no month in 

which the temperature rises to 10 degrees Celsius or above.</rdfs:comment></rdfs:Class><rdfs:Class rdf:ID="PoliceCaptain"><rdfs:subClassOf rdf:resource="#PoliceOfficer" /><rdfs:comment>A PoliceOfficer who is in charge of a precinct.</rdfs:comment></rdfs:Class><rdfs:Class rdf:ID="PoliceDetective"><rdfs:subClassOf rdf:resource="#PoliceOfficer" /><rdfs:comment>The Profession of being a police 

detective, i.e. being a PoliceOfficer whose duties include the 

investigation of crimes.</rdfs:comment></rdfs:Class><rdfs:Class rdf:ID="PoliceOfficer"><rdfs:subClassOf rdf:resource="#GovernmentOfficer" /><rdfs:comment>The Profession of being a police officer, i.e. 

working for a law enforcement agency that is part of a Government.</rdfs:comment></rdfs:Class><rdfs:Class rdf:ID="PoliceSergeant"><rdfs:subClassOf rdf:resource="#PoliceOfficer" /><rdfs:comment>A PoliceOfficer with the rank of sergeant.</rdfs:comment></rdfs:Class><rdfs:Class rdf:ID="PoliticalCrime"><rdfs:subClassOf rdf:resource="#CriminalAction" /><rdfs:subClassOf rdf:resource="http://reliant.teknowledge.com/DAML/SUMO.owl#PoliticalProcess" /><rdfs:comment>A CriminalAction that is committed by or 

against Governments.</rdfs:comment></rdfs:Class><rdfs:Class rdf:ID="PoliticalParty"><rdfs:subClassOf rdf:resource="http://reliant.teknowledge.com/DAML/SUMO.owl#PoliticalOrganization" /><rdfs:comment>PoliticalParty is the class of 

PoliticalOrganizations that may sponsor candidates for Elections.</rdfs:comment></rdfs:Class><rdfs:Class rdf:ID="PoliticalRevolution"><rdfs:subClassOf rdf:resource="http://reliant.teknowledge.com/DAML/SUMO.owl#PoliticalProcess" /><rdfs:subClassOf rdf:resource="http://reliant.teknowledge.com/DAML/SUMO.owl#ViolentContest" /><rdfs:comment>The violent overthrow of one Government 

and its replacement by another.  This covers grass-roots revolutions, as well 

as coups d'etat.</rdfs:comment></rdfs:Class><rdfs:Class rdf:ID="PoliticoEconomicAttribute"><rdfs:subClassOf rdf:resource="http://reliant.teknowledge.com/DAML/SUMO.owl#RelationalAttribute" /><rdfs:comment>Any Attribute of a Government 

which specifies some aspect of the political or economic system of the 

Government.</rdfs:comment></rdfs:Class><rdfs:Class rdf:ID="Polling"><rdfs:subClassOf rdf:resource="http://reliant.teknowledge.com/DAML/SUMO.owl#Investigating" /><rdfs:comment>Investigating what people believe (and in what proportions) 

by asking a set of structured questions to a random sample of people.</rdfs:comment></rdfs:Class><rdfs:Class rdf:ID="Polygon"><rdfs:subClassOf rdf:resource="http://reliant.teknowledge.com/DAML/SUMO.owl#ClosedTwoDimensionalFigure" /><rdfs:comment>A ClosedTwoDimensionalFigure that is composed 

exclusively of straight lines, i.e. OneDimensionalFigures.</rdfs:comment></rdfs:Class><rdfs:Class rdf:ID="PolyphonicMusic"><rdfs:subClassOf rdf:resource="http://reliant.teknowledge.com/DAML/SUMO.owl#Music" /><rdfs:comment>Music which has two or more parts, i.e. Music 

which can be divided into two or more contemporaneous subProcesses which are 

also instances of Music.</rdfs:comment></rdfs:Class><rdfs:Class rdf:ID="PopularElection"><rdfs:subClassOf rdf:resource="#GeneralElection" /><rdfs:comment>PopularElection is the class of 

Elections in which office-holders and issues are determined directly by 

the outcome of the votes cast by the enfranchised.  For example, U.S.  

Senators and Representatives are elected by PopularElection.  By 

contrast, U.S. Presidents are elected by indirect elections, in which the 

Electoral College determines the actual outcome.  See electionWinner.</rdfs:comment></rdfs:Class><rdfs:Class rdf:ID="Porch"><rdfs:subClassOf rdf:resource="http://reliant.teknowledge.com/DAML/SUMO.owl#StationaryArtifact" /><rdfs:comment>A StationaryArtifact which is connected to a 

Building and which provides some shelter in entering or leaving the 

Building or in sitting outside.</rdfs:comment></rdfs:Class><rdfs:Class rdf:ID="Pork"><rdfs:subClassOf rdf:resource="http://reliant.teknowledge.com/DAML/SUMO.owl#Meat" /><rdfs:comment>Meat that was originally part of a Pig.</rdfs:comment></rdfs:Class><rdfs:Class rdf:ID="PortFacility"><rdfs:subClassOf rdf:resource="http://reliant.teknowledge.com/DAML/SUMO.owl#GeopoliticalArea" /><rdfs:comment>PortFacility is the class of port 

complexes, including piers and docking space, moorings, cargo-handling 

and other support facilities for marine traffic.  Ships are loaded and 

unloaded at a PortFacility.</rdfs:comment></rdfs:Class><rdfs:Class rdf:ID="Portrait"><rdfs:subClassOf rdf:resource="#PaintedPicture" /><rdfs:comment>A PaintedPicture that represents someone's Face.</rdfs:comment></rdfs:Class><rdfs:Class rdf:ID="PostMeridiem"><rdfs:subClassOf rdf:resource="http://reliant.teknowledge.com/DAML/SUMO.owl#TimeInterval" /><rdfs:comment>The class of TimeIntervals that begin at noon and 

end at midnight.</rdfs:comment></rdfs:Class><rdfs:Class rdf:ID="PostSecondarySchool"><rdfs:subClassOf rdf:resource="#School" /><rdfs:comment>The class of Schools that offer 

an associate's degree, a bachelor's degree or a graduate degree.</rdfs:comment></rdfs:Class><rdfs:Class rdf:ID="PotOrPan"><rdfs:subClassOf rdf:resource="#Container" /><rdfs:comment>A Container which has a handle and is used for 

Cooking.</rdfs:comment></rdfs:Class><rdfs:Class rdf:ID="Potassium"><rdfs:subClassOf rdf:resource="http://reliant.teknowledge.com/DAML/SUMO.owl#ElementalSubstance" /><atomicNumber>19</atomicNumber><rdfs:comment>Soft silvery metallic element belonging to group 

1 of the periodic table (alkali metals).  Occurs naturally in seawater and 

a many minerals.  Highly reactive, chemically, it resembles sodium in its 

behavior and compounds.  Discovered by Sir Humphry Davy in 1807.</rdfs:comment></rdfs:Class><rdfs:Class rdf:ID="Potter"><rdfs:subClassOf rdf:resource="#OccupationalTrade" /><rdfs:comment>Any occupation that involves the creation of Pottery.</rdfs:comment></rdfs:Class><rdfs:Class rdf:ID="Pottery"><rdfs:subClassOf rdf:resource="http://reliant.teknowledge.com/DAML/SUMO.owl#Artifact" /><rdfs:comment>Household Artifacts that are made out of baked Clay.</rdfs:comment></rdfs:Class><rdfs:Class rdf:ID="PoundForce"><rdfs:subClassOf rdf:resource="http://reliant.teknowledge.com/DAML/SUMO.owl#FunctionQuantity" /><rdf:type rdf:resource="http://reliant.teknowledge.com/DAML/SUMO.owl#UnitOfMeasure" /><rdfs:comment>English pound of force. The conversion

factor depends on the local value of the acceleration of free fall. A

mean value is used in the conversion axiom associated with this 

constant.</rdfs:comment></rdfs:Class><rdfs:Class rdf:ID="Pouring"><rdfs:subClassOf rdf:resource="http://reliant.teknowledge.com/DAML/SUMO.owl#LiquidMotion" /><rdfs:subClassOf rdf:resource="http://reliant.teknowledge.com/DAML/SUMO.owl#Transfer" /><rdfs:comment>Any instance of Transfer from one Container to 

another, where the thing transferred is a Liquid.</rdfs:comment></rdfs:Class><rdfs:Class rdf:ID="Powder"><rdfs:subClassOf rdf:resource="http://reliant.teknowledge.com/DAML/SUMO.owl#Substance" /><rdfs:comment>Any Solid Substance which consists of loose, 

identical, and very small particles.</rdfs:comment></rdfs:Class><rdfs:Class rdf:ID="Praying"><rdfs:subClassOf rdf:resource="http://reliant.teknowledge.com/DAML/SUMO.owl#ReligiousProcess" /><rdfs:subClassOf rdf:resource="http://reliant.teknowledge.com/DAML/SUMO.owl#Requesting" /><rdfs:comment>A formal or informal process of private worship which 

may or may not be carried out in a ReligiousBuilding.</rdfs:comment></rdfs:Class><rdfs:Class rdf:ID="PreparedFood"><rdfs:subClassOf rdf:resource="http://reliant.teknowledge.com/DAML/SUMO.owl#Food" /><rdfs:comment>Food that is the result of Cooking.</rdfs:comment></rdfs:Class><rdfs:Class rdf:ID="PressureMeasuringDevice"><rdfs:subClassOf rdf:resource="http://reliant.teknowledge.com/DAML/SUMO.owl#MeasuringDevice" /><rdfs:comment>Any Device that measures and 

represents AtmosphericPressureMeasure.</rdfs:comment></rdfs:Class><rdfs:Class rdf:ID="Prison"><rdfs:subClassOf rdf:resource="http://reliant.teknowledge.com/DAML/SUMO.owl#StationaryArtifact" /><rdfs:comment>An installation which is owned and maintained by 

a Government for the purpose of Confining people.  This class covers 

jails, federal prisons, concentration camps, gulags, etc.</rdfs:comment></rdfs:Class><rdfs:Class rdf:ID="PrivateDetective"><rdfs:subClassOf rdf:resource="#Profession" /><sumo:disjoint rdf:resource="#PoliceDetective" /><rdfs:comment>The Profession of being a private detective, 

i.e. a detective who can be hired for a fee to investigate something.</rdfs:comment></rdfs:Class><rdfs:Class rdf:ID="PrivateSchool"><rdfs:subClassOf rdf:resource="#School" /><sumo:disjoint rdf:resource="http://reliant.teknowledge.com/DAML/SUMO.owl#GovernmentOrganization" /><rdfs:comment>A School which is not publicly owned.</rdfs:comment></rdfs:Class><rdfs:Class rdf:ID="ProcessingACheck"><rdfs:subClassOf rdf:resource="#AuthorizationOfTransaction" /><rdfs:comment>An activity of paying the amount specified on the 

check from funds on deposit.</rdfs:comment></rdfs:Class><rdfs:Class rdf:ID="Proclaiming"><rdfs:subClassOf rdf:resource="#Lecture" /><rdfs:subClassOf rdf:resource="http://reliant.teknowledge.com/DAML/SUMO.owl#Declaring" /><rdfs:comment>Any instance of Speaking before an assembled 

audience that effects an institutional change, e.g. a change in the laws of 

the government.</rdfs:comment></rdfs:Class><rdfs:Class rdf:ID="Profession"><rdfs:subClassOf rdf:resource="#SkilledOccupation" /><sumo:disjoint rdf:resource="#OccupationalTrade" /><rdfs:comment>Any occupation that requires at least a bachelor's

degree.</rdfs:comment></rdfs:Class><rdfs:Class rdf:ID="Professor"><rdfs:subClassOf rdf:resource="#Teacher" /><rdfs:comment>The Profession of being a teacher at a 

PostSecondarySchool.</rdfs:comment></rdfs:Class><rdfs:Class rdf:ID="ProfitSharingPlan"><rdfs:subClassOf rdf:resource="#PensionPlan" /><rdfs:comment>An arrangement in which an employer 

shares its profits with its employees.  The compensation can be stocks, 

bonds or cash, and can be immediate or deferred until retirement.</rdfs:comment></rdfs:Class><rdfs:Class rdf:ID="Projectile"><rdfs:subClassOf rdf:resource="http://reliant.teknowledge.com/DAML/SUMO.owl#Weapon" /><rdfs:comment>A missile, bullet, etc. that is fired from 

a Weapon.</rdfs:comment></rdfs:Class><rdfs:Class rdf:ID="ProjectileLauncher"><rdfs:subClassOf rdf:resource="http://reliant.teknowledge.com/DAML/SUMO.owl#Weapon" /><rdfs:comment>A Weapon that shoots a Projectile.</rdfs:comment></rdfs:Class><rdfs:Class rdf:ID="ProjectileShell"><rdfs:subClassOf rdf:resource="#Container" /><rdfs:comment>The case or cartridge of a Projectile.</rdfs:comment></rdfs:Class><rdfs:Class rdf:ID="ProjectionScreen"><rdfs:subClassOf rdf:resource="#CommunicationDevice" /><rdfs:comment>A CommunicationDevice upon which images 

are projected so that they can be viewed.</rdfs:comment></rdfs:Class><rdfs:Class rdf:ID="Proprietorship"><rdfs:subClassOf rdf:resource="http://reliant.teknowledge.com/DAML/SUMO.owl#CommercialAgent" /><rdfs:comment>A CommercialAgent that is owned by a 

single person.</rdfs:comment></rdfs:Class><rdfs:Class rdf:ID="Protozoa"><rdfs:subClassOf rdf:resource="http://reliant.teknowledge.com/DAML/SUMO.owl#Microorganism" /><rdfs:comment>Unicellular Organisms that are capable of movement 

and that are found in almost every part of the world.  This class includes 

amoebas, sporozoans, and paramecia.</rdfs:comment></rdfs:Class><rdfs:Class rdf:ID="PseudoGraph"><rdfs:subClassOf rdf:resource="#Graph" /><rdfs:comment>The Class of pseudographs.  A pseudograph 

is a Graph containing at least one GraphLoop.</rdfs:comment></rdfs:Class><rdfs:Class rdf:ID="Psychosis"><rdfs:subClassOf rdf:resource="http://reliant.teknowledge.com/DAML/SUMO.owl#PsychologicalDysfunction" /><rdfs:comment>Any PsychologicalDysfunction which is the 

result of an organic impairment of the NervousSystem.</rdfs:comment></rdfs:Class><rdfs:Class rdf:ID="PublicDefender"><rdfs:subClassOf rdf:resource="#Attorney" /><rdfs:subClassOf rdf:resource="#GovernmentOfficer" /><rdfs:comment>An Attorney who defends criminal cases for a 

GovernmentOrganization.</rdfs:comment></rdfs:Class><rdfs:Class rdf:ID="PublicLibrary"><rdfs:subClassOf rdf:resource="#Library" /><rdfs:subClassOf rdf:resource="http://reliant.teknowledge.com/DAML/SUMO.owl#GovernmentOrganization" /><rdfs:comment>A Library which is financed by taxes and which 

is open to everyone.</rdfs:comment></rdfs:Class><rdfs:Class rdf:ID="PublicPark"><rdfs:subClassOf rdf:resource="#Park" /><rdfs:comment>A Park that is publicly owned, i.e. owned 

by a Government.</rdfs:comment></rdfs:Class><rdfs:Class rdf:ID="PublicProsecutor"><rdfs:subClassOf rdf:resource="#Attorney" /><rdfs:subClassOf rdf:resource="#GovernmentOfficer" /><rdfs:comment>An Attorney who prosecutes criminal cases for 

a GovernmentOrganization.</rdfs:comment></rdfs:Class><rdfs:Class rdf:ID="PublicSchool"><rdfs:subClassOf rdf:resource="#School" /><rdfs:subClassOf rdf:resource="http://reliant.teknowledge.com/DAML/SUMO.owl#GovernmentOrganization" /><rdfs:comment>A School which is financed primarily by taxes.</rdfs:comment></rdfs:Class><rdfs:Class rdf:ID="Publisher"><rdfs:subClassOf rdf:resource="http://reliant.teknowledge.com/DAML/SUMO.owl#CommercialAgent" /><rdfs:comment>Any business whose services include the 

Publication of Texts.</rdfs:comment></rdfs:Class><rdfs:Class rdf:ID="Pulling"><rdfs:subClassOf rdf:resource="#LandTransportation" /><rdfs:comment>Any instance of LandTransportation, where a 

TransportationDevice is dragged by something else, whether the something 

else is an Animal or a self-powered TransportationDevice.</rdfs:comment></rdfs:Class><rdfs:Class rdf:ID="PulmonaryArtery"><rdfs:subClassOf rdf:resource="#Artery" /><rdfs:comment>An Artery that carries Blood from 

the Heart to the Lungs.</rdfs:comment></rdfs:Class><rdfs:Class rdf:ID="PulmonaryVein"><rdfs:subClassOf rdf:resource="#Vein" /><rdfs:comment>A Vein that carries Blood from the 

Lungs to the Heart.</rdfs:comment></rdfs:Class><rdfs:Class rdf:ID="Pump"><rdfs:subClassOf rdf:resource="http://reliant.teknowledge.com/DAML/SUMO.owl#TransportationDevice" /><rdfs:comment>A Device that moves Fluids by means of pressure or suction.</rdfs:comment></rdfs:Class><rdfs:Class rdf:ID="Punching"><rdfs:subClassOf rdf:resource="http://reliant.teknowledge.com/DAML/SUMO.owl#Impelling" /><rdfs:comment>Any instance of Impelling where the instrument 

is a Fist of the agent.</rdfs:comment></rdfs:Class><rdfs:Class rdf:ID="Punishing"><rdfs:subClassOf rdf:resource="http://reliant.teknowledge.com/DAML/SUMO.owl#RegulatoryProcess" /><rdfs:comment>A RegulatoryProcess where the agent does 

something to the destination that the agent knows is undesirable 

for the destination.</rdfs:comment></rdfs:Class><rdfs:Class rdf:ID="PuttingOnClothing"><rdfs:subClassOf rdf:resource="http://reliant.teknowledge.com/DAML/SUMO.owl#Covering" /><rdfs:comment>Putting Clothing on a Human or 

Animal in such a way that the Human or Animal wears the Clothing.</rdfs:comment></rdfs:Class><rdfs:Class rdf:ID="Quadrilateral"><rdfs:subClassOf rdf:resource="#Polygon" /><rdfs:comment>Any four-sided Polygon.</rdfs:comment></rdfs:Class><rdfs:Class rdf:ID="QueenInsect"><rdfs:subClassOf rdf:resource="http://reliant.teknowledge.com/DAML/SUMO.owl#Insect" /><sumo:disjoint rdf:resource="#WorkerInsect" /><rdfs:comment>A Female Insect which is the sole member of 

her colony with the capability to reproduce.</rdfs:comment></rdfs:Class><rdfs:Class rdf:ID="Question"><rdfs:subClassOf rdf:resource="http://reliant.teknowledge.com/DAML/SUMO.owl#Sentence" /><rdfs:comment>An interrogative Sentence, a Sentence that 

poses a question.</rdfs:comment></rdfs:Class><rdfs:Class rdf:ID="Rabbit"><rdfs:subClassOf rdf:resource="http://reliant.teknowledge.com/DAML/SUMO.owl#Rodent" /><rdfs:comment>A burrowing Rodent with a short tail and long ears.</rdfs:comment></rdfs:Class><rdfs:Class rdf:ID="RacialEthnicGroup"><rdfs:subClassOf rdf:resource="http://reliant.teknowledge.com/DAML/SUMO.owl#EthnicGroup" /><rdfs:comment>A RacialEthnicGroup is an 

EthnicGroup based on common racial background.</rdfs:comment></rdfs:Class><rdfs:Class rdf:ID="Racing"><rdfs:subClassOf rdf:resource="http://reliant.teknowledge.com/DAML/SUMO.owl#Sport" /><rdfs:comment>A sport which involves a contest of speed between the 

participants.  Note that this covers a variety of things, including auto 

racing, running competitions, etc.</rdfs:comment></rdfs:Class><rdfs:Class rdf:ID="RadarOrSonar"><rdfs:subClassOf rdf:resource="#ElectricDevice" /><rdfs:comment>An ElectricDevice that emits and receives 

microwave radiation for the purpose of locating and tracking distant objects.</rdfs:comment></rdfs:Class><rdfs:Class rdf:ID="RadiatingInfrared"><rdfs:subClassOf rdf:resource="http://reliant.teknowledge.com/DAML/SUMO.owl#Radiating" /><sumo:disjoint rdf:resource="http://reliant.teknowledge.com/DAML/SUMO.owl#RadiatingLight" /><sumo:disjoint rdf:resource="#RadioEmission" /><rdfs:comment>Any instance of Radiating where the 

wavelengths are longer than those of visible light and shorter than those 

of radio emissions.</rdfs:comment></rdfs:Class><rdfs:Class rdf:ID="RadiatingSoundUltrasonic"><rdfs:subClassOf rdf:resource="http://reliant.teknowledge.com/DAML/SUMO.owl#RadiatingSound" /><rdfs:comment>All sound waves that have frequencies 

above those that normal Human ears can detect.</rdfs:comment></rdfs:Class><rdfs:Class rdf:ID="RadiatingUltraviolet"><rdfs:subClassOf rdf:resource="http://reliant.teknowledge.com/DAML/SUMO.owl#Radiating" /><sumo:disjoint rdf:resource="http://reliant.teknowledge.com/DAML/SUMO.owl#RadiatingLight" /><sumo:disjoint rdf:resource="#XRayRadiation" /><rdfs:comment>Any instance of Radiating where the 

wavelengths are shorter than those of visible light and longer than those 

of X-Rays.</rdfs:comment></rdfs:Class><rdfs:Class rdf:ID="RadiatingVisibleLight"><rdfs:subClassOf rdf:resource="http://reliant.teknowledge.com/DAML/SUMO.owl#RadiatingLight" /><sumo:disjoint rdf:resource="#RadiatingUltraviolet" /><rdfs:comment>Any instance of RadiatingLight that can 

be detected by normal human visual perception.</rdfs:comment></rdfs:Class><rdfs:Class rdf:ID="RadioBroadcasting"><rdfs:subClassOf rdf:resource="#Broadcasting" /><rdfs:comment>Any instance of Broadcasting which is 

intended to be received by a Radio.</rdfs:comment></rdfs:Class><rdfs:Class rdf:ID="RadioEmission"><rdfs:subClassOf rdf:resource="http://reliant.teknowledge.com/DAML/SUMO.owl#Radiating" /><rdfs:comment>Any instance of Radiating 

where the waves have a wavelength between 5 milimeters and 30,000 meters.</rdfs:comment></rdfs:Class><rdfs:Class rdf:ID="RadioReceiver"><rdfs:subClassOf rdf:resource="#ReceiverDevice" /><rdfs:comment>A RadioReceiver is a Device for receiving 

radio broadcast signals from a RadioStation.</rdfs:comment></rdfs:Class><rdfs:Class rdf:ID="RadioStation"><rdfs:subClassOf rdf:resource="#BroadcastingStation" /><rdfs:comment>A RadioStation is a BroadcastingStation 

that broadcasts programs that are intended to be received by Radios.</rdfs:comment></rdfs:Class><rdfs:Class rdf:ID="RadioactiveWeapon"><rdfs:subClassOf rdf:resource="#WeaponOfMassDestruction" /><sumo:disjoint rdf:resource="#BiochemicalWeapon" /><rdfs:comment>A WeaponOfMassDestruction which 

achieves its effect through radioactivity, either by an explosion resulting 

from nuclear fission or by a conventional explosive device that scatters 

radioactive debris.</rdfs:comment></rdfs:Class><rdfs:Class rdf:ID="RadiologicalWeapon"><rdfs:comment>Weapons which are designed to spread 

radioactive particles over a large area by means of a conventional 

explosive device rather than a nuclear reaction.  These weapons are often 

referred to as 'dirty bombs'.</rdfs:comment><rdfs:subClassOf rdf:resource="#RadioactiveWeapon" /></rdfs:Class><rdfs:Class rdf:ID="Radish"><rdfs:subClassOf rdf:resource="#PlantRoot" /><rdfs:subClassOf rdf:resource="http://reliant.teknowledge.com/DAML/SUMO.owl#Food" /><rdfs:comment>A PlantRoot that is often used in salads.</rdfs:comment></rdfs:Class><rdfs:Class rdf:ID="RailTransportationSystem"><rdfs:subClassOf rdf:resource="#TransportationSystem" /><rdfs:comment>RailTransportationSystem 

is the subclass of TransportationSystems whose routes are Railways.</rdfs:comment></rdfs:Class><rdfs:Class rdf:ID="Railcar"><rdfs:subClassOf rdf:resource="#RollingStock" /><sumo:disjoint rdf:resource="#SelfPoweredVehicle" /><rdfs:comment>Railcar is the subclass of RollingStock that 

includes all non-locomotive, non-self-powered RailwayVehicles.</rdfs:comment></rdfs:Class><rdfs:Class rdf:ID="RailroadCompany"><rdfs:subClassOf rdf:resource="#TransportationCompany" /><rdfs:comment>Any TransportationCompany whose services 

include Transportation by Train.</rdfs:comment></rdfs:Class><rdfs:Class rdf:ID="RailroadTrack"><rdfs:subClassOf rdf:resource="http://reliant.teknowledge.com/DAML/SUMO.owl#StationaryArtifact" /><rdfs:comment>RailroadTrack is the class of 

StationaryArtifacts consisting of rails laid on supports to form 

a track for railway vehicles.</rdfs:comment></rdfs:Class><rdfs:Class rdf:ID="Railway"><rdfs:subClassOf rdf:resource="http://reliant.teknowledge.com/DAML/SUMO.owl#LandTransitway" /><rdfs:subClassOf rdf:resource="http://reliant.teknowledge.com/DAML/SUMO.owl#StationaryArtifact" /><rdfs:comment>Railway is the subclass of 

LandTransitways that have rails along which Trains may travel.  

A railway consists of the rail bed, sleepers, tracks, electric 

rails, switches, sensors, lights, crossing grades, and any other 

integral machinery or parts of a section of railway.</rdfs:comment></rdfs:Class><rdfs:Class rdf:ID="RailwayTerminal"><rdfs:subClassOf rdf:resource="#TransitTerminal" /><rdfs:comment>RailwayTerminal is the subclass of 

TransitTerminals designed for Trains.  A RailwayTerminal includes 

all the RailroadTrack and any outbuildings or other related structure 

in the terminal, as well as the TrainStation (if there is one).</rdfs:comment></rdfs:Class><rdfs:Class rdf:ID="RailwayVehicle"><rdfs:subClassOf rdf:resource="#LandVehicle" /><rdfs:comment>RailwayVehicle is the subclass of 

Vehicles that are designed to run on Railways, including both Trains 

and individual cars (RollingStock).</rdfs:comment></rdfs:Class><rdfs:Class rdf:ID="Raining"><rdfs:subClassOf rdf:resource="http://reliant.teknowledge.com/DAML/SUMO.owl#Precipitation" /><rdfs:comment>Raining is a precipitation process 

in which water falls in a Liquid state.</rdfs:comment></rdfs:Class><rdfs:Class rdf:ID="Ramp"><rdfs:subClassOf rdf:resource="http://reliant.teknowledge.com/DAML/SUMO.owl#Object" /><rdfs:comment>Ramp is the class of Objects that are 

inclined planes used for moving objects from one level to another, 

especially used for wheeled vehicles and people who cannot climb stairs.</rdfs:comment></rdfs:Class><rdfs:Class rdf:ID="Raping"><rdfs:subClassOf rdf:resource="#Mating" /><rdfs:subClassOf rdf:resource="#CriminalAction" /><rdfs:comment>Any instance of Mating where one participant does not 

consent.</rdfs:comment></rdfs:Class><rdfs:Class rdf:ID="Rat"><rdfs:subClassOf rdf:resource="http://reliant.teknowledge.com/DAML/SUMO.owl#Rodent" /><rdfs:comment>A Rodent that has a hairless tail like a Mouse 

but that is larger than a Mouse.</rdfs:comment></rdfs:Class><rdfs:Class rdf:ID="Rattlesnake"><rdfs:subClassOf rdf:resource="#Snake" /><rdfs:comment>A subclass of Snake which derives its name 

from the fact that it can manipulate its tail in such a way as to produce 

a sound like that of a rattle.</rdfs:comment></rdfs:Class><rdfs:Class rdf:ID="RawFood"><rdfs:subClassOf rdf:resource="http://reliant.teknowledge.com/DAML/SUMO.owl#Food" /><rdfs:comment>Food that is not the result of Cooking.</rdfs:comment></rdfs:Class><rdfs:Class rdf:ID="RealEstate"><rdfs:subClassOf rdf:resource="http://reliant.teknowledge.com/DAML/SUMO.owl#CorpuscularObject" /><rdfs:comment>Land, including all the natural resources and permanent buildings on it.</rdfs:comment></rdfs:Class><rdfs:Class rdf:ID="RearWindow"><rdfs:subClassOf rdf:resource="#VehicleWindow" /><rdfs:comment>Any VehicleWindow which is located at the back 

of an Automobile.</rdfs:comment></rdfs:Class><rdfs:Class rdf:ID="ReceiverDevice"><rdfs:subClassOf rdf:resource="#CommunicationDevice" /><rdfs:subClassOf rdf:resource="#ElectricDevice" /><rdfs:comment>An ElectricDevice that is capable of 

receiving and decoding RadioEmissions, e.g. Radios and Televisions.</rdfs:comment></rdfs:Class><rdfs:Class rdf:ID="Reciting"><rdfs:subClassOf rdf:resource="http://reliant.teknowledge.com/DAML/SUMO.owl#Speaking" /><rdfs:comment>Any instance of Speaking where what is 

uttered is contained within a Text.</rdfs:comment></rdfs:Class><rdfs:Class rdf:ID="RecordAlbum"><rdfs:subClassOf rdf:resource="#AudioRecording" /><rdfs:comment>A AudioRecording that has the form of a 

plastic or glass disk with continuous grooves that are transformed into 

sound by a record player.</rdfs:comment></rdfs:Class><rdfs:Class rdf:ID="RecoveringFromIllness"><rdfs:subClassOf rdf:resource="http://reliant.teknowledge.com/DAML/SUMO.owl#OrganismProcess" /><rdfs:comment>Any Process where the experiencer recovers 

from a DiseaseOrSyndrome.</rdfs:comment></rdfs:Class><rdfs:Class rdf:ID="RecreationOrExerciseDevice"><rdfs:subClassOf rdf:resource="http://reliant.teknowledge.com/DAML/SUMO.owl#Device" /><rdfs:comment>A Device whose purpose is RecreationOrExercise.</rdfs:comment></rdfs:Class><rdfs:Class rdf:ID="Rectangle"><rdfs:subClassOf rdf:resource="#Quadrilateral" /><rdfs:comment>Any Quadrilateral whose angles are all 

RightAngles.</rdfs:comment></rdfs:Class><rdfs:Class rdf:ID="RedBloodCell"><rdfs:subClassOf rdf:resource="#BloodCell" /><rdfs:comment>BloodCells that contain hemoglobin, lack a 

CellNucleus, and carry Oxygen to the tissues of the body.</rdfs:comment></rdfs:Class><rdfs:Class rdf:ID="RedcoatSoldier"><rdfs:subClassOf rdf:resource="#Soldier" /><rdfs:comment>Any Soldier that served on the British side during 

the American revolutionary war.</rdfs:comment></rdfs:Class><rdfs:Class rdf:ID="ReferenceText"><rdfs:subClassOf rdf:resource="http://reliant.teknowledge.com/DAML/SUMO.owl#FactualText" /><rdfs:comment>A Text which is not intended to be read 

from beginning to end, but which is meant to be consulted to answer specific 

factual questions, e.g. about the meaning of a word, the location of a 

country, etc.</rdfs:comment></rdfs:Class><rdfs:Class rdf:ID="RefinedPetroleumProduct"><rdfs:subClassOf rdf:resource="#PetroleumProduct" /><rdfs:comment>RefinedPetroleumProduct is the 

subclass of PetroleumProducts that are refined from Petroleum (crude oil).</rdfs:comment></rdfs:Class><rdfs:Class rdf:ID="Reflecting"><rdfs:subClassOf rdf:resource="http://reliant.teknowledge.com/DAML/SUMO.owl#Radiating" /><rdfs:comment>Any instance of Radiating where the radiated 

waves rebound from a surface, e.g. an echo of sound or a reflection of 

light.</rdfs:comment></rdfs:Class><rdfs:Class rdf:ID="ReflectingLight"><rdfs:subClassOf rdf:resource="#Reflecting" /><rdfs:subClassOf rdf:resource="http://reliant.teknowledge.com/DAML/SUMO.owl#RadiatingLight" /><rdfs:comment>Those instances of RadiatingLight where the 

instrument is not a light source, but is simply a surface which bends light 

waves that come in contact with it.</rdfs:comment></rdfs:Class><rdfs:Class rdf:ID="ReflexiveProcess"><rdfs:subClassOf rdf:resource="http://reliant.teknowledge.com/DAML/SUMO.owl#AutonomicProcess" /><rdfs:comment>Any Muscle reaction which is a response 

to a specific stimulus and which does not reach the level of consciousness.</rdfs:comment></rdfs:Class><rdfs:Class rdf:ID="Refrigerator"><rdfs:subClassOf rdf:resource="#CoolingDevice" /><rdfs:subClassOf rdf:resource="#ElectricDevice" /><rdfs:subClassOf rdf:resource="#Container" /><rdfs:comment>The intersection of Containers and ElectricDevices 

in which the temperature is reduced from that of the outside air by a Cooling 

process.</rdfs:comment></rdfs:Class><rdfs:Class rdf:ID="Registering"><rdfs:subClassOf rdf:resource="http://reliant.teknowledge.com/DAML/SUMO.owl#Stating" /><rdfs:subClassOf rdf:resource="http://reliant.teknowledge.com/DAML/SUMO.owl#PoliticalProcess" /><rdfs:comment>Submitting official paperwork to an organization, 

typically a GovernmentOrganization or an EducationalOrganization.  This 

class covers things like filing for divorce, making a legal claim against someone, 

enrolling in an educational program, etc.</rdfs:comment></rdfs:Class><rdfs:Class rdf:ID="Regretting"><rdfs:subClassOf rdf:resource="#ExpressingDisapproval" /><rdfs:comment>ExpressingDisapproval about a state of affairs 

that has already occurred.</rdfs:comment></rdfs:Class><rdfs:Class rdf:ID="Releasing"><rdfs:subClassOf rdf:resource="http://reliant.teknowledge.com/DAML/SUMO.owl#Translocation" /><sumo:disjoint rdf:resource="#Escaping" /><rdfs:comment>Any instance of Translocation where the experiencer 

is released from confinement by right.</rdfs:comment></rdfs:Class><rdfs:Class rdf:ID="RelievingPain"><rdfs:subClassOf rdf:resource="http://reliant.teknowledge.com/DAML/SUMO.owl#TherapeuticProcess" /><rdfs:subClassOf rdf:resource="#CausingHappiness" /><rdfs:comment>Any TherapeuticProcess that removes Pain from 

the patient of the process.</rdfs:comment></rdfs:Class><rdfs:Class rdf:ID="ReligiousBuilding"><rdfs:subClassOf rdf:resource="http://reliant.teknowledge.com/DAML/SUMO.owl#Building" /><rdfs:comment>A Building which is intended to be 

used for religious worship.  This class covers churches, temples, 

religious shrines, etc.</rdfs:comment></rdfs:Class><rdfs:Class rdf:ID="ReligiousPosition"><rdfs:subClassOf rdf:resource="http://reliant.teknowledge.com/DAML/SUMO.owl#Position" /><rdfs:comment>Any Position within a ReligousOrganization.</rdfs:comment></rdfs:Class><rdfs:Class rdf:ID="ReligiousService"><rdfs:subClassOf rdf:resource="http://reliant.teknowledge.com/DAML/SUMO.owl#ReligiousProcess" /><rdfs:subClassOf rdf:resource="http://reliant.teknowledge.com/DAML/SUMO.owl#Demonstrating" /><rdfs:comment>A formal process of public worship which is 

typically carried out in a church, temple or other sanctified building and 

which typically accords with a prescribed set of rules.</rdfs:comment></rdfs:Class><rdfs:Class rdf:ID="Reminding"><rdfs:subClassOf rdf:resource="http://reliant.teknowledge.com/DAML/SUMO.owl#Requesting" /><rdfs:comment>Any Requesting that is intended to cause a 

Remembering of something.</rdfs:comment></rdfs:Class><rdfs:Class rdf:ID="RemovingClothing"><rdfs:subClassOf rdf:resource="http://reliant.teknowledge.com/DAML/SUMO.owl#Uncovering" /><rdfs:comment>Removing Clothing from a Human or 

Animal in such a way that the Human or Animal no longer wears the 

Clothing.</rdfs:comment></rdfs:Class><rdfs:Class rdf:ID="Renting"><rdfs:subClassOf rdf:resource="http://reliant.teknowledge.com/DAML/SUMO.owl#FinancialTransaction" /><rdfs:subClassOf rdf:resource="http://reliant.teknowledge.com/DAML/SUMO.owl#Borrowing" /><rdfs:comment>Giving money to the owner of an Object in 

exchange for the right to use the Object for a fixed time period.</rdfs:comment></rdfs:Class><rdfs:Class rdf:ID="Report"><rdfs:subClassOf rdf:resource="http://reliant.teknowledge.com/DAML/SUMO.owl#FactualText" /><rdfs:subClassOf rdf:resource="http://reliant.teknowledge.com/DAML/SUMO.owl#Article" /><rdfs:comment>A relatively brief FactualText, often it 

describes the findings of a study or experiment, or a series of 

observations.</rdfs:comment></rdfs:Class><rdfs:Class rdf:ID="Request"><rdfs:subClassOf rdf:resource="http://reliant.teknowledge.com/DAML/SUMO.owl#Sentence" /><rdfs:comment>A Sentence that expresses a request for something or 

that something be done.</rdfs:comment></rdfs:Class><rdfs:Class rdf:ID="Researcher"><rdfs:subClassOf rdf:resource="#Profession" /><rdfs:comment>The Profession of being a scientific 

researcher.</rdfs:comment></rdfs:Class><rdfs:Class rdf:ID="Resigning"><rdfs:subClassOf rdf:resource="http://reliant.teknowledge.com/DAML/SUMO.owl#TerminatingEmployment" /><rdfs:comment>Voluntarily ending one's employment.</rdfs:comment></rdfs:Class><rdfs:Class rdf:ID="Resistor"><rdfs:subClassOf rdf:resource="http://reliant.teknowledge.com/DAML/SUMO.owl#EngineeringComponent" /><rdfs:comment>A Device which resists passage of an electric current 

through it.  It is used for various purposes in an electrical circuit.</rdfs:comment></rdfs:Class><rdfs:Class rdf:ID="Resolution"><rdfs:subClassOf rdf:resource="http://reliant.teknowledge.com/DAML/SUMO.owl#Deciding" /><rdfs:comment>Any instance of Deciding which is conducted at a 

FormalMeeting and where the agent is an Organization.</rdfs:comment></rdfs:Class><rdfs:Class rdf:ID="Restaurant"><rdfs:subClassOf rdf:resource="http://reliant.teknowledge.com/DAML/SUMO.owl#CommercialAgent" /><rdfs:comment>Any CommercialAgent whose services include selling 

Food to customers which is intended to be eaten on the premises.</rdfs:comment></rdfs:Class><rdfs:Class rdf:ID="RetailStore"><rdfs:subClassOf rdf:resource="http://reliant.teknowledge.com/DAML/SUMO.owl#MercantileOrganization" /><sumo:disjoint rdf:resource="#WholesaleStore" /><rdfs:comment>The complement of WholesaleStore, i.e. 

MercantileOrganizations that sell their goods to the general public.</rdfs:comment></rdfs:Class><rdfs:Class rdf:ID="Retina"><rdfs:subClassOf rdf:resource="http://reliant.teknowledge.com/DAML/SUMO.owl#Organ" /><rdfs:subClassOf rdf:resource="http://reliant.teknowledge.com/DAML/SUMO.owl#AnimalAnatomicalStructure" /><rdfs:comment>A membrane that covers the Eye and converts 

the image formed by the lens of the Eye into neurochemical impulses 

which can be processed by the Brain.</rdfs:comment></rdfs:Class><rdfs:Class rdf:ID="Retiring"><rdfs:subClassOf rdf:resource="#Resigning" /><rdfs:comment>Voluntarily leaving employment at the end of one's 

career in order to take time off in the later years of one's life.</rdfs:comment></rdfs:Class><rdfs:Class rdf:ID="Returning"><rdfs:subClassOf rdf:resource="http://reliant.teknowledge.com/DAML/SUMO.owl#Translocation" /><rdfs:comment>Any instance of Translocation where the agent 

goes to a location where he/she had been before the Translocation took place.</rdfs:comment></rdfs:Class><rdfs:Class rdf:ID="Reversing"><rdfs:subClassOf rdf:resource="http://reliant.teknowledge.com/DAML/SUMO.owl#Motion" /><rdfs:comment>Moving something in such a way that its top 

becomes its bottom and vice versa.</rdfs:comment></rdfs:Class><rdfs:Class rdf:ID="RevolverGun"><rdfs:subClassOf rdf:resource="#Pistol" /><rdfs:comment>A Pistol whose magazine is a revolving cylinder with 

six chambers for Bullets.</rdfs:comment></rdfs:Class><rdfs:Class rdf:ID="Rice"><rdfs:subClassOf rdf:resource="#CerealGrain" /><rdfs:comment>A CerealGrain which has short and long grain varieties 

and which is usually prepared for eating by steaming.</rdfs:comment></rdfs:Class><rdfs:Class rdf:ID="Rifle"><rdfs:subClassOf rdf:resource="#Firearm" /><rdfs:comment>A Firearm with a long barrel that is intended to be fired 

from the shoulder.</rdfs:comment></rdfs:Class><rdfs:Class rdf:ID="RightAngle"><rdfs:subClassOf rdf:resource="http://reliant.teknowledge.com/DAML/SUMO.owl#TwoDimensionalAngle" /><rdfs:comment>Any TwoDimensionalAngle that has the 

angularMeasure of 90 AngularDegrees.</rdfs:comment></rdfs:Class><rdfs:Class rdf:ID="RightTriangle"><rdfs:subClassOf rdf:resource="#Triangle" /><rdfs:comment>Any Triangle that contains a RightAngle.</rdfs:comment></rdfs:Class><rdfs:Class rdf:ID="Ringing"><rdfs:subClassOf rdf:resource="http://reliant.teknowledge.com/DAML/SUMO.owl#RadiatingSound" /><rdfs:comment>Any instance of RadiatingSound which is produced by 

a Bell.</rdfs:comment></rdfs:Class><rdfs:Class rdf:ID="River"><rdfs:subClassOf rdf:resource="#BodyOfWater" /><rdfs:subClassOf rdf:resource="http://reliant.teknowledge.com/DAML/SUMO.owl#StreamWaterArea" /><rdfs:subClassOf rdf:resource="http://reliant.teknowledge.com/DAML/SUMO.owl#FreshWaterArea" /><rdfs:comment>River is the class of large streams of fresh 

water flowing through land into a lake, ocean, or other body of water.</rdfs:comment></rdfs:Class><rdfs:Class rdf:ID="RoadJunction"><rdfs:subClassOf rdf:resource="#TransitwayJunction" /><rdfs:subClassOf rdf:resource="http://reliant.teknowledge.com/DAML/SUMO.owl#Roadway" /><rdfs:comment>RoadJunction is the subclass of 

TransitwayJunctions where two or more Roadways come together.</rdfs:comment></rdfs:Class><rdfs:Class rdf:ID="RoadTransportationSystem"><rdfs:subClassOf rdf:resource="#TransportationSystem" /><rdfs:comment>RoadTransportationSystem 

is the subclass of TransportationSystems whose routes are Roadways.</rdfs:comment></rdfs:Class><rdfs:Class rdf:ID="RoadVehicle"><rdfs:subClassOf rdf:resource="#LandVehicle" /><rdfs:comment>The class of LandVehicles that are not 

RollingStock.</rdfs:comment></rdfs:Class><rdfs:Class rdf:ID="Robbing"><rdfs:subClassOf rdf:resource="#Stealing" /><rdfs:comment>Any instance of Stealing which involves the threat 

of the use of force.</rdfs:comment></rdfs:Class><rdfs:Class rdf:ID="Rock"><rdfs:subClassOf rdf:resource="http://reliant.teknowledge.com/DAML/SUMO.owl#Substance" /><rdfs:comment>Rock is any naturally formed aggregate of 

one or more minerals, consolidated or not, with some degree of 

mineralogic and chemical constancy; in popular use the term is 

usually restricted to those aggregates that are hard, compact, 

and coherent.</rdfs:comment></rdfs:Class><rdfs:Class rdf:ID="Rocket"><rdfs:subClassOf rdf:resource="#Spacecraft" /><rdfs:comment>A Spacecraft which has the shape of a cylinder 

with a cone on top and which is powered by a jet engine.</rdfs:comment></rdfs:Class><rdfs:Class rdf:ID="RollingStock"><rdfs:subClassOf rdf:resource="#RailwayVehicle" /><rdfs:comment>RollingStock is the subclass of 

RailwayVehicles that are individual railway cars.  RollingStock includes 

locomotives, motorized transit cars, trolleys, and all kinds of railcars.</rdfs:comment></rdfs:Class><rdfs:Class rdf:ID="Roof"><rdfs:subClassOf rdf:resource="http://reliant.teknowledge.com/DAML/SUMO.owl#StationaryArtifact" /><rdfs:comment>The top of a Building.</rdfs:comment></rdfs:Class><rdfs:Class rdf:ID="Rooster"><rdfs:subClassOf rdf:resource="#Chicken" /><rdfs:comment>A Male Chicken.</rdfs:comment></rdfs:Class><rdfs:Class rdf:ID="Rotating"><rdfs:subClassOf rdf:resource="http://reliant.teknowledge.com/DAML/SUMO.owl#Motion" /><rdfs:comment>Motion that begins and ends at the same point, 

because the trajectory of the Motion is circular.</rdfs:comment></rdfs:Class><rdfs:Class rdf:ID="Rotor"><rdfs:subClassOf rdf:resource="http://reliant.teknowledge.com/DAML/SUMO.owl#EngineeringComponent" /><rdfs:comment>The Rotating component of a motor, generator or similar 

Device.</rdfs:comment></rdfs:Class><rdfs:Class rdf:ID="Rowing"><rdfs:subClassOf rdf:resource="#WaterTransportation" /><rdfs:comment>Any instance of WaterTransportation where the 

instrument is an Oar that is manually powered.</rdfs:comment></rdfs:Class><rdfs:Class rdf:ID="Rubber"><rdfs:subClassOf rdf:resource="http://reliant.teknowledge.com/DAML/SUMO.owl#PlantSubstance" /><rdfs:comment>A latex that is produced by certain species of 

BotanticalTrees.</rdfs:comment></rdfs:Class><rdfs:Class rdf:ID="Rug"><rdfs:subClassOf rdf:resource="#FabricArtifact" /><rdfs:comment>A piece of Fabric whose purpose is to cover a Floor.</rdfs:comment></rdfs:Class><rdfs:Class rdf:ID="Runway"><rdfs:subClassOf rdf:resource="http://reliant.teknowledge.com/DAML/SUMO.owl#LandTransitway" /><rdfs:comment>Runway is the class of Transitways that are 

used for the takeoff and landing of Airplanes.  Runways are 

Transitways for an intermodal transit, which begins with a land transit 

and ends with air transit, or vice versa.</rdfs:comment></rdfs:Class><rdfs:Class rdf:ID="Saddle"><rdfs:subClassOf rdf:resource="#Holder" /><rdfs:comment>A Device which allows a Human to ride on a 

Horse.</rdfs:comment></rdfs:Class><rdfs:Class rdf:ID="SafeContainer"><rdfs:subClassOf rdf:resource="#Container" /><rdfs:subClassOf rdf:resource="#SecurityDevice" /><rdfs:comment>A Container with a Lock which is intended 

to secure items from theft.  Note that this covers safes, lockers, and locked 

storage compartments.</rdfs:comment></rdfs:Class><rdfs:Class rdf:ID="Sailor"><rdfs:subClassOf rdf:resource="#SkilledOccupation" /><rdfs:comment>The class of Positions which involve working on a 

ship, whether a merchant ship or a navy ship.</rdfs:comment></rdfs:Class><rdfs:Class rdf:ID="SalesPosition"><rdfs:subClassOf rdf:resource="#SkilledOccupation" /><rdfs:comment>Any Position which involves Selling 

or trying to sell items.</rdfs:comment></rdfs:Class><rdfs:Class rdf:ID="SalineSolution"><rdfs:subClassOf rdf:resource="http://reliant.teknowledge.com/DAML/SUMO.owl#Solution" /><rdfs:comment>A Solution consisting of SodiumChloride 

and Water.</rdfs:comment></rdfs:Class><rdfs:Class rdf:ID="SaltLake"><rdfs:subClassOf rdf:resource="http://reliant.teknowledge.com/DAML/SUMO.owl#SaltWaterArea" /><rdfs:subClassOf rdf:resource="#LandlockedWater" /><rdfs:comment>SaltLake is the class of landlocked 

bodies of salt water, including those referred to as 'Seas', e.g., 

the CaspianSea.  But note that the MediterraneanSea is a Sea.</rdfs:comment></rdfs:Class><rdfs:Class rdf:ID="Sand"><rdfs:subClassOf rdf:resource="#Soil" /><rdfs:comment>Sand is loose fragments of minerals or rocks. 

Smaller than gravel and larger than silt and clay, sand particles 

range from 8/10,000 to 8/100 inch (0.02 to 2 millimeters) in diameter. 

Sand is formed by the Erosion of rocks through the action of water, 

ice, or air.</rdfs:comment></rdfs:Class><rdfs:Class rdf:ID="Sandwich"><rdfs:subClassOf rdf:resource="#PreparedFood" /><rdfs:comment>Any Food which consists of two or more pieces 

of bread and some sort of filling between the two pieces of bread.</rdfs:comment></rdfs:Class><rdfs:Class rdf:ID="Satellite"><rdfs:comment>Satellite is the collection of bodies that 

revolve around some  astronomical body, e.g., planets around a star.</rdfs:comment></rdfs:Class><rdfs:Class rdf:ID="Saving"><rdfs:subClassOf rdf:resource="http://reliant.teknowledge.com/DAML/SUMO.owl#Decreasing" /><rdfs:comment>Any instance of Decreasing where the PhysicalQuantity 

involved is a CurrencyMeasure.</rdfs:comment></rdfs:Class><rdfs:Class rdf:ID="SavingsAccount"><rdfs:subClassOf rdf:resource="#InterestBearingAccount" /><rdfs:subClassOf rdf:resource="#DepositAccount" /><rdfs:comment>An account in a bank on which interest is 

usually paid and from which withdrawals can be made usually only by 

presentation of a passbook or by written authorization on a prescribed form.</rdfs:comment></rdfs:Class><rdfs:Class rdf:ID="SavingsAndLoan"><rdfs:subClassOf rdf:resource="#FinancialCompany" /><rdfs:comment>A federally or state chartered 

FinancialCompany that takes Deposits from individuals, funds 

Mortgages, and pays Dividends.</rdfs:comment></rdfs:Class><rdfs:Class rdf:ID="Scar"><rdfs:subClassOf rdf:resource="http://reliant.teknowledge.com/DAML/SUMO.owl#AbnormalAnatomicalStructure" /><rdfs:comment>Any AbnormalAnatomicalStructure which results from the 

healing of a Lesion.</rdfs:comment></rdfs:Class><rdfs:Class rdf:ID="Scholarship"><rdfs:subClassOf rdf:resource="http://reliant.teknowledge.com/DAML/SUMO.owl#Funding" /><rdfs:comment>Any Funding which is made on the basis of merit 

and whose purpose is to allow the destination to realize an 

EducationalProgram.</rdfs:comment></rdfs:Class><rdfs:Class rdf:ID="School"><rdfs:subClassOf rdf:resource="http://reliant.teknowledge.com/DAML/SUMO.owl#EducationalOrganization" /><rdfs:comment>An EducationalOrganization with a curriculum, 

teachers, and students.  Most Schools are housed in a Building 

dedicated to the EducationalOrganization.</rdfs:comment></rdfs:Class><rdfs:Class rdf:ID="Science"><rdfs:subClassOf rdf:resource="http://reliant.teknowledge.com/DAML/SUMO.owl#FieldOfStudy" /><rdfs:comment>Any FieldOfStudy which tests theories on the basis of 

careful observations and/or experiments and which has a cumulative body of results.</rdfs:comment></rdfs:Class><rdfs:Class rdf:ID="Score"><rdfs:subClassOf rdf:resource="#GameShot" /><rdfs:comment>A successful attempt to score a point in a Game.</rdfs:comment></rdfs:Class><rdfs:Class rdf:ID="Screw"><rdfs:subClassOf rdf:resource="http://reliant.teknowledge.com/DAML/SUMO.owl#AttachingDevice" /><rdfs:comment>An AttachingDevice which contains a spiral of grooves to 

hold it in place and which is fastened with a screwdriver.</rdfs:comment></rdfs:Class><rdfs:Class rdf:ID="Sculpture"><rdfs:subClassOf rdf:resource="http://reliant.teknowledge.com/DAML/SUMO.owl#ArtWork" /><rdfs:comment>Any ArtWork which is not constructed on the 

two-dimensional surface of a canvas, piece of paper, etc.</rdfs:comment></rdfs:Class><rdfs:Class rdf:ID="Sea"><rdfs:subClassOf rdf:resource="http://reliant.teknowledge.com/DAML/SUMO.owl#SaltWaterArea" /><rdfs:subClassOf rdf:resource="#BodyOfWater" /><rdfs:comment>Sea is the class of smaller subdivisions of 

the WorldOcean, typically partially surrounded by land.</rdfs:comment></rdfs:Class><rdfs:Class rdf:ID="SeasonOfYear"><rdfs:subClassOf rdf:resource="http://reliant.teknowledge.com/DAML/SUMO.owl#TimeInterval" /><rdfs:comment>SeasonOfYear is the class of four 

seasons correlated with the calendar Year and associated with 

changes in the length of daylight and with overall temperature 

changes. Depending upon the GeographicArea, a SeasonOfYear 

may also be associated with weather patterns (e.g., rainy, dry, 

windy). The characteristics of seasons (cold vs. hot temperatures, 

long vs. short days) are reversed from the NorthernHemisphere 

to the SouthernHemisphere.</rdfs:comment></rdfs:Class><rdfs:Class rdf:ID="Seat"><rdfs:subClassOf rdf:resource="#Furniture" /><rdfs:comment>Any instance of Furniture which is designed to 

accommodate Humans who are Sitting.</rdfs:comment></rdfs:Class><rdfs:Class rdf:ID="Seating"><rdfs:subClassOf rdf:resource="http://reliant.teknowledge.com/DAML/SUMO.owl#Guiding" /><rdfs:comment>Guiding someone to a Seat, e.g. as when an usher 

shows someone to a Seat in an Auditorium.</rdfs:comment></rdfs:Class><rdfs:Class rdf:ID="SecondaryColor"><rdfs:subClassOf rdf:resource="http://reliant.teknowledge.com/DAML/SUMO.owl#ColorAttribute" /><rdfs:comment>A color that is the product of mixing together 

two or more PrimaryColors.</rdfs:comment></rdfs:Class><rdfs:Class rdf:ID="SecondarySchool"><rdfs:subClassOf rdf:resource="#School" /><rdfs:comment>A School which admits students who have 

graduated from a middle school and which normally covers the ninth through 

twelfth grades.  A SecondarySchool confers a high school diploma.</rdfs:comment></rdfs:Class><rdfs:Class rdf:ID="Security"><rdfs:subClassOf rdf:resource="http://reliant.teknowledge.com/DAML/SUMO.owl#FinancialInstrument" /><rdfs:comment>An investment instrument, other than an insurance 

policy or a fixed annuity issued by a corporation, government, or other 

organization which offers evidence of debt or equity.</rdfs:comment></rdfs:Class><rdfs:Class rdf:ID="SecurityAlarm"><rdfs:subClassOf rdf:resource="#SecurityDevice" /><rdfs:subClassOf rdf:resource="#ElectricDevice" /><rdfs:comment>A SecurityDevice that detects intrusions to 

a StationaryArtifact and issues a warning of some sort.</rdfs:comment></rdfs:Class><rdfs:Class rdf:ID="SecurityDevice"><rdfs:subClassOf rdf:resource="http://reliant.teknowledge.com/DAML/SUMO.owl#Device" /><rdfs:comment>A Device whose purpose is to protect people or 

property from kidnappers and/or thieves.</rdfs:comment></rdfs:Class><rdfs:Class rdf:ID="SecurityUnit"><rdfs:subClassOf rdf:resource="http://reliant.teknowledge.com/DAML/SUMO.owl#Organization" /><rdfs:comment>The Organization that is charged with 

ensuring the security of members of the overall Organization and the 

property of the Organization.</rdfs:comment></rdfs:Class><rdfs:Class rdf:ID="SeizingProperty"><rdfs:subClassOf rdf:resource="http://reliant.teknowledge.com/DAML/SUMO.owl#UnilateralGetting" /><rdfs:comment>Any instance of UnilateralGetting which is done by 

a Government and which is not permitted by the origin of the UnilateralGetting.</rdfs:comment></rdfs:Class><rdfs:Class rdf:ID="SelfPoweredDevice"><rdfs:subClassOf rdf:resource="http://reliant.teknowledge.com/DAML/SUMO.owl#Device" /><rdfs:comment>SelfPoweredDevice is the subclass of Devices whose action is 

powered by some kind of on-board component or power source (not the user).</rdfs:comment></rdfs:Class><rdfs:Class rdf:ID="SelfPoweredRoadVehicle"><rdfs:subClassOf rdf:resource="#RoadVehicle" /><rdfs:subClassOf rdf:resource="#SelfPoweredVehicle" /><rdfs:comment>SelfPoweredRoadVehicle is the 

class of RoadVehicles that are also SelfPoweredVehicles.  

SelfPoweredRoadVehicle covers motorcycles, semi-trailers, RVs, etc., 

as well as Automobiles.  This class includes vehicles powered by 

electricity, gasoline, diesel, and other fuels.</rdfs:comment></rdfs:Class><rdfs:Class rdf:ID="SelfPoweredVehicle"><rdfs:subClassOf rdf:resource="http://reliant.teknowledge.com/DAML/SUMO.owl#Vehicle" /><rdfs:subClassOf rdf:resource="#SelfPoweredDevice" /><rdfs:comment>SelfPoweredVehicle is the subclass 

of Vehicles whose motion is powered by some kind of on-board power 

source.</rdfs:comment></rdfs:Class><rdfs:Class rdf:ID="Sentencing"><rdfs:subClassOf rdf:resource="http://reliant.teknowledge.com/DAML/SUMO.owl#LegalDecision" /><rdfs:comment>Any LegalDecision where the defendant is assigned 

a punishment for a CriminalAction which was the subject of an earlier 

LegalConviction.</rdfs:comment></rdfs:Class><rdfs:Class rdf:ID="Sergeant"><rdfs:subClassOf rdf:resource="#MilitaryOfficer" /><rdfs:comment>A noncomissioned MilitaryOfficer.</rdfs:comment></rdfs:Class><rdfs:Class rdf:ID="Sermon"><rdfs:subClassOf rdf:resource="#Lecture" /><rdfs:comment>A Lecture that is part of a ReligiousService.</rdfs:comment></rdfs:Class><rdfs:Class rdf:ID="Serum"><rdfs:subClassOf rdf:resource="#LiquidBodySubstance" /><sumo:disjoint rdf:resource="http://reliant.teknowledge.com/DAML/SUMO.owl#Blood" /><rdfs:comment>Any LiquidBodySubstance other than Blood.</rdfs:comment></rdfs:Class><rdfs:Class rdf:ID="ServicePosition"><rdfs:subClassOf rdf:resource="#SkilledOccupation" /><rdfs:comment>Any Position which involves working 

as a waiter or servant, either for an Organization (e.g. a restaurant) 

or for a person or family.</rdfs:comment></rdfs:Class><rdfs:Class rdf:ID="Sewage"><rdfs:subClassOf rdf:resource="http://reliant.teknowledge.com/DAML/SUMO.owl#Mixture" /><rdfs:comment>Waste products produced by Humans.</rdfs:comment></rdfs:Class><rdfs:Class rdf:ID="SewageSystem"><rdfs:subClassOf rdf:resource="#Pipeline" /><rdfs:comment>A Pipline which is used to transport human 

waste to an area where it can be treated and/or disposed of.</rdfs:comment></rdfs:Class><rdfs:Class rdf:ID="Sewing"><rdfs:subClassOf rdf:resource="http://reliant.teknowledge.com/DAML/SUMO.owl#Attaching" /><rdfs:comment>Attaching two pieces of Fabric or one part of a 

piece of Fabric to another part by means of needle and thread.</rdfs:comment></rdfs:Class><rdfs:Class rdf:ID="Share"><rdfs:subClassOf rdf:resource="http://reliant.teknowledge.com/DAML/SUMO.owl#CurrencyMeasure" /><rdf:type rdf:resource="http://reliant.teknowledge.com/DAML/SUMO.owl#UnitOfMeasure" /><rdfs:comment>A UnitOfMeasure representing one unit of ownership 

in a corporation, MutualFund, or limited partnership.</rdfs:comment></rdfs:Class><rdfs:Class rdf:ID="Sharing"><rdfs:subClassOf rdf:resource="http://reliant.teknowledge.com/DAML/SUMO.owl#ChangeOfPossession" /><rdfs:comment>The subclass of ChangeOfPossession where a 

properPart of the patient is given by the agent to the destination.</rdfs:comment></rdfs:Class><rdfs:Class rdf:ID="Sheep"><rdfs:subClassOf rdf:resource="http://reliant.teknowledge.com/DAML/SUMO.owl#HoofedMammal" /><rdfs:subClassOf rdf:resource="#DomesticAnimal" /><rdfs:comment>A domesticated HoofedMammal that is bred for its 

wool and for its meat (known as mutton).</rdfs:comment></rdfs:Class><rdfs:Class rdf:ID="Shelf"><rdfs:subClassOf rdf:resource="http://reliant.teknowledge.com/DAML/SUMO.owl#Artifact" /><rdfs:comment>An piece of Furniture or part of a piece of Furniture 

that is used for keeping or displaying things.</rdfs:comment></rdfs:Class><rdfs:Class rdf:ID="Sheriff"><rdfs:subClassOf rdf:resource="#PoliceOfficer" /><rdfs:comment>A PoliceOfficer whose jurisdiction is a County.</rdfs:comment></rdfs:Class><rdfs:Class rdf:ID="Shield"><rdfs:subClassOf rdf:resource="http://reliant.teknowledge.com/DAML/SUMO.owl#Artifact" /><rdfs:comment>An Artifact that is held by the hand or whole arm and 

is used to prevent injuries from Weapons.</rdfs:comment></rdfs:Class><rdfs:Class rdf:ID="Ship"><rdfs:subClassOf rdf:resource="#DisplacementHullWatercraft" /><rdfs:comment>Ship is the class of large Watercraft used 

for travel on oceans, seas, or large lakes.</rdfs:comment></rdfs:Class><rdfs:Class rdf:ID="ShipCaptain"><rdfs:subClassOf rdf:resource="#SkilledOccupation" /><rdfs:comment>The class of Positions which involve the command 

of a ship.</rdfs:comment></rdfs:Class><rdfs:Class rdf:ID="ShipMate"><rdfs:subClassOf rdf:resource="#SkilledOccupation" /><rdfs:comment>The class of Positions that involve some responsibility 

on a ship and are lower in rank than ShipCaptain.</rdfs:comment></rdfs:Class><rdfs:Class rdf:ID="ShipOfficer"><rdfs:subClassOf rdf:resource="#Sailor" /><rdfs:comment>The class of Sailors which have a position of 

responsibility on a Ship.</rdfs:comment></rdfs:Class><rdfs:Class rdf:ID="Shipping"><rdfs:subClassOf rdf:resource="http://reliant.teknowledge.com/DAML/SUMO.owl#Transportation" /><rdfs:comment>Shipping is the subclass of Transportation 

events in which goods are transported from one place to another by an 

agent who is entrusted with the goods temporarily just in order to move 

them.  Shipping may be done within an organization or it may be done 

by an outside commercial agent.  See CommercialShipping.</rdfs:comment></rdfs:Class><rdfs:Class rdf:ID="Shirt"><rdfs:subClassOf rdf:resource="http://reliant.teknowledge.com/DAML/SUMO.owl#Clothing" /><rdfs:comment>An item of Clothing which covers the upper body of a 

Human.</rdfs:comment></rdfs:Class><rdfs:Class rdf:ID="Shoe"><rdfs:subClassOf rdf:resource="http://reliant.teknowledge.com/DAML/SUMO.owl#Clothing" /><rdfs:comment>Clothing that is intended to be worn on the Foot.  

It consists of an upper, a sole, and a heel.</rdfs:comment></rdfs:Class><rdfs:Class rdf:ID="ShoppingMall"><rdfs:subClassOf rdf:resource="http://reliant.teknowledge.com/DAML/SUMO.owl#MercantileOrganization" /><rdfs:comment>A MercantileOrganization which is a collection 

of various shops gathered together in a single, modern development.</rdfs:comment></rdfs:Class><rdfs:Class rdf:ID="ShortStory"><rdfs:subClassOf rdf:resource="http://reliant.teknowledge.com/DAML/SUMO.owl#FictionalText" /><rdfs:subClassOf rdf:resource="http://reliant.teknowledge.com/DAML/SUMO.owl#Article" /><rdfs:comment>A brief work of fiction, often bound with other 

short stories in a Book or Periodical.</rdfs:comment></rdfs:Class><rdfs:Class rdf:ID="Shortening"><rdfs:subClassOf rdf:resource="http://reliant.teknowledge.com/DAML/SUMO.owl#Decreasing" /><rdfs:comment>Decreasing the length of something.</rdfs:comment></rdfs:Class><rdfs:Class rdf:ID="ShotBall"><rdfs:subClassOf rdf:resource="#Ball" /><rdfs:comment>A solid metal Ball that is used in the sport of 

shotput.</rdfs:comment></rdfs:Class><rdfs:Class rdf:ID="Shoulder"><rdfs:subClassOf rdf:resource="http://reliant.teknowledge.com/DAML/SUMO.owl#AnimalAnatomicalStructure" /><rdfs:subClassOf rdf:resource="http://reliant.teknowledge.com/DAML/SUMO.owl#BodyPart" /><rdfs:comment>The part of a Primate between the Arm and 

the neck.</rdfs:comment></rdfs:Class><rdfs:Class rdf:ID="Shrub"><rdfs:subClassOf rdf:resource="http://reliant.teknowledge.com/DAML/SUMO.owl#FloweringPlant" /><rdfs:comment>Shrub is the class of low, perennial, 

typically multi-stemmed woody plants, called shrubs or bushes.</rdfs:comment></rdfs:Class><rdfs:Class rdf:ID="Shrugging"><rdfs:subClassOf rdf:resource="http://reliant.teknowledge.com/DAML/SUMO.owl#Gesture" /><rdfs:comment>Moving the Shoulders in such a way that the motion 

is intended to express something to someone else.</rdfs:comment></rdfs:Class><rdfs:Class rdf:ID="Sidewalk"><rdfs:subClassOf rdf:resource="http://reliant.teknowledge.com/DAML/SUMO.owl#StationaryArtifact" /><rdfs:comment>A prepared path for pedestrians alongside a Roadway.</rdfs:comment></rdfs:Class><rdfs:Class rdf:ID="Siemens"><rdfs:subClassOf rdf:resource="http://reliant.teknowledge.com/DAML/SUMO.owl#FunctionQuantity" /><rdf:type rdf:resource="http://reliant.teknowledge.com/DAML/SUMO.owl#SystemeInternationalUnit" /><rdfs:comment>SI electric conductance measure.  Symbol:  S.  

In the case of direct current, the conductance in Siemens is the 

reciprocal of the resistance in Ohms; in the case of alternating current, 

it is the reciprocal of the impedance in ohms.  siemens = A/V = 

m^(-2)*kg(-1)*s^(3)*A^2.</rdfs:comment></rdfs:Class><rdfs:Class rdf:ID="Sievert"><rdfs:subClassOf rdf:resource="http://reliant.teknowledge.com/DAML/SUMO.owl#FunctionQuantity" /><rdf:type rdf:resource="http://reliant.teknowledge.com/DAML/SUMO.owl#SystemeInternationalUnit" /><rdfs:comment>SI dose equivalent measure.  Symbol: Sv.  It is 

a unit of biologic dose of ionizing radiation.  The Sievert makes it 

possible to normalize doses of different types of radiation. It takes 

into account the relative biologic effectiveness of ionizing radiation, 

since each form of such radiation--e.g., X rays, gamma rays, neutrons--

has a slightly different effect on living tissue for a given absorbed 

dose. The dose equivalent of a given type of radiation (in Sievert) is 

the dose of the radiation in Gray multiplied by a quality factor that 

is based on the relative biologic effectiveness of the radiation. 

Accordingly, one Sievert is generally defined as the amount of radiation 

roughly equivalent in biologic effectiveness to one Gray of gamma 

radiation.  Sievert = J/kg = m^2*s^(-2)</rdfs:comment></rdfs:Class><rdfs:Class rdf:ID="Signalling"><rdfs:subClassOf rdf:resource="http://reliant.teknowledge.com/DAML/SUMO.owl#Guiding" /><rdfs:comment>Signalling is the subclass of Guiding 

processes in which an agent, animate or inanimate, sends a signal to 

another Object.  In many cases, this signal will be an electrical or 

electronic one.  Some signals may directly control the behavior of 

the object signalled, while others may merely cause information to be 

presented.  Instances of electrical Signalling are typically more 

complex than simply than operation of a DeviceSwitch, though in some 

cases, Signalling involves remote activation of such a switch by another 

device.</rdfs:comment></rdfs:Class><rdfs:Class rdf:ID="SigningADocument"><rdfs:subClassOf rdf:resource="http://reliant.teknowledge.com/DAML/SUMO.owl#Committing" /><rdfs:comment>SigningADocument is the class of 

actions in which an agent affixes a signature, stamp, or other evidence 

of authorization or attestation to a document.  The document and signature 

may be electronic.  Signings count as SocialInteractions even if done in 

private, because their significance derives from a social context.</rdfs:comment></rdfs:Class><rdfs:Class rdf:ID="Silk"><rdfs:subClassOf rdf:resource="http://reliant.teknowledge.com/DAML/SUMO.owl#Fabric" /><rdfs:comment>Fabric that is woven from the strands produced by 

certain Larval Insects.</rdfs:comment></rdfs:Class><rdfs:Class rdf:ID="Silver"><rdfs:subClassOf rdf:resource="http://reliant.teknowledge.com/DAML/SUMO.owl#ElementalSubstance" /><atomicNumber>47</atomicNumber><rdfs:comment>White lustrous soft metallic transition element.  

Found in both its elemental form and in minerals.  Used in jewellery, 

tableware and so on.  Less reactive than silver, chemically.</rdfs:comment></rdfs:Class><rdfs:Class rdf:ID="Sinking"><rdfs:subClassOf rdf:resource="#Falling" /><rdfs:comment>The class of Falling processes that occur 

in a BodyOfWater.</rdfs:comment></rdfs:Class><rdfs:Class rdf:ID="SittingDown"><rdfs:subClassOf rdf:resource="http://reliant.teknowledge.com/DAML/SUMO.owl#BodyMotion" /><rdfs:comment>The BodyMotion of moving from a Standing 

to a Sitting position.</rdfs:comment></rdfs:Class><rdfs:Class rdf:ID="Skeleton"><rdfs:subClassOf rdf:resource="http://reliant.teknowledge.com/DAML/SUMO.owl#AnimalAnatomicalStructure" /><rdfs:subClassOf rdf:resource="http://reliant.teknowledge.com/DAML/SUMO.owl#BodyPart" /><rdfs:comment>The system of Bones that make up the supporting structure 

of Vertebrates.</rdfs:comment></rdfs:Class><rdfs:Class rdf:ID="Sketch"><rdfs:subClassOf rdf:resource="http://reliant.teknowledge.com/DAML/SUMO.owl#ArtWork" /><rdfs:comment>Any ArtWork which is produced by a pencil or 

piece of charcoal.</rdfs:comment></rdfs:Class><rdfs:Class rdf:ID="SkilledOccupation"><rdfs:subClassOf rdf:resource="http://reliant.teknowledge.com/DAML/SUMO.owl#Position" /><rdfs:comment>Any Position which requires 

learning a set of skills.</rdfs:comment></rdfs:Class><rdfs:Class rdf:ID="Skin"><rdfs:subClassOf rdf:resource="http://reliant.teknowledge.com/DAML/SUMO.owl#BodyCovering" /><rdfs:comment>A BodyCovering that comprises part of the surface 

of Organisms.</rdfs:comment></rdfs:Class><rdfs:Class rdf:ID="Skull"><rdfs:subClassOf rdf:resource="http://reliant.teknowledge.com/DAML/SUMO.owl#Bone" /><rdfs:comment>The Bone that is found in the Heads of Vertebrates.</rdfs:comment></rdfs:Class><rdfs:Class rdf:ID="Skylight"><rdfs:subClassOf rdf:resource="#Window" /><rdfs:comment>A Window that is part of the Ceiling of 

a Room.</rdfs:comment></rdfs:Class><rdfs:Class rdf:ID="Sleeve"><rdfs:subClassOf rdf:resource="http://reliant.teknowledge.com/DAML/SUMO.owl#Clothing" /><rdfs:comment>A piece of Clothing that covers the Arm.  A 

Sleeve is always part of a Coat or a Shirt.</rdfs:comment></rdfs:Class><rdfs:Class rdf:ID="SlopedArea"><rdfs:subClassOf rdf:resource="#LandForm" /><rdfs:comment>A SlopedArea is a land surface which lies at an 

angle to the horizontal so that some points on it are higher than others; a 

slope.</rdfs:comment></rdfs:Class><rdfs:Class rdf:ID="Slug"><rdfs:subClassOf rdf:resource="http://reliant.teknowledge.com/DAML/SUMO.owl#MassMeasure" /><rdf:type rdf:resource="http://reliant.teknowledge.com/DAML/SUMO.owl#UnitOfMeasure" /><rdfs:comment>English mass unit of slugs.</rdfs:comment></rdfs:Class><rdfs:Class rdf:ID="Smiling"><rdfs:subClassOf rdf:resource="#FacialExpression" /><rdfs:comment>Spreading the lips in such a way as to convey 

happiness.</rdfs:comment></rdfs:Class><rdfs:Class rdf:ID="Smoking"><rdfs:subClassOf rdf:resource="http://reliant.teknowledge.com/DAML/SUMO.owl#RecreationOrExercise" /><rdfs:comment>Inhaling and exhaling Smoke produced by a 

SmokingDevice.</rdfs:comment></rdfs:Class><rdfs:Class rdf:ID="SmokingDevice"><rdfs:subClassOf rdf:resource="http://reliant.teknowledge.com/DAML/SUMO.owl#Device" /><rdfs:comment>Any Device whose purpose is Smoking.</rdfs:comment></rdfs:Class><rdfs:Class rdf:ID="SmokingPipe"><rdfs:subClassOf rdf:resource="#SmokingDevice" /><rdfs:comment>A SmokingDevice consisting of a tube and a small 

bowl.</rdfs:comment></rdfs:Class><rdfs:Class rdf:ID="Smuggling"><rdfs:subClassOf rdf:resource="http://reliant.teknowledge.com/DAML/SUMO.owl#Transportation" /><rdfs:subClassOf rdf:resource="#CriminalAction" /><rdfs:comment>Any instance Transportation which is also a 

CriminalAction.</rdfs:comment></rdfs:Class><rdfs:Class rdf:ID="Snake"><rdfs:subClassOf rdf:resource="http://reliant.teknowledge.com/DAML/SUMO.owl#Reptile" /><rdfs:comment>A long and narrow Reptile which lacks Limbs.</rdfs:comment></rdfs:Class><rdfs:Class rdf:ID="Snowing"><rdfs:subClassOf rdf:resource="http://reliant.teknowledge.com/DAML/SUMO.owl#Precipitation" /><rdfs:comment>Snowing is a precipitation process 

in which water falls in a Solid state.</rdfs:comment></rdfs:Class><rdfs:Class rdf:ID="SoberingUp"><rdfs:subClassOf rdf:resource="http://reliant.teknowledge.com/DAML/SUMO.owl#PsychologicalProcess" /><rdfs:comment>The process of transitioning from a state of 

being Drunk to a state of being Sober.</rdfs:comment></rdfs:Class><rdfs:Class rdf:ID="SocialParty"><rdfs:subClassOf rdf:resource="http://reliant.teknowledge.com/DAML/SUMO.owl#Meeting" /><rdfs:subClassOf rdf:resource="http://reliant.teknowledge.com/DAML/SUMO.owl#RecreationOrExercise" /><rdfs:comment>Any Meeting where the intent is primarily 

to socialize and be entertained.</rdfs:comment></rdfs:Class><rdfs:Class rdf:ID="SocialScience"><rdfs:subClassOf rdf:resource="#Science" /><rdfs:comment>Any Science which studies human behavior, either in 

the aggregate, as do, for example, Economics and Linguistics, or with respect to 

the individual, as does Psychology.</rdfs:comment></rdfs:Class><rdfs:Class rdf:ID="Sock"><rdfs:subClassOf rdf:resource="http://reliant.teknowledge.com/DAML/SUMO.owl#Clothing" /><rdfs:comment>A piece of Clothing that is made of a soft Fabric 

like Cotton and that is intended to be worn on the Foot.</rdfs:comment></rdfs:Class><rdfs:Class rdf:ID="Sodium"><rdfs:subClassOf rdf:resource="http://reliant.teknowledge.com/DAML/SUMO.owl#ElementalSubstance" /><atomicNumber>11</atomicNumber><rdfs:comment>Soft silvery reactive element belonging to group 1 

of the periodic table (alkali metals).  It is highly reactive, oxidizing 

in air and reacting violently with water, forcing it to be kept under oil.  

It was first isolated by Humphrey Davy in 1807.</rdfs:comment></rdfs:Class><rdfs:Class rdf:ID="SodiumChloride"><rdfs:subClassOf rdf:resource="http://reliant.teknowledge.com/DAML/SUMO.owl#CompoundSubstance" /><rdfs:comment>The CompoundSubstance formed from Sodium 

and Chlorine.</rdfs:comment></rdfs:Class><rdfs:Class rdf:ID="Sofa"><rdfs:subClassOf rdf:resource="#Seat" /><rdfs:comment>A padded Seat that is designed to accommodate more 

than one Human.</rdfs:comment></rdfs:Class><rdfs:Class rdf:ID="Soil"><rdfs:subClassOf rdf:resource="http://reliant.teknowledge.com/DAML/SUMO.owl#Mixture" /><rdfs:comment>Soil is a substance composed of fine rock material 

disintegrated by geological processes, mixed with humus, the organic remains 

of decomposed vegetation.</rdfs:comment></rdfs:Class><rdfs:Class rdf:ID="SolarSystem"><rdfs:subClassOf rdf:resource="http://reliant.teknowledge.com/DAML/SUMO.owl#Collection" /><rdfs:comment>SolarSystem is the class of systems that 

consist of a star or stars and any encircling astronomical bodies.</rdfs:comment></rdfs:Class><rdfs:Class rdf:ID="Soldering"><rdfs:subClassOf rdf:resource="http://reliant.teknowledge.com/DAML/SUMO.owl#Attaching" /><rdfs:comment>Attaching two things by means of a MetallicAlloy.</rdfs:comment></rdfs:Class><rdfs:Class rdf:ID="Soldier"><rdfs:subClassOf rdf:resource="#SkilledOccupation" /><rdfs:comment>The class of Positions which involve serving in 

the armed forces of a Nation.</rdfs:comment></rdfs:Class><rdfs:Class rdf:ID="Somersaulting"><rdfs:subClassOf rdf:resource="http://reliant.teknowledge.com/DAML/SUMO.owl#BodyMotion" /><rdfs:comment>Any BodyMotion which begins and ends in 

a Sitting position and where the feet roll over the head and return to 

their original position.</rdfs:comment></rdfs:Class><rdfs:Class rdf:ID="Song"><rdfs:subClassOf rdf:resource="#MusicalComposition" /><rdfs:comment>Any MusicalComposition which contains Lyrics.</rdfs:comment></rdfs:Class><rdfs:Class rdf:ID="SoupStock"><rdfs:subClassOf rdf:resource="#PreparedFood" /><rdfs:comment>Food which is prepared by reducing Meat 

and/or FruitOrVegetables to a translucent broth which can be used as 

a base for soups or sauces.</rdfs:comment></rdfs:Class><rdfs:Class rdf:ID="SpaceRegion"><rdfs:subClassOf rdf:resource="http://reliant.teknowledge.com/DAML/SUMO.owl#Region" /><sumo:disjoint rdf:resource="http://reliant.teknowledge.com/DAML/SUMO.owl#GeographicArea" /><rdfs:comment>The class of all Regions which are not 

GeographicAreas.</rdfs:comment></rdfs:Class><rdfs:Class rdf:ID="SpaceTransportation"><rdfs:subClassOf rdf:resource="http://reliant.teknowledge.com/DAML/SUMO.owl#Transportation" /><rdfs:comment>Any instance of Transportation where the 

instrument is a Spacecraft and which is through a SpaceRegion.</rdfs:comment></rdfs:Class><rdfs:Class rdf:ID="Spacecraft"><rdfs:subClassOf rdf:resource="http://reliant.teknowledge.com/DAML/SUMO.owl#Vehicle" /><rdfs:comment>Any Vehicle which is capable of 

SpaceTransportation.</rdfs:comment></rdfs:Class><rdfs:Class rdf:ID="Spear"><rdfs:subClassOf rdf:resource="http://reliant.teknowledge.com/DAML/SUMO.owl#Weapon" /><rdfs:comment>A Weapon with a long handle and a short 

blade.</rdfs:comment></rdfs:Class><rdfs:Class rdf:ID="Sphere"><rdfs:subClassOf rdf:resource="http://reliant.teknowledge.com/DAML/SUMO.owl#ThreeDimensionalFigure" /><rdfs:comment>The class of ThreeDimensionalFigures such that 

all GeometricPoints that make up the Sphere are equidistant from a 

single GeometricPoint, known as the center of the Sphere.</rdfs:comment></rdfs:Class><rdfs:Class rdf:ID="SpinalColumn"><rdfs:subClassOf rdf:resource="http://reliant.teknowledge.com/DAML/SUMO.owl#Bone" /><rdfs:comment>A flexible column made out of bones called 

vertebrae. The main function of the SpinalColumn is to protect the 

spinal cord.</rdfs:comment></rdfs:Class><rdfs:Class rdf:ID="SpinalCord"><rdfs:subClassOf rdf:resource="http://reliant.teknowledge.com/DAML/SUMO.owl#Organ" /><rdfs:comment>A cord of nerves that carries impulses to 

and from the Brain.  It is contained within the SpinalColumn.</rdfs:comment></rdfs:Class><rdfs:Class rdf:ID="Spitting"><rdfs:subClassOf rdf:resource="http://reliant.teknowledge.com/DAML/SUMO.owl#Impelling" /><rdfs:comment>Any instance of Impelling where the origin is 

the Mouth of the agent.</rdfs:comment></rdfs:Class><rdfs:Class rdf:ID="Spleen"><rdfs:subClassOf rdf:resource="http://reliant.teknowledge.com/DAML/SUMO.owl#Organ" /><rdfs:subClassOf rdf:resource="http://reliant.teknowledge.com/DAML/SUMO.owl#AnimalAnatomicalStructure" /><rdfs:comment>An Organ on the left side of the body that produces 

Cells that play a crucial role in immune response.</rdfs:comment></rdfs:Class><rdfs:Class rdf:ID="SportServe"><rdfs:subClassOf rdf:resource="#GameShot" /><rdfs:comment>A GameShot which is part of a Sport and 

which serves to start the Sport, e.g. the beginning shot in Tennis, 

Badminton or Squash.</rdfs:comment></rdfs:Class><rdfs:Class rdf:ID="SportsAttribute"><rdfs:subClassOf rdf:resource="#GameAttribute" /><rdfs:comment>Any GameAttribute that is specific to 

a Sport.</rdfs:comment></rdfs:Class><rdfs:Class rdf:ID="SportsFacility"><rdfs:subClassOf rdf:resource="http://reliant.teknowledge.com/DAML/SUMO.owl#StationaryArtifact" /><rdfs:comment>A specially designated and maintained facility 

where Sports are played.  Note that this covers sports fields, stadiums, 

and gymnasiums.</rdfs:comment></rdfs:Class><rdfs:Class rdf:ID="SportsLeague"><rdfs:subClassOf rdf:resource="http://reliant.teknowledge.com/DAML/SUMO.owl#Organization" /><rdfs:comment>An Organization whose members are SportsTeams 

and whose purpose is to set up games between its members.</rdfs:comment></rdfs:Class><rdfs:Class rdf:ID="SportsPlay"><rdfs:subClassOf rdf:resource="http://reliant.teknowledge.com/DAML/SUMO.owl#Plan" /><rdfs:comment>A Plan for a Maneuver within a TeamSport.</rdfs:comment></rdfs:Class><rdfs:Class rdf:ID="SportsPosition"><rdfs:subClassOf rdf:resource="#SkilledOccupation" /><rdfs:comment>A Position which is filled by someone on a 

SportsTeam and which represents the role played by the person on the team.</rdfs:comment></rdfs:Class><rdfs:Class rdf:ID="SportsTeam"><rdfs:subClassOf rdf:resource="http://reliant.teknowledge.com/DAML/SUMO.owl#Organization" /><rdfs:comment>An Organization which habitually plays a Sport 

together, either as an occupation or as a leisure activity.</rdfs:comment></rdfs:Class><rdfs:Class rdf:ID="Spraying"><rdfs:subClassOf rdf:resource="http://reliant.teknowledge.com/DAML/SUMO.owl#LiquidMotion" /><rdfs:subClassOf rdf:resource="http://reliant.teknowledge.com/DAML/SUMO.owl#Transfer" /><rdfs:comment>Any instance of Transfer of a Liquid which is 

accomplished by converting the Liquid into a mist.</rdfs:comment></rdfs:Class><rdfs:Class rdf:ID="SpringSeason"><rdfs:subClassOf rdf:resource="#SeasonOfYear" /><rdfs:comment>The SeasonOfYear that begins at the spring 

equinox and ends at the summer solstice.</rdfs:comment></rdfs:Class><rdfs:Class rdf:ID="Square"><rdfs:subClassOf rdf:resource="#Rectangle" /><rdfs:comment>Any Rectangle whose sides are all equal.</rdfs:comment></rdfs:Class><rdfs:Class rdf:ID="SquareMeter"><rdf:type rdf:resource="http://reliant.teknowledge.com/DAML/SUMO.owl#UnitOfMeasure" /><rdfs:subClassOf rdf:resource="http://reliant.teknowledge.com/DAML/SUMO.owl#AreaMeasure" /><rdfs:comment>SquareMeter represents a UnitOfMeasure 

equal to one square Meter.</rdfs:comment></rdfs:Class><rdfs:Class rdf:ID="SquareMile"><rdf:type rdf:resource="http://reliant.teknowledge.com/DAML/SUMO.owl#UnitOfMeasure" /><rdfs:subClassOf rdf:resource="http://reliant.teknowledge.com/DAML/SUMO.owl#AreaMeasure" /><rdfs:comment>SquareMile represents a UnitOfMeasure 

equal to one square Mile.</rdfs:comment></rdfs:Class><rdfs:Class rdf:ID="SquareYard"><rdf:type rdf:resource="http://reliant.teknowledge.com/DAML/SUMO.owl#UnitOfMeasure" /><rdfs:subClassOf rdf:resource="http://reliant.teknowledge.com/DAML/SUMO.owl#AreaMeasure" /><rdfs:comment>SquareYard represents a UnitOfMeasure 

equal to one square YardLength.</rdfs:comment></rdfs:Class><rdfs:Class rdf:ID="Squirrel"><rdfs:subClassOf rdf:resource="http://reliant.teknowledge.com/DAML/SUMO.owl#Rodent" /><rdfs:comment>A tree-dwelling Rodent with a bushy tail.</rdfs:comment></rdfs:Class><rdfs:Class rdf:ID="StageCoach"><rdfs:subClassOf rdf:resource="#Wagon" /><rdfs:comment>A Wagon that is pulled by Horses and whose purpose 

was to transport Humans and their luggage from one City to the next, especially 

in areas which did not have an established transportation system, e.g. the old west.</rdfs:comment></rdfs:Class><rdfs:Class rdf:ID="Stairway"><rdfs:subClassOf rdf:resource="http://reliant.teknowledge.com/DAML/SUMO.owl#StationaryArtifact" /><rdfs:comment>A StationaryArtifact which allows one to climb, step 

by step, from one level to another.</rdfs:comment></rdfs:Class><rdfs:Class rdf:ID="StandardBearer"><rdfs:subClassOf rdf:resource="#Soldier" /><rdfs:comment>Any Soldier who is tasked with carrying the colors of 

his/her unit in Battles and parades.</rdfs:comment></rdfs:Class><rdfs:Class rdf:ID="StandingUp"><rdfs:subClassOf rdf:resource="http://reliant.teknowledge.com/DAML/SUMO.owl#BodyMotion" /><rdfs:comment>The BodyMotion of moving from a Sitting 

to a Standing position.</rdfs:comment></rdfs:Class><rdfs:Class rdf:ID="Star"><rdfs:subClassOf rdf:resource="http://reliant.teknowledge.com/DAML/SUMO.owl#AstronomicalBody" /><rdfs:comment>Star is the class of hot gaseous astronomical bodies.</rdfs:comment></rdfs:Class><rdfs:Class rdf:ID="Starch"><rdfs:subClassOf rdf:resource="http://reliant.teknowledge.com/DAML/SUMO.owl#Carbohydrate" /><rdfs:comment>A complex Carbohydrate that is the main form in 

which Carbohydrates are stored.</rdfs:comment></rdfs:Class><rdfs:Class rdf:ID="Starving"><rdfs:subClassOf rdf:resource="http://reliant.teknowledge.com/DAML/SUMO.owl#Killing" /><rdfs:comment>Killing someone by depriving them of Food.</rdfs:comment></rdfs:Class><rdfs:Class rdf:ID="StateGovernment"><rdfs:subClassOf rdf:resource="http://reliant.teknowledge.com/DAML/SUMO.owl#Government" /><rdfs:comment>The class of Governments whose 

jurisdictions are StateOrProvinces.</rdfs:comment></rdfs:Class><rdfs:Class rdf:ID="Statement"><rdfs:subClassOf rdf:resource="http://reliant.teknowledge.com/DAML/SUMO.owl#Sentence" /><rdfs:comment>A Sentence that is stated to be true.</rdfs:comment></rdfs:Class><rdfs:Class rdf:ID="Stealing"><rdfs:subClassOf rdf:resource="http://reliant.teknowledge.com/DAML/SUMO.owl#UnilateralGetting" /><rdfs:subClassOf rdf:resource="#CriminalAction" /><rdfs:comment>Any UnilateralGetting which is not permitted by the 

origin of the UnilateralGetting.  These cases of UnilateralGetting are 

distinguished from ones where the destination is the subject of charity or 

other forms of benefaction.</rdfs:comment></rdfs:Class><rdfs:Class rdf:ID="SteamEngine"><rdfs:subClassOf rdf:resource="#Engine" /><rdfs:comment>SteamEngine is the subclass of Engines 

that produce mechanical power from heat and steam pressure.</rdfs:comment></rdfs:Class><rdfs:Class rdf:ID="Steel"><rdfs:subClassOf rdf:resource="#MetallicAlloy" /><rdfs:comment>A MetallicAlloy made from Iron and other elements.</rdfs:comment></rdfs:Class><rdfs:Class rdf:ID="Steeple"><rdfs:subClassOf rdf:resource="http://reliant.teknowledge.com/DAML/SUMO.owl#StationaryArtifact" /><rdfs:comment>A component of a ReligiousBuilding that is tall 

and narrow and symbolizes the connection between humanity and a deity.</rdfs:comment></rdfs:Class><rdfs:Class rdf:ID="SteeringWheel"><rdfs:subClassOf rdf:resource="#VehicleController" /><rdfs:comment>A VehicleController which enables one to steer 

a Vehicle.</rdfs:comment></rdfs:Class><rdfs:Class rdf:ID="SteppeClimateZone"><rdfs:subClassOf rdf:resource="#AridClimateZone" /><rdfs:comment>SteppeClimateZone 

is the class of AridClimateZones where the dominant 

vegetation type is grasses, with no trees.  Koeppen 

system 'BS'.</rdfs:comment></rdfs:Class><rdfs:Class rdf:ID="Stepping"><rdfs:subClassOf rdf:resource="http://reliant.teknowledge.com/DAML/SUMO.owl#BodyMotion" /><rdfs:comment>The BodyMotion of extending one foot forward 

and then bringing the other foot to the same lateral position as the 

first leg.</rdfs:comment></rdfs:Class><rdfs:Class rdf:ID="Steroid"><rdfs:subClassOf rdf:resource="#OrganicCompound" /><rdfs:subClassOf rdf:resource="http://reliant.teknowledge.com/DAML/SUMO.owl#BiologicallyActiveSubstance" /><rdfs:comment>A class of OrganicCompounds having the same basic 

chemical structure and having significant physiological effects.</rdfs:comment></rdfs:Class><rdfs:Class rdf:ID="Stimulant"><rdfs:subClassOf rdf:resource="http://reliant.teknowledge.com/DAML/SUMO.owl#BiologicallyActiveSubstance" /><sumo:disjoint rdf:resource="#Depressant" /><rdfs:comment>Any BiologicallyActiveSubstance which has 

the effect of stimulating the central nervous system, i.e. increasing 

function or activity in the Brain or SpinalCord.</rdfs:comment></rdfs:Class><rdfs:Class rdf:ID="Stirring"><rdfs:subClassOf rdf:resource="http://reliant.teknowledge.com/DAML/SUMO.owl#LiquidMotion" /><rdfs:subClassOf rdf:resource="http://reliant.teknowledge.com/DAML/SUMO.owl#Combining" /><rdfs:comment>Any instance of LiquidMotion which is also an 

instance of Combining two or more Liquids.</rdfs:comment></rdfs:Class><rdfs:Class rdf:ID="Stock"><rdfs:subClassOf rdf:resource="http://reliant.teknowledge.com/DAML/SUMO.owl#FinancialInstrument" /><rdfs:comment>An instrument that signifies an ownership position, 

or equity, in a Corporation, and represents a claim on its proportionate 

share in the corporation's assets and profits.</rdfs:comment></rdfs:Class><rdfs:Class rdf:ID="StockMarket"><rdfs:subClassOf rdf:resource="http://reliant.teknowledge.com/DAML/SUMO.owl#Organization" /><rdfs:comment>General term for organizations where stocks are traded, 

either in formal exchanges or over-the-counter.</rdfs:comment></rdfs:Class><rdfs:Class rdf:ID="Stomach"><rdfs:subClassOf rdf:resource="http://reliant.teknowledge.com/DAML/SUMO.owl#Organ" /><rdfs:subClassOf rdf:resource="http://reliant.teknowledge.com/DAML/SUMO.owl#AnimalAnatomicalStructure" /><rdfs:comment>A muscular sac that is the principal organ of 

digestion.</rdfs:comment></rdfs:Class><rdfs:Class rdf:ID="Store"><rdfs:subClassOf rdf:resource="http://reliant.teknowledge.com/DAML/SUMO.owl#Building" /><rdfs:comment>A Building that has the purpose of housing

FinancialTransactions.</rdfs:comment></rdfs:Class><rdfs:Class rdf:ID="StormFront"><rdfs:subClassOf rdf:resource="#AtmosphericRegion" /><rdfs:comment>The Region where two or more unstable air 

masses meet.</rdfs:comment></rdfs:Class><rdfs:Class rdf:ID="Stove"><rdfs:subClassOf rdf:resource="#HeatingDevice" /><rdfs:comment>A HeatingDevice which consists one or more burners for 

heating pots and pans of Food.</rdfs:comment></rdfs:Class><rdfs:Class rdf:ID="Strait"><rdfs:subClassOf rdf:resource="#BodyOfWater" /><rdfs:comment>Strait is the subclass of BodyOfWater that 

consists of narrow water areas connecting two larger bodies of water.  

Straits are naturally occurring bodies of water.</rdfs:comment></rdfs:Class><rdfs:Class rdf:ID="Strangling"><rdfs:subClassOf rdf:resource="http://reliant.teknowledge.com/DAML/SUMO.owl#Grabbing" /><rdfs:comment>Any instance of Grabbing where the patient is 

someone else's throat and the intention is to make it impossible for the other 

person to breathe.</rdfs:comment></rdfs:Class><rdfs:Class rdf:ID="Streetcar"><rdfs:subClassOf rdf:resource="#ElectrifiedRailwayCar" /><rdfs:comment>Streetcar is the subclass of 

ElectrifiedRailwayCars that run on tracks laid into, along, or 

beside city Streets.</rdfs:comment></rdfs:Class><rdfs:Class rdf:ID="Stretching"><rdfs:subClassOf rdf:resource="#Lengthening" /><rdfs:comment>Lengthening an object by pulling two sides 

of it in opposite directions.</rdfs:comment></rdfs:Class><rdfs:Class rdf:ID="String"><rdfs:subClassOf rdf:resource="http://reliant.teknowledge.com/DAML/SUMO.owl#Artifact" /><rdfs:comment>A long, thin strand of Fabric that is used for Tying 

things together, etc.  Note that this class covers a cord of any width, including 

rope, twine, and thread, for example.</rdfs:comment></rdfs:Class><rdfs:Class rdf:ID="StringInstrument"><rdfs:subClassOf rdf:resource="http://reliant.teknowledge.com/DAML/SUMO.owl#MusicalInstrument" /><rdfs:comment>A MusicalInstrument which is played by 

striking strings, either directly as with a guitar or indirectly via keys 

as with Pianos.</rdfs:comment></rdfs:Class><rdfs:Class rdf:ID="Submarine"><rdfs:subClassOf rdf:resource="#Watercraft" /><rdfs:comment>A Watercraft which is capable of travelling 

under the water level by filling tanks water.</rdfs:comment></rdfs:Class><rdfs:Class rdf:ID="SubtropicalDesertClimateZone"><rdfs:subClassOf rdf:resource="#DesertClimateZone" /><rdfs:comment>SubtropicalDesertClimateZone is a subclass of DesertClimateZone 

that is characterized by an average temperature greater than 18 

degrees Celsius, as well as very low rainfall.  This is Koeppen 

system 'BWh'.</rdfs:comment></rdfs:Class><rdfs:Class rdf:ID="SubwaySystem"><rdfs:subClassOf rdf:resource="#RailTransportationSystem" /><rdfs:comment>Any RailTransportationSystem that runs 

exclusively through Tunnels.</rdfs:comment></rdfs:Class><rdfs:Class rdf:ID="Suffocating"><rdfs:subClassOf rdf:resource="http://reliant.teknowledge.com/DAML/SUMO.owl#Killing" /><rdfs:comment>Killing someone by asphyxiation, i.e. by 

depriving them of oxygen.</rdfs:comment></rdfs:Class><rdfs:Class rdf:ID="Sugar"><rdfs:subClassOf rdf:resource="http://reliant.teknowledge.com/DAML/SUMO.owl#Carbohydrate" /><rdfs:comment>A simple Carbohydrate that has a sweet taste and 

consists mostly or entirely of sucrose.</rdfs:comment></rdfs:Class><rdfs:Class rdf:ID="Suicide"><rdfs:subClassOf rdf:resource="http://reliant.teknowledge.com/DAML/SUMO.owl#Killing" /><rdfs:comment>Any instance of Killing where the agent and 

the patient are identical.</rdfs:comment></rdfs:Class><rdfs:Class rdf:ID="SummerSeason"><rdfs:subClassOf rdf:resource="#SeasonOfYear" /><rdfs:comment>The SeasonOfYear that begins at the summer 

solstice and ends at the autumnal equinox.</rdfs:comment></rdfs:Class><rdfs:Class rdf:ID="Sunlight"><rdfs:subClassOf rdf:resource="http://reliant.teknowledge.com/DAML/SUMO.owl#RadiatingLight" /><rdfs:comment>Any instance of RadiatingLight where the 

Sun (Sol) is the origin.</rdfs:comment></rdfs:Class><rdfs:Class rdf:ID="Sunrise"><rdfs:subClassOf rdf:resource="http://reliant.teknowledge.com/DAML/SUMO.owl#TimeInterval" /><rdfs:comment>The TimeInterval of each Day when the sun is rising 

and is partially overlapped by the horizon line.</rdfs:comment></rdfs:Class><rdfs:Class rdf:ID="Sunset"><rdfs:subClassOf rdf:resource="http://reliant.teknowledge.com/DAML/SUMO.owl#TimeInterval" /><rdfs:comment>The TimeInterval of each Day when the sun is setting 

and is partially overlapped by the horizon line.</rdfs:comment></rdfs:Class><rdfs:Class rdf:ID="Supposition"><rdfs:subClassOf rdf:resource="http://reliant.teknowledge.com/DAML/SUMO.owl#Sentence" /><rdfs:comment>A Sentence that is assumed to be true, possibly 

just for the sake of argument.</rdfs:comment></rdfs:Class><rdfs:Class rdf:ID="SurfacedRoadway"><rdfs:subClassOf rdf:resource="http://reliant.teknowledge.com/DAML/SUMO.owl#Roadway" /><sumo:disjoint rdf:resource="#UnsurfacedRoadway" /><rdfs:comment>SurfacedRoadway is the subclass of 

Roadways that have been improved by covering them with a substance 

to increase the hardness and smoothness of the surface.  Covering 

materials include pavement, concrete, asphalt, macadam, and gravel.</rdfs:comment></rdfs:Class><rdfs:Class rdf:ID="Surgeon"><rdfs:subClassOf rdf:resource="#MedicalDoctor" /><rdfs:comment>The Profession of being a surgeon, i.e. being a 

medical doctor who specializes in performing surgical operations.</rdfs:comment></rdfs:Class><rdfs:Class rdf:ID="Swamp"><rdfs:subClassOf rdf:resource="http://reliant.teknowledge.com/DAML/SUMO.owl#StaticWaterArea" /><rdfs:comment>Swamp is a subclass of StaticWaterAreas that are 

stagnant and relatively shallow.  They are situated in low, wet land with 

grasses and possibly trees as vegetation.</rdfs:comment></rdfs:Class><rdfs:Class rdf:ID="Sweat"><rdfs:subClassOf rdf:resource="http://reliant.teknowledge.com/DAML/SUMO.owl#AnimalSubstance" /><rdfs:comment>An AnimalSubstance that contains SodiumChloride 

and is produced by the sweat glands.</rdfs:comment></rdfs:Class><rdfs:Class rdf:ID="Sweeping"><rdfs:subClassOf rdf:resource="http://reliant.teknowledge.com/DAML/SUMO.owl#Removing" /><rdfs:comment>Removing small particles from the floor by means of 

a Broom.</rdfs:comment></rdfs:Class><rdfs:Class rdf:ID="Swimming"><rdfs:subClassOf rdf:resource="http://reliant.teknowledge.com/DAML/SUMO.owl#BodyMotion" /><rdfs:comment>Any deliberate and controlled BodyMotion 

through water that is accomplished by an Organism.</rdfs:comment></rdfs:Class><rdfs:Class rdf:ID="SwimmingPool"><rdfs:subClassOf rdf:resource="#FluidContainer" /><rdfs:subClassOf rdf:resource="http://reliant.teknowledge.com/DAML/SUMO.owl#StationaryArtifact" /><rdfs:comment>A FluidContainer that is filled with Water 

and that is used for Swimming.</rdfs:comment></rdfs:Class><rdfs:Class rdf:ID="SwitchDevice"><rdfs:subClassOf rdf:resource="http://reliant.teknowledge.com/DAML/SUMO.owl#EngineeringComponent" /><rdfs:comment>An EngineeringComponent which is capable of turning 

an ElectricDevice on and off.</rdfs:comment></rdfs:Class><rdfs:Class rdf:ID="Sword"><rdfs:subClassOf rdf:resource="http://reliant.teknowledge.com/DAML/SUMO.owl#Weapon" /><rdfs:comment>A Weapon with a long blade and covered 

handle.</rdfs:comment></rdfs:Class><rdfs:Class rdf:ID="Syllable"><rdfs:subClassOf rdf:resource="http://reliant.teknowledge.com/DAML/SUMO.owl#SymbolicString" /><rdfs:comment>A sequence of Characters from the same Word 

that denote a single sound.</rdfs:comment></rdfs:Class><rdfs:Class rdf:ID="Table"><rdfs:subClassOf rdf:resource="#Furniture" /><rdfs:comment>A piece of Furniture that is elevated from the floor 

and has a flat top.  It is used for eating, paperwork, manual work, meetings, 

etc.</rdfs:comment></rdfs:Class><rdfs:Class rdf:ID="Tableware"><rdfs:subClassOf rdf:resource="http://reliant.teknowledge.com/DAML/SUMO.owl#Device" /><rdfs:comment>Devices that are used in Ingesting (Eating 

and/or Drinking) a meal.  This coves dishware, flatware, and glassware.</rdfs:comment></rdfs:Class><rdfs:Class rdf:ID="Tail"><rdfs:subClassOf rdf:resource="http://reliant.teknowledge.com/DAML/SUMO.owl#AnimalAnatomicalStructure" /><rdfs:comment>A BodyPart which extends from the rear of the 

main body of some Vertebrates.</rdfs:comment></rdfs:Class><rdfs:Class rdf:ID="Taillight"><rdfs:subClassOf rdf:resource="#VehicleLight" /><rdfs:comment>Any VehicleLight which is attached to the back 

of a Vehicle.</rdfs:comment></rdfs:Class><rdfs:Class rdf:ID="TakingIll"><rdfs:subClassOf rdf:resource="http://reliant.teknowledge.com/DAML/SUMO.owl#PathologicProcess" /><rdfs:comment>Any Process where the experiencer contracts a 

DiseaseOrSyndrome.</rdfs:comment></rdfs:Class><rdfs:Class rdf:ID="TakingOff"><rdfs:subClassOf rdf:resource="http://reliant.teknowledge.com/DAML/SUMO.owl#Translocation" /><rdfs:comment>Any instance of Translocation which starts 

on something other than an AtmosphericRegion and which has an instance 

of Flying as a subProcess.</rdfs:comment></rdfs:Class><rdfs:Class rdf:ID="Tape"><rdfs:subClassOf rdf:resource="http://reliant.teknowledge.com/DAML/SUMO.owl#AttachingDevice" /><rdfs:comment>A thin strip of Fabric or Paper that is used to attach 

two things.</rdfs:comment></rdfs:Class><rdfs:Class rdf:ID="Tavern"><rdfs:subClassOf rdf:resource="#Restaurant" /><rdfs:comment>A Restaurant whose primary service is selling 

AlcoholicBeverages to customers.</rdfs:comment></rdfs:Class><rdfs:Class rdf:ID="Tax"><rdfs:subClassOf rdf:resource="#ChargingAFee" /><rdfs:comment>A fee charged by a government on a product, income 

or activity.</rdfs:comment></rdfs:Class><rdfs:Class rdf:ID="TaxReturn"><rdfs:subClassOf rdf:resource="#FormText" /><rdfs:comment>A FormText that is used for calculating the amount 

of income tax owed in a given year.</rdfs:comment></rdfs:Class><rdfs:Class rdf:ID="Taxicab"><rdfs:subClassOf rdf:resource="#Automobile" /><rdfs:comment>An Automobile which is used to transport people 

on short trips in exchange for a fare.</rdfs:comment></rdfs:Class><rdfs:Class rdf:ID="Tea"><rdfs:subClassOf rdf:resource="http://reliant.teknowledge.com/DAML/SUMO.owl#Beverage" /><rdfs:subClassOf rdf:resource="#PreparedFood" /><rdfs:comment>A Beverage which is prepared by infusing tea leaves 

into hot water.</rdfs:comment></rdfs:Class><rdfs:Class rdf:ID="Teacher"><rdfs:subClassOf rdf:resource="#Profession" /><rdfs:comment>The Profession of being a teacher.</rdfs:comment></rdfs:Class><rdfs:Class rdf:ID="TeamSport"><rdfs:subClassOf rdf:resource="http://reliant.teknowledge.com/DAML/SUMO.owl#Sport" /><rdfs:comment>Any Sport which is played by SportsTeams, e.g. 

Baseball and Football.</rdfs:comment></rdfs:Class><rdfs:Class rdf:ID="TearSubstance"><rdfs:subClassOf rdf:resource="#LiquidBodySubstance" /><rdfs:subClassOf rdf:resource="#SalineSolution" /><rdfs:comment>The class of SalineSolutions produced by 

the lacrimal glands of the Eyes.</rdfs:comment></rdfs:Class><rdfs:Class rdf:ID="Teenager"><rdfs:subClassOf rdf:resource="#HumanYouth" /><rdfs:comment>A HumanYouth between puberty and the age of 19.</rdfs:comment></rdfs:Class><rdfs:Class rdf:ID="Telegraph"><rdfs:subClassOf rdf:resource="#ElectricDevice" /><rdfs:subClassOf rdf:resource="#CommunicationDevice" /><rdfs:comment>A Device that permits LinguisticCommunication 

between remote points by means of a code of aural dots and dashes that can 

be converted into letters of an alphabet.</rdfs:comment></rdfs:Class><rdfs:Class rdf:ID="Telephone"><rdfs:subClassOf rdf:resource="#ElectricDevice" /><rdfs:subClassOf rdf:resource="#CommunicationDevice" /><rdfs:comment>A Device that permits LinguisticCommunication 

between remote points by converting sound into electrical signals that are 

then transmitted.  When the signals are received, they are converted back 

into sound.</rdfs:comment></rdfs:Class><rdfs:Class rdf:ID="TelephoneLine"><rdfs:subClassOf rdf:resource="#WireLine" /><rdfs:comment>A WireLine that carries telephone signals and 

allows users of Telephones or Telegraphs to communicate with one another.</rdfs:comment></rdfs:Class><rdfs:Class rdf:ID="Telephoning"><rdfs:subClassOf rdf:resource="http://reliant.teknowledge.com/DAML/SUMO.owl#Speaking" /><rdfs:comment>Any instance of Speaking where the 

instrument of Communication is a Telephone.</rdfs:comment></rdfs:Class><rdfs:Class rdf:ID="TelevisionBroadcasting"><rdfs:subClassOf rdf:resource="#Broadcasting" /><rdfs:comment>Any instance of Broadcasting which 

is intended to be received by a TelevisionReceiver.</rdfs:comment></rdfs:Class><rdfs:Class rdf:ID="TelevisionReceiver"><rdfs:subClassOf rdf:resource="#ReceiverDevice" /><rdfs:comment>A TelevisionReceiver is a Device for 

receiving television broadcast signals from a TelevisionStation.</rdfs:comment></rdfs:Class><rdfs:Class rdf:ID="TelevisionStation"><rdfs:subClassOf rdf:resource="#BroadcastingStation" /><rdfs:comment>A TelevisionStation is a 

BroadcastingStation that broadcasts programs that are intended to be 

received by a TelevisionReceiver.</rdfs:comment></rdfs:Class><rdfs:Class rdf:ID="TellingALie"><rdfs:subClassOf rdf:resource="http://reliant.teknowledge.com/DAML/SUMO.owl#Stating" /><rdfs:comment>Any Stating which is both False and believed 

to be False by the agent of the Stating.</rdfs:comment></rdfs:Class><rdfs:Class rdf:ID="TemperateClimateZone"><rdfs:subClassOf rdf:resource="#ClimateZone" /><rdfs:comment>TemperateClimateZone is the 

subclass of ClimateZone whose warmest month has an average 

temperature greater than 10 degrees Celsius and whose coolest month 

has an average temperature between 18 degrees and -3 degrees Celsius. 

This is Class C in the Koeppen climate system.</rdfs:comment></rdfs:Class><rdfs:Class rdf:ID="TemperateSummerDryClimateZone"><rdfs:subClassOf rdf:resource="#TemperateClimateZone" /><rdfs:comment>TemperateSummerDryClimateZone is the subclass of TemperateClimateZone 

that is characterized by dry summers, and in which the wettest winter month 

has at least three times the moisture of the driest summer month.  The 

driest month has less than an average of 30 mm of precipitation.  Koeppen 

climate system type 'Cs'.</rdfs:comment></rdfs:Class><rdfs:Class rdf:ID="TemperateWinterDryClimateZone"><rdfs:subClassOf rdf:resource="#TemperateClimateZone" /><rdfs:comment>TemperateWinterDryClimateZone is a subclass of TemperateClimateZone 

characterized by having at least 10 times as much precipitation in the 

wettest summer month as in the driest winter month. Koeppen climate 

system type 'Cw'.</rdfs:comment></rdfs:Class><rdfs:Class rdf:ID="Tendon"><rdfs:subClassOf rdf:resource="http://reliant.teknowledge.com/DAML/SUMO.owl#Tissue" /><rdfs:subClassOf rdf:resource="http://reliant.teknowledge.com/DAML/SUMO.owl#AnimalSubstance" /><rdfs:comment>Tissue that connects Muscle to Bone.</rdfs:comment></rdfs:Class><rdfs:Class rdf:ID="Tent"><rdfs:subClassOf rdf:resource="#MobileResidence" /><rdfs:comment>A MobileResidence that is made of Fabric and poles and 

can be easily assembled and disassembled.</rdfs:comment></rdfs:Class><rdfs:Class rdf:ID="TerminalBuilding"><rdfs:subClassOf rdf:resource="http://reliant.teknowledge.com/DAML/SUMO.owl#Building" /><rdfs:comment>A TerminalBuilding is a Building 

located at a TransitTerminal and used in connection with its 

functions.</rdfs:comment></rdfs:Class><rdfs:Class rdf:ID="Tesla"><rdfs:subClassOf rdf:resource="http://reliant.teknowledge.com/DAML/SUMO.owl#FunctionQuantity" /><rdf:type rdf:resource="http://reliant.teknowledge.com/DAML/SUMO.owl#SystemeInternationalUnit" /><rdfs:comment>SI magnetic flux density measure.  Symbol:  T.

One Tesla equals one Weber per square Meter.  Tesla = Wb/m^2 = 

kg*s^(-2)*A^(-1).</rdfs:comment></rdfs:Class><rdfs:Class rdf:ID="TestForm"><rdfs:subClassOf rdf:resource="#FormText" /><rdfs:subClassOf rdf:resource="http://reliant.teknowledge.com/DAML/SUMO.owl#MeasuringDevice" /><rdfs:comment>A FormText which is intended to measure some aspect 

of the cognitive capabilities, e.g. intelligence or knowledge of a domain, 

of the person taking the test.</rdfs:comment></rdfs:Class><rdfs:Class rdf:ID="Testament"><rdfs:subClassOf rdf:resource="http://reliant.teknowledge.com/DAML/SUMO.owl#Certificate" /><rdfs:comment>A Certificate that describes how a person's 

property is to be distributed after the death of the person.</rdfs:comment></rdfs:Class><rdfs:Class rdf:ID="Testifying"><rdfs:subClassOf rdf:resource="http://reliant.teknowledge.com/DAML/SUMO.owl#Stating" /><rdfs:comment>Giving testimony as part of a JudicialProcess.</rdfs:comment></rdfs:Class><rdfs:Class rdf:ID="Thanking"><rdfs:subClassOf rdf:resource="#ExpressingApproval" /><rdfs:comment>Any ExpressingApproval to a person for something 

that the person did in the past and that is regarded as being to the thanker's 

benefit.</rdfs:comment></rdfs:Class><rdfs:Class rdf:ID="TheaterProfession"><rdfs:subClassOf rdf:resource="#EntertainmentProfession" /><rdfs:comment>Often know as the stage, Positions which 

involve performing live plays.</rdfs:comment></rdfs:Class><rdfs:Class rdf:ID="Thermometer"><rdfs:subClassOf rdf:resource="http://reliant.teknowledge.com/DAML/SUMO.owl#MeasuringDevice" /><rdfs:comment>Any Device that measures and represents 

TemperatureMeasure.</rdfs:comment></rdfs:Class><rdfs:Class rdf:ID="Threatening"><rdfs:subClassOf rdf:resource="http://reliant.teknowledge.com/DAML/SUMO.owl#Committing" /><rdfs:comment>Any Committing where the thing promised 

is something that is deemed undesirable by the destination of the 

Committing.</rdfs:comment></rdfs:Class><rdfs:Class rdf:ID="Throat"><rdfs:subClassOf rdf:resource="http://reliant.teknowledge.com/DAML/SUMO.owl#AnimalAnatomicalStructure" /><rdfs:subClassOf rdf:resource="http://reliant.teknowledge.com/DAML/SUMO.owl#BodyVessel" /><rdfs:comment>A BodyVessel which connects the Mouth to the 

lungs and stomach.</rdfs:comment></rdfs:Class><rdfs:Class rdf:ID="Throwing"><rdfs:subClassOf rdf:resource="http://reliant.teknowledge.com/DAML/SUMO.owl#Impelling" /><rdfs:subClassOf rdf:resource="http://reliant.teknowledge.com/DAML/SUMO.owl#BodyMotion" /><rdfs:comment>Any instance of Impelling where the instrument is 

an Arm.</rdfs:comment></rdfs:Class><rdfs:Class rdf:ID="Thumb"><rdfs:subClassOf rdf:resource="#Finger" /><rdfs:comment>The thick, short Finger of each Hand.</rdfs:comment></rdfs:Class><rdfs:Class rdf:ID="Thunder"><rdfs:subClassOf rdf:resource="http://reliant.teknowledge.com/DAML/SUMO.owl#WeatherProcess" /><rdfs:subClassOf rdf:resource="http://reliant.teknowledge.com/DAML/SUMO.owl#RadiatingSound" /><rdfs:comment>Any instance of RadiatingSound which is caused by 

an instance of Lightning.</rdfs:comment></rdfs:Class><rdfs:Class rdf:ID="ThyroidGland"><rdfs:subClassOf rdf:resource="#Gland" /><rdfs:comment>A Gland in the neck that produces 

ThyroidHormone, which regulates body weight, metabolic rate, etc.</rdfs:comment></rdfs:Class><rdfs:Class rdf:ID="ThyroidHormone"><rdfs:subClassOf rdf:resource="#Hormone" /><rdfs:comment>A Hormone secreted by the ThyroidGland.</rdfs:comment></rdfs:Class><rdfs:Class rdf:ID="Ticket"><rdfs:subClassOf rdf:resource="http://reliant.teknowledge.com/DAML/SUMO.owl#Certificate" /><rdfs:comment>A Certificate that allows the holder to perform 

a specified act once, e.g. ride a bus, attend a concert, obtain a prize, 

etc.</rdfs:comment></rdfs:Class><rdfs:Class rdf:ID="TidalProcess"><rdfs:subClassOf rdf:resource="http://reliant.teknowledge.com/DAML/SUMO.owl#InternalChange" /><rdfs:comment>TidalProcess is the class of daily 

recurring events in which the water level in a BodyOfWater rises 

and falls with the changing position between Earth and the Moon.</rdfs:comment></rdfs:Class><rdfs:Class rdf:ID="TieClothing"><rdfs:subClassOf rdf:resource="http://reliant.teknowledge.com/DAML/SUMO.owl#Clothing" /><rdfs:comment>Clothing that is intended to be worn around the 

Neck and knotted at the front.</rdfs:comment></rdfs:Class><rdfs:Class rdf:ID="Tilling"><rdfs:subClassOf rdf:resource="#Digging" /><rdfs:comment>Any Process of Digging, e.g. breaking and 

turning over the earth that facilitates Agriculture.</rdfs:comment></rdfs:Class><rdfs:Class rdf:ID="Tin"><rdfs:subClassOf rdf:resource="http://reliant.teknowledge.com/DAML/SUMO.owl#ElementalSubstance" /><atomicNumber>50</atomicNumber><rdfs:comment>Silvery malleable metallic element belonging to group 

14 of the periodic table.  Twenty-six isotopes are known, five of which 

are radioactive.  Chemically reactive.  Combines directly with chlorine 

and oxygen and displaces hydrogen from dilute acids.  </rdfs:comment></rdfs:Class><rdfs:Class rdf:ID="Toad"><rdfs:subClassOf rdf:resource="http://reliant.teknowledge.com/DAML/SUMO.owl#Amphibian" /><rdfs:comment>An Amphibian that lacks a Tail and lives at least 

partially outside of water.</rdfs:comment></rdfs:Class><rdfs:Class rdf:ID="Tobacco"><rdfs:subClassOf rdf:resource="http://reliant.teknowledge.com/DAML/SUMO.owl#FloweringPlant" /><rdfs:comment>A FloweringPlant containing nicotine whose leaves 

are dried and then smoked or ingested.</rdfs:comment></rdfs:Class><rdfs:Class rdf:ID="Toe"><rdfs:subClassOf rdf:resource="#DigitAppendage" /><rdfs:comment>The five extremities of a Foot.</rdfs:comment></rdfs:Class><rdfs:Class rdf:ID="Toilet"><rdfs:subClassOf rdf:resource="http://reliant.teknowledge.com/DAML/SUMO.owl#Device" /><rdfs:comment>A Device for urination and defecation.</rdfs:comment></rdfs:Class><rdfs:Class rdf:ID="Tomb"><rdfs:subClassOf rdf:resource="http://reliant.teknowledge.com/DAML/SUMO.owl#StationaryArtifact" /><rdfs:comment>A StationaryArtifact which is meant to contain someone 

who is Dead.</rdfs:comment></rdfs:Class><rdfs:Class rdf:ID="TonMass"><rdfs:subClassOf rdf:resource="http://reliant.teknowledge.com/DAML/SUMO.owl#MassMeasure" /><rdf:type rdf:resource="http://reliant.teknowledge.com/DAML/SUMO.owl#UnitOfMeasure" /><rdfs:comment>English mass unit that is equal to 2000 pounds.</rdfs:comment></rdfs:Class><rdfs:Class rdf:ID="TonalLanguage"><rdfs:subClassOf rdf:resource="http://reliant.teknowledge.com/DAML/SUMO.owl#SpokenHumanLanguage" /><rdfs:comment>Any SpokenHumanLanguage that uses pitch to 

differentiate otherwise identical words, e.g. Chinese.</rdfs:comment></rdfs:Class><rdfs:Class rdf:ID="Tongue"><rdfs:subClassOf rdf:resource="http://reliant.teknowledge.com/DAML/SUMO.owl#AnimalAnatomicalStructure" /><rdfs:subClassOf rdf:resource="http://reliant.teknowledge.com/DAML/SUMO.owl#BodyPart" /><rdfs:comment>Part of the Mouth, used for Tasting Food, 

Vocalizing, and the initial stage of Digesting.</rdfs:comment></rdfs:Class><rdfs:Class rdf:ID="Tooth"><rdfs:subClassOf rdf:resource="http://reliant.teknowledge.com/DAML/SUMO.owl#Bone" /><rdfs:comment>Part of the Mouth, used for biting and chewing.</rdfs:comment></rdfs:Class><rdfs:Class rdf:ID="Torso"><rdfs:subClassOf rdf:resource="http://reliant.teknowledge.com/DAML/SUMO.owl#AnimalAnatomicalStructure" /><rdfs:subClassOf rdf:resource="http://reliant.teknowledge.com/DAML/SUMO.owl#BodyPart" /><rdfs:comment>The body of a Primate excluding its Limbs.</rdfs:comment></rdfs:Class><rdfs:Class rdf:ID="Towel"><rdfs:subClassOf rdf:resource="#FabricArtifact" /><rdfs:comment>A piece of Fabric which is used for Drying.</rdfs:comment></rdfs:Class><rdfs:Class rdf:ID="Tracing"><rdfs:subClassOf rdf:resource="http://reliant.teknowledge.com/DAML/SUMO.owl#ContentDevelopment" /><rdfs:subClassOf rdf:resource="http://reliant.teknowledge.com/DAML/SUMO.owl#SurfaceChange" /><rdfs:comment>Any ContentDevelopment that results in a Blueprint.</rdfs:comment></rdfs:Class><rdfs:Class rdf:ID="TractorTrailer"><rdfs:subClassOf rdf:resource="#RoadVehicle" /><rdfs:comment>TractorTrailer is the subclass of 

RoadVehicles that are truck tractor- truck trailer combinations.</rdfs:comment></rdfs:Class><rdfs:Class rdf:ID="Trailer"><rdfs:subClassOf rdf:resource="#RoadVehicle" /><sumo:disjoint rdf:resource="#SelfPoweredVehicle" /><sumo:disjoint rdf:resource="#UserPoweredVehicle" /><rdfs:comment>Trailer is the class of RoadVehicles that 

are designed for towing with another RoadVehicle.</rdfs:comment></rdfs:Class><rdfs:Class rdf:ID="Train"><rdfs:subClassOf rdf:resource="#RailwayVehicle" /><rdfs:subClassOf rdf:resource="#SelfPoweredVehicle" /><rdfs:subClassOf rdf:resource="http://reliant.teknowledge.com/DAML/SUMO.owl#Collection" /><rdfs:comment>Train is the subclass of TransportationDevice 

whose instances are linked sequences of RollingStock whose motion is 

driven by one or more Locomotives or MotorizedRailwayCars.</rdfs:comment></rdfs:Class><rdfs:Class rdf:ID="TrainStation"><rdfs:subClassOf rdf:resource="#TerminalBuilding" /><rdfs:comment>TrainStation is the subclass of 

Buildings that are located at a RailwayTerminal and used in support  

of its functions, especially for the handling of passengers and freight.</rdfs:comment></rdfs:Class><rdfs:Class rdf:ID="Transducer"><rdfs:subClassOf rdf:resource="http://reliant.teknowledge.com/DAML/SUMO.owl#Machine" /><rdfs:comment>A Device which is capable of converting one form of 

energy into another.</rdfs:comment></rdfs:Class><rdfs:Class rdf:ID="TransferringPosition"><rdfs:subClassOf rdf:resource="http://reliant.teknowledge.com/DAML/SUMO.owl#OrganizationalProcess" /><rdfs:comment>Any process within an Organization 

where a person is moved from one Position to another, e.g. the promotion 

or demotion of an employee.</rdfs:comment></rdfs:Class><rdfs:Class rdf:ID="TransitTerminal"><rdfs:subClassOf rdf:resource="http://reliant.teknowledge.com/DAML/SUMO.owl#StationaryArtifact" /><rdfs:comment>A TransitTerminal is a place where 

travellers or transportation devices begin or end their journeys, or 

where passengers and/or goods may be transferred.  At a terminal, 

Vehicles may be received, assigned, sent out, or 

stored.</rdfs:comment></rdfs:Class><rdfs:Class rdf:about="http://reliant.teknowledge.com/DAML/SUMO.owl#Transitway"><rdfs:subClassOf rdf:resource="http://reliant.teknowledge.com/DAML/SUMO.owl#Region" /><rdfs:subClassOf rdf:resource="http://reliant.teknowledge.com/DAML/SUMO.owl#SelfConnectedObject" /><rdfs:comment>Transitway is the broadest class 

of regions which may be passed through as a path in instances 

of Translocation.  Transitway includes land, air, and sea 

regions, and it includes both natural and artificial transitways.</rdfs:comment></rdfs:Class><rdfs:Class rdf:ID="TransitwayJunction"><rdfs:subClassOf rdf:resource="http://reliant.teknowledge.com/DAML/SUMO.owl#Transitway" /><rdfs:comment>TransitwayJunction is the class of 

regions where two or more Transitways meet and traffic may transfer 

from one transitway to another.</rdfs:comment></rdfs:Class><rdfs:Class rdf:ID="TransportationCompany"><rdfs:subClassOf rdf:resource="http://reliant.teknowledge.com/DAML/SUMO.owl#CommercialAgent" /><rdfs:comment>A CommercialAgent whose services 

include Transportation, e.g. a RailroadCompany, an airline, a cruise 

ship line, etc.</rdfs:comment></rdfs:Class><rdfs:Class rdf:ID="TransportationSystem"><rdfs:subClassOf rdf:resource="http://reliant.teknowledge.com/DAML/SUMO.owl#Object" /><rdfs:comment>TransportationSystem is the 

subclass of complex Objects consisting of networks of Transitways 

and TransitJunctions that link together a number of GeographicRegions 

or TransitTerminals.  TransportationSystem covers worldwide 

networks, such as internationally recognized shipping lanes or air 

corridors, also route systems such as those flown by a single airline, 

as well as LocalTransitSystems such as BART (Bay Area Rapid Transit).</rdfs:comment></rdfs:Class><rdfs:Class rdf:ID="TrapOrCage"><rdfs:subClassOf rdf:resource="#Holder" /><rdfs:comment>A Device whose purpose is to trap or cage Animals, 

i.e. to be in instrument in an act of Confining.</rdfs:comment></rdfs:Class><rdfs:Class rdf:ID="TravelContainer"><rdfs:subClassOf rdf:resource="#Container" /><rdfs:comment>Any Container which is intended to be 

used for carrying personal effects from one point to another.  This class 

covers suitcases, briefcases, backpacks, etc.</rdfs:comment></rdfs:Class><rdfs:Class rdf:ID="Tray"><rdfs:subClassOf rdf:resource="#Holder" /><rdfs:comment>A Holder that is designed for Food, dishes, and 

flatware.</rdfs:comment></rdfs:Class><rdfs:Class rdf:ID="Treasurer"><rdfs:subClassOf rdf:resource="#SkilledOccupation" /><rdfs:comment>Any SkilledOccupation which involves receiving 

and disbursing money.</rdfs:comment></rdfs:Class><rdfs:Class rdf:ID="TreeBranch"><rdfs:subClassOf rdf:resource="#PlantBranch" /><rdfs:comment>Any PlantBranch which is part of a 

BotanicalTree.</rdfs:comment></rdfs:Class><rdfs:Class rdf:ID="TreeGraph"><rdfs:subClassOf rdf:resource="#Graph" /><rdfs:comment>A TreeGraph is a DirectedGraph that has no 

GraphLoops.</rdfs:comment></rdfs:Class><rdfs:Class rdf:ID="Trembling"><rdfs:subClassOf rdf:resource="http://reliant.teknowledge.com/DAML/SUMO.owl#BodyMotion" /><rdfs:subClassOf rdf:resource="#Tremor" /><sumo:disjoint rdf:resource="http://reliant.teknowledge.com/DAML/SUMO.owl#IntentionalProcess" /><rdfs:comment>Any BodyMotion which is involuntary and which is 

repeated many times over a short time frame, e.g. a spasm in the hands.</rdfs:comment></rdfs:Class><rdfs:Class rdf:ID="Tremor"><rdfs:subClassOf rdf:resource="#Rotating" /><rdfs:comment>Motion that involves rapidly Rotating between 

two positions.</rdfs:comment></rdfs:Class><rdfs:Class rdf:ID="Trespassing"><rdfs:subClassOf rdf:resource="#CriminalAction" /><rdfs:subClassOf rdf:resource="http://reliant.teknowledge.com/DAML/SUMO.owl#Translocation" /><rdfs:comment>Entering property that does not belong to one and without 

the permission of the owner of the property.</rdfs:comment></rdfs:Class><rdfs:Class rdf:ID="Triangle"><rdfs:subClassOf rdf:resource="#Polygon" /><rdfs:comment>Any three-sided Polygon.</rdfs:comment></rdfs:Class><rdfs:Class rdf:ID="TropicalClimateZone"><rdfs:subClassOf rdf:resource="#ClimateZone" /><rdfs:comment>TropicalClimateZone is a  

subclass of ClimateZone in which the average temperature of the 

coldest month is greater than 18 degrees Celsius.  This is Class 

'A' in the Koeppen climate classification system.</rdfs:comment></rdfs:Class><rdfs:Class rdf:ID="Trousers"><rdfs:subClassOf rdf:resource="http://reliant.teknowledge.com/DAML/SUMO.owl#Clothing" /><rdfs:comment>A piece of Clothing that covers each Leg 

of a person separately.</rdfs:comment></rdfs:Class><rdfs:Class rdf:ID="Truck"><rdfs:subClassOf rdf:resource="#SelfPoweredRoadVehicle" /><rdfs:comment>Truck is the subclass of RoadVehicles that 

are designed primarily for transporting various kinds of non-passenger 

loads.  Truck is the class of single-bodied trucks or TruckTractors.  

Note: TractorTrailer combinations are a distinct class.</rdfs:comment></rdfs:Class><rdfs:Class rdf:ID="TruckTractor"><rdfs:subClassOf rdf:resource="#Truck" /><rdfs:comment>TruckTractor is the subclass of Trucks 

that are used to tow truck trailers.  Truck tractors are the cab portions 

of tractor-trailers.  See also TruckTrailer.</rdfs:comment></rdfs:Class><rdfs:Class rdf:ID="TruckTrailer"><rdfs:subClassOf rdf:resource="#Trailer" /><rdfs:comment>TruckTrailer is the subclass of Trailers 

that are towed by TruckTractors.  These are the trailers used in 

tractor-trailer (semi-trailer) rigs.</rdfs:comment></rdfs:Class><rdfs:Class rdf:ID="Tube"><rdfs:subClassOf rdf:resource="http://reliant.teknowledge.com/DAML/SUMO.owl#Artifact" /><rdfs:comment>A long, narrow, and hollow Artifact that is designed for 

moving Fluids from place to another.</rdfs:comment></rdfs:Class><rdfs:Class rdf:ID="Tumor"><rdfs:subClassOf rdf:resource="http://reliant.teknowledge.com/DAML/SUMO.owl#AbnormalAnatomicalStructure" /><rdfs:comment>Any AbnormalAnatomicalStructure which consists of a 

mass of Tissue.  Note that this class covers both malignant (i.e. cancerous) 

and benign tumors.</rdfs:comment></rdfs:Class><rdfs:Class rdf:ID="TundraClimateZone"><rdfs:subClassOf rdf:resource="#PolarClimateZone" /><rdfs:comment>TundraClimateZone is a subclass of 

PolarClimateZone characterized by having an average temperature 

above zero degrees Celsius (but below 10 degrees) in the warmest month.  

Koeppen subtype 'ET'.</rdfs:comment></rdfs:Class><rdfs:Class rdf:ID="Tunnel"><rdfs:subClassOf rdf:resource="http://reliant.teknowledge.com/DAML/SUMO.owl#LandTransitway" /><rdfs:subClassOf rdf:resource="http://reliant.teknowledge.com/DAML/SUMO.owl#StationaryArtifact" /><rdfs:comment>Tunnel is a subclass of Transitways that 

consist of a lengthwise enclosed Hole that allows for transit 

underground, as through mountains, below a body of water, or beneath a 

city.</rdfs:comment></rdfs:Class><rdfs:Class rdf:ID="Turbine"><rdfs:subClassOf rdf:resource="#Engine" /><rdfs:comment>An Engine which converts the kinetic energy of a moving 

Liquid (typically Water) into mechanical energy.</rdfs:comment></rdfs:Class><rdfs:Class rdf:ID="TurningOffDevice"><rdfs:subClassOf rdf:resource="http://reliant.teknowledge.com/DAML/SUMO.owl#InternalChange" /><rdfs:comment>Any Process whose result is that the patient 

of the process is in the state of DeviceOff.  In other words, this class covers 

any process of turning off a device, e.g. turning off the lights, switching off a 

television set, etc.</rdfs:comment></rdfs:Class><rdfs:Class rdf:ID="TurningOnDevice"><rdfs:subClassOf rdf:resource="http://reliant.teknowledge.com/DAML/SUMO.owl#InternalChange" /><rdfs:comment>Any Process whose result is that the patient 

of the process is in the state of DeviceOn.  In other words, this class covers 

any process of turning on a device, e.g. turning on the lights, switching on a 

television set, etc.</rdfs:comment></rdfs:Class><rdfs:Class rdf:ID="Tying"><rdfs:subClassOf rdf:resource="http://reliant.teknowledge.com/DAML/SUMO.owl#Attaching" /><rdfs:comment>The Process of tying two things, or two strands of 

the same thing, together.</rdfs:comment></rdfs:Class><rdfs:Class rdf:ID="UnionOrganization"><rdfs:subClassOf rdf:resource="http://reliant.teknowledge.com/DAML/SUMO.owl#Organization" /><rdfs:comment>An Organization comprised of workers from 

the same Corporation or Industry.  The purpose of the UnionOrganization 

is to strengthen its representation in bargaining with the Corporation or 

Industry.</rdfs:comment></rdfs:Class><rdfs:Class rdf:ID="UnionSoldier"><rdfs:subClassOf rdf:resource="#Soldier" /><rdfs:comment>Any Soldier that served on the union side during 

the American Civil War.</rdfs:comment></rdfs:Class><rdfs:Class rdf:ID="UnitedKingdomGallon"><rdfs:subClassOf rdf:resource="http://reliant.teknowledge.com/DAML/SUMO.owl#VolumeMeasure" /><rdf:type rdf:resource="http://reliant.teknowledge.com/DAML/SUMO.owl#UnitOfMeasure" /><sumo:relatedInternalConcept rdf:resource="http://reliant.teknowledge.com/DAML/SUMO.owl#UnitedStatesGallon" /><rdfs:comment>Unit of volume commonly used in the 

United Kingdom.</rdfs:comment></rdfs:Class><rdfs:Class rdf:ID="University"><rdfs:subClassOf rdf:resource="#PostSecondarySchool" /><rdfs:comment>A School which admits students that 

have graduated from high school (known as undergraduate students) and 

students who have received a bachelor's degree (known as graduate 

students).  A University confers both bachelor's and graduate 

degrees.</rdfs:comment></rdfs:Class><rdfs:Class rdf:ID="UnskilledOccupation"><rdfs:subClassOf rdf:resource="#ManualLabor" /><sumo:disjoint rdf:resource="#SkilledOccupation" /><rdfs:comment>Any Position which does not 

require learning a set of skills.</rdfs:comment></rdfs:Class><rdfs:Class rdf:ID="UnsurfacedRoadway"><rdfs:subClassOf rdf:resource="http://reliant.teknowledge.com/DAML/SUMO.owl#Roadway" /><rdfs:comment>UnsurfacedRoadway is the subclass 

of Roadways that have natural, unimproved surfaces of dirt or sand.</rdfs:comment></rdfs:Class><rdfs:Class rdf:ID="Untying"><rdfs:subClassOf rdf:resource="http://reliant.teknowledge.com/DAML/SUMO.owl#Detaching" /><sumo:disjoint rdf:resource="#Tying" /><rdfs:comment>The Process of untying two things, or two strands 

of the same thing.</rdfs:comment></rdfs:Class><rdfs:Class rdf:ID="UplandArea"><rdfs:subClassOf rdf:resource="#LandForm" /><rdfs:comment>An UplandArea is a LandArea elevated above the surrounding terrain.</rdfs:comment></rdfs:Class><rdfs:Class rdf:ID="Urea"><rdfs:subClassOf rdf:resource="#OrganicCompound" /><rdfs:comment>Urea is a dry, soluble, nitrogenous substance 

that is the major solid component of the urine of mammals, and which 

may be synthesized from ammonia and carbon dioxide; it is useful in the 

production of Plastic and in Fertilizers.</rdfs:comment></rdfs:Class><rdfs:Class rdf:ID="UserPoweredDevice"><rdfs:subClassOf rdf:resource="#Engine" /><rdfs:comment>UserPoweredDevice is a subclass of 

Engine that perform work when a power input is supplied by the user.</rdfs:comment></rdfs:Class><rdfs:Class rdf:ID="UserPoweredVehicle"><rdfs:subClassOf rdf:resource="http://reliant.teknowledge.com/DAML/SUMO.owl#Vehicle" /><rdfs:subClassOf rdf:resource="#UserPoweredDevice" /><rdfs:comment>UserPoweredVehicle is the subclass of 

Vehicles whose power source is the rider or user.  Examples: Bicycles, 

Canoes, grocery carts.</rdfs:comment></rdfs:Class><rdfs:Class rdf:ID="UsingAnAccount"><rdfs:subClassOf rdf:resource="http://reliant.teknowledge.com/DAML/SUMO.owl#FinancialTransaction" /><rdfs:comment>An activity of using a financial account</rdfs:comment></rdfs:Class><rdfs:Class rdf:ID="Vacationing"><rdfs:subClassOf rdf:resource="http://reliant.teknowledge.com/DAML/SUMO.owl#RecreationOrExercise" /><rdfs:comment>Taking time off from one's occupation.</rdfs:comment></rdfs:Class><rdfs:Class rdf:ID="VehicleBrake"><rdfs:subClassOf rdf:resource="#VehicleController" /><rdfs:comment>A VehicleController which is capable of stopping 

the motion of a Vehicle.</rdfs:comment></rdfs:Class><rdfs:Class rdf:ID="VehicleController"><rdfs:subClassOf rdf:resource="http://reliant.teknowledge.com/DAML/SUMO.owl#Device" /><rdfs:comment>Any Device which is used to start, stop or 

control the movements of a Vehicle.  This class covers steering wheels, brakes, 

acceleration pedals, airplane sticks, etc.</rdfs:comment></rdfs:Class><rdfs:Class rdf:ID="VehicleLight"><rdfs:subClassOf rdf:resource="#IlluminationDevice" /><rdfs:comment>Any IlluminationDevice which is attached to the 

surface of a Vehicle and whose purpose is to illuminate that area around 

the Vehicle so that potential obstacles can be detected or alerted.</rdfs:comment></rdfs:Class><rdfs:Class rdf:ID="VehicleThrottle"><rdfs:subClassOf rdf:resource="#VehicleController" /><rdfs:comment>A VehicleController which controls the amount 

of Fuel which is supplied to the Engine.</rdfs:comment></rdfs:Class><rdfs:Class rdf:ID="VehicleTire"><rdfs:subClassOf rdf:resource="http://reliant.teknowledge.com/DAML/SUMO.owl#Artifact" /><rdfs:comment>A covering, usually made of rubber, for a Wheel.</rdfs:comment></rdfs:Class><rdfs:Class rdf:ID="VehicleWheel"><rdfs:subClassOf rdf:resource="#Wheel" /><rdfs:comment>VehicleWheel is a class of cylindrical 

Devices used to move a RoadVehicle along a road, running either  

directly on the wheel rims or on tires attached to the wheel rims.</rdfs:comment></rdfs:Class><rdfs:Class rdf:ID="VehicleWindow"><rdfs:subClassOf rdf:resource="#Window" /><rdfs:comment>Any Window which is part of a Vehicle, 

e.g. the Windshield and RearWindow of an Automobile.</rdfs:comment></rdfs:Class><rdfs:Class rdf:ID="Vein"><rdfs:subClassOf rdf:resource="#BloodVessel" /><sumo:relatedInternalConcept rdf:resource="#Artery" /><rdfs:comment>Any BloodVessel which transfers Blood from 

the extremities of the body to the Heart.</rdfs:comment></rdfs:Class><rdfs:Class rdf:ID="VendingDevice"><rdfs:subClassOf rdf:resource="http://reliant.teknowledge.com/DAML/SUMO.owl#Device" /><rdfs:comment>A Device which is capable of Selling a Product 

to a customer automatically when the customer inserts the appropriate amount of 

Currency.</rdfs:comment></rdfs:Class><rdfs:Class rdf:ID="Violin"><rdfs:subClassOf rdf:resource="#StringInstrument" /><rdfs:comment>A StringInstrument that has four strings, a hollow 

body, and is played on the shoulder with a bow.</rdfs:comment></rdfs:Class><rdfs:Class rdf:ID="ViralDisease"><rdfs:subClassOf rdf:resource="#InfectiousDisease" /><rdfs:comment>A disease that is caused by instances of 

Virus.</rdfs:comment></rdfs:Class><rdfs:Class rdf:ID="VocalMusic"><rdfs:subClassOf rdf:resource="http://reliant.teknowledge.com/DAML/SUMO.owl#Music" /><rdfs:comment>Music which is produced (at least in part)

by Singing.</rdfs:comment></rdfs:Class><rdfs:Class rdf:ID="VocationalSchool"><rdfs:subClassOf rdf:resource="#School" /><rdfs:comment>Any School whose aim is to teach 

students an OccupationalTrade.</rdfs:comment></rdfs:Class><rdfs:Class rdf:ID="Volt"><rdfs:subClassOf rdf:resource="http://reliant.teknowledge.com/DAML/SUMO.owl#FunctionQuantity" /><rdf:type rdf:resource="http://reliant.teknowledge.com/DAML/SUMO.owl#SystemeInternationalUnit" /><rdfs:comment>SI electric potential measure.  Symbol: V.  It is 

the difference of electric potential between two points of a conducting 

wire carrying a constant current of 1 Ampere, when the power dissipated 

between these points is equal to 1 Watt.  Volt = W/A = 

m^2*kg*s^(-3)*A^(-1).</rdfs:comment></rdfs:Class><rdfs:Class rdf:ID="VotingPoll"><rdfs:subClassOf rdf:resource="http://reliant.teknowledge.com/DAML/SUMO.owl#StationaryArtifact" /><rdfs:comment>A structure where Voting for an Election 

takes place.</rdfs:comment></rdfs:Class><rdfs:Class rdf:ID="Vowel"><rdfs:subClassOf rdf:resource="#AlphabeticCharacter" /><rdfs:comment>An AlphabeticCharacter that denotes a speech sound that 

does not result in audible friction when it is pronounced.</rdfs:comment></rdfs:Class><rdfs:Class rdf:ID="Vulture"><rdfs:subClassOf rdf:resource="http://reliant.teknowledge.com/DAML/SUMO.owl#Bird" /><rdfs:comment>A diurnal bird of prey with a bald head that 

feeds on carrion.</rdfs:comment></rdfs:Class><rdfs:Class rdf:ID="Wading"><rdfs:subClassOf rdf:resource="http://reliant.teknowledge.com/DAML/SUMO.owl#Walking" /><rdfs:comment>Any instance of Walking which occurs through a 

BodyOfWater.</rdfs:comment></rdfs:Class><rdfs:Class rdf:ID="Wagon"><rdfs:subClassOf rdf:resource="#LandVehicle" /><rdfs:comment>A Landcraft that is not self-propelled, but must be 

pulled by either an Animal or a self-propelled Vehicle to move along the 

ground.</rdfs:comment></rdfs:Class><rdfs:Class rdf:ID="WakingUp"><rdfs:subClassOf rdf:resource="http://reliant.teknowledge.com/DAML/SUMO.owl#PsychologicalProcess" /><rdfs:comment>The process of transitioning from a state of being 

Asleep to a state of being Awake.</rdfs:comment></rdfs:Class><rdfs:Class rdf:ID="WalkingCane"><rdfs:subClassOf rdf:resource="http://reliant.teknowledge.com/DAML/SUMO.owl#Device" /><rdfs:comment>A Device which has the form of a staff with 

a handle and which enables some people to walk with greater assurance.</rdfs:comment></rdfs:Class><rdfs:Class rdf:ID="Wall"><rdfs:subClassOf rdf:resource="http://reliant.teknowledge.com/DAML/SUMO.owl#StationaryArtifact" /><rdfs:comment>A StationaryArtifact that supports a Building or 

partitions it into Rooms.</rdfs:comment></rdfs:Class><rdfs:Class rdf:ID="Wallpaper"><rdfs:subClassOf rdf:resource="http://reliant.teknowledge.com/DAML/SUMO.owl#ArtWork" /><rdfs:comment>Any decorative paper that is used to cover the 

Walls of Rooms.</rdfs:comment></rdfs:Class><rdfs:Class rdf:ID="Warehouse"><rdfs:subClassOf rdf:resource="#CommercialBuilding" /><rdfs:comment>A very large CommercialBuilding whose purpose is 

to store commodities.</rdfs:comment></rdfs:Class><rdfs:Class rdf:ID="WashBasin"><rdfs:subClassOf rdf:resource="#WashingDevice" /><rdfs:comment>A WashingDevice which is intended to be used by 

Humans for washing their Hands.</rdfs:comment></rdfs:Class><rdfs:Class rdf:ID="Washing"><rdfs:subClassOf rdf:resource="http://reliant.teknowledge.com/DAML/SUMO.owl#Removing" /><rdfs:comment>Removing small particles from something by means of 

a Detergent and Water.</rdfs:comment></rdfs:Class><rdfs:Class rdf:ID="WashingDevice"><rdfs:subClassOf rdf:resource="http://reliant.teknowledge.com/DAML/SUMO.owl#Device" /><rdfs:comment>Any Device whose purpose is Washing 

something, e.g. washing machines, dishwashers, bathtubs, etc.</rdfs:comment></rdfs:Class><rdfs:Class rdf:ID="Wastebasket"><rdfs:subClassOf rdf:resource="#Container" /><rdfs:comment>A Container which is used for trash.</rdfs:comment></rdfs:Class><rdfs:Class rdf:ID="WatchClock"><rdfs:subClassOf rdf:resource="#Clock" /><rdfs:comment>A Clock that can be worn on the Wrist.</rdfs:comment></rdfs:Class><rdfs:Class rdf:ID="WaterMotion"><rdfs:subClassOf rdf:resource="http://reliant.teknowledge.com/DAML/SUMO.owl#LiquidMotion" /><rdfs:comment>Any LiquidMotion where the Liquid is Water.</rdfs:comment></rdfs:Class><rdfs:Class rdf:ID="WaterTransportation"><rdfs:subClassOf rdf:resource="http://reliant.teknowledge.com/DAML/SUMO.owl#Transportation" /><rdfs:comment>Any instance of Transportation where 

the instrument is a Watercraft.</rdfs:comment></rdfs:Class><rdfs:Class rdf:ID="WaterWave"><rdfs:subClassOf rdf:resource="#WaterMotion" /><rdfs:comment>A WaterWave is a raised ridge of water 

moving along the surface of a body of water.  The WaterWave moves 

in a direction approximately transverse to the crest line of the wave.  

The patient of the WaterWave is successive regions of water, which 

do not travel in the direction of the wave or with it.</rdfs:comment></rdfs:Class><rdfs:Class rdf:ID="WatercolorPaint"><rdfs:subClassOf rdf:resource="#Paint" /><rdfs:comment>Any Paint which is a water-based Solution.</rdfs:comment></rdfs:Class><rdfs:Class rdf:ID="WatercolorPicture"><rdfs:subClassOf rdf:resource="#PaintedPicture" /><rdfs:comment>Any PaintedPicture which is created 

with water-based paints.</rdfs:comment></rdfs:Class><rdfs:Class rdf:ID="Watercraft"><rdfs:subClassOf rdf:resource="http://reliant.teknowledge.com/DAML/SUMO.owl#Vehicle" /><rdfs:comment>Watercraft is the class of all Vehicles 

used to travel on or in water.</rdfs:comment></rdfs:Class><rdfs:Class rdf:ID="Waterfall"><rdfs:subClassOf rdf:resource="http://reliant.teknowledge.com/DAML/SUMO.owl#StreamWaterArea" /><rdfs:comment>Waterfall is the subclass of StreamWaterAreas 

where running water falls steeply downhill.</rdfs:comment></rdfs:Class><rdfs:Class rdf:ID="Waterway"><rdfs:subClassOf rdf:resource="http://reliant.teknowledge.com/DAML/SUMO.owl#Transitway" /><rdfs:subClassOf rdf:resource="http://reliant.teknowledge.com/DAML/SUMO.owl#WaterArea" /><rdfs:comment>Waterway is the class of navigable waters, 

including oceans, seaLanes, rivers, canals, lakes, and inland bodies 

of water.</rdfs:comment></rdfs:Class><rdfs:Class rdf:ID="Watt"><rdfs:subClassOf rdf:resource="http://reliant.teknowledge.com/DAML/SUMO.owl#FunctionQuantity" /><rdf:type rdf:resource="http://reliant.teknowledge.com/DAML/SUMO.owl#SystemeInternationalUnit" /><rdfs:comment>SI power measure.  Symbol: W.  A UnitOfMeasure 

that measures power, i.e. energy produced or expended divided by 

TimeDuration. It is the power which gives rise to the production 

of energy (or work) at the rate of one Joule per SecondDuration.  

Watt = J/s = m^2*kg*s^(-3).</rdfs:comment></rdfs:Class><rdfs:Class rdf:ID="Waving"><rdfs:subClassOf rdf:resource="#HandGesture" /><rdfs:comment>Moving a Hand to indicate a greeting, farewell, 

recognition, goodwill, etc.</rdfs:comment></rdfs:Class><rdfs:Class rdf:ID="Wax"><rdfs:subClassOf rdf:resource="http://reliant.teknowledge.com/DAML/SUMO.owl#Substance" /><rdfs:comment>Any Substance of high molecular weight that resembles 

beeswax.</rdfs:comment></rdfs:Class><rdfs:Class rdf:ID="WeaponOfMassDestruction"><rdfs:subClassOf rdf:resource="http://reliant.teknowledge.com/DAML/SUMO.owl#Weapon" /><rdfs:comment>Nuclear, chemical and biological weapons.  

What these weapons have in common is that they are designed to kill large numbers 

of people indiscriminately.</rdfs:comment></rdfs:Class><rdfs:Class rdf:ID="WeatherFront"><rdfs:subClassOf rdf:resource="http://reliant.teknowledge.com/DAML/SUMO.owl#WeatherProcess" /><rdfs:comment>WeatherFront is the class of weather 

processes that are involve relationships between two air masses, such 

as a high pressure weather system or a low pressure system.</rdfs:comment></rdfs:Class><rdfs:Class rdf:ID="Weber"><rdfs:subClassOf rdf:resource="http://reliant.teknowledge.com/DAML/SUMO.owl#FunctionQuantity" /><rdf:type rdf:resource="http://reliant.teknowledge.com/DAML/SUMO.owl#SystemeInternationalUnit" /><rdfs:comment>SI magnetic flux measure.  Symbol: Wb. It is the 

magnetic flux which, linking a circuit of one turn, produces in it an

electromotive force of 1 Volt as it is reduced to zero at a uniform

rate in 1 SecondDuration.  Weber = V*s = m^2*kg*s^(-2)*A^(-1).</rdfs:comment></rdfs:Class><rdfs:Class rdf:ID="Weekend"><rdfs:subClassOf rdf:resource="http://reliant.teknowledge.com/DAML/SUMO.owl#TimeInterval" /><rdfs:comment>Any Saturday and Sunday which are contiguous.</rdfs:comment></rdfs:Class><rdfs:Class rdf:ID="Weeping"><rdfs:subClassOf rdf:resource="#FacialExpression" /><rdfs:comment>Expressing unhappiness by shedding tears.</rdfs:comment></rdfs:Class><rdfs:Class rdf:ID="Welfare"><rdfs:subClassOf rdf:resource="http://reliant.teknowledge.com/DAML/SUMO.owl#Funding" /><rdfs:comment>Any Funding which is provided by a ServiceOrganization 

to people in need.</rdfs:comment></rdfs:Class><rdfs:Class rdf:ID="WetTropicalClimateZone"><rdfs:subClassOf rdf:resource="#TropicalClimateZone" /><rdfs:comment>WetTropicalClimateZone is 

the subclass of TropicalClimateZone that is characterized by having 

no dry months.  At least 60 mm of rainfall occur in the driest month. 

This is subtype 'Af' in the Koeppen climate system.</rdfs:comment></rdfs:Class><rdfs:Class rdf:ID="Wheat"><rdfs:subClassOf rdf:resource="#CerealGrain" /><rdfs:comment>A long CerealGrain which is produced by certain grasses and 

which is used to make BreadOrBiscuits.</rdfs:comment></rdfs:Class><rdfs:Class rdf:ID="Wheel"><rdfs:subClassOf rdf:resource="http://reliant.teknowledge.com/DAML/SUMO.owl#Artifact" /><rdfs:comment>A circular Artifact which is a component of 

LandVehicles and of some Devices.</rdfs:comment></rdfs:Class><rdfs:Class rdf:ID="Whip"><rdfs:subClassOf rdf:resource="http://reliant.teknowledge.com/DAML/SUMO.owl#Weapon" /><rdfs:comment>A Weapon that consists of a thin strand of 

Fabric, usually Leather, and a handle by which the strand is 

impelled at a high rate of speed.</rdfs:comment></rdfs:Class><rdfs:Class rdf:ID="Whiskey"><rdfs:subClassOf rdf:resource="#DistilledAlcoholicBeverage" /><rdfs:comment>A DistilledAlcoholicBeverage that is prepared by 

distilling fermented grain mash.</rdfs:comment></rdfs:Class><rdfs:Class rdf:ID="WhiteBloodCell"><rdfs:subClassOf rdf:resource="#BloodCell" /><rdfs:comment>BloodCells that lack hemoglobin, contain a 

CellNucleus, and have no color.</rdfs:comment></rdfs:Class><rdfs:Class rdf:ID="WholesaleStore"><rdfs:subClassOf rdf:resource="http://reliant.teknowledge.com/DAML/SUMO.owl#MercantileOrganization" /><rdfs:subClassOf rdf:resource="#Agency" /><rdfs:comment>A MercantileOrganization that sells its 

goods exclusively to Corporations.</rdfs:comment></rdfs:Class><rdfs:Class rdf:ID="WillowTree"><rdfs:subClassOf rdf:resource="#BotanicalTree" /><rdfs:comment>A BotanicalTree of the genus Salix.</rdfs:comment></rdfs:Class><rdfs:Class rdf:ID="WindInstrument"><rdfs:subClassOf rdf:resource="http://reliant.teknowledge.com/DAML/SUMO.owl#MusicalInstrument" /><rdfs:comment>A MusicalInstrument which is played by 

blowing it and which uses a reed.</rdfs:comment></rdfs:Class><rdfs:Class rdf:ID="Windmill"><rdfs:subClassOf rdf:resource="#Engine" /><rdfs:comment>Windmill is the subclass of Engines that 

produce mechanical power from Wind energy.</rdfs:comment></rdfs:Class><rdfs:Class rdf:ID="Window"><rdfs:subClassOf rdf:resource="http://reliant.teknowledge.com/DAML/SUMO.owl#Artifact" /><rdfs:comment>An Artifact composed of transparent glass or 

plastic that admits light (and possibly air) into a Room, Building 

or Vehicle.</rdfs:comment></rdfs:Class><rdfs:Class rdf:ID="WindowCovering"><rdfs:subClassOf rdf:resource="http://reliant.teknowledge.com/DAML/SUMO.owl#Artifact" /><rdfs:comment>An Artifact that is used to cover 

Windows.  Note that this class includes blinds, drapes, shutters, 

etc.</rdfs:comment></rdfs:Class><rdfs:Class rdf:ID="Windshield"><rdfs:subClassOf rdf:resource="#VehicleWindow" /><sumo:disjoint rdf:resource="#RearWindow" /><rdfs:comment>Any VehicleWindow which located at the front 

of an Automobile.</rdfs:comment></rdfs:Class><rdfs:Class rdf:ID="Wine"><rdfs:subClassOf rdf:resource="#AlcoholicBeverage" /><rdfs:comment>An AlcoholicBeverage that is prepared by fermenting 

the juice of grapes.</rdfs:comment></rdfs:Class><rdfs:Class rdf:ID="Wing"><rdfs:subClassOf rdf:resource="#Limb" /><rdfs:comment>Any Limb which is capable of being an 

instrument in Flying.</rdfs:comment></rdfs:Class><rdfs:Class rdf:ID="WingDevice"><rdfs:subClassOf rdf:resource="http://reliant.teknowledge.com/DAML/SUMO.owl#EngineeringComponent" /><rdfs:comment>The wings of Aircraft, i.e. the parts of Aircraft 

that allow them to become and remain airborne.</rdfs:comment></rdfs:Class><rdfs:Class rdf:ID="Winking"><rdfs:subClassOf rdf:resource="#ClosingEyes" /><rdfs:subClassOf rdf:resource="http://reliant.teknowledge.com/DAML/SUMO.owl#Gesture" /><rdfs:comment>Any instance of ClosingEyes which is intended to 

express something to someone else.</rdfs:comment></rdfs:Class><rdfs:Class rdf:ID="WinterSeason"><rdfs:subClassOf rdf:resource="#SeasonOfYear" /><rdfs:comment>The SeasonOfYear that begins at the winter 

solstice and ends at the spring equinox.</rdfs:comment></rdfs:Class><rdfs:Class rdf:ID="Wire"><rdfs:subClassOf rdf:resource="http://reliant.teknowledge.com/DAML/SUMO.owl#Artifact" /><rdfs:comment>A long, thin strand of Metal that is used in a wide 

range of applications, including the wiring of electrical systems, creating 

bundles and the construction of cages.</rdfs:comment></rdfs:Class><rdfs:Class rdf:ID="WireLine"><rdfs:subClassOf rdf:resource="#Wire" /><rdfs:subClassOf rdf:resource="http://reliant.teknowledge.com/DAML/SUMO.owl#EngineeringComponent" /><rdfs:comment>A Wire that is designed for conducting electricity.</rdfs:comment></rdfs:Class><rdfs:Class rdf:ID="WireSpring"><rdfs:subClassOf rdf:resource="#Wire" /><rdfs:subClassOf rdf:resource="http://reliant.teknowledge.com/DAML/SUMO.owl#EngineeringComponent" /><rdfs:comment>An EngineeringComponent consisting of a coil of 

Wire that returns to its original shape when pulled apart or pressed together.</rdfs:comment></rdfs:Class><rdfs:Class rdf:ID="Withdrawal"><rdfs:subClassOf rdf:resource="http://reliant.teknowledge.com/DAML/SUMO.owl#FinancialTransaction" /><rdfs:comment>An activity of money being transferred from a customer's 

account at a financial institution.</rdfs:comment></rdfs:Class><rdfs:Class rdf:ID="Wood"><rdfs:subClassOf rdf:resource="http://reliant.teknowledge.com/DAML/SUMO.owl#Tissue" /><rdfs:subClassOf rdf:resource="http://reliant.teknowledge.com/DAML/SUMO.owl#PlantSubstance" /><sumo:relatedInternalConcept rdf:resource="#WoodArtifact" /><rdfs:comment>Tissue that comprises the inner trunk of Trees.  

It is often used in constructing Buildings and other Artifacts.</rdfs:comment></rdfs:Class><rdfs:Class rdf:ID="WoodArtifact"><rdfs:subClassOf rdf:resource="http://reliant.teknowledge.com/DAML/SUMO.owl#Artifact" /><rdfs:comment>Wood that has been cut (and perhaps treated) for 

some purpose, e.g. Constructing or Combustion.  Note that this class covers 

both lumber and firewood.</rdfs:comment></rdfs:Class><rdfs:Class rdf:ID="Wool"><rdfs:subClassOf rdf:resource="http://reliant.teknowledge.com/DAML/SUMO.owl#Fabric" /><rdfs:comment>Fabric that is made from the Hair of Sheep.</rdfs:comment></rdfs:Class><rdfs:Class rdf:ID="WorkerInsect"><rdfs:subClassOf rdf:resource="http://reliant.teknowledge.com/DAML/SUMO.owl#Insect" /><rdfs:comment>Sterile members of an Insect colony which 

are responsible for locating food and caring for eggs, larvae, etc.</rdfs:comment></rdfs:Class><rdfs:Class rdf:ID="Workshop"><rdfs:subClassOf rdf:resource="http://reliant.teknowledge.com/DAML/SUMO.owl#StationaryArtifact" /><rdfs:comment>A Room, suite of Rooms or Building which is 

devoted to hand-crafting Artifacts.</rdfs:comment></rdfs:Class><rdfs:Class rdf:ID="Wrist"><rdfs:subClassOf rdf:resource="#BodyJoint" /><rdfs:comment>The joint in the Arm connecting the radius and carpal 

bones.</rdfs:comment></rdfs:Class><rdfs:Class rdf:ID="WritingDevice"><rdfs:subClassOf rdf:resource="http://reliant.teknowledge.com/DAML/SUMO.owl#Device" /><rdfs:comment>A Device whose purpose is to be an instrument 

of Writing, e.g. pens, pencils, crayons, etc.</rdfs:comment></rdfs:Class><rdfs:Class rdf:ID="WrittenCommunication"><rdfs:subClassOf rdf:resource="http://reliant.teknowledge.com/DAML/SUMO.owl#LinguisticCommunication" /><rdfs:comment>Any LinguisticCommunication where the 

instrument is a Text, e.g. a letter, an email, a memo, etc.</rdfs:comment></rdfs:Class><rdfs:Class rdf:ID="XRayRadiation"><rdfs:subClassOf rdf:resource="http://reliant.teknowledge.com/DAML/SUMO.owl#Radiating" /><rdfs:comment>Electro-magnetic radiation of short wavelength, 

often made use of by devices that scan the inside of objects.</rdfs:comment></rdfs:Class><rdfs:Class rdf:ID="YardLength"><rdfs:subClassOf rdf:resource="http://reliant.teknowledge.com/DAML/SUMO.owl#LengthMeasure" /><rdf:type rdf:resource="http://reliant.teknowledge.com/DAML/SUMO.owl#UnitOfMeasure" /><rdfs:comment>English unit of length, equal to 3 FeetLength.</rdfs:comment></rdfs:Class><rdfs:Class rdf:ID="Zinc"><rdfs:subClassOf rdf:resource="http://reliant.teknowledge.com/DAML/SUMO.owl#ElementalSubstance" /><atomicNumber>30</atomicNumber><rdfs:comment>Blue-white metallic element.  Occurs in multiple 

compounds naturally.  Five stable isotopes are six radioactive isotopes 

have been found.  Chemically a reactive metal, combines with oxygen and 

other non-metals, reacts with dilute acids to release hydrogen.</rdfs:comment></rdfs:Class><owl:ObjectProperty rdf:ID="BeginNodeFn"><rdfs:comment>A UnaryFunction that maps a GraphPath 

to the GraphNode that is the beginning of the GraphPath.  Note that, 

unlike InitialNodeFn (which relates a GraphArc to a GraphNode),  

BeginNodeFn is a total function - every GraphPath has a beginning.</rdfs:comment><rdf:type rdf:resource="http://reliant.teknowledge.com/DAML/SUMO.owl#UnaryFunction" /><rdf:type rdf:resource="http://reliant.teknowledge.com/DAML/SUMO.owl#TotalValuedRelation" /><rdfs:domain rdf:resource="#GraphPath" /><rdfs:range rdf:resource="#GraphNode" /><sumo:relatedInternalConcept rdf:resource="#InitialNodeFn" /></owl:ObjectProperty><owl:ObjectProperty rdf:ID="CenterOfCircleFn"><rdfs:comment>(CenterOfCircleFn ?CIRCLE) denotes the 

GeometricPoint that is the center of the Circle ?CIRCLE.</rdfs:comment><rdf:type rdf:resource="http://reliant.teknowledge.com/DAML/SUMO.owl#UnaryFunction" /><rdf:type rdf:resource="http://reliant.teknowledge.com/DAML/SUMO.owl#TotalValuedRelation" /><rdfs:domain rdf:resource="#Circle" /><rdfs:range rdf:resource="http://reliant.teknowledge.com/DAML/SUMO.owl#GeometricPoint" /></owl:ObjectProperty><owl:ObjectProperty rdf:ID="CitizenryFn"><rdfs:comment>(CitizenryFn ?AREA) denotes the 

GroupOfPeople who are legal and permanent residents of the 

GeopoliticalArea ?AREA.</rdfs:comment><rdfs:domain rdf:resource="http://reliant.teknowledge.com/DAML/SUMO.owl#GeopoliticalArea" /><rdfs:range rdf:resource="http://reliant.teknowledge.com/DAML/SUMO.owl#GroupOfPeople" /><rdfs:subPropertyOf rdf:resource="#ResidentFn" /></owl:ObjectProperty><owl:ObjectProperty rdf:ID="CutSetFn"><rdfs:comment>A UnaryFunction that assigns a Graph the 

Class of GraphPaths that partition the graph into two separate 

graphs if cut.  There may be more than one cutset for a given graph.</rdfs:comment><rdf:type rdf:resource="http://reliant.teknowledge.com/DAML/SUMO.owl#UnaryFunction" /><rdfs:domain rdf:resource="#Graph" /><sumo:rangeSubclass rdf:resource="#GraphPath" /></owl:ObjectProperty><owl:ObjectProperty rdf:ID="DescendantsFn"><rdfs:comment>(DescendantsFn ?PERSON) denotes all and only 

the descendants of ?PERSON, i.e. the Group consisting of ?OFFSPRING who 

satisfy the following formula:  (ancestor ?OFFSPRING ?PERSON).</rdfs:comment><rdf:type rdf:resource="http://reliant.teknowledge.com/DAML/SUMO.owl#UnaryFunction" /><rdfs:domain rdf:resource="http://reliant.teknowledge.com/DAML/SUMO.owl#Human" /><rdfs:range rdf:resource="http://reliant.teknowledge.com/DAML/SUMO.owl#FamilyGroup" /></owl:ObjectProperty><owl:ObjectProperty rdf:ID="DiameterFn"><rdfs:comment>(DiameterFn ?CIRCLE) denotes the length of the 

diameter of the Circle ?CIRCLE.</rdfs:comment><rdf:type rdf:resource="http://reliant.teknowledge.com/DAML/SUMO.owl#UnaryFunction" /><rdf:type rdf:resource="http://reliant.teknowledge.com/DAML/SUMO.owl#TotalValuedRelation" /><rdfs:domain rdf:resource="#Circle" /><rdfs:range rdf:resource="http://reliant.teknowledge.com/DAML/SUMO.owl#LengthMeasure" /></owl:ObjectProperty><owl:ObjectProperty rdf:ID="DocumentFn"><rdfs:comment>(DocumentFn ?PROP) denotes the class 

of ContentBearingObjects that contain the information ?PROP.</rdfs:comment><rdf:type rdf:resource="http://reliant.teknowledge.com/DAML/SUMO.owl#UnaryFunction" /><rdfs:domain rdf:resource="http://reliant.teknowledge.com/DAML/SUMO.owl#Proposition" /><sumo:rangeSubclass rdf:resource="http://reliant.teknowledge.com/DAML/SUMO.owl#Text" /></owl:ObjectProperty><owl:ObjectProperty rdf:ID="EndNodeFn"><rdfs:comment>A UnaryFunction that maps a GraphPath 

to the GraphNode that is the end of the GraphPath.  Note that, unlike 

TerminalNodeFn (which relates a GraphArc to a GraphNode),  

EndNodeFn is a total function - every GraphPath has a end.</rdfs:comment><rdf:type rdf:resource="http://reliant.teknowledge.com/DAML/SUMO.owl#UnaryFunction" /><rdf:type rdf:resource="http://reliant.teknowledge.com/DAML/SUMO.owl#TotalValuedRelation" /><rdfs:domain rdf:resource="#GraphPath" /><rdfs:range rdf:resource="#GraphNode" /><sumo:relatedInternalConcept rdf:resource="#TerminalNodeFn" /></owl:ObjectProperty><owl:ObjectProperty rdf:ID="ExecutiveBranchFn"><rdfs:comment>(ExecutiveBranchFn ?ORG) denotes the 

executive branch of ?ORG, with all its officials and agencies, considered 

as a whole.</rdfs:comment><rdf:type rdf:resource="http://reliant.teknowledge.com/DAML/SUMO.owl#UnaryFunction" /><rdfs:domain rdf:resource="http://reliant.teknowledge.com/DAML/SUMO.owl#Agent" /><rdfs:range rdf:resource="http://reliant.teknowledge.com/DAML/SUMO.owl#Organization" /></owl:ObjectProperty><owl:ObjectProperty rdf:ID="FirstFn"><rdfs:comment>(FirstFn ?LIST) returns the first item in 

the List ?LIST.  For example, (FirstFn (ListFn Monday Tuesday 

Wednesday)) would return the value of Monday.</rdfs:comment><rdf:type rdf:resource="http://reliant.teknowledge.com/DAML/SUMO.owl#UnaryFunction" /><rdfs:domain rdf:resource="http://reliant.teknowledge.com/DAML/SUMO.owl#List" /><rdfs:range rdf:resource="http://reliant.teknowledge.com/DAML/SUMO.owl#Entity" /></owl:ObjectProperty><owl:ObjectProperty rdf:ID="InitialNodeFn"><rdfs:comment>A UnaryFunction that maps a 

GraphArc to the initial node of the GraphArc.  Note

that this is a partial function.  In particular, the function is 

undefined for GraphArcs that are not part of a DirectedGraph.</rdfs:comment><rdf:type rdf:resource="http://reliant.teknowledge.com/DAML/SUMO.owl#UnaryFunction" /><rdf:type rdf:resource="http://reliant.teknowledge.com/DAML/SUMO.owl#PartialValuedRelation" /><rdfs:domain rdf:resource="#GraphArc" /><rdfs:range rdf:resource="#GraphNode" /></owl:ObjectProperty><owl:ObjectProperty rdf:ID="JudiciaryFn"><rdfs:comment>(JudiciaryFn ?AREA) denotes the judicial 

branch of the GeopoliticalArea ?AREA, that is, the 

JudicialOrganization(s) associated with the government of ?AREA, 

considered as a whole.</rdfs:comment><rdf:type rdf:resource="http://reliant.teknowledge.com/DAML/SUMO.owl#UnaryFunction" /><rdfs:domain rdf:resource="http://reliant.teknowledge.com/DAML/SUMO.owl#GeopoliticalArea" /><rdfs:range rdf:resource="http://reliant.teknowledge.com/DAML/SUMO.owl#GovernmentOrganization" /><rdfs:range rdf:resource="http://reliant.teknowledge.com/DAML/SUMO.owl#JudicialOrganization" /></owl:ObjectProperty><owl:ObjectProperty rdf:ID="LastFn"><rdfs:comment>(LastFn ?LIST) returns the last item in the 

List ?LIST.  For example, (LastFn (ListFn Monday Tuesday 

Wednesday)) would return the value of Wednesday.</rdfs:comment><rdf:type rdf:resource="http://reliant.teknowledge.com/DAML/SUMO.owl#UnaryFunction" /><rdfs:domain rdf:resource="http://reliant.teknowledge.com/DAML/SUMO.owl#List" /><rdfs:range rdf:resource="http://reliant.teknowledge.com/DAML/SUMO.owl#Entity" /></owl:ObjectProperty><owl:ObjectProperty rdf:ID="LegislatureFn"><rdfs:comment>(LegislatureFn ?AREA) denotes the 

legislative branch of the GeopoliticalArea ?AREA.</rdfs:comment><rdf:type rdf:resource="http://reliant.teknowledge.com/DAML/SUMO.owl#UnaryFunction" /><rdfs:domain rdf:resource="http://reliant.teknowledge.com/DAML/SUMO.owl#GeopoliticalArea" /><rdfs:range rdf:resource="#LegislativeOrganization" /></owl:ObjectProperty><owl:ObjectProperty rdf:ID="MinimalCutSetFn"><rdfs:comment>A UnaryFunction that assigns a Graph 

the Class of GraphPaths which comprise cutsets for the Graph and 

which have the least number of GraphArcs.</rdfs:comment><rdf:type rdf:resource="http://reliant.teknowledge.com/DAML/SUMO.owl#UnaryFunction" /><rdfs:domain rdf:resource="#Graph" /><sumo:rangeSubclass rdf:resource="#GraphPath" /><sumo:relatedInternalConcept rdf:resource="#CutSetFn" /></owl:ObjectProperty><owl:ObjectProperty rdf:ID="OccupationFn"><rdfs:comment>(OccupationFn ?PROCESS) denotes the 

subclass of ?PROCESS where instances of ?PROCESS are performed as 

one's occupation, i.e. as part of a FinancialTransaction where one 

earns money for the performance of ?PROCESS.</rdfs:comment><rdf:type rdf:resource="http://reliant.teknowledge.com/DAML/SUMO.owl#UnaryFunction" /><rdfs:domain rdf:resource="http://reliant.teknowledge.com/DAML/SUMO.owl#IntentionalProcess" /><sumo:rangeSubclass rdf:resource="http://reliant.teknowledge.com/DAML/SUMO.owl#FinancialTransaction" /></owl:ObjectProperty><owl:ObjectProperty rdf:ID="OperatingFn"><rdfs:comment>(OperatingFn ?TYPE) denotes the class 

of events in which a Device of ?TYPE is being operated.</rdfs:comment><rdf:type rdf:resource="http://reliant.teknowledge.com/DAML/SUMO.owl#UnaryFunction" /><rdfs:domain rdf:resource="http://reliant.teknowledge.com/DAML/SUMO.owl#Device" /><sumo:rangeSubclass rdf:resource="http://reliant.teknowledge.com/DAML/SUMO.owl#Process" /></owl:ObjectProperty><owl:DatatypeProperty rdf:ID="PathWeightFn"><rdfs:comment>A UnaryFunction that maps a 

GraphPath to the sum of the arcWeights on the GraphArcs in 

the GraphPath.</rdfs:comment><rdf:type rdf:resource="http://reliant.teknowledge.com/DAML/SUMO.owl#UnaryFunction" /><rdfs:domain rdf:resource="#GraphPath" /><rdfs:range rdf:resource="http://reliant.teknowledge.com/DAML/SUMO.owl#RealNumber" /></owl:DatatypeProperty><owl:DatatypeProperty rdf:ID="PopulationFn"><rdfs:comment>(PopulationFn ?AREA) denotes the Integer 

that represents the count of the number of people inhabiting the 

GeopoliticalArea ?AREA.  The total population presents one overall 

measure of the potential impact of the country on the world and within its 

region.</rdfs:comment><rdf:type rdf:resource="http://reliant.teknowledge.com/DAML/SUMO.owl#UnaryFunction" /><rdfs:range rdf:resource="http://reliant.teknowledge.com/DAML/SUMO.owl#Integer" /><sumo:domain rdf:resource="http://reliant.teknowledge.com/DAML/SUMO.owl#GeopoliticalArea" /></owl:DatatypeProperty><owl:ObjectProperty rdf:ID="RadiusFn"><rdfs:comment>(RadiusFn ?CIRCLE) denotes the length of the radius 

of the Circle ?CIRCLE.</rdfs:comment><rdf:type rdf:resource="http://reliant.teknowledge.com/DAML/SUMO.owl#UnaryFunction" /><rdf:type rdf:resource="http://reliant.teknowledge.com/DAML/SUMO.owl#TotalValuedRelation" /><rdfs:domain rdf:resource="#Circle" /><rdfs:range rdf:resource="http://reliant.teknowledge.com/DAML/SUMO.owl#LengthMeasure" /></owl:ObjectProperty><owl:ObjectProperty rdf:ID="ResidentFn"><rdfs:comment>(ResidentFn ?AREA) denotes the 

GroupOfPeople who have their home in ?AREA.</rdfs:comment><rdf:type rdf:resource="http://reliant.teknowledge.com/DAML/SUMO.owl#UnaryFunction" /><rdfs:domain rdf:resource="http://reliant.teknowledge.com/DAML/SUMO.owl#GeopoliticalArea" /><rdfs:range rdf:resource="http://reliant.teknowledge.com/DAML/SUMO.owl#GroupOfPeople" /></owl:ObjectProperty><owl:ObjectProperty rdf:ID="StartFn"><rdfs:comment>(StartFn ?PROCESS) denotes IntentionalProcesses 

of bringing it about that Processes of type ?PROCESS begin, e.g. start 

working, begin running, etc.</rdfs:comment><rdf:type rdf:resource="http://reliant.teknowledge.com/DAML/SUMO.owl#UnaryFunction" /><rdfs:domain rdf:resource="http://reliant.teknowledge.com/DAML/SUMO.owl#Process" /><sumo:rangeSubclass rdf:resource="http://reliant.teknowledge.com/DAML/SUMO.owl#IntentionalProcess" /></owl:ObjectProperty><owl:ObjectProperty rdf:ID="StopFn"><rdfs:comment>(StopFn ?PROCESS) denotes IntentionalProcesses 

of bringing it about that Processes of type ?PROCESS end, e.g. stop 

walking, quit working, etc.</rdfs:comment><rdf:type rdf:resource="http://reliant.teknowledge.com/DAML/SUMO.owl#UnaryFunction" /><rdfs:domain rdf:resource="http://reliant.teknowledge.com/DAML/SUMO.owl#Process" /><sumo:rangeSubclass rdf:resource="http://reliant.teknowledge.com/DAML/SUMO.owl#IntentionalProcess" /></owl:ObjectProperty><owl:ObjectProperty rdf:ID="TerminalNodeFn"><rdfs:comment>A UnaryFunction that maps a 

GraphArc to the terminal node of the GraphArc.  Note that this 

is a partial function.  In particular, the function is undefined 

for GraphArcs that are not part of a DirectedGraph.</rdfs:comment><rdf:type rdf:resource="http://reliant.teknowledge.com/DAML/SUMO.owl#UnaryFunction" /><rdf:type rdf:resource="http://reliant.teknowledge.com/DAML/SUMO.owl#PartialValuedRelation" /><rdfs:domain rdf:resource="#GraphArc" /><rdfs:range rdf:resource="#GraphNode" /></owl:ObjectProperty><owl:ObjectProperty rdf:ID="abbreviation"><rdfs:comment>(abbreviation ?STRING ?THING) means that 

?STRING is an abbreviation used to refer to ?THING.  Abbreviations include 

acronyms and other abbreviated forms.</rdfs:comment><rdfs:subPropertyOf rdf:resource="#conventionalShortName" /></owl:ObjectProperty><owl:ObjectProperty rdf:ID="accountHolder"><rdfs:comment>(accountHolder ?Account ?Agent) means that 

?Agent is the account holder of the FinancialAccount ?Account.</rdfs:comment><rdfs:domain rdf:resource="#FinancialAccount" /><rdfs:range rdf:resource="http://reliant.teknowledge.com/DAML/SUMO.owl#CognitiveAgent" /><rdfs:subPropertyOf rdf:resource="#agreementMember" /></owl:ObjectProperty><owl:ObjectProperty rdf:ID="address"><rdfs:comment>(address ?AGENT ?ADDRESS) means that ?ADDRESS 

is an address or part of an address for the Agent ?AGENT.</rdfs:comment><rdf:type rdf:resource="http://reliant.teknowledge.com/DAML/SUMO.owl#BinaryPredicate" /><rdfs:domain rdf:resource="http://reliant.teknowledge.com/DAML/SUMO.owl#Agent" /><rdfs:range rdf:resource="#Address" /></owl:ObjectProperty><owl:ObjectProperty rdf:ID="administrativeCenter"><rdfs:comment>(administrativeCenter ?CENTER 

?REGION) means that ?CENTER is the City (or other area) from which 

the larger GeopoliticalArea ?REGION is administered.</rdfs:comment><rdf:type rdf:resource="http://reliant.teknowledge.com/DAML/SUMO.owl#BinaryPredicate" /><rdfs:domain rdf:resource="http://reliant.teknowledge.com/DAML/SUMO.owl#GeopoliticalArea" /><rdfs:range rdf:resource="http://reliant.teknowledge.com/DAML/SUMO.owl#GeopoliticalArea" /><rdfs:subPropertyOf rdf:resource="http://reliant.teknowledge.com/DAML/SUMO.owl#geopoliticalSubdivision" /></owl:ObjectProperty><owl:ObjectProperty rdf:ID="affiliatedOrganization"><rdf:type rdf:resource="http://reliant.teknowledge.com/DAML/SUMO.owl#BinaryPredicate" /><rdfs:domain rdf:resource="http://reliant.teknowledge.com/DAML/SUMO.owl#CognitiveAgent" /><rdfs:range rdf:resource="http://reliant.teknowledge.com/DAML/SUMO.owl#CognitiveAgent" /></owl:ObjectProperty><owl:ObjectProperty rdf:about="http://reliant.teknowledge.com/DAML/SUMO.owl#agent"><rdfs:subPropertyOf rdf:resource="#involvedInEvent" /></owl:ObjectProperty><owl:ObjectProperty rdf:ID="agentOperatesInArea"><rdfs:comment>(agentOperatesInArea ?ORG ?AREA) means that the Organization 

?ORG conducts operations (i.e. instances of IntentionalProcess) in ?AREA.</rdfs:comment><rdfs:domain rdf:resource="http://reliant.teknowledge.com/DAML/SUMO.owl#Organization" /><rdfs:range rdf:resource="http://reliant.teknowledge.com/DAML/SUMO.owl#GeopoliticalArea" /><rdfs:subPropertyOf rdf:resource="http://reliant.teknowledge.com/DAML/SUMO.owl#located" /></owl:ObjectProperty><owl:ObjectProperty rdf:ID="agreementMember"><rdfs:comment>(agreementMember ?Agreement ?Agent) 

means that ?Agent is one of the participants of the DeonticAttribute 

?Agreement.</rdfs:comment><rdf:type rdf:resource="http://reliant.teknowledge.com/DAML/SUMO.owl#BinaryPredicate" /><rdf:type rdf:resource="http://reliant.teknowledge.com/DAML/SUMO.owl#TotalValuedRelation" /><rdfs:domain rdf:resource="http://reliant.teknowledge.com/DAML/SUMO.owl#DeonticAttribute" /><rdfs:range rdf:resource="http://reliant.teknowledge.com/DAML/SUMO.owl#Agent" /></owl:ObjectProperty><owl:ObjectProperty rdf:ID="agreementPeriod"><rdfs:comment>(agreementPeriod ?Agreement ?Period) holds if 

?Period specifies a Time interval during which ?Agreement is in force.</rdfs:comment><rdf:type rdf:resource="http://reliant.teknowledge.com/DAML/SUMO.owl#BinaryPredicate" /><rdfs:domain rdf:resource="http://reliant.teknowledge.com/DAML/SUMO.owl#Contract" /><rdfs:range rdf:resource="http://reliant.teknowledge.com/DAML/SUMO.owl#TimeInterval" /></owl:ObjectProperty><owl:ObjectProperty rdf:ID="airTemperature"><rdfs:comment>(airTemperature ?AREA ?TEMP) means that 

the temperature of the air at ?AREA is ?TEMP.  Temperature is expressed 

in units of TemperatureMeasure, including CelsiusDegree and 

FahrenheitDegree, among others.</rdfs:comment><rdf:type rdf:resource="http://reliant.teknowledge.com/DAML/SUMO.owl#AsymmetricRelation" /><rdfs:domain rdf:resource="http://reliant.teknowledge.com/DAML/SUMO.owl#Object" /><rdfs:range rdf:resource="http://reliant.teknowledge.com/DAML/SUMO.owl#TemperatureMeasure" /><rdfs:subPropertyOf rdf:resource="http://reliant.teknowledge.com/DAML/SUMO.owl#measure" /></owl:ObjectProperty><owl:ObjectProperty rdf:ID="allegiance"><rdfs:comment>(allegiance ?AGENT ?ENTITY) means that the CognitiveAgent 

?AGENT owes its allegiance to the political entity ?ENTITY.</rdfs:comment><rdf:type rdf:resource="http://reliant.teknowledge.com/DAML/SUMO.owl#BinaryPredicate" /><rdfs:domain rdf:resource="http://reliant.teknowledge.com/DAML/SUMO.owl#CognitiveAgent" /><rdfs:range rdf:resource="http://reliant.teknowledge.com/DAML/SUMO.owl#CognitiveAgent" /></owl:ObjectProperty><owl:ObjectProperty rdf:ID="ancestorOrganization"><rdfs:comment>(ancestorOrganization ?ORG1 ?ORG2) means that 

the Organization ?ORG1 descended from the Organization ?ORG2.</rdfs:comment><rdf:type rdf:resource="http://reliant.teknowledge.com/DAML/SUMO.owl#BinaryPredicate" /><rdf:type rdf:resource="http://reliant.teknowledge.com/DAML/SUMO.owl#TransitiveRelation" /><rdf:type rdf:resource="http://reliant.teknowledge.com/DAML/SUMO.owl#IrreflexiveRelation" /><rdfs:domain rdf:resource="http://reliant.teknowledge.com/DAML/SUMO.owl#Organization" /><rdfs:range rdf:resource="http://reliant.teknowledge.com/DAML/SUMO.owl#Organization" /><sumo:disjointRelation rdf:resource="http://reliant.teknowledge.com/DAML/SUMO.owl#subOrganization" /></owl:ObjectProperty><owl:ObjectProperty rdf:ID="anniversary"><rdfs:comment>(anniversary ?PHYSICAL ?TIME) means that 

?TIME is the class of TimeIntervals which mark the anniversary of 

?PHYSICAL.  For example, (anniversary Christmas (DayFn 35 December)) 

means that Christmas is celebrated each year on the 25th of December.</rdfs:comment><rdf:type rdf:resource="http://reliant.teknowledge.com/DAML/SUMO.owl#BinaryPredicate" /><rdf:type rdf:resource="http://reliant.teknowledge.com/DAML/SUMO.owl#TemporalRelation" /><rdfs:domain rdf:resource="http://reliant.teknowledge.com/DAML/SUMO.owl#Physical" /><rdfs:range rdf:resource="http://reliant.teknowledge.com/DAML/SUMO.owl#TimeInterval" /></owl:ObjectProperty><owl:DatatypeProperty rdf:ID="arcWeight"><rdfs:comment>This predicate indicates the value of a 

GraphArc in a Graph.  This could map to the length of a road in 

a road network or the flow rate of a pipe in a plumbing system.</rdfs:comment><rdf:type rdf:resource="http://reliant.teknowledge.com/DAML/SUMO.owl#BinaryPredicate" /><rdf:type rdf:resource="http://reliant.teknowledge.com/DAML/SUMO.owl#SingleValuedRelation" /><rdfs:domain rdf:resource="#GraphArc" /><rdfs:range rdf:resource="http://reliant.teknowledge.com/DAML/SUMO.owl#RealNumber" /></owl:DatatypeProperty><owl:DatatypeProperty rdf:ID="atomicNumber"><rdfs:comment>(atomicNumber ?ELEMENT ?NUMBER) means that the 

ElementalSubstance ?ELEMENT has the atomic number ?NUMBER. The atomic number 

is the number of Protons in the nucleus of an Atom.</rdfs:comment><rdfs:domain rdf:resource="http://reliant.teknowledge.com/DAML/SUMO.owl#ElementalSubstance" /><rdfs:range rdf:resource="http://reliant.teknowledge.com/DAML/SUMO.owl#PositiveInteger" /><rdfs:subPropertyOf rdf:resource="#protonNumber" /></owl:DatatypeProperty><owl:ObjectProperty rdf:ID="aunt"><rdfs:comment>(aunt ?AUNT ?PERSON) means that ?AUNT is 

the sister of a parent of ?PERSON.</rdfs:comment><rdfs:domain rdf:resource="http://reliant.teknowledge.com/DAML/SUMO.owl#Woman" /><rdfs:range rdf:resource="http://reliant.teknowledge.com/DAML/SUMO.owl#Human" /><rdfs:subPropertyOf rdf:resource="http://reliant.teknowledge.com/DAML/SUMO.owl#familyRelation" /></owl:ObjectProperty><owl:DatatypeProperty rdf:ID="average"><rdfs:comment>A partial function that relates a List to a 

RealNumber, provided that the List only has list elements that are 

RealNumbers. The RealNumber associated with the List is equal to the 

mathematical average of the RealNumbers in the List divided by the total

number of list elements.</rdfs:comment><rdf:type rdf:resource="http://reliant.teknowledge.com/DAML/SUMO.owl#BinaryPredicate" /><rdf:type rdf:resource="http://reliant.teknowledge.com/DAML/SUMO.owl#PartialValuedRelation" /><rdf:type rdf:resource="http://reliant.teknowledge.com/DAML/SUMO.owl#SingleValuedRelation" /><rdfs:domain rdf:resource="http://reliant.teknowledge.com/DAML/SUMO.owl#List" /><rdfs:range rdf:resource="http://reliant.teknowledge.com/DAML/SUMO.owl#RealNumber" /></owl:DatatypeProperty><owl:ObjectProperty rdf:ID="barometricPressure"><rdfs:comment>(barometricPressure ?AREA ?PRESSURE) 

means that the atmospheric pressure measured at ?AREA is ?PRESSURE.  

Barometric pressure is typically expressed in units of InchMercury or 

MmMercury.  For example, standard sea level pressure is 29.92 inches 

(760 mm) of mercury: (barometricPressure SeaLevel (MeasureFn 29.92 

InchMercury)).</rdfs:comment><rdf:type rdf:resource="http://reliant.teknowledge.com/DAML/SUMO.owl#BinaryPredicate" /><rdf:type rdf:resource="http://reliant.teknowledge.com/DAML/SUMO.owl#AsymmetricRelation" /><rdfs:domain rdf:resource="http://reliant.teknowledge.com/DAML/SUMO.owl#Object" /><rdfs:range rdf:resource="#AtmosphericPressureMeasure" /><rdfs:subPropertyOf rdf:resource="http://reliant.teknowledge.com/DAML/SUMO.owl#measure" /></owl:ObjectProperty><owl:ObjectProperty rdf:ID="birthday"><rdfs:comment>(birthday ?PERSON ?DAY) means that ?DAY is the 

anniversary each year of the birth of ?PERSON.  For example, (birthday 

WilliamJeffersonClinton (DayFn 19 August)) means that Bill Clinton's 

birthday is August 19th.</rdfs:comment><rdfs:domain rdf:resource="http://reliant.teknowledge.com/DAML/SUMO.owl#Human" /><rdfs:range rdf:resource="http://reliant.teknowledge.com/DAML/SUMO.owl#Day" /><rdfs:subPropertyOf rdf:resource="#anniversary" /></owl:ObjectProperty><owl:ObjectProperty rdf:ID="birthplace"><rdfs:comment>(birthplace ?INDIV ?PLACE) means that the Animal ?INDIV was born 

at the location ?PLACE.  The location may be a geographic area or a building, such as a hospital.</rdfs:comment><rdf:type rdf:resource="http://reliant.teknowledge.com/DAML/SUMO.owl#BinaryPredicate" /><rdfs:domain rdf:resource="http://reliant.teknowledge.com/DAML/SUMO.owl#Animal" /><rdfs:range rdf:resource="http://reliant.teknowledge.com/DAML/SUMO.owl#Object" /></owl:ObjectProperty><owl:ObjectProperty rdf:ID="borrower"><rdfs:comment>(borrower ?Loan ?Agent) means that ?Agent is a borrower of the ?Loan</rdfs:comment><rdfs:domain rdf:resource="#Loan" /><rdfs:range rdf:resource="http://reliant.teknowledge.com/DAML/SUMO.owl#CognitiveAgent" /><rdfs:subPropertyOf rdf:resource="#agreementMember" /></owl:ObjectProperty><owl:ObjectProperty rdf:ID="brandName"><rdfs:comment>(brandName ?NAME ?PRODUCT) means that ?NAME 

is the brand name for the product class ?PRODUCT, e.g. Cheerios is the 

brand name for a certain class of breakfast cereal.</rdfs:comment><rdfs:range rdf:resource="http://reliant.teknowledge.com/DAML/SUMO.owl#Product" /><rdfs:subPropertyOf rdf:resource="http://reliant.teknowledge.com/DAML/SUMO.owl#names" /><sumo:domain rdf:resource="http://reliant.teknowledge.com/DAML/SUMO.owl#SymbolicString" /></owl:ObjectProperty><owl:ObjectProperty rdf:ID="capacity"><rdfs:comment>(capacity ?OBJ ?QUANTITY) means that ?OBJ can contain 

something that has the measure of ?QUANTITY.  This predicate denotes maximal 

capacity, i.e. ?OBJ can hold no more than ?QUANTITY.  Note, however, that this 

does not mean that capacity is a SingleValuedRelation, since an object may 

have various maximal capacities across different dimensions, e.g. a particular 

box may have a capacity of 3 pounds and a capacity of 1 liter.</rdfs:comment><rdf:type rdf:resource="http://reliant.teknowledge.com/DAML/SUMO.owl#BinaryPredicate" /><rdfs:domain rdf:resource="http://reliant.teknowledge.com/DAML/SUMO.owl#SelfConnectedObject" /><rdfs:range rdf:resource="http://reliant.teknowledge.com/DAML/SUMO.owl#ConstantQuantity" /><sumo:relatedInternalConcept rdf:resource="#humanCapacity" /></owl:ObjectProperty><owl:ObjectProperty rdf:ID="capitalCity"><rdfs:comment>(capitalCity ?CITY ?REGION) means that the 

City ?CITY is the capital of the GeopoliticalArea ?REGION.</rdfs:comment><rdf:type rdf:resource="http://reliant.teknowledge.com/DAML/SUMO.owl#BinaryPredicate" /><rdfs:domain rdf:resource="http://reliant.teknowledge.com/DAML/SUMO.owl#City" /><rdfs:range rdf:resource="http://reliant.teknowledge.com/DAML/SUMO.owl#GeopoliticalArea" /><rdfs:subPropertyOf rdf:resource="#administrativeCenter" /></owl:ObjectProperty><owl:ObjectProperty rdf:ID="cargoType"><rdfs:comment>(cargoType ?DEVICE ?TYPE) means that the 

TransportationDevice ?DEVICE can, and typically does, carry cargo of 

the kind ?TYPE.</rdfs:comment><rdf:type rdf:resource="http://reliant.teknowledge.com/DAML/SUMO.owl#BinaryPredicate" /><rdfs:domain rdf:resource="http://reliant.teknowledge.com/DAML/SUMO.owl#TransportationDevice" /><rdfs:range rdf:resource="http://reliant.teknowledge.com/DAML/SUMO.owl#Object" /></owl:ObjectProperty><owl:ObjectProperty rdf:about="http://reliant.teknowledge.com/DAML/SUMO.owl#causes"><rdfs:subPropertyOf rdf:resource="#relatedEvent" /></owl:ObjectProperty><owl:ObjectProperty rdf:ID="checkAccount"><rdfs:comment>(checkAccount ?Check ?Account) means that ?Account 

is the FinancialAccount from which the amount specifed on the check is paid.</rdfs:comment><rdf:type rdf:resource="http://reliant.teknowledge.com/DAML/SUMO.owl#BinaryPredicate" /><rdfs:domain rdf:resource="#Check" /><rdfs:range rdf:resource="#FinancialAccount" /></owl:ObjectProperty><owl:ObjectProperty rdf:ID="cityAddress"><rdfs:comment>(cityAddress ?CITY ?ADDRESS) means that the 

City ?CITY is part of the address ?ADDRESS.</rdfs:comment><rdfs:domain rdf:resource="http://reliant.teknowledge.com/DAML/SUMO.owl#City" /><rdfs:range rdf:resource="#Address" /><rdfs:subPropertyOf rdf:resource="#address" /></owl:ObjectProperty><owl:ObjectProperty rdf:ID="climateTypeInArea"><rdfs:comment>(climateTypeInArea ?TYPE ?REGION) 

means that all or part of the GeographicArea ?REGION is of the 

ClimateZone ?TYPE.</rdfs:comment><rdf:type rdf:resource="http://reliant.teknowledge.com/DAML/SUMO.owl#BinaryPredicate" /><rdfs:domain rdf:resource="http://reliant.teknowledge.com/DAML/SUMO.owl#GeographicArea" /><rdfs:range rdf:resource="#ClimateZone" /></owl:ObjectProperty><owl:ObjectProperty rdf:ID="conjugate"><rdfs:comment>(conjugate ?COMPOUND1 ?COMPOUND2) means that 

?COMPOUND1 and ?COMPOUND2 are identical CompoundSubstances except that 

one has one more Proton than the other.</rdfs:comment><rdf:type rdf:resource="http://reliant.teknowledge.com/DAML/SUMO.owl#BinaryPredicate" /><rdf:type rdf:resource="http://reliant.teknowledge.com/DAML/SUMO.owl#IrreflexiveRelation" /><rdf:type rdf:resource="http://reliant.teknowledge.com/DAML/SUMO.owl#SymmetricRelation" /><rdf:type rdf:resource="http://reliant.teknowledge.com/DAML/SUMO.owl#TransitiveRelation" /><rdfs:domain rdf:resource="http://reliant.teknowledge.com/DAML/SUMO.owl#CompoundSubstance" /><rdfs:range rdf:resource="http://reliant.teknowledge.com/DAML/SUMO.owl#CompoundSubstance" /></owl:ObjectProperty><owl:ObjectProperty rdf:ID="contestParticipant"><rdfs:comment>(contestParticipant ?CONTEST ?AGENT) 

means that ?AGENT is one of the sides in the Contest ?CONTEST.  For 

example, if the ?CONTEST is a football game, then ?AGENT would be one of 

the opposing teams.  For another example, if ?CONTEST is a Battle, then 

?AGENT would be one of the sides fighting each other.</rdfs:comment><rdf:type rdf:resource="http://reliant.teknowledge.com/DAML/SUMO.owl#TotalValuedRelation" /><rdfs:domain rdf:resource="http://reliant.teknowledge.com/DAML/SUMO.owl#Contest" /><rdfs:range rdf:resource="http://reliant.teknowledge.com/DAML/SUMO.owl#Agent" /><rdfs:subPropertyOf rdf:resource="http://reliant.teknowledge.com/DAML/SUMO.owl#agent" /><rdfs:subPropertyOf rdf:resource="#involvedInEvent" /></owl:ObjectProperty><owl:ObjectProperty rdf:ID="conventionalLongName"><rdfs:comment>(conventionalLongName ?NAME ?THING) 

means that the string ?NAME is the long form of the name conventionally 

used for ?THING.</rdfs:comment><rdfs:subPropertyOf rdf:resource="http://reliant.teknowledge.com/DAML/SUMO.owl#names" /></owl:ObjectProperty><owl:ObjectProperty rdf:ID="conventionalShortName"><rdfs:comment>(conventionalShortName ?NAME 

?THING) means that the string ?NAME is the short form of the name 

conventionally used for ?THING.  For a more specialized subset of short 

names, see abbreviation.</rdfs:comment><rdfs:subPropertyOf rdf:resource="http://reliant.teknowledge.com/DAML/SUMO.owl#names" /></owl:ObjectProperty><owl:ObjectProperty rdf:ID="couponInterest"><rdfs:comment>(couponInterest ?BOND ?INTEREST) means that ?INTEREST is 

the periodic interest payment made to bondholders during the life of the ?BOND.</rdfs:comment><rdf:type rdf:resource="http://reliant.teknowledge.com/DAML/SUMO.owl#BinaryPredicate" /><rdfs:domain rdf:resource="#Bond" /><rdfs:range rdf:resource="http://reliant.teknowledge.com/DAML/SUMO.owl#CurrencyMeasure" /></owl:ObjectProperty><owl:ObjectProperty rdf:ID="cousin"><rdfs:comment>(cousin ?PERSON1 ?PERSON2) means that ?PERSON1 

and ?PERSON2 are cousins, i.e. ?PERSON1 and ?PERSON2 have grandparents 

(but not parents) in common.</rdfs:comment><rdfs:domain rdf:resource="http://reliant.teknowledge.com/DAML/SUMO.owl#Human" /><rdfs:range rdf:resource="http://reliant.teknowledge.com/DAML/SUMO.owl#Human" /><rdfs:subPropertyOf rdf:resource="http://reliant.teknowledge.com/DAML/SUMO.owl#familyRelation" /></owl:ObjectProperty><owl:ObjectProperty rdf:ID="currencyType"><rdfs:comment>(currencyType ?AREA ?UNIT) means 

that the official currency used in the GeopoliticalArea ?AREA 

is the UnitOfMeasure ?UNIT.</rdfs:comment><rdf:type rdf:resource="http://reliant.teknowledge.com/DAML/SUMO.owl#BinaryPredicate" /><rdfs:domain rdf:resource="http://reliant.teknowledge.com/DAML/SUMO.owl#GeopoliticalArea" /><rdfs:range rdf:resource="http://reliant.teknowledge.com/DAML/SUMO.owl#UnitOfMeasure" /><rdfs:range rdf:resource="http://reliant.teknowledge.com/DAML/SUMO.owl#CurrencyMeasure" /></owl:ObjectProperty><owl:ObjectProperty rdf:ID="customer"><rdfs:comment>A very general relation that exists whenever there

is a CommercialService between an Agent and an Organization.  

(customer ?AGENT ?ORG) means that ?AGENT is a customer of the Corporation 

?ORG.</rdfs:comment><rdf:type rdf:resource="http://reliant.teknowledge.com/DAML/SUMO.owl#IrreflexiveRelation" /><rdf:type rdf:resource="http://reliant.teknowledge.com/DAML/SUMO.owl#AsymmetricRelation" /><rdf:type rdf:resource="http://reliant.teknowledge.com/DAML/SUMO.owl#BinaryPredicate" /><rdfs:domain rdf:resource="http://reliant.teknowledge.com/DAML/SUMO.owl#Agent" /><rdfs:range rdf:resource="http://reliant.teknowledge.com/DAML/SUMO.owl#Corporation" /></owl:ObjectProperty><owl:ObjectProperty rdf:ID="defendant"><rdfs:comment>(defendant ?AGENT ?ACTION) means the LegalAction 

?ACTION makes a legal claim against ?AGENT.</rdfs:comment><rdfs:domain rdf:resource="http://reliant.teknowledge.com/DAML/SUMO.owl#CognitiveAgent" /><rdfs:range rdf:resource="http://reliant.teknowledge.com/DAML/SUMO.owl#LegalAction" /><rdfs:subPropertyOf rdf:resource="http://reliant.teknowledge.com/DAML/SUMO.owl#patient" /><rdfs:subPropertyOf rdf:resource="#involvedInEvent" /></owl:ObjectProperty><owl:ObjectProperty rdf:ID="dependentGeopoliticalArea"><rdfs:comment>(dependentGeopoliticalArea 

?AREA1 ?AREA2) means that ?AREA1 is a geopolitical possession of the 

GeopoliticalArea ?AREA2 and is not a geopoliticalSubdivision of 

?AREA2.  For example, (dependentGeopoliticalArea Guam UnitedStates), 

because Guam is a territory of the UnitedStates, not one of the fifty 

U.S. states.  Contrast primaryGeopoliticalSubdivision.</rdfs:comment><rdf:type rdf:resource="http://reliant.teknowledge.com/DAML/SUMO.owl#AsymmetricRelation" /><rdf:type rdf:resource="http://reliant.teknowledge.com/DAML/SUMO.owl#TransitiveRelation" /><rdfs:domain rdf:resource="http://reliant.teknowledge.com/DAML/SUMO.owl#GeopoliticalArea" /><rdfs:range rdf:resource="http://reliant.teknowledge.com/DAML/SUMO.owl#GeopoliticalArea" /><sumo:relatedInternalConcept rdf:resource="#primaryGeopoliticalSubdivision" /></owl:ObjectProperty><owl:ObjectProperty rdf:about="http://reliant.teknowledge.com/DAML/SUMO.owl#destination"><rdfs:subPropertyOf rdf:resource="#involvedInEvent" /></owl:ObjectProperty><owl:ObjectProperty rdf:ID="detainee"><rdfs:comment>(detainee ?EVENT ?OBJECT) means that in the 

Confining ?EVENT, the Object ?OBJECT is restrained by force, threat, or 

other form of intimidation.</rdfs:comment><rdf:type rdf:resource="http://reliant.teknowledge.com/DAML/SUMO.owl#CaseRole" /><rdfs:domain rdf:resource="http://reliant.teknowledge.com/DAML/SUMO.owl#Confining" /><rdfs:range rdf:resource="http://reliant.teknowledge.com/DAML/SUMO.owl#Animal" /><rdfs:subPropertyOf rdf:resource="http://reliant.teknowledge.com/DAML/SUMO.owl#patient" /><rdfs:subPropertyOf rdf:resource="#involvedInEvent" /></owl:ObjectProperty><owl:ObjectProperty rdf:ID="deviceState"><rdfs:comment>(deviceState ?DEVICE ?STATE) means that 

the Object ?DEVICE is in the DeviceStateAttribute ?STATE.</rdfs:comment><rdf:type rdf:resource="http://reliant.teknowledge.com/DAML/SUMO.owl#BinaryPredicate" /><rdfs:domain rdf:resource="http://reliant.teknowledge.com/DAML/SUMO.owl#Object" /><rdfs:range rdf:resource="#DeviceStateAttribute" /></owl:ObjectProperty><owl:ObjectProperty rdf:about="http://reliant.teknowledge.com/DAML/SUMO.owl#direction"><rdfs:subPropertyOf rdf:resource="#involvedInEvent" /></owl:ObjectProperty><owl:ObjectProperty rdf:ID="disapproves"><rdfs:comment>(disapproves ?AGENT ?FORMULA) means that 

?AGENT has a feeling of antipathy to the state of affairs represented by 

?FORMULA, i.e. ?AGENT believes that the realization of ?FORMULA will 

thwart one of his/her goals.  Note that there is no implication that what 

is disapproved of by an agent is not already true.</rdfs:comment><rdf:type rdf:resource="http://reliant.teknowledge.com/DAML/SUMO.owl#PropositionalAttitude" /><rdfs:domain rdf:resource="http://reliant.teknowledge.com/DAML/SUMO.owl#CognitiveAgent" /><rdfs:range rdf:resource="http://reliant.teknowledge.com/DAML/SUMO.owl#Formula" /><rdfs:subPropertyOf rdf:resource="http://reliant.teknowledge.com/DAML/SUMO.owl#inScopeOfInterest" /><sumo:disjointRelation rdf:resource="http://reliant.teknowledge.com/DAML/SUMO.owl#desires" /></owl:ObjectProperty><owl:ObjectProperty rdf:ID="dislikes"><rdfs:comment>(dislikes ?AGENT ?OBJECT) means that ?AGENT has a 

feeling of antipathy to ?OBJECT, i.e. ?AGENT believes that ?OBJECT will 

thwart one of his/her goals.  Note that there is no implication that what 

is hated by an agent is not already possessed by the agent.</rdfs:comment><rdf:type rdf:resource="http://reliant.teknowledge.com/DAML/SUMO.owl#ObjectAttitude" /><rdfs:domain rdf:resource="http://reliant.teknowledge.com/DAML/SUMO.owl#CognitiveAgent" /><rdfs:range rdf:resource="http://reliant.teknowledge.com/DAML/SUMO.owl#Object" /><rdfs:subPropertyOf rdf:resource="http://reliant.teknowledge.com/DAML/SUMO.owl#inScopeOfInterest" /><sumo:disjointRelation rdf:resource="http://reliant.teknowledge.com/DAML/SUMO.owl#wants" /><sumo:relatedInternalConcept rdf:resource="#disapproves" /></owl:ObjectProperty><owl:ObjectProperty rdf:ID="doubts"><rdfs:comment>(doubts ?AGENT ?FORMULA) means that ?AGENT is unsure 

about the truth of ?FORMULA, in particular ?AGENT does not believe that 

?FORMULA is true.</rdfs:comment><rdf:type rdf:resource="http://reliant.teknowledge.com/DAML/SUMO.owl#PropositionalAttitude" /><rdfs:domain rdf:resource="http://reliant.teknowledge.com/DAML/SUMO.owl#CognitiveAgent" /><rdfs:range rdf:resource="http://reliant.teknowledge.com/DAML/SUMO.owl#Formula" /></owl:ObjectProperty><owl:ObjectProperty rdf:ID="economyType"><rdfs:comment>(economyType ?POLITY ?TYPE) means that the 

GeopoliticalArea ?POLITY has an economic system of TYPE.</rdfs:comment><rdf:type rdf:resource="http://reliant.teknowledge.com/DAML/SUMO.owl#BinaryPredicate" /><rdfs:domain rdf:resource="http://reliant.teknowledge.com/DAML/SUMO.owl#Agent" /><rdfs:range rdf:resource="#EconomicAttribute" /><rdfs:subPropertyOf rdf:resource="http://reliant.teknowledge.com/DAML/SUMO.owl#attribute" /></owl:ObjectProperty><owl:ObjectProperty rdf:ID="electionForPosition"><rdfs:comment>(electionForPosition ?ELECTION 

?POSITION) means that in the Election ?ELECTION, candidates run for 

election to the role(s) ?POSITION.</rdfs:comment><rdf:type rdf:resource="http://reliant.teknowledge.com/DAML/SUMO.owl#BinaryPredicate" /><rdfs:domain rdf:resource="http://reliant.teknowledge.com/DAML/SUMO.owl#Election" /><rdfs:range rdf:resource="http://reliant.teknowledge.com/DAML/SUMO.owl#SocialRole" /></owl:ObjectProperty><owl:DatatypeProperty rdf:ID="electronNumber"><rdfs:comment>(electronNumber ?SUBSTANCE ?NUMBER) means that 

the PureSubstance ?SUBSTANCE has the number of Electrons ?NUMBER.</rdfs:comment><rdf:type rdf:resource="http://reliant.teknowledge.com/DAML/SUMO.owl#BinaryPredicate" /><rdf:type rdf:resource="http://reliant.teknowledge.com/DAML/SUMO.owl#SingleValuedRelation" /><rdf:type rdf:resource="http://reliant.teknowledge.com/DAML/SUMO.owl#TotalValuedRelation" /><rdfs:domain rdf:resource="http://reliant.teknowledge.com/DAML/SUMO.owl#PureSubstance" /><rdfs:range rdf:resource="http://reliant.teknowledge.com/DAML/SUMO.owl#PositiveInteger" /></owl:DatatypeProperty><owl:ObjectProperty rdf:ID="enjoys"><rdfs:comment>(enjoys ?AGENT ?PROCESS) means that the 

CognitiveAgent ?AGENT tends to enjoy actions of type ?PROCESS, 

i.e. tends to enjoy being the agent or experiencer of such 

actions.</rdfs:comment><rdfs:domain rdf:resource="http://reliant.teknowledge.com/DAML/SUMO.owl#CognitiveAgent" /><rdfs:range rdf:resource="http://reliant.teknowledge.com/DAML/SUMO.owl#IntentionalProcess" /><rdfs:subPropertyOf rdf:resource="http://reliant.teknowledge.com/DAML/SUMO.owl#inScopeOfInterest" /></owl:ObjectProperty><owl:ObjectProperty rdf:ID="equipmentType"><rdfs:comment>(equipmentType ?THING ?TYPE) means that 

the Artifact ?THING has a component or attachment of Device ?TYPE. 

See also equipmentTypeCount.</rdfs:comment><rdf:type rdf:resource="http://reliant.teknowledge.com/DAML/SUMO.owl#BinaryPredicate" /><rdfs:domain rdf:resource="http://reliant.teknowledge.com/DAML/SUMO.owl#Artifact" /><rdfs:range rdf:resource="http://reliant.teknowledge.com/DAML/SUMO.owl#Device" /></owl:ObjectProperty><owl:ObjectProperty rdf:ID="expects"><rdfs:comment>Any belief about the future.  (expects 

?AGENT ?BELIEF) means that (believes ?AGENT ?BELIEF) and, if 

?BELIEF happens, it will happen in the future, i.e. after the 

expectation.</rdfs:comment><rdfs:subPropertyOf rdf:resource="http://reliant.teknowledge.com/DAML/SUMO.owl#believes" /></owl:ObjectProperty><owl:ObjectProperty rdf:about="http://reliant.teknowledge.com/DAML/SUMO.owl#experiencer"><rdfs:subPropertyOf rdf:resource="#involvedInEvent" /></owl:ObjectProperty><owl:ObjectProperty rdf:ID="experimentalControl"><rdfs:comment>(experimentalControl ?EXPERIMENT ?OBJ) 

means that the Object ?OBJ serves as a control in the instance of 

Experimenting ?EXPERIMENT, i.e. ?OBJ is the standard against which something 

else in the experiment can be compared.</rdfs:comment><rdf:type rdf:resource="http://reliant.teknowledge.com/DAML/SUMO.owl#CaseRole" /><rdfs:domain rdf:resource="http://reliant.teknowledge.com/DAML/SUMO.owl#Experimenting" /><rdfs:range rdf:resource="http://reliant.teknowledge.com/DAML/SUMO.owl#Object" /><rdfs:subPropertyOf rdf:resource="#involvedInEvent" /></owl:ObjectProperty><owl:ObjectProperty rdf:ID="expirationDate"><rdfs:comment>(expirationDate ?CERTIFICATE ?DAY) means that 

?DAY is the date on which ?CERTIFICATE expires.</rdfs:comment><rdf:type rdf:resource="http://reliant.teknowledge.com/DAML/SUMO.owl#BinaryPredicate" /><rdfs:domain rdf:resource="http://reliant.teknowledge.com/DAML/SUMO.owl#Certificate" /><rdfs:range rdf:resource="http://reliant.teknowledge.com/DAML/SUMO.owl#Day" /></owl:ObjectProperty><owl:ObjectProperty rdf:ID="fears"><rdfs:comment>(fears ?AGENT ?FORMULA) means that ?AGENT fears that 

the proposition ?FORMULA will be true, i.e. he/she believes that it will 

come to pass in the future and that it will be undesirable for ?AGENT.</rdfs:comment><rdfs:subPropertyOf rdf:resource="#expects" /></owl:ObjectProperty><owl:ObjectProperty rdf:ID="financialAccount"><rdfs:comment>A formal banking, brokerage, or business 

relationship established to provide for regular services, dealings, and 

other financial transactions.  (accountAt ?ACCOUNT ?ORG) means that 

?ACCOUNT is a financial account opened at the FinancialCompany 

?ORG.</rdfs:comment><rdfs:domain rdf:resource="#FinancialAccount" /><rdfs:range rdf:resource="#FinancialCompany" /><rdfs:subPropertyOf rdf:resource="#agreementMember" /></owl:ObjectProperty><owl:ObjectProperty rdf:ID="financialAsset"><rdfs:comment>A predicate that relates an Agent to any 

item of economic value owned by the Agent.  Examples of financial assets 

are cash, securities, accounts receivable, inventory, office equipment, a 

house, a car, and other property.</rdfs:comment><rdfs:domain rdf:resource="http://reliant.teknowledge.com/DAML/SUMO.owl#Agent" /><rdfs:range rdf:resource="http://reliant.teknowledge.com/DAML/SUMO.owl#Object" /><rdfs:subPropertyOf rdf:resource="http://reliant.teknowledge.com/DAML/SUMO.owl#possesses" /></owl:ObjectProperty><owl:ObjectProperty rdf:ID="firstName"><rdfs:comment>(firstName ?CHAR ?INDIV) means that the 

SymbolicString ?CHAR contains the first (or given) name of the 

Human ?INDIV.</rdfs:comment><rdfs:comment>(firstName ?CHAR ?INDIV) means that the 

SymbolicString ?CHAR contains the first (or given) name of the 

Human ?INDIV.</rdfs:comment><rdf:type rdf:resource="http://reliant.teknowledge.com/DAML/SUMO.owl#BinaryPredicate" /><rdf:type rdf:resource="http://reliant.teknowledge.com/DAML/SUMO.owl#AsymmetricRelation" /><rdf:type rdf:resource="http://reliant.teknowledge.com/DAML/SUMO.owl#BinaryPredicate" /><rdf:type rdf:resource="http://reliant.teknowledge.com/DAML/SUMO.owl#AsymmetricRelation" /><rdfs:domain rdf:resource="http://reliant.teknowledge.com/DAML/SUMO.owl#SymbolicString" /><rdfs:range rdf:resource="http://reliant.teknowledge.com/DAML/SUMO.owl#Human" /><rdfs:subPropertyOf rdf:resource="http://reliant.teknowledge.com/DAML/SUMO.owl#names" /><rdfs:subPropertyOf rdf:resource="http://reliant.teknowledge.com/DAML/SUMO.owl#names" /></owl:ObjectProperty><owl:ObjectProperty rdf:ID="fiscalYearPeriod"><rdfs:comment>The predicate fiscalYearPeriod 

indicates the period that an Agent or Organization uses as its 

12-month accounting period.  (fiscalYearPeriod ?AGENT Year) means 

that ?AGENT observes its 12-month accounting period during the 

regular calendar year (CY), from January to December.  For 

fiscal years with other beginning and ending months (FYs), use 

(fiscalYearPeriod ?AGENT (RecurrentTimeIntervalFn ?STARTMONTH ?ENDMONTH)).  

For example, (fiscalYearPeriod (GovernmentFn UnitedStates) 

(RecurrentTimeIntervalFn October September)).  For FYs that begin 

or end mid-month, days may be specified within RecurrentTimeIntervalFn.</rdfs:comment><rdf:type rdf:resource="http://reliant.teknowledge.com/DAML/SUMO.owl#BinaryPredicate" /><rdfs:domain rdf:resource="http://reliant.teknowledge.com/DAML/SUMO.owl#Agent" /><rdfs:range rdf:resource="http://reliant.teknowledge.com/DAML/SUMO.owl#TimeInterval" /></owl:ObjectProperty><owl:ObjectProperty rdf:ID="formerName"><rdfs:comment>(formerName ?NAME ?THING) means that the 

string ?NAME is a name formerly used for ?THING.</rdfs:comment><rdfs:subPropertyOf rdf:resource="http://reliant.teknowledge.com/DAML/SUMO.owl#names" /></owl:ObjectProperty><owl:ObjectProperty rdf:ID="governmentType"><rdfs:comment>(governmentType ?BODY ?FORM) means that 

the GeopoliticalArea or Organization ?BODY has a government with 

characteristic(s) of the type ?FORM.</rdfs:comment><rdf:type rdf:resource="http://reliant.teknowledge.com/DAML/SUMO.owl#BinaryPredicate" /><rdfs:domain rdf:resource="http://reliant.teknowledge.com/DAML/SUMO.owl#Agent" /><rdfs:range rdf:resource="#FormOfGovernment" /><rdfs:subPropertyOf rdf:resource="http://reliant.teknowledge.com/DAML/SUMO.owl#attribute" /></owl:ObjectProperty><owl:ObjectProperty rdf:ID="grammaticalRelation"><rdfs:comment>(grammaticalRelation ?PHRASE ?SENTENCE) 

means that the Phrase ?PHRASE has a grammatical relation to the Sentence 

?SENTENCE, i.e. it is a subject, object, main verb, etc. of the ?SENTENCE.</rdfs:comment><rdf:type rdf:resource="http://reliant.teknowledge.com/DAML/SUMO.owl#BinaryPredicate" /><rdfs:domain rdf:resource="http://reliant.teknowledge.com/DAML/SUMO.owl#Phrase" /><rdfs:range rdf:resource="http://reliant.teknowledge.com/DAML/SUMO.owl#Sentence" /></owl:ObjectProperty><owl:ObjectProperty rdf:ID="grandfather"><rdfs:comment>(grandfather ?PERSON ?PARENT) means that 

?PARENT is the grandfather of ?PERSON.</rdfs:comment><rdfs:domain rdf:resource="http://reliant.teknowledge.com/DAML/SUMO.owl#Human" /><rdfs:range rdf:resource="http://reliant.teknowledge.com/DAML/SUMO.owl#Man" /><rdfs:subPropertyOf rdf:resource="http://reliant.teknowledge.com/DAML/SUMO.owl#familyRelation" /></owl:ObjectProperty><owl:ObjectProperty rdf:ID="grandmother"><rdfs:comment>(grandmother ?PERSON ?PARENT) means that 

?PARENT is the grandmother of ?PERSON.</rdfs:comment><rdfs:domain rdf:resource="http://reliant.teknowledge.com/DAML/SUMO.owl#Human" /><rdfs:range rdf:resource="http://reliant.teknowledge.com/DAML/SUMO.owl#Man" /><rdfs:subPropertyOf rdf:resource="http://reliant.teknowledge.com/DAML/SUMO.owl#familyRelation" /></owl:ObjectProperty><owl:ObjectProperty rdf:ID="graphPart"><rdfs:comment>A basic relation for Graphs and their 

parts.  (graphPart ?PART ?GRAPH) means that ?PART is a GraphArc 

or GraphNode of the Graph ?GRAPH.</rdfs:comment><rdf:type rdf:resource="http://reliant.teknowledge.com/DAML/SUMO.owl#BinaryPredicate" /><rdf:type rdf:resource="http://reliant.teknowledge.com/DAML/SUMO.owl#AsymmetricRelation" /><rdf:type rdf:resource="http://reliant.teknowledge.com/DAML/SUMO.owl#IrreflexiveRelation" /><rdfs:domain rdf:resource="#GraphElement" /><rdfs:range rdf:resource="#Graph" /></owl:ObjectProperty><owl:ObjectProperty rdf:ID="groupMember"><rdfs:comment>A subrelation of member, groupMember 

is used to relate a Human to a GroupOfPeople of which he/she is a 

member.</rdfs:comment><rdfs:domain rdf:resource="http://reliant.teknowledge.com/DAML/SUMO.owl#Human" /><rdfs:range rdf:resource="http://reliant.teknowledge.com/DAML/SUMO.owl#GroupOfPeople" /><rdfs:subPropertyOf rdf:resource="http://reliant.teknowledge.com/DAML/SUMO.owl#member" /></owl:ObjectProperty><owl:ObjectProperty rdf:ID="half"><rdfs:comment>(half ?HALF ?WHOLE) means that ?HALF is one half 

of ?WHOLE.</rdfs:comment><rdfs:subPropertyOf rdf:resource="http://reliant.teknowledge.com/DAML/SUMO.owl#part" /></owl:ObjectProperty><owl:ObjectProperty rdf:ID="hasExpertise"><rdfs:comment>(hasExpertise ?AGENT ?FIELD) means that ?AGENT has 

studied the FieldOfStudy ?FIELD and is regarded as an expert.</rdfs:comment><rdf:type rdf:resource="http://reliant.teknowledge.com/DAML/SUMO.owl#BinaryPredicate" /><rdfs:domain rdf:resource="http://reliant.teknowledge.com/DAML/SUMO.owl#CognitiveAgent" /><rdfs:range rdf:resource="http://reliant.teknowledge.com/DAML/SUMO.owl#FieldOfStudy" /></owl:ObjectProperty><owl:ObjectProperty rdf:ID="headquartersOfOrganization"><rdfs:comment>(headquartersOfOrganization ?ORG ?AREA) 

means that the Organization ?ORG is headquartered in ?AREA.</rdfs:comment><rdfs:domain rdf:resource="http://reliant.teknowledge.com/DAML/SUMO.owl#Organization" /><rdfs:range rdf:resource="http://reliant.teknowledge.com/DAML/SUMO.owl#GeopoliticalArea" /><rdfs:subPropertyOf rdf:resource="http://reliant.teknowledge.com/DAML/SUMO.owl#located" /></owl:ObjectProperty><owl:ObjectProperty rdf:ID="hopes"><rdfs:comment>(hopes ?AGENT ?FORMULA) means that ?AGENT hopes that 

the proposition ?FORMULA will be true, i.e. he/she believes that it will 

come to pass in the future and that it will be desirable for ?AGENT.</rdfs:comment><rdfs:subPropertyOf rdf:resource="#expects" /></owl:ObjectProperty><owl:ObjectProperty rdf:ID="hostileForces"><rdfs:comment>(hostileForces ?UNIT1 ?UNIT2) means that 

the MilitaryUnits ?UNIT1 and ?UNIT2 are, respectively, allied with 

GeopoliticalAreas that are at war with one another.</rdfs:comment><rdf:type rdf:resource="http://reliant.teknowledge.com/DAML/SUMO.owl#BinaryPredicate" /><rdf:type rdf:resource="http://reliant.teknowledge.com/DAML/SUMO.owl#IrreflexiveRelation" /><rdfs:domain rdf:resource="#MilitaryUnit" /><rdfs:range rdf:resource="#MilitaryUnit" /></owl:ObjectProperty><owl:DatatypeProperty rdf:ID="humanCapacity"><rdfs:comment>(humanCapacity ?CONSTRUCT ?NUMBER) means that the 

StationaryArtifact ?CONSTRUCT, e.g. a Building or a Room, can hold a maximum 

of ?NUMBER Humans without crowding.</rdfs:comment><rdf:type rdf:resource="http://reliant.teknowledge.com/DAML/SUMO.owl#BinaryPredicate" /><rdf:type rdf:resource="http://reliant.teknowledge.com/DAML/SUMO.owl#SingleValuedRelation" /><rdfs:domain rdf:resource="http://reliant.teknowledge.com/DAML/SUMO.owl#StationaryArtifact" /><rdfs:range rdf:resource="http://reliant.teknowledge.com/DAML/SUMO.owl#PositiveInteger" /></owl:DatatypeProperty><owl:ObjectProperty rdf:ID="ideologicalAffiliationOfOrganization"><rdfs:comment>(ideologicalAffiliationOfOrganization 

?ORG ?GOV) means that one of the goals of ?ORG is to realize the FormOfGovernment ?GOV.</rdfs:comment><rdf:type rdf:resource="http://reliant.teknowledge.com/DAML/SUMO.owl#BinaryPredicate" /><rdfs:domain rdf:resource="http://reliant.teknowledge.com/DAML/SUMO.owl#Organization" /><rdfs:range rdf:resource="#FormOfGovernment" /></owl:ObjectProperty><owl:ObjectProperty rdf:ID="industryOfArea"><rdfs:comment>(industryOfArea ?AREA ?SECTOR) 

means that the GeopoliticalArea ?AREA produces goods or services 

in the economic area ?SECTOR.</rdfs:comment><rdf:type rdf:resource="http://reliant.teknowledge.com/DAML/SUMO.owl#BinaryPredicate" /><rdfs:domain rdf:resource="http://reliant.teknowledge.com/DAML/SUMO.owl#GeopoliticalArea" /><rdfs:range rdf:resource="http://reliant.teknowledge.com/DAML/SUMO.owl#Physical" /></owl:ObjectProperty><owl:ObjectProperty rdf:ID="industryProductType"><rdfs:comment>(industryProductType ?INDUSTRY ?TYPE) means that the Industry ?INDUSTRY 

produces products of the kind ?TYPE.</rdfs:comment><rdf:type rdf:resource="http://reliant.teknowledge.com/DAML/SUMO.owl#BinaryPredicate" /><rdfs:domain rdf:resource="#Industry" /><rdfs:range rdf:resource="http://reliant.teknowledge.com/DAML/SUMO.owl#Product" /></owl:ObjectProperty><owl:ObjectProperty rdf:about="http://reliant.teknowledge.com/DAML/SUMO.owl#instrument"><rdfs:subPropertyOf rdf:resource="#involvedInEvent" /></owl:ObjectProperty><owl:ObjectProperty rdf:ID="insured"><rdfs:comment>(insured ?Contract ?Org) means that ?Contract is insured 

by the ?Organization.</rdfs:comment><rdf:type rdf:resource="http://reliant.teknowledge.com/DAML/SUMO.owl#BinaryPredicate" /><rdfs:domain rdf:resource="http://reliant.teknowledge.com/DAML/SUMO.owl#Contract" /><rdfs:range rdf:resource="http://reliant.teknowledge.com/DAML/SUMO.owl#Organization" /></owl:ObjectProperty><owl:DatatypeProperty rdf:ID="intelligenceQuotient"><rdfs:comment>(intelligenceQuotient ?PERSON ?NUMBER) 

means that ?NUMBER is the I.Q. of ?PERSON.  The I.Q. of a person is the ratio 

of their mental age (determined by a standardized test) divided by their 

chronological age, multiplied by 100.</rdfs:comment><rdf:type rdf:resource="http://reliant.teknowledge.com/DAML/SUMO.owl#BinaryPredicate" /><rdf:type rdf:resource="http://reliant.teknowledge.com/DAML/SUMO.owl#SingleValuedRelation" /><rdfs:domain rdf:resource="http://reliant.teknowledge.com/DAML/SUMO.owl#Human" /><rdfs:range rdf:resource="http://reliant.teknowledge.com/DAML/SUMO.owl#RationalNumber" /></owl:DatatypeProperty><owl:ObjectProperty rdf:ID="inventory"><rdfs:comment>(inventory ?CBO ?COLLECTION) means that 

the ContentBearingObject ?CBO contains a list or enumeration of the 

members of the Collection ?COLLECTION.</rdfs:comment><rdf:type rdf:resource="http://reliant.teknowledge.com/DAML/SUMO.owl#BinaryPredicate" /><rdfs:domain rdf:resource="http://reliant.teknowledge.com/DAML/SUMO.owl#ContentBearingObject" /><rdfs:range rdf:resource="http://reliant.teknowledge.com/DAML/SUMO.owl#Collection" /></owl:ObjectProperty><owl:ObjectProperty rdf:ID="involvedInEvent"><rdfs:comment>(involvedInEvent ?EVENT ?THING) means 

that in the Process ?EVENT, the Entity ?THING plays some CaseRole.</rdfs:comment><rdf:type rdf:resource="http://reliant.teknowledge.com/DAML/SUMO.owl#BinaryPredicate" /><rdf:type rdf:resource="http://reliant.teknowledge.com/DAML/SUMO.owl#AsymmetricRelation" /><rdfs:domain rdf:resource="http://reliant.teknowledge.com/DAML/SUMO.owl#Process" /><rdfs:range rdf:resource="http://reliant.teknowledge.com/DAML/SUMO.owl#Entity" /></owl:ObjectProperty><owl:ObjectProperty rdf:ID="issuedBy"><rdfs:comment>(issuedBy ?Certificate ?Agent) means that the 

Certificate ?Certificate is produced and offered by ?Agent.</rdfs:comment><rdf:type rdf:resource="http://reliant.teknowledge.com/DAML/SUMO.owl#BinaryPredicate" /><rdfs:domain rdf:resource="http://reliant.teknowledge.com/DAML/SUMO.owl#Certificate" /><rdfs:range rdf:resource="http://reliant.teknowledge.com/DAML/SUMO.owl#CognitiveAgent" /></owl:ObjectProperty><owl:ObjectProperty rdf:ID="lacks"><rdfs:comment>(lacks ?AGENT ?OBJECT) means that ?AGENT needs 

?OBJECT and it is not the case that ?AGENT possesses ?OBJECT.</rdfs:comment><rdfs:subPropertyOf rdf:resource="http://reliant.teknowledge.com/DAML/SUMO.owl#needs" /></owl:ObjectProperty><owl:ObjectProperty rdf:ID="landlord"><rdfs:comment>(landlord ?PERSON ?UNIT) means that ?PERSON is a 

landlord of the Residence ?UNIT, i.e. he or she owns ?UNIT and is renting 

the unit to someone else.</rdfs:comment><rdf:type rdf:resource="http://reliant.teknowledge.com/DAML/SUMO.owl#BinaryPredicate" /><rdfs:domain rdf:resource="http://reliant.teknowledge.com/DAML/SUMO.owl#Human" /><sumo:domain rdf:resource="http://reliant.teknowledge.com/DAML/SUMO.owl#PermanentResidence" /></owl:ObjectProperty><owl:ObjectProperty rdf:ID="lastName"><rdfs:comment>(lastName ?CHAR ?INDIV) means that the 

SymbolicString ?CHAR contains the last (surname or family) name of the 

Human ?INDIV.</rdfs:comment><rdfs:comment>(lastName ?CHAR ?INDIV) means that the 

SymbolicString ?CHAR contains the last (surname or family) name of the 

Human ?INDIV.</rdfs:comment><rdf:type rdf:resource="http://reliant.teknowledge.com/DAML/SUMO.owl#BinaryPredicate" /><rdf:type rdf:resource="http://reliant.teknowledge.com/DAML/SUMO.owl#AsymmetricRelation" /><rdf:type rdf:resource="http://reliant.teknowledge.com/DAML/SUMO.owl#BinaryPredicate" /><rdf:type rdf:resource="http://reliant.teknowledge.com/DAML/SUMO.owl#AsymmetricRelation" /><rdfs:domain rdf:resource="http://reliant.teknowledge.com/DAML/SUMO.owl#SymbolicString" /><rdfs:range rdf:resource="http://reliant.teknowledge.com/DAML/SUMO.owl#Human" /><rdfs:subPropertyOf rdf:resource="http://reliant.teknowledge.com/DAML/SUMO.owl#names" /><rdfs:subPropertyOf rdf:resource="http://reliant.teknowledge.com/DAML/SUMO.owl#names" /></owl:ObjectProperty><owl:ObjectProperty rdf:ID="leaderPosition"><rdfs:comment>(leaderPosition ?ORG ?ROLE)

means that in the organization ?ORG, the leader is the person 

who holds the Position ?ROLE in the organization.</rdfs:comment><rdf:type rdf:resource="http://reliant.teknowledge.com/DAML/SUMO.owl#BinaryPredicate" /><rdf:type rdf:resource="http://reliant.teknowledge.com/DAML/SUMO.owl#AsymmetricRelation" /><rdfs:domain rdf:resource="http://reliant.teknowledge.com/DAML/SUMO.owl#Agent" /><rdfs:range rdf:resource="http://reliant.teknowledge.com/DAML/SUMO.owl#Position" /></owl:ObjectProperty><owl:ObjectProperty rdf:ID="legalSystemType"><rdfs:comment>(legalSystemType ?AREA ?TYPE) means 

that the GeopoliticalArea ?AREA has a legal system characterized by 

the LegalSystemAttribute ?TYPE.  For example, (legalSystemType 

UnitedStates EnglishCommonLaw).  A legal system may have multiple 

characteristics.</rdfs:comment><rdf:type rdf:resource="http://reliant.teknowledge.com/DAML/SUMO.owl#BinaryPredicate" /><rdfs:domain rdf:resource="http://reliant.teknowledge.com/DAML/SUMO.owl#GeopoliticalArea" /><rdfs:range rdf:resource="#LegalSystemAttribute" /></owl:ObjectProperty><owl:ObjectProperty rdf:ID="lender"><rdfs:comment>(lender ?Loan ?Agent) means that ?Agent is a private, public or 

institutional entity that put up the funds for the ?Loan.</rdfs:comment><rdfs:domain rdf:resource="#Loan" /><rdfs:range rdf:resource="http://reliant.teknowledge.com/DAML/SUMO.owl#CognitiveAgent" /><rdfs:subPropertyOf rdf:resource="#agreementMember" /></owl:ObjectProperty><owl:ObjectProperty rdf:ID="loanForPurchase"><rdfs:comment>(loanForPurchase ?ACCOUNT ?PRODUCT) means that ?ACCOUNT is a 

loan to finance the purchase of ?PRODUCT.</rdfs:comment><rdf:type rdf:resource="http://reliant.teknowledge.com/DAML/SUMO.owl#BinaryPredicate" /><rdfs:domain rdf:resource="#Loan" /><rdfs:range rdf:resource="http://reliant.teknowledge.com/DAML/SUMO.owl#Object" /></owl:ObjectProperty><owl:ObjectProperty rdf:ID="localLongName"><rdfs:comment>(localLongName ?NAME ?THING) means that 

the string ?NAME is the long form of the name used for ?THING in its local 

area or language.</rdfs:comment><rdfs:subPropertyOf rdf:resource="http://reliant.teknowledge.com/DAML/SUMO.owl#names" /></owl:ObjectProperty><owl:ObjectProperty rdf:ID="localShortName"><rdfs:comment>(localShortName ?NAME ?THING) means that 

the string ?NAME is the short form of the name used for ?THING in its 

local area or language.</rdfs:comment><rdfs:subPropertyOf rdf:resource="http://reliant.teknowledge.com/DAML/SUMO.owl#names" /></owl:ObjectProperty><owl:ObjectProperty rdf:ID="loss"><rdfs:comment>The amount by which the cost of an investment or 

business operation exceeds its return, i.e. the negative quantity left 

after subtracting for all expenses.</rdfs:comment><rdf:type rdf:resource="http://reliant.teknowledge.com/DAML/SUMO.owl#AsymmetricRelation" /><rdfs:domain rdf:resource="http://reliant.teknowledge.com/DAML/SUMO.owl#FinancialTransaction" /><rdfs:range rdf:resource="http://reliant.teknowledge.com/DAML/SUMO.owl#CurrencyMeasure" /></owl:ObjectProperty><owl:ObjectProperty rdf:ID="maturityDate"><rdfs:comment>The date on which the principal amount of the account 

becomes due and payable.</rdfs:comment><rdf:type rdf:resource="http://reliant.teknowledge.com/DAML/SUMO.owl#BinaryPredicate" /><rdfs:domain rdf:resource="#FinancialAccount" /><rdfs:range rdf:resource="http://reliant.teknowledge.com/DAML/SUMO.owl#Day" /></owl:ObjectProperty><owl:ObjectProperty rdf:ID="measurementReading"><rdfs:comment>(measurementReading ?DEVICE ?QUANTITY) 

means that ?QUANTITY is a reading of the MeasuringDevice ?DEVICE, e.g. if 

?THERMOMETER is a Thermometer, (measurementReading ?THERMOMETER 

(MeasureFn 42 CelsiusDegree)) would mean that ?THERMOMETER registers 42 

degrees Celsius.</rdfs:comment><rdf:type rdf:resource="http://reliant.teknowledge.com/DAML/SUMO.owl#BinaryPredicate" /><rdfs:domain rdf:resource="http://reliant.teknowledge.com/DAML/SUMO.owl#MeasuringDevice" /><rdfs:range rdf:resource="http://reliant.teknowledge.com/DAML/SUMO.owl#ConstantQuantity" /></owl:ObjectProperty><owl:ObjectProperty rdf:ID="memberType"><rdfs:comment>(memberType ?GROUP ?TYPE) means that all 

the members of the Collection ?GROUP belong to the SetOrClass 

?TYPE.</rdfs:comment><rdf:type rdf:resource="http://reliant.teknowledge.com/DAML/SUMO.owl#BinaryPredicate" /><rdfs:domain rdf:resource="http://reliant.teknowledge.com/DAML/SUMO.owl#Collection" /><rdfs:range rdf:resource="http://reliant.teknowledge.com/DAML/SUMO.owl#SetOrClass" /></owl:ObjectProperty><owl:ObjectProperty rdf:ID="middleName"><rdfs:comment>(middleName ?CHAR ?INDIV) means that the 

SymbolicString ?CHAR contains the middle name of the Human ?INDIV.</rdfs:comment><rdfs:comment>(middleName ?CHAR ?INDIV) means that the 

SymbolicString ?CHAR contains the middle name of the Human ?INDIV.</rdfs:comment><rdf:type rdf:resource="http://reliant.teknowledge.com/DAML/SUMO.owl#BinaryPredicate" /><rdf:type rdf:resource="http://reliant.teknowledge.com/DAML/SUMO.owl#AsymmetricRelation" /><rdf:type rdf:resource="http://reliant.teknowledge.com/DAML/SUMO.owl#BinaryPredicate" /><rdf:type rdf:resource="http://reliant.teknowledge.com/DAML/SUMO.owl#AsymmetricRelation" /><rdfs:domain rdf:resource="http://reliant.teknowledge.com/DAML/SUMO.owl#SymbolicString" /><rdfs:range rdf:resource="http://reliant.teknowledge.com/DAML/SUMO.owl#Human" /><rdfs:subPropertyOf rdf:resource="http://reliant.teknowledge.com/DAML/SUMO.owl#names" /><rdfs:subPropertyOf rdf:resource="http://reliant.teknowledge.com/DAML/SUMO.owl#names" /></owl:ObjectProperty><owl:ObjectProperty rdf:ID="most"><rdfs:comment>(most ?MOST ?WHOLE) means that ?MOST is a part 

of ?WHOLE that is greater than half of ?WHOLE.</rdfs:comment><rdfs:subPropertyOf rdf:resource="http://reliant.teknowledge.com/DAML/SUMO.owl#part" /></owl:ObjectProperty><owl:DatatypeProperty rdf:ID="multiplicativeFactor"><rdfs:comment>(multiplicativeFactor ?NUMBER1 ?NUMBER2) 

means that ?NUMBER1 is a factor of ?NUMBER2, i.e. ?NUMBER1 can be multiplied by 

some Integer to give ?NUMBER2 as a result.</rdfs:comment><rdf:type rdf:resource="http://reliant.teknowledge.com/DAML/SUMO.owl#BinaryPredicate" /><rdf:type rdf:resource="http://reliant.teknowledge.com/DAML/SUMO.owl#TransitiveRelation" /><rdfs:domain rdf:resource="http://reliant.teknowledge.com/DAML/SUMO.owl#Integer" /><rdfs:range rdf:resource="http://reliant.teknowledge.com/DAML/SUMO.owl#Integer" /></owl:DatatypeProperty><owl:ObjectProperty rdf:ID="neighbor"><rdfs:comment>(neighbor ?PERSON1 ?PERSON2) means that ?PERSON1 is 

a neighbor of ?PERSON2, i.e. ?PERSON1 and ?PERSON2 have their homes Near 

one another.</rdfs:comment><rdf:type rdf:resource="http://reliant.teknowledge.com/DAML/SUMO.owl#BinaryPredicate" /><rdf:type rdf:resource="http://reliant.teknowledge.com/DAML/SUMO.owl#SymmetricRelation" /><rdf:type rdf:resource="http://reliant.teknowledge.com/DAML/SUMO.owl#IrreflexiveRelation" /><rdfs:domain rdf:resource="http://reliant.teknowledge.com/DAML/SUMO.owl#Human" /><rdfs:range rdf:resource="http://reliant.teknowledge.com/DAML/SUMO.owl#Human" /></owl:ObjectProperty><owl:ObjectProperty rdf:ID="nephew"><rdfs:comment>(nephew ?NEPHEW ?PERSON) means that ?NEPHEW is 

the son of a sibling of ?PERSON.</rdfs:comment><rdfs:domain rdf:resource="http://reliant.teknowledge.com/DAML/SUMO.owl#Man" /><rdfs:range rdf:resource="http://reliant.teknowledge.com/DAML/SUMO.owl#Human" /><rdfs:subPropertyOf rdf:resource="http://reliant.teknowledge.com/DAML/SUMO.owl#familyRelation" /></owl:ObjectProperty><owl:ObjectProperty rdf:ID="niece"><rdfs:comment>(niece ?NIECE ?PERSON) means that ?NIECE is 

the daughter of a sibling of ?PERSON.</rdfs:comment><rdfs:domain rdf:resource="http://reliant.teknowledge.com/DAML/SUMO.owl#Woman" /><rdfs:range rdf:resource="http://reliant.teknowledge.com/DAML/SUMO.owl#Human" /><rdfs:subPropertyOf rdf:resource="http://reliant.teknowledge.com/DAML/SUMO.owl#familyRelation" /></owl:ObjectProperty><owl:ObjectProperty rdf:ID="occupation"><rdfs:comment>(occupation ?PERSON ?TYPE) means that the occupation 

of ?PERSON is ?TYPE.  This predicate is most often used in combination with the 

function OccupationFn, e.g. (occupation PoliceOfficerWilkins (OccupationFn 

LawEnforcement)).</rdfs:comment><rdf:type rdf:resource="http://reliant.teknowledge.com/DAML/SUMO.owl#BinaryPredicate" /><rdfs:domain rdf:resource="http://reliant.teknowledge.com/DAML/SUMO.owl#Human" /><rdfs:range rdf:resource="http://reliant.teknowledge.com/DAML/SUMO.owl#FinancialTransaction" /></owl:ObjectProperty><owl:ObjectProperty rdf:ID="older"><rdfs:comment>(older ?OBJ1 ?OBJ2) means that ?OBJ1 is older than 

?OBJ2, i.e. the age of ?OBJ1 is greaterThan the age of ?OBJ2.</rdfs:comment><rdf:type rdf:resource="http://reliant.teknowledge.com/DAML/SUMO.owl#BinaryPredicate" /><rdfs:domain rdf:resource="http://reliant.teknowledge.com/DAML/SUMO.owl#Object" /><rdfs:range rdf:resource="http://reliant.teknowledge.com/DAML/SUMO.owl#Object" /></owl:ObjectProperty><owl:ObjectProperty rdf:ID="onboard"><rdfs:comment>(onboard ?OBJ ?VEHICLE) means that the 

SelfConnectedObject ?OBJ is inside the Vehicle ?VEHICLE.</rdfs:comment><rdfs:domain rdf:resource="http://reliant.teknowledge.com/DAML/SUMO.owl#SelfConnectedObject" /><rdfs:range rdf:resource="http://reliant.teknowledge.com/DAML/SUMO.owl#Vehicle" /><rdfs:subPropertyOf rdf:resource="http://reliant.teknowledge.com/DAML/SUMO.owl#located" /></owl:ObjectProperty><owl:ObjectProperty rdf:ID="orbits"><rdfs:comment>(orbits ?SATELLITE ?FOCUS) means that the Object 

?SATELLITE revolves around the AstronomicalBody ?FOCUS.</rdfs:comment><rdf:type rdf:resource="http://reliant.teknowledge.com/DAML/SUMO.owl#BinaryPredicate" /><rdf:type rdf:resource="http://reliant.teknowledge.com/DAML/SUMO.owl#AsymmetricRelation" /><rdfs:domain rdf:resource="http://reliant.teknowledge.com/DAML/SUMO.owl#Object" /><rdfs:range rdf:resource="http://reliant.teknowledge.com/DAML/SUMO.owl#AstronomicalBody" /></owl:ObjectProperty><owl:ObjectProperty rdf:about="http://reliant.teknowledge.com/DAML/SUMO.owl#origin"><rdfs:subPropertyOf rdf:resource="#involvedInEvent" /></owl:ObjectProperty><owl:ObjectProperty rdf:ID="parasite"><rdfs:comment>(parasite ?ORGANISM1 ?ORGANISM2) means that there 

is a parasitic relationship between ?ORGANISM1 and ?ORGANISM2, i.e. ?ORGANISM1 

inhabits and obtains nourishment from ?ORGANISM2 in such a way that 

?ORGANISM2 is injured.</rdfs:comment><rdf:type rdf:resource="http://reliant.teknowledge.com/DAML/SUMO.owl#BinaryPredicate" /><rdfs:domain rdf:resource="http://reliant.teknowledge.com/DAML/SUMO.owl#Organism" /><rdfs:range rdf:resource="http://reliant.teknowledge.com/DAML/SUMO.owl#Organism" /></owl:ObjectProperty><owl:ObjectProperty rdf:about="http://reliant.teknowledge.com/DAML/SUMO.owl#path"><rdfs:subPropertyOf rdf:resource="#involvedInEvent" /></owl:ObjectProperty><owl:ObjectProperty rdf:ID="pathInSystem"><rdfs:comment>(pathInSystem ?PATH ?SYSTEM) means that 

the Physical thing ?PATH consists of one or more connected routes in 

the PhysicalSystem ?SYSTEM.</rdfs:comment><rdf:type rdf:resource="http://reliant.teknowledge.com/DAML/SUMO.owl#BinaryPredicate" /><rdfs:domain rdf:resource="http://reliant.teknowledge.com/DAML/SUMO.owl#Transitway" /><rdfs:range rdf:resource="#TransportationSystem" /><rdfs:subPropertyOf rdf:resource="http://reliant.teknowledge.com/DAML/SUMO.owl#part" /></owl:ObjectProperty><owl:DatatypeProperty rdf:ID="pathLength"><rdfs:comment>A BinaryPredicate that specifies the 

length (in number of GraphNodes) of a GraphPath.

(pathLength ?PATH ?NUMBER) means that there are ?NUMBER nodes in 

the GraphPath ?PATH.</rdfs:comment><rdf:type rdf:resource="http://reliant.teknowledge.com/DAML/SUMO.owl#BinaryPredicate" /><rdf:type rdf:resource="http://reliant.teknowledge.com/DAML/SUMO.owl#AsymmetricRelation" /><rdf:type rdf:resource="http://reliant.teknowledge.com/DAML/SUMO.owl#IrreflexiveRelation" /><rdfs:domain rdf:resource="#GraphPath" /><rdfs:range rdf:resource="http://reliant.teknowledge.com/DAML/SUMO.owl#PositiveInteger" /></owl:DatatypeProperty><owl:ObjectProperty rdf:about="http://reliant.teknowledge.com/DAML/SUMO.owl#patient"><rdfs:subPropertyOf rdf:resource="#involvedInEvent" /></owl:ObjectProperty><owl:ObjectProperty rdf:ID="patientMedical"><rdfs:comment>The relation of receiving medical care 

from a recognized medical practitioner.  (patientMedical ?PATIENT 

?DOCTOR) means that ?PATIENT is the patient of ?DOCTOR.  Note that 

argument type restriction on the second argument is CognitiveAgent 

to allow for cases where someone is the patient of an Organization, 

viz. a CareOrganization.</rdfs:comment><rdf:type rdf:resource="http://reliant.teknowledge.com/DAML/SUMO.owl#BinaryPredicate" /><rdfs:domain rdf:resource="http://reliant.teknowledge.com/DAML/SUMO.owl#Human" /><rdfs:range rdf:resource="http://reliant.teknowledge.com/DAML/SUMO.owl#CognitiveAgent" /></owl:ObjectProperty><owl:ObjectProperty rdf:ID="placeOfDeath"><rdfs:comment>(placeOfDeath ?INDIV ?PLACE) means that the Animal ?INDIV died 

at the location ?PLACE.  The location may be a geographic area or a building, such as a hospital.</rdfs:comment><rdf:type rdf:resource="http://reliant.teknowledge.com/DAML/SUMO.owl#BinaryPredicate" /><rdfs:domain rdf:resource="http://reliant.teknowledge.com/DAML/SUMO.owl#Animal" /><rdfs:range rdf:resource="http://reliant.teknowledge.com/DAML/SUMO.owl#Object" /></owl:ObjectProperty><owl:ObjectProperty rdf:ID="plaintiff"><rdfs:comment>(plaintiff ?AGENT ?ACTION) means that ?AGENT 

is responsible for initiating the LegalAction ?ACTION.</rdfs:comment><rdfs:domain rdf:resource="http://reliant.teknowledge.com/DAML/SUMO.owl#CognitiveAgent" /><rdfs:range rdf:resource="http://reliant.teknowledge.com/DAML/SUMO.owl#LegalAction" /><rdfs:subPropertyOf rdf:resource="http://reliant.teknowledge.com/DAML/SUMO.owl#agent" /><rdfs:subPropertyOf rdf:resource="#involvedInEvent" /></owl:ObjectProperty><owl:ObjectProperty rdf:ID="postalBoxNumber"><rdfs:comment>(postalBoxNumber ?NUMBER ?ADDRESS) means 

that the post office box ?NUMBER is part of the address ?ADDRESS.</rdfs:comment><rdfs:domain rdf:resource="http://reliant.teknowledge.com/DAML/SUMO.owl#PositiveInteger" /><rdfs:range rdf:resource="#Address" /><rdfs:subPropertyOf rdf:resource="http://reliant.teknowledge.com/DAML/SUMO.owl#uniqueIdentifier" /></owl:ObjectProperty><owl:ObjectProperty rdf:ID="postalCode"><rdfs:comment>(postalCode ?NUMBER ?ADDRESS) means that the 

the postal code, e.g. zip code, ?NUMBER is part of the address ?ADDRESS.</rdfs:comment><rdfs:domain rdf:resource="http://reliant.teknowledge.com/DAML/SUMO.owl#PositiveInteger" /><rdfs:range rdf:resource="#Address" /><rdfs:subPropertyOf rdf:resource="http://reliant.teknowledge.com/DAML/SUMO.owl#uniqueIdentifier" /></owl:ObjectProperty><owl:DatatypeProperty rdf:ID="potentialOfHydrogen"><rdfs:comment>(potentialOfHydrogen ?SOLUTION ?NUMBER) 

means that the Solution ?SOLUTION has a pH value of ?NUMBER.  The ph varies 

between 0 and 14, and it is a measure of the acidity or alkalinity of ?SOLUTION.  

More precisely,  and it is the logarithm of the reciprocal of the quantity of 

AtomGrams of Hydrogen ions.</rdfs:comment><rdf:type rdf:resource="http://reliant.teknowledge.com/DAML/SUMO.owl#BinaryPredicate" /><rdfs:domain rdf:resource="http://reliant.teknowledge.com/DAML/SUMO.owl#Solution" /><rdfs:range rdf:resource="http://reliant.teknowledge.com/DAML/SUMO.owl#RealNumber" /></owl:DatatypeProperty><owl:ObjectProperty rdf:ID="powerPlant"><rdfs:comment>(powerPlant ?GENERATOR ?THING) means that 

the Device ?GENERATOR is the power-producing component of the Artifact 

?THING which provides the energy for its operation.</rdfs:comment><rdf:type rdf:resource="http://reliant.teknowledge.com/DAML/SUMO.owl#BinaryPredicate" /><rdf:type rdf:resource="http://reliant.teknowledge.com/DAML/SUMO.owl#AsymmetricRelation" /><rdf:type rdf:resource="http://reliant.teknowledge.com/DAML/SUMO.owl#IrreflexiveRelation" /><rdfs:domain rdf:resource="http://reliant.teknowledge.com/DAML/SUMO.owl#Device" /><rdfs:range rdf:resource="http://reliant.teknowledge.com/DAML/SUMO.owl#Artifact" /><rdfs:subPropertyOf rdf:resource="http://reliant.teknowledge.com/DAML/SUMO.owl#component" /></owl:ObjectProperty><owl:ObjectProperty rdf:ID="primaryGeopoliticalSubdivision"><rdfs:comment>(primaryGeopoliticalSubdivision ?AREA ?COUNTRY) means that the 

GeopoliticalArea ?AREA is one of the first-order administrative 

divisions of the Nation ?COUNTRY.  For example, in the United States, 

any of the fifty states.  This does not include subordinate regions that 

have a lesser status, such as British Crown colonies, U.S. territories, 

or protectorates.  See geopoliticalSubdivision.</rdfs:comment><rdf:type rdf:resource="http://reliant.teknowledge.com/DAML/SUMO.owl#BinaryPredicate" /><rdf:type rdf:resource="http://reliant.teknowledge.com/DAML/SUMO.owl#AsymmetricRelation" /><rdfs:domain rdf:resource="http://reliant.teknowledge.com/DAML/SUMO.owl#GeopoliticalArea" /><rdfs:range rdf:resource="http://reliant.teknowledge.com/DAML/SUMO.owl#GeopoliticalArea" /><rdfs:subPropertyOf rdf:resource="http://reliant.teknowledge.com/DAML/SUMO.owl#geopoliticalSubdivision" /></owl:ObjectProperty><owl:ObjectProperty rdf:ID="principalAmount"><rdfs:comment>(principalAmount ?ACCOUNT ?BALANCE) means 

that ?BALANCE is the amount originally borrowed (excluding interest).</rdfs:comment><rdf:type rdf:resource="http://reliant.teknowledge.com/DAML/SUMO.owl#BinaryPredicate" /><rdfs:domain rdf:resource="#FinancialAccount" /><rdfs:range rdf:resource="http://reliant.teknowledge.com/DAML/SUMO.owl#CurrencyMeasure" /></owl:ObjectProperty><owl:ObjectProperty rdf:ID="profit"><rdfs:comment>The positive gain from an investment or business 

operation after subtracting for all expenses.</rdfs:comment><rdf:type rdf:resource="http://reliant.teknowledge.com/DAML/SUMO.owl#AsymmetricRelation" /><rdfs:domain rdf:resource="http://reliant.teknowledge.com/DAML/SUMO.owl#FinancialTransaction" /><rdfs:range rdf:resource="http://reliant.teknowledge.com/DAML/SUMO.owl#CurrencyMeasure" /></owl:ObjectProperty><owl:DatatypeProperty rdf:ID="protonNumber"><rdfs:comment>(protonNumber ?SUBSTANCE ?NUMBER) means that 

the PureSubstance ?SUBSTANCE has the number of Protons ?NUMBER.</rdfs:comment><rdf:type rdf:resource="http://reliant.teknowledge.com/DAML/SUMO.owl#BinaryPredicate" /><rdf:type rdf:resource="http://reliant.teknowledge.com/DAML/SUMO.owl#SingleValuedRelation" /><rdf:type rdf:resource="http://reliant.teknowledge.com/DAML/SUMO.owl#TotalValuedRelation" /><rdfs:domain rdf:resource="http://reliant.teknowledge.com/DAML/SUMO.owl#PureSubstance" /><rdfs:range rdf:resource="http://reliant.teknowledge.com/DAML/SUMO.owl#PositiveInteger" /></owl:DatatypeProperty><owl:ObjectProperty rdf:ID="quarter"><rdfs:comment>(quarter ?QUART ?WHOLE) means that ?QUART is a 

quarter of ?WHOLE.</rdfs:comment><rdfs:subPropertyOf rdf:resource="http://reliant.teknowledge.com/DAML/SUMO.owl#part" /></owl:ObjectProperty><owl:ObjectProperty rdf:ID="reactant"><rdfs:comment>(reactant ?PROCESS ?SUBSTANCE) means that ?SUBSTANCE 

is a chemical reactant in the chemical reaction ?PROCESS, i.e. ?SUBSTANCE is 

present at the beginning of the chemical reaction ?PROCESS.</rdfs:comment><rdfs:domain rdf:resource="http://reliant.teknowledge.com/DAML/SUMO.owl#ChemicalProcess" /><rdfs:range rdf:resource="http://reliant.teknowledge.com/DAML/SUMO.owl#Substance" /><rdfs:subPropertyOf rdf:resource="http://reliant.teknowledge.com/DAML/SUMO.owl#resource" /></owl:ObjectProperty><owl:ObjectProperty rdf:ID="reagent"><rdfs:comment>(reagent ?PROCESS ?SUBSTANCE) means that ?SUBSTANCE 

is a chemical agent in the chemical reaction ?PROCESS.</rdfs:comment><rdfs:domain rdf:resource="http://reliant.teknowledge.com/DAML/SUMO.owl#ChemicalProcess" /><rdfs:range rdf:resource="http://reliant.teknowledge.com/DAML/SUMO.owl#Substance" /><rdfs:subPropertyOf rdf:resource="http://reliant.teknowledge.com/DAML/SUMO.owl#instrument" /></owl:ObjectProperty><owl:ObjectProperty rdf:ID="registeredItem"><rdfs:comment>(registeredItem ?DOCUMENT ?ITEM) means 

that the Text ?DOCUMENT contains an official record of the Physical 

thing ?ITEM.  The registered item could be an object or an event, e.g., 

an automobile, a ship, a marriage, an adoption.</rdfs:comment><rdf:type rdf:resource="http://reliant.teknowledge.com/DAML/SUMO.owl#BinaryPredicate" /><rdfs:domain rdf:resource="http://reliant.teknowledge.com/DAML/SUMO.owl#Text" /><rdfs:range rdf:resource="http://reliant.teknowledge.com/DAML/SUMO.owl#Physical" /><rdfs:subPropertyOf rdf:resource="http://reliant.teknowledge.com/DAML/SUMO.owl#refers" /></owl:ObjectProperty><owl:ObjectProperty rdf:ID="relatedEvent"><rdfs:comment>(relatedEvent ?EVENT1 ?EVENT2) means 

that the Process ?EVENT1 is related to the Process ?EVENT2.  The 

relationship is between separate individual events, not events and 

their subprocesses.  On the other hand, two subProcesses of the same 

overarching event may be relatedEvents.  The argument order does not 

imply temporal ordering.</rdfs:comment><rdf:type rdf:resource="http://reliant.teknowledge.com/DAML/SUMO.owl#BinaryPredicate" /><rdf:type rdf:resource="http://reliant.teknowledge.com/DAML/SUMO.owl#SymmetricRelation" /><rdfs:domain rdf:resource="http://reliant.teknowledge.com/DAML/SUMO.owl#Process" /></owl:ObjectProperty><owl:ObjectProperty rdf:ID="religiousAffiliationOfOrganization"><rdfs:comment>(religiousAffiliationOfOrganization 

?ORG ?BELIEF) means that one of the goals of ?ORG is to advance the religious teachings 

of the BeliefGroup ?BELIEF.</rdfs:comment><rdf:type rdf:resource="http://reliant.teknowledge.com/DAML/SUMO.owl#BinaryPredicate" /><rdfs:domain rdf:resource="http://reliant.teknowledge.com/DAML/SUMO.owl#Organization" /><rdfs:range rdf:resource="http://reliant.teknowledge.com/DAML/SUMO.owl#BeliefGroup" /></owl:ObjectProperty><owl:ObjectProperty rdf:about="http://reliant.teknowledge.com/DAML/SUMO.owl#resource"><rdfs:subPropertyOf rdf:resource="#involvedInEvent" /></owl:ObjectProperty><owl:ObjectProperty rdf:about="http://reliant.teknowledge.com/DAML/SUMO.owl#result"><rdfs:subPropertyOf rdf:resource="#involvedInEvent" /></owl:ObjectProperty><owl:ObjectProperty rdf:ID="routeInSystem"><rdfs:comment>(routeInSystem ?PART ?SYSTEM) means that 

the Transitway ?PART is an established route of the 

TransportationSystem ?SYSTEM.</rdfs:comment><rdf:type rdf:resource="http://reliant.teknowledge.com/DAML/SUMO.owl#BinaryPredicate" /><rdfs:domain rdf:resource="http://reliant.teknowledge.com/DAML/SUMO.owl#Transitway" /><rdfs:range rdf:resource="#TransportationSystem" /><rdfs:subPropertyOf rdf:resource="#pathInSystem" /></owl:ObjectProperty><owl:ObjectProperty rdf:ID="secretesSubstance"><rdfs:comment>(secretesSubstance ?OBJ ?STUFF) means 

that the subclass of OrganicObject (either Organism or BodyPart) 

?OBJ produces the subclass of Substance ?STUFF.</rdfs:comment><rdf:type rdf:resource="http://reliant.teknowledge.com/DAML/SUMO.owl#BinaryPredicate" /><rdfs:domain rdf:resource="http://reliant.teknowledge.com/DAML/SUMO.owl#OrganicObject" /><rdfs:range rdf:resource="http://reliant.teknowledge.com/DAML/SUMO.owl#NaturalSubstance" /></owl:ObjectProperty><owl:ObjectProperty rdf:ID="securedBy"><rdfs:comment>Assets pledged by a borrower to secure a loan 

or other credit, and subject to seizure in the event of FinancialDefault.</rdfs:comment><rdf:type rdf:resource="http://reliant.teknowledge.com/DAML/SUMO.owl#BinaryPredicate" /><rdfs:domain rdf:resource="#FinancialAccount" /><rdfs:range rdf:resource="http://reliant.teknowledge.com/DAML/SUMO.owl#Object" /></owl:ObjectProperty><owl:ObjectProperty rdf:ID="sententialObject"><rdfs:comment>(sententialObject ?OBJECT ?SENTENCE) 

means that the NounPhrase ?OBJECT is the object of the Sentence 

?SENTENCE.</rdfs:comment><rdfs:domain rdf:resource="http://reliant.teknowledge.com/DAML/SUMO.owl#NounPhrase" /><rdfs:range rdf:resource="http://reliant.teknowledge.com/DAML/SUMO.owl#Sentence" /><rdfs:subPropertyOf rdf:resource="#grammaticalRelation" /></owl:ObjectProperty><owl:ObjectProperty rdf:ID="sententialSubject"><rdfs:comment>(sententialSubject ?SUBJECT ?SENTENCE) 

means that the NounPhrase ?SUBJECT is the subject of the Sentence 

?SENTENCE.</rdfs:comment><rdfs:domain rdf:resource="http://reliant.teknowledge.com/DAML/SUMO.owl#NounPhrase" /><rdfs:range rdf:resource="http://reliant.teknowledge.com/DAML/SUMO.owl#Sentence" /><rdfs:subPropertyOf rdf:resource="#grammaticalRelation" /></owl:ObjectProperty><owl:ObjectProperty rdf:ID="sideOfFigure"><rdfs:comment>(sideOfFigure ?SIDE ?FIGURE) means that the 

OneDimensionalFigure ?SIDE is a side of the Polygon ?FIGURE.</rdfs:comment><rdfs:domain rdf:resource="http://reliant.teknowledge.com/DAML/SUMO.owl#OneDimensionalFigure" /><rdfs:range rdf:resource="#Polygon" /><rdfs:subPropertyOf rdf:resource="http://reliant.teknowledge.com/DAML/SUMO.owl#geometricPart" /></owl:ObjectProperty><owl:ObjectProperty rdf:ID="signedBy"><rdfs:comment>(signedBy ?Certificate ?Agent) means that ?Certificate 

has been signed by ?Agent.</rdfs:comment><rdf:type rdf:resource="http://reliant.teknowledge.com/DAML/SUMO.owl#BinaryPredicate" /><rdfs:domain rdf:resource="http://reliant.teknowledge.com/DAML/SUMO.owl#Certificate" /><rdfs:range rdf:resource="http://reliant.teknowledge.com/DAML/SUMO.owl#CognitiveAgent" /></owl:ObjectProperty><owl:ObjectProperty rdf:ID="speaksLanguage"><rdfs:comment>(speaksLanguage ?AGENT ?LANGUAGE) means that the 

SentientAgent ?AGENT is capable of understanding and/or generating the Language 

?LANGUAGE.</rdfs:comment><rdf:type rdf:resource="http://reliant.teknowledge.com/DAML/SUMO.owl#BinaryPredicate" /><rdfs:domain rdf:resource="http://reliant.teknowledge.com/DAML/SUMO.owl#SentientAgent" /><rdfs:range rdf:resource="http://reliant.teknowledge.com/DAML/SUMO.owl#Language" /></owl:ObjectProperty><owl:ObjectProperty rdf:ID="stepfather"><rdfs:comment>(stepfather ?PERSON ?FATHER) means that ?FATHER 

is the stepfather of ?PERSON, i.e. ?FATHER is the spouse of the mother 

of ?PERSON, without also being the father of ?PERSON.</rdfs:comment><rdfs:domain rdf:resource="http://reliant.teknowledge.com/DAML/SUMO.owl#Human" /><rdfs:range rdf:resource="http://reliant.teknowledge.com/DAML/SUMO.owl#Man" /><rdfs:subPropertyOf rdf:resource="http://reliant.teknowledge.com/DAML/SUMO.owl#legalRelation" /></owl:ObjectProperty><owl:ObjectProperty rdf:ID="stepmother"><rdfs:comment>(stepmother ?PERSON ?MOTHER) means that ?MOTHER 

is the stepmother of ?PERSON, i.e. ?MOTHER is the spouse of the father 

of ?PERSON, without also being the mother of ?PERSON.</rdfs:comment><rdfs:domain rdf:resource="http://reliant.teknowledge.com/DAML/SUMO.owl#Human" /><rdfs:range rdf:resource="http://reliant.teknowledge.com/DAML/SUMO.owl#Woman" /><rdfs:subPropertyOf rdf:resource="http://reliant.teknowledge.com/DAML/SUMO.owl#legalRelation" /></owl:ObjectProperty><owl:ObjectProperty rdf:ID="stockHolder"><rdfs:comment>(stockHolder ?Stock ?Agent) means that 

?Agent possesses the Stock ?Stock.</rdfs:comment><rdf:type rdf:resource="http://reliant.teknowledge.com/DAML/SUMO.owl#BinaryPredicate" /><rdfs:domain rdf:resource="#Stock" /><rdfs:range rdf:resource="http://reliant.teknowledge.com/DAML/SUMO.owl#CognitiveAgent" /></owl:ObjectProperty><owl:ObjectProperty rdf:ID="streetAddress"><rdfs:comment>(streetAddress ?STREET ?ADDRESS) means 

that the Roadway ?STREET is part of the address ?ADDRESS.</rdfs:comment><rdfs:domain rdf:resource="http://reliant.teknowledge.com/DAML/SUMO.owl#Roadway" /><rdfs:range rdf:resource="#Address" /><rdfs:subPropertyOf rdf:resource="#address" /></owl:ObjectProperty><owl:ObjectProperty rdf:ID="streetNumber"><rdfs:comment>(streetNumber ?BUILDING ?ADDRESS) means 

that the Building ?BUILDING is part of the address ?ADDRESS.</rdfs:comment><rdfs:domain rdf:resource="http://reliant.teknowledge.com/DAML/SUMO.owl#Building" /><rdfs:range rdf:resource="#Address" /><rdfs:subPropertyOf rdf:resource="#address" /></owl:ObjectProperty><owl:ObjectProperty rdf:ID="student"><rdfs:comment>(student ?AGENT ?ORG) means that ?AGENT is enrolled 

in the EducationalOrganization ?ORG.</rdfs:comment><rdfs:domain rdf:resource="http://reliant.teknowledge.com/DAML/SUMO.owl#CognitiveAgent" /><rdfs:range rdf:resource="http://reliant.teknowledge.com/DAML/SUMO.owl#EducationalOrganization" /><rdfs:subPropertyOf rdf:resource="http://reliant.teknowledge.com/DAML/SUMO.owl#member" /></owl:ObjectProperty><owl:ObjectProperty rdf:ID="subField"><rdfs:comment>(subField ?FIELD1 ?FIELD2) means that ?FIELD1 is a proper 

part of the FieldOfStudy ?FIELD2.  For example, Physiology is a subField of 

Biology.</rdfs:comment><rdf:type rdf:resource="http://reliant.teknowledge.com/DAML/SUMO.owl#TransitiveRelation" /><rdf:type rdf:resource="http://reliant.teknowledge.com/DAML/SUMO.owl#IrreflexiveRelation" /><rdfs:domain rdf:resource="http://reliant.teknowledge.com/DAML/SUMO.owl#FieldOfStudy" /><rdfs:range rdf:resource="http://reliant.teknowledge.com/DAML/SUMO.owl#FieldOfStudy" /><rdfs:subPropertyOf rdf:resource="http://reliant.teknowledge.com/DAML/SUMO.owl#subProposition" /></owl:ObjectProperty><owl:ObjectProperty rdf:ID="subGraph"><rdfs:comment>The relation between two Graphs when one 

Graph is a part of the other.  (subGraph ?GRAPH1 ?GRAPH2) means 

that ?GRAPH1 is a part of ?GRAPH2.</rdfs:comment><rdf:type rdf:resource="http://reliant.teknowledge.com/DAML/SUMO.owl#BinaryPredicate" /><rdf:type rdf:resource="http://reliant.teknowledge.com/DAML/SUMO.owl#ReflexiveRelation" /><rdf:type rdf:resource="http://reliant.teknowledge.com/DAML/SUMO.owl#TransitiveRelation" /><rdfs:domain rdf:resource="#Graph" /><rdfs:range rdf:resource="#Graph" /></owl:ObjectProperty><owl:ObjectProperty rdf:ID="subRegion"><rdfs:comment>(subRegion ?PART ?WHOLE) means that the Region 

?PART is a part of the Region ?WHOLE.</rdfs:comment><rdfs:domain rdf:resource="http://reliant.teknowledge.com/DAML/SUMO.owl#Region" /><rdfs:range rdf:resource="http://reliant.teknowledge.com/DAML/SUMO.owl#Region" /><rdfs:subPropertyOf rdf:resource="http://reliant.teknowledge.com/DAML/SUMO.owl#part" /></owl:ObjectProperty><owl:ObjectProperty rdf:ID="tangent"><rdfs:comment>(tangent ?LINE ?CIRCLE) means that the straight line 

?LINE is tangent to the Circle ?CIRCLE, i.e. ?LINE touches ?CIRCLE without 

intersecting it.</rdfs:comment><rdf:type rdf:resource="http://reliant.teknowledge.com/DAML/SUMO.owl#BinaryPredicate" /><rdfs:domain rdf:resource="http://reliant.teknowledge.com/DAML/SUMO.owl#OneDimensionalFigure" /><rdfs:range rdf:resource="#Circle" /></owl:ObjectProperty><owl:ObjectProperty rdf:ID="targetInAttack"><rdf:type rdf:resource="http://reliant.teknowledge.com/DAML/SUMO.owl#BinaryPredicate" /><rdfs:domain rdf:resource="http://reliant.teknowledge.com/DAML/SUMO.owl#Process" /><rdfs:range rdf:resource="http://reliant.teknowledge.com/DAML/SUMO.owl#Object" /></owl:ObjectProperty><owl:ObjectProperty rdf:ID="teacher"><rdfs:comment>(teacher ?AGENT ?ORG) means that ?AGENT is a 

teacher at the EducationalOrganization ?ORG.</rdfs:comment><rdfs:domain rdf:resource="http://reliant.teknowledge.com/DAML/SUMO.owl#CognitiveAgent" /><rdfs:range rdf:resource="http://reliant.teknowledge.com/DAML/SUMO.owl#EducationalOrganization" /><rdfs:subPropertyOf rdf:resource="http://reliant.teknowledge.com/DAML/SUMO.owl#member" /></owl:ObjectProperty><owl:ObjectProperty rdf:ID="telephoneNumber"><rdfs:comment>(telephoneNumber ?NUMBER ?AGENT) means 

that ?NUMBER is a telephone number at which ?AGENT can be regularly contacted.</rdfs:comment><rdfs:domain rdf:resource="http://reliant.teknowledge.com/DAML/SUMO.owl#SymbolicString" /><rdfs:range rdf:resource="http://reliant.teknowledge.com/DAML/SUMO.owl#Agent" /><rdfs:subPropertyOf rdf:resource="http://reliant.teknowledge.com/DAML/SUMO.owl#uniqueIdentifier" /><sumo:relatedInternalConcept rdf:resource="#address" /></owl:ObjectProperty><owl:ObjectProperty rdf:ID="tenant"><rdfs:comment>(tenant ?PERSON ?UNIT) means that ?PERSON is a tenant 

of the Residence ?UNIT, i.e. he or she is renting the unit.</rdfs:comment><rdf:type rdf:resource="http://reliant.teknowledge.com/DAML/SUMO.owl#BinaryPredicate" /><rdfs:domain rdf:resource="http://reliant.teknowledge.com/DAML/SUMO.owl#Human" /><rdfs:range rdf:resource="http://reliant.teknowledge.com/DAML/SUMO.owl#Residence" /></owl:ObjectProperty><owl:ObjectProperty rdf:ID="third"><rdfs:comment>(third ?THIRD ?WHOLE) means that ?THIRD is one 

third of ?WHOLE.</rdfs:comment><rdfs:subPropertyOf rdf:resource="http://reliant.teknowledge.com/DAML/SUMO.owl#part" /></owl:ObjectProperty><owl:ObjectProperty rdf:ID="titles"><rdfs:comment>A predicate used to indicate the title of a Text.  

Note that the second argument type restriction is a subclass, rather than 

an instance, of Text.  Thus, the title Murder_on_the_Orient_Express 

corresponds to a large class of Books, and not just to a single copy of 

the book.</rdfs:comment><rdfs:domain rdf:resource="http://reliant.teknowledge.com/DAML/SUMO.owl#SymbolicString" /><rdfs:subPropertyOf rdf:resource="http://reliant.teknowledge.com/DAML/SUMO.owl#names" /></owl:ObjectProperty><owl:ObjectProperty rdf:ID="totalGDP"><rdfs:comment>(totalGDP ?AREA ?AMOUNT) means that the value 

of all final goods and services produced within the GeopoliticalArea 

?AREA is ?AMOUNT, in U.S. dollars, calculated on a purchasing power parity 

basis.  This represents Gross Domestic Product (GDP).</rdfs:comment><rdf:type rdf:resource="http://reliant.teknowledge.com/DAML/SUMO.owl#BinaryPredicate" /><rdfs:domain rdf:resource="http://reliant.teknowledge.com/DAML/SUMO.owl#GeopoliticalArea" /><rdfs:range rdf:resource="http://reliant.teknowledge.com/DAML/SUMO.owl#CurrencyMeasure" /></owl:ObjectProperty><owl:ObjectProperty rdf:ID="uncle"><rdfs:comment>(uncle ?UNCLE ?PERSON) means that ?UNCLE is 

the brother of a parent of ?PERSON.</rdfs:comment><rdfs:domain rdf:resource="http://reliant.teknowledge.com/DAML/SUMO.owl#Man" /><rdfs:range rdf:resource="http://reliant.teknowledge.com/DAML/SUMO.owl#Human" /><rdfs:subPropertyOf rdf:resource="http://reliant.teknowledge.com/DAML/SUMO.owl#familyRelation" /></owl:ObjectProperty><owl:ObjectProperty rdf:ID="unitNumber"><rdfs:comment>(unitNumber ?UNIT ?ADDRESS) means that the 

StationaryArtifact ?UNIT is part of the address ?ADDRESS.</rdfs:comment><rdfs:domain rdf:resource="http://reliant.teknowledge.com/DAML/SUMO.owl#StationaryArtifact" /><rdfs:range rdf:resource="#Address" /><rdfs:subPropertyOf rdf:resource="#address" /></owl:ObjectProperty><owl:ObjectProperty rdf:ID="waterDepth"><rdfs:comment>(waterDepth ?AREA ?LENGTH) means that the 

depth of water at the Region ?AREA is ?LENGTH.</rdfs:comment><rdfs:domain rdf:resource="http://reliant.teknowledge.com/DAML/SUMO.owl#WaterArea" /><rdfs:range rdf:resource="http://reliant.teknowledge.com/DAML/SUMO.owl#LengthMeasure" /><rdfs:subPropertyOf rdf:resource="http://reliant.teknowledge.com/DAML/SUMO.owl#length" /></owl:ObjectProperty><owl:ObjectProperty rdf:ID="wavelength"><rdfs:comment>(wavelength ?RADIATION ?MEASURE) means that the 

instance of radiation, ?RADIATION, has an average wavelength of ?MEASURE.</rdfs:comment><rdf:type rdf:resource="http://reliant.teknowledge.com/DAML/SUMO.owl#SingleValuedRelation" /><rdfs:domain rdf:resource="http://reliant.teknowledge.com/DAML/SUMO.owl#Radiating" /><rdfs:range rdf:resource="http://reliant.teknowledge.com/DAML/SUMO.owl#LengthMeasure" /><rdfs:subPropertyOf rdf:resource="http://reliant.teknowledge.com/DAML/SUMO.owl#measure" /></owl:ObjectProperty><owl:DatatypeProperty rdf:ID="yearOfFounding"><rdfs:comment>(yearOfFounding ?ORG ?NUMBER) means that the Organization 

?ORG was founded in the year expressed in ?NUMBER.</rdfs:comment><rdf:type rdf:resource="http://reliant.teknowledge.com/DAML/SUMO.owl#BinaryPredicate" /><rdf:type rdf:resource="http://reliant.teknowledge.com/DAML/SUMO.owl#AsymmetricRelation" /><rdfs:domain rdf:resource="http://reliant.teknowledge.com/DAML/SUMO.owl#Organization" /><rdfs:range rdf:resource="http://reliant.teknowledge.com/DAML/SUMO.owl#Integer" /></owl:DatatypeProperty><rdf:Description rdf:ID="AbsoluteMonarchy"><sumo:subAttribute rdf:resource="#Monarchy" /><sumo:subAttribute rdf:resource="#AuthoritarianRegime" /></rdf:Description><rdf:Description rdf:ID="Africa"><rdf:type rdf:resource="http://reliant.teknowledge.com/DAML/SUMO.owl#Continent" /></rdf:Description><rdf:Description rdf:ID="Alabama"><rdf:type rdf:resource="#AmericanState" /><rdfs:comment>A state in the southeastern UnitedStates that 

borders on the Gulf of Mexico.</rdfs:comment></rdf:Description><rdf:Description rdf:ID="Alaska"><rdf:type rdf:resource="#AmericanState" /><rdfs:comment>The largest state in the UnitedStates.</rdfs:comment></rdf:Description><rdf:Description rdf:ID="AmerindianEthnicity"><rdf:type rdf:resource="#RacialEthnicGroup" /><rdfs:comment>A broad ethnic group encompassing any

of the North, Central, or South American tribal peoples.</rdfs:comment></rdf:Description><rdf:Description rdf:ID="Anarchy"><rdf:type rdf:resource="#FormOfGovernment" /></rdf:Description><rdf:Description rdf:ID="Anger"><sumo:subAttribute rdf:resource="#Unhappiness" /><rdfs:comment>The state of being wrathful, irate or indignant.</rdfs:comment></rdf:Description><rdf:Description rdf:ID="Antarctica"><rdf:type rdf:resource="http://reliant.teknowledge.com/DAML/SUMO.owl#Continent" /></rdf:Description><rdf:Description rdf:ID="Anthropology"><rdf:type rdf:resource="#SocialScience" /><rdfs:comment>The field of anthropology.</rdfs:comment></rdf:Description><rdf:Description rdf:ID="Antisemitism"><rdf:type rdf:resource="http://reliant.teknowledge.com/DAML/SUMO.owl#BeliefGroup" /><rdfs:comment>The BeliefGroup that is characterized by a 

dislike for Judaism.</rdfs:comment></rdf:Description><rdf:Description rdf:ID="Anxiety"><sumo:subAttribute rdf:resource="#Unhappiness" /><rdfs:comment>The state of being worried, troubled or uneasy.</rdfs:comment></rdf:Description><rdf:Description rdf:ID="ArabianSea"><rdf:type rdf:resource="#Sea" /></rdf:Description><rdf:Description rdf:ID="Architecture"><rdf:type rdf:resource="http://reliant.teknowledge.com/DAML/SUMO.owl#FieldOfStudy" /><rdfs:comment>The FieldOfStudy of designing Buildings, i.e. 

creating Blueprints for Buildings.</rdfs:comment></rdf:Description><rdf:Description rdf:ID="ArcticRegion"><rdf:type rdf:resource="http://reliant.teknowledge.com/DAML/SUMO.owl#GeographicArea" /><rdfs:comment>The ArcticRegion is the region of 

PlanetEarth that lies north of the Arctic Circle (approximately 

66 and one half degrees North latitude) or beyond the northern 

treeline: 'The Arctic'. See also ArcticArea.</rdfs:comment></rdf:Description><rdf:Description rdf:ID="Arkansas"><rdf:type rdf:resource="#AmericanState" /><rdfs:comment>A state in the southeastern UnitedStates that was 

part of the Confederacy.</rdfs:comment></rdf:Description><rdf:Description rdf:ID="Asia"><rdf:type rdf:resource="http://reliant.teknowledge.com/DAML/SUMO.owl#Continent" /></rdf:Description><rdf:Description rdf:ID="AtlantaGeorgia"><rdf:type rdf:resource="#AmericanCity" /><sumo:part rdf:resource="#Georgia" /><rdfs:comment>The largest City in Georgia.</rdfs:comment></rdf:Description><rdf:Description rdf:ID="AtlanticOcean"><rdf:type rdf:resource="#Ocean" /><rdfs:comment>AtlanticOcean represents the Atlantic 

Ocean.</rdfs:comment></rdf:Description><rdf:Description rdf:ID="Australia"><rdf:type rdf:resource="http://reliant.teknowledge.com/DAML/SUMO.owl#Nation" /><sumo:part rdf:resource="#Oceania" /><rdfs:comment>An industrialized Nation that occupies the entire 

continent of Oceania.</rdfs:comment></rdf:Description><rdf:Description rdf:ID="AuthoritarianRegime"><rdf:type rdf:resource="#FormOfGovernment" /><rdfs:comment>AuthoritarianRegime is the 

attribute of a government that rules autocratically, not allowing 

opposition.</rdfs:comment><sumo:contraryAttribute rdf:resource="#MultipartyDemocracy" /></rdf:Description><rdf:Description rdf:ID="AuthoritarianSocialist"><rdf:type rdf:resource="#FormOfGovernment" /><sumo:subAttribute rdf:resource="#AuthoritarianRegime" /></rdf:Description><rdf:Description rdf:ID="BalticSea"><rdf:type rdf:resource="#Sea" /></rdf:Description><rdf:Description rdf:ID="BaltimoreMaryland"><rdf:type rdf:resource="#AmericanCity" /><sumo:part rdf:resource="#Maryland" /><rdfs:comment>The largest City in Maryland.</rdfs:comment></rdf:Description><rdf:Description rdf:ID="BaseballStrike"><rdf:type rdf:resource="#BaseballManeuver" /><sumo:disjoint rdf:resource="#BaseballHit" /><rdfs:comment>A baseball pitch that is in the strike zone 

and that is not hit by the batter.</rdfs:comment></rdf:Description><rdf:Description rdf:ID="BeforeCommonEra"><rdf:type rdf:resource="http://reliant.teknowledge.com/DAML/SUMO.owl#TimeInterval" /><rdfs:comment>The TimeInterval that runs from 

NegativeInfinity to the time of the birth of Christ.</rdfs:comment></rdf:Description><rdf:Description rdf:ID="BeringSea"><rdf:type rdf:resource="#Sea" /></rdf:Description><rdf:Description rdf:ID="BerlinGermany"><rdf:type rdf:resource="#EuropeanCity" /><capitalCity rdf:resource="#Germany" /><rdfs:comment>The capital of Germany and the largest 

City of the country.</rdfs:comment></rdf:Description><rdf:Description rdf:ID="BernSwitzerland"><rdf:type rdf:resource="#EuropeanCity" /><capitalCity rdf:resource="#Switzerland" /><rdfs:comment>The capital of Switzerland.</rdfs:comment></rdf:Description><rdf:Description rdf:ID="Biology"><rdf:type rdf:resource="#Science" /><rdfs:comment>The study of the classification, development, and 

functioning of Organisms.</rdfs:comment></rdf:Description><rdf:Description rdf:ID="BlackEthnicity"><rdf:type rdf:resource="#RacialEthnicGroup" /><rdfs:comment>A broad racial division encompassing

various African, African-American, and Caribbean peoples.</rdfs:comment></rdf:Description><rdf:Description rdf:ID="BlackSea"><rdf:type rdf:resource="#Sea" /></rdf:Description><rdf:Description rdf:ID="Blind"><rdf:type rdf:resource="http://reliant.teknowledge.com/DAML/SUMO.owl#BiologicalAttribute" /><rdfs:comment>The Attribute that applies to Animals and Humans 

that are unable to see.</rdfs:comment></rdf:Description><rdf:Description rdf:ID="BostonMassachusetts"><rdf:type rdf:resource="#AmericanCity" /><sumo:part rdf:resource="#Massachusetts" /><rdfs:comment>The largest City in Massachusetts.</rdfs:comment></rdf:Description><rdf:Description rdf:ID="Brown"><rdf:type rdf:resource="#SecondaryColor" /><rdfs:comment>A SecondaryColor that results from mixing Black and 

White and resembles the color of wood or of soil.</rdfs:comment></rdf:Description><rdf:Description rdf:ID="California"><rdf:type rdf:resource="#AmericanState" /><rdfs:comment>The AmericanState with the highest population.</rdfs:comment></rdf:Description><rdf:Description rdf:ID="Canada"><rdf:type rdf:resource="http://reliant.teknowledge.com/DAML/SUMO.owl#Nation" /><sumo:meetsSpatially rdf:resource="#UnitedStates" /><rdfs:comment>A Nation in North America.</rdfs:comment></rdf:Description><rdf:Description rdf:ID="Cancer"><rdf:type rdf:resource="http://reliant.teknowledge.com/DAML/SUMO.owl#DiseaseOrSyndrome" /><rdfs:comment>A DiseaseOrSyndrome characterized by pathologic and 

uncontrolled cell division that results in a Tumor.</rdfs:comment></rdf:Description><rdf:Description rdf:ID="CapitalistEconomy"><rdf:type rdf:resource="#EconomicSystemAttribute" /><rdfs:comment>CapitalistEconomy is the 

Attribute used to characterize a country whose economy is based 

on private ownership of the means of production and distribution, 

and on private accumulation of capital.</rdfs:comment></rdf:Description><rdf:Description rdf:ID="CaribbeanSea"><rdf:type rdf:resource="#Sea" /></rdf:Description><rdf:Description rdf:ID="CentralTimeZone"><rdf:type rdf:resource="http://reliant.teknowledge.com/DAML/SUMO.owl#TimeZone" /><rdfs:comment>A TimeZone that covers much of the 

midwestern United States.</rdfs:comment></rdf:Description><rdf:Description rdf:ID="CentrallyPlannedEconomy"><rdf:type rdf:resource="#EconomicSystemAttribute" /><sumo:subAttribute rdf:resource="#GovernmentRegulatedEconomy" /><rdfs:comment>CentrallyPlannedEconomy 

is a term used mainly to describe communist or formerly communist 

states, many of which are now evolving away from command economies 

towards market-oriented systems.  Also known as a 'command economy'.</rdfs:comment></rdf:Description><rdf:Description rdf:ID="Chairman"><rdf:type rdf:resource="http://reliant.teknowledge.com/DAML/SUMO.owl#Position" /></rdf:Description><rdf:Description rdf:ID="ChemicalEquilibrium"><rdf:type rdf:resource="http://reliant.teknowledge.com/DAML/SUMO.owl#InternalAttribute" /><rdfs:comment>The Attribute of being in a chemically 

stable state, i.e. the relative proportions of resources and results will 

not longer change.</rdfs:comment></rdf:Description><rdf:Description rdf:ID="Chemistry"><rdf:type rdf:resource="#Science" /><rdfs:comment>The study of the compositions, properties, and 

reactions of Substances.</rdfs:comment></rdf:Description><rdf:Description rdf:ID="ChicagoIllinois"><rdf:type rdf:resource="#AmericanCity" /><sumo:part rdf:resource="#Illinois" /><rdfs:comment>Often referred to as the second city, 

ChicagoIllinois is the largest city in the midwestern United States.</rdfs:comment></rdf:Description><rdf:Description rdf:ID="Chiefdom"><rdf:type rdf:resource="#FormOfGovernment" /><sumo:subAttribute rdf:resource="#Monarchy" /></rdf:Description><rdf:Description rdf:ID="China"><rdf:type rdf:resource="http://reliant.teknowledge.com/DAML/SUMO.owl#Nation" /><rdfs:comment>An Asian Nation, which is the most populous 

Nation in the world.</rdfs:comment></rdf:Description><rdf:Description rdf:ID="Christianity"><rdf:type rdf:resource="http://reliant.teknowledge.com/DAML/SUMO.owl#BeliefGroup" /><rdfs:comment>The religion derived from Jesus Christ, based on 

the Bible as sacred scripture, and professed by Eastern, Catholic, and 

Protestant bodies, among other subdivisions.</rdfs:comment></rdf:Description><rdf:Description rdf:ID="ChurchOfEngland"><rdf:type rdf:resource="http://reliant.teknowledge.com/DAML/SUMO.owl#ReligiousOrganization" /><rdfs:comment>The ChurchOfEngland is the

ReligiousOrganization that promulgates Anglicanism.</rdfs:comment></rdf:Description><rdf:Description rdf:ID="CivilLaw"><rdf:type rdf:resource="#LegalSystemAttribute" /><rdfs:comment>CivilLaw is the attribute of legal systems 

based ultimately on the code of civil law developed in Ancient Rome.  

Civil law systems are characterized by their expression of laws in written 

code and statute and by their effort to use general principles to define 

and rationalize the laws.</rdfs:comment></rdf:Description><rdf:Description rdf:ID="ClevelandOhio"><rdf:type rdf:resource="#AmericanCity" /><sumo:part rdf:resource="#Ohio" /><rdfs:comment>Bordering Lake Erie, ClevelandOhio is 

the largest City in Ohio.</rdfs:comment></rdf:Description><rdf:Description rdf:ID="Colorado"><rdf:type rdf:resource="#AmericanState" /><rdfs:comment>A large western state in the UnitedStates.</rdfs:comment></rdf:Description><rdf:Description rdf:ID="ColumbusOhio"><rdf:type rdf:resource="#AmericanCity" /><capitalCity rdf:resource="#Ohio" /><rdfs:comment>The capital of Ohio, located in the middle 

of the state.</rdfs:comment></rdf:Description><rdf:Description rdf:ID="CommonEra"><rdf:type rdf:resource="http://reliant.teknowledge.com/DAML/SUMO.owl#TimeInterval" /><rdfs:comment>The TimeInterval that runs from the supposed 

time of the death of Christ to PositiveInfinity.</rdfs:comment></rdf:Description><rdf:Description rdf:ID="Commonwealth"><rdf:type rdf:resource="#FormOfGovernment" /></rdf:Description><rdf:Description rdf:ID="CommunalLandOwnershipEconomy"><rdf:type rdf:resource="#EconomicSystemAttribute" /><sumo:subAttribute rdf:resource="#SocialistEconomy" /></rdf:Description><rdf:Description rdf:ID="CommunistState"><rdf:type rdf:resource="#FormOfGovernment" /><sumo:subAttribute rdf:resource="#AuthoritarianRegime" /></rdf:Description><rdf:Description rdf:ID="CompactOfFreeAssociationWithNewZealand"><rdf:type rdf:resource="#FormOfGovernment" /></rdf:Description><rdf:Description rdf:ID="CompactOfFreeAssociationWithUnitedStates"><rdf:type rdf:resource="#FormOfGovernment" /></rdf:Description><rdf:Description rdf:ID="ConfederateStatesOfAmerica"><rdf:type rdf:resource="http://reliant.teknowledge.com/DAML/SUMO.owl#GeopoliticalArea" /><rdfs:comment>The eleven states of the UnitedStates 

that tried to secede from the UnitedStates.</rdfs:comment></rdf:Description><rdf:Description rdf:ID="Connecticut"><rdf:type rdf:resource="#AmericanState" /><sumo:part rdf:resource="#NewEngland" /><rdfs:comment>A state in NewEngland, one of the original thirteen 

colonies.</rdfs:comment></rdf:Description><rdf:Description rdf:ID="ConstitutionalDemocracy"><sumo:subAttribute rdf:resource="#ConstitutionalGovernment" /></rdf:Description><rdf:Description rdf:ID="ConstitutionalDemocraticRepublic"><rdf:type rdf:resource="#FormOfGovernment" /><sumo:subAttribute rdf:resource="#Republic" /><sumo:subAttribute rdf:resource="#Democracy" /></rdf:Description><rdf:Description rdf:ID="ConstitutionalGovernment"><rdf:type rdf:resource="#FormOfGovernment" /><rdfs:comment>ConstitutionalGovernment is 

the attribute of a government whose authority and rule are guided by  

principles expressed in a written Constitution.</rdfs:comment></rdf:Description><rdf:Description rdf:ID="ConstitutionalMonarchy"><rdf:type rdf:resource="#FormOfGovernment" /><sumo:subAttribute rdf:resource="#Monarchy" /><sumo:subAttribute rdf:resource="#ConstitutionalGovernment" /></rdf:Description><rdf:Description rdf:ID="ConstitutionalParliamentaryDemocracy"><rdf:type rdf:resource="#FormOfGovernment" /><sumo:subAttribute rdf:resource="#ParliamentaryGovernment" /><sumo:subAttribute rdf:resource="#Democracy" /><sumo:subAttribute rdf:resource="#ConstitutionalDemocracy" /></rdf:Description><rdf:Description rdf:ID="ConstitutionalRepublic"><rdf:type rdf:resource="#FormOfGovernment" /><sumo:subAttribute rdf:resource="#Republic" /><sumo:subAttribute rdf:resource="#ConstitutionalGovernment" /></rdf:Description><rdf:Description rdf:ID="ContainerEmpty"><rdf:type rdf:resource="http://reliant.teknowledge.com/DAML/SUMO.owl#RelationalAttribute" /><rdfs:comment>ContainerEmpty is the Attribute of a 

Container that is empty.</rdfs:comment></rdf:Description><rdf:Description rdf:ID="ContainerFull"><rdf:type rdf:resource="http://reliant.teknowledge.com/DAML/SUMO.owl#RelationalAttribute" /><rdfs:comment>ContainerFull is the Attribute of a 

Container that is full to capacity.</rdfs:comment></rdf:Description><rdf:Description rdf:ID="CopenhagenDenmark"><rdf:type rdf:resource="#EuropeanCity" /><capitalCity rdf:resource="#Denmark" /><rdfs:comment>The capital of Denmark and the largest 

City of the country.</rdfs:comment></rdf:Description><rdf:Description rdf:ID="Coprincipality"><rdf:type rdf:resource="#FormOfGovernment" /></rdf:Description><rdf:Description rdf:ID="Cuba"><rdf:type rdf:resource="http://reliant.teknowledge.com/DAML/SUMO.owl#Nation" /><rdf:type rdf:resource="http://reliant.teknowledge.com/DAML/SUMO.owl#Island" /><rdfs:comment>An Island Nation in the Carribbean.</rdfs:comment></rdf:Description><rdf:Description rdf:ID="Czechoslovakia"><rdf:type rdf:resource="#EuropeanNation" /><rdfs:comment>The former eastern bloc nation.  It is currently 

divided into two independent Nations, the Czech Republic and Slovakia.</rdfs:comment></rdf:Description><rdf:Description rdf:ID="DallasTexas"><rdf:type rdf:resource="#AmericanCity" /><sumo:part rdf:resource="#Texas" /><rdfs:comment>A large City in northeastern Texas.</rdfs:comment></rdf:Description><rdf:Description rdf:ID="Deaf"><rdf:type rdf:resource="http://reliant.teknowledge.com/DAML/SUMO.owl#BiologicalAttribute" /><rdfs:comment>The Attribute that applies to Animals and Humans 

that are unable to hear.</rdfs:comment></rdf:Description><rdf:Description rdf:ID="Democracy"><rdf:type rdf:resource="#FormOfGovernment" /><rdfs:comment>Democracy is the attribute of a government 

whose authority and rule are based in the will of the people governed.  

The will of the people is usually expressed through Elections, direct or 

indirect.</rdfs:comment></rdf:Description><rdf:Description rdf:ID="DemocraticParty"><rdf:type rdf:resource="#PoliticalParty" /><rdfs:comment>One of the two major political parties in 

the UnitedStates.  The DemocraticParty represents liberal values.</rdfs:comment></rdf:Description><rdf:Description rdf:ID="DemocraticSocialism"><rdf:type rdf:resource="#EconomicSystemAttribute" /><sumo:subAttribute rdf:resource="#SocialistEconomy" /><rdfs:comment>DemocraticSocialism is an  

Attribute that describes a country in which socialism is promoted 

by a political party or parties within a democratic government. 

Under DemocraticSocialism, the government participates in central 

planning of the economy and may also manage nationalized industries.</rdfs:comment></rdf:Description><rdf:Description rdf:ID="Denmark"><rdf:type rdf:resource="#EuropeanNation" /><rdfs:comment>A Nation in scandinavian Europe.</rdfs:comment></rdf:Description><rdf:Description rdf:ID="DenverColorado"><rdf:type rdf:resource="#AmericanCity" /><capitalCity rdf:resource="#Colorado" /><rdfs:comment>The capital and largest City in Colorado.</rdfs:comment></rdf:Description><rdf:Description rdf:ID="DetroitMichigan"><rdf:type rdf:resource="#AmericanCity" /><sumo:part rdf:resource="#Michigan" /><rdfs:comment>The largest City in Michigan.</rdfs:comment></rdf:Description><rdf:Description rdf:ID="DeviceClosed"><rdf:type rdf:resource="#DeviceStateAttribute" /><rdf:type rdf:resource="http://reliant.teknowledge.com/DAML/SUMO.owl#RelationalAttribute" /></rdf:Description><rdf:Description rdf:ID="DeviceOff"><rdf:type rdf:resource="#DeviceStateAttribute" /><rdf:type rdf:resource="http://reliant.teknowledge.com/DAML/SUMO.owl#InternalAttribute" /></rdf:Description><rdf:Description rdf:ID="DeviceOn"><rdf:type rdf:resource="#DeviceStateAttribute" /><rdf:type rdf:resource="http://reliant.teknowledge.com/DAML/SUMO.owl#InternalAttribute" /></rdf:Description><rdf:Description rdf:ID="DeviceOpen"><rdf:type rdf:resource="#DeviceStateAttribute" /><rdf:type rdf:resource="http://reliant.teknowledge.com/DAML/SUMO.owl#RelationalAttribute" /></rdf:Description><rdf:Description rdf:ID="Diarrhea"><rdf:type rdf:resource="http://reliant.teknowledge.com/DAML/SUMO.owl#DiseaseOrSyndrome" /><rdfs:comment>A DiseaseOrSyndrome of frequent, watery bowel 

movements.</rdfs:comment></rdf:Description><rdf:Description rdf:ID="Dictatorship"><rdf:type rdf:resource="#FormOfGovernment" /><sumo:subAttribute rdf:resource="#AuthoritarianRegime" /></rdf:Description><rdf:Description rdf:ID="Downstairs"><rdf:type rdf:resource="http://reliant.teknowledge.com/DAML/SUMO.owl#PositionalAttribute" /><rdfs:comment>A PositionalAttribute to indicate that one thing is 

one or more floors below a second thing in the same building.</rdfs:comment></rdf:Description><rdf:Description rdf:ID="Drugged"><rdf:type rdf:resource="http://reliant.teknowledge.com/DAML/SUMO.owl#ConsciousnessAttribute" /><sumo:contraryAttribute rdf:resource="#Sober" /><rdfs:comment>The ConsciousnessAttribute of someone whose motor and/or 

cognitive faculties are significantly impaired by a BiologicallyActiveSubstance.</rdfs:comment></rdf:Description><rdf:Description rdf:ID="Drunk"><sumo:subAttribute rdf:resource="#Drugged" /><rdfs:comment>The ConsciousnessAttribute of someone whose motor and 

cognitive faculties are significantly impaired by Alcohol.</rdfs:comment></rdf:Description><rdf:Description rdf:ID="EarthsAtmosphere"><rdf:type rdf:resource="#Atmosphere" /><rdfs:comment>EarthsAtmosphere is the layer of gases, 

a mixture of mainly oxygen and nitrogen, surrounding PlanetEarth.  See 

also Air.</rdfs:comment></rdf:Description><rdf:Description rdf:ID="EarthsMoon"><rdf:type rdf:resource="#Moon" /><orbits rdf:resource="#PlanetEarth" /><rdfs:comment>EarthsMoon is the Moon of PlanetEarth.</rdfs:comment></rdf:Description><rdf:Description rdf:ID="EasternHemisphere"><rdf:type rdf:resource="#Hemisphere" /><rdfs:comment>The half of the Earth that includes Europe, 

Asia, Africa, and Australia.</rdfs:comment></rdf:Description><rdf:Description rdf:ID="EasternTimeZone"><rdf:type rdf:resource="http://reliant.teknowledge.com/DAML/SUMO.owl#TimeZone" /><rdfs:comment>A TimeZone that covers much of the 

eastern United States.</rdfs:comment></rdf:Description><rdf:Description rdf:ID="EcclesiasticalGovernment"><rdf:type rdf:resource="#FormOfGovernment" /><sumo:subAttribute rdf:resource="#TheocraticGovernment" /></rdf:Description><rdf:Description rdf:ID="Economics"><rdf:type rdf:resource="#SocialScience" /><rdfs:comment>The field of economics.</rdfs:comment></rdf:Description><rdf:Description rdf:ID="EmergingDemocracy"><rdf:type rdf:resource="#FormOfGovernment" /><sumo:subAttribute rdf:resource="#Democracy" /><sumo:subAttribute rdf:resource="#TransitionalGovernment" /></rdf:Description><rdf:Description rdf:ID="Emphysema"><rdf:type rdf:resource="http://reliant.teknowledge.com/DAML/SUMO.owl#DiseaseOrSyndrome" /><rdfs:comment>A DiseaseOrSyndrome that affects the Lungs and 

which results in a decrease of breathing ability.</rdfs:comment></rdf:Description><rdf:Description rdf:ID="Engineering"><rdf:type rdf:resource="#Science" /><rdfs:comment>The application of instances of Science to the solution 

of practical problems, i.e. the creation of various forms of technology.</rdfs:comment></rdf:Description><rdf:Description rdf:ID="EnglishCommonLaw"><rdf:type rdf:resource="#LegalSystemAttribute" /><rdfs:comment>EnglishCommonLaw is the attribute of 

legal systems based on the common law developed in England and influential  

in its English-speaking colonies.  Common law is characterized by laws and 

rulings based on precedent and custom, rather than on written statute.</rdfs:comment></rdf:Description><rdf:Description rdf:ID="EnglishLanguage"><rdf:type rdf:resource="http://reliant.teknowledge.com/DAML/SUMO.owl#SpokenHumanLanguage" /><rdf:type rdf:resource="http://reliant.teknowledge.com/DAML/SUMO.owl#NaturalLanguage" /><rdfs:comment>A Germanic language that incorporates many roots 

from the Romance languages.  It is the official language of the UnitedStates, 

the UnitedKingdomOfGreatBritainAndNorthernIreland, and many other countries.</rdfs:comment></rdf:Description><rdf:Description rdf:ID="Europe"><rdf:type rdf:resource="http://reliant.teknowledge.com/DAML/SUMO.owl#Continent" /><rdfs:comment>The second smallest Continent.</rdfs:comment></rdf:Description><rdf:Description rdf:ID="Excitement"><sumo:subAttribute rdf:resource="#Happiness" /><rdfs:comment>The state of being happy about a state of 

affairs that might occur in the future.</rdfs:comment></rdf:Description><rdf:Description rdf:ID="Factionalism"><rdf:type rdf:resource="#FormOfGovernment" /><sumo:subAttribute rdf:resource="#TransitionalGovernment" /></rdf:Description><rdf:Description rdf:ID="FargoNorthDakota"><rdf:type rdf:resource="#AmericanCity" /><sumo:part rdf:resource="#NorthDakota" /><rdfs:comment>The largest City in NorthDakota.</rdfs:comment></rdf:Description><rdf:Description rdf:ID="FederalDemocraticRepublic"><rdf:type rdf:resource="#FormOfGovernment" /><sumo:subAttribute rdf:resource="#FederalGovernment" /><sumo:subAttribute rdf:resource="#Republic" /><sumo:subAttribute rdf:resource="#Democracy" /></rdf:Description><rdf:Description rdf:ID="FederalGovernment"><rdf:type rdf:resource="#FormOfGovernment" /><rdfs:comment>FederalGovernment is the attribute of 

a government that is formed by agreement between a collection of political 

units that agree to give up some of their power to the central government, 

while reserving some powers to themselves.  The government of the 

UnitedStates is a federal government, in which power is shared between 

the states and the central goverment, as set out in the U.S. 

Constitution.</rdfs:comment><sumo:contraryAttribute rdf:resource="#UnitaryRule" /><sumo:contraryAttribute rdf:resource="#AuthoritarianRegime" /></rdf:Description><rdf:Description rdf:ID="FederalParliamentaryDemocracy"><rdf:type rdf:resource="#FormOfGovernment" /><sumo:subAttribute rdf:resource="#ParliamentaryGovernment" /><sumo:subAttribute rdf:resource="#FederalGovernment" /><sumo:subAttribute rdf:resource="#Democracy" /></rdf:Description><rdf:Description rdf:ID="FederalRepublic"><rdf:type rdf:resource="#FormOfGovernment" /><sumo:subAttribute rdf:resource="#FederalGovernment" /><sumo:subAttribute rdf:resource="#Republic" /></rdf:Description><rdf:Description rdf:ID="Federation"><rdf:type rdf:resource="#FormOfGovernment" /><sumo:subAttribute rdf:resource="#FederalGovernment" /></rdf:Description><rdf:Description rdf:ID="Fever"><rdf:type rdf:resource="http://reliant.teknowledge.com/DAML/SUMO.owl#DiseaseOrSyndrome" /><rdfs:comment>Having a body temperature which is (significantly) greater 

than 98.6 degrees Fahrenheit.  This syndrome is often associated with dehydration 

and chills.</rdfs:comment></rdf:Description><rdf:Description rdf:ID="FieldOfLaw"><rdf:type rdf:resource="http://reliant.teknowledge.com/DAML/SUMO.owl#FieldOfStudy" /><rdfs:comment>The study of legal principles and the framework of national 

and/or international laws.</rdfs:comment></rdf:Description><rdf:Description rdf:ID="Fist"><rdf:type rdf:resource="http://reliant.teknowledge.com/DAML/SUMO.owl#BodyPosition" /><rdfs:comment>The BodyPosition of having the fingers drawn into 

the palm so that the hand can be used for striking something.</rdfs:comment></rdf:Description><rdf:Description rdf:ID="Florida"><rdf:type rdf:resource="#AmericanState" /><rdfs:comment>A state in the southeastern UnitedStates between 

the Gulf of Mexico and the Atlantic Ocean.</rdfs:comment></rdf:Description><rdf:Description rdf:ID="Foul"><rdf:type rdf:resource="#SportsAttribute" /><rdfs:comment>A SportsAttribute that indicates that the GamePiece of 

a Sport is no longer in play because it has gone beyond the limits of the 

sports field.</rdfs:comment></rdf:Description><rdf:Description rdf:ID="Fragile"><rdf:type rdf:resource="#BreakabilityAttribute" /><rdfs:comment>An Attribute which indicates that the 

associated Object is very breakable.</rdfs:comment></rdf:Description><rdf:Description rdf:ID="France"><rdf:type rdf:resource="#EuropeanNation" /><rdfs:comment>A large, industrialized European Nation.</rdfs:comment></rdf:Description><rdf:Description rdf:ID="FrenchLanguage"><rdf:type rdf:resource="http://reliant.teknowledge.com/DAML/SUMO.owl#SpokenHumanLanguage" /><rdf:type rdf:resource="http://reliant.teknowledge.com/DAML/SUMO.owl#NaturalLanguage" /><rdfs:comment>A Romance language that is the official language 

of France and Belgium, and is widely spoken in Africa.</rdfs:comment></rdf:Description><rdf:Description rdf:ID="Functioning"><rdf:type rdf:resource="#DeviceAttribute" /><sumo:contraryAttribute rdf:resource="#Malfunctioning" /><rdfs:comment>Indicates that a Device is performing its 

intended function.</rdfs:comment></rdf:Description><rdf:Description rdf:ID="Georgia"><rdf:type rdf:resource="#AmericanState" /><rdfs:comment>A state in the southeastern UnitedStates.</rdfs:comment></rdf:Description><rdf:Description rdf:ID="GermanLanguage"><rdf:type rdf:resource="http://reliant.teknowledge.com/DAML/SUMO.owl#SpokenHumanLanguage" /><rdf:type rdf:resource="http://reliant.teknowledge.com/DAML/SUMO.owl#NaturalLanguage" /><rdfs:comment>A Germanic language that is spoken primarily in 

Germany and Austria.</rdfs:comment></rdf:Description><rdf:Description rdf:ID="Germany"><rdf:type rdf:resource="#EuropeanNation" /><rdfs:comment>A large European Nation.</rdfs:comment></rdf:Description><rdf:Description rdf:ID="Goiter"><rdf:type rdf:resource="http://reliant.teknowledge.com/DAML/SUMO.owl#DiseaseOrSyndrome" /><rdfs:comment>A DiseaseOrSyndrome which is due to an Iodine deficiency 

and which results in an enlarged ThyroidGland.</rdfs:comment></rdf:Description><rdf:Description rdf:ID="GovernmentDeputy"><rdf:type rdf:resource="http://reliant.teknowledge.com/DAML/SUMO.owl#Position" /></rdf:Description><rdf:Description rdf:ID="GovernmentRegulatedEconomy"><rdf:type rdf:resource="#EconomicSystemAttribute" /><rdfs:comment>GovernmentRegulatedEconomy 

is an Attribute that describes the economy of a country in which the 

government determines prices, production, wages, allocation of resources, 

or other economic factors.  An economy that is wholly government planned 

is a CentrallyPlannedEconomy.</rdfs:comment></rdf:Description><rdf:Description rdf:ID="GovernmentSubsidizedEconomy"><rdf:type rdf:resource="#EconomicSystemAttribute" /><rdfs:comment>GovernmentSubsidizedEconomy 

is an Attribute describing an economy in which the government provides 

subsidies to various industries, workers, or other groups as part of its 

economic policy.</rdfs:comment></rdf:Description><rdf:Description rdf:ID="Governor"><rdf:type rdf:resource="http://reliant.teknowledge.com/DAML/SUMO.owl#Position" /><rdfs:comment>The head of the Government of an AmericanState.</rdfs:comment></rdf:Description><rdf:Description rdf:ID="Greece"><rdf:type rdf:resource="#EuropeanNation" /><rdfs:comment>A small Balkan Nation that is known primarily for the 

literature, philosophy, and art produced there during the ancient period.</rdfs:comment></rdf:Description><rdf:Description rdf:ID="GreekLanguage"><rdf:type rdf:resource="http://reliant.teknowledge.com/DAML/SUMO.owl#SpokenHumanLanguage" /><rdf:type rdf:resource="http://reliant.teknowledge.com/DAML/SUMO.owl#NaturalLanguage" /><rdfs:comment>An Indo-European language that is spoken in Greece.</rdfs:comment></rdf:Description><rdf:Description rdf:ID="Green"><rdf:type rdf:resource="#SecondaryColor" /><rdfs:comment>A SecondaryColor that results from mixing Blue and 

Yellow and resembles the color of fresh grass.</rdfs:comment></rdf:Description><rdf:Description rdf:ID="Guam"><rdf:type rdf:resource="http://reliant.teknowledge.com/DAML/SUMO.owl#Island" /><rdfs:comment>An Island in the PacificOcean that is a 

protectorate of the UnitedStates.</rdfs:comment></rdf:Description><rdf:Description rdf:ID="Handstand"><rdf:type rdf:resource="http://reliant.teknowledge.com/DAML/SUMO.owl#BodyPosition" /><rdfs:comment>The BodyPosition where one rests on one's hands 

and extends one's feet in the air.</rdfs:comment></rdf:Description><rdf:Description rdf:ID="Happiness"><rdf:type rdf:resource="http://reliant.teknowledge.com/DAML/SUMO.owl#EmotionalState" /><rdfs:comment>The state of being happy, experiencing pleasure, 

joy or contentment.  Note that this Attribute covers both active enjoyment, 

as well as the emotional state of simply being free from anxiety or fear.</rdfs:comment></rdf:Description><rdf:Description rdf:ID="Hawaii"><rdf:type rdf:resource="#AmericanState" /><sumo:meetsSpatially rdf:resource="#PacificOcean" /><rdfs:comment>An AmericanState that consists of several Islands in 

the central PacificOcean.</rdfs:comment></rdf:Description><rdf:Description rdf:ID="Headache"><sumo:subAttribute rdf:resource="#Pain" /><rdfs:comment>Pain that that is restricted to the Head.</rdfs:comment></rdf:Description><rdf:Description rdf:ID="HereditaryMonarchy"><rdf:type rdf:resource="#FormOfGovernment" /><sumo:subAttribute rdf:resource="#Monarchy" /></rdf:Description><rdf:Description rdf:ID="Hinduism"><rdf:type rdf:resource="http://reliant.teknowledge.com/DAML/SUMO.owl#BeliefGroup" /><rdfs:comment>Hinduism represents the major religious 

BeliefGroup of India.</rdfs:comment></rdf:Description><rdf:Description rdf:ID="History"><rdf:type rdf:resource="http://reliant.teknowledge.com/DAML/SUMO.owl#FieldOfStudy" /><rdfs:comment>The recording and interpretation of past events involving 

Humans, including political events and cultural practices.</rdfs:comment></rdf:Description><rdf:Description rdf:ID="HonoluluHawaii"><rdf:type rdf:resource="#AmericanCity" /><capitalCity rdf:resource="#Hawaii" /><rdfs:comment>The capital and largest City in Hawaii.</rdfs:comment></rdf:Description><rdf:Description rdf:ID="Housewife"><sumo:subAttribute rdf:resource="http://reliant.teknowledge.com/DAML/SUMO.owl#Unemployed" /><rdfs:comment>A role occupied by a wife who manages the home 

while her husband earns income for the family.</rdfs:comment></rdf:Description><rdf:Description rdf:ID="HoustonTexas"><rdf:type rdf:resource="#AmericanCity" /><sumo:part rdf:resource="#Texas" /><rdfs:comment>Located in southeastern Texas, the largest 

City in the state.</rdfs:comment></rdf:Description><rdf:Description rdf:ID="HudsonRiver"><rdf:type rdf:resource="#River" /><sumo:part rdf:resource="#NewYorkState" /><rdfs:comment>A large River in NewYorkState.</rdfs:comment></rdf:Description><rdf:Description rdf:ID="Hungry"><rdf:type rdf:resource="http://reliant.teknowledge.com/DAML/SUMO.owl#BiologicalAttribute" /><rdfs:comment>The Attribute that applies to Animals and Humans 

when they want Food.</rdfs:comment></rdf:Description><rdf:Description rdf:ID="Illegal"><sumo:subAttribute rdf:resource="http://reliant.teknowledge.com/DAML/SUMO.owl#Prohibition" /><sumo:contraryAttribute rdf:resource="#Legal" /><rdfs:comment>A proposition is Illegal just in case it is inconsistent 

with any proposition that is a Law.</rdfs:comment></rdf:Description><rdf:Description rdf:ID="Illinois"><rdf:type rdf:resource="#AmericanState" /><rdfs:comment>A populous and industrial state in the midwestern 

UnitedStates.</rdfs:comment></rdf:Description><rdf:Description rdf:ID="India"><rdf:type rdf:resource="http://reliant.teknowledge.com/DAML/SUMO.owl#Nation" /><rdfs:comment>A Nation in southern Asia which is the second 

most populous Nation in the world.</rdfs:comment></rdf:Description><rdf:Description rdf:ID="InteriorDesign"><rdf:type rdf:resource="http://reliant.teknowledge.com/DAML/SUMO.owl#FieldOfStudy" /><rdfs:comment>The FieldOfStudy of designing the interiors of 

Buildings.</rdfs:comment></rdf:Description><rdf:Description rdf:ID="InternationalLaw"><sumo:subAttribute rdf:resource="http://reliant.teknowledge.com/DAML/SUMO.owl#Law" /><rdfs:comment>An Attribute that applies to Propositions 

that express Laws concerning the relations between Nations.</rdfs:comment></rdf:Description><rdf:Description rdf:ID="Ireland"><rdf:type rdf:resource="#EuropeanNation" /><rdfs:comment>An independent Nation that borders on the Irish Sea.</rdfs:comment></rdf:Description><rdf:Description rdf:ID="Islam"><rdf:type rdf:resource="http://reliant.teknowledge.com/DAML/SUMO.owl#BeliefGroup" /><rdfs:comment>Islam represents the BeliefGroup of Islamic 

believers.</rdfs:comment></rdf:Description><rdf:Description rdf:ID="IslamicGovernment"><rdf:type rdf:resource="#FormOfGovernment" /><sumo:subAttribute rdf:resource="#TheocraticGovernment" /></rdf:Description><rdf:Description rdf:ID="Israel"><rdf:type rdf:resource="http://reliant.teknowledge.com/DAML/SUMO.owl#Nation" /><rdfs:comment>A Nation in the Middle East.</rdfs:comment></rdf:Description><rdf:Description rdf:ID="Italy"><rdf:type rdf:resource="#EuropeanNation" /><rdfs:comment>A large, industrialized European Nation.</rdfs:comment></rdf:Description><rdf:Description rdf:ID="Japan"><rdf:type rdf:resource="http://reliant.teknowledge.com/DAML/SUMO.owl#Nation" /><rdf:type rdf:resource="http://reliant.teknowledge.com/DAML/SUMO.owl#Island" /><rdfs:comment>A large industrialized Asian Nation.</rdfs:comment></rdf:Description><rdf:Description rdf:ID="JerusalemIsrael"><rdf:type rdf:resource="http://reliant.teknowledge.com/DAML/SUMO.owl#City" /><capitalCity rdf:resource="#Israel" /><rdfs:comment>The capital and largest City in Israel.  

It is regarded as a holy city by Muslims, Jews, and Christians.</rdfs:comment></rdf:Description><rdf:Description rdf:ID="Judaism"><rdf:type rdf:resource="http://reliant.teknowledge.com/DAML/SUMO.owl#BeliefGroup" /><rdfs:comment>The religion developed among the ancient Hebrews and

characterized by belief in one transcendent God who has revealed Himself to

Abraham, Moses, and the Hebrew prophets and by a religious life in accordance

with Scriptures and rabbinic traditions.</rdfs:comment></rdf:Description><rdf:Description rdf:ID="KansasCityMissouri"><rdf:type rdf:resource="#AmericanCity" /><sumo:part rdf:resource="#Missouri" /><rdfs:comment>A large City at the western edge of 

Missouri.</rdfs:comment></rdf:Description><rdf:Description rdf:ID="Kentucky"><rdf:type rdf:resource="#AmericanState" /><rdfs:comment>A state in the southeastern UnitedStates.</rdfs:comment></rdf:Description><rdf:Description rdf:ID="King"><sumo:subAttribute rdf:resource="#Monarch" /></rdf:Description><rdf:Description rdf:ID="Kneeling"><rdf:type rdf:resource="http://reliant.teknowledge.com/DAML/SUMO.owl#BodyPosition" /><rdfs:comment>The BodyPosition of resting one's weight on one's 

Knees.</rdfs:comment></rdf:Description><rdf:Description rdf:ID="Knight"><rdf:type rdf:resource="http://reliant.teknowledge.com/DAML/SUMO.owl#SocialRole" /><rdfs:comment>A SocialRole that is assigned by the 

UnitedKingdomOfGreatBritianAndNorthernIreland to persons for 

reasons of personal merit.</rdfs:comment></rdf:Description><rdf:Description rdf:ID="KoreanPeninsula"><rdf:type rdf:resource="#Peninsula" /><sumo:part rdf:resource="#Asia" /><rdfs:comment>A Peninsula in Asia that separates 

the Yellow Sea from the Sea of Japan.  It is occupied by the nations of 

North and South Korea.</rdfs:comment></rdf:Description><rdf:Description rdf:ID="Laos"><rdf:type rdf:resource="http://reliant.teknowledge.com/DAML/SUMO.owl#Nation" /><rdfs:comment>A Nation in southeastern Asia.</rdfs:comment></rdf:Description><rdf:Description rdf:ID="LatinLanguage"><rdf:type rdf:resource="http://reliant.teknowledge.com/DAML/SUMO.owl#SpokenHumanLanguage" /><rdf:type rdf:resource="http://reliant.teknowledge.com/DAML/SUMO.owl#NaturalLanguage" /><rdfs:comment>A Language that was spoken in ancient Rome and 

is still the official language of the Vatican.</rdfs:comment></rdf:Description><rdf:Description rdf:ID="Legal"><sumo:subAttribute rdf:resource="http://reliant.teknowledge.com/DAML/SUMO.owl#Permission" /><rdfs:comment>A proposition is Legal just in case it is not inconsistent 

with any proposition that is a Law.</rdfs:comment></rdf:Description><rdf:Description rdf:ID="LegislativeBill"><rdf:type rdf:resource="http://reliant.teknowledge.com/DAML/SUMO.owl#DeonticAttribute" /><rdfs:comment>The Attribute of being a proposed law, 

i.e. being under consideration by a legislative body of Government.</rdfs:comment></rdf:Description><rdf:Description rdf:ID="LevelShape"><rdf:type rdf:resource="http://reliant.teknowledge.com/DAML/SUMO.owl#ShapeAttribute" /><rdfs:comment>The ShapeAttribute of Objects where no 

part of the top of the Object is higher than any other part of the 

top.</rdfs:comment></rdf:Description><rdf:Description rdf:ID="LieutenantGovernor"><rdf:type rdf:resource="http://reliant.teknowledge.com/DAML/SUMO.owl#Position" /><rdfs:comment>The second-in-command of some Governments 

of AmericanStates.</rdfs:comment></rdf:Description><rdf:Description rdf:ID="LineFormation"><rdf:type rdf:resource="http://reliant.teknowledge.com/DAML/SUMO.owl#ShapeAttribute" /><rdfs:comment>A ShapeAttribute that applies to 

Collections and indicates that all of the members of the Collection 

are arrayed in a line, i.e. each member (except possibly the first) is 

behind or to the side of exactly one other member.</rdfs:comment></rdf:Description><rdf:Description rdf:ID="Linguistics"><rdf:type rdf:resource="#SocialScience" /><rdfs:comment>The field of linguistics.</rdfs:comment></rdf:Description><rdf:Description rdf:ID="LiteracyAttribute"><rdf:type rdf:resource="http://reliant.teknowledge.com/DAML/SUMO.owl#TraitAttribute" /><rdfs:comment>The ability to read and write.  Someone who 

has this Attribute is able to read and write.</rdfs:comment></rdf:Description><rdf:Description rdf:ID="Literature"><rdf:type rdf:resource="http://reliant.teknowledge.com/DAML/SUMO.owl#FieldOfStudy" /><rdfs:comment>The study of literature, i.e. instances of FictionalText 

that are regarded as having special merit.</rdfs:comment></rdf:Description><rdf:Description rdf:ID="LondonUnitedKingdom"><rdf:type rdf:resource="#EuropeanCity" /><capitalCity rdf:resource="#UnitedKingdomOfGreatBritainAndNorthernIreland" /><rdfs:comment>The capital city and the largest city of the

UnitedKingdomOfGreatBritainAndNorthernIreland.</rdfs:comment></rdf:Description><rdf:Description rdf:ID="LongIsland"><rdf:type rdf:resource="http://reliant.teknowledge.com/DAML/SUMO.owl#Island" /><sumo:part rdf:resource="#NewYorkState" /><rdfs:comment>A large Island off the coast of NewYorkState.  

The boroughs of Queens and Brooklyn make up the western end of this 

Island.</rdfs:comment></rdf:Description><rdf:Description rdf:ID="LosAngelesCalifornia"><rdf:type rdf:resource="#AmericanCity" /><sumo:part rdf:resource="#California" /><rdfs:comment>The largest City in California.</rdfs:comment></rdf:Description><rdf:Description rdf:ID="Lost"><rdf:type rdf:resource="http://reliant.teknowledge.com/DAML/SUMO.owl#ContestAttribute" /><rdfs:comment>The ContestAttribute that applies to a contestParticipant 

who has lost the Contest.</rdfs:comment></rdf:Description><rdf:Description rdf:ID="Louisiana"><rdf:type rdf:resource="#AmericanState" /><rdfs:comment>A state in the south-central part of the UnitedStates.  

It borders on the Gulf of Mexico and is for its bayous and cajun culture.</rdfs:comment></rdf:Description><rdf:Description rdf:ID="Malfunctioning"><rdf:type rdf:resource="#DeviceAttribute" /><rdfs:comment>Indicates that a Device is not performing 

its intended function.</rdfs:comment></rdf:Description><rdf:Description rdf:ID="ManchesterNewHampshire"><rdf:type rdf:resource="#AmericanCity" /><rdfs:comment>The largest City in New Hampshire.</rdfs:comment></rdf:Description><rdf:Description rdf:ID="MarketEconomy"><rdf:type rdf:resource="#EconomicSystemAttribute" /><rdfs:comment>MarketEconomy is an Attribute that 

describes an economy in which market forces, specifically supply and 

demand, provide input for privately managed decisions about pricing 

and production of goods.</rdfs:comment></rdf:Description><rdf:Description rdf:ID="MarketSocialism"><rdf:type rdf:resource="#EconomicSystemAttribute" /><sumo:subAttribute rdf:resource="#PartialMarketEconomy" /></rdf:Description><rdf:Description rdf:ID="MarriageContract"><sumo:subAttribute rdf:resource="http://reliant.teknowledge.com/DAML/SUMO.owl#Contract" /><rdfs:comment>A Contract between a married couple 

about how assets owned by the couple will be distributed in the event 

that the couple is divorced.</rdfs:comment></rdf:Description><rdf:Description rdf:ID="Maryland"><rdf:type rdf:resource="#AmericanState" /><sumo:meetsSpatially rdf:resource="#WashingtonDC" /><rdfs:comment>A state in the eastern UnitedStates that 

borders on WashingtonDC.</rdfs:comment></rdf:Description><rdf:Description rdf:ID="Massachusetts"><rdf:type rdf:resource="#AmericanState" /><sumo:part rdf:resource="#NewEngland" /><rdfs:comment>A northeastern AmericanState.  Its largest City 

is BostonMassachusetts.</rdfs:comment></rdf:Description><rdf:Description rdf:ID="Mathematics"><rdf:type rdf:resource="http://reliant.teknowledge.com/DAML/SUMO.owl#FieldOfStudy" /><rdfs:comment>The FieldOfStudy dealing with quantities and their 

relations to one another.</rdfs:comment></rdf:Description><rdf:Description rdf:ID="Mayor"><rdf:type rdf:resource="http://reliant.teknowledge.com/DAML/SUMO.owl#Position" /><rdfs:comment>The head of the Government of a City.</rdfs:comment></rdf:Description><rdf:Description rdf:ID="MediterraneanSea"><rdf:type rdf:resource="#Sea" /></rdf:Description><rdf:Description rdf:ID="MemphisTennessee"><rdf:type rdf:resource="#AmericanCity" /><sumo:part rdf:resource="#Tennessee" /><rdfs:comment>The largest City in Tennessee, 

located on the MississippiRiver.</rdfs:comment></rdf:Description><rdf:Description rdf:ID="Mexico"><rdf:type rdf:resource="http://reliant.teknowledge.com/DAML/SUMO.owl#Nation" /><sumo:meetsSpatially rdf:resource="#UnitedStates" /><rdfs:comment>A large Spanish-speaking country that borders on 

the UnitedStates.</rdfs:comment></rdf:Description><rdf:Description rdf:ID="Michigan"><rdf:type rdf:resource="#AmericanState" /><rdfs:comment>A populous and industrial state in the midwestern 

UnitedStates.</rdfs:comment></rdf:Description><rdf:Description rdf:ID="MilitaryCommander"><rdf:type rdf:resource="http://reliant.teknowledge.com/DAML/SUMO.owl#Position" /></rdf:Description><rdf:Description rdf:ID="MilitaryDictatorship"><rdf:type rdf:resource="#FormOfGovernment" /><sumo:subAttribute rdf:resource="#Dictatorship" /></rdf:Description><rdf:Description rdf:ID="MilitaryScience"><rdf:type rdf:resource="http://reliant.teknowledge.com/DAML/SUMO.owl#FieldOfStudy" /><rdfs:comment>The study of the principles of war.</rdfs:comment></rdf:Description><rdf:Description rdf:ID="MinneapolisMinnesota"><rdf:type rdf:resource="#AmericanCity" /><sumo:part rdf:resource="#Minnesota" /><rdfs:comment>The largest City in Minnesota.</rdfs:comment></rdf:Description><rdf:Description rdf:ID="Minnesota"><rdf:type rdf:resource="#AmericanState" /><rdfs:comment>A state in the northern midwest of the UnitedStates.</rdfs:comment></rdf:Description><rdf:Description rdf:ID="Mississippi"><rdf:type rdf:resource="#AmericanState" /><rdfs:comment>A state in the southeastern UnitedStates that 

borders on the Gulf of Mexico.</rdfs:comment></rdf:Description><rdf:Description rdf:ID="MississippiRiver"><rdf:type rdf:resource="#River" /><sumo:part rdf:resource="#UnitedStates" /><rdfs:comment>The major River in the UnitedStates.  

It runs almost the entire width of the UnitedStates, from Minnesota 

to the Gulf of Mexico.</rdfs:comment></rdf:Description><rdf:Description rdf:ID="Missouri"><rdf:type rdf:resource="#AmericanState" /><rdfs:comment>A state in the central UnitedStates.</rdfs:comment></rdf:Description><rdf:Description rdf:ID="MixedEconomy"><rdf:type rdf:resource="#EconomicSystemAttribute" /><rdfs:comment>MixedEconomy is the Attribute 

of a country whose economy has elements of more than one pure 

economic system, e.g., a market economy with government welfare 

for unemployed workers.  A mixed-economy country may be a 

country in transition, as from a prior communist economy to 

capitalism, but a mixed economy may also be a stable combination 

of different economic approaches in different areas of a national 

economy, e.g., nationally managed health care and education systems 

in an otherwise private-enterprise economy.</rdfs:comment></rdf:Description><rdf:Description rdf:ID="Monarch"><rdf:type rdf:resource="http://reliant.teknowledge.com/DAML/SUMO.owl#Position" /></rdf:Description><rdf:Description rdf:ID="Monarchy"><rdf:type rdf:resource="#FormOfGovernment" /><rdfs:comment>Monarchy is the attribute of a government 

that is ruled by a monarch, which is usually a hereditary role.</rdfs:comment><sumo:contraryAttribute rdf:resource="#Republic" /><sumo:contraryAttribute rdf:resource="#Federation" /></rdf:Description><rdf:Description rdf:ID="MontrealCanada"><rdf:type rdf:resource="http://reliant.teknowledge.com/DAML/SUMO.owl#City" /><sumo:part rdf:resource="#Canada" /><rdfs:comment>A large City in eastern Canada.</rdfs:comment></rdf:Description><rdf:Description rdf:ID="Morocco"><rdf:type rdf:resource="http://reliant.teknowledge.com/DAML/SUMO.owl#Nation" /><sumo:part rdf:resource="#Africa" /><rdfs:comment>A Nation in northwestern Africa.</rdfs:comment></rdf:Description><rdf:Description rdf:ID="MoscowRussia"><rdf:type rdf:resource="#EuropeanCity" /><capitalCity rdf:resource="#Russia" /><rdfs:comment>The capital of Russia and the largest 

City of the country.</rdfs:comment></rdf:Description><rdf:Description rdf:ID="MountainTimeZone"><rdf:type rdf:resource="http://reliant.teknowledge.com/DAML/SUMO.owl#TimeZone" /><rdfs:comment>A TimeZone that covers much of the 

Rocky Mountain region of the United States.</rdfs:comment></rdf:Description><rdf:Description rdf:ID="MultipartyDemocracy"><rdf:type rdf:resource="#FormOfGovernment" /><sumo:subAttribute rdf:resource="#Democracy" /></rdf:Description><rdf:Description rdf:ID="Myanmar"><rdf:type rdf:resource="http://reliant.teknowledge.com/DAML/SUMO.owl#Nation" /><rdfs:comment>A Nation in southeastern Asia, formerly known 

as Burma.</rdfs:comment></rdf:Description><rdf:Description rdf:ID="NapoleonicCode"><sumo:subAttribute rdf:resource="#CivilLaw" /><rdf:type rdf:resource="#LegalSystemAttribute" /><rdfs:comment>NapoleonicCode is the specialization of 

CivilLaw developed in France under Napoleon Bonaparte.  It is still the 

basis of French law as well as of legal systems developed under French 

influence.</rdfs:comment></rdf:Description><rdf:Description rdf:ID="NashvilleTennessee"><rdf:type rdf:resource="#AmericanCity" /><sumo:part rdf:resource="#Tennessee" /><rdfs:comment>A large City in Tennessee.</rdfs:comment></rdf:Description><rdf:Description rdf:ID="NationalizedIndustryEconomy"><rdf:type rdf:resource="#EconomicSystemAttribute" /><sumo:subAttribute rdf:resource="#GovernmentRegulatedEconomy" /><rdfs:comment>NationalizedIndustryEconomy 

is an Attribute describing an economy in which the major industries,  

such as energy and transportation, are owned by the national government.</rdfs:comment></rdf:Description><rdf:Description rdf:ID="NaziParty"><rdf:type rdf:resource="#PoliticalParty" /><rdfs:comment>The German PoliticalParty headed by Adolf Hitler.</rdfs:comment></rdf:Description><rdf:Description rdf:ID="Netherlands"><rdf:type rdf:resource="#EuropeanNation" /><rdfs:comment>A small Nation in western Europe.</rdfs:comment></rdf:Description><rdf:Description rdf:ID="NewEngland"><rdf:type rdf:resource="http://reliant.teknowledge.com/DAML/SUMO.owl#GeographicArea" /><sumo:part rdf:resource="#UnitedStates" /><rdfs:comment>A GeographicArea in the UnitedStates that is 

made up of the states of Maine, New Hampshire, Vermont, Massachusetts, Rhode Island, 

and Connecticut.</rdfs:comment></rdf:Description><rdf:Description rdf:ID="NewMexico"><rdf:type rdf:resource="#AmericanState" /><rdfs:comment>A southwestern state in the UnitedStates.</rdfs:comment></rdf:Description><rdf:Description rdf:ID="NewYorkCity"><rdf:type rdf:resource="#AmericanCity" /><sumo:part rdf:resource="#NewYorkState" /><rdfs:comment>The largest city in the UnitedStates.  

A worldwide center of finance and culture, it is comprised of five boroughs.</rdfs:comment></rdf:Description><rdf:Description rdf:ID="NewYorkState"><rdf:type rdf:resource="#AmericanState" /><rdfs:comment>A populous state in the northeastern UnitedStates.</rdfs:comment></rdf:Description><rdf:Description rdf:ID="NorthAmerica"><rdf:type rdf:resource="http://reliant.teknowledge.com/DAML/SUMO.owl#Continent" /></rdf:Description><rdf:Description rdf:ID="NorthCarolina"><rdf:type rdf:resource="#AmericanState" /><rdfs:comment>A state in the southeastern UnitedStates.</rdfs:comment></rdf:Description><rdf:Description rdf:ID="NorthDakota"><rdf:type rdf:resource="#AmericanState" /><rdfs:comment>A state in the northern midwest of the UnitedStates.</rdfs:comment></rdf:Description><rdf:Description rdf:ID="NorthSea"><rdf:type rdf:resource="#Sea" /></rdf:Description><rdf:Description rdf:ID="NorthernHemisphere"><rdf:type rdf:resource="#Hemisphere" /><rdfs:comment>The half of the Earth that lies above the 

equator.</rdfs:comment></rdf:Description><rdf:Description rdf:ID="Oceania"><rdf:type rdf:resource="http://reliant.teknowledge.com/DAML/SUMO.owl#Continent" /></rdf:Description><rdf:Description rdf:ID="Ohio"><rdf:type rdf:resource="#AmericanState" /><rdfs:comment>A populous and industrial state in the midwestern 

UnitedStates.</rdfs:comment></rdf:Description><rdf:Description rdf:ID="OrangeColor"><rdf:type rdf:resource="#SecondaryColor" /><rdfs:comment>A SecondaryColor that results from mixing Red 

and Yellow and resembles the color of a ripe orange fruit.</rdfs:comment></rdf:Description><rdf:Description rdf:ID="PacificOcean"><rdf:type rdf:resource="#Ocean" /><rdfs:comment>PacificOcean represents the Pacific  

Ocean.</rdfs:comment></rdf:Description><rdf:Description rdf:ID="PacificTimeZone"><rdf:type rdf:resource="http://reliant.teknowledge.com/DAML/SUMO.owl#TimeZone" /><rdfs:comment>A TimeZone that covers much of the 

western part of the United States.</rdfs:comment></rdf:Description><rdf:Description rdf:ID="Pain"><sumo:subAttribute rdf:resource="#Unhappiness" /><rdfs:comment>A physical sensation of discomfort which can vary widely 

in intensity.</rdfs:comment></rdf:Description><rdf:Description rdf:ID="Palestine"><rdf:type rdf:resource="#OverseasArea" /><dependentGeopoliticalArea rdf:resource="#UnitedKingdomOfGreatBritainAndNorthernIreland" /><rdfs:comment>A GeopoliticalArea that was divided by the 

UnitedKingdomOfGreatBritainAndNorthernIreland into Israel and 

Jordan in 1948.</rdfs:comment></rdf:Description><rdf:Description rdf:ID="ParisFrance"><rdf:type rdf:resource="#EuropeanCity" /><capitalCity rdf:resource="#France" /><rdfs:comment>The capital of France and the largest City 

of the country.</rdfs:comment></rdf:Description><rdf:Description rdf:ID="ParliamentaryDemocracy"><rdf:type rdf:resource="#FormOfGovernment" /><sumo:subAttribute rdf:resource="#ParliamentaryGovernment" /><sumo:subAttribute rdf:resource="#Democracy" /></rdf:Description><rdf:Description rdf:ID="ParliamentaryDemocraticRepublic"><rdf:type rdf:resource="#FormOfGovernment" /><sumo:subAttribute rdf:resource="#Republic" /><sumo:subAttribute rdf:resource="#Democracy" /></rdf:Description><rdf:Description rdf:ID="ParliamentaryGovernment"><rdf:type rdf:resource="#FormOfGovernment" /><rdfs:comment>ParliamentaryGovernment is the 

attribute of a government whose chief LegislativeOrganization is a 

Parliament.  A parliamentary government is compatible with various 

other government types, including Monarchy.</rdfs:comment></rdf:Description><rdf:Description rdf:ID="ParliamentaryRepublic"><rdf:type rdf:resource="#FormOfGovernment" /><sumo:subAttribute rdf:resource="#ParliamentaryGovernment" /><sumo:subAttribute rdf:resource="#Republic" /></rdf:Description><rdf:Description rdf:ID="PartialMarketEconomy"><rdf:type rdf:resource="#EconomicSystemAttribute" /><sumo:subAttribute rdf:resource="#MixedEconomy" /></rdf:Description><rdf:Description rdf:ID="Pennsylvania"><rdf:type rdf:resource="#AmericanState" /><rdfs:comment>A mid-Atlantic AmericanState.  Its two major cities 

are Philadelphia and Pittsburgh.</rdfs:comment></rdf:Description><rdf:Description rdf:ID="PhiladelphiaPennsylvania"><rdf:type rdf:resource="#AmericanCity" /><sumo:part rdf:resource="#Pennsylvania" /><rdfs:comment>The largest City in Pennsylvania.</rdfs:comment></rdf:Description><rdf:Description rdf:ID="Philosophy"><rdf:type rdf:resource="http://reliant.teknowledge.com/DAML/SUMO.owl#FieldOfStudy" /><rdfs:comment>The study of first principles, including epistemology, 

metaphysics, and ethics.</rdfs:comment></rdf:Description><rdf:Description rdf:ID="Physics"><rdf:type rdf:resource="#Science" /><rdfs:comment>The study of matter and energy and their relations.</rdfs:comment></rdf:Description><rdf:Description rdf:ID="Pink"><rdf:type rdf:resource="#SecondaryColor" /><rdfs:comment>A SecondaryColor that results from mixing Red and 

White.</rdfs:comment></rdf:Description><rdf:Description rdf:ID="PittsburghPennsylvania"><rdf:type rdf:resource="#AmericanCity" /><sumo:part rdf:resource="#Pennsylvania" /><rdfs:comment>The second largest City in 

Pennsylvania.  It was once a center of steel production in the 

UnitedStates.</rdfs:comment></rdf:Description><rdf:Description rdf:ID="PlanetEarth"><rdf:type rdf:resource="#Planet" /><orbits rdf:resource="#Sol" /></rdf:Description><rdf:Description rdf:ID="PlanetJupiter"><rdf:type rdf:resource="#Planet" /><orbits rdf:resource="#Sol" /></rdf:Description><rdf:Description rdf:ID="PlanetMars"><rdf:type rdf:resource="#Planet" /><orbits rdf:resource="#Sol" /></rdf:Description><rdf:Description rdf:ID="PlanetMercury"><rdf:type rdf:resource="#Planet" /><orbits rdf:resource="#Sol" /></rdf:Description><rdf:Description rdf:ID="PlanetNeptune"><rdf:type rdf:resource="#Planet" /><orbits rdf:resource="#Sol" /></rdf:Description><rdf:Description rdf:ID="PlanetPluto"><rdf:type rdf:resource="#Planet" /><orbits rdf:resource="#Sol" /></rdf:Description><rdf:Description rdf:ID="PlanetSaturn"><rdf:type rdf:resource="#Planet" /><orbits rdf:resource="#Sol" /></rdf:Description><rdf:Description rdf:ID="PlanetUranus"><rdf:type rdf:resource="#Planet" /><orbits rdf:resource="#Sol" /></rdf:Description><rdf:Description rdf:ID="PlanetVenus"><rdf:type rdf:resource="#Planet" /><orbits rdf:resource="#Sol" /></rdf:Description><rdf:Description rdf:ID="Pliable"><rdf:type rdf:resource="http://reliant.teknowledge.com/DAML/SUMO.owl#ShapeAttribute" /><rdfs:comment>The shape of an Object with this Attribute 

can be altered.</rdfs:comment></rdf:Description><rdf:Description rdf:ID="Poland"><rdf:type rdf:resource="#EuropeanNation" /><rdfs:comment>A EuropeanNation in central Europe.</rdfs:comment></rdf:Description><rdf:Description rdf:ID="PoliticalScience"><rdf:type rdf:resource="#SocialScience" /><rdfs:comment>The field of political science.</rdfs:comment></rdf:Description><rdf:Description rdf:ID="Pope"><rdf:type rdf:resource="http://reliant.teknowledge.com/DAML/SUMO.owl#Position" /><rdfs:comment>The Position of head of the RomanCatholicChurch.</rdfs:comment></rdf:Description><rdf:Description rdf:ID="Pregnant"><rdf:type rdf:resource="http://reliant.teknowledge.com/DAML/SUMO.owl#BiologicalAttribute" /><rdfs:comment>The Attribute that applies to Female Animals and 

Humans that have an embryo or fetus growing inside of them as the result of 

having one of the Female's Eggs fertilized.</rdfs:comment></rdf:Description><rdf:Description rdf:ID="President"><rdf:type rdf:resource="http://reliant.teknowledge.com/DAML/SUMO.owl#Position" /></rdf:Description><rdf:Description rdf:ID="PresidentOfTheUnitedStates"><rdf:type rdf:resource="http://reliant.teknowledge.com/DAML/SUMO.owl#Position" /><rdfs:comment>The position of being head of the 

UnitedStates.</rdfs:comment></rdf:Description><rdf:Description rdf:ID="PresidentialGovernment"><rdf:type rdf:resource="#FormOfGovernment" /></rdf:Description><rdf:Description rdf:ID="PrimeMinister"><rdf:type rdf:resource="http://reliant.teknowledge.com/DAML/SUMO.owl#Position" /></rdf:Description><rdf:Description rdf:ID="PrivateEnterpriseEconomy"><rdf:type rdf:resource="#EconomicSystemAttribute" /><sumo:subAttribute rdf:resource="#CapitalistEconomy" /><rdfs:comment>PrivateEnterpriseEconomy is 

the Attribute used to characterize a country in which private 

enterprise is the main source of economic wealth.</rdfs:comment></rdf:Description><rdf:Description rdf:ID="PrivatizingEconomy"><rdf:type rdf:resource="#EconomicSystemAttribute" /><sumo:subAttribute rdf:resource="#MixedEconomy" /><rdfs:comment>PrivatizingEconomy is an 

Attribute that describes a country in which formerly government-

owned industries are being transferred into private holdings.</rdfs:comment></rdf:Description><rdf:Description rdf:ID="ProvidenceRhodeIsland"><rdf:type rdf:resource="#AmericanCity" /><capitalCity rdf:resource="#RhodeIsland" /><rdfs:comment>The largest and capital city of 

RhodeIsland.</rdfs:comment></rdf:Description><rdf:Description rdf:ID="Psychology"><rdf:type rdf:resource="#SocialScience" /><rdfs:comment>The field of psychology.</rdfs:comment></rdf:Description><rdf:Description rdf:ID="Puberty"><sumo:subAttribute rdf:resource="http://reliant.teknowledge.com/DAML/SUMO.owl#NonFullyFormed" /><rdfs:comment>The DevelopmentalAttribute of having functional sex 

glands which are not fully mature.</rdfs:comment></rdf:Description><rdf:Description rdf:ID="PuertoRico"><rdf:type rdf:resource="http://reliant.teknowledge.com/DAML/SUMO.owl#Island" /><sumo:part rdf:resource="#UnitedStates" /><rdfs:comment>An autonomous part of the UnitedStates.</rdfs:comment></rdf:Description><rdf:Description rdf:ID="PurchaseContract"><sumo:subAttribute rdf:resource="http://reliant.teknowledge.com/DAML/SUMO.owl#Contract" /><rdfs:comment>A Contract between two Agents in 

which one Agent agrees to render the other some good or service in 

exchange for currency.</rdfs:comment></rdf:Description><rdf:Description rdf:ID="PureCapitalistEconomy"><rdf:type rdf:resource="#EconomicSystemAttribute" /><sumo:subAttribute rdf:resource="#CapitalistEconomy" /><sumo:contraryAttribute rdf:resource="#MixedEconomy" /><rdfs:comment>PureCapitalistEconomy is an 

Attribute representing a capitalist economy that has no admixture of 

socialism.</rdfs:comment></rdf:Description><rdf:Description rdf:ID="PureSocialistEconomy"><rdf:type rdf:resource="#EconomicSystemAttribute" /><sumo:subAttribute rdf:resource="#SocialistEconomy" /><sumo:contraryAttribute rdf:resource="#MixedEconomy" /><sumo:contraryAttribute rdf:resource="#PureCapitalistEconomy" /><rdfs:comment>PureSocialistEconomy is an 

Attribute representing a socialist economy that has no admixture of 

capitalism.</rdfs:comment></rdf:Description><rdf:Description rdf:ID="Purple"><rdf:type rdf:resource="#SecondaryColor" /><rdfs:comment>A SecondaryColor that results from mixing Red and 

Blue.</rdfs:comment></rdf:Description><rdf:Description rdf:ID="Queen"><sumo:subAttribute rdf:resource="#Monarch" /></rdf:Description><rdf:Description rdf:ID="RedRiver"><rdf:type rdf:resource="#River" /><sumo:part rdf:resource="#MississippiRiver" /><rdfs:comment>A tributary of the Mississippi River.</rdfs:comment></rdf:Description><rdf:Description rdf:ID="RedSea"><rdf:type rdf:resource="#Sea" /></rdf:Description><rdf:Description rdf:ID="Republic"><rdf:type rdf:resource="#FormOfGovernment" /><rdfs:comment>Republic is the attribute of a government 

whose power and authority are vested in its members, who elect 

representatives to exercise that power.</rdfs:comment></rdf:Description><rdf:Description rdf:ID="RepublicanParty"><rdf:type rdf:resource="#PoliticalParty" /><rdfs:comment>One of the two major political parties in 

the UnitedStates.  The RepublicanParty represents traditional, 

conservative values.</rdfs:comment></rdf:Description><rdf:Description rdf:ID="RhodeIsland"><rdf:type rdf:resource="#AmericanState" /><sumo:part rdf:resource="#NewEngland" /><rdfs:comment>A northeastern AmericanState.  Its capital city is 

ProvidenceRhodeIsland.</rdfs:comment></rdf:Description><rdf:Description rdf:ID="RichmondVirginia"><rdf:type rdf:resource="#AmericanCity" /><capitalCity rdf:resource="#Virginia" /><rdfs:comment>The capital of Virginia, located in the 

east-central part of the state.</rdfs:comment></rdf:Description><rdf:Description rdf:ID="Rigid"><rdf:type rdf:resource="http://reliant.teknowledge.com/DAML/SUMO.owl#ShapeAttribute" /><sumo:contraryAttribute rdf:resource="#Pliable" /><rdfs:comment>The shape of an Object with this Attribute 

cannot be altered.</rdfs:comment></rdf:Description><rdf:Description rdf:ID="RomanCatholicChurch"><rdf:type rdf:resource="http://reliant.teknowledge.com/DAML/SUMO.owl#ReligiousOrganization" /><rdfs:comment>The RomanCatholicChurch is the

ReligiousOrganization that promulgates RomanCatholicism.</rdfs:comment></rdf:Description><rdf:Description rdf:ID="RomeItaly"><rdf:type rdf:resource="#EuropeanCity" /><capitalCity rdf:resource="#Italy" /><rdfs:comment>The capital of Italy and the largest City 

of the country.</rdfs:comment></rdf:Description><rdf:Description rdf:ID="Russia"><rdf:type rdf:resource="#EuropeanNation" /><rdfs:comment>A Nation which is currently independent, but which 

was once part of the SovietUnion.</rdfs:comment></rdf:Description><rdf:Description rdf:ID="RussianLanguage"><rdf:type rdf:resource="http://reliant.teknowledge.com/DAML/SUMO.owl#SpokenHumanLanguage" /><rdf:type rdf:resource="http://reliant.teknowledge.com/DAML/SUMO.owl#NaturalLanguage" /><rdfs:comment>A Slavic language that is spoken in Russia.</rdfs:comment></rdf:Description><rdf:Description rdf:ID="SaintLouisMissouri"><rdf:type rdf:resource="#AmericanCity" /><sumo:part rdf:resource="#Missouri" /><rdfs:comment>A large City in Missouri.</rdfs:comment></rdf:Description><rdf:Description rdf:ID="SaintPaulMinnesota"><rdf:type rdf:resource="#AmericanCity" /><capitalCity rdf:resource="#Minnesota" /><sumo:meetsSpatially rdf:resource="#MinneapolisMinnesota" /><rdfs:comment>The capital of Minnesota, borders 

MinneapolisMinnesota.</rdfs:comment></rdf:Description><rdf:Description rdf:ID="SanFranciscoCalifornia"><rdf:type rdf:resource="#AmericanCity" /><sumo:part rdf:resource="#California" /><rdfs:comment>A large City in California, 

located on the San Francisco Bay.</rdfs:comment></rdf:Description><rdf:Description rdf:ID="Satisfaction"><sumo:subAttribute rdf:resource="#Happiness" /><rdfs:comment>The state of being happy about a state of

affairs that occurred in the past.  In cases where that state of affairs 

is the product of one's own doing, this is known as pride.</rdfs:comment></rdf:Description><rdf:Description rdf:ID="SavannahGeorgia"><rdf:type rdf:resource="#AmericanCity" /><sumo:part rdf:resource="#Georgia" /><rdfs:comment>A City in Georgia near the mouth of 

the Savannah River.</rdfs:comment></rdf:Description><rdf:Description rdf:ID="Scotland"><rdf:type rdf:resource="http://reliant.teknowledge.com/DAML/SUMO.owl#GeopoliticalArea" /><sumo:part rdf:resource="#UnitedKingdomOfGreatBritainAndNorthernIreland" /><rdfs:comment>A division of the UnitedKingdomOfGreatBritainAndNorthernIreland.</rdfs:comment></rdf:Description><rdf:Description rdf:ID="SecretaryOfTheInterior"><rdf:type rdf:resource="#GovernmentSecretary" /><rdfs:comment>The head of the UnitedStatesDepartmentOfInterior.</rdfs:comment></rdf:Description><rdf:Description rdf:ID="SecretaryOfTheTreasury"><rdf:type rdf:resource="#GovernmentSecretary" /><rdfs:comment>The head of the United States Treasury Department.</rdfs:comment></rdf:Description><rdf:Description rdf:ID="ServiceContract"><sumo:subAttribute rdf:resource="http://reliant.teknowledge.com/DAML/SUMO.owl#Contract" /><rdfs:comment>A Contract where an Agent agrees to 

perform a service for another Agent (usually for a price).</rdfs:comment></rdf:Description><rdf:Description rdf:ID="Sober"><rdf:type rdf:resource="http://reliant.teknowledge.com/DAML/SUMO.owl#ConsciousnessAttribute" /><rdfs:comment>The ConsciousnessAttribute of someone whose motor and

cognitive faculties are not significantly impaired by a BiologicallyActiveSubstance.</rdfs:comment></rdf:Description><rdf:Description rdf:ID="SocialistEconomy"><rdf:type rdf:resource="#EconomicSystemAttribute" /><rdfs:comment>SocialistEconomy is the Attribute 

used to characterize a country in which there is government ownership 

or direction of the means of production and distribution.</rdfs:comment></rdf:Description><rdf:Description rdf:ID="Sol"><rdf:type rdf:resource="#Star" /><rdfs:comment>Sol is the nearest Star to PlanetEarth and 

the focus of its SolarSystem.</rdfs:comment></rdf:Description><rdf:Description rdf:ID="SouthAmerica"><rdf:type rdf:resource="http://reliant.teknowledge.com/DAML/SUMO.owl#Continent" /></rdf:Description><rdf:Description rdf:ID="SouthernHemisphere"><rdf:type rdf:resource="#Hemisphere" /><rdfs:comment>The half of the Earth that lies below the 

equator.</rdfs:comment></rdf:Description><rdf:Description rdf:ID="SovietUnion"><rdf:type rdf:resource="#EuropeanNation" /><rdfs:comment>The former communist nation of the Soviet Union.</rdfs:comment></rdf:Description><rdf:Description rdf:ID="Spain"><rdf:type rdf:resource="#EuropeanNation" /><rdfs:comment>A large, industrialized European Nation.</rdfs:comment></rdf:Description><rdf:Description rdf:ID="SpanishLanguage"><rdf:type rdf:resource="http://reliant.teknowledge.com/DAML/SUMO.owl#SpokenHumanLanguage" /><rdf:type rdf:resource="http://reliant.teknowledge.com/DAML/SUMO.owl#NaturalLanguage" /><rdfs:comment>A Romance language that is the official language 

of Spain, Mexico, and many Central and South American countries.</rdfs:comment></rdf:Description><rdf:Description rdf:ID="Splitting"><rdf:type rdf:resource="http://reliant.teknowledge.com/DAML/SUMO.owl#BodyPosition" /><rdfs:comment>The BodyPosition of extending one's Legs at 

right angles to one's Torso.</rdfs:comment></rdf:Description><rdf:Description rdf:ID="SportsOut"><rdf:type rdf:resource="#SportsAttribute" /><rdfs:comment>A SportsAttribute that indicates that a player in 

a Sport can no longer compete because he has been tagged with the GamePiece.</rdfs:comment></rdf:Description><rdf:Description rdf:ID="Squatting"><sumo:subAttribute rdf:resource="http://reliant.teknowledge.com/DAML/SUMO.owl#Sitting" /><rdfs:comment>Sitting on one's heels.</rdfs:comment></rdf:Description><rdf:Description rdf:ID="Stressed"><rdf:type rdf:resource="#LinguisticAttribute" /><rdfs:comment>A LinguisticAttribute of Syllables.  It denotes 

the quality of being emphasized over the other Syllables in the same 

Word.</rdfs:comment></rdf:Description><rdf:Description rdf:ID="Surprise"><rdf:type rdf:resource="http://reliant.teknowledge.com/DAML/SUMO.owl#EmotionalState" /><rdfs:comment>The EmotionalState that one experiences when something 

unexpected and of significance occurs.</rdfs:comment></rdf:Description><rdf:Description rdf:ID="Sweden"><rdf:type rdf:resource="#EuropeanNation" /><rdfs:comment>A Nation in scandinavian Europe.</rdfs:comment></rdf:Description><rdf:Description rdf:ID="Switzerland"><rdf:type rdf:resource="#EuropeanNation" /><rdfs:comment>A small politically neutral Nation in central 

Europe.</rdfs:comment></rdf:Description><rdf:Description rdf:ID="SymmetricShape"><rdf:type rdf:resource="http://reliant.teknowledge.com/DAML/SUMO.owl#ShapeAttribute" /><rdfs:comment>A ShapeAttribute that applies to a 

SelfConnectedObject that can be divided into two copies of each other.</rdfs:comment></rdf:Description><rdf:Description rdf:ID="Tennessee"><rdf:type rdf:resource="#AmericanState" /><rdfs:comment>A state in the southeastern UnitedStates.</rdfs:comment></rdf:Description><rdf:Description rdf:ID="Texas"><rdf:type rdf:resource="#AmericanState" /><rdfs:comment>The second largest AmericanState, located in the southwest 

on the Gulf of Mexico.</rdfs:comment></rdf:Description><rdf:Description rdf:ID="TheocraticGovernment"><rdf:type rdf:resource="#FormOfGovernment" /><sumo:subAttribute rdf:resource="#AuthoritarianRegime" /><rdfs:comment>TheocraticGovernment is the 

attribute of a government that bases its authority on Religion.</rdfs:comment></rdf:Description><rdf:Description rdf:ID="TheocraticRepublic"><rdf:type rdf:resource="#FormOfGovernment" /><sumo:subAttribute rdf:resource="#TheocraticGovernment" /></rdf:Description><rdf:Description rdf:ID="Theology"><rdf:type rdf:resource="http://reliant.teknowledge.com/DAML/SUMO.owl#FieldOfStudy" /><rdfs:comment>The systematic study of religious practice and religious truth.</rdfs:comment></rdf:Description><rdf:Description rdf:ID="TieScore"><rdf:type rdf:resource="http://reliant.teknowledge.com/DAML/SUMO.owl#ContestAttribute" /><rdfs:comment>The ContestAttribute that applies to all contestParticipants 

in a Contest when none of them have Won or Lost the Contest.</rdfs:comment></rdf:Description><rdf:Description rdf:ID="TokyoJapan"><rdf:type rdf:resource="http://reliant.teknowledge.com/DAML/SUMO.owl#City" /><capitalCity rdf:resource="#Japan" /><rdfs:comment>The capital and largest City in Japan.</rdfs:comment></rdf:Description><rdf:Description rdf:ID="Tourist"><rdf:type rdf:resource="http://reliant.teknowledge.com/DAML/SUMO.owl#SocialRole" /><rdfs:comment>Tourist is a SocialRole assumed by a person 

who is travelling for pleasure.</rdfs:comment></rdf:Description><rdf:Description rdf:ID="Tranquility"><sumo:subAttribute rdf:resource="#Happiness" /><sumo:contraryAttribute rdf:resource="#Anxiety" /><rdfs:comment>The state of being free from Anxiety.</rdfs:comment></rdf:Description><rdf:Description rdf:ID="TransitionalGovernment"><rdf:type rdf:resource="#FormOfGovernment" /><rdfs:comment>TransitionalGovernment is the 

attribute of a government that is changing from one form of government 

to another.  This may be accompanied by social unrest or instability.</rdfs:comment></rdf:Description><rdf:Description rdf:ID="Treaty"><sumo:subAttribute rdf:resource="http://reliant.teknowledge.com/DAML/SUMO.owl#Contract" /><rdfs:comment>Any Contract which holds between two or more 

Nations.</rdfs:comment></rdf:Description><rdf:Description rdf:ID="Tuberculosis"><rdf:type rdf:resource="#BacterialDisease" /><rdfs:comment>A BacterialDisease caused by the Tubercle Bacillus 

that results in lesions on various body parts, especially the Lungs.</rdfs:comment></rdf:Description><rdf:Description rdf:ID="Unbreakable"><rdf:type rdf:resource="#BreakabilityAttribute" /><sumo:contraryAttribute rdf:resource="#Fragile" /><rdfs:comment>An Attribute which indicates that the 

associated Object cannot be broken.</rdfs:comment></rdf:Description><rdf:Description rdf:ID="Unhappiness"><rdf:type rdf:resource="http://reliant.teknowledge.com/DAML/SUMO.owl#EmotionalState" /><sumo:contraryAttribute rdf:resource="#Happiness" /><rdfs:comment>The state of being unhappy, experiencing pain, 

sorrow or unease.</rdfs:comment></rdf:Description><rdf:Description rdf:ID="UnionStatesOfAmerica"><rdf:type rdf:resource="http://reliant.teknowledge.com/DAML/SUMO.owl#GeopoliticalArea" /><rdfs:comment>The states of the UnitedStates that the 

ConfederateStatesOfAmerica seceded from.</rdfs:comment></rdf:Description><rdf:Description rdf:ID="UnitaryRule"><rdf:type rdf:resource="#FormOfGovernment" /><rdfs:comment>UnitaryRule is a FormOfGovernment in which 

the central government controls affairs at all levels, including the local 

level.</rdfs:comment></rdf:Description><rdf:Description rdf:ID="UnitedKingdomOfGreatBritainAndNorthernIreland"><rdf:type rdf:resource="#EuropeanNation" /><rdfs:comment>The Nation comprising 

England, Scotland, Wales, and Northern Ireland.</rdfs:comment></rdf:Description><rdf:Description rdf:ID="UnitedNations"><rdf:type rdf:resource="#OrganizationOfNations" /><rdfs:comment>The UnitedNations has six principal 

subOrganizations: the Secretariat, the General Assembly, the Security 

Council, the Economic and Social Council, the Trusteeship Council 

(currently inactive), and the International Court of Justice.  The United 

Nations has numerous subordinate agencies and bodies within those six 

major subdivisions.</rdfs:comment></rdf:Description><rdf:Description rdf:ID="UnitedStates"><rdf:type rdf:resource="http://reliant.teknowledge.com/DAML/SUMO.owl#Nation" /><rdfs:comment>The North American republic of 50 states.</rdfs:comment></rdf:Description><rdf:Description rdf:ID="UnitedStatesCongress"><rdf:type rdf:resource="#LegislativeOrganization" /><rdfs:comment>The legislative branch of the government 

of the UnitedStates.</rdfs:comment></rdf:Description><rdf:Description rdf:ID="UnitedStatesDepartmentOfAgriculture"><rdf:type rdf:resource="http://reliant.teknowledge.com/DAML/SUMO.owl#GovernmentOrganization" /><rdfs:comment>Provides services to farmers in 

the UnitedStates.</rdfs:comment></rdf:Description><rdf:Description rdf:ID="UnitedStatesDepartmentOfDefense"><rdf:type rdf:resource="http://reliant.teknowledge.com/DAML/SUMO.owl#GovernmentOrganization" /><rdfs:comment>Entrusted with the national 

security of the UnitedStates.</rdfs:comment></rdf:Description><rdf:Description rdf:ID="UnitedStatesDepartmentOfInterior"><rdf:type rdf:resource="http://reliant.teknowledge.com/DAML/SUMO.owl#GovernmentOrganization" /><rdfs:comment>Manages and preserves public lands 

and natural resources in the UnitedStates.</rdfs:comment></rdf:Description><rdf:Description rdf:ID="UnitedStatesDepartmentOfState"><rdf:type rdf:resource="http://reliant.teknowledge.com/DAML/SUMO.owl#GovernmentOrganization" /><rdfs:comment>The subOrganization of the US 

government that sets and enforces foreign policy.</rdfs:comment></rdf:Description><rdf:Description rdf:ID="UnitedStatesHouseOfRepresentatives"><rdf:type rdf:resource="#LegislativeOrganization" /><sumo:part rdf:resource="#UnitedStatesCongress" /><rdfs:comment>One of the two legislatures 

that make up the UnitedStatesCongress.</rdfs:comment></rdf:Description><rdf:Description rdf:ID="UnitedStatesPostalService"><rdf:type rdf:resource="http://reliant.teknowledge.com/DAML/SUMO.owl#GovernmentOrganization" /><rdfs:comment>The GovernmentOrganization of the 

UnitedStates that is entrusted with delivering the mail.</rdfs:comment></rdf:Description><rdf:Description rdf:ID="UnitedStatesSenate"><rdf:type rdf:resource="#LegislativeOrganization" /><sumo:part rdf:resource="#UnitedStatesCongress" /><rdfs:comment>One of the two legislatures that make 

up the UnitedStatesCongress.</rdfs:comment></rdf:Description><rdf:Description rdf:ID="Upstairs"><rdf:type rdf:resource="http://reliant.teknowledge.com/DAML/SUMO.owl#PositionalAttribute" /><rdfs:comment>A PositionalAttribute to indicate that one thing is 

one or more floors above a second thing in the same building.</rdfs:comment></rdf:Description><rdf:Description rdf:ID="Vermont"><rdf:type rdf:resource="#AmericanState" /><sumo:part rdf:resource="#NewEngland" /><rdfs:comment>A northeastern AmericanState know for its small towns 

and rustic beauty.</rdfs:comment></rdf:Description><rdf:Description rdf:ID="Veteran"><rdf:type rdf:resource="http://reliant.teknowledge.com/DAML/SUMO.owl#SocialRole" /><rdfs:comment>The Attribute that applies to someone who was a 

Soldier at one time, but is not currently a Soldier.</rdfs:comment></rdf:Description><rdf:Description rdf:ID="ViceChairman"><rdf:type rdf:resource="http://reliant.teknowledge.com/DAML/SUMO.owl#Position" /></rdf:Description><rdf:Description rdf:ID="VicePresident"><rdf:type rdf:resource="http://reliant.teknowledge.com/DAML/SUMO.owl#Position" /></rdf:Description><rdf:Description rdf:ID="VirginIslands"><rdf:type rdf:resource="http://reliant.teknowledge.com/DAML/SUMO.owl#Collection" /><rdfs:comment>A Collection of Islands in the 

West Indies that are dependencies of the UnitedStates and the 

UnitedKingdomOfGreatBritainAndNorthernIreland.</rdfs:comment></rdf:Description><rdf:Description rdf:ID="Virginia"><rdf:type rdf:resource="#AmericanState" /><sumo:meetsSpatially rdf:resource="#WashingtonDC" /><rdfs:comment>A state in the southeastern UnitedStates 

that borders on WashingtonDC.</rdfs:comment></rdf:Description><rdf:Description rdf:ID="Warranty"><sumo:subAttribute rdf:resource="#ServiceContract" /><rdfs:comment>A Contract that states the cirumstances 

under which defects in the product will be corrected for no charge.  

A Warranty is usually limited to a length of time that is specified 

in the Warranty itself.  A Warranty also includes information about 

what is not covered and actions that invalidate the Warranty.</rdfs:comment></rdf:Description><rdf:Description rdf:ID="WarsawPoland"><rdf:type rdf:resource="#EuropeanCity" /><capitalCity rdf:resource="#Poland" /><rdfs:comment>The capital City of Poland.</rdfs:comment></rdf:Description><rdf:Description rdf:ID="Washington"><rdf:type rdf:resource="#AmericanState" /><rdfs:comment>An AmericanState on the PacificOcean.</rdfs:comment></rdf:Description><rdf:Description rdf:ID="WashingtonDC"><rdf:type rdf:resource="#AmericanCity" /><capitalCity rdf:resource="#UnitedStates" /><rdfs:comment>The capital city of the UnitedStates.</rdfs:comment></rdf:Description><rdf:Description rdf:ID="WelfareCapitalism"><rdf:type rdf:resource="#EconomicSystemAttribute" /><sumo:subAttribute rdf:resource="#MixedEconomy" /><sumo:subAttribute rdf:resource="#GovernmentSubsidizedEconomy" /><rdfs:comment>WelfareCapitalism is an Attribute 

describing an economy in which the government provides economic subsidies 

to unemployed or disabled individuals.</rdfs:comment></rdf:Description><rdf:Description rdf:ID="WesternHemisphere"><rdf:type rdf:resource="#Hemisphere" /><rdfs:comment>The half of the Earth that includes North 

and South America.</rdfs:comment></rdf:Description><rdf:Description rdf:ID="WhiteEthnicity"><rdf:type rdf:resource="#RacialEthnicGroup" /><rdfs:comment>A broad ethnic division encompassing 

various European, Hispanic, and Middle Eastern peoples. Also known as 

Caucasian.</rdfs:comment></rdf:Description><rdf:Description rdf:ID="Widowed"><rdf:type rdf:resource="http://reliant.teknowledge.com/DAML/SUMO.owl#SocialRole" /><rdfs:comment>The Attribute that applies to someone who was 

married to someone who has died, and who has not remarried.</rdfs:comment></rdf:Description><rdf:Description rdf:ID="Won"><rdf:type rdf:resource="http://reliant.teknowledge.com/DAML/SUMO.owl#ContestAttribute" /><rdfs:comment>The ContestAttribute that applies to a contestParticipant 

who has won the Contest.</rdfs:comment></rdf:Description><rdf:Description rdf:ID="WorldOcean"><rdf:type rdf:resource="http://reliant.teknowledge.com/DAML/SUMO.owl#SaltWaterArea" /><rdf:type rdf:resource="#BodyOfWater" /><rdfs:comment>The WorldOcean is the collective mass of 

sea water that covers 70% of the surface of PlanetEarth, surrounding 

all of its dry land areas.  Earth's individual Oceans are parts of 

the WorldOcean.</rdfs:comment></rdf:Description><rdf:Description rdf:ID="Wyoming"><rdf:type rdf:resource="#AmericanState" /><rdfs:comment>A large western state in the UnitedStates.</rdfs:comment></rdf:Description></rdf:RDF>