<?xml version="1.0" encoding="utf-8"?><rdf:RDF xmlns:rdfs="http://www.w3.org/2000/01/rdf-schema#" xmlns:rdf="http://www.w3.org/1999/02/22-rdf-syntax-ns#" xmlns:dc="http://purl.org/dc/elements/1.1/" xmlns:dcterms="http://purl.org/dc/terms/" xmlns:foaf="http://xmlns.com/foaf/0.1/" xmlns:owl="http://www.w3.org/2002/07/owl#" xmlns:ex="http://purl.org/net/ns/ex#" xml:base="http://purl.org/net/ns/musicalbaton" xml:lang="en"><owl:Ontology rdf:about=""><dc:title>Musical baton vocabulary</dc:title><dc:description>Vocabulary to describe musical baton entries with FOAF and others, just for fun. Can describe relationship between batons, or a baton and a person.</dc:description><dc:description xml:lang="ja">2005年の5〜6月に流行した遊び「ミュージカルバトン」をFOAFと合わせて表現する語彙。バトンどうしの（送った、受け取ったという）関係や、バトンと人との関係も記述できる。</dc:description><dcterms:created>2005-06-17</dcterms:created><dcterms:modified>2005-06-20</dcterms:modified><owl:versionInfo>Version 0.30</owl:versionInfo><foaf:maker><foaf:Person rdf:about="urn:pin:MK705"><foaf:name xml:lang="ja">神崎正英</foaf:name><foaf:mbox rdf:resource="webmaster@kanzaki.com" /><rdfs:seeAlso rdf:resource="http://www.kanzaki.com/info/webwho.rdf" /></foaf:Person></foaf:maker></owl:Ontology><!-- ==== Class definitions ==== --><rdfs:Class rdf:ID="MusicalBaton"><rdfs:label>Musical Baton</rdfs:label><rdfs:comment>A special kind of baton that represents a person's musical environment on a given period of time, and can be passed or received between baton holders</rdfs:comment><rdfs:comment xml:lang="ja">ある人のある時の音楽環境を表し、人に送ったり受け取ったりできる特殊なバトン</rdfs:comment></rdfs:Class><!-- ==== Property definitions ==== --><rdf:Property rdf:ID="total_volume_of_music_files_on_my_computer"><rdfs:label>Total volume of music files on my computer</rdfs:label><rdfs:comment>Just as the label says. The first question of Musical Baton chain.</rdfs:comment><rdfs:comment xml:lang="ja">バトン保有者が自分のコンピュータに保有している音楽データファイルの量</rdfs:comment></rdf:Property><rdf:Property rdf:ID="song_playing_right_now"><rdfs:label>Song playing right now</rdfs:label><rdfs:comment>The song which the baton holder is/was listening to at that moment. The second question of Musical Baton chain.</rdfs:comment><rdfs:comment xml:lang="ja">バトン保有者がこのバトンを保有している（バトンを記述している）時に聴いている音楽</rdfs:comment></rdf:Property><rdf:Property rdf:ID="last_CD_I_bought"><rdfs:label>The last CD I bought</rdfs:label><rdfs:comment>The newset CD for the baton holder at that moment. The third question of Musical Baton chain.</rdfs:comment><rdfs:comment xml:lang="ja">バトン保有者が（バトンを保有している時点から見て）最近購入したCD</rdfs:comment></rdf:Property><rdf:Property rdf:ID="five_tunes_I_listen_to_a_lot_or_that_mean_a_lot_to_me"><rdfs:label>Five songs(tunes) I listen to a lot, or that mean a lot to me</rdfs:label><rdfs:comment>The list of five songs the baton holder listens to a lot, at that moment. The fourth question of Musical Baton chain. Generally, RDF container (rdf:Bag) is the object.</rdfs:comment><rdfs:comment xml:lang="ja">バトン保有者が（バトンを保有している時点で）よく聴く、あるいは思い入れのある曲5曲のリスト。一般にはrdf:Bagを目的語とする</rdfs:comment></rdf:Property><rdf:Property rdf:ID="description"><rdfs:label>Description</rdfs:label><rdfs:comment>Additional comment/description on the mentioned tune, eivironment, experience etc.</rdfs:comment><rdfs:comment xml:lang="ja">バトンのアイテムとして記述されている曲や環境などについての追記</rdfs:comment></rdf:Property><rdf:Property rdf:ID="hasBaton"><rdfs:label>Has Baton</rdfs:label><rdfs:comment>The subject person holds the object musical baton</rdfs:comment><rdfs:comment xml:lang="ja">主語の人物が目的語のバトンを保有している</rdfs:comment><rdfs:domain rdf:resource="http://xmlns.com/foaf/0.1/Person" /><rdfs:range rdf:resource="#MusicalBaton" /></rdf:Property><rdf:Property rdf:ID="batonHolder"><rdfs:label>Baton Holder</rdfs:label><rdfs:comment>A person who holds the subject baton</rdfs:comment><rdfs:comment xml:lang="ja">主語バトンを保有している人。hasBatonの逆プロパティ</rdfs:comment><rdfs:domain rdf:resource="#MusicalBaton" /><rdfs:range rdf:resource="http://xmlns.com/foaf/0.1/Person" /><owl:inverseOf rdf:resource="#hasBaton" /></rdf:Property><rdf:Property rdf:ID="batonFrom"><rdfs:label>Baton From</rdfs:label><rdfs:comment>relates current baton and previous one</rdfs:comment><rdfs:comment xml:lang="ja">現在のバトンと前の保有者のバトンを結びつける</rdfs:comment><rdfs:domain rdf:resource="#MusicalBaton" /><rdfs:range rdf:resource="#MusicalBaton" /></rdf:Property><rdf:Property rdf:ID="batonTo"><rdfs:label>Baton To</rdfs:label><rdfs:comment>relates current baton and next one. Use 'passedTo' if the next baton does not exist yet.</rdfs:comment><rdfs:comment xml:lang="ja">現在のバトンと次の保有者のバトンを結びつける。次の保有者のバトンが分からない場合は、passToで現在のバトンを次の「人」と結びつける</rdfs:comment><rdfs:domain rdf:resource="#MusicalBaton" /><rdfs:range rdf:resource="#MusicalBaton" /><owl:inverseOf rdf:resource="#batonFrom" /></rdf:Property><rdf:Property rdf:ID="receivedFrom"><rdfs:label>Received From</rdfs:label><rdfs:comment>A person from whom this baton comes. Generally, use 'batonFrom' to express relationship between batons.</rdfs:comment><rdfs:comment xml:lang="ja">バトン保有者にこのバトンを送った人。通常は、batonFromを用いて、人ではなくバトンとバトンを結びつける</rdfs:comment><rdfs:domain rdf:resource="#MusicalBaton" /><rdfs:range rdf:resource="http://xmlns.com/foaf/0.1/Person" /></rdf:Property><rdf:Property rdf:ID="passedTo"><rdfs:label>Passed To</rdfs:label><rdfs:comment>A person to whom the next baton to be passed. Usually five person, i.e. five instances of this property.</rdfs:comment><rdfs:comment xml:lang="ja">バトン保有者がこのバトンを送る人。通常5名（RDFコンテナを使うのではなく、passedToプロパティを5回記述する）。</rdfs:comment><rdfs:domain rdf:resource="#MusicalBaton" /><rdfs:range rdf:resource="http://xmlns.com/foaf/0.1/Person" /></rdf:Property><rdf:Property rdf:ID="batonPage"><rdf:type rdf:resource="http://www.w3.org/2002/07/owl#InverseFunctionalProperty" /><rdfs:label>Baton Page</rdfs:label><rdfs:comment>A webpage where the Musical Baton entries are described for human readers. Works as an IFP of the baton.</rdfs:comment><rdfs:comment xml:lang="ja">ある人のバトンが（HTMLなどの形で）読めるように記述されているページ。バトンのIFPとして機能する</rdfs:comment><rdfs:domain rdf:resource="#MusicalBaton" /><rdfs:range rdf:resource="http://xmlns.com/foaf/0.1/Document" /></rdf:Property><!-- ==== Examples ==== --><ex:Example><dc:description>A simple dirty example. Each baton-question property has mere literal value. Note MusicalBaton has dc:date and mb:batonPage properties to identify it.</dc:description><dc:description xml:lang="ja">シンプルな例。dc:dateとmb:batonPageでバトンの日付やバトン自身を識別する。</dc:description><ex:pfx>mb:</ex:pfx><ex:code><![CDATA[
 <foaf:Person rdf:about="urn:pin:MK705">
  <foaf:nick>masaka</foaf:nick>
  <foaf:mbox rdf:resource="mailto:webmaster&#64;kanzaki.com"/>
  <mb:hasBaton>
   <mb:MusicalBaton>
    <dc:date>2005-06-17</dc:date>
    <mb:batonPage rdf:resource="http://example.org/my_baton_entry"/>
    <mb:total_volume_of_music_files_on_my_computer>242MB</mb:total_volume_of_music_files_on_my_computer>
    <mb:song_playing_right_now>An MD recording of the recital by Tomoko Kawada.</mb:song_playing_right_now>
    <mb:last_CD_I_bought>Mendelssohn: Symphony No.3/No.4, conducted by Sir Roger Norrington, performed by SWR RSO Stuttgart</mb:last_CD_I_bought>
    <mb:five_tunes_I_listen_to_a_lot_or_that_mean_a_lot_to_me>
     <rdf:Bag>
      <rdf:li>Britten: Peter Grimes</rdf:li>
      <rdf:li>バルトーク: 弦楽四重奏曲</rdf:li>
      <rdf:li>ブラームス: ピアノ協奏曲第2番</rdf:li>
      <rdf:li>マーラー: 大地の歌</rdf:li>
      <rdf:li>ニールセン: 交響曲第5番</rdf:li>
     </rdf:Bag>
    </mb:five_tunes_I_listen_to_a_lot_or_that_mean_a_lot_to_me>
   </mb:MusicalBaton>
  <mb:hasBaton>

 </foaf:Person>
 ]]></ex:code></ex:Example><ex:Example><dc:description>A little bit structured example. Note the description of the relationship between batons (and holders) with 'batonFrom' and 'passedTo'.</dc:description><dc:description xml:lang="ja">少し構造化した例。バトンの受領はバトンどうしの関係（batonFrom）で記述しているのに対し、送り先は、その時点では対象となるバトンが分からないので、バトンと送り先の人物との関係（passedTo）を記述している点に注意。</dc:description><ex:pfx>mb:</ex:pfx><ex:code><![CDATA[
 <foaf:Person rdf:about="urn:pin:MK705">
  <foaf:nick>masaka</foaf:nick>
  <foaf:mbox rdf:resource="mailto:webmaster&#64;kanzaki.com"/>
  <mb:hasBaton>
   <mb:MusicalBaton>
    <dc:date>2005-06-17</dc:date>
    <mb:batonPage rdf:resource="http://example.org/my_baton_entry"/>
    <mb:total_volume_of_music_files_on_my_computer>242MB</mb:total_volume_of_music_files_on_my_computer>
    <mb:song_playing_right_now>2004年9月23日の川田知子のバイオリンリサイタル</mb:song_playing_right_now>
    <mb:last_CD_I_bought>
     <mm:Album rdf:about="http://www.kanzaki.com/norrington/discography/93-133">
      <dc:title>Mendelssohn: Symphony No.3/No.4</dc:title>
      <dc:creator>
       <m:Conductor>
        <foaf:name>Sir Roger Norrington</foaf:name>
       </m:Conductor>
      </dc:creator>
      <dc:creator>
       <m:Orchestra>
        <foaf:name>SWR RSO Stuttgart</foaf:name>
       </m:Orchestra>
      </dc:creator>
     </mm:Album>
    </mb:last_CD_I_bought>
    <mb:five_tunes_I_listen_to_a_lot_or_that_mean_a_lot_to_me>
     <rdf:Bag>
      <rdf:li>
       <m:Opera>
        <m:composer rdf:parseType="Resource">
         <foaf:name>Britten</foaf:name>
        </m:composer>
        <dc:title>Peter Grimes</dc:title>
       </m:Opera>
      </rdf:li>
      <rdf:li>
       <m:String_Quartette>
        <m:composer rdf:parseType="Resource">
         <foaf:name>バルトーク</foaf:name>
        </m:composer>
        <dc:title>弦楽四重奏曲</dc:title>
       </m:String_Quartette>
      </rdf:li>
      ...
     </rdf:Bag>
    </mb:five_tunes_I_listen_to_a_lot_or_that_mean_a_lot_to_me>
    <mb:batonFrom>
     <mb:MusicalBaton>
      <mb:batonHolder rdf:parseType="Resource">
       <foaf:nick>foo</foaf:nick>
      </mb:batonHolder>
      <mb:batonPage rdf:resource="http://example.org/foo/baton_entry"/>
     </mb:MusicalBaton>
    </mb:batonFrom>
    <mb:passedTo>
     <foaf:Person>
      <foaf:nick>bar</foaf:nick>
      <foaf:weblog rdf:resource="http://example.org/bar/"/>
     </foaf:Person>
    </mb:passedTo>
   </mb:MusicalBaton>
  <mb:hasBaton>

 </foaf:Person>
 ]]></ex:code></ex:Example><ex:Example><dc:description>Adding rdfs:seeAlso to an instance of MusicalBaton will help robots to collect RDF/XML data.</dc:description><dc:description xml:lang="ja">MusicalBatonのインスタンスにrdfs:seeAlsoでバトンを記述したRDF/XMLファイルのURIを加えると、FOAFと同様、ロボットによる自動収集も可能になる。</dc:description><ex:pfx>mb:</ex:pfx><ex:code><![CDATA[
 <mb:batonFrom>
  <mb:MusicalBaton>
   <mb:batonHolder rdf:parseType="Resource">
    <foaf:nick>foo</foaf:nick>
   </mb:batonHolder>
   <mb:batonPage rdf:resource="http://example.org/foo/baton_entry"/>
   <rdfs:seeAlso rdf:resource="http://example.org/foo/baton.xml"/>
  </mb:MusicalBaton>
 </mb:batonFrom>

 ]]></ex:code></ex:Example></rdf:RDF>