<?xml version="1.0"?><!DOCTYPE rdf:RDF[
   <!ENTITY schema "http://sw.nokia.com/rdfq/schemas/RDFQ-1.0.rdf">
   <!ENTITY rdf    "http://www.w3.org/1999/02/22-rdf-syntax-ns">
   <!ENTITY rdfs   "http://www.w3.org/2000/01/rdf-schema">
   <!ENTITY owl     "http://www.w3.org/2002/07/owl">
   <!ENTITY xsd    "http://www.w3.org/2001/XMLSchema">
   <!ENTITY dc     "http://purl.org/dc/elements/1.1">
   <!ENTITY rss    "http://purl.org/rss/1.0">
   <!ENTITY voc    "http://sw.nokia.com/VOC-1">
   <!ENTITY rdfq   "http://sw.nokia.com/RDFQ-1">
]><rdf:RDF xml:base="&schema;" xmlns:rdf="http://www.w3.org/1999/02/22-rdf-syntax-ns#" xmlns:rdfs="http://www.w3.org/2000/01/rdf-schema#" xmlns:owl="http://www.w3.org/2002/07/owl#" xmlns:xsd="http://www.w3.org/2001/XMLSchema#" xmlns:dc="&dc;/" xmlns:rss="&rss;/" xmlns:voc="&voc;/" xmlns:rdfq="&rdfq;/"><rdf:Description rdf:about="&schema;"><dc:title xmlns:dc="http://purl.org/dc/elements/1.1/">Definition of the RDF Query Vocabulary 1.0</dc:title><dc:creator xmlns:dc="http://purl.org/dc/elements/1.1/">Patrick Stickler (patrick.stickler@nokia.com)</dc:creator><dc:publisher xmlns:dc="http://purl.org/dc/elements/1.1/">Nokia</dc:publisher><dc:format xmlns:dc="http://purl.org/dc/elements/1.1/">application/rdf+xml</dc:format><dc:rights xmlns:dc="http://purl.org/dc/elements/1.1/">
Copyright (C) 2003 Nokia. All rights reserved.

This document may be copied, published, and distributed, without restriction
of any kind, provided it is not modified in any way.

THIS DOCUMENT IS PROVIDED ON AN "AS IS" BASIS, WITHOUT WARRANTY OF ANY KIND, 
EITHER EXPRESSED OR IMPLIED, INCLUDING, WITHOUT LIMITATION, WARRANTIES THAT
THE DOCUMENT IS FREE OF DEFECTS, MERCHANTABLE, FIT FOR A PARTICULAR PURPOSE 
OR NON-INFRINGING. THE ENTIRE RISK AS TO THE QUALITY AND USABILITY OF THIS
DOCUMENT IS WITH YOU. SHOULD THIS DOCUMENT PROVE DEFECTIVE IN ANY RESPECT, 
YOU (NOT NOKIA, ITS LICENSORS OR AFFILIATES OR ANY OTHER CONTRIBUTOR) ASSUME
THE COST OF ANY NECESSARY SERVICING, REPAIR OR CORRECTION.
   </dc:rights></rdf:Description><voc:Vocabulary rdf:about="&rdfq;" xmlns:voc="http://sw.nokia.com/VOC-1/"><dc:title xmlns:dc="http://purl.org/dc/elements/1.1/">RDFQ: RDF Query Vocabulary 1.0</dc:title><rdfs:comment>
RDFQ is an RDF vocabulary and query model for resource and resource
knowledge discovery.

RDFQ is a tool for knowledge discovery, rather than for knowledge
management or knowledge manipulation. Requesting agents submitting
RDFQ queries need not know how knowledge is organized, partitioned,
modeled, stored, accessed, or manipulated internally by the server.

The RDFQ vocabulary provides for the definition of templates which
can be matched against actual resource descriptions. The results of
an RDFQ query is a an RDF graph containing either (a) the concise
bounded descriptions of all resources matched by one or more of the
specified target templates, or (b) a set of variable binding
declarations. Any number of queries can be submitted in the same
request, and any number of templates can be specified as part of
the same query, and the results of all matched templates and queries
specified in the input request are merged together in the results.

A typical RDFQ query corresponds to the request: "Tell me everything
you know about the resources which have the following characteristics..."

In addition to one or more target templates, an input request may
contain any amount of auxilliary knowledge which will be taken into
account when executing the query.  For servers which provide basic
inference support, this is particularly useful for asserting
vocabulary relationships between terms used by the server and terms
used by the requesting agent, to tailor the results to the agent's
needs, or to impose agent-specific assumptions on the evaluation of
the query which are not shared by the server.
   </rdfs:comment><voc:term><rdfs:Class rdf:about="&rdfq;/Query"><rdfs:label>Query</rdfs:label><rdfs:comment>
A query is a collection of one or more templates to be matched
against resource descriptions. It also may specify an RSS 1.0
channel, in terms of which the results are organized.
         </rdfs:comment><voc:partOf rdf:resource="&rdfq;" /><rdfs:isDefinedBy rdf:resource="&schema;" /></rdfs:Class></voc:term><voc:term><rdfs:Class rdf:about="&rdfq;/Target"><rdfs:label>Query Target</rdfs:label><rdfs:comment>
A target is a template to be matched against resource descriptions.

Property values for target resources may be exact, or qualified.

A target property specified with an unqualified rdfq:Value will match any target
property value, but at least one target property value must exist
for the match to succeed.
         </rdfs:comment><voc:partOf rdf:resource="&rdfq;" /><rdfs:isDefinedBy rdf:resource="&schema;" /></rdfs:Class></voc:term><voc:term><rdfs:Class rdf:about="&rdfq;/Graph"><rdfs:label>Target Graph</rdfs:label><rdfs:comment>
A target graph is a template to be matched against named graphs,
if supported by the query service. 

A named graph corresponds to a particular set of RDF statements
(a graph) identified explicitly by a URI and typically qualified
by one or more warrants providing a means to verify the source,
authority, and validity of the graph. 

Comparison of resource target templates is restricted to named graphs
which match a target graph template. 

Property values for target graphs may be exact, or qualified. 
         </rdfs:comment><voc:partOf rdf:resource="&rdfq;" /><rdfs:isDefinedBy rdf:resource="&schema;" /></rdfs:Class></voc:term><voc:term><rdfs:Class rdf:about="&rdfq;/Value"><rdfs:label>Qualified Value</rdfs:label><rdfs:comment>
A qualified value is a target property value which matches
an actual resource value according to one or more operators.

All operators must match in order for the qualified value to
match the resource value.

If no operators are specified, then the qualified value will
match any target property value, but at least one target property
value must exist for the match to succeed. 
         </rdfs:comment><voc:partOf rdf:resource="&rdfq;" /><rdfs:isDefinedBy rdf:resource="&schema;" /></rdfs:Class></voc:term><voc:term><rdfs:Class rdf:about="&rdfq;/OptionalValue"><rdfs:label>Optional Value</rdfs:label><rdfs:comment>
A optional value is a qualified value which need not match,
but if it does, is bound to any specified local identifier
specified with rdfq:id which can be selected using rdfq:select. 
         </rdfs:comment><rdfs:subClassOf rdf:resource="&rdfq;/Value" /><voc:partOf rdf:resource="&rdfq;" /><rdfs:isDefinedBy rdf:resource="&schema;" /></rdfs:Class></voc:term><voc:term><rdfs:Class rdf:about="&rdfq;/Predicate"><rdfs:label>Predicate</rdfs:label><rdfs:comment>
A predicate of an RDF statement.
         </rdfs:comment><voc:partOf rdf:resource="&rdfq;" /><rdfs:isDefinedBy rdf:resource="&schema;" /></rdfs:Class></voc:term><voc:term><rdf:Property rdf:about="&rdfq;/select"><rdfs:label>variable selection</rdfs:label><rdfs:comment>
Specifies a list (set) of variables for which bindings should be 
defined in the results.

If a variable selection list is specified for an rdfq:Query,
the results of that query will be output as variable bindings
rather than outputting the concise bounded descriptions of all
matched targets in the query.
         </rdfs:comment><rdfs:domain rdf:resource="&rdfq;/Query" /><rdfs:range rdf:resource="http://www.w3.org/1999/02/22-rdf-syntax-ns#List" /><voc:partOf rdf:resource="&rdfq;" /><rdfs:isDefinedBy rdf:resource="&schema;" /></rdf:Property></voc:term><voc:term><rdf:Property rdf:about="&rdfq;/graph"><rdfs:label>target graph</rdfs:label><rdfs:comment>
Specifies a target graph to be matched. 

If the specified target is an anonymous target graph
template, the template is matched against all named
graphs in the knowledge base, with the statements of
all matched graphs being included in the scope of the
query. If the target graph is an explicitly named graph,
the statements of that graph are included in the scope
of the query. 
         </rdfs:comment><rdfs:domain rdf:resource="&rdfq;/Query" /><rdfs:range rdf:resource="&rdfq;/Graph" /><voc:partOf rdf:resource="&rdfq;" /><rdfs:isDefinedBy rdf:resource="&schema;" /></rdf:Property></voc:term><voc:term><rdf:Property rdf:about="&rdfq;/target"><rdfs:label>query target</rdfs:label><rdfs:comment>
Specifies a target to be matched.

If the specified target is an anonymous target template, the template
is matched against all resources in the knowledge base. If the target
is a named resource, the description of that resource is included in
the results.
         </rdfs:comment><rdfs:domain rdf:resource="&rdfq;/Query" /><rdfs:range rdf:resource="&rdfq;/Target" /><owl:minCardinality rdf:datatype="http://www.w3.org/2001/XMLSchema#nonNegativeInteger">1</owl:minCardinality><voc:partOf rdf:resource="&rdfq;" /><rdfs:isDefinedBy rdf:resource="&schema;" /></rdf:Property></voc:term><voc:term><rdf:Property rdf:about="&rdfq;/property"><rdfs:label>property</rdfs:label><rdfs:comment>
The super-property of all properties. Every property is inferred
to be a subproperty of this property; thus, this property matches
every property in the graph.

Not to be confused with rdfq:predicate.
         </rdfs:comment><rdfs:domain rdf:resource="&rdfq;/Target" /><rdfs:range rdf:resource="&rdfq;/Value" /><voc:partOf rdf:resource="&rdfq;" /><rdfs:isDefinedBy rdf:resource="&schema;" /></rdf:Property></voc:term><voc:term><rdf:Property rdf:about="&rdfq;/predicate"><rdfs:label>predicate</rdfs:label><rdfs:comment>
The predicate of a particular property:value pair.

Not to be confused with rdfq:property.
         </rdfs:comment><rdfs:domain rdf:resource="&rdfq;/Value" /><rdfs:range rdf:resource="http://www.w3.org/1999/02/22-rdf-syntax-ns#Property" /><voc:partOf rdf:resource="&rdfq;" /><rdfs:isDefinedBy rdf:resource="&schema;" /></rdf:Property></voc:term><voc:term><rdf:Property rdf:about="&rdfq;/ne"><rdfs:label>not equal to</rdfs:label><rdfs:comment>
The resource value is not equal to the specified value.
         </rdfs:comment><rdfs:domain rdf:resource="&rdfq;/Value" /><voc:partOf rdf:resource="&rdfq;" /><rdfs:isDefinedBy rdf:resource="&schema;" /></rdf:Property></voc:term><voc:term><rdf:Property rdf:about="&rdfq;/lt"><rdfs:label>less than</rdfs:label><rdfs:comment>
The resource value is less than the specified value.
         </rdfs:comment><rdfs:domain rdf:resource="&rdfq;/Value" /><voc:partOf rdf:resource="&rdfq;" /><rdfs:isDefinedBy rdf:resource="&schema;" /></rdf:Property></voc:term><voc:term><rdf:Property rdf:about="&rdfq;/gt"><rdfs:label>greater than</rdfs:label><rdfs:comment>
The resource value is greater than the specified value.
         </rdfs:comment><rdfs:domain rdf:resource="&rdfq;/Value" /><voc:partOf rdf:resource="&rdfq;" /><rdfs:isDefinedBy rdf:resource="&schema;" /></rdf:Property></voc:term><voc:term><rdf:Property rdf:about="&rdfq;/le"><rdfs:label>less than or equal to</rdfs:label><rdfs:comment>
The resource value is less than or equal to the specified value.
         </rdfs:comment><rdfs:domain rdf:resource="&rdfq;/Value" /><voc:partOf rdf:resource="&rdfq;" /><rdfs:isDefinedBy rdf:resource="&schema;" /></rdf:Property></voc:term><voc:term><rdf:Property rdf:about="&rdfq;/ge"><rdfs:label>greater than or equal to</rdfs:label><rdfs:comment>
The resource value is greater than or equal to the specified value.
         </rdfs:comment><rdfs:domain rdf:resource="&rdfq;/Value" /><voc:partOf rdf:resource="&rdfq;" /><rdfs:isDefinedBy rdf:resource="&schema;" /></rdf:Property></voc:term><voc:term><rdf:Property rdf:about="&rdfq;/re"><rdfs:label>matches regular expression</rdfs:label><rdfs:comment>
The resource value's string representation matches the specified regular
expression. Applies to literal values only. For typed literals, the string
representation corresponds to the lexical form. For plain literals, the
string representation is the literal itself, irrespective of language
tag.
         </rdfs:comment><rdfs:domain rdf:resource="&rdfq;/Value" /><voc:partOf rdf:resource="&rdfq;" /><rdfs:isDefinedBy rdf:resource="&schema;" /></rdf:Property></voc:term><voc:term><rdf:Property rdf:about="&rdfq;/lang"><rdfs:label>language tag</rdfs:label><rdfs:comment>
The resource value's language tag matches the specified language tag. Applies
to plain literal values only. Comparison of language tags is case insensitive.
         </rdfs:comment><rdfs:domain rdf:resource="&rdfq;/Value" /><voc:partOf rdf:resource="&rdfq;" /><rdfs:isDefinedBy rdf:resource="&schema;" /></rdf:Property></voc:term><voc:term><rdf:Description rdf:about="&rdfq;/id"><rdfs:label>local identifier</rdfs:label><rdfs:comment>
A local identifier (variable) associated with a node within a particular
target template.

Local identifiers are used both for equating two or more otherwise unspecified
values (e.g. two property values are the same, no matter what those values are)
as well as binding variables for result set output as specified by an rdfq:select
variable list.
         </rdfs:comment><rdfs:range rdf:resource="http://www.w3.org/2000/01/rdf-schema#Literal" /><voc:partOf rdf:resource="&rdfq;" /><rdfs:isDefinedBy rdf:resource="&schema;" /></rdf:Description></voc:term><voc:term><rdf:Description rdf:about="&rdfq;/one-hour-ago"><rdfs:label>one hour ago</rdfs:label><rdfs:comment>
Denotes the date and time exactly one hour ago from the present.
         </rdfs:comment><voc:partOf rdf:resource="&rdfq;" /><rdfs:isDefinedBy rdf:resource="&schema;" /></rdf:Description></voc:term><voc:term><rdf:Description rdf:about="&rdfq;/one-day-ago"><rdfs:label>one day ago</rdfs:label><rdfs:comment>
Denotes the date and time exactly one day ago from the present.
         </rdfs:comment><voc:partOf rdf:resource="&rdfq;" /><rdfs:isDefinedBy rdf:resource="&schema;" /></rdf:Description></voc:term><voc:term><rdf:Description rdf:about="&rdfq;/one-week-ago"><rdfs:label>one week ago</rdfs:label><rdfs:comment>
Denotes the date and time exactly one week ago from the present.
         </rdfs:comment><voc:partOf rdf:resource="&rdfq;" /><rdfs:isDefinedBy rdf:resource="&schema;" /></rdf:Description></voc:term><voc:term><rdf:Description rdf:about="&rdfq;/one-month-ago"><rdfs:label>one month ago</rdfs:label><rdfs:comment>
Denotes the date and time exactly one month ago from the present.
         </rdfs:comment><voc:partOf rdf:resource="&rdfq;" /><rdfs:isDefinedBy rdf:resource="&schema;" /></rdf:Description></voc:term><voc:term><rdf:Description rdf:about="&rdfq;/one-year-ago"><rdfs:label>one year ago</rdfs:label><rdfs:comment>
Denotes the date and time exactly one year ago from the present.
         </rdfs:comment><voc:partOf rdf:resource="&rdfq;" /><rdfs:isDefinedBy rdf:resource="&schema;" /></rdf:Description></voc:term><voc:term><rdf:Description rdf:about="&rdfq;/null"><rdfs:label>no defined value</rdfs:label><rdfs:comment>
Denotes the absence of any defined value.
         </rdfs:comment><voc:partOf rdf:resource="&rdfq;" /><rdfs:isDefinedBy rdf:resource="&schema;" /></rdf:Description></voc:term><rdfs:isDefinedBy rdf:resource="&schema;" /></voc:Vocabulary></rdf:RDF>