<?xml version="1.0"?><!-- This is an  RDF Schema for RooDolF, a
representation of a Google Result Set in RDF written by
  Alexander Loeser, aloeser@cs.tu-berlin.de --><rdf:RDF xmlns="http://nutria.cs.tu-berlin.de/roodolf/rdfs#" xmlns:rdf="http://www.w3.org/1999/02/22-rdf-syntax-ns#" xmlns:rdfs="http://www.w3.org/2000/01/rdf-schema#" xmlns:xsd="http://www.w3.org/1999/XMLSchema-datatypes#"><rdfs:Class rdf:about="http://nutria.cs.tu-berlin.de/roodolf/rdfs#GoogleSearchResult"><rdfs:comment>Each time you issue a search request to the Google service,
        a response is returned back to you. A GoogleSearchResult is such a response.
        GoogleSearchResult encapsulates the complete results returned by the Google Web APIs search call.
        (Taken from the Google Api Description, Copyright by Google INC.)
      </rdfs:comment></rdfs:Class><rdfs:Class rdf:about="http://nutria.cs.tu-berlin.de/roodolf/rdfs#Results"><rdfs:comment>Includes a sequence of result elements for the query. The
        element order is done by Google.
      </rdfs:comment><rdfs:domain rdfs:resource="rdf:Seq" /></rdfs:Class><rdfs:Class rdf:about="http://nutria.cs.tu-berlin.de/roodolf/rdfs#DirectoryCategories"><rdfs:comment>Includes a bag of directory categories for
        the query. The elements are not ordered and are
        recommended by Google.
      </rdfs:comment><rdfs:domain rdfs:resource="rdf:Bag" /></rdfs:Class><rdfs:Class rdf:about="http://nutria.cs.tu-berlin.de/roodolf/rdfs#ResultElement"><rdfs:comment>ResultElement contains an individual search result component
        of a Result.
        (Taken from the Google Api Description, Copyright by Google INC.)
        </rdfs:comment></rdfs:Class><rdfs:Class rdf:about="http://nutria.cs.tu-berlin.de/roodolf/rdfs#DirectoryCategoryElement"><rdfs:comment>DirectoryCategory encapsulates the directory category portion of GoogleSearchResult.
        (Taken from the Google Api Description, Copyright by Google INC.)
        </rdfs:comment></rdfs:Class><!-- RooDoolF:URL=dc.identifier
    <rdfs:Class rdf:about="http://nutria.cs.tu-berlin.de/roodolf/rdfs#URL">
        <rdfs:comment>URL of the ResultElement.
      </rdfs:comment>
      <rdfs:domain rdfs:resource="http://nutria.cs.tu-berlin.de/roodolf/rdfs#ResultElement"/>
      <rdfs:range rdf:resource="xsd:uri"/>
    </rdfs:Class>
--><rdfs:Class rdf:about="http://nutria.cs.tu-berlin.de/roodolf/rdfs#relatedInformationPresentURI"><rdfs:comment>If #relatedInformationPresent is true it shows the RooDolF Query URI for related
        Links.
        </rdfs:comment><rdfs:domain rdf:resource="http://nutria.cs.tu-berlin.de/roodolf/rdfs#ResultElement" /><rdfs:range rdf:resource="xsd:uriReference" /></rdfs:Class><rdf:Property rdf:about="http://nutria.cs.tu-berlin.de/roodolf/rdfs#documentFiltering"><rdfs:comment>A Boolean value indicating whether filtering was performed on the search
        results. This will be "true" only if (a) you requested filtering and (b) filtering actually occurred
        (Taken from the Google Api Description, Copyright by Google INC.)
        </rdfs:comment><rdfs:domain rdf:resource="http://nutria.cs.tu-berlin.de/roodolf/rdfs#GoogleSearchResult" /><rdfs:label>documentFiltering</rdfs:label><rdfs:range rdf:resource="xsd:boolean" /></rdf:Property><rdf:Property rdf:about="http://nutria.cs.tu-berlin.de/roodolf/rdfs#estimatedTotalResultCount"><rdfs:comment>The estimated total number of results that exist for the query.
        Note: The estimated number may be either higher or lower than the actual number of results that exist.
        (Taken from the Google Api Description, Copyright by Google INC.)
        </rdfs:comment><rdfs:domain rdf:resource="http://nutria.cs.tu-berlin.de/roodolf/rdfs#GoogleSearchResult" /><rdfs:label>estimatedTotalResultCount</rdfs:label><rdfs:range rdf:resource="xsd:nonNegativeInteger" /></rdf:Property><rdf:Property rdf:about="http://nutria.cs.tu-berlin.de/roodolf/rdfs#estimateIsExact"><rdfs:comment>A Boolean value indicating that the estimate is actually the exact value.
        (Taken from the Google Api Description, Copyright by Google INC.)
        </rdfs:comment><rdfs:domain rdf:resource="http://nutria.cs.tu-berlin.de/roodolf/rdfs#GoogleSearchResult" /><rdfs:label>estimateIsExact</rdfs:label><rdfs:range rdf:resource="xsd:boolean" /></rdf:Property><rdf:Property rdf:about="http://nutria.cs.tu-berlin.de/roodolf/rdfs#searchQuery"><rdfs:comment>This is the value of 'q' for the search request.
        (Taken from the Google Api Description, Copyright by Google INC.)
        </rdfs:comment><rdfs:domain rdf:resource="http://nutria.cs.tu-berlin.de/roodolf/rdfs#GoogleSearchResult" /><rdfs:label>searchQuery</rdfs:label><rdfs:range rdf:resource="xsd:uriReference" /></rdf:Property><rdf:Property rdf:about="http://nutria.cs.tu-berlin.de/roodolf/rdfs#startIndex"><rdfs:comment>Indicates the index (1-based) of the first search result in a GoogleSearchResult.
        (Taken from the Google Api Description, Copyright by Google INC.)
        </rdfs:comment><rdfs:domain rdf:resource="http://nutria.cs.tu-berlin.de/roodolf/rdfs#GoogleSearchResult" /><rdfs:label>startIndex</rdfs:label><rdfs:range rdf:resource="xsd:nonNegativeInteger" /></rdf:Property><rdf:Property rdf:about="http://nutria.cs.tu-berlin.de/roodolf/rdfs#endIndex"><rdfs:comment>Indicates the index (1-based) of the first search result in GoogleSearchResult.
        (Taken from the Google Api Description, Copyright by Google INC.)
        </rdfs:comment><rdfs:domain rdf:resource="http://nutria.cs.tu-berlin.de/roodolf/rdfs#GoogleSearchResult" /><rdfs:label>endIndex</rdfs:label><rdfs:range rdf:resource="xsd:nonNegativeInteger" /></rdf:Property><rdf:Property rdf:about="http://nutria.cs.tu-berlin.de/roodolf/rdfs#searchTips"><rdfs:comment>A text string intended for display to the end user. It provides instructive
        suggestions on how to use Google.
        (Taken from the Google Api Description, Copyright by Google INC.)
        </rdfs:comment><rdfs:domain rdf:resource="http://nutria.cs.tu-berlin.de/roodolf/rdfs#GoogleSearchResult" /><rdfs:label>searchTips</rdfs:label><rdfs:range rdf:resource="xsd:string" /></rdf:Property><rdf:Property rdf:about="http://nutria.cs.tu-berlin.de/roodolf/rdfs#searchTime"><rdfs:comment>Text, floating-point number indicating the total server time to
        return the search results, measured in seconds.
        (Taken from the Google Api Description, Copyright by Google INC.)
        </rdfs:comment><rdfs:domain rdf:resource="http://nutria.cs.tu-berlin.de/roodolf/rdfs#GoogleSearchResult" /><rdfs:label>searchTips</rdfs:label><rdfs:range rdf:resource="xsd:string" /></rdf:Property><rdf:Property rdf:about="http://nutria.cs.tu-berlin.de/roodolf/rdfs#cachedSize"><rdfs:comment>Text (Integer + "k"). Indicates that a cached version of the 'URL'
        is available; size is indicated in kilobytes.
        (Taken from the Google Api Description, Copyright by Google INC.)
        </rdfs:comment><rdfs:domain rdf:resource="http://nutria.cs.tu-berlin.de/roodolf/rdfs#ResultElement" /><rdfs:label>cachedSize</rdfs:label><rdfs:range rdf:resource="xsd:string" /></rdf:Property><rdf:Property rdf:about="http://nutria.cs.tu-berlin.de/roodolf/rdfs#directoryCategory"><rdfs:comment>Returns the ODP directory name for the current ODP category
        (Taken from the Google Api Description, Copyright by Google INC.)
        </rdfs:comment><rdfs:domain rdf:resource="http://nutria.cs.tu-berlin.de/roodolf/rdfs#ResultElement" /><rdfs:label>directoryCategory</rdfs:label><rdfs:range rdf:resource="xsd:string" /></rdf:Property><rdf:Property rdf:about="http://nutria.cs.tu-berlin.de/roodolf/rdfs#directoryTitle"><rdfs:comment>If the URL for this resultElement is contained in the ODP directory,
        the title that appears in the directory appears here as a text string. Note that the
        directoryTitle may be different from the URL's title.
        (Taken from the Google Api Description, Copyright by Google INC.)
        </rdfs:comment><rdfs:domain rdf:resource="http://nutria.cs.tu-berlin.de/roodolf/rdfs#ResultElement" /><rdfs:label>directoryTitle</rdfs:label><rdfs:range rdf:resource="xsd:string" /></rdf:Property><rdf:Property rdf:about="http://nutria.cs.tu-berlin.de/roodolf/rdfs#hostName"><rdfs:comment>When filtering occurs, a maximum of two results from any given host
        is returned. When this occurs, the second resultElement that comes from that host
        contains the host name in this parameter.
        (Taken from the Google Api Description, Copyright by Google INC.)
        </rdfs:comment><rdfs:domain rdf:resource="http://nutria.cs.tu-berlin.de/roodolf/rdfs#ResultElement" /><rdfs:label>hostName</rdfs:label><rdfs:range rdf:resource="xsd:uriReference" /></rdf:Property><rdf:Property rdf:about="http://nutria.cs.tu-berlin.de/roodolf/rdfs#relatedInformationPresent"><rdfs:comment>Boolean indicating that the "related:" query term is supported for the URL
        of the ResultSet.
        (Taken from the Google Api Description, Copyright by Google INC.)
        </rdfs:comment><rdfs:domain rdf:resource="http://nutria.cs.tu-berlin.de/roodolf/rdfs#ResultElement" /><rdfs:label>relatedInformationPresent</rdfs:label><rdfs:range rdf:resource="xsd:boolean" /></rdf:Property><!-- RooDoolF:snippet=dc:description
   <rdf:Property rdf:about="http://nutria.cs.tu-berlin.de/roodolf/rdfs#snippet">
        <rdfs:comment>A snippet which shows the query in context on the URL where it appears.
        This is formatted HTML and usually includes 'B' tags within it. Note that the query
        term does not always appear in the snippet. Note: Query terms will be in highlighted in
        bold in the results, and line breaks will be included for proper text wrapping.
        (returned as HTML)
        (Taken from the Google Api Description, Copyright by Google INC.)
        </rdfs:comment>
        <rdfs:domain rdf:resource="http://nutria.cs.tu-berlin.de/roodolf/rdfs#ResultElement"/>
        <rdfs:label>snippet</rdfs:label>
        <rdfs:range rdf:resource="xsd:string"/>
    </rdf:Property>
--><!-- RooDoolF:summary=dc:subject
   <rdf:Property rdf:about="http://nutria.cs.tu-berlin.de/roodolf/rdfs#summary">
        <rdfs:comment>If the search result has a listing in the ODP directory, the
        ODP summary appears here as a text string. (returned as HTML)
        (Taken from the Google Api Description, Copyright by Google INC.)
        </rdfs:comment>
        <rdfs:domain rdf:resource="http://nutria.cs.tu-berlin.de/roodolf/rdfs#ResultElement"/>
        <rdfs:label>summary</rdfs:label>
        <rdfs:range rdf:resource="xsd:string"/>
    </rdf:Property>
--><!-- RooDoolF:title=dc:title
   <rdf:Property rdf:about="http://nutria.cs.tu-berlin.de/roodolf/rdfs#title">
        <rdfs:comment>The title of the search result, returned as HTML
        (Taken from the Google Api Description, Copyright by Google INC.)
        </rdfs:comment>
        <rdfs:domain rdf:resource="http://nutria.cs.tu-berlin.de/roodolf/rdfs#ResultElement"/>
        <rdfs:label>title</rdfs:label>
        <rdfs:range rdf:resource="xsd:string"/>
    </rdf:Property>
--><rdf:Property rdf:about="http://nutria.cs.tu-berlin.de/roodolf/rdfs#fullViewableName"><rdfs:comment>Text, containing the ODP directory name for the current ODP category
        (Taken from the Google Api Description, Copyright by Google INC.)
        </rdfs:comment><rdfs:domain rdf:resource="http://nutria.cs.tu-berlin.de/roodolf/rdfs#DirectoryCategory" /><rdfs:label>fullViewableName</rdfs:label><rdfs:range rdf:resource="xsd:string" /></rdf:Property><rdf:Property rdf:about="http://nutria.cs.tu-berlin.de/roodolf/rdfs#specialEncoding"><rdfs:comment>Specifies the encoding scheme of the directory information.
        (Taken from the Google Api Description, Copyright by Google INC.)
        </rdfs:comment><rdfs:domain rdf:resource="http://nutria.cs.tu-berlin.de/roodolf/rdfs#DirectoryCategory" /><rdfs:label>specialEncoding</rdfs:label><rdfs:range rdf:resource="xsd:string" /></rdf:Property></rdf:RDF>