<?xml version="1.0"?>

<!DOCTYPE rdf:RDF [
   <!ENTITY schema "http://sw.nokia.com/schemas/general/VOC-1.0.rdf">
   <!ENTITY rdf    "http://www.w3.org/1999/02/22-rdf-syntax-ns">
   <!ENTITY rdfs   "http://www.w3.org/2000/01/rdf-schema">
   <!ENTITY owl    "http://www.w3.org/2002/07/owl">
   <!ENTITY dc     "http://purl.org/dc/elements/1.1">
   <!ENTITY voc    "http://sw.nokia.com/VOC-1">
]>

<rdf:RDF
   xml:base   ="&schema;"
   xmlns:rdf  ="&rdf;#"
   xmlns:rdfs ="&rdfs;#"
   xmlns:owl  ="&owl;#"
   xmlns:dc   ="&dc;/"
   xmlns:voc  ="&voc;/"
>

<rdf:Description rdf:about="&schema;">
   <dc:title>Definition of the Vocabulary for Vocabulary Definitions 1.0</dc:title>
   <dc:creator>Patrick Stickler (patrick.stickler@nokia.com)</dc:creator>
   <dc:publisher>Nokia</dc:publisher>
   <dc:format>application/rdf+xml</dc:format>
   <dc:rights>
Copyright (C) 2000-2003 Nokia. All rights reserved.

This document may be copied, published, and distributed, without restriction
of any kind, provided it is not modified in any way.

THIS DOCUMENT IS PROVIDED ON AN "AS IS" BASIS, WITHOUT WARRANTY OF ANY KIND, 
EITHER EXPRESSED OR IMPLIED, INCLUDING, WITHOUT LIMITATION, WARRANTIES THAT
THE DOCUMENT IS FREE OF DEFECTS, MERCHANTABLE, FIT FOR A PARTICULAR PURPOSE 
OR NON-INFRINGING. THE ENTIRE RISK AS TO THE QUALITY AND USABILITY OF THIS
DOCUMENT IS WITH YOU. SHOULD THIS DOCUMENT PROVE DEFECTIVE IN ANY RESPECT, 
YOU (NOT NOKIA, ITS LICENSORS OR AFFILIATES OR ANY OTHER CONTRIBUTOR) ASSUME
THE COST OF ANY NECESSARY SERVICING, REPAIR OR CORRECTION.
   </dc:rights>
</rdf:Description>

<voc:Vocabulary rdf:about="&voc;">

   <voc:term>
      <rdfs:Class rdf:about="&voc;/Vocabulary">
         <rdfs:label>Vocabulary</rdfs:label>
         <rdfs:comment>
A vocabulary is a set of terms.
         </rdfs:comment>
         <rdfs:subClassOf rdf:resource="&rdfs;#Container"/>
         <voc:partOf rdf:resource="&voc;"/>
         <rdfs:isDefinedBy rdf:resource="&schema;"/>
      </rdfs:Class>
   </voc:term>

   <voc:term>
      <rdfs:Class rdf:about="&voc;/Term">
         <rdfs:label>Vocabulary Term</rdfs:label>
         <rdfs:comment>
A vocbulary term is a member of a vocabulary.
         </rdfs:comment>
         <voc:partOf rdf:resource="&voc;"/>
         <rdfs:isDefinedBy rdf:resource="&schema;"/>
      </rdfs:Class>
   </voc:term>

   <voc:term>
      <rdfs:Class rdf:about="&voc;/Deprecated">
         <rdfs:label>Deprecated</rdfs:label>
         <rdfs:comment>
Should no longer be used for new resource descriptions or applications.
         </rdfs:comment>
         <voc:partOf rdf:resource="&voc;"/>
         <rdfs:isDefinedBy rdf:resource="&schema;"/>
      </rdfs:Class>
   </voc:term>

   <voc:term>
      <rdf:Property rdf:about="&voc;/vocabulary">
         <rdfs:label>vocabulary</rdfs:label>
         <rdfs:comment>
Relates a vocabulary to a resource. If the subject is also a
vocabulary, then terms belonging to the object vocabulary are
considered to also belong to the subject vocabulary. If the
subject is an RDF Class, then the object vocabulary is
taken as relevant for describing instances of that class.
         </rdfs:comment>
         <rdf:type rdf:resource="&rdfs;#ContainerMembershipProperty"/>
         <rdfs:subPropertyOf rdf:resource="&rdfs;#member"/>
         <rdfs:range  rdf:resource="&voc;/Vocabulary"/>
         <voc:partOf rdf:resource="&voc;"/>
         <rdfs:isDefinedBy rdf:resource="&schema;"/>
      </rdf:Property>
   </voc:term>

   <voc:term>
      <rdf:Property rdf:about="&voc;/term">
         <rdfs:label>term</rdfs:label>
         <rdfs:comment>
A term belonging to a vocabulary.
         </rdfs:comment>
         <rdf:type rdf:resource="&rdfs;#ContainerMembershipProperty"/>
         <rdfs:subPropertyOf rdf:resource="&rdfs;#member"/>
         <rdfs:domain rdf:resource="&voc;/Vocabulary"/>
         <rdfs:range  rdf:resource="&voc;/Term"/>
         <voc:partOf rdf:resource="&voc;"/>
         <rdfs:isDefinedBy rdf:resource="&schema;"/>
      </rdf:Property>
   </voc:term>

   <voc:term>
      <rdf:Property rdf:about="&voc;/partOf">
         <rdfs:label>part of</rdfs:label>
         <rdfs:comment>
A vocabulary to which a term or subvocabulary belongs.
         </rdfs:comment>
         <rdfs:range  rdf:resource="&voc;/Vocabulary"/>
         <owl:inverseOf rdf:resource="&rdfs;#member"/>
         <voc:partOf rdf:resource="&voc;"/>
         <rdfs:isDefinedBy rdf:resource="&schema;"/>
      </rdf:Property>
   </voc:term>

   <voc:term>
      <rdf:Property rdf:about="&voc;/specializationOf">
         <rdfs:label>specialization of</rdfs:label>
         <rdfs:comment>
The subject term is a specialization of the object term.
         </rdfs:comment>
         <rdfs:domain rdf:resource="&voc;/Term"/>
         <rdfs:range  rdf:resource="&voc;/Term"/>
         <owl:inverseOf rdf:resource="&voc;/generalizationOf"/>
         <voc:partOf rdf:resource="&voc;"/>
         <rdfs:isDefinedBy rdf:resource="&schema;"/>
      </rdf:Property>
   </voc:term>

   <voc:term>
      <rdf:Property rdf:about="&voc;/generalizationOf">
         <rdfs:label>generalization of</rdfs:label>
         <rdfs:comment>
The subject term is a generalization of the object term.
         </rdfs:comment>
         <rdfs:domain rdf:resource="&voc;/Term"/>
         <rdfs:range  rdf:resource="&voc;/Term"/>
         <owl:inverseOf rdf:resource="&voc;/specializationOf"/>
         <voc:partOf rdf:resource="&voc;"/>
         <rdfs:isDefinedBy rdf:resource="&schema;"/>
      </rdf:Property>
   </voc:term>

   <rdfs:isDefinedBy rdf:resource="&schema;"/>
</voc:Vocabulary>

</rdf:RDF>
