<?xml version="1.0" encoding="UTF-8"?>
<rdf:RDF xmlns:rdf="http://www.w3.org/1999/02/22-rdf-syntax-ns#"
  xmlns:owl="http://www.w3.org/2002/07/owl#"
  xmlns:dc="http://purl.org/dc/elements/1.1/"
  xmlns:vann="http://purl.org/vocab/vann/"
  xmlns:foaf="http://xmlns.com/foaf/0.1/"
  xmlns:rdfs="http://www.w3.org/2000/01/rdf-schema#">

  <owl:Ontology rdf:about="http://vocab.sindice.net/dataset">
    <dc:title>Sindice dataset vocabulary</dc:title>
    <dc:modified rdf:datatype="http://www.w3.org/2001/XMLSchema#date">2012-05-26</dc:modified>
    <vann:preferredNamespaceUri>https://vocab.sindice.net/dataset/1.0/</vann:preferredNamespaceUri>
    <vann:preferredNamespacePrefix>dataset</vann:preferredNamespacePrefix>
    <foaf:page rdf:resource="http://vocab.sindice.net/dataset.html"/>
    <dc:creator rdf:resource="http://vocab.sindice.net/dataset#gabvul"/>
  </owl:Ontology>

  <foaf:Person rdf:about="http://vocab.sindice.net/dataset#gabvul">
    <foaf:name>Gabriela Vulcu</foaf:name>
    <foaf:homepage></foaf:homepage>
  </foaf:Person>

  <rdf:Property rdf:about="https://vocab.sindice.net/dataset/1.0/name">
    <rdf:type rdf:resource="http://www.w3.org/2002/07/owl#DatatypeProperty"/>
    <rdfs:isDefinedBy rdf:resource="http://vocab.sindice.net/dataset"/>
    <rdfs:label>Name</rdfs:label>
    <rdfs:comment>Property used to describe the dataset name as string.</rdfs:comment>
    <rdfs:range rdf:resource="http://www.w3.org/2001/XMLSchema#string"/>
  </rdf:Property>

  <rdf:Property rdf:about="https://vocab.sindice.net/dataset/1.0/type">
    <rdfs:isDefinedBy rdf:resource="http://vocab.sindice.net/dataset"/>
    <rdfs:label>Type</rdfs:label>
    <rdfs:comment>Property used to describe the dataset type. At the moment we distinguish between two dataset types: dataset:type/dump and dataset:type/website.</rdfs:comment>
  </rdf:Property>

  <rdf:Property rdf:about="https://vocab.sindice.net/dataset/1.0/uri">
    <rdfs:isDefinedBy rdf:resource="http://vocab.sindice.net/dataset"/>
    <rdfs:label>Uri</rdfs:label>
    <rdfs:comment>Property used to uniquely identify a dataset.</rdfs:comment>
  </rdf:Property>

  <rdf:Property rdf:about="https://vocab.sindice.net/dataset/1.0/domain-uri">
    <rdfs:isDefinedBy rdf:resource="http://vocab.sindice.net/dataset"/>
    <rdfs:label>domain-uri</rdfs:label>
    <rdfs:comment>Property used to define the dataset domain URI.</rdfs:comment>
  </rdf:Property>

  <rdf:Property rdf:about="https://vocab.sindice.net/dataset/1.0/domain">
    <rdf:type rdf:resource="http://www.w3.org/2002/07/owl#DatatypeProperty"/>
    <rdfs:isDefinedBy rdf:resource="http://vocab.sindice.net/dataset"/>
    <rdfs:label>domain</rdfs:label>
    <rdfs:comment>Property used to describe the dataset domain as string.</rdfs:comment>
    <rdfs:range rdf:resource="http://www.w3.org/2001/XMLSchema#string"/>
  </rdf:Property>

  <rdf:Property rdf:about="https://vocab.sindice.net/dataset/1.0/second-level-domain-uri">
    <rdfs:isDefinedBy rdf:resource="http://vocab.sindice.net/dataset"/>
    <rdfs:label>Second-level-domain-uri</rdfs:label>
    <rdfs:comment>Property used to define define the dataset secodn-level-domain URI.</rdfs:comment>
  </rdf:Property>

  <rdf:Property rdf:about="https://vocab.sindice.net/dataset/1.0/second-level-domain">
    <rdfs:isDefinedBy rdf:resource="http://vocab.sindice.net/dataset"/>
    <rdfs:label>second-level-domain</rdfs:label>
    <rdfs:comment>Property used to describe the dataset secodn level domain as string.</rdfs:comment>
  </rdf:Property>

  <rdf:Property rdf:about="https://vocab.sindice.net/dataset/1.0/snapshot">
    <rdf:type rdf:resource="http://www.w3.org/2002/07/owl#DatatypeProperty"/>
    <rdfs:isDefinedBy rdf:resource="http://vocab.sindice.net/dataset"/>
    <rdfs:label>Snapshot</rdfs:label>
    <rdfs:comment>Property used to describe the dataset version that distinguishes between different results of the dataset processing procedure. </rdfs:comment>
    <rdfs:range rdf:resource="http://www.w3.org/2001/XMLSchema#string"/>
  </rdf:Property>

  <rdf:Property rdf:about="https://vocab.sindice.net/dataset/1.0/void">
    <rdfs:isDefinedBy rdf:resource="http://vocab.sindice.net/dataset"/>
    <rdfs:label>void</rdfs:label>
    <rdfs:comment>Property used to describe the URI of the graph containing the datasetâ€™s VOID meta-data.</rdfs:comment>
  </rdf:Property>

  <rdf:Property rdf:about="https://vocab.sindice.net/dataset/1.0/dataset">
    <rdfs:isDefinedBy rdf:resource="http://vocab.sindice.net/dataset"/>
    <rdfs:label>dataset</rdfs:label>
    <rdfs:comment>Property used to identify the dataset URI to which an RDF graph belongs to.</rdfs:comment>
  </rdf:Property>

  <rdf:Property rdf:about="https://vocab.sindice.net/dataset/1.0/dataspace">
    <rdfs:isDefinedBy rdf:resource="http://vocab.sindice.net/dataset"/>
    <rdfs:label>dataspace</rdfs:label>
    <rdfs:comment>Property used to describe the URI prefix of the current dataspace. </rdfs:comment>
  </rdf:Property>

</rdf:RDF>