<?xml version="1.0"?>
<rdf:RDF xml:lang="en"
    xmlns:rdf ="http://www.w3.org/1999/02/22-rdf-syntax-ns#"
    xmlns:rdfs="http://www.w3.org/2000/01/rdf-schema#">

<rdfs:Class rdf:about="http://www.eyrie.org/~zednenem/2002/wail/Place">
    <rdfs:isDefinedBy rdf:resource="http://www.eyrie.org/~zednenem/2002/wail/wail.rdf"/>
    <rdfs:label>Place</rdfs:label>
    <rdfs:comment>
        Anything which can be considered a place, such as your house or Europe
    </rdfs:comment>
</rdfs:Class>

<rdfs:Class rdf:about="http://www.eyrie.org/~zednenem/2002/wail/Country">
    <rdfs:isDefinedBy rdf:resource="http://www.eyrie.org/~zednenem/2002/wail/wail.rdf"/>
    <rdfs:label>Country</rdfs:label>
    <rdfs:comment>
        An internationally-recognized country; anything which has an ISO country code
    </rdfs:comment>
    <rdfs:subClassOf rdf:resource="http://www.eyrie.org/~zednenem/2002/wail/Place"/>
</rdfs:Class>

<rdfs:Class rdf:about="http://www.eyrie.org/~zednenem/2002/wail/Region">
    <rdfs:isDefinedBy rdf:resource="http://www.eyrie.org/~zednenem/2002/wail/wail.rdf"/>
    <rdfs:label>Region</rdfs:label>
    <rdfs:comment>
        A subdivision of a Country with a well-known name and area
    </rdfs:comment>
    <rdfs:subClassOf rdf:resource="http://www.eyrie.org/~zednenem/2002/wail/Place"/>
</rdfs:Class>

<rdfs:Class rdf:about="http://www.eyrie.org/~zednenem/2002/wail/State">
    <rdfs:isDefinedBy rdf:resource="http://www.eyrie.org/~zednenem/2002/wail/wail.rdf"/>
    <rdfs:label>State</rdfs:label>
    <rdfs:comment>
        A type of Region used in federal systems such as the United States
    </rdfs:comment>
    <rdfs:subClassOf rdf:resource="http://www.eyrie.org/~zednenem/2002/wail/Region"/>
</rdfs:Class>

<rdfs:Class rdf:about="http://www.eyrie.org/~zednenem/2002/wail/Province">
    <rdfs:isDefinedBy rdf:resource="http://www.eyrie.org/~zednenem/2002/wail/wail.rdf"/>
    <rdfs:label>Province</rdfs:label>
    <rdfs:comment>
        A type of Region used in federal systems such as Canada
    </rdfs:comment>
    <rdfs:subClassOf rdf:resource="http://www.eyrie.org/~zednenem/2002/wail/Region"/>
</rdfs:Class>

<rdfs:Class rdf:about="http://www.eyrie.org/~zednenem/2002/wail/County">
    <rdfs:isDefinedBy rdf:resource="http://www.eyrie.org/~zednenem/2002/wail/wail.rdf"/>
    <rdfs:label>County</rdfs:label>
    <rdfs:comment>
        A type of Region; usually a subdivision of a larger Region
        containing several Cities
    </rdfs:comment>
    <rdfs:subClassOf rdf:resource="http://www.eyrie.org/~zednenem/2002/wail/Region"/>
</rdfs:Class>

<rdfs:Class rdf:about="http://www.eyrie.org/~zednenem/2002/wail/City">
    <rdfs:isDefinedBy rdf:resource="http://www.eyrie.org/~zednenem/2002/wail/wail.rdf"/>
    <rdfs:label>City</rdfs:label>
    <rdfs:comment>
        A subdivision of Region corresponding to a center of population, such
        as a city, town, village, etc. Does not necessarily correspond to an
        actual municipal government.
    </rdfs:comment>
    <rdfs:subClassOf rdf:resource="http://www.eyrie.org/~zednenem/2002/wail/Place"/>
</rdfs:Class>

<rdfs:Class rdf:about="http://www.eyrie.org/~zednenem/2002/wail/Neighborhood">
    <rdfs:isDefinedBy rdf:resource="http://www.eyrie.org/~zednenem/2002/wail/wail.rdf"/>
    <rdfs:label>Neighborhood</rdfs:label>
    <rdfs:comment>
        A subdivision of a City
    </rdfs:comment>
    <rdfs:subClassOf rdf:resource="http://www.eyrie.org/~zednenem/2002/wail/Place"/>
</rdfs:Class>

<rdfs:Class rdf:about="http://www.eyrie.org/~zednenem/2002/wail/Address">
    <rdfs:isDefinedBy rdf:resource="http://www.eyrie.org/~zednenem/2002/wail/wail.rdf"/>
    <rdfs:label>Address</rdfs:label>
    <rdfs:comment>
        A specific home, office, apartment, place of business, etc.
    </rdfs:comment>
    <rdfs:subClassOf rdf:resource="http://www.eyrie.org/~zednenem/2002/wail/Place"/>
</rdfs:Class>

<rdf:Property rdf:about="http://www.eyrie.org/~zednenem/2002/wail/homeAddress">
    <rdfs:isDefinedBy rdf:resource="http://www.eyrie.org/~zednenem/2002/wail/wail.rdf"/>
    <rdfs:label>homeAddress</rdfs:label>
    <rdfs:comment>
        A place where the subject lives
    </rdfs:comment>
    <rdfs:range rdf:resource="http://www.eyrie.org/~zednenem/2002/wail/Place"/>
</rdf:Property>

<rdf:Property rdf:about="http://www.eyrie.org/~zednenem/2002/wail/workAddress">
    <rdfs:isDefinedBy rdf:resource="http://www.eyrie.org/~zednenem/2002/wail/wail.rdf"/>
    <rdfs:label>workAddress</rdfs:label>
    <rdfs:comment>
        A place where the subject works
    </rdfs:comment>
    <rdfs:range rdf:resource="http://www.eyrie.org/~zednenem/2002/wail/Place"/>
</rdf:Property>

<rdf:Property rdf:about="http://www.eyrie.org/~zednenem/2002/wail/location">
    <rdfs:isDefinedBy rdf:resource="http://www.eyrie.org/~zednenem/2002/wail/wail.rdf"/>
    <rdfs:label>location</rdfs:label>
    <rdfs:comment>
        A place where something is located
    </rdfs:comment>
    <rdfs:range rdf:resource="http://www.eyrie.org/~zednenem/2002/wail/Place"/>
</rdf:Property>

<rdf:Property rdf:about="http://www.eyrie.org/~zednenem/2002/wail/locatedIn">
    <rdfs:isDefinedBy rdf:resource="http://www.eyrie.org/~zednenem/2002/wail/wail.rdf"/>
    <rdfs:label>locatedIn</rdfs:label>
    <rdfs:comment>
        Indicates that the subject Place is located within another Place
    </rdfs:comment>
    <rdfs:domain rdf:resource="http://www.eyrie.org/~zednenem/2002/wail/Place"/>
    <rdfs:range rdf:resource="http://www.eyrie.org/~zednenem/2002/wail/Place"/>
</rdf:Property>

<rdf:Property rdf:about="http://www.eyrie.org/~zednenem/2002/wail/name">
    <rdfs:isDefinedBy rdf:resource="http://www.eyrie.org/~zednenem/2002/wail/wail.rdf"/>
    <rdfs:label>name</rdfs:label>
    <rdfs:comment>
        A name by which this Place is known
    </rdfs:comment>
    <rdfs:domain rdf:resource="http://www.eyrie.org/~zednenem/2002/wail/Place"/>
    <rdfs:range rdf:resource="http://www.w3.org/2000/01/rdf-schema#Literal"/>
    <rdfs:subPropertyOf rdf:resource="http://purl.org/dc/elements/1.1/title"/>
</rdf:Property>

<rdf:Property rdf:about="http://www.eyrie.org/~zednenem/2002/wail/code">
    <rdfs:isDefinedBy rdf:resource="http://www.eyrie.org/~zednenem/2002/wail/wail.rdf"/>
    <rdfs:label>code</rdfs:label>
    <rdfs:comment>
        A well-known code by which this place is known; when applied to a Country,
        the value must be an ISO 3166-1 country code; when applied to a Region,
        the value must be an ISO 3166-2 region code
    </rdfs:comment>
    <rdfs:domain rdf:resource="http://www.eyrie.org/~zednenem/2002/wail/Place"/>
    <rdfs:range rdf:resource="http://www.w3.org/2000/01/rdf-schema#Literal"/>
    <rdfs:subPropertyOf rdf:resource="http://purl.org/dc/elements/1.1/identifier"/>
</rdf:Property>

<rdf:Property rdf:about="http://www.eyrie.org/~zednenem/2002/wail/streetName">
    <rdfs:isDefinedBy rdf:resource="http://www.eyrie.org/~zednenem/2002/wail/wail.rdf"/>
    <rdfs:label>streetName</rdfs:label>
    <rdfs:comment>
        The street name portion of a street address
    </rdfs:comment>
    <rdfs:domain rdf:resource="http://www.eyrie.org/~zednenem/2002/wail/Address"/>
    <rdfs:range rdf:resource="http://www.w3.org/2000/01/rdf-schema#Literal"/>
</rdf:Property>

<rdf:Property rdf:about="http://www.eyrie.org/~zednenem/2002/wail/streetNumber">
    <rdfs:isDefinedBy rdf:resource="http://www.eyrie.org/~zednenem/2002/wail/wail.rdf"/>
    <rdfs:label>streetNumber</rdfs:label>
    <rdfs:comment>
        The number portion of a street address (not limited to digits)
    </rdfs:comment>
    <rdfs:domain rdf:resource="http://www.eyrie.org/~zednenem/2002/wail/Address"/>
    <rdfs:range rdf:resource="http://www.w3.org/2000/01/rdf-schema#Literal"/>
</rdf:Property>

<rdf:Property rdf:about="http://www.eyrie.org/~zednenem/2002/wail/officeNumber">
    <rdfs:isDefinedBy rdf:resource="http://www.eyrie.org/~zednenem/2002/wail/wail.rdf"/>
    <rdfs:label>officeNumber</rdfs:label>
    <rdfs:comment>
        A code distinguishing offices at the same street address
    </rdfs:comment>
    <rdfs:domain rdf:resource="http://www.eyrie.org/~zednenem/2002/wail/Address"/>
    <rdfs:range rdf:resource="http://www.w3.org/2000/01/rdf-schema#Literal"/>
</rdf:Property>

<rdf:Property rdf:about="http://www.eyrie.org/~zednenem/2002/wail/apartmentNumber">
    <rdfs:isDefinedBy rdf:resource="http://www.eyrie.org/~zednenem/2002/wail/wail.rdf"/>
    <rdfs:label>apartmentNumber</rdfs:label>
    <rdfs:comment>
        A code distinguishing apartments with the same street address
    </rdfs:comment>
    <rdfs:domain rdf:resource="http://www.eyrie.org/~zednenem/2002/wail/Address"/>
    <rdfs:range rdf:resource="http://www.w3.org/2000/01/rdf-schema#Literal"/>
</rdf:Property>

<rdf:Property rdf:about="http://www.eyrie.org/~zednenem/2002/wail/postalCode">
    <rdfs:isDefinedBy rdf:resource="http://www.eyrie.org/~zednenem/2002/wail/wail.rdf"/>
    <rdfs:label>postalCode</rdfs:label>
    <rdfs:comment>
        A code used by postal services as part of a standard address;
        In the US, this would be a ZIP or ZIP+4 code
    </rdfs:comment>
    <rdfs:domain rdf:resource="http://www.eyrie.org/~zednenem/2002/wail/Address"/>
    <rdfs:range rdf:resource="http://www.w3.org/2000/01/rdf-schema#Literal"/>
</rdf:Property>

</rdf:RDF>
