<?xml version="1.0" encoding="utf-8"?>
<rdf:RDF
  xmlns:dcterms="http://purl.org/dc/terms/"
  xmlns:foaf="http://xmlns.com/foaf/0.1/"
  xmlns:owl="http://www.w3.org/2002/07/owl#"
  xmlns:prv="http://purl.org/net/provenance/ns#"
  xmlns:rdf="http://www.w3.org/1999/02/22-rdf-syntax-ns#"
  xmlns:rdfs="http://www.w3.org/2000/01/rdf-schema#"
  xmlns:wot="http://xmlns.com/wot/0.1/"
  xmlns:xhv="http://www.w3.org/1999/xhtml/vocab#"
  xmlns:xml="http://www.w3.org/XML/1998/namespace"
  xmlns:xsd="http://www.w3.org/2001/XMLSchema#"
>
  <owl:DatatypeProperty rdf:about="http://purl.org/dc/terms/description"/>
  <owl:DeprecatedProperty rdf:about="http://purl.org/net/provenance/ns#encodedBy">
    <rdfs:range>
      <owl:Class rdf:about="http://purl.org/net/provenance/ns#File">
        <rdfs:subClassOf>
          <owl:Class rdf:about="http://purl.org/net/provenance/ns#Artifact">
            <rdfs:subClassOf>
              <owl:Restriction>
                <owl:onProperty>
                  <owl:ObjectProperty rdf:about="http://purl.org/net/provenance/ns#retrievedBy">
                    <rdfs:range rdf:resource="http://purl.org/net/provenance/ns#DataAccess"/>
                    <rdfs:label xml:lang="en">retrieved by</rdfs:label>
                    <rdfs:domain rdf:resource="http://purl.org/net/provenance/ns#Artifact"/>
                    <rdfs:isDefinedBy rdf:resource="http://purl.org/net/provenance/ns#"/>
                    <rdfs:comment xml:lang="en">This property refers to the data access by which a Web representation of data has been retrieved from the Web.</rdfs:comment>
                    <rdfs:subPropertyOf rdf:resource="http://purl.org/net/provenance/ns#yieldedBy"/>
                  </owl:ObjectProperty>
                </owl:onProperty>
                <owl:maxCardinality rdf:datatype="http://www.w3.org/2001/XMLSchema#nonNegativeInteger">1</owl:maxCardinality>
              </owl:Restriction>
            </rdfs:subClassOf>
            <rdfs:label xml:lang="en">Artifact</rdfs:label>
            <rdfs:isDefinedBy>
              <owl:Ontology rdf:about="http://purl.org/net/provenance/ns#">
                <dcterms:description xml:lang="en">The Provenance Vocabulary provides classes and properties to describe the provenance of data from the Web. Hence, this vocabulary enables providers of Web data to publish provenance-related metadata about their data. The Provenance Vocabulary Core Ontology provides the main classes and properties required to describe provenance of data on the Web. Notice, this vocabulary is not designed to describe provenance of other kinds of content such as documents.</dcterms:description>
                <dcterms:title xml:lang="en">Provenance Vocabulary Core Ontology namespace</dcterms:title>
                <dcterms:creator>
                  <foaf:Person rdf:about="http://users.ox.ac.uk/~zool0770/foaf.rdf#me">
                    <foaf:homepage rdf:resource="http://users.ox.ac.uk/~zool0770/"/>
                    <foaf:name xml:lang="en">Jun Zhao</foaf:name>
                  </foaf:Person>
                </dcterms:creator>
                <dcterms:creator>
                  <foaf:Person rdf:about="http://olafhartig.de/foaf.rdf#olaf">
                    <foaf:homepage rdf:resource="http://olafhartig.de/"/>
                    <foaf:name xml:lang="en">Olaf Hartig</foaf:name>
                  </foaf:Person>
                </dcterms:creator>
                <dcterms:created rdf:datatype="http://www.w3.org/2001/XMLSchema#dateTime">20101-01-25T12:00:00Z</dcterms:created>
              </owl:Ontology>
            </rdfs:isDefinedBy>
            <rdfs:comment xml:lang="en">Artifact is a general class that represents artifacts which can be used during the execution (see the class Execution) of an action or a process and which can also be the result of such an execution.</rdfs:comment>
            <owl:disjointWith>
              <owl:Class rdf:about="http://purl.org/net/provenance/ns#Actor">
                <owl:equivalentClass>
                  <owl:Class rdf:about="http://xmlns.com/foaf/0.1/Agent"/>
                </owl:equivalentClass>
                <rdfs:isDefinedBy rdf:resource="http://purl.org/net/provenance/ns#"/>
                <rdfs:label xml:lang="en">Actor</rdfs:label>
                <rdfs:comment xml:lang="en">Actor is a general class that represents active entities. Actors usually perform the execution (see the class Execution) of an action or a process.</rdfs:comment>
              </owl:Class>
            </owl:disjointWith>
            <owl:disjointWith>
              <owl:Class rdf:about="http://purl.org/net/provenance/ns#Execution">
                <rdfs:subClassOf>
                  <owl:Restriction>
                    <owl:onProperty rdf:resource="http://purl.org/net/provenance/ns#performedAt"/>
                    <owl:maxCardinality rdf:datatype="http://www.w3.org/2001/XMLSchema#nonNegativeInteger">1</owl:maxCardinality>
                  </owl:Restriction>
                </rdfs:subClassOf>
                <rdfs:label xml:lang="en">Execution</rdfs:label>
                <rdfs:isDefinedBy rdf:resource="http://purl.org/net/provenance/ns#"/>
                <rdfs:comment xml:lang="en">Execution is a general class that represents completed executions of actions or processes. An execution is usually performed by an actor (see the class Actor) and an execution, in most cases, yielded an artifact (see the class Artifact).</rdfs:comment>
                <owl:disjointWith rdf:resource="http://purl.org/net/provenance/ns#Artifact"/>
                <owl:disjointWith rdf:resource="http://purl.org/net/provenance/ns#Actor"/>
              </owl:Class>
            </owl:disjointWith>
          </owl:Class>
        </rdfs:subClassOf>
        <rdfs:label xml:lang="en">File</rdfs:label>
        <rdfs:isDefinedBy rdf:resource="http://purl.org/net/provenance/ns#"/>
        <rdfs:comment xml:lang="en">File is a general class that represents computer files/documents of any kind.</rdfs:comment>
        <owl:disjointWith>
          <owl:Class rdf:about="http://purl.org/net/provenance/ns#DataItem">
            <rdfs:subClassOf rdf:resource="http://purl.org/net/provenance/ns#Artifact"/>
            <rdfs:subClassOf>
              <owl:Class rdf:about="http://www.ontologydesignpatterns.org/cp/owl/informationrealization.owl#InformationRealization"/>
            </rdfs:subClassOf>
            <rdfs:label xml:lang="en">Data Item</rdfs:label>
            <rdfs:isDefinedBy rdf:resource="http://purl.org/net/provenance/ns#"/>
            <rdfs:comment xml:lang="en">DataItem is a general class that represents any kind of representation of a data item.</rdfs:comment>
            <owl:disjointWith rdf:resource="http://purl.org/net/provenance/ns#File"/>
          </owl:Class>
        </owl:disjointWith>
      </owl:Class>
    </rdfs:range>
    <rdf:type rdf:resource="http://www.w3.org/2002/07/owl#ObjectProperty"/>
    <rdfs:label xml:lang="en">encoded by</rdfs:label>
    <rdfs:domain rdf:resource="http://purl.org/net/provenance/ns#DataItem"/>
    <rdfs:isDefinedBy rdf:resource="http://purl.org/net/provenance/ns#"/>
    <rdfs:comment xml:lang="en">This property is deprecated and will be removed from the Provenance Vocabulary shortly. Use prv:serializedBy instead. prv:encodedBy was deprecated because the new name prv:serializedBy is more suitable.</rdfs:comment>
  </owl:DeprecatedProperty>
  <owl:ObjectProperty rdf:about="http://purl.org/net/provenance/ns#operatedBy">
    <rdfs:range>
      <owl:Class rdf:about="http://purl.org/net/provenance/ns#HumanActor">
        <rdfs:subClassOf rdf:resource="http://purl.org/net/provenance/ns#Actor"/>
        <rdfs:label xml:lang="en">Human Actor</rdfs:label>
        <rdfs:isDefinedBy rdf:resource="http://purl.org/net/provenance/ns#"/>
        <rdfs:comment xml:lang="en">HumanActor is a general class that represents actors who are social beings such as persons, organizations, companies.</rdfs:comment>
        <owl:disjointWith rdf:resource="http://purl.org/net/provenance/ns#Artifact"/>
        <owl:disjointWith>
          <owl:Class rdf:about="http://purl.org/net/provenance/ns#NonHumanActor">
            <rdfs:subClassOf rdf:resource="http://purl.org/net/provenance/ns#Actor"/>
            <rdfs:label xml:lang="en">Non-Human Actor</rdfs:label>
            <rdfs:isDefinedBy rdf:resource="http://purl.org/net/provenance/ns#"/>
            <rdfs:comment xml:lang="en">NonHumanActor is a general class that represents actors who are not social beings.</rdfs:comment>
            <owl:disjointWith rdf:resource="http://purl.org/net/provenance/ns#HumanActor"/>
          </owl:Class>
        </owl:disjointWith>
        <owl:disjointWith rdf:resource="http://purl.org/net/provenance/ns#Execution"/>
      </owl:Class>
    </rdfs:range>
    <rdfs:label xml:lang="en">operated by</rdfs:label>
    <rdfs:domain rdf:resource="http://purl.org/net/provenance/ns#NonHumanActor"/>
    <rdfs:isDefinedBy rdf:resource="http://purl.org/net/provenance/ns#"/>
    <rdfs:comment xml:lang="en">This property refers to a human actor who was operating a non-human actor at the time the provenance description refers to. For instance, a service provider operated a data providing service (see class prv:DataProvidingService). Another example is a human actor who operated a non-human data creating actor.</rdfs:comment>
  </owl:ObjectProperty>
  <owl:DatatypeProperty rdf:about="http://xmlns.com/foaf/0.1/name"/>
  <owl:ObjectProperty rdf:about="http://xmlns.com/wot/0.1/endorser"/>
  <owl:ObjectProperty rdf:about="http://purl.org/net/provenance/ns#deployedSoftware">
    <rdfs:domain rdf:resource="http://purl.org/net/provenance/ns#NonHumanActor"/>
    <rdfs:isDefinedBy rdf:resource="http://purl.org/net/provenance/ns#"/>
    <rdfs:label xml:lang="en">runs</rdfs:label>
    <rdfs:comment xml:lang="en">This property refers to the software that was run by a non-human actor (usually a service).</rdfs:comment>
  </owl:ObjectProperty>
  <owl:ObjectProperty rdf:about="http://purl.org/net/provenance/ns#containedBy">
    <rdfs:range rdf:resource="http://purl.org/net/provenance/ns#DataItem"/>
    <rdfs:label xml:lang="en">contained in</rdfs:label>
    <rdfs:domain rdf:resource="http://purl.org/net/provenance/ns#DataItem"/>
    <rdfs:isDefinedBy rdf:resource="http://purl.org/net/provenance/ns#"/>
    <rdfs:comment xml:lang="en">This property refers to a data item that contained a data item. Hence, this property refers to another data item of a larger granularity (e.g. an RDF statement is usually contained in an RDF graph).</rdfs:comment>
  </owl:ObjectProperty>
  <owl:ObjectProperty rdf:about="http://www.w3.org/1999/xhtml/vocab#alternate"/>
  <foaf:Document rdf:about="http://purl.org/net/provenance/ns.rdf"/>
  <owl:Class rdf:about="http://xmlns.com/foaf/0.1/Organization">
    <rdfs:subClassOf rdf:resource="http://purl.org/net/provenance/ns#HumanActor"/>
  </owl:Class>
  <owl:ObjectProperty rdf:about="http://xmlns.com/wot/0.1/assurance"/>
  <owl:ObjectProperty rdf:about="http://purl.org/dc/terms/conformsTo"/>
  <owl:ObjectProperty rdf:about="http://purl.org/net/provenance/ns#usedBy">
    <rdfs:range>
      <owl:Class rdf:about="http://purl.org/net/provenance/ns#DataPublisher">
        <rdfs:subClassOf rdf:resource="http://purl.org/net/provenance/ns#HumanActor"/>
        <rdfs:isDefinedBy rdf:resource="http://purl.org/net/provenance/ns#"/>
        <rdfs:label xml:lang="en">Data Publisher</rdfs:label>
        <rdfs:comment xml:lang="en">DataPublisher is a class that represents entities such as persons, groups, or organizations who use a data providing service (see class prv:DataProvidingService) to publish data on the Web.</rdfs:comment>
      </owl:Class>
    </rdfs:range>
    <rdfs:label xml:lang="en">used by</rdfs:label>
    <rdfs:domain>
      <owl:Class rdf:about="http://purl.org/net/provenance/ns#DataProvidingService">
        <rdfs:subClassOf rdf:resource="http://purl.org/net/provenance/ns#NonHumanActor"/>
        <rdfs:isDefinedBy rdf:resource="http://purl.org/net/provenance/ns#"/>
        <rdfs:label xml:lang="en">Data Providing Service</rdfs:label>
        <rdfs:comment xml:lang="en">DataProvidingService is a class that represents a non-human actor - usually a Web service or a server (software) - that processes data access requests and actually sends the requested Web representations over the Web.</rdfs:comment>
      </owl:Class>
    </rdfs:domain>
    <rdfs:isDefinedBy rdf:resource="http://purl.org/net/provenance/ns#"/>
    <rdfs:comment xml:lang="en">This property refers to a data publisher who used a data providing services at the time the provenance description refers to.</rdfs:comment>
  </owl:ObjectProperty>
  <owl:Class rdf:about="http://purl.org/net/provenance/ns#Representation">
    <rdfs:subClassOf rdf:resource="http://purl.org/net/provenance/ns#Artifact"/>
    <rdfs:subClassOf>
      <owl:Class rdf:about="http://sw.nokia.com/WebArch-1/Representation"/>
    </rdfs:subClassOf>
    <rdfs:subClassOf>
      <owl:Class rdf:about="http://www.ontologydesignpatterns.org/ont/web/irw.owl#WebRepresentation"/>
    </rdfs:subClassOf>
    <rdf:type rdf:resource="http://www.w3.org/2002/07/owl#DeprecatedClass"/>
    <rdfs:label xml:lang="en">Web Representation</rdfs:label>
    <rdfs:isDefinedBy rdf:resource="http://purl.org/net/provenance/ns#"/>
    <rdfs:comment xml:lang="en">This class is deprecated and will be removed from the Provenance Vocabulary in the next revision. Use prv:DataItem instead. prv:Representation was deprecated because the Provenance Vocabulary does not distinguish Web representations of data and the general kind of representations (as prv:DataItem represents).</rdfs:comment>
    <owl:disjointWith rdf:resource="http://purl.org/net/provenance/ns#File"/>
  </owl:Class>
  <owl:Class rdf:about="http://sw.nokia.com/WebArch-1/Server">
    <rdfs:subClassOf rdf:resource="http://purl.org/net/provenance/ns#DataProvidingService"/>
  </owl:Class>
  <owl:ObjectProperty rdf:about="http://xmlns.com/foaf/0.1/primaryTopic"/>
  <owl:Class rdf:about="http://sw.nokia.com/WebArch-1/Service">
    <rdfs:subClassOf rdf:resource="http://purl.org/net/provenance/ns#DataProvidingService"/>
  </owl:Class>
  <owl:DatatypeProperty rdf:about="http://purl.org/dc/terms/created"/>
  <owl:Class rdf:about="http://www.ontologydesignpatterns.org/ont/web/irw.owl#WebServer">
    <rdfs:subClassOf rdf:resource="http://purl.org/net/provenance/ns#DataProvidingService"/>
  </owl:Class>
  <owl:ObjectProperty rdf:about="http://purl.org/net/provenance/ns#performedBy">
    <rdfs:range rdf:resource="http://purl.org/net/provenance/ns#Actor"/>
    <rdfs:label xml:lang="en">performed by</rdfs:label>
    <rdfs:domain rdf:resource="http://purl.org/net/provenance/ns#Execution"/>
    <rdfs:isDefinedBy rdf:resource="http://purl.org/net/provenance/ns#"/>
    <rdfs:comment xml:lang="en">This property refers to an actor that/who performed an execution.</rdfs:comment>
    <rdfs:subPropertyOf>
      <owl:ObjectProperty rdf:about="http://purl.org/net/provenance/ns#involvedActor">
        <rdfs:range rdf:resource="http://purl.org/net/provenance/ns#Actor"/>
        <rdfs:label xml:lang="en">involved</rdfs:label>
        <rdfs:domain rdf:resource="http://purl.org/net/provenance/ns#Execution"/>
        <rdfs:isDefinedBy rdf:resource="http://purl.org/net/provenance/ns#"/>
        <rdfs:comment xml:lang="en">This is an abstract property that refers to an actor involved in an execution.</rdfs:comment>
      </owl:ObjectProperty>
    </rdfs:subPropertyOf>
  </owl:ObjectProperty>
  <owl:ObjectProperty rdf:about="http://purl.org/dc/terms/creator"/>
  <foaf:Document rdf:about="http://trdf.sourceforge.net/provenance/ns.html">
    <dcterms:description xml:lang="en">This documents specifies the classes and properties introduced by the Provenance Vocabulary Core Ontology.</dcterms:description>
    <foaf:primaryTopic rdf:resource="http://purl.org/net/provenance/ns#"/>
    <rdfs:label xml:lang="en">Document that defines the core ontology of the Provenance Vocabulary</rdfs:label>
    <dcterms:title xml:lang="en">Provenance Vocabulary Core Ontology Specification</dcterms:title>
    <xhv:license>
      <owl:Thing rdf:about="http://creativecommons.org/licenses/by/1.0/"/>
    </xhv:license>
    <xhv:alternate rdf:resource="http://trdf.sourceforge.net/provenance/ns.rdf"/>
    <wot:assurance>
      <wot:Endorsement rdf:about="http://trdf.sourceforge.net/provenance/ns.html.sig">
        <dcterms:title xml:lang="en">Detached signature</dcterms:title>
        <wot:endorser>
          <wot:PubKey rdf:about="http://olafhartig.de/foaf.rdf#pubkey2009"/>
        </wot:endorser>
      </wot:Endorsement>
    </wot:assurance>
    <dcterms:conformsTo>
      <owl:Thing rdf:about="http://www.w3.org/TR/rdfa-syntax"/>
    </dcterms:conformsTo>
  </foaf:Document>
  <owl:DatatypeProperty rdf:about="http://purl.org/dc/terms/title"/>
  <owl:Class rdf:about="http://xmlns.com/foaf/0.1/Group">
    <rdfs:subClassOf rdf:resource="http://purl.org/net/provenance/ns#HumanActor"/>
  </owl:Class>
  <owl:ObjectProperty rdf:about="http://xmlns.com/foaf/0.1/homepage"/>
  <owl:ObjectProperty rdf:about="http://www.w3.org/1999/xhtml/vocab#license"/>
  <owl:ObjectProperty rdf:about="http://purl.org/net/provenance/ns#precededBy">
    <rdfs:range rdf:resource="http://purl.org/net/provenance/ns#DataItem"/>
    <rdfs:label xml:lang="en">immediately preceded by</rdfs:label>
    <rdfs:domain rdf:resource="http://purl.org/net/provenance/ns#DataItem"/>
    <rdfs:isDefinedBy rdf:resource="http://purl.org/net/provenance/ns#"/>
    <rdfs:comment xml:lang="en">This property refers to an immediately preceding version of a data item; hence, the new version (i.e. the subject) has been created using the old version (i.e. the object). We strongly encourage to also describe this creation of the new version explicitly.</rdfs:comment>
    <rdfs:subPropertyOf>
      <owl:ObjectProperty rdf:about="http://purl.org/dc/terms/replaces"/>
    </rdfs:subPropertyOf>
  </owl:ObjectProperty>
  <owl:ObjectProperty rdf:about="http://purl.org/net/provenance/ns#usedGuideline">
    <rdfs:range>
      <owl:Class rdf:about="http://purl.org/net/provenance/ns#CreationGuideline">
        <rdfs:subClassOf rdf:resource="http://purl.org/net/provenance/ns#DataItem"/>
        <rdfs:isDefinedBy rdf:resource="http://purl.org/net/provenance/ns#"/>
        <rdfs:label xml:lang="en">Creation Guideline</rdfs:label>
        <rdfs:comment xml:lang="en">CreationGuideline is a class that represents a guideline used to guide the execution of a data creation. Examples for creation guidelines are transformation rules, mapping definitions, entailment rules, and database queries.</rdfs:comment>
      </owl:Class>
    </rdfs:range>
    <rdfs:label xml:lang="en">guided by</rdfs:label>
    <rdfs:domain>
      <owl:Class rdf:about="http://purl.org/net/provenance/ns#DataCreation">
        <rdfs:subClassOf rdf:resource="http://purl.org/net/provenance/ns#Execution"/>
        <rdfs:label xml:lang="en">Data Creation</rdfs:label>
        <rdfs:isDefinedBy rdf:resource="http://purl.org/net/provenance/ns#"/>
        <rdfs:comment xml:lang="en">DataCreation is a class that represents the completed creation of a data item.</rdfs:comment>
        <owl:disjointWith>
          <owl:Class rdf:about="http://purl.org/net/provenance/ns#DataAccess">
            <rdfs:subClassOf>
              <owl:Restriction>
                <owl:onProperty>
                  <owl:ObjectProperty rdf:about="http://purl.org/net/provenance/ns#accessedResource">
                    <rdfs:range rdf:resource="http://www.ontologydesignpatterns.org/ont/web/irw.owl#WebResource"/>
                    <rdfs:label xml:lang="en">accessed</rdfs:label>
                    <rdfs:domain rdf:resource="http://purl.org/net/provenance/ns#DataAccess"/>
                    <rdfs:isDefinedBy rdf:resource="http://purl.org/net/provenance/ns#"/>
                    <rdfs:comment xml:lang="en">This property refers to the Web resource that has been accessed during the execution of a data access. More precisely, the request of the referenced Web resource resulted in retrieving the representation that has been retrieved by the corresponding prv:DataAccess execution.</rdfs:comment>
                    <rdfs:subPropertyOf rdf:resource="http://purl.org/net/provenance/ns#employedArtifact"/>
                  </owl:ObjectProperty>
                </owl:onProperty>
                <owl:maxCardinality rdf:datatype="http://www.w3.org/2001/XMLSchema#nonNegativeInteger">1</owl:maxCardinality>
              </owl:Restriction>
            </rdfs:subClassOf>
            <rdfs:subClassOf>
              <owl:Restriction>
                <owl:onProperty>
                  <owl:ObjectProperty rdf:about="http://purl.org/net/provenance/ns#accessedService">
                    <rdfs:range rdf:resource="http://purl.org/net/provenance/ns#DataProvidingService"/>
                    <rdfs:label xml:lang="en">accessed</rdfs:label>
                    <rdfs:domain rdf:resource="http://purl.org/net/provenance/ns#DataAccess"/>
                    <rdfs:isDefinedBy rdf:resource="http://purl.org/net/provenance/ns#"/>
                    <rdfs:comment xml:lang="en">This property refers to the service that provided the Web representation during the execution of a data access.</rdfs:comment>
                    <rdfs:subPropertyOf rdf:resource="http://purl.org/net/provenance/ns#involvedActor"/>
                  </owl:ObjectProperty>
                </owl:onProperty>
                <owl:maxCardinality rdf:datatype="http://www.w3.org/2001/XMLSchema#nonNegativeInteger">1</owl:maxCardinality>
              </owl:Restriction>
            </rdfs:subClassOf>
            <rdfs:subClassOf rdf:resource="http://purl.org/net/provenance/ns#Execution"/>
            <rdfs:label xml:lang="en">Data Access</rdfs:label>
            <rdfs:isDefinedBy rdf:resource="http://purl.org/net/provenance/ns#"/>
            <rdfs:comment xml:lang="en">DataAccess is a class that represents the completed execution of accessing a data item on the Web.</rdfs:comment>
            <owl:disjointWith rdf:resource="http://purl.org/net/provenance/ns#DataCreation"/>
          </owl:Class>
        </owl:disjointWith>
      </owl:Class>
    </rdfs:domain>
    <rdfs:isDefinedBy rdf:resource="http://purl.org/net/provenance/ns#"/>
    <rdfs:comment xml:lang="en">This property refers to a creation guideline which guided the execution of a data creation. Examples for creation guidelines are transformation rules, mapping definitions, entailment rules, and database queries. Notice, all creation guidelines have provenance; we strongly encourage to describe this provenance as well, at least as far as available information permits.</rdfs:comment>
    <rdfs:subPropertyOf>
      <owl:ObjectProperty rdf:about="http://purl.org/net/provenance/ns#usedData">
        <rdfs:range rdf:resource="http://purl.org/net/provenance/ns#DataItem"/>
        <rdfs:label xml:lang="en">used</rdfs:label>
        <rdfs:domain rdf:resource="http://purl.org/net/provenance/ns#DataCreation"/>
        <rdfs:isDefinedBy rdf:resource="http://purl.org/net/provenance/ns#"/>
        <rdfs:comment xml:lang="en">This property refers to a source data item that has been used during the creation of a data item. Examples for source data are the content of a document used for machine learning, the statements in a knowledge base used to entail a new statement, and the entries in a database used to answer a query. Notice, all source data has provenance; we strongly encourage to describe this provenance as well, at least as far as available information permits.</rdfs:comment>
        <rdfs:subPropertyOf>
          <owl:ObjectProperty rdf:about="http://purl.org/net/provenance/ns#employedArtifact">
            <rdfs:range rdf:resource="http://purl.org/net/provenance/ns#Artifact"/>
            <rdfs:label xml:lang="en">used</rdfs:label>
            <rdfs:domain rdf:resource="http://purl.org/net/provenance/ns#Execution"/>
            <rdfs:isDefinedBy rdf:resource="http://purl.org/net/provenance/ns#"/>
            <rdfs:comment xml:lang="en">This is an abstract property that refers to an artifact which was used during an execution.</rdfs:comment>
          </owl:ObjectProperty>
        </rdfs:subPropertyOf>
        <rdfs:seeAlso rdf:resource="http://purl.org/net/provenance/files#"/>
      </owl:ObjectProperty>
    </rdfs:subPropertyOf>
    <rdfs:seeAlso rdf:resource="http://purl.org/net/provenance/files#"/>
  </owl:ObjectProperty>
  <owl:Class rdf:about="http://xmlns.com/wot/0.1/Endorsement"/>
  <owl:Class rdf:nodeID="ORkakCRv11">
    <owl:unionOf rdf:parseType="Collection">
      <rdf:Description rdf:about="http://purl.org/net/provenance/ns#DataItem"/>
      <rdf:Description rdf:about="http://purl.org/net/provenance/ns#File"/>
    </owl:unionOf>
  </owl:Class>
  <owl:Class rdf:about="http://xmlns.com/wot/0.1/PubKey"/>
  <owl:Class rdf:about="http://www.ontologydesignpatterns.org/ont/web/irw.owl#WebResource"/>
  <foaf:Document rdf:about="http://users.ox.ac.uk/~zool0770/"/>
  <rdfs:List rdf:nodeID="ORkakCRv17">
    <rdf:rest/>
    <rdf:first>
      <owl:ObjectProperty rdf:about="http://purl.org/net/provenance/ns#serializedBy">
        <rdfs:range rdf:resource="http://purl.org/net/provenance/ns#File"/>
        <rdfs:isDefinedBy rdf:resource="http://purl.org/net/provenance/ns#"/>
        <rdfs:label xml:lang="en">serialized by</rdfs:label>
        <rdfs:comment xml:lang="en">This property refers to a file that serialized a data item.</rdfs:comment>
      </owl:ObjectProperty>
    </rdf:first>
  </rdfs:List>
  <owl:DatatypeProperty rdf:about="http://purl.org/net/provenance/ns#performedAt">
    <rdfs:range rdf:resource="http://www.w3.org/2001/XMLSchema#dateTime"/>
    <rdfs:label xml:lang="en">executed at</rdfs:label>
    <rdfs:domain rdf:resource="http://purl.org/net/provenance/ns#Execution"/>
    <rdfs:isDefinedBy rdf:resource="http://purl.org/net/provenance/ns#"/>
    <rdfs:comment xml:lang="en">This property refers to the time an execution has been performed at.</rdfs:comment>
  </owl:DatatypeProperty>
  <owl:ObjectProperty rdf:about="http://purl.org/net/provenance/ns#createdBy">
    <rdfs:range rdf:resource="http://purl.org/net/provenance/ns#DataCreation"/>
    <rdfs:label xml:lang="en">created by</rdfs:label>
    <rdfs:domain rdf:nodeID="ORkakCRv11"/>
    <owl:propertyChainAxiom rdf:parseType="Collection">
      <rdf:Description rdf:about="http://purl.org/net/provenance/ns#serializedBy"/>
      <rdf:Description rdf:about="http://purl.org/net/provenance/ns#createdBy"/>
    </owl:propertyChainAxiom>
    <rdfs:isDefinedBy rdf:resource="http://purl.org/net/provenance/ns#"/>
    <rdfs:comment xml:lang="en">This property refers to the creation of a data item.</rdfs:comment>
    <rdfs:subPropertyOf>
      <owl:ObjectProperty rdf:about="http://purl.org/net/provenance/ns#yieldedBy">
        <rdfs:range rdf:resource="http://purl.org/net/provenance/ns#Execution"/>
        <rdfs:label xml:lang="en">yielded by</rdfs:label>
        <rdfs:domain rdf:resource="http://purl.org/net/provenance/ns#Artifact"/>
        <rdfs:isDefinedBy rdf:resource="http://purl.org/net/provenance/ns#"/>
        <rdfs:comment xml:lang="en">This is an abstract property that refers to the execution by which an artifact was yielded.</rdfs:comment>
      </owl:ObjectProperty>
    </rdfs:subPropertyOf>
  </owl:ObjectProperty>
  <foaf:Document rdf:about="http://olafhartig.de/"/>
  <owl:Class rdf:about="http://xmlns.com/foaf/0.1/Person">
    <rdfs:subClassOf rdf:resource="http://purl.org/net/provenance/ns#HumanActor"/>
  </owl:Class>
  <owl:Class rdf:about="http://xmlns.com/foaf/0.1/Document"/>
</rdf:RDF>
